Prefix: : <http://openenergy-platform.org/ontology/oeo/>
Prefix: bfo: <http://purl.obolibrary.org/obo/bfo.owl#>
Prefix: dc: <http://purl.org/dc/elements/1.1/>
Prefix: obda: <https://w3id.org/obda/vocabulary#>
Prefix: oeo: <http://openenergy-platform.org/ontology/v0.0.1/oeo/>
Prefix: owl: <http://www.w3.org/2002/07/owl#>
Prefix: rdf: <http://www.w3.org/1999/02/22-rdf-syntax-ns#>
Prefix: rdfs: <http://www.w3.org/2000/01/rdf-schema#>
Prefix: xml: <http://www.w3.org/XML/1998/namespace>
Prefix: xsd: <http://www.w3.org/2001/XMLSchema#>



Ontology: <http://openenergy-platform.org/ontology/oeo/>
<http://openenergy-platform.org/ontology/v0.0.1/oeo/>
Import: <https://raw.githubusercontent.com/BFO-ontology/BFO/v2.0/bfo.owl>

Annotations: 
    dc:contributor "Christian Winger",
    dc:contributor "Fabian Neuhaus",
    dc:contributor "Hannah Förster",
    dc:contributor "Lukas Emele",
    dc:contributor "Martin Glauer",
    dc:contributor "Sebastian Cordes",
    <http://purl.org/dc/terms/title> "Open Energy Ontology",
    rdfs:comment "Include description of the ontology (in particular its scope) here ..."

AnnotationProperty: <http://purl.obolibrary.org/obo/IAO_0000112>

    
AnnotationProperty: <http://purl.obolibrary.org/obo/IAO_0000115>

    
AnnotationProperty: <http://purl.obolibrary.org/obo/IAO_0000116>

    
AnnotationProperty: <http://purl.obolibrary.org/obo/IAO_0000119>

    
AnnotationProperty: <http://purl.org/dc/terms/title>

    
AnnotationProperty: dc:contributor

    
AnnotationProperty: definition

    SubPropertyOf: 
        rdfs:comment
    
    
AnnotationProperty: rdfs:comment

    
AnnotationProperty: rdfs:isDefinedBy

    
AnnotationProperty: rdfs:label

    
Datatype: rdf:PlainLiteral

    
ObjectProperty: appliesTo

    
ObjectProperty: comparesTo

    
ObjectProperty: conforms_to

    Domain: 
        conforms_to some SectorConcept
    
    Range: 
        Sector
    
    
ObjectProperty: contains

    
ObjectProperty: covers

    Annotations: 
        <http://purl.obolibrary.org/obo/IAO_0000115> "A relation that holds between a publication/model calculation/model and the thing it covers."@en
    
    
ObjectProperty: covers_region

    Annotations: 
        <http://purl.obolibrary.org/obo/IAO_0000115> "A relation that holds between a publication/model calculation/model and the region it covers."@en
    
    SubPropertyOf: 
        covers
    
    
ObjectProperty: covers_sector

    Annotations: 
        <http://purl.obolibrary.org/obo/IAO_0000115> "A relation that holds between a publication/model calculation/model and the sector it models."@en
    
    SubPropertyOf: 
        covers
    
    Range: 
        Sector
    
    
ObjectProperty: covers_technology

    Annotations: 
        <http://purl.obolibrary.org/obo/IAO_0000115> "A relation that holds between a publication/model calculation/model and the technology it models."@en
    
    SubPropertyOf: 
        covers
    
    
ObjectProperty: covers_timeframe

    Annotations: 
        <http://purl.obolibrary.org/obo/IAO_0000115> "A relation that holds between a publication/model calculation/model and the timeframe it covers."@en
    
    SubPropertyOf: 
        covers
    
    
ObjectProperty: depends_on

    
ObjectProperty: distributes

    SubPropertyOf: 
        owl:topObjectProperty
    
    
ObjectProperty: g_depends_on

    SubPropertyOf: 
        depends_on
    
    
ObjectProperty: generates_dataset

    SubPropertyOf: 
        has_output
    
    
ObjectProperty: handles_uncertainty

    SubPropertyOf: 
        owl:topObjectProperty
    
    
ObjectProperty: has

    SubPropertyOf: 
        owl:topObjectProperty
    
    
ObjectProperty: hasMaximum

    SubPropertyOf: 
        comparesTo
    
    
ObjectProperty: hasMinimum

    SubPropertyOf: 
        comparesTo
    
    
ObjectProperty: hasNumeral

    
ObjectProperty: hasUnitofMeasurement

    
ObjectProperty: hasYear

    
ObjectProperty: has_Percentage

    SubPropertyOf: 
        comparesTo
    
    
ObjectProperty: has_author

    Annotations: 
        <http://purl.obolibrary.org/obo/IAO_0000115> "A relation that holds between a publication/model and its author."@en
    
    SubPropertyOf: 
        has_participant
    
    Domain: 
        Publication
    
    Range: 
        Agent
    
    
ObjectProperty: has_client

    Annotations: 
        <http://purl.obolibrary.org/obo/IAO_0000115> "A relation that holds between a publication/model and the client that requested its creation."@en
    
    SubPropertyOf: 
        has_participant
    
    Domain: 
        Publication
    
    Range: 
        Agent
    
    
ObjectProperty: has_complexity

    SubPropertyOf: 
        owl:topObjectProperty
    
    
ObjectProperty: has_constraint

    Annotations: 
        <http://purl.obolibrary.org/obo/IAO_0000115> "A relation that holds between a transformation and the constraints it has to fulfill."@en
    
    SubPropertyOf: 
        has_input
    
    
ObjectProperty: has_contact

    Annotations: 
        <http://purl.obolibrary.org/obo/IAO_0000115> "A relation that holds between a publication/model and the person to contact with issues about it."@en
    
    SubPropertyOf: 
        has_participant
    
    
ObjectProperty: has_disposition

    
ObjectProperty: has_documentation

    SubPropertyOf: 
        has
    
    
ObjectProperty: has_function

    SubPropertyOf: 
        has_disposition
    
    
ObjectProperty: has_funding_source

    Annotations: 
        <http://purl.obolibrary.org/obo/IAO_0000115> "A relation that holds between a publication/model and its source of funding."@en
    
    SubPropertyOf: 
        has_participant
    
    Domain: 
        Publication
    
    Range: 
        Agent
    
    
ObjectProperty: has_globalwarmingpotential

    SubPropertyOf: 
        owl:topObjectProperty
    
    Domain: 
        GreenhouseGas
    
    Range: 
        GlobalWarmingPotential
    
    
ObjectProperty: has_input

    Annotations: 
        <http://purl.obolibrary.org/obo/IAO_0000115> "A relation that holds between a transformation and its input."@en
    
    SubPropertyOf: 
        has
    
    
ObjectProperty: has_institution

    Annotations: 
        <http://purl.obolibrary.org/obo/IAO_0000115> "A relation that holds between a publication and the institution in which it was created."@en
    
    SubPropertyOf: 
        has_participant
    
    
ObjectProperty: has_license

    SubPropertyOf: 
        has_participant
    
    
ObjectProperty: has_logo

    SubPropertyOf: 
        has
    
    
ObjectProperty: has_normal_state_of_matter

    Annotations: 
        <http://purl.obolibrary.org/obo/IAO_0000115> "x has_normal_state_of_matter y if and only if a portion of x occurs in state y under normal pressure and temperature"
    
    Range: 
        StateOfMatter
    
    
ObjectProperty: has_numercical_input

    Annotations: 
        <http://purl.obolibrary.org/obo/IAO_0000115> "A relation that holds between a transformation and its input."@en
    
    SubPropertyOf: 
        has_input
    
    Characteristics: 
        Irreflexive,
        Asymmetric
    
    Domain: 
        Transformation
    
    Range: 
        InformationArtifact
    
    
ObjectProperty: has_numerical_output

    Annotations: 
        <http://purl.obolibrary.org/obo/IAO_0000115> "A relation that holds between a transformation and its output."@en
    
    SubPropertyOf: 
        has_output
    
    Characteristics: 
        Irreflexive,
        Asymmetric
    
    Domain: 
        Transformation
    
    Range: 
        InformationArtifact
    
    
ObjectProperty: has_objective

    Annotations: 
        <http://purl.obolibrary.org/obo/IAO_0000115> "A relation that holds between an optimization and its objective function or objective variable."@en
    
    Domain: 
        Optimization
    
    Range: 
        SoftwareElement
    
    
ObjectProperty: has_objectivefunction

    Annotations: 
        <http://purl.obolibrary.org/obo/IAO_0000115> "A relation that holds between an optimization and its objective function."@en
    
    SubPropertyOf: 
        has_objective
    
    
ObjectProperty: has_objectivevariable

    Annotations: 
        <http://purl.obolibrary.org/obo/IAO_0000115> "A relation that holds between an optimization and its objective variable."@en
    
    SubPropertyOf: 
        has_objective
    
    
ObjectProperty: has_output

    Annotations: 
        <http://purl.obolibrary.org/obo/IAO_0000115> "A relation that holds between a transformation and its output."@en
    
    SubPropertyOf: 
        has_participant
    
    
ObjectProperty: has_part

    Annotations: 
        <http://purl.obolibrary.org/obo/IAO_0000115> "A relation that holds between a whole and its part."@en
    
    SubPropertyOf: 
        owl:topObjectProperty
    
    InverseOf: 
        part_of
    
    
ObjectProperty: has_participant

    
ObjectProperty: has_physical_input

    Annotations: 
        <http://purl.obolibrary.org/obo/IAO_0000115> "A relation that holds between a transformation and its input."@en
    
    SubPropertyOf: 
        has_input
    
    Characteristics: 
        Functional,
        Irreflexive,
        Asymmetric
    
    Domain: 
        EnergyGeneratorTechnology
    
    Range: 
        EnergyCarrier
    
    
ObjectProperty: has_physical_output

    Annotations: 
        <http://purl.obolibrary.org/obo/IAO_0000115> "A relation that holds between a transformation and its output."@en
    
    SubPropertyOf: 
        has_output
    
    Characteristics: 
        Irreflexive,
        Asymmetric
    
    Domain: 
        EnergyGeneratorTechnology
    
    Range: 
        Power
    
    
ObjectProperty: has_pollutant

    SubPropertyOf: 
        owl:topObjectProperty
    
    Domain: 
        Emission
    
    Range: 
        Pollutant
    
    
ObjectProperty: has_programvariable

    Annotations: 
        <http://purl.obolibrary.org/obo/IAO_0000115> "A relation that holds between a model and a program variable it uses."@en
    
    SubPropertyOf: 
        has_participant
    
    
ObjectProperty: has_quality

    
ObjectProperty: has_resolution

    Annotations: 
        <http://purl.obolibrary.org/obo/IAO_0000115> "A relation thst holds between a publication/model/model calculation and the resolution it uses."@en
    
    
ObjectProperty: has_role

    
ObjectProperty: has_sink

    SubPropertyOf: 
        is_connected_to
    
    DisjointWith: 
        has_source
    
    
ObjectProperty: has_source

    SubPropertyOf: 
        is_connected_to
    
    DisjointWith: 
        has_sink
    
    
ObjectProperty: has_spatial_resolution

    Annotations: 
        <http://purl.obolibrary.org/obo/IAO_0000115> "A relation thst holds between a publication/model/model calculation and the spacial resolution it uses."@en
    
    SubPropertyOf: 
        has_resolution
    
    
ObjectProperty: has_subregion

    Annotations: 
        <http://purl.obolibrary.org/obo/IAO_0000115> "A relation that holds between a region and a smaller region within."@en
    
    SubPropertyOf: 
        has_part
    
    
ObjectProperty: has_temporal_resolution

    Annotations: 
        <http://purl.obolibrary.org/obo/IAO_0000115> "A relation thst holds between a publication/model/model calculation and the time resolution it uses."@en
    
    SubPropertyOf: 
        has_resolution
    
    
ObjectProperty: has_tool

    Annotations: 
        <http://purl.obolibrary.org/obo/IAO_0000115> "A relation that  holds between a model calculation and the model it is using."@en
    
    SubPropertyOf: 
        has_participant
    
    Domain: 
        ModelCalculation
    
    Range: 
        Model
    
    
ObjectProperty: has_website

    SubPropertyOf: 
        is_referenced_by
    
    
ObjectProperty: isEqual

    SubPropertyOf: 
        comparesTo
    
    
ObjectProperty: is_connected_to

    SubPropertyOf: 
        owl:topObjectProperty
    
    Characteristics: 
        Symmetric
    
    
ObjectProperty: is_equivalent_to

    Annotations: 
        <http://purl.obolibrary.org/obo/IAO_0000115> "A relation that holds between an definition and its synonym."@en
    
    SubPropertyOf: 
        owl:topObjectProperty
    
    
ObjectProperty: is_referenced_by

    SubPropertyOf: 
        owl:topObjectProperty
    
    InverseOf: 
        references
    
    
ObjectProperty: is_used_by

    SubPropertyOf: 
        owl:topObjectProperty
    
    InverseOf: 
        uses
    
    
ObjectProperty: makes_assumption

    Annotations: 
        <http://purl.obolibrary.org/obo/IAO_0000115> "A relation that holds between a transformation and and an assumption made for its execution."@en
    
    SubPropertyOf: 
        owl:topObjectProperty
    
    
ObjectProperty: owl:topObjectProperty

    
ObjectProperty: part_of

    Annotations: 
        <http://purl.obolibrary.org/obo/IAO_0000115> "A relation that holds between a part and the whole it belongs to."@en
    
    Characteristics: 
        Transitive
    
    InverseOf: 
        has_part
    
    
ObjectProperty: references

    SubPropertyOf: 
        owl:topObjectProperty
    
    InverseOf: 
        is_referenced_by
    
    
ObjectProperty: s_depends_on

    SubPropertyOf: 
        depends_on
    
    
ObjectProperty: transmits

    SubPropertyOf: 
        owl:topObjectProperty
    
    
ObjectProperty: uses

    SubPropertyOf: 
        owl:topObjectProperty
    
    InverseOf: 
        is_used_by
    
    
ObjectProperty: uses_dataset

    Annotations: 
        <http://purl.obolibrary.org/obo/IAO_0000115> "A relation that holds between a transformation and a dataset it uses as input."@en
    
    SubPropertyOf: 
        uses
    
    
ObjectProperty: uses_external_optimizer

    SubPropertyOf: 
        uses
    
    
ObjectProperty: uses_software

    SubPropertyOf: 
        uses
    
    
Class: <http://purl.obolibrary.org/obo/BFO_0000002>

    
Class: <http://purl.obolibrary.org/obo/BFO_0000003>

    
Class: <http://purl.obolibrary.org/obo/BFO_0000006>

    
Class: <http://purl.obolibrary.org/obo/BFO_0000009>

    
Class: <http://purl.obolibrary.org/obo/BFO_0000015>

    
Class: <http://purl.obolibrary.org/obo/BFO_0000016>

    
Class: <http://purl.obolibrary.org/obo/BFO_0000019>

    
Class: <http://purl.obolibrary.org/obo/BFO_0000023>

    
Class: <http://purl.obolibrary.org/obo/BFO_0000024>

    
Class: <http://purl.obolibrary.org/obo/BFO_0000027>

    
Class: <http://purl.obolibrary.org/obo/BFO_0000028>

    
Class: <http://purl.obolibrary.org/obo/BFO_0000029>

    
Class: <http://purl.obolibrary.org/obo/BFO_0000030>

    
Class: <http://purl.obolibrary.org/obo/BFO_0000031>

    
Class: <http://purl.obolibrary.org/obo/BFO_0000141>

    
Class: <http://www.semanticweb.org/izzet_kilicarslan/ontologies/2019/9/untitled-ontology-10#AcDcCoupling>

    SubClassOf: 
        <http://www.semanticweb.org/izzet_kilicarslan/ontologies/2019/9/untitled-ontology-10#TechnicalDataStorage>
    
    
Class: <http://www.semanticweb.org/izzet_kilicarslan/ontologies/2019/9/untitled-ontology-10#AreaOfApplication>

    SubClassOf: 
        <http://www.semanticweb.org/izzet_kilicarslan/ontologies/2019/9/untitled-ontology-10#SolarEntityDataset>
    
    
Class: <http://www.semanticweb.org/izzet_kilicarslan/ontologies/2019/9/untitled-ontology-10#AssignedEffectivePowerInverter>

    SubClassOf: 
        <http://www.semanticweb.org/izzet_kilicarslan/ontologies/2019/9/untitled-ontology-10#TechnicalDataStorage>
    
    
Class: <http://www.semanticweb.org/izzet_kilicarslan/ontologies/2019/9/untitled-ontology-10#AssignedEffectivePowerInverterSolar>

    SubClassOf: 
        <http://www.semanticweb.org/izzet_kilicarslan/ontologies/2019/9/untitled-ontology-10#SolarEntityDataset>
    
    
Class: <http://www.semanticweb.org/izzet_kilicarslan/ontologies/2019/9/untitled-ontology-10#Batterytechnology>

    SubClassOf: 
        <http://www.semanticweb.org/izzet_kilicarslan/ontologies/2019/9/untitled-ontology-10#TechnicalDataStorage>
    
    
Class: <http://www.semanticweb.org/izzet_kilicarslan/ontologies/2019/9/untitled-ontology-10#BlackStartCapacity>

    SubClassOf: 
        PowerPlantData
    
    
Class: <http://www.semanticweb.org/izzet_kilicarslan/ontologies/2019/9/untitled-ontology-10#CapacitiyLimitation>

    SubClassOf: 
        <http://www.semanticweb.org/izzet_kilicarslan/ontologies/2019/9/untitled-ontology-10#SolarEntityDataset>
    
    
Class: <http://www.semanticweb.org/izzet_kilicarslan/ontologies/2019/9/untitled-ontology-10#ClusterBalticSea>

    SubClassOf: 
        SeaRegion
    
    
Class: <http://www.semanticweb.org/izzet_kilicarslan/ontologies/2019/9/untitled-ontology-10#ClusterNorthSea>

    SubClassOf: 
        SeaRegion
    
    
Class: <http://www.semanticweb.org/izzet_kilicarslan/ontologies/2019/9/untitled-ontology-10#CoastDistance>

    SubClassOf: 
        <http://purl.obolibrary.org/obo/BFO_0000009>
    
    
Class: <http://www.semanticweb.org/izzet_kilicarslan/ontologies/2019/9/untitled-ontology-10#CommissioningData>

    SubClassOf: 
        PlantOperation
    
    
Class: <http://www.semanticweb.org/izzet_kilicarslan/ontologies/2019/9/untitled-ontology-10#CommonInverterWithStorage>

    SubClassOf: 
        <http://www.semanticweb.org/izzet_kilicarslan/ontologies/2019/9/untitled-ontology-10#SolarEntityDataset>
    
    
Class: <http://www.semanticweb.org/izzet_kilicarslan/ontologies/2019/9/untitled-ontology-10#Community>

    SubClassOf: 
        LandRegion
    
    
Class: <http://www.semanticweb.org/izzet_kilicarslan/ontologies/2019/9/untitled-ontology-10#ConnectionToMaximumOrHighVoltage>

    SubClassOf: 
        PowerPlantData
    
    
Class: <http://www.semanticweb.org/izzet_kilicarslan/ontologies/2019/9/untitled-ontology-10#County>

    SubClassOf: 
        LandRegion
    
    
Class: <http://www.semanticweb.org/izzet_kilicarslan/ontologies/2019/9/untitled-ontology-10#DataFinalDecommissioning>

    SubClassOf: 
        PlantOperation
    
    
Class: <http://www.semanticweb.org/izzet_kilicarslan/ontologies/2019/9/untitled-ontology-10#DataRestartOperation>

    SubClassOf: 
        PlantOperation
    
    
Class: <http://www.semanticweb.org/izzet_kilicarslan/ontologies/2019/9/untitled-ontology-10#DataStartTemporaryDecommissioning>

    SubClassOf: 
        PlantOperation
    
    
Class: <http://www.semanticweb.org/izzet_kilicarslan/ontologies/2019/9/untitled-ontology-10#DateStartOfTemporaryorFinalDecommissioning>

    SubClassOf: 
        <http://www.semanticweb.org/izzet_kilicarslan/ontologies/2019/9/untitled-ontology-10#HydroEntityDataset>
    
    
Class: <http://www.semanticweb.org/izzet_kilicarslan/ontologies/2019/9/untitled-ontology-10#DisplayOfDecommissioning>

    SubClassOf: 
        <http://www.semanticweb.org/izzet_kilicarslan/ontologies/2019/9/untitled-ontology-10#HydroEntityDataset>
    
    
Class: <http://www.semanticweb.org/izzet_kilicarslan/ontologies/2019/9/untitled-ontology-10#District>

    SubClassOf: 
        LandRegion
    
    
Class: <http://www.semanticweb.org/izzet_kilicarslan/ontologies/2019/9/untitled-ontology-10#EmergencyGenerator>

    SubClassOf: 
        <http://www.semanticweb.org/izzet_kilicarslan/ontologies/2019/9/untitled-ontology-10#TechnicalDataStorage>
    
    
Class: <http://www.semanticweb.org/izzet_kilicarslan/ontologies/2019/9/untitled-ontology-10#EnergyCarrier>

    SubClassOf: 
        PowerPlantData
    
    
Class: <http://www.semanticweb.org/izzet_kilicarslan/ontologies/2019/9/untitled-ontology-10#EntityOperationStatus>

    SubClassOf: 
        PlantOperation
    
    
Class: <http://www.semanticweb.org/izzet_kilicarslan/ontologies/2019/9/untitled-ontology-10#FeedingType>

    SubClassOf: 
        PowerPlantData
    
    
Class: <http://www.semanticweb.org/izzet_kilicarslan/ontologies/2019/9/untitled-ontology-10#GaussKrügerEast>

    SubClassOf: 
        GeopgraphicCoordinate
    
    
Class: <http://www.semanticweb.org/izzet_kilicarslan/ontologies/2019/9/untitled-ontology-10#GaussKrügerNorth>

    SubClassOf: 
        GeopgraphicCoordinate
    
    
Class: <http://www.semanticweb.org/izzet_kilicarslan/ontologies/2019/9/untitled-ontology-10#GrossCapacity>

    SubClassOf: 
        PowerPlantData
    
    
Class: <http://www.semanticweb.org/izzet_kilicarslan/ontologies/2019/9/untitled-ontology-10#HouseNumber>

    SubClassOf: 
        GeographicRegion
    
    
Class: <http://www.semanticweb.org/izzet_kilicarslan/ontologies/2019/9/untitled-ontology-10#HubHeight>

    SubClassOf: 
        <http://www.semanticweb.org/izzet_kilicarslan/ontologies/2019/9/untitled-ontology-10#TechnicalDataWind>
    
    
Class: <http://www.semanticweb.org/izzet_kilicarslan/ontologies/2019/9/untitled-ontology-10#HydroEntityDataset>

    SubClassOf: 
        ElectricityProductionUnit
    
    
Class: <http://www.semanticweb.org/izzet_kilicarslan/ontologies/2019/9/untitled-ontology-10#IsolatedOperationCapability>

    SubClassOf: 
        PowerPlantData
    
    
Class: <http://www.semanticweb.org/izzet_kilicarslan/ontologies/2019/9/untitled-ontology-10#Latitude>

    SubClassOf: 
        GeopgraphicCoordinate
    
    
Class: <http://www.semanticweb.org/izzet_kilicarslan/ontologies/2019/9/untitled-ontology-10#Longitude>

    SubClassOf: 
        GeopgraphicCoordinate
    
    
Class: <http://www.semanticweb.org/izzet_kilicarslan/ontologies/2019/9/untitled-ontology-10#MainOrientation>

    SubClassOf: 
        <http://www.semanticweb.org/izzet_kilicarslan/ontologies/2019/9/untitled-ontology-10#SolarEntityDataset>
    
    
Class: <http://www.semanticweb.org/izzet_kilicarslan/ontologies/2019/9/untitled-ontology-10#MainOrientationTilt>

    SubClassOf: 
        <http://www.semanticweb.org/izzet_kilicarslan/ontologies/2019/9/untitled-ontology-10#SolarEntityDataset>
    
    
Class: <http://www.semanticweb.org/izzet_kilicarslan/ontologies/2019/9/untitled-ontology-10#NameElectricityProducerEntity>

    SubClassOf: 
        PowerPlantData
    
    
Class: <http://www.semanticweb.org/izzet_kilicarslan/ontologies/2019/9/untitled-ontology-10#NamePowerPlant>

    SubClassOf: 
        <http://www.semanticweb.org/izzet_kilicarslan/ontologies/2019/9/untitled-ontology-10#HydroEntityDataset>
    
    
Class: <http://www.semanticweb.org/izzet_kilicarslan/ontologies/2019/9/untitled-ontology-10#NetCapacity>

    SubClassOf: 
        PowerPlantData
    
    
Class: <http://www.semanticweb.org/izzet_kilicarslan/ontologies/2019/9/untitled-ontology-10#NetCapacityGermany>

    SubClassOf: 
        <http://www.semanticweb.org/izzet_kilicarslan/ontologies/2019/9/untitled-ontology-10#TechnicalDataStorage>
    
    
Class: <http://www.semanticweb.org/izzet_kilicarslan/ontologies/2019/9/untitled-ontology-10#NetCapacityGermanyHydro>

    SubClassOf: 
        <http://www.semanticweb.org/izzet_kilicarslan/ontologies/2019/9/untitled-ontology-10#HydroEntityDataset>
    
    
Class: <http://www.semanticweb.org/izzet_kilicarslan/ontologies/2019/9/untitled-ontology-10#NumbersOfModules>

    SubClassOf: 
        <http://www.semanticweb.org/izzet_kilicarslan/ontologies/2019/9/untitled-ontology-10#SolarEntityDataset>
    
    
Class: <http://www.semanticweb.org/izzet_kilicarslan/ontologies/2019/9/untitled-ontology-10#OccupiedArableLand>

    SubClassOf: 
        <http://www.semanticweb.org/izzet_kilicarslan/ontologies/2019/9/untitled-ontology-10#SolarEntityDataset>
    
    
Class: <http://www.semanticweb.org/izzet_kilicarslan/ontologies/2019/9/untitled-ontology-10#OccupiedArea>

    SubClassOf: 
        <http://www.semanticweb.org/izzet_kilicarslan/ontologies/2019/9/untitled-ontology-10#SolarEntityDataset>
    
    
Class: <http://www.semanticweb.org/izzet_kilicarslan/ontologies/2019/9/untitled-ontology-10#OperationSite>

    SubClassOf: 
        StorageUnitDataset
    
    
Class: <http://www.semanticweb.org/izzet_kilicarslan/ontologies/2019/9/untitled-ontology-10#ParcelNumber>

    SubClassOf: 
        GeographicRegion
    
    
Class: <http://www.semanticweb.org/izzet_kilicarslan/ontologies/2019/9/untitled-ontology-10#PartOfMarginalPowerPlant>

    SubClassOf: 
        <http://www.semanticweb.org/izzet_kilicarslan/ontologies/2019/9/untitled-ontology-10#TechnicalDataStorage>
    
    
Class: <http://www.semanticweb.org/izzet_kilicarslan/ontologies/2019/9/untitled-ontology-10#PartOfMarginalPowerPlantHydro>

    SubClassOf: 
        <http://www.semanticweb.org/izzet_kilicarslan/ontologies/2019/9/untitled-ontology-10#HydroEntityDataset>
    
    
Class: <http://www.semanticweb.org/izzet_kilicarslan/ontologies/2019/9/untitled-ontology-10#PlannedCommissioningData>

    SubClassOf: 
        PlantOperation
    
    
Class: <http://www.semanticweb.org/izzet_kilicarslan/ontologies/2019/9/untitled-ontology-10#PositionSolar>

    SubClassOf: 
        <http://www.semanticweb.org/izzet_kilicarslan/ontologies/2019/9/untitled-ontology-10#SolarEntityDataset>
    
    
Class: <http://www.semanticweb.org/izzet_kilicarslan/ontologies/2019/9/untitled-ontology-10#PostalCode>

    SubClassOf: 
        GeographicRegion
    
    
Class: <http://www.semanticweb.org/izzet_kilicarslan/ontologies/2019/9/untitled-ontology-10#PowerPlantnumber>

    SubClassOf: 
        PowerPlantData
    
    
Class: <http://www.semanticweb.org/izzet_kilicarslan/ontologies/2019/9/untitled-ontology-10#PrequalifiedForControlEnergy>

    SubClassOf: 
        PowerPlantData
    
    
Class: <http://www.semanticweb.org/izzet_kilicarslan/ontologies/2019/9/untitled-ontology-10#PumpOperationContinouslyAdjustable>

    SubClassOf: 
        <http://www.semanticweb.org/izzet_kilicarslan/ontologies/2019/9/untitled-ontology-10#TechnicalDataStorage>
    
    
Class: <http://www.semanticweb.org/izzet_kilicarslan/ontologies/2019/9/untitled-ontology-10#PumpOperationPowerConsumption>

    SubClassOf: 
        <http://www.semanticweb.org/izzet_kilicarslan/ontologies/2019/9/untitled-ontology-10#TechnicalDataStorage>
    
    
Class: <http://www.semanticweb.org/izzet_kilicarslan/ontologies/2019/9/untitled-ontology-10#PumpStorageTechnology>

    SubClassOf: 
        <http://www.semanticweb.org/izzet_kilicarslan/ontologies/2019/9/untitled-ontology-10#TechnicalDataStorage>
    
    
Class: <http://www.semanticweb.org/izzet_kilicarslan/ontologies/2019/9/untitled-ontology-10#ReductionElectricityGeneration>

    SubClassOf: 
        <http://www.semanticweb.org/izzet_kilicarslan/ontologies/2019/9/untitled-ontology-10#HydroEntityDataset>
    
    
Class: <http://www.semanticweb.org/izzet_kilicarslan/ontologies/2019/9/untitled-ontology-10#RemoteControl>

    SubClassOf: 
        PowerPlantData
    
    
Class: <http://www.semanticweb.org/izzet_kilicarslan/ontologies/2019/9/untitled-ontology-10#RemoteControlByThirdParties>

    SubClassOf: 
        <http://www.semanticweb.org/izzet_kilicarslan/ontologies/2019/9/untitled-ontology-10#RemoteControl>
    
    
Class: <http://www.semanticweb.org/izzet_kilicarslan/ontologies/2019/9/untitled-ontology-10#RemoteControlDirectMarketer>

    SubClassOf: 
        <http://www.semanticweb.org/izzet_kilicarslan/ontologies/2019/9/untitled-ontology-10#RemoteControl>
    
    
Class: <http://www.semanticweb.org/izzet_kilicarslan/ontologies/2019/9/untitled-ontology-10#RemoteControlGridOperator>

    SubClassOf: 
        <http://www.semanticweb.org/izzet_kilicarslan/ontologies/2019/9/untitled-ontology-10#RemoteControl>
    
    
Class: <http://www.semanticweb.org/izzet_kilicarslan/ontologies/2019/9/untitled-ontology-10#RequierementSwitchOffAnimalProtection>

    SubClassOf: 
        <http://www.semanticweb.org/izzet_kilicarslan/ontologies/2019/9/untitled-ontology-10#Requierements>
    
    
Class: <http://www.semanticweb.org/izzet_kilicarslan/ontologies/2019/9/untitled-ontology-10#RequierementSwitchOffCapacityLimitation>

    SubClassOf: 
        <http://www.semanticweb.org/izzet_kilicarslan/ontologies/2019/9/untitled-ontology-10#Requierements>
    
    
Class: <http://www.semanticweb.org/izzet_kilicarslan/ontologies/2019/9/untitled-ontology-10#RequierementSwitchOffIceFalling>

    SubClassOf: 
        <http://www.semanticweb.org/izzet_kilicarslan/ontologies/2019/9/untitled-ontology-10#Requierements>
    
    
Class: <http://www.semanticweb.org/izzet_kilicarslan/ontologies/2019/9/untitled-ontology-10#RequierementSwitchOffNoiseImmissionProtectionByDay>

    SubClassOf: 
        <http://www.semanticweb.org/izzet_kilicarslan/ontologies/2019/9/untitled-ontology-10#Requierements>
    
    
Class: <http://www.semanticweb.org/izzet_kilicarslan/ontologies/2019/9/untitled-ontology-10#RequierementSwitchOffNoiseImmissionProtectionNights>

    SubClassOf: 
        <http://www.semanticweb.org/izzet_kilicarslan/ontologies/2019/9/untitled-ontology-10#Requierements>
    
    
Class: <http://www.semanticweb.org/izzet_kilicarslan/ontologies/2019/9/untitled-ontology-10#RequierementSwitchOffOthers>

    SubClassOf: 
        <http://www.semanticweb.org/izzet_kilicarslan/ontologies/2019/9/untitled-ontology-10#Requierements>
    
    
Class: <http://www.semanticweb.org/izzet_kilicarslan/ontologies/2019/9/untitled-ontology-10#RequierementSwitchOffShadowing>

    SubClassOf: 
        <http://www.semanticweb.org/izzet_kilicarslan/ontologies/2019/9/untitled-ontology-10#Requierements>
    
    
Class: <http://www.semanticweb.org/izzet_kilicarslan/ontologies/2019/9/untitled-ontology-10#Requierements>

    SubClassOf: 
        WindEntityDataset
    
    
Class: <http://www.semanticweb.org/izzet_kilicarslan/ontologies/2019/9/untitled-ontology-10#RotorBladeDeIcingSystem>

    SubClassOf: 
        <http://www.semanticweb.org/izzet_kilicarslan/ontologies/2019/9/untitled-ontology-10#TechnicalDataWind>
    
    
Class: <http://www.semanticweb.org/izzet_kilicarslan/ontologies/2019/9/untitled-ontology-10#RotorDiameter>

    SubClassOf: 
        <http://www.semanticweb.org/izzet_kilicarslan/ontologies/2019/9/untitled-ontology-10#TechnicalDataWind>
    
    
Class: <http://www.semanticweb.org/izzet_kilicarslan/ontologies/2019/9/untitled-ontology-10#SeasideLocation>

    SubClassOf: 
        SeaRegion
    
    
Class: <http://www.semanticweb.org/izzet_kilicarslan/ontologies/2019/9/untitled-ontology-10#SecondaryOrientation>

    SubClassOf: 
        <http://www.semanticweb.org/izzet_kilicarslan/ontologies/2019/9/untitled-ontology-10#SolarEntityDataset>
    
    
Class: <http://www.semanticweb.org/izzet_kilicarslan/ontologies/2019/9/untitled-ontology-10#SecondaryOrientationTilt>

    SubClassOf: 
        <http://www.semanticweb.org/izzet_kilicarslan/ontologies/2019/9/untitled-ontology-10#SolarEntityDataset>
    
    
Class: <http://www.semanticweb.org/izzet_kilicarslan/ontologies/2019/9/untitled-ontology-10#SolarEntityDataset>

    SubClassOf: 
        ElectricityProductionUnit
    
    
Class: <http://www.semanticweb.org/izzet_kilicarslan/ontologies/2019/9/untitled-ontology-10#Street>

    SubClassOf: 
        LandRegion
    
    
Class: <http://www.semanticweb.org/izzet_kilicarslan/ontologies/2019/9/untitled-ontology-10#TechnicalDataStorage>

    SubClassOf: 
        StorageUnitDataset
    
    
Class: <http://www.semanticweb.org/izzet_kilicarslan/ontologies/2019/9/untitled-ontology-10#TechnicalDataWind>

    SubClassOf: 
        WindEntityDataset
    
    
Class: <http://www.semanticweb.org/izzet_kilicarslan/ontologies/2019/9/untitled-ontology-10#Technology>

    SubClassOf: 
        <http://www.semanticweb.org/izzet_kilicarslan/ontologies/2019/9/untitled-ontology-10#TechnicalDataStorage>,
        <http://www.semanticweb.org/izzet_kilicarslan/ontologies/2019/9/untitled-ontology-10#TechnicalDataWind>
    
    
Class: <http://www.semanticweb.org/izzet_kilicarslan/ontologies/2019/9/untitled-ontology-10#TypeOfArea>

    SubClassOf: 
        <http://www.semanticweb.org/izzet_kilicarslan/ontologies/2019/9/untitled-ontology-10#SolarEntityDataset>
    
    
Class: <http://www.semanticweb.org/izzet_kilicarslan/ontologies/2019/9/untitled-ontology-10#TypeOfDecommissioning>

    SubClassOf: 
        <http://www.semanticweb.org/izzet_kilicarslan/ontologies/2019/9/untitled-ontology-10#HydroEntityDataset>
    
    
Class: <http://www.semanticweb.org/izzet_kilicarslan/ontologies/2019/9/untitled-ontology-10#TypeOfHydroPowerPlant>

    SubClassOf: 
        <http://www.semanticweb.org/izzet_kilicarslan/ontologies/2019/9/untitled-ontology-10#HydroEntityDataset>
    
    
Class: <http://www.semanticweb.org/izzet_kilicarslan/ontologies/2019/9/untitled-ontology-10#TypeOfInflows>

    SubClassOf: 
        <http://www.semanticweb.org/izzet_kilicarslan/ontologies/2019/9/untitled-ontology-10#HydroEntityDataset>
    
    
Class: <http://www.semanticweb.org/izzet_kilicarslan/ontologies/2019/9/untitled-ontology-10#UniformOrientationAndTilt>

    SubClassOf: 
        <http://www.semanticweb.org/izzet_kilicarslan/ontologies/2019/9/untitled-ontology-10#SolarEntityDataset>
    
    
Class: <http://www.semanticweb.org/izzet_kilicarslan/ontologies/2019/9/untitled-ontology-10#UseableStorageCapacity>

    SubClassOf: 
        <http://www.semanticweb.org/izzet_kilicarslan/ontologies/2019/9/untitled-ontology-10#TechnicalDataStorage>
    
    
Class: <http://www.semanticweb.org/izzet_kilicarslan/ontologies/2019/9/untitled-ontology-10#UtmEast>

    SubClassOf: 
        GeopgraphicCoordinate
    
    
Class: <http://www.semanticweb.org/izzet_kilicarslan/ontologies/2019/9/untitled-ontology-10#UtmNorth>

    SubClassOf: 
        GeopgraphicCoordinate
    
    
Class: <http://www.semanticweb.org/izzet_kilicarslan/ontologies/2019/9/untitled-ontology-10#UtmZoneValue>

    SubClassOf: 
        GeopgraphicCoordinate
    
    
Class: <http://www.semanticweb.org/izzet_kilicarslan/ontologies/2019/9/untitled-ontology-10#WaterDepth>

    SubClassOf: 
        <http://purl.obolibrary.org/obo/BFO_0000009>
    
    
Class: <http://www.semanticweb.org/izzet_kilicarslan/ontologies/2019/9/untitled-ontology-10#Weic>

    SubClassOf: 
        PowerPlantData
    
    
Class: <http://www.semanticweb.org/izzet_kilicarslan/ontologies/2019/9/untitled-ontology-10#WeicDisplayName>

    SubClassOf: 
        PowerPlantData
    
    
Class: ACLine

    Annotations: 
        <http://purl.obolibrary.org/obo/IAO_0000115> "Alternating current high voltage transmission line. Can comprise multiple cables and multiple circuits.
Generally, flows in the model can not be controlled but are a function of the resitance and electrochemical potential difference."@en,
        rdfs:comment "undirected",
        rdfs:label "AC-Line"@en
    
    SubClassOf: 
        Line
    
    
Class: API

    SubClassOf: 
        Interface
    
    DisjointWith: 
        GUI
    
    
Class: Acronym

    Annotations: 
        <http://purl.obolibrary.org/obo/IAO_0000115> "An acronym is a abbreviation of the title by using the first letters of each part of the title."@en
    
    SubClassOf: 
        Identifier
    
    
Class: AdditionalToAddress

    SubClassOf: 
        GeographicRegion
    
    
Class: Agent

    Annotations: 
        <http://purl.obolibrary.org/obo/IAO_0000115> "An autonomous entity which acts, directing its activity towards achieving goals [...], upon an environment using observation through sensors and consequent actuators"@en,
        <http://purl.obolibrary.org/obo/IAO_0000119> "https://en.wikipedia.org/wiki/Intelligent_agent"@en
    
    SubClassOf: 
        <http://purl.obolibrary.org/obo/BFO_0000023>
    
    
Class: AgriculturalDemand

    SubClassOf: 
        Demand
    
    
Class: Air

    Annotations: 
        <http://purl.obolibrary.org/obo/IAO_0000115> "Air is compressed using surplus energy to store energy."@en
    
    SubClassOf: 
        EnergyCarrier,
        is_used_by some StorageUnit
    
    
Class: AirPollutant

    Annotations: 
        <http://purl.obolibrary.org/obo/IAO_0000115> "Air pollution occurs when harmful or excessive quantities of substances including gases, particles, and biological molecules are introduced into Earth's atmosphere."@en,
        <http://purl.obolibrary.org/obo/IAO_0000119> "https://en.wikipedia.org/w/index.php?title=Air_pollution&oldid=877082014"@en
    
    SubClassOf: 
        Pollutant
    
    
Class: AmbientHeat

    Annotations: 
        <http://purl.obolibrary.org/obo/IAO_0000115> "Ambient heat, understood as heat that is naturally around us in its diffuse and extended form, emanates from a diversity of heat sources, including earth, water, or air, and is increasingly attracting the attention of those concerned with energy and sustainability."@en,
        <http://purl.obolibrary.org/obo/IAO_0000119> "Urchueguia, J. F. (2016). Shallow geothermal and ambient heat technologies for renewable heating. In Renewable Heating and Cooling (pp. 89-118). Woodhead Publishing."@en
    
    SubClassOf: 
        Heat
    
    
Class: AnalyticalApproach

    SubClassOf: 
        ContentDescriptor
    
    
Class: Anthracite

    Annotations: 
        <http://purl.obolibrary.org/obo/IAO_0000115> "High rank coal used for industrial and residential applications. It has generally less than 10 % volatile matter and a high carbon content (about 90 % fixed carbon). Its gross calorific value is greater than 23 865 kJ/kg (5 700 kcal/kg) on an ash-free but moist basis."@en,
        <http://purl.obolibrary.org/obo/IAO_0000119> "REGULATION (EC) No 1099/2008 OF THE EUROPEAN PARLIAMENT AND OF THE COUNCIL of 22 October 2008 on energy statistics https://eur-lex.europa.eu/legal-content/EN/TXT/HTML/?uri=CELEX:32008R1099&from=EN"@en
    
    SubClassOf: 
        HardCoal
    
    
Class: Appliance

    SubClassOf: 
        ResidentialDemand
    
    
Class: AssociatedGas

    Annotations: 
        <http://purl.obolibrary.org/obo/IAO_0000115> "Natural gas produced in association with crude oil."@en,
        <http://purl.obolibrary.org/obo/IAO_0000119> "REGULATION (EC) No 1099/2008 OF THE EUROPEAN PARLIAMENT AND OF THE COUNCIL of 22 October 2008 on energy statistics https://eur-lex.europa.eu/legal-content/EN/TXT/HTML/?uri=CELEX:32008R1099&from=EN"@en
    
    SubClassOf: 
        NaturalGas
    
    
Class: Assumption

    Annotations: 
        <http://purl.obolibrary.org/obo/IAO_0000112> "The predicted demographic development for a country in the future."@en,
        <http://purl.obolibrary.org/obo/IAO_0000115> "An assumption is a statement about a property of a system or process that is considered to be true."@en
    
    SubClassOf: 
        InformationArtifact
    
    
Class: Author

    SubClassOf: 
        Agent
    
    
Class: AutoModelGenerator

    SubClassOf: 
        SoftwareElement
    
    
Class: Aviation

    SubClassOf: 
        TransportDemand
    
    
Class: AviationGasoline

    Annotations: 
        <http://purl.obolibrary.org/obo/IAO_0000115> "Motor spirit prepared especially for aviation piston engines, with an octane number suited to the engine, a freezing point of - 60 °C and a distillation range usually within the limits of 30 °C and 180 °C."@en,
        <http://purl.obolibrary.org/obo/IAO_0000119> "REGULATION (EC) No 1099/2008 OF THE EUROPEAN PARLIAMENT AND OF THE COUNCIL of 22 October 2008 on energy statistics https://eur-lex.europa.eu/legal-content/EN/TXT/HTML/?uri=CELEX:32008R1099&from=EN"@en
    
    SubClassOf: 
        Gasoline
    
    
Class: Battery

    Annotations: 
        <http://purl.obolibrary.org/obo/IAO_0000115> "A Battery is a device using different chemical or physical reactions to store energy."@en
    
    SubClassOf: 
        EnergyStorageTechnology,
        is_used_by some StorageUnit
    
    
Class: BatteryElectric

    SubClassOf: 
        TransportDemand
    
    
Class: BatteryStorage

    Annotations: 
        <http://purl.obolibrary.org/obo/IAO_0000115> "A battery storage is a energy storage that uses batteries to store energy."@en
    
    SubClassOf: 
        EnergyStorageTechnology
    
    DisjointWith: 
        MethanationGasStorage
    
    
Class: BioElectricityGenerator

    Annotations: 
        <http://purl.obolibrary.org/obo/IAO_0000115> "A bio electricity generator is a renewable energy generator that uses biomass or biogas to generate electricity."@en
    
    SubClassOf: 
        RenewableGeneratorTechnology
    
    
Class: BioGasGenerator

    Annotations: 
        <http://purl.obolibrary.org/obo/IAO_0000115> "A biogas generator uses biogas to generate electricity."@en
    
    SubClassOf: 
        EnergyGeneratorTechnology,
        has_physical_output some Power,
        has_physical_input only Biogas
    
    
Class: Biodiesel

    Annotations: 
        <http://purl.obolibrary.org/obo/IAO_0000115> "This category includes bio-diesel (a methyl-ester produced from vegetable or animal oil, of diesel quality), biodimethylether (dimethylether produced from biomass), Fischer-Tropsch (Fischer-Tropsch produced from biomass), cold extracted bio-oil (oil produced from oil seed through mechanical processing only) and all other liquid biofuels which are added to, blended with or used straight as transport diesel.",
        <http://purl.obolibrary.org/obo/IAO_0000119> "REGULATION (EC) No 1099/2008 OF THE EUROPEAN PARLIAMENT AND OF THE COUNCIL of 22 October 2008 on energy statistics https://eur-lex.europa.eu/legal-content/EN/TXT/HTML/?uri=CELEX:32008R1099&from=EN"
    
    SubClassOf: 
        LiquidBiofuel
    
    
Class: Biofuel

    Annotations: 
        <http://purl.obolibrary.org/obo/IAO_0000115> "A biofuel is a fuel that is produced through contemporary biological processes, such as agriculture and anaerobic digestion, rather than a fuel produced by geological processes such as those involved in the formation of fossil fuels, such as coal and petroleum, from prehistoric biological matter.

Biofuels can be derived directly from plants (i.e. energy crops), or indirectly from agricultural, commercial, domestic, and/or industrial wastes.[1] Renewable biofuels generally involve contemporary carbon fixation, such as those that occur in plants or microalgae through the process of photosynthesis. Other renewable biofuels are made through the use or conversion of biomass (referring to recently living organisms, most often referring to plants or plant-derived materials). This biomass can be converted to convenient energy-containing substances in three different ways: thermal conversion, chemical conversion, and biochemical conversion. This biomass conversion can result in fuel in solid, liquid, or gas form. This new biomass can also be used directly for biofuels.",
        <http://purl.obolibrary.org/obo/IAO_0000119> "https://en.wikipedia.org/w/index.php?title=Biofuel&oldid=866432109"
    
    SubClassOf: 
        Fuel
    
    
Class: Biogas

    Annotations: 
        <http://purl.obolibrary.org/obo/IAO_0000119> "REGULATION (EC) No 1099/2008 OF THE EUROPEAN PARLIAMENT AND OF THE COUNCIL of 22 October 2008 on energy statistics https://eur-lex.europa.eu/legal-content/EN/TXT/HTML/?uri=CELEX:32008R1099&from=EN",
        <http://purl.obolibrary.org/obo/IAO_0000119> "https://en.wikipedia.org/w/index.php?title=Biogas&oldid=867559571"
    
    SubClassOf: 
        Biofuel
    
    
Class: BiogasElectricityGenerator

    Annotations: 
        <http://purl.obolibrary.org/obo/IAO_0000115> "A biogas electricity generator is a bio energy generator that uses biogas to generate electricity."@en
    
    SubClassOf: 
        BioElectricityGenerator
    
    DisjointWith: 
        BiomassElectricityGenerator
    
    
Class: Biogasoline

    Annotations: 
        <http://purl.obolibrary.org/obo/IAO_0000115> "This category includes bioethanol (ethanol produced from biomass and/or the biodegradable fraction of waste), biomethanol (methanol produced from biomass and/or the biodegradable fraction of waste), bioETBE (ethyl-tertio-butyl-ether produced on the basis of bioethanol; the percentage by volume of bioETBE that is calculated as biofuel is 47 %) and bioMTBE (methyl-tertio-butyl-ether produced on the basis of biomethanol: the percentage by volume of bioMTBE that is calculated as biofuel is 36 %)",
        <http://purl.obolibrary.org/obo/IAO_0000119> "REGULATION (EC) No 1099/2008 OF THE EUROPEAN PARLIAMENT AND OF THE COUNCIL of 22 October 2008 on energy statistics https://eur-lex.europa.eu/legal-content/EN/TXT/HTML/?uri=CELEX:32008R1099&from=EN",
        rdfs:label "Bioethanol"@en,
        rdfs:label "Biogasoline"@en
    
    SubClassOf: 
        LiquidBiofuel
    
    
Class: BiomassElectricityGenerator

    Annotations: 
        <http://purl.obolibrary.org/obo/IAO_0000115> "A biomass electricity generator is a bio energy generator that uses biomass to generate electricity."@en
    
    SubClassOf: 
        BioElectricityGenerator
    
    DisjointWith: 
        BiogasElectricityGenerator
    
    
Class: BiomassPowerplant

    Annotations: 
        <http://purl.obolibrary.org/obo/IAO_0000115> "A biomass powerplant uses biomass to generate electricity or heat."@en
    
    SubClassOf: 
        RegenerativePowerplant,
        has_part some SteamTurbine
    
    
Class: BlastFurnaceGas

    Annotations: 
        <http://purl.obolibrary.org/obo/IAO_0000115> "Produced during the combustion of coke in blast furnaces in the iron and steel industry. It is recovered and used as a fuel partly within the plant and partly in other steel industry processes or in power stations equipped to burn it. The quantity of fuel should be reported on a gross calorific value basis."@en,
        <http://purl.obolibrary.org/obo/IAO_0000119> "REGULATION (EC) No 1099/2008 OF THE EUROPEAN PARLIAMENT AND OF THE COUNCIL of 22 October 2008 on energy statistics https://eur-lex.europa.eu/legal-content/EN/TXT/HTML/?uri=CELEX:32008R1099&from=EN"@en
    
    SubClassOf: 
        ManufacturedCoalBasedGas
    
    
Class: BooleanVariable

    Annotations: 
        <http://purl.obolibrary.org/obo/IAO_0000115> "A boolean variable is a variable that can only be true or false."@en
    
    SubClassOf: 
        InformationArtifact
    
    
Class: Bus

    Annotations: 
        <http://purl.obolibrary.org/obo/IAO_0000115> "A node in an electrical network."@en,
        rdfs:label "Bus"@en
    
    SubClassOf: 
        NetworkNode
    
    
Class: CapacitanceUnit

    Annotations: 
        <http://purl.obolibrary.org/obo/IAO_0000115> "A capacitance unit is a unit of measurement used to express the ratio of the change in an electric charge in a system to the corresponding change in its electric potential."@en
    
    SubClassOf: 
        UnitOfMeasurement
    
    
Class: CarbonDioxideEmission

    Annotations: 
        <http://purl.obolibrary.org/obo/IAO_0000115> "A carbon dioxide emission quantity is a quantity that is about carbon dioxide."@en
    
    SubClassOf: 
        Emission
    
    
Class: CarbonDioxideEmissionTrafficSector

    Annotations: 
        <http://purl.obolibrary.org/obo/IAO_0000115> "A carbon dioxide emission traffic sector quantity is a carbon dioxide emission quantity that is restricted to carbon dioxide from the traffic sector."@en
    
    SubClassOf: 
        CarbonDioxideEmission
    
    
Class: Charcoal

    Annotations: 
        <http://purl.obolibrary.org/obo/IAO_0000115> "The solid residue of the destructive distillation and pyrolysis of wood and other vegetal material."@en,
        <http://purl.obolibrary.org/obo/IAO_0000119> "REGULATION (EC) No 1099/2008 OF THE EUROPEAN PARLIAMENT AND OF THE COUNCIL of 22 October 2008 on energy statistics https://eur-lex.europa.eu/legal-content/EN/TXT/HTML/?uri=CELEX:32008R1099&from=EN"@en
    
    SubClassOf: 
        SolidBiomass
    
    
Class: Citation

    SubClassOf: 
        Identifier
    
    
Class: CitationReference

    SubClassOf: 
        Reference
    
    
Class: City

    Annotations: 
        <http://purl.obolibrary.org/obo/IAO_0000115> "A city is a large human settlement."@en
    
    SubClassOf: 
        LandRegion
    
    
Class: Client

    SubClassOf: 
        Agent
    
    
Class: Coal

    Annotations: 
        <http://purl.obolibrary.org/obo/IAO_0000115> "Coal is a combustible black or brownish-black sedimentary rock, formed as rock strata called coal seams. Coal is mostly carbon with variable amounts of other elements; chiefly hydrogen, sulfur, oxygen, and nitrogen.Coal is formed if dead plant matter decays into peat and over millions of years the heat and pressure of deep burial converts the peat into coal."@en,
        <http://purl.obolibrary.org/obo/IAO_0000119> "https://en.wikipedia.org/w/index.php?title=Coal&oldid=907331967"
    
    SubClassOf: 
        SolidFossilFuels,
        has_normal_state_of_matter value solid
    
    
Class: CoalElectricityGenerator

    Annotations: 
        <http://purl.obolibrary.org/obo/IAO_0000115> "A coal electricity generator technology uses coal to generate electricity."@en
    
    SubClassOf: 
        FossilGeneratorTechnology
    
    
Class: CoalPowerplant

    Annotations: 
        <http://purl.obolibrary.org/obo/IAO_0000115> "A coal-fired power station or coal power plant is a thermal power station which burns coal to generate electricity."@en,
        <http://purl.obolibrary.org/obo/IAO_0000119> "https://en.wikipedia.org/w/index.php?title=Coal-fired_power_station&oldid=905322370"
    
    SubClassOf: 
        FossilePowerplant,
        has_part some SteamTurbine
    
    
Class: CodeDocumentation

    SubClassOf: 
        Documentation
    
    
Class: CodeSource

    SubClassOf: 
        DataDescriptor,
        OpenSource
    
    
Class: CokeOvenGas

    Annotations: 
        <http://purl.obolibrary.org/obo/IAO_0000115> "Obtained as a by-product of the manufacture of coke oven coke for the production of iron and steel."@en,
        <http://purl.obolibrary.org/obo/IAO_0000119> "REGULATION (EC) No 1099/2008 OF THE EUROPEAN PARLIAMENT AND OF THE COUNCIL of 22 October 2008 on energy statistics https://eur-lex.europa.eu/legal-content/EN/TXT/HTML/?uri=CELEX:32008R1099&from=EN"@en
    
    SubClassOf: 
        ManufacturedCoalBasedGas
    
    
Class: CokingCoal

    Annotations: 
        <http://purl.obolibrary.org/obo/IAO_0000115> "Bituminous coal with a quality that allows the production of a coke suitable to support a blast furnace charge. Its gross calorific value is greater than 23 865 kJ/kg (5 700 kcal/kg) on an ash-free but moist basis."@en,
        <http://purl.obolibrary.org/obo/IAO_0000119> "REGULATION (EC) No 1099/2008 OF THE EUROPEAN PARLIAMENT AND OF THE COUNCIL of 22 October 2008 on energy statistics https://eur-lex.europa.eu/legal-content/EN/TXT/HTML/?uri=CELEX:32008R1099&from=EN"@en
    
    SubClassOf: 
        HardCoal
    
    
Class: CollaborativeProgramming

    SubClassOf: 
        OpenSource
    
    
Class: CollieryGas

    Annotations: 
        <http://purl.obolibrary.org/obo/IAO_0000115> "Methane produced at coal mines or from coal seams, piped to the surface and consumed at collieries or transmitted by pipeline to consumers."@en,
        <http://purl.obolibrary.org/obo/IAO_0000115> "REGULATION (EC) No 1099/2008 OF THE EUROPEAN PARLIAMENT AND OF THE COUNCIL of 22 October 2008 on energy statistics https://eur-lex.europa.eu/legal-content/EN/TXT/HTML/?uri=CELEX:32008R1099&from=EN"@en
    
    SubClassOf: 
        NaturalGas
    
    
Class: Combustion

    SubClassOf: 
        TransportDemand
    
    
Class: CommerceSector

    Annotations: 
        rdfs:label "ServiceSector"@en
    
    SubClassOf: 
        Sector
    
    
Class: CommericalDemand

    SubClassOf: 
        Demand
    
    
Class: CommonParameters

    SubClassOf: 
        ElectricityProductionUnit
    
    
Class: Community

    Annotations: 
        <http://purl.obolibrary.org/obo/IAO_0000115> "A consumer is a person or organization that uses economic services or commodities. A consumer is one that buys good for consumption and not for the resale and commercial purpose. The consumer is an individual who pays some amount of money or the thing required to consume goods and services produced."@en,
        <http://purl.obolibrary.org/obo/IAO_0000119> "https://en.wikipedia.org/w/index.php?title=Consumer&oldid=906220763"@en
    
    SubClassOf: 
        Support
    
    
Class: CompressedAir

    Annotations: 
        <http://purl.obolibrary.org/obo/IAO_0000115> "Air is compressed to store energy. To discharge energy, the air is expaned."@en
    
    SubClassOf: 
        Air
    
    
Class: ComputationTime

    SubClassOf: 
        SoftwareDescriptor
    
    
Class: Constraint

    Annotations: 
        <http://purl.obolibrary.org/obo/IAO_0000112> "\"The carbon dioxide emissions in Germany have to be reduced by 95% till 2050.\" is a constraint for a model calculation about the energy system."@en,
        <http://purl.obolibrary.org/obo/IAO_0000115> "A constraint is a condition that has to be fullfilled within a calculation."@en
    
    SubClassOf: 
        InformationArtifact
    
    
Class: Consumer

    Annotations: 
        <http://purl.obolibrary.org/obo/IAO_0000115> "A consumer is a person or organization that uses economic services or commodities. A consumer is one that buys good for consumption and not for the resale and commercial purpose. The consumer is an individual who pays some amount of money or the thing required to consume goods and services produced."@en,
        <http://purl.obolibrary.org/obo/IAO_0000119> "https://en.wikipedia.org/w/index.php?title=Consumer&oldid=906220763"@en
    
    SubClassOf: 
        Agent
    
    
Class: ConsumptionQuantity

    Annotations: 
        <http://purl.obolibrary.org/obo/IAO_0000115> "A consumption quantity is a quantity that describes the amount of consumption of some resource."@en
    
    SubClassOf: 
        Quantity
    
    
Class: Contact

    SubClassOf: 
        InformationArtifact
    
    
Class: ContactPerson

    SubClassOf: 
        Agent
    
    
Class: ContentDescriptor

    SubClassOf: 
        InformationArtifact
    
    
Class: Continent

    Annotations: 
        <http://purl.obolibrary.org/obo/IAO_0000115> "A continent is a large landmass on the earth."@en
    
    SubClassOf: 
        LandRegion
    
    
Class: CorporateIdentity

    SubClassOf: 
        InformationArtifact
    
    
Class: Cost

    SubClassOf: 
        ModelVariable
    
    
Class: Country

    Annotations: 
        <http://purl.obolibrary.org/obo/IAO_0000115> "A country is a geographic region that is an distinct political entity."@en
    
    SubClassOf: 
        LandRegion
    
    
Class: CrudeOil

    Annotations: 
        <http://purl.obolibrary.org/obo/IAO_0000115> "Crude oil is a mineral oil of natural origin comprising a mixture of hydrocarbons and associated impurities, such as sulphur. It exists in the liquid phase under normal surface temperature and pressure and its physical characteristics (density, viscosity, etc.) are highly variable. This category includes field or lease condensate recovered from associated and non-associated gas where it is commingled with the commercial crude oil stream."@en,
        <http://purl.obolibrary.org/obo/IAO_0000119> "REGULATION (EC) No 1099/2008 OF THE EUROPEAN PARLIAMENT AND OF THE COUNCIL of 22 October 2008 on energy statistics https://eur-lex.europa.eu/legal-content/EN/TXT/HTML/?uri=CELEX:32008R1099&from=EN"@en
    
    SubClassOf: 
        Liquid,
        OilAndPetroleumProducts
    
    
Class: DCLine

    Annotations: 
        <http://purl.obolibrary.org/obo/IAO_0000115> "Transmission system usind high voltage direct current.
Genreally, flows in the model can be controlled/optimized."@en,
        rdfs:comment "directed",
        rdfs:label "HVDC-Line"@en
    
    SubClassOf: 
        Line
    
    
Class: DOI

    Annotations: 
        <http://purl.obolibrary.org/obo/IAO_0000115> "A DOI (digital object identifier) is a persistent identifier or handle used to uniquely identify objects, standardized by the International Organization for Standardization (ISO).
source: https://en.wikipedia.org/wiki/Digital_object_identifier"@en
    
    SubClassOf: 
        Identifier
    
    
Class: DammedWater

    Annotations: 
        <http://purl.obolibrary.org/obo/IAO_0000115> "A dam is a barrier that stops or restricts the flow of water or underground streams. Reservoirs created by dams not only suppress floods but also provide water for activities such as irrigation, human consumption, industrial use, aquaculture, and navigability. Hydropower is often used in conjunction with dams to generate electricity."@en,
        <http://purl.obolibrary.org/obo/IAO_0000119> "https://en.wikipedia.org/w/index.php?title=Dam&oldid=906014627"@en
    
    SubClassOf: 
        Hydroelectricity,
        is_used_by some StorageUnit
    
    
Class: DataDescriptor

    SubClassOf: 
        InformationArtifact
    
    
Class: DataFormat

    SubClassOf: 
        DataDescriptor
    
    DisjointWith: 
        OpenSource
    
    
Class: DataPostprocessing

    SubClassOf: 
        DataProcessing
    
    
Class: DataPreprocessing

    SubClassOf: 
        DataProcessing
    
    
Class: DataProcessing

    SubClassOf: 
        SoftwareElement
    
    
Class: DataProcessingSoftware

    SubClassOf: 
        Software
    
    
Class: Database

    SubClassOf: 
        DataFormat
    
    DisjointWith: 
        Plot
    
    
Class: Dataset

    Annotations: 
        <http://purl.obolibrary.org/obo/IAO_0000112> "A list of power plants.
The measurement series of an expiriment."@en,
        <http://purl.obolibrary.org/obo/IAO_0000115> "A dataset is a collection of information artifacts of the same type about a common topic."@en
    
    SubClassOf: 
        InformationArtifact
    
    
Class: Demand

    Annotations: 
        <http://purl.obolibrary.org/obo/IAO_0000115> "Demand is generally the need for energy, colloquially referred to as energy consumption.
Source: https://wiki.openmod-initiative.org/wiki/Demand"@en
    
    SubClassOf: 
        ConsumptionQuantity
    
    
Class: DemandSector

    Annotations: 
        <http://purl.obolibrary.org/obo/IAO_0000115> "A demand sector is a general term for different consumptions (households; industry; commercial sector; transport). It includes only energy demand sectors."@en
    
    SubClassOf: 
        Sector
    
    
Class: DemographicalAssumption

    Annotations: 
        <http://purl.obolibrary.org/obo/IAO_0000112> "The predicted demographic development of some country, city or the world."@en,
        <http://purl.obolibrary.org/obo/IAO_0000115> "A demographical assumption is an assumption about the population of a region."@en
    
    SubClassOf: 
        Assumption
    
    
Class: DerivedHeat

    Annotations: 
        <http://purl.obolibrary.org/obo/IAO_0000115> "Derived heat covers the total heat production in heating plants and in combined heat and power plants. It includes the heat used by the auxiliaries of the installation which use hot fluid (space heating, liquid fuel heating, etc.) And losses in the installation/network heat exchanges. For autoproducing entities (= entities generating electricity and/or heat wholly or partially for their own use as an activity which supports their primary activity) the heat used by the undertaking for its own processes is not included."@en,
        <http://purl.obolibrary.org/obo/IAO_0000119> "https://ec.europa.eu/eurostat/ramon/nomenclatures/index.cfm?TargetUrl=DSP_GLOSSARY_NOM_DTL_VIEW&StrNom=CODED2&StrLanguageCode=EN&IntKey=16452285&RdoSearch=&TxtSearch=&CboTheme=&IntCurrentPage=1"@en
    
    EquivalentTo: 
        DistrictHeat
    
    SubClassOf: 
        Heat
    
    
Class: Developer

    SubClassOf: 
        Agent
    
    
Class: DieselFuel

    Annotations: 
        <http://purl.obolibrary.org/obo/IAO_0000115> "On-road diesel oil for diesel compression ignition (cars, trucks, etc.), usually of low sulphur content."@en,
        <http://purl.obolibrary.org/obo/IAO_0000119> "REGULATION (EC) No 1099/2008 OF THE EUROPEAN PARLIAMENT AND OF THE COUNCIL of 22 October 2008 on energy statistics https://eur-lex.europa.eu/legal-content/EN/TXT/HTML/?uri=CELEX:32008R1099&from=EN"@en,
        rdfs:label "DieselFuel"@en,
        rdfs:label "TransportDiesel"@en
    
    SubClassOf: 
        GasDieselOil
    
    
Class: DistrictHeat

    Annotations: 
        <http://purl.obolibrary.org/obo/IAO_0000115> "District heating (also known as heat networks or teleheating) is a system for distributing heat generated in a centralized location through a system of insulated pipes for residential and commercial heating requirements such as space heating and water heating. The heat is often obtained from a cogeneration plant burning fossil fuels or biomass, but heat-only boiler stations, geothermal heating, heat pumps and central solar heating are also used, as well as heat waste from nuclear power electricity generation. "@en,
        <http://purl.obolibrary.org/obo/IAO_0000119> "https://en.wikipedia.org/w/index.php?title=District_heating&oldid=906646999"@en
    
    EquivalentTo: 
        DerivedHeat
    
    SubClassOf: 
        Heat
    
    
Class: Documentation

    SubClassOf: 
        SoftwareMaintenance
    
    
Class: Ecological

    SubClassOf: 
        Type
    
    
Class: Economical

    SubClassOf: 
        Type
    
    
Class: EconomicalAssumption

    Annotations: 
        <http://purl.obolibrary.org/obo/IAO_0000112> "The predicted development of GDP of a country."@en,
        <http://purl.obolibrary.org/obo/IAO_0000112> "The predicted prizes of fossil fuel."@en,
        <http://purl.obolibrary.org/obo/IAO_0000115> "An economical assumption is an assumption about the economical state or development of a region."@en
    
    SubClassOf: 
        Assumption
    
    
Class: ElectricChargeUnit

    Annotations: 
        <http://purl.obolibrary.org/obo/IAO_0000115> "An electric charge unit is a unit of measurement used to express the physical property of matter that causes it to experience a force when placed in an electromagnetic field."@en
    
    SubClassOf: 
        UnitOfMeasurement
    
    
Class: ElectricCurrentUnit

    Annotations: 
        <http://purl.obolibrary.org/obo/IAO_0000115> "An electric current unit is a unit of measurement used to express the flow of electric charge."@en
    
    SubClassOf: 
        UnitOfMeasurement
    
    
Class: ElectricVehicle

    Annotations: 
        <http://purl.obolibrary.org/obo/IAO_0000115> "An electric vehicle, also called an EV, uses one or more electric motors or traction motors for propulsion. An electric vehicle may be powered through a collector system by electricity from off-vehicle sources, or may be self-contained with a battery, solar panels or an electric generator to convert fuel to electricity."@en,
        <http://purl.obolibrary.org/obo/IAO_0000119> "https://en.wikipedia.org/w/index.php?title=Electric_vehicle&oldid=906776214"@en
    
    SubClassOf: 
        EnergyStorageTechnology
    
    
Class: ElectricalEnergy

    Annotations: 
        <http://purl.obolibrary.org/obo/IAO_0000115> "Electrical energy is energy derived from electric potential energy or kinetic energy. [...] This energy is supplied by the combination of electric current and electric potential that is delivered by an electrical circuit"@en,
        <http://purl.obolibrary.org/obo/IAO_0000119> "https://en.wikipedia.org/wiki/Electrical_energy"@en
    
    SubClassOf: 
        EnergyCarrier
    
    
Class: ElectricalLoad

    Annotations: 
        <http://purl.obolibrary.org/obo/IAO_0000115> "An electrical load is an electrical component or portion of a circuit that consumes (active) electric power. This is opposed to a power source, such as a battery or generator, which produces power. In electric power circuits examples of loads are appliances and lights. The term may also refer to the power consumed by a circuit.

    Source: https://en.wikipedia.org/wiki/Electrical_load"@en,
        rdfs:label "ElectricalDemand"@en,
        rdfs:label "ElectricalLoad"@en
    
    SubClassOf: 
        Demand
    
    
Class: ElectricityConsumption

    Annotations: 
        <http://purl.obolibrary.org/obo/IAO_0000115> "An electricity consumption quantity is a consumption quantity about electricity."@en
    
    SubClassOf: 
        ConsumptionQuantity
    
    
Class: ElectricityExport

    Annotations: 
        <http://purl.obolibrary.org/obo/IAO_0000115> "An electricity export quantity is a quantity that describes the amount of electricity that is exported from a geographic region."@en
    
    SubClassOf: 
        Quantity
    
    
Class: ElectricityGeneratorTechnology

    Annotations: 
        <http://purl.obolibrary.org/obo/IAO_0000115> "An electricity generator technology is an technology used to transform energy from some source into electricity."@en
    
    SubClassOf: 
        Technology
    
    
Class: ElectricityGrid

    Annotations: 
        <http://purl.obolibrary.org/obo/IAO_0000115> "An electrical grid is an interconnected network for delivering electricity from producers to consumers.
Source: https://en.wikipedia.org/wiki/Electrical_grid"@en,
        rdfs:comment "Synonym: Network"@en
    
    SubClassOf: 
        <http://purl.obolibrary.org/obo/BFO_0000031>,
        has_part some ElectricityGridComponent,
        has_part min 1 EnergyGeneratorTechnology,
        has_part min 1 Line
    
    
Class: ElectricityGridComponent

    Annotations: 
        <http://purl.obolibrary.org/obo/IAO_0000115> "A grid component is a part of an electrical grid."@en
    
    SubClassOf: 
        <http://purl.obolibrary.org/obo/BFO_0000031>,
        part_of some ElectricityGrid
    
    
Class: ElectricityProductionUnit

    SubClassOf: 
        ElectricityGridComponent
    
    
Class: ElectricitySector

    Annotations: 
        <http://purl.obolibrary.org/obo/IAO_0000115> "Covers all areas that deal with electrical energy (power generation; electricity transmission; electricity storage; electricity use)."@en,
        <http://purl.obolibrary.org/obo/IAO_0000119> "https://wiki.openmod-initiative.org/wiki/Electricity_sector"@en
    
    SubClassOf: 
        Sector
    
    
Class: Email

    SubClassOf: 
        Contact
    
    
Class: Emission

    Annotations: 
        <http://purl.obolibrary.org/obo/IAO_0000115> "1. Emissions are waste from production, distribution and consumption, which are distributed to environmental media. Emmision is often restricted to pollutants.
        
        2. Emissions generally means discharge of any interference in the environment. The source is called the issuer. Each emission causes an immission."@en,
        <http://purl.obolibrary.org/obo/IAO_0000119> "https://wiki.openmod-initiative.org/wiki/Emmision"@en
    
    SubClassOf: 
        Quantity
    
    
Class: EmissionFactor

    Annotations: 
        <http://purl.obolibrary.org/obo/IAO_0000115> "Emission factors assume a linear relation between the intensity of the activity and the emission resulting from this activity:

Emission (pollutant) = Activity * Emission Factor (pollutant)",
        <http://purl.obolibrary.org/obo/IAO_0000115> "https://en.wikipedia.org/w/index.php?title=Emission_intensity&oldid=881841342"
    
    SubClassOf: 
        Quantity
    
    
Class: EmpiricalDataset

    Annotations: 
        <http://purl.obolibrary.org/obo/IAO_0000112> "The measurement series of some experiment."@en,
        <http://purl.obolibrary.org/obo/IAO_0000115> "An empirical dataset is a dataset that is optained from observations in the real world."@en
    
    SubClassOf: 
        Dataset
    
    DisjointWith: 
        SynthethicDataset
    
    
Class: EnergyCarrier

    Annotations: 
        <http://purl.obolibrary.org/obo/IAO_0000115> "According to ISO 13600, an energy carrier is either a substance or a phenomenon that can be used to produce mechanical work or heat or to operate chemical or physical processes. It is any system or substance that contains energy for conversion as usable energy later or somewhere else. This could be converted for use in, for example, an appliance or vehicle. Such carriers include springs, electrical batteries, capacitors, pressurized air, dammed water, hydrogen, petroleum, coal, wood, and natural gas."@en,
        <http://purl.obolibrary.org/obo/IAO_0000119> "https://en.wikipedia.org/w/index.php?title=Energy_carrier&oldid=828742268"
    
    SubClassOf: 
        <http://purl.obolibrary.org/obo/BFO_0000030>
    
    
Class: EnergyCarrierQuantity

    Annotations: 
        <http://purl.obolibrary.org/obo/IAO_0000115> "An energy carrier quantity is a quantity about the amount of energy from a certain energy carrier."@en
    
    SubClassOf: 
        Quantity
    
    
Class: EnergyConsumption

    Annotations: 
        <http://purl.obolibrary.org/obo/IAO_0000115> "An energy consumption quantity is a consumption quantity about energy."@en
    
    SubClassOf: 
        ConsumptionQuantity
    
    
Class: EnergyFromAlternativeFuelsAndPropulsionInTraffic

    Annotations: 
        <http://purl.obolibrary.org/obo/IAO_0000115> "A energy from alternative fuels and populsion in traffic quantity is a energy carrier quantity that describes the amount alternative energy carriers are used in the traffic sector."@en
    
    SubClassOf: 
        EnergyCarrierQuantity
    
    
Class: EnergyFromBioFuelInTraffic

    Annotations: 
        <http://purl.obolibrary.org/obo/IAO_0000115> "A energy from bio fuel in traffic quantity is a energy carrier quantity that describes the amount of bio fuel as energy carrier in traffic."@en
    
    SubClassOf: 
        EnergyCarrierQuantity
    
    
Class: EnergyFromElectricityInTraffic

    Annotations: 
        <http://purl.obolibrary.org/obo/IAO_0000115> "A energy from electricity in traffic quantity is a energy carrier quantity that describes the amount of electricity used as energy carrier in traffic."@en
    
    SubClassOf: 
        EnergyCarrierQuantity
    
    
Class: EnergyGeneratorTechnology

    Annotations: 
        <http://purl.obolibrary.org/obo/IAO_0000115> "An energy generator technology is an technology used to transform energy into a form such that it is useable."@en
    
    SubClassOf: 
        Technology,
        has_physical_input some EnergyCarrier,
        has_physical_output some Power
    
    
Class: EnergySector

    Annotations: 
        <http://purl.obolibrary.org/obo/IAO_0000115> "An energy sector is a sector that contains the energy production."@en
    
    SubClassOf: 
        Sector
    
    
Class: EnergyStorageTechnology

    Annotations: 
        <http://purl.obolibrary.org/obo/IAO_0000115> "An energy storage technology is a technology used for storing energy."@en
    
    SubClassOf: 
        Technology
    
    
Class: EnergyTransferTechnology

    Annotations: 
        <http://purl.obolibrary.org/obo/IAO_0000115> "An energy transfer technology is a technology used to transport energy or a carrier of energy."@en
    
    SubClassOf: 
        Technology
    
    
Class: EnergyUnit

    Annotations: 
        <http://purl.obolibrary.org/obo/IAO_0000112> "Joule, kWh"@en,
        <http://purl.obolibrary.org/obo/IAO_0000115> "A energy unit is a unit of measurement used to express the energy of an object or the energy transformed during a process."@en
    
    SubClassOf: 
        UnitOfMeasurement
    
    
Class: ExternalOptimizer

    SubClassOf: 
        Software
    
    
Class: Factsheet

    SubClassOf: 
        EmpiricalDataset
    
    
Class: Fax

    SubClassOf: 
        Contact
    
    
Class: FederalState

    Annotations: 
        <http://purl.obolibrary.org/obo/IAO_0000115> "A federal state is a geographic region that is a political entity within a country. It is partially self governing."@en
    
    SubClassOf: 
        LandRegion
    
    
Class: FieldPhotovoltaicGenerator

    Annotations: 
        <http://purl.obolibrary.org/obo/IAO_0000115> "A field photovoltaic electricity generator is a photovoltaic electricity generator that is installed out in the open on the ground."@en
    
    SubClassOf: 
        PhotovoltaicElectricityGenerator
    
    DisjointWith: 
        RooftopPhotovoltaicGenerator
    
    
Class: Fission

    Annotations: 
        <http://purl.obolibrary.org/obo/IAO_0000115> "In nuclear physics and nuclear chemistry, nuclear fission is a nuclear reaction or a radioactive decay process in which the nucleus of an atom splits into smaller, lighter nuclei. The fission process often produces free neutrons and gamma photons, and releases a very large amount of energy even by the energetic standards of radioactive decay. "@en,
        <http://purl.obolibrary.org/obo/IAO_0000119> "https://en.wikipedia.org/w/index.php?title=Nuclear_fission&oldid=905727345"@en
    
    SubClassOf: 
        Nuclear
    
    
Class: FixedOperationCost

    SubClassOf: 
        Cost
    
    
Class: FlourinatedGas

    Annotations: 
        <http://purl.obolibrary.org/obo/IAO_0000115> "Fluorinated gases (F-gases) are man-made gases that can stay in the atmosphere for centuries and contribute to a global greenhouse effect. There are four types: hydrofluorocarbons (HFCs), perfluorocarbons (PFCs), sulfur hexafluoride (SF6) and nitrogen trifluoride (NF3)."@en,
        <http://purl.obolibrary.org/obo/IAO_0000119> "https://en.wikipedia.org/w/index.php?title=Fluorinated_gases&oldid=902170998"@en
    
    SubClassOf: 
        Gas,
        has_disposition some GreenhouseGas
    
    
Class: Flow

    Annotations: 
        <http://purl.obolibrary.org/obo/IAO_0000115> ""
    
    SubClassOf: 
        Water
    
    DisjointWith: 
        Ocean
    
    
Class: FlowBattery

    Annotations: 
        <http://purl.obolibrary.org/obo/IAO_0000115> "A flow battery, or redox flow battery (after reduction–oxidation), is a type of electrochemical cell where chemical energy is provided by two chemical components dissolved in liquids contained within the system and separated by a membrane. Ion exchange (accompanied by flow of electric current) occurs through the membrane while both liquids circulate in their own respective space."@en,
        <http://purl.obolibrary.org/obo/IAO_0000119> "https://en.wikipedia.org/w/index.php?title=Flow_battery&oldid=907053515"@en
    
    SubClassOf: 
        Battery
    
    
Class: Forum

    SubClassOf: 
        Support
    
    
Class: FossilGeneratorTechnology

    Annotations: 
        <http://purl.obolibrary.org/obo/IAO_0000115> "A fossil electricity generator technology is an electricity generator techonolgy that uses fossil fuels such as oil, coal and natural gas to generate electricity."@en
    
    SubClassOf: 
        ElectricityGeneratorTechnology
    
    DisjointWith: 
        RenewableGeneratorTechnology
    
    
Class: FossilePowerplant

    SubClassOf: 
        PowerGeneratingUnit
    
    
Class: Framework

    SubClassOf: 
        SoftwareElement
    
    
Class: FrameworkFactsheet

    SubClassOf: 
        Factsheet
    
    
Class: Fuel

    Annotations: 
        <http://purl.obolibrary.org/obo/IAO_0000115> "A fuel is any material that can be made to react with other substances so that it releases energy as heat energy or to be used for work. The concept was originally applied solely to those materials capable of releasing chemical energy but has since also been applied to other sources of heat energy such as nuclear energy (via nuclear fission and nuclear fusion).",
        <http://purl.obolibrary.org/obo/IAO_0000119> "https://en.wikipedia.org/w/index.php?title=Fuel&oldid=866720145"
    
    SubClassOf: 
        EnergyCarrier
    
    
Class: FuelPrice

    SubClassOf: 
        Cost
    
    
Class: Funding

    SubClassOf: 
        SoftwareMaintenance
    
    
Class: Fusion

    Annotations: 
        <http://purl.obolibrary.org/obo/IAO_0000115> "In nuclear chemistry, nuclear fusion is a reaction in which two or more atomic nuclei are combined to form one or more different atomic nuclei and subatomic particles (neutrons or protons). The difference in mass between the reactants and products is manifested as either the release or absorption of energy."@en,
        <http://purl.obolibrary.org/obo/IAO_0000119> "https://en.wikipedia.org/w/index.php?title=Nuclear_fusion&oldid=906947069"@en
    
    SubClassOf: 
        Nuclear
    
    
Class: GUI

    SubClassOf: 
        Interface
    
    DisjointWith: 
        API
    
    
Class: Gas

    Annotations: 
        <http://purl.obolibrary.org/obo/IAO_0000115> "Gas is one of the four fundamental states of matter (the others being solid, liquid, and plasma). A pure gas may be made up of individual atoms (e.g. a noble gas like neon), elemental molecules made from one type of atom (e.g. oxygen), or compound molecules made from a variety of atoms (e.g. carbon dioxide). A gas mixture, such as air, contains a variety of pure gases. What distinguishes a gas from liquids and solids is the vast separation of the individual gas particles. This separation usually makes a colorless gas invisible to the human observer."@en,
        <http://purl.obolibrary.org/obo/IAO_0000119> "https://en.wikipedia.org/w/index.php?title=Gas&oldid=904791916"@en
    
    SubClassOf: 
        StateOfMatter
    
    
Class: GasDieselOil

    Annotations: 
        <http://purl.obolibrary.org/obo/IAO_0000115> "Gas/diesel oil is primarily a medium distillate distilling between 180 °C and 380 °C. Includes blending components. Several grades are available depending on uses."@en,
        <http://purl.obolibrary.org/obo/IAO_0000119> "REGULATION (EC) No 1099/2008 OF THE EUROPEAN PARLIAMENT AND OF THE COUNCIL of 22 October 2008 on energy statistics https://eur-lex.europa.eu/legal-content/EN/TXT/HTML/?uri=CELEX:32008R1099&from=EN"@en
    
    SubClassOf: 
        OilAndPetroleumProducts,
        has_normal_state_of_matter value liquid
    
    
Class: GasPowerplant

    Annotations: 
        <http://purl.obolibrary.org/obo/IAO_0000115> "A gas-fired power plant or gas-fired power station or natural gas power plant is a thermal power station which burns natural gas to generate electricity. Natural gas power stations generate a quarter of world electricity and a significant part of global greenhouse gas emissions and thus global warming."@en,
        <http://purl.obolibrary.org/obo/IAO_0000119> "https://en.wikipedia.org/w/index.php?title=Gas-fired_power_plant&oldid=905149105"@en
    
    SubClassOf: 
        FossilePowerplant,
        has_part some GasTurbine
    
    
Class: GasTurbine

    Annotations: 
        <http://purl.obolibrary.org/obo/IAO_0000115> "A gas turbine, also called a combustion turbine, is a type of continuous combustion, internal combustion engine."@en,
        <http://purl.obolibrary.org/obo/IAO_0000119> "https://en.wikipedia.org/w/index.php?title=Gas_turbine&oldid=901583703"@en
    
    SubClassOf: 
        Turbine,
        has_physical_output some Power,
        has_physical_input only NaturalGas
    
    
Class: GasTurbineGenerator

    Annotations: 
        <http://purl.obolibrary.org/obo/IAO_0000115> "A gas turbine generator is a electricity generator that uses hot or high pressure gas to produce electricity."@en
    
    SubClassOf: 
        ElectricityGeneratorTechnology
    
    
Class: Gasoline

    Annotations: 
        <http://purl.obolibrary.org/obo/IAO_0000115> "Gasoline (American English) or petrol (British English) is a transparent petroleum-derived liquid that is used primarily as a fuel in spark-ignited internal combustion engines. It consists mostly of organic compounds obtained by the fractional distillation of petroleum, enhanced with a variety of additives.",
        <http://purl.obolibrary.org/obo/IAO_0000115> "https://en.wikipedia.org/w/index.php?title=Gasoline&oldid=867948640"
    
    SubClassOf: 
        OilAndPetroleumProducts,
        has_normal_state_of_matter value liquid
    
    
Class: GasworksGas

    Annotations: 
        <http://purl.obolibrary.org/obo/IAO_0000115> "Covers all types of gases produced in public utility or private plants, whose main purpose is manufacture, transport and distribution of gas. It includes gas produced by carbonisation (including gas produced by coke ovens and transferred to gasworks gas), by total gasification with or without enrichment with oil products (LPG, residual fuel oil, etc.), and by reforming and simple mixing of gases and/or air, reported under the rows ‘from other sources’. Under the transformation sector identify amounts of gasworks gas transferred to blended natural gas which will be distributed and consumed through the natural gas grid.

The production of other coal gases (i.e. coke oven gas, blast furnace gas and oxygen steel furnace gas) should be reported in the columns concerning such gases, and not as production of gasworks gas. The coal gases transferred to gasworks plants should then be reported (in their own column) in the transformation sector in the gasworks plants row. The total amount of gasworks gas resulting from transfers of other coal gases should appear in the production line for gasworks gas."@en,
        <http://purl.obolibrary.org/obo/IAO_0000119> "REGULATION (EC) No 1099/2008 OF THE EUROPEAN PARLIAMENT AND OF THE COUNCIL of 22 October 2008 on energy statistics https://eur-lex.europa.eu/legal-content/EN/TXT/HTML/?uri=CELEX:32008R1099&from=EN"@en
    
    SubClassOf: 
        ManufacturedCoalBasedGas
    
    
Class: Generator

    Annotations: 
        <http://purl.obolibrary.org/obo/IAO_0000115> "A generator is a grid component that converts motive power (mechanical energy) into electrical power for use in an external circuit.
Source: https://en.wikipedia.org/wiki/Electric_generator"@en
    
    SubClassOf: 
        ElectricityGridComponent,
        uses some EnergyCarrier,
        uses some EnergyGeneratorTechnology
    
    DisjointWith: 
        Line
    
    
Class: GeographicRegion

    Annotations: 
        <http://purl.obolibrary.org/obo/IAO_0000115> "A geographic region is a delimited part of the earth."@en
    
    SubClassOf: 
        <http://purl.obolibrary.org/obo/BFO_0000006>
    
    
Class: GeopgraphicCoordinate

    SubClassOf: 
        <http://purl.obolibrary.org/obo/BFO_0000141>
    
    
Class: Geothermal

    Annotations: 
        <http://purl.obolibrary.org/obo/IAO_0000115> "Energy available as heat emitted from within the earth's crust, usually in the form of hot water or steam. This energy production is the difference between the enthalpy of the fluid produced in the production borehole and that of the fluid eventually disposed of. It is exploited at suitable sites:
— for electricity generation using dry steam or high enthalpy brine after flashing,
— directly as heat for district heating, agriculture etc"@en,
        <http://purl.obolibrary.org/obo/IAO_0000119> "REGULATION (EC) No 1099/2008 OF THE EUROPEAN PARLIAMENT AND OF THE COUNCIL of 22 October 2008 on energy statistics https://eur-lex.europa.eu/legal-content/EN/TXT/HTML/?uri=CELEX:32008R1099&from=EN"@en
    
    SubClassOf: 
        Heat
    
    
Class: GeothermalGenerator

    SubClassOf: 
        Generator,
        uses some Heat
    
    
Class: GeothermalPowerplant

    Annotations: 
        <http://purl.obolibrary.org/obo/IAO_0000115> "A geothermal generator uses geothermal energy to generate electricity."@en
    
    SubClassOf: 
        RegenerativePowerplant,
        has_part some SteamTurbine
    
    
Class: GitHub

    Annotations: 
        <http://purl.obolibrary.org/obo/IAO_0000115> "A geothermal generator uses geothermal energy to generate electricity."@en
    
    SubClassOf: 
        Weblink
    
    
Class: GlobalWarmingPotential

    Annotations: 
        <http://purl.obolibrary.org/obo/IAO_0000115> "Global warming potential (GWP) is a measure of how much heat a greenhouse gas traps in the atmosphere up to a specific time horizon, relative to carbon dioxide. It compares the amount of heat trapped by a certain mass of the gas in question to the amount of heat trapped by a similar mass of carbon dioxide and is expressed as a factor of carbon dioxide (whose GWP is standardized to 1).

A GWP is calculated over a specific time horizon, commonly 20, 100, or 500 years. User related choices such as the time horizon can greatly affect the numerical values obtained for carbon dioxide equivalents.",
        <http://purl.obolibrary.org/obo/IAO_0000119> "https://en.wikipedia.org/w/index.php?title=Global_warming_potential&oldid=878160191"
    
    SubClassOf: 
        Quantity
    
    
Class: Graph

    SubClassOf: 
        <http://purl.obolibrary.org/obo/BFO_0000024>
    
    
Class: GreenhouseGas

    Annotations: 
        <http://purl.obolibrary.org/obo/IAO_0000115> "A greenhouse gas is a gas that absorbs and emits radiant energy within the thermal infrared range. Greenhouse gases cause the greenhouse effect.",
        <http://purl.obolibrary.org/obo/IAO_0000119> "https://en.wikipedia.org/w/index.php?title=Greenhouse_gas&oldid=880592155"
    
    SubClassOf: 
        Pollutant
    
    
Class: GridModel

    SubClassOf: 
        SoftwareElement
    
    
Class: HFC

    Annotations: 
        <http://purl.obolibrary.org/obo/IAO_0000115> "Hydrofluorocarbons (HFCs) are organic compounds that contain fluorine and hydrogen atoms, and are the most common type of organofluorine compounds. They are frequently used in air conditioning and as refrigerants in place of the older chlorofluorocarbons such as R-12 and hydrochlorofluorocarbons such as R-21."@en,
        <http://purl.obolibrary.org/obo/IAO_0000119> "https://en.wikipedia.org/w/index.php?title=Hydrofluorocarbon&oldid=904556263"@en
    
    EquivalentTo: 
        Hydrofluorocarbon
    
    SubClassOf: 
        FlourinatedGas
    
    
Class: HardCoal

    Annotations: 
        <http://purl.obolibrary.org/obo/IAO_0000115> "The term ‘hard coal’ refers to coal of gross calorific value greater than 23 865 kJ/kg (5 700 kcal/kg) on an ashfree but moist basis and with a mean random reflectance of vitrinite of at least 0,6."@en,
        <http://purl.obolibrary.org/obo/IAO_0000119> "REGULATION (EC) No 1099/2008 OF THE EUROPEAN PARLIAMENT AND OF THE COUNCIL of 22 October 2008 on energy statistics https://eur-lex.europa.eu/legal-content/EN/TXT/HTML/?uri=CELEX:32008R1099&from=EN"@en
    
    SubClassOf: 
        Coal
    
    DisjointWith: 
        Lignite
    
    
Class: HardCoalPowerplant

    Annotations: 
        <http://purl.obolibrary.org/obo/IAO_0000115> "A hard coal powerplant burns coal to generate electricity."@en
    
    SubClassOf: 
        CoalPowerplant
    
    
Class: Hardware

    Annotations: 
        <http://purl.obolibrary.org/obo/IAO_0000115> "In thermodynamics, heat is energy in transfer to or from a thermodynamic system, by mechanisms other than thermodynamic work or transfer of matter.
       The mechanisms include conduction, through direct contact of immobile bodies, or through a wall or barrier that is impermeable to matter; or radiation between separated bodies; or isochoric mechanical work done by the surroundings on the system of interest; or Joule heating by an electric current driven through the system of interest by an external system; or a combination of these."@en,
        <http://purl.obolibrary.org/obo/IAO_0000119> "https://en.wikipedia.org/w/index.php?title=Heat&oldid=90563031157"@en
    
    SubClassOf: 
        ModelingTechnology
    
    
Class: Heat

    Annotations: 
        <http://purl.obolibrary.org/obo/IAO_0000115> "In thermodynamics, heat is energy in transfer to or from a thermodynamic system, by mechanisms other than thermodynamic work or transfer of matter.
       The mechanisms include conduction, through direct contact of immobile bodies, or through a wall or barrier that is impermeable to matter; or radiation between separated bodies; or isochoric mechanical work done by the surroundings on the system of interest; or Joule heating by an electric current driven through the system of interest by an external system; or a combination of these."@en,
        <http://purl.obolibrary.org/obo/IAO_0000119> "https://en.wikipedia.org/w/index.php?title=Heat&oldid=90563031157"@en
    
    SubClassOf: 
        EnergyCarrier
    
    
Class: HeatConsumption

    Annotations: 
        <http://purl.obolibrary.org/obo/IAO_0000115> "A heat consumption quantity is a consumption quantity about heat."@en
    
    SubClassOf: 
        ConsumptionQuantity
    
    
Class: HeatDemand

    Annotations: 
        <http://purl.obolibrary.org/obo/IAO_0000115> "The heat demand describes the needed amount of heat."@en
    
    SubClassOf: 
        Demand
    
    
Class: HeatGeneratorTechnology

    Annotations: 
        <http://purl.obolibrary.org/obo/IAO_0000115> "A heat generator technology is an technology used to transform energy from some source into heat."@en
    
    SubClassOf: 
        Technology
    
    
Class: HeatPumpHeatGenerator

    Annotations: 
        <http://purl.obolibrary.org/obo/IAO_0000115> "A heat pump heat generator is a heat generator that uses a heat pump to generate heat."@en
    
    SubClassOf: 
        HeatGeneratorTechnology
    
    
Class: HeatSector

    Annotations: 
        <http://purl.obolibrary.org/obo/IAO_0000115> "Energy used for heating and cooling for buildings and industry"@en,
        rdfs:label "HeatingCoolingSector"@en
    
    SubClassOf: 
        Sector
    
    
Class: HeatingOil

    Annotations: 
        <http://purl.obolibrary.org/obo/IAO_0000115> "Light heating oil for industrial and commercial uses, marine diesel and diesel used in rail traffic, other gas oil, including heavy gas oils which distil between 380 °C and 540 °C and which are used as petrochemical feedstocks."@en,
        <http://purl.obolibrary.org/obo/IAO_0000119> "REGULATION (EC) No 1099/2008 OF THE EUROPEAN PARLIAMENT AND OF THE COUNCIL of 22 October 2008 on energy statistics https://eur-lex.europa.eu/legal-content/EN/TXT/HTML/?uri=CELEX:32008R1099&from=EN"@en,
        rdfs:label "HeatingOil"@en,
        rdfs:label "OtherGasOil"@en
    
    SubClassOf: 
        GasDieselOil
    
    
Class: HouseholdSector

    Annotations: 
        <http://purl.obolibrary.org/obo/IAO_0000115> "The household sector covers all private entities. A household is a  shared living unit."@en
    
    SubClassOf: 
        Sector
    
    
Class: HubHeight

    SubClassOf: 
        TechnicalDataWind
    
    
Class: HydroPowerplant

    SubClassOf: 
        Generator
    
    
Class: HydroelectricPowerplant

    Annotations: 
        <http://purl.obolibrary.org/obo/IAO_0000115> "A hydroelectric powerplant uses water to generate electricity."@en
    
    SubClassOf: 
        PowerGeneratingUnit,
        has_part some WaterTurbine
    
    
Class: Hydroelectricity

    Annotations: 
        <http://purl.obolibrary.org/obo/IAO_0000115> "Potential and kinetic energy of water converted into electricity in hydroelectric plants.",
        <http://purl.obolibrary.org/obo/IAO_0000119> "REGULATION (EC) No 1099/2008 OF THE EUROPEAN PARLIAMENT AND OF THE COUNCIL of 22 October 2008 on energy statistics https://eur-lex.europa.eu/legal-content/EN/TXT/HTML/?uri=CELEX:32008R1099&from=EN"
    
    SubClassOf: 
        EnergyStorageTechnology,
        Hydropower
    
    
Class: Hydrofluorocarbon

    Annotations: 
        <http://purl.obolibrary.org/obo/IAO_0000115> "Hydrofluorocarbons (HFCs) are organic compounds that contain fluorine and hydrogen atoms, and are the most common type of organofluorine compounds. They are frequently used in air conditioning and as refrigerants in place of the older chlorofluorocarbons such as R-12 and hydrochlorofluorocarbons such as R-21."@en,
        <http://purl.obolibrary.org/obo/IAO_0000119> "https://en.wikipedia.org/w/index.php?title=Hydrofluorocarbon&oldid=904556263"@en
    
    EquivalentTo: 
        HFC
    
    SubClassOf: 
        FlourinatedGas
    
    
Class: Hydrogen

    Annotations: 
        <http://purl.obolibrary.org/obo/IAO_0000115> "Hydrogen is a chemical element with chemical symbol H and atomic number 1. It is used in water electrolysis during the power-to-gas process as a storage medium for excess electricty."@en,
        <http://purl.obolibrary.org/obo/IAO_0000119> "https://wiki.openmod-initiative.org/wiki/Hydrogen"@en
    
    SubClassOf: 
        EnergyStorageTechnology
    
    
Class: HydrogenPowerplant

    Annotations: 
        <http://purl.obolibrary.org/obo/IAO_0000115> "A hydrogen powerplant uses hydrogen to generate electricity."@en
    
    SubClassOf: 
        ReactivePowerplant,
        has_part some HydrogenTurbine
    
    
Class: HydrogenTurbine

    Annotations: 
        <http://purl.obolibrary.org/obo/IAO_0000115> "A hydrogen turbine is a turbine fueled with liquid hydrogen."@en
    
    SubClassOf: 
        Turbine,
        has_physical_output some Power,
        has_physical_input only Hydrogen
    
    
Class: HydrogenVehicle

    SubClassOf: 
        TransportDemand
    
    
Class: Hydropower

    Annotations: 
        <http://purl.obolibrary.org/obo/IAO_0000115> "Hydropower or water power [...] is power derived from the energy of falling water or fast running water, which may be harnessed for useful purposes."@en,
        <http://purl.obolibrary.org/obo/IAO_0000119> "https://en.wikipedia.org/w/index.php?title=Hydropower&oldid=906980683"@en
    
    SubClassOf: 
        EnergyCarrier
    
    
Class: Identifier

    Annotations: 
        <http://purl.obolibrary.org/obo/IAO_0000115> "An Identifier is an information artifact used to identify an entity."@en
    
    SubClassOf: 
        InformationArtifact
    
    
Class: IndustrialWaste

    Annotations: 
        <http://purl.obolibrary.org/obo/IAO_0000115> "Report wastes of industrial non-renewable origin (solids or liquids) combusted directly for the production of electricity and/or heat. The quantity of fuel used should be reported on a net calorific value basis. Renewable industrial waste should be reported in the solid biomass, biogas and/or liquid biofuels categories."@en,
        <http://purl.obolibrary.org/obo/IAO_0000119> "REGULATION (EC) No 1099/2008 OF THE EUROPEAN PARLIAMENT AND OF THE COUNCIL of 22 October 2008 on energy statistics https://eur-lex.europa.eu/legal-content/EN/TXT/HTML/?uri=CELEX:32008R1099&from=EN"@en
    
    SubClassOf: 
        Waste
    
    
Class: IndustrySector

    Annotations: 
        <http://purl.obolibrary.org/obo/IAO_0000115> "Industry consumption is specified as follows (energy used for transport by industry is not included here but is reported under transport):

* Iron and steel industry
* Chemical and petrochemical industry
* Non-ferrous metals
* Non-metallic minerals
* Transport equipment
* Machinery
* Mining (excluding fuels) and quarrying
* Food and tobacco
* Paper, pulp and print
* Wood and wood products (other than pulp and paper)
* Construction
* Textile and leather
* Non-specified (any manufacturing industry not included above)"@en
    
    SubClassOf: 
        Sector
    
    
Class: InformationArtifact

    Annotations: 
        <http://purl.obolibrary.org/obo/IAO_0000115> "An information artifact is an entity that contains information about some thing in digital or written form."@en
    
    SubClassOf: 
        <http://purl.obolibrary.org/obo/BFO_0000031>
    
    
Class: InstallationGuide

    SubClassOf: 
        Documentation
    
    
Class: InstalledHeatFromHeatPump

    Annotations: 
        <http://purl.obolibrary.org/obo/IAO_0000115> "An installed power from heat pump quantity is a installed power quantity restricted to heat pump power plants."@en
    
    SubClassOf: 
        InstalledPowerQuantity
    
    
Class: InstalledHeatFromSolar

    Annotations: 
        <http://purl.obolibrary.org/obo/IAO_0000115> "An installed power from solar quantity is a installed power quantity restricted to solar heat power plants."@en
    
    SubClassOf: 
        InstalledPowerQuantity
    
    
Class: InstalledPowerFromBiomass

    Annotations: 
        <http://purl.obolibrary.org/obo/IAO_0000115> "An installed power from biomass quantity is a installed power quantity restricted to biomass power plants."@en
    
    SubClassOf: 
        InstalledPowerQuantity
    
    
Class: InstalledPowerFromCoalPowerPlants

    Annotations: 
        <http://purl.obolibrary.org/obo/IAO_0000115> "An installed power from coal power plants quantity is a installed power quantity restricted to coal power plants."@en
    
    SubClassOf: 
        InstalledPowerQuantity
    
    
Class: InstalledPowerFromGas

    Annotations: 
        <http://purl.obolibrary.org/obo/IAO_0000115> "An installed power from gas quantity is a installed power quantity restricted to gas power plants."@en
    
    SubClassOf: 
        InstalledPowerQuantity
    
    
Class: InstalledPowerFromPhotovoltaics

    Annotations: 
        <http://purl.obolibrary.org/obo/IAO_0000115> "An installed power from photovoltaics quantity is a installed power quantity restricted to photovoltaic power plants."@en
    
    SubClassOf: 
        InstalledPowerQuantity
    
    
Class: InstalledPowerFromThermalPowerPlants

    Annotations: 
        <http://purl.obolibrary.org/obo/IAO_0000115> "An installed power from thermal power plants quantity is a installed power quantity restricted to thermal power plants."@en
    
    SubClassOf: 
        InstalledPowerQuantity
    
    
Class: InstalledPowerFromWind

    Annotations: 
        <http://purl.obolibrary.org/obo/IAO_0000115> "An installed power from wind quantity is a installed power quantity restricted to wind power plants."@en
    
    SubClassOf: 
        InstalledPowerQuantity
    
    
Class: InstalledPowerQuantity

    Annotations: 
        <http://purl.obolibrary.org/obo/IAO_0000115> "An installed power quantity is a quantity that describes the amount of power that some generators can generate."@en
    
    SubClassOf: 
        Quantity
    
    
Class: Institution

    Annotations: 
        <http://purl.obolibrary.org/obo/IAO_0000115> "An institution is an organization that serve a social purpose."@en
    
    SubClassOf: 
        Organization
    
    
Class: Interface

    SubClassOf: 
        SoftwareElement
    
    
Class: InvestmentCost

    SubClassOf: 
        Cost
    
    
Class: JetFuel

    Annotations: 
        <http://purl.obolibrary.org/obo/IAO_0000115> "Distillate used for aviation turbine power units. It has the same distillation characteristics between 150 °C and 300 °C (generally not above 250 °C) and flash point as kerosene. In addition, it has particular specifications (such as freezing point) which are established by the International Air Transport Association (IATA)."@en,
        <http://purl.obolibrary.org/obo/IAO_0000119> "REGULATION (EC) No 1099/2008 OF THE EUROPEAN PARLIAMENT AND OF THE COUNCIL of 22 October 2008 on energy statistics https://eur-lex.europa.eu/legal-content/EN/TXT/HTML/?uri=CELEX:32008R1099&from=EN"@en,
        rdfs:label "JetFuel"@en,
        rdfs:label "KeroseneTypeJetFuel"@en
    
    SubClassOf: 
        Kerosene
    
    
Class: Kerosene

    Annotations: 
        <http://purl.obolibrary.org/obo/IAO_0000115> "Kerosene, also known as paraffin, lamp oil, and coal oil (an obsolete term), is a combustible hydrocarbon liquid which is derived from petroleum. It is widely used as a fuel in industry as well as households. Its name derives from Greek: κηρός (keros) meaning wax, and was registered as a trademark by Canadian geologist and inventor Abraham Gesner in 1854 before evolving into a genericized trademark. It is sometimes spelled kerosine in scientific and industrial usage.
[...]

Kerosene is widely used to power jet engines of aircraft (jet fuel) and some rocket engines and is also commonly used as a cooking and lighting fuel and for fire toys such as poi. In parts of Asia, kerosene is sometimes used as fuel for small outboard motors or even motorcycles.",
        <http://purl.obolibrary.org/obo/IAO_0000119> "https://en.wikipedia.org/w/index.php?title=Kerosene&oldid=867958484"
    
    SubClassOf: 
        OilAndPetroleumProducts,
        has_normal_state_of_matter value liquid
    
    
Class: LandRegion

    SubClassOf: 
        <http://purl.obolibrary.org/obo/BFO_0000028>
    
    
Class: LengthUnit

    Annotations: 
        <http://purl.obolibrary.org/obo/IAO_0000112> "metre"@en,
        <http://purl.obolibrary.org/obo/IAO_0000115> "A length unit is a unit of measurement used to express the distance of two points."@en
    
    SubClassOf: 
        UnitOfMeasurement
    
    
Class: Li-ionBattery

    Annotations: 
        <http://purl.obolibrary.org/obo/IAO_0000115> "A lithium-ion battery or Li-ion battery (abbreviated as LIB) is a type of rechargeable battery [...] In the batteries lithium ions move from the negative electrode to the positive electrode during discharge and back when charging. Li-ion batteries use an intercalated lithium compound as one electrode material, compared to the metallic lithium used in a non-rechargeable lithium battery. "@en,
        <http://purl.obolibrary.org/obo/IAO_0000119> "https://en.wikipedia.org/w/index.php?title=Lithium-ion_battery&oldid=906786251"@en
    
    SubClassOf: 
        Battery
    
    
Class: License

    SubClassOf: 
        SoftwareDescriptor
    
    
Class: Lignite

    Annotations: 
        <http://purl.obolibrary.org/obo/IAO_0000115> "Non-agglomerating coal with a gross calorific value less than 17 435 kJ/kg (4 165 kcal/kg) and greater than 31 % volatile matter on a dry mineral matter free basis.

Oil shale and tar sands produced and combusted directly should be reported in this category. Oil shale and tar sands used as inputs for other transformation processes should also be reported in this category.

This includes the portion of the oil shale or tar sands consumed in the transformation process."@en,
        <http://purl.obolibrary.org/obo/IAO_0000119> "REGULATION (EC) No 1099/2008 OF THE EUROPEAN PARLIAMENT AND OF THE COUNCIL of 22 October 2008 on energy statistics https://eur-lex.europa.eu/legal-content/EN/TXT/HTML/?uri=CELEX:32008R1099&from=EN"@en
    
    SubClassOf: 
        Coal
    
    DisjointWith: 
        HardCoal
    
    
Class: LignitePowerplant

    Annotations: 
        <http://purl.obolibrary.org/obo/IAO_0000115> "A lignite powerplant burns lignite to generate electricity."@en
    
    SubClassOf: 
        CoalPowerplant
    
    
Class: Line

    Annotations: 
        <http://purl.obolibrary.org/obo/IAO_0000115> "An uninterrupted transmission system between two nodes in the electric grid."@en,
        rdfs:label "PowerLine"@en
    
    SubClassOf: 
        Link
    
    DisjointWith: 
        Generator
    
    
Class: LinearOptimalPowerflow

    SubClassOf: 
        GridModel
    
    
Class: Link

    SubClassOf: 
        <http://purl.obolibrary.org/obo/BFO_0000024>
    
    DisjointWith: 
        Node
    
    
Class: Liquid

    Annotations: 
        <http://purl.obolibrary.org/obo/IAO_0000115> "A liquid is a nearly incompressible fluid that conforms to the shape of its container but retains a (nearly) constant volume independent of pressure. As such, it is one of the four fundamental states of matter (the others being solid, gas, and plasma), and is the only state with a definite volume but no fixed shape. A liquid is made up of tiny vibrating particles of matter, such as atoms, held together by intermolecular bonds."@en,
        <http://purl.obolibrary.org/obo/IAO_0000119> "https://en.wikipedia.org/w/index.php?title=Liquid&oldid=904993133"@en
    
    SubClassOf: 
        StateOfMatter
    
    
Class: LiquidAir

    Annotations: 
        <http://purl.obolibrary.org/obo/IAO_0000115> "Air is compressed and cooled to store energy. To discharge energy, the air is expaned."@en
    
    SubClassOf: 
        Air
    
    
Class: LiquidBiofuel

    Annotations: 
        <http://purl.obolibrary.org/obo/IAO_0000115> "The quantities of liquid biofuels reported in this category should relate to the quantities of biofuel and not to the total volume of liquids into which the biofuels are blended.

The following liquid biofuels are concerned: biogasoline, bio-diesels, other liquid biofuels"@en,
        <http://purl.obolibrary.org/obo/IAO_0000119> "REGULATION (EC) No 1099/2008 OF THE EUROPEAN PARLIAMENT AND OF THE COUNCIL of 22 October 2008 on energy statistics https://eur-lex.europa.eu/legal-content/EN/TXT/HTML/?uri=CELEX:32008R1099&from=EN"@en
    
    SubClassOf: 
        Biofuel,
        has_normal_state_of_matter value liquid
    
    
Class: LiquidMetalBattery

    Annotations: 
        <http://purl.obolibrary.org/obo/IAO_0000115> "Rechargeable liquid-metal batteries are used for electric vehicles and potentially also for grid energy storage, to balance out intermittent renewable power sources such as solar panels and wind turbines."@en,
        <http://purl.obolibrary.org/obo/IAO_0000119> "https://en.wikipedia.org/w/index.php?title=Molten-salt_battery&oldid=900557096"@en
    
    SubClassOf: 
        MoltenStateBattery
    
    
Class: LoadArea

    Annotations: 
        <http://purl.obolibrary.org/obo/IAO_0000115> "A load area is an area that contains energy consumption.

Source: https://wiki.openmod-initiative.org/wiki/Load_area"@en
    
    SubClassOf: 
        LandRegion
    
    
Class: Logo

    SubClassOf: 
        CorporateIdentity
    
    
Class: MaStR

    SubClassOf: 
        EmpiricalDataset
    
    
Class: Mail

    SubClassOf: 
        Support
    
    
Class: ManufacturedCoalBasedGas

    Annotations: 
        <http://purl.obolibrary.org/obo/IAO_0000115> "Coal gasification is the process of producing syngas–a mixture consisting primarily of carbon monoxide (CO), hydrogen (H2), carbon dioxide (CO2), natural gas (CH4) , and water vapour (H2O)–from coal and water, air and/or oxygen."@en,
        <http://purl.obolibrary.org/obo/IAO_0000119> "https://en.wikipedia.org/w/index.php?title=Coal_gasification&oldid=904933607"@en
    
    SubClassOf: 
        SolidFossilFuels,
        has_normal_state_of_matter value gaseous
    
    
Class: Manufacturer

    SubClassOf: 
        ManufacturerSpecifications
    
    
Class: ManufacturerSpecifications

    SubClassOf: 
        WindEntityData,
        WindEntityDataset
    
    
Class: MarketModel

    SubClassOf: 
        Model
    
    
Class: MassUnit

    Annotations: 
        <http://purl.obolibrary.org/obo/IAO_0000112> "kg"@en,
        <http://purl.obolibrary.org/obo/IAO_0000115> "A mass unit is a unit of measurement used to express the mass of an object."@en
    
    SubClassOf: 
        UnitOfMeasurement
    
    
Class: MathematicalConcept

    SubClassOf: 
        ModelElement
    
    
Class: Maximization

    SubClassOf: 
        ModelFunction
    
    
Class: MethanationGasStorage

    Annotations: 
        <http://purl.obolibrary.org/obo/IAO_0000115> "A methanation gas storage is a energy storage that uses carbon dioxide and hydrogen from electrolysis to produce methan and store this. The methan can then be used to produce electricity or heat in a gas generator."@en
    
    SubClassOf: 
        EnergyStorageTechnology
    
    DisjointWith: 
        BatteryStorage
    
    
Class: MethodicalFocus

    SubClassOf: 
        ContentDescriptor
    
    
Class: Microgrid

    Annotations: 
        <http://purl.obolibrary.org/obo/IAO_0000115> "A microgrid is a localized group of electricity sources and loads that normally operates connected to and synchronous with the traditional wide area synchronous grid (macrogrid), but can also disconnect to \"island mode\" — and function autonomously as physical or economic conditions dictate. In this way, a microgrid can effectively integrate various sources of distributed generation (DG), especially Renewable Energy Sources (RES) - renewable electricity, and can supply emergency power, changing between island and connected modes. "@en,
        <http://purl.obolibrary.org/obo/IAO_0000119> "https://en.wikipedia.org/w/index.php?title=Microgrid&oldid=906195407"@en
    
    SubClassOf: 
        ElectricityGrid,
        Subgrid
    
    
Class: Minimization

    SubClassOf: 
        ModelFunction
    
    
Class: Model

    Annotations: 
        <http://purl.obolibrary.org/obo/IAO_0000115> "A model is a tool for computing the behavior of a system using an idealized representation."@en
    
    SubClassOf: 
        ModelingSoftware,
        has_part some SoftwareElement
    
    
Class: ModelCalculation

    Annotations: 
        <http://purl.obolibrary.org/obo/IAO_0000115> "A model calculation is a transformation using at least one model."@en
    
    SubClassOf: 
        Transformation,
        has_tool some Model
    
    
Class: ModelElement

    Annotations: 
        <http://purl.obolibrary.org/obo/IAO_0000115> "A model element is an elementary model component."@en
    
    SubClassOf: 
        InformationArtifact,
        <http://purl.obolibrary.org/obo/BFO_0000031>,
        part_of some Model
    
    
Class: ModelExamples

    SubClassOf: 
        Support
    
    
Class: ModelFactsheet

    SubClassOf: 
        Factsheet
    
    
Class: ModelFunction

    Annotations: 
        <http://purl.obolibrary.org/obo/IAO_0000112> "The function that calculates the costs of the energy system in a simulation."@en,
        <http://purl.obolibrary.org/obo/IAO_0000115> "A model function is a model component that is a function."@en
    
    SubClassOf: 
        Model
    
    
Class: ModelVariable

    Annotations: 
        <http://purl.obolibrary.org/obo/IAO_0000115> "A model variable is a variable inside a model."@en
    
    SubClassOf: 
        ModelElement
    
    
Class: ModelingSoftware

    SubClassOf: 
        Software
    
    
Class: ModelingTechnology

    SubClassOf: 
        Technology
    
    
Class: Modus

    SubClassOf: 
        InformationArtifact
    
    
Class: MoltenSaltBattery

    Annotations: 
        <http://purl.obolibrary.org/obo/IAO_0000115> "Molten-salt batteries are a class of battery that uses molten salts as an electrolyte and offers both a high energy density and a high power density."@en,
        <http://purl.obolibrary.org/obo/IAO_0000119> "https://en.wikipedia.org/w/index.php?title=Molten-salt_battery&oldid=900557096"@en
    
    SubClassOf: 
        MoltenStateBattery,
        SoftwareElement
    
    
Class: MoltenStateBattery

    Annotations: 
        <http://purl.obolibrary.org/obo/IAO_0000115> "Molten-state batteries consist of two molten metal alloys separated by an electrolyte."@en
    
    SubClassOf: 
        Battery
    
    
Class: MotorGasoline

    Annotations: 
        <http://purl.obolibrary.org/obo/IAO_0000115> "Motor gasoline consists of a mixture of light hydrocarbons distilling between 35 oC and 215 oC. It is used as a fuel for land based spark ignition engines. Motor gasoline may include additives, oxygenates and octane enhancers, including lead compounds such as TEL and TML.

Includes motor gasoline blending components (excluding additives/oxygenates), e.g. alkylates, isomerate, reformate, cracked gasoline destined for use as finished motor gasoline."@en,
        <http://purl.obolibrary.org/obo/IAO_0000119> "REGULATION (EC) No 1099/2008 OF THE EUROPEAN PARLIAMENT AND OF THE COUNCIL of 22 October 2008 on energy statistics https://eur-lex.europa.eu/legal-content/EN/TXT/HTML/?uri=CELEX:32008R1099&from=EN"@en
    
    SubClassOf: 
        Gasoline
    
    
Class: MunicipalWaste

    Annotations: 
        <http://purl.obolibrary.org/obo/IAO_0000115> "Wastes produced by households, hospitals and the tertiary sector incinerated at specific installations, on a net calorific value basis."@en,
        <http://purl.obolibrary.org/obo/IAO_0000119> "REGULATION (EC) No 1099/2008 OF THE EUROPEAN PARLIAMENT AND OF THE COUNCIL of 22 October 2008 on energy statistics https://eur-lex.europa.eu/legal-content/EN/TXT/HTML/?uri=CELEX:32008R1099&from=EN"@en
    
    SubClassOf: 
        Waste
    
    
Class: Name

    SubClassOf: 
        Identifier
    
    
Class: NaturalGas

    Annotations: 
        <http://purl.obolibrary.org/obo/IAO_0000115> "This data collection applies to natural gas, which comprises gases occurring in underground deposits, whether liquefied or gaseous, consisting mainly of methane.

It includes both ‘non-associated’ gas originating from fields producing hydrocarbons only in gaseous form, and ‘associated’ gas produced in association with crude oil as well as methane recovered from coal mines (colliery gas) or from coal seams (coal seam gas).

It does not include gases created by anaerobic digestion of biomass (e.g. municipal or sewage gas) nor gasworks gas."@en,
        <http://purl.obolibrary.org/obo/IAO_0000119> "REGULATION (EC) No 1099/2008 OF THE EUROPEAN PARLIAMENT AND OF THE COUNCIL of 22 October 2008 on energy statistics https://eur-lex.europa.eu/legal-content/EN/TXT/HTML/?uri=CELEX:32008R1099&from=EN"@en
    
    SubClassOf: 
        Fuel,
        has_normal_state_of_matter value gaseous
    
    
Class: NaturalGasGenerator

    Annotations: 
        <http://purl.obolibrary.org/obo/IAO_0000115> "A natural gas electricity generator technology uses natural gas to generate electricity."@en
    
    SubClassOf: 
        FossilGeneratorTechnology
    
    
Class: NetworkNode

    Annotations: 
        <http://purl.obolibrary.org/obo/IAO_0000115> "A network node is a node in an electrical grid."@en
    
    SubClassOf: 
        Node
    
    
Class: NewPowerFromPhotovoltaics

    Annotations: 
        <http://purl.obolibrary.org/obo/IAO_0000115> "A new power from photovoltaics quantity is a quantity that describes the amount of power from photovoltaic power plants that are going to be build in the future."@en
    
    SubClassOf: 
        Quantity
    
    
Class: Node

    SubClassOf: 
        <http://purl.obolibrary.org/obo/BFO_0000024>
    
    DisjointWith: 
        Link
    
    
Class: NonAssociatedGas

    Annotations: 
        <http://purl.obolibrary.org/obo/IAO_0000115> "Natural gas originating from fields producing hydrocarbons only in gaseous form.",
        <http://purl.obolibrary.org/obo/IAO_0000119> "REGULATION (EC) No 1099/2008 OF THE EUROPEAN PARLIAMENT AND OF THE COUNCIL of 22 October 2008 on energy statistics https://eur-lex.europa.eu/legal-content/EN/TXT/HTML/?uri=CELEX:32008R1099&from=EN"
    
    SubClassOf: 
        NaturalGas
    
    
Class: NonMethaneVolatileOrganicCompound

    Annotations: 
        <http://purl.obolibrary.org/obo/IAO_0000115> "Non-methane volatile organic compounds (NMVOCs) are a large variety of chemically different compounds, such as benzene, ethanol, formaldehyde, cyclohexane, 1,1,1-trichloroethane or acetone.
       Essentially, NMVOCs are identical to volatile organic compounds (VOCs), but with methane excluded. An important subset of NMVOCs are the non-methane hydrocarbons (NMHCs). Methane is excluded in air-pollution contexts because it is not harmful. Its low reactivity and thus long lifetime in the atmosphere, however, makes it an important greenhouse gas."@en,
        <http://purl.obolibrary.org/obo/IAO_0000119> "https://en.wikipedia.org/w/index.php?title=Non-methane_volatile_organic_compound&oldid=890812257"@en
    
    SubClassOf: 
        VolatileOrganicCompound
    
    
Class: NonRenewableMunicipalWaste

    Annotations: 
        <http://purl.obolibrary.org/obo/IAO_0000115> "The portion of municipal waste which is of non-biological origin."@en,
        <http://purl.obolibrary.org/obo/IAO_0000119> "REGULATION (EC) No 1099/2008 OF THE EUROPEAN PARLIAMENT AND OF THE COUNCIL of 22 October 2008 on energy statistics https://eur-lex.europa.eu/legal-content/EN/TXT/HTML/?uri=CELEX:32008R1099&from=EN"@en
    
    SubClassOf: 
        MunicipalWaste
    
    
Class: Nuclear

    Annotations: 
        <http://purl.obolibrary.org/obo/IAO_0000115> "Nuclear power is the use of nuclear reactions that release nuclear energy to generate heat, which most frequently is then used in steam turbines to produce electricity in a nuclear power plant. Nuclear power can be obtained from nuclear fission, nuclear decay and nuclear fusion. Presently, the vast majority of electricity from nuclear power is produced by nuclear fission of elements in the actinide series of the periodic table. Nuclear decay processes are used in niche applications such as radioisotope thermoelectric generators. The possibility of generating electricity from nuclear fusion is still at a research phase with no commercial applications. This article mostly deals with nuclear fission power for electricity generation."@en,
        <http://purl.obolibrary.org/obo/IAO_0000119> "https://en.wikipedia.org/w/index.php?title=Nuclear_power&oldid=868476098"@en
    
    SubClassOf: 
        EnergyCarrier
    
    
Class: NuclearPowerGenerator

    Annotations: 
        <http://purl.obolibrary.org/obo/IAO_0000115> "A nuclear generator technology is a fossil electricity generator that uses nuclear reactions to generate electricity."@en
    
    SubClassOf: 
        FossilGeneratorTechnology
    
    
Class: NuclearPowerplant

    Annotations: 
        <http://purl.obolibrary.org/obo/IAO_0000115> "A nuclear power plant or nuclear power station is a thermal power station in which the heat source is a nuclear reactor. As it is typical of thermal power stations, heat is used to generate steam that drives a steam turbine connected to a generator that produces electricity.",
        <http://purl.obolibrary.org/obo/IAO_0000119> "https://en.wikipedia.org/w/index.php?title=Nuclear_power_plant&oldid=867102016"
    
    SubClassOf: 
        ReactivePowerplant,
        has_part some SteamTurbine
    
    
Class: ObjectiveFunction

    SubClassOf: 
        ModelElement
    
    
Class: Ocean

    SubClassOf: 
        Water
    
    DisjointWith: 
        Flow
    
    
Class: OceanPowerplant

    SubClassOf: 
        Generator
    
    
Class: OffShoreWindElectricityGenerator

    Annotations: 
        <http://purl.obolibrary.org/obo/IAO_0000115> "An off shore wind electricity generator is a wind electricity generator that is build off shore above or in the ocean."@en
    
    SubClassOf: 
        WindElectricityGenerator
    
    DisjointWith: 
        OnShoreWindElectricityGenerator
    
    
Class: Office

    SubClassOf: 
        CommericalDemand
    
    
Class: OilAndPetroleumProducts

    Annotations: 
        <http://purl.obolibrary.org/obo/IAO_0000115> "Petroleum (/pəˈtroʊliəm/) is a naturally occurring, yellowish-black liquid found in geological formations beneath the Earth's surface. It is commonly refined into various types of fuels. Components of petroleum are separated using a technique called fractional distillation, i.e. separation of a liquid mixture into fractions differing in boiling point by means of distillation, typically using a fractionating column.

It consists of hydrocarbons of various molecular weights and other organic compounds. The name petroleum covers both naturally occurring unprocessed crude oil and petroleum products that are made up of refined crude oil. A fossil fuel, petroleum is formed when large quantities of dead organisms, mostly zooplankton and algae, are buried underneath sedimentary rock and subjected to both intense heat and pressure."@en,
        <http://purl.obolibrary.org/obo/IAO_0000119> "https://en.wikipedia.org/w/index.php?title=Petroleum&oldid=868006507"@en
    
    SubClassOf: 
        Fuel
    
    
Class: OilElectricityGenerator

    Annotations: 
        <http://purl.obolibrary.org/obo/IAO_0000115> "A oil electricity generator technology uses oil to generate electricity."@en
    
    SubClassOf: 
        FossilGeneratorTechnology
    
    
Class: OilPowerplant

    SubClassOf: 
        FossilePowerplant,
        has_part some SteamTurbine
    
    
Class: OnShoreWindElectricityGenerator

    Annotations: 
        <http://purl.obolibrary.org/obo/IAO_0000115> "An on shore wind electricity generator is a wind electricity generator that is build on land."@en
    
    SubClassOf: 
        WindElectricityGenerator
    
    DisjointWith: 
        OffShoreWindElectricityGenerator
    
    
Class: OpenSource

    SubClassOf: 
        DataDescriptor,
        SoftwareDescriptor
    
    DisjointWith: 
        DataFormat
    
    
Class: Optimization

    Annotations: 
        <http://purl.obolibrary.org/obo/IAO_0000115> "An optimization is a model calculation with the goal to find a best choice or result for at least one variable or function in the model."@en
    
    SubClassOf: 
        ModelCalculation
    
    DisjointWith: 
        Simulation
    
    
Class: OptimizationModel

    Annotations: 
        <http://purl.obolibrary.org/obo/IAO_0000115> "An optimization model is a model that optimizes a target function."@en
    
    SubClassOf: 
        Model
    
    
Class: Organization

    Annotations: 
        <http://purl.obolibrary.org/obo/IAO_0000115> "An organization is a structure with multiple people that has a collective goal."@en
    
    SubClassOf: 
        <http://purl.obolibrary.org/obo/BFO_0000031>
    
    DisjointWith: 
        Person
    
    
Class: OtherBituminousCoal

    Annotations: 
        <http://purl.obolibrary.org/obo/IAO_0000115> "Coal used for steam raising purposes and includes all bituminous coal that is neither included under coking coal nor anthracite. It is characterised by higher volatile matter than anthracite (more than 10 %) and lower carbon content (less than 90 % fixed carbon). Its gross calorific value is greater than 23 865 kJ/kg (5 700 kcal/kg) on an ash-free but moist basis. If bituminous coal is used in coke ovens it should be reported as coking coal."@en,
        <http://purl.obolibrary.org/obo/IAO_0000119> "REGULATION (EC) No 1099/2008 OF THE EUROPEAN PARLIAMENT AND OF THE COUNCIL of 22 October 2008 on energy statistics https://eur-lex.europa.eu/legal-content/EN/TXT/HTML/?uri=CELEX:32008R1099&from=EN"@en,
        rdfs:label "OtherBituminousCoal"@en,
        rdfs:label "SteamCoal"@en
    
    SubClassOf: 
        HardCoal
    
    
Class: OtherKerosene

    Annotations: 
        <http://purl.obolibrary.org/obo/IAO_0000115> "REGULATION (EC) No 1099/2008 OF THE EUROPEAN PARLIAMENT AND OF THE COUNCIL of 22 October 2008 on energy statistics https://eur-lex.europa.eu/legal-content/EN/TXT/HTML/?uri=CELEX:32008R1099&from=EN"@en,
        <http://purl.obolibrary.org/obo/IAO_0000115> "Refined petroleum distillate used in sectors other than aircraft transport. It distils between 150 °C and 300 °C."@en
    
    SubClassOf: 
        Kerosene
    
    
Class: OtherLiquidBiofuels

    Annotations: 
        <http://purl.obolibrary.org/obo/IAO_0000119> "Liquid biofuels, used directly as fuel, not included in biogasoline or bio-diesels."@en,
        <http://purl.obolibrary.org/obo/IAO_0000119> "REGULATION (EC) No 1099/2008 OF THE EUROPEAN PARLIAMENT AND OF THE COUNCIL of 22 October 2008 on energy statistics https://eur-lex.europa.eu/legal-content/EN/TXT/HTML/?uri=CELEX:32008R1099&from=EN"@en
    
    SubClassOf: 
        LiquidBiofuel
    
    
Class: PFC

    Annotations: 
        <http://purl.obolibrary.org/obo/IAO_0000115> "Fluorocarbons, sometimes referred to as perfluorocarbons or PFCs, are, strictly speaking, organofluorine compounds with the formula CxFy, i.e. they contain only carbon and fluorine, though the terminology is not strictly followed. Compounds with the prefix perfluoro- are hydrocarbons, including those with heteroatoms, wherein all C-H bonds have been replaced by C-F bonds."@en,
        <http://purl.obolibrary.org/obo/IAO_0000119> "https://en.wikipedia.org/w/index.php?title=Fluorocarbon&oldid=881053361"@en
    
    EquivalentTo: 
        Perfluorocarbon
    
    SubClassOf: 
        FlourinatedGas
    
    
Class: PVPanel

    Annotations: 
        <http://purl.obolibrary.org/obo/IAO_0000115> "hotovoltaic solar panels absorb sunlight as a source of energy to generate electricity. A photovoltaic (PV) module is a packaged, connected assembly of typically 6x10 photovoltaic solar cells. Photovoltaic modules constitute the photovoltaic array of a photovoltaic system that generates and supplies solar electricity in commercial and residential applications."@en,
        <http://purl.obolibrary.org/obo/IAO_0000119> "https://en.wikipedia.org/w/index.php?title=Solar_panel&oldid=906976047"@en
    
    SubClassOf: 
        EnergyGeneratorTechnology,
        has_physical_output some Power,
        has_physical_input only SolarPhotovoltaic
    
    
Class: ParticulateMatter

    Annotations: 
        <http://purl.obolibrary.org/obo/IAO_0000115> "Atmospheric aerosol particles – also known as atmospheric particulate matter, particulate matter (PM), particulates, or suspended particulate matter (SPM) – are microscopic solid or liquid matter suspended in the atmosphere of Earth. The term aerosol commonly refers to the particulate/air mixture, as opposed to the particulate matter alone.Sources of particulate matter can be natural or anthropogenic.They have impacts on climate and precipitation that adversely affect human health, in addition to direct inhalation. "@en,
        <http://purl.obolibrary.org/obo/IAO_0000119> "https://en.wikipedia.org/w/index.php?title=Particulates&oldid=906795232"@en
    
    SubClassOf: 
        AirPollutant
    
    
Class: Peat

    Annotations: 
        <http://purl.obolibrary.org/obo/IAO_0000115> "A combustible soft, porous or compressed, sedimentary deposit of plant origin with high water content (up to 90 % in the raw state), easily cut, of light to dark brown colour. Peat used for non-energy purposes is not included.

This definition is without prejudice to the definition of renewable energy sources in Directive 2001/77/EC and to the 2006 IPCC Guidelines for National Greenhouse Gas Inventories."@en,
        <http://purl.obolibrary.org/obo/IAO_0000119> "REGULATION (EC) No 1099/2008 OF THE EUROPEAN PARLIAMENT AND OF THE COUNCIL of 22 October 2008 on energy statistics https://eur-lex.europa.eu/legal-content/EN/TXT/HTML/?uri=CELEX:32008R1099&from=EN"@en
    
    SubClassOf: 
        SolidFossilFuels,
        has_normal_state_of_matter value solid
    
    
Class: Percentage

    Annotations: 
        <http://purl.obolibrary.org/obo/IAO_0000115> "A percentage is a ratio given as a fraction of 100."@en
    
    SubClassOf: 
        Quantity
    
    
Class: Perfluorocarbon

    Annotations: 
        <http://purl.obolibrary.org/obo/IAO_0000115> "Fluorocarbons, sometimes referred to as perfluorocarbons or PFCs, are, strictly speaking, organofluorine compounds with the formula CxFy, i.e. they contain only carbon and fluorine, though the terminology is not strictly followed. Compounds with the prefix perfluoro- are hydrocarbons, including those with heteroatoms, wherein all C-H bonds have been replaced by C-F bonds."@en,
        <http://purl.obolibrary.org/obo/IAO_0000119> "https://en.wikipedia.org/w/index.php?title=Fluorocarbon&oldid=881053361"@en
    
    EquivalentTo: 
        PFC
    
    SubClassOf: 
        FlourinatedGas
    
    
Class: Person

    Annotations: 
        <http://purl.obolibrary.org/obo/IAO_0000115> "A person is a human beeing."@en
    
    SubClassOf: 
        <http://purl.obolibrary.org/obo/BFO_0000030>
    
    DisjointWith: 
        Organization
    
    
Class: Phone

    SubClassOf: 
        Contact
    
    
Class: PhotovoltaicElectricityGenerator

    Annotations: 
        <http://purl.obolibrary.org/obo/IAO_0000115> "A photovoltaic electricity generator is a renewable energy generator that uses power from the sun to generate electricity."@en
    
    SubClassOf: 
        RenewableGeneratorTechnology
    
    
Class: PhotovoltaicGenerator

    SubClassOf: 
        Generator,
        uses some SolarEnergy
    
    
Class: PhotovoltaicPowerplant

    Annotations: 
        <http://purl.obolibrary.org/obo/IAO_0000115> "A photovoltaic generator uses PVPanels and solar energy to generate electricity."@en
    
    SubClassOf: 
        SolarPowerPlant,
        has_part some PVPanel
    
    
Class: PlantOperation

    SubClassOf: 
        CommonParameters
    
    
Class: Plot

    SubClassOf: 
        DataFormat
    
    DisjointWith: 
        Database
    
    
Class: Plotting

    SubClassOf: 
        DataProcessing
    
    
Class: PoliticalAssumption

    Annotations: 
        <http://purl.obolibrary.org/obo/IAO_0000115> "A political assumption is an assumption about political measures taken."@en
    
    SubClassOf: 
        Assumption
    
    
Class: PoliticalParty

    Annotations: 
        <http://purl.obolibrary.org/obo/IAO_0000115> "A political party is a organization of a group of people with common views or goals that wants to have influence in politics."@en
    
    SubClassOf: 
        Organization
    
    
Class: Pollutant

    Annotations: 
        <http://purl.obolibrary.org/obo/IAO_0000115> "A pollutant is a substance or energy introduced into the environment that has undesired effects, or adversely affects the usefulness of a resource. A pollutant may cause long- or short-term damage by changing the growth rate of plant or animal species, or by interfering with human amenities, comfort, health, or property values."@en,
        <http://purl.obolibrary.org/obo/IAO_0000119> "https://en.wikipedia.org/w/index.php?title=Pollutant&oldid=906519011"@en
    
    SubClassOf: 
        <http://purl.obolibrary.org/obo/BFO_0000016>
    
    
Class: Postprocessing

    Annotations: 
        <http://purl.obolibrary.org/obo/IAO_0000115> "Postprocessing is a transformation that transforms the output of a model calculation into a form that is suitable for presentation."@en
    
    SubClassOf: 
        Transformation
    
    
Class: Power

    Annotations: 
        <http://purl.obolibrary.org/obo/IAO_0000115> "Power is the rate of doing work, the amount of energy transferred per unit time.
Source: https://en.wikipedia.org/wiki/Power_(physics)"@en
    
    SubClassOf: 
        Quantity
    
    
Class: PowerGeneratingUnit

    SubClassOf: 
        NetworkNode,
        uses some EnergyGeneratorTechnology,
        uses some EnergyStorageTechnology,
        uses some EnergyTransferTechnology
    
    
Class: PowerPlantData

    SubClassOf: 
        CommonParameters
    
    
Class: PowerToGas

    Annotations: 
        <http://purl.obolibrary.org/obo/IAO_0000115> "Power-to-gas (often abbreviated P2G) is a technology that converts electrical power to a gas fuel. When using surplus power from wind generation, the concept is sometimes called windgas. There are currently three methods in use; all use electricity to split water into hydrogen and oxygen by means of electrolysis."@en,
        <http://purl.obolibrary.org/obo/IAO_0000119> "https://en.wikipedia.org/w/index.php?title=Power-to-gas&oldid=907220452"@en
    
    SubClassOf: 
        EnergyStorageTechnology
    
    
Class: PowerUnit

    Annotations: 
        <http://purl.obolibrary.org/obo/IAO_0000115> "A power unit is a unit of measurement used to express the rate of doing work, the amount of energy transferred per unit time."@en
    
    SubClassOf: 
        UnitOfMeasurement
    
    
Class: Preprocessing

    Annotations: 
        <http://purl.obolibrary.org/obo/IAO_0000115> "Preprocessing is a transformation that transforms the input into a form that is useable for a model calculation."@en
    
    SubClassOf: 
        Transformation
    
    
Class: PrimaryOutputs

    SubClassOf: 
        ContentDescriptor
    
    
Class: PrimaryPurpose

    SubClassOf: 
        ContentDescriptor
    
    
Class: Private

    SubClassOf: 
        Funding
    
    
Class: ProgramParameter

    Annotations: 
        <http://purl.obolibrary.org/obo/IAO_0000112> "Settings for a random number generator."@en,
        <http://purl.obolibrary.org/obo/IAO_0000115> "A program parameter is a variable that influences the output of  a calculation in the program but has no meaning outside of the program."@en
    
    SubClassOf: 
        ModelElement
    
    
Class: Project

    SubClassOf: 
        Reference
    
    
Class: Prosumer

    Annotations: 
        <http://purl.obolibrary.org/obo/IAO_0000115> "A prosumer is a person who consumes and produces a product. It is derived from \"prosumption\", a dot-com era business term meaning \"production by consumers\"."@en,
        <http://purl.obolibrary.org/obo/IAO_0000119> "https://en.wikipedia.org/w/index.php?title=Prosumer&oldid=881861680"@en
    
    SubClassOf: 
        Agent
    
    
Class: Public

    SubClassOf: 
        Funding
    
    
Class: Publication

    Annotations: 
        <http://purl.obolibrary.org/obo/IAO_0000115> "A publication is a collection of information artifacts that has been published."@en
    
    SubClassOf: 
        Reference
    
    
Class: PumpedStorage

    Annotations: 
        <http://purl.obolibrary.org/obo/IAO_0000115> "A pumped storage (pumped-storage hdyroelectricity) uses water from a higher reservoir to generate energy"@en
    
    SubClassOf: 
        EnergyStorageTechnology,
        is_used_by some StorageUnit
    
    
Class: PumpedStoragePlant

    Annotations: 
        <http://purl.obolibrary.org/obo/IAO_0000115> "A pumped storage plant pumps water using surplus energy from a lower level to a higher reservoir. The reservoir functions as a storage unit. If needed, energy can be generated by letting the water flow back to the lower level"@en
    
    SubClassOf: 
        HydroelectricPowerplant
    
    
Class: PumpedWater

    Annotations: 
        <http://purl.obolibrary.org/obo/IAO_0000115> "energy in the form of gravitational potential energy of water, pumped from a lower elevation reservoir to a higher elevation"@en,
        <http://purl.obolibrary.org/obo/IAO_0000119> "https://en.wikipedia.org/w/index.php?title=Pumped-storage_hydroelectricity&oldid=906590319"@en
    
    SubClassOf: 
        Hydroelectricity,
        is_used_by some StorageUnit
    
    
Class: PumpstoragePowerplant

    SubClassOf: 
        ReservoirPowerplant
    
    
Class: PumpstoragePowerplantWithNaturalInflux

    SubClassOf: 
        ReservoirPowerplant
    
    
Class: Quality

    SubClassOf: 
        SoftwareDescriptor
    
    
Class: Quantity

    Annotations: 
        <http://purl.obolibrary.org/obo/IAO_0000115> "Idea: A quantity is a property that is quantifiable by measurement."@en,
        <http://purl.obolibrary.org/obo/IAO_0000115> "Other Idea: A number together with a unit of measurement to quantify an entity."@en
    
    SubClassOf: 
        <http://purl.obolibrary.org/obo/BFO_0000031>
    
    
Class: Rail

    SubClassOf: 
        TransportDemand
    
    
Class: ReactivePowerplant

    SubClassOf: 
        PowerGeneratingUnit,
        has_part some Turbine
    
    
Class: Reference

    SubClassOf: 
        InformationArtifact
    
    
Class: RegenerativePowerplant

    SubClassOf: 
        PowerGeneratingUnit,
        has_part some WindTurbine
    
    
Class: RegulationAssumption

    Annotations: 
        <http://purl.obolibrary.org/obo/IAO_0000115> "A regulation assumption is an assumption about political regulations and prohibitions."@en
    
    SubClassOf: 
        PoliticalAssumption
    
    DisjointWith: 
        SubsidyAssumption
    
    
Class: RenewableGeneratorTechnology

    Annotations: 
        <http://purl.obolibrary.org/obo/IAO_0000115> "A renewable electricity generator technology is an electricity generator techonolgy that uses resources that are practically unlimited or regenerate quickly to generate electricity."@en
    
    SubClassOf: 
        ElectricityGeneratorTechnology
    
    DisjointWith: 
        FossilGeneratorTechnology
    
    
Class: RenewableMunicipalWaste

    Annotations: 
        <http://purl.obolibrary.org/obo/IAO_0000115> "The portion of municipal waste which is of biological origin."@en,
        <http://purl.obolibrary.org/obo/IAO_0000119> "REGULATION (EC) No 1099/2008 OF THE EUROPEAN PARLIAMENT AND OF THE COUNCIL of 22 October 2008 on energy statistics https://eur-lex.europa.eu/legal-content/EN/TXT/HTML/?uri=CELEX:32008R1099&from=EN"@en
    
    SubClassOf: 
        Biofuel,
        MunicipalWaste
    
    
Class: RequierementSwitchOffAnimalProtection

    SubClassOf: 
        Requierements
    
    
Class: RequierementSwitchOffCapacityLimitation

    SubClassOf: 
        Requierements
    
    
Class: RequierementSwitchOffIceFalling

    SubClassOf: 
        Requierements
    
    
Class: RequierementSwitchOffNoiseImmissionProtectionByDay

    SubClassOf: 
        Requierements
    
    
Class: RequierementSwitchOffNoiseImmissionProtectionNights

    SubClassOf: 
        Requierements
    
    
Class: RequierementSwitchOffOthers

    SubClassOf: 
        Requierements
    
    
Class: RequierementSwitchOffShadowing

    SubClassOf: 
        Requierements
    
    
Class: Requierements

    SubClassOf: 
        WindEntityData
    
    
Class: ReservoirPowerplant

    SubClassOf: 
        HydroPowerplant
    
    DisjointWith: 
        RunOfRiverPowerplant
    
    
Class: ResidentialDemand

    SubClassOf: 
        Demand
    
    
Class: ResistanceUnit

    Annotations: 
        <http://purl.obolibrary.org/obo/IAO_0000115> "A resistance unit is a unit of measurement used to express difficulty to pass an electric current through a conductor."@en
    
    SubClassOf: 
        UnitOfMeasurement
    
    
Class: Retail

    SubClassOf: 
        CommericalDemand
    
    
Class: Robustness

    SubClassOf: 
        Validation
    
    
Class: RooftopPhotovoltaicGenerator

    Annotations: 
        <http://purl.obolibrary.org/obo/IAO_0000115> "A rooftop photovoltaic electricity generator is a photovoltaic electricity generator that is installed on top of the roof of a building."@en
    
    SubClassOf: 
        PhotovoltaicElectricityGenerator
    
    DisjointWith: 
        FieldPhotovoltaicGenerator
    
    
Class: RotorBladeDeIcingSystem

    SubClassOf: 
        TechnicalDataWind
    
    
Class: RotorDiameter

    SubClassOf: 
        TechnicalDataWind
    
    
Class: RunOfRiverElectricityGenerator

    Annotations: 
        <http://purl.obolibrary.org/obo/IAO_0000115> "A run of river electricity generator is a water energy generator that stores little or no water and produces electricity."@en
    
    SubClassOf: 
        WaterElectricityGenerator
    
    
Class: RunOfRiverPowerplant

    Annotations: 
        <http://purl.obolibrary.org/obo/IAO_0000115> "water turbine installed on naturally running streams (in contrast to pump storage lakes)"@en
    
    SubClassOf: 
        HydroelectricPowerplant,
        uses some Flow
    
    DisjointWith: 
        ReservoirPowerplant, TidalPowerPlant
    
    
Class: Scenario

    Annotations: 
        <http://purl.obolibrary.org/obo/IAO_0000115> "(WIP) A scenario is a collection of assumptions about the energy system.
There is not yet a consens about the definition."@en
    
    SubClassOf: 
        SoftwareElement
    
    
Class: ScenarioFactsheet

    SubClassOf: 
        Factsheet
    
    
Class: SeaRegion

    SubClassOf: 
        <http://purl.obolibrary.org/obo/BFO_0000028>
    
    
Class: Sector

    Annotations: 
        <http://purl.obolibrary.org/obo/IAO_0000115> "A sector is a subdivision in an economic system."@en
    
    SubClassOf: 
        <http://purl.obolibrary.org/obo/BFO_0000027>
    
    
Class: SectorConcept

    Annotations: 
        <http://purl.obolibrary.org/obo/IAO_0000115> "A sector concept contains concepts of possible sectors."@en
    
    SubClassOf: 
        <http://purl.obolibrary.org/obo/BFO_0000031>
    
    
Class: ShuntImpedance

    Annotations: 
        <http://purl.obolibrary.org/obo/IAO_0000115> "In electronics, a shunt is a device which allows electric current to pass around another point in the circuit by creating a low resistance path. The term is also widely used in photovoltaics to describe an unwanted short circuit between the front and back surface contacts of a solar cell, usually caused by wafer damage.

Source: https://en.wikipedia.org/wiki/Shunt_%28electrical%29"@en
    
    SubClassOf: 
        NetworkNode
    
    
Class: Simulation

    Annotations: 
        <http://purl.obolibrary.org/obo/IAO_0000115> "A simulation is a model calculation that simulates a process or system behavior from the real world."@en
    
    SubClassOf: 
        ModelCalculation
    
    DisjointWith: 
        Optimization
    
    
Class: SimulationModel

    Annotations: 
        <http://purl.obolibrary.org/obo/IAO_0000115> "A simultaion model is a model that simulates the behaviour of a system without a target function."@en
    
    SubClassOf: 
        Model
    
    
Class: SingleNodeModel

    SubClassOf: 
        GridModel
    
    
Class: Social

    SubClassOf: 
        Type
    
    
Class: Sodium-IonBattery

    Annotations: 
        <http://purl.obolibrary.org/obo/IAO_0000115> "Sodium-ion batteries (SIB) are a type of rechargeable metal-ion battery that uses sodium ions as charge carriers."@en,
        <http://purl.obolibrary.org/obo/IAO_0000119> "https://en.wikipedia.org/w/index.php?title=Sodium-ion_battery&oldid=906459441"@en
    
    SubClassOf: 
        Battery
    
    
Class: Sodium-SulfurBattery

    Annotations: 
        <http://purl.obolibrary.org/obo/IAO_0000115> "A sodium–sulfur battery is a type of molten-salt battery constructed from liquid sodium (Na) and sulfur (S).This type of battery has a high energy density, high efficiency of charge/discharge and long cycle life, and is fabricated from inexpensive materials. The operating temperatures of 300 to 350 °C and the highly corrosive nature of the sodium polysulfides, primarily make them suitable for stationary energy storage applications. The cell becomes more economical with increasing size."@en,
        <http://purl.obolibrary.org/obo/IAO_0000119> "https://en.wikipedia.org/w/index.php?title=Sodium%E2%80%93sulfur_battery&oldid=900392594"@en
    
    SubClassOf: 
        MoltenStateBattery
    
    
Class: Software

    Annotations: 
        <http://purl.obolibrary.org/obo/IAO_0000115> "A collection of information artifacts that tell a computer how to work."@en
    
    SubClassOf: 
        ModelingTechnology
    
    
Class: SoftwareDescriptor

    SubClassOf: 
        InformationArtifact
    
    
Class: SoftwareElement

    Annotations: 
        <http://purl.obolibrary.org/obo/IAO_0000115> "A model component is a part of a model."@en
    
    SubClassOf: 
        Software
    
    
Class: SoftwareMaintenance

    SubClassOf: 
        InformationArtifact
    
    
Class: Solar

    Annotations: 
        <http://purl.obolibrary.org/obo/IAO_0000115> "Solar radiation exploited for hot water production and electricity generation. This energy production is the heat available to the heat transfer medium, i.e. the incident solar energy less the optical and collectors' losses. Passive solar energy for the direct heating, cooling and lighting of dwellings or other buildings is not included."@en,
        <http://purl.obolibrary.org/obo/IAO_0000119> "REGULATION (EC) No 1099/2008 OF THE EUROPEAN PARLIAMENT AND OF THE COUNCIL of 22 October 2008 on energy statistics https://eur-lex.europa.eu/legal-content/EN/TXT/HTML/?uri=CELEX:32008R1099&from=EN"@en
    
    SubClassOf: 
        EnergyCarrier
    
    
Class: SolarEnergy

    Annotations: 
        <http://purl.obolibrary.org/obo/IAO_0000115> "Solar radiation exploited for hot water production and electricity generation. This energy production is the heat available to the heat transfer medium, i.e. the incident solar energy less the optical and collectors' losses. Passive solar energy for the direct heating, cooling and lighting of dwellings or other buildings is not included."@en,
        <http://purl.obolibrary.org/obo/IAO_0000119> "REGULATION (EC) No 1099/2008 OF THE EUROPEAN PARLIAMENT AND OF THE COUNCIL of 22 October 2008 on energy statistics https://eur-lex.europa.eu/legal-content/EN/TXT/HTML/?uri=CELEX:32008R1099&from=EN"@en
    
    SubClassOf: 
        EnergyCarrier
    
    
Class: SolarPhotovoltaic

    Annotations: 
        <http://purl.obolibrary.org/obo/IAO_0000115> "Sunlight converted into electricity by the use of solar cells usually made of semi-conducting material which exposed to light will generate electricity."@en,
        <http://purl.obolibrary.org/obo/IAO_0000119> "REGULATION (EC) No 1099/2008 OF THE EUROPEAN PARLIAMENT AND OF THE COUNCIL of 22 October 2008 on energy statistics https://eur-lex.europa.eu/legal-content/EN/TXT/HTML/?uri=CELEX:32008R1099&from=EN"@en
    
    SubClassOf: 
        Solar
    
    
Class: SolarPowerPlant

    Annotations: 
        <http://purl.obolibrary.org/obo/IAO_0000115> "Solar power is the conversion of energy from sunlight into electricity, either directly using photovoltaics (PV), indirectly using concentrated solar power, or a combination. Concentrated solar power systems use lenses or mirrors and tracking systems to focus a large area of sunlight into a small beam. Photovoltaic cells convert light into an electric current using the photovoltaic effect."@en,
        <http://purl.obolibrary.org/obo/IAO_0000119> "https://en.wikipedia.org/w/index.php?title=Solar_power&oldid=904827092"@en
    
    SubClassOf: 
        PowerGeneratingUnit,
        Turbine or (has_part some PVPanel)
    
    
Class: SolarThermal

    Annotations: 
        <http://purl.obolibrary.org/obo/IAO_0000115> "Heat from solar radiation; can consist of:
(a) solar thermal-electric plants; or
(b) equipment for the production of domestic hot water or for the seasonal heating of swimming pools (e.g. flat plate collectors, mainly of the thermosyphon type)."@en,
        <http://purl.obolibrary.org/obo/IAO_0000119> "REGULATION (EC) No 1099/2008 OF THE EUROPEAN PARLIAMENT AND OF THE COUNCIL of 22 October 2008 on energy statistics https://eur-lex.europa.eu/legal-content/EN/TXT/HTML/?uri=CELEX:32008R1099&from=EN"@en
    
    SubClassOf: 
        Heat
    
    
Class: SolarThermalCollector

    Annotations: 
        <http://purl.obolibrary.org/obo/IAO_0000115> "A solar thermal collector collects heat by absorbing sunlight. The term \"solar collector\" commonly refers to a device for solar hot water heating, but may refer to large power generating installations such as solar parabolic troughs and solar towers or non water heating devices such as solar air heaters."@en,
        <http://purl.obolibrary.org/obo/IAO_0000119> "https://en.wikipedia.org/w/index.php?title=Solar_thermal_collector&oldid=903948846"@en
    
    SubClassOf: 
        EnergyGeneratorTechnology,
        has_physical_output some Power,
        has_physical_input only SolarThermal
    
    
Class: SolarThermalHeatGenerator

    Annotations: 
        <http://purl.obolibrary.org/obo/IAO_0000115> "A solar thermal heat generator is a heat generator that uses solar power to produce heat."@en
    
    SubClassOf: 
        HeatGeneratorTechnology
    
    
Class: SolarThermalPowerplant

    Annotations: 
        <http://purl.obolibrary.org/obo/IAO_0000115> "uses solar thermal energy to generate electrical energy"@en
    
    SubClassOf: 
        SolarPowerPlant,
        has_part some SteamTurbine
    
    
Class: Solid

    Annotations: 
        <http://purl.obolibrary.org/obo/IAO_0000115> "Solid is one of the four fundamental states of matter (the others being liquid, gas, and plasma). In solids particles are closely packed. It is characterized by structural rigidity and resistance to changes of shape or volume."@en,
        <http://purl.obolibrary.org/obo/IAO_0000119> "https://en.wikipedia.org/w/index.php?title=Solid&oldid=906779814"
    
    SubClassOf: 
        StateOfMatter
    
    
Class: SolidBiomass

    Annotations: 
        <http://purl.obolibrary.org/obo/IAO_0000115> "Covers organic, non-fossil material of biological origin which may be used as fuel for heat production or electricity generation.",
        <http://purl.obolibrary.org/obo/IAO_0000119> "https://eur-lex.europa.eu/legal-content/EN/TXT/HTML/?uri=CELEX:32008R1099&from=EN",
        rdfs:label "SolidBiofuel"@en,
        rdfs:label "SolidBiomass"@en
    
    SubClassOf: 
        Biofuel,
        has_normal_state_of_matter value solid
    
    
Class: SolidFossilFuels

    Annotations: 
        <http://purl.obolibrary.org/obo/IAO_0000115> "Coal is a combustible black or brownish-black sedimentary rock usually occurring in rock strata in layers or veins called coal beds or coal seams. The harder forms, such as anthracite coal, can be regarded as metamorphic rock because of later exposure to elevated temperature and pressure. Coal is composed primarily of carbon, along with variable quantities of other elements, chiefly hydrogen, sulfur, oxygen, and nitrogen.[1] Coal is a fossil fuel that forms when dead plant matter is converted into peat, which in turn is converted into lignite, then sub-bituminous coal, after that bituminous coal, and lastly anthracite. This involves biological and geological processes. The geological processes take place over millions of years."@en,
        <http://purl.obolibrary.org/obo/IAO_0000119> "https://en.wikipedia.org/w/index.php?title=Coal&oldid=868515262"@en
    
    SubClassOf: 
        Fuel
    
    
Class: Solver

    SubClassOf: 
        SoftwareElement
    
    
Class: StateOfMatter

    Annotations: 
        <http://purl.obolibrary.org/obo/IAO_0000115> "In physics, a state of matter is one of the distinct forms in which matter can exist. Four states of matter are observable in everyday life: solid, liquid, gas, and plasma. Many intermediate states are known to exist, such as liquid crystal, and some states only exist under extreme conditions"@en,
        <http://purl.obolibrary.org/obo/IAO_0000119> "https://en.wikipedia.org/w/index.php?title=State_of_matter&oldid=903680856"
    
    SubClassOf: 
        <http://purl.obolibrary.org/obo/BFO_0000030>
    
    
Class: SteamTurbine

    Annotations: 
        <http://purl.obolibrary.org/obo/IAO_0000115> "A steam turbine is a device that extracts thermal energy from pressurized steam and uses it to do mechanical work on a rotating output shaft.",
        <http://purl.obolibrary.org/obo/IAO_0000119> "https://en.wikipedia.org/w/index.php?title=Steam_turbine&oldid=906022336"
    
    SubClassOf: 
        Turbine,
        (has_physical_input some NaturalGas) or (has_physical_input some Nuclear) or (has_physical_input some OilAndPetroleumProducts) or (has_physical_input some Solar) or (has_physical_input some SolidBiomass) or (has_physical_input some SolidFossilFuels),
        has_physical_output some Power
    
    
Class: StorageHydropowerplant

    SubClassOf: 
        ReservoirPowerplant
    
    
Class: StorageUnit

    Annotations: 
        <http://purl.obolibrary.org/obo/IAO_0000115> "A storage unit is a grid component that stores electrical energy."@en
    
    SubClassOf: 
        ElectricityGridComponent,
        part_of some ElectricityGrid,
        uses some EnergyStorageTechnology
    
    
Class: StorageUnitDataset

    SubClassOf: 
        MaStR
    
    
Class: Study

    SubClassOf: 
        Reference
    
    
Class: SubBituminousCoal

    Annotations: 
        <http://purl.obolibrary.org/obo/IAO_0000115> "Refers to non-agglomerating coal with a gross calorific value between 17 435 kJ/kg (4 165 kcal/kg) and 23 865 kJ/kg (5 700 kcal/kg) containing more than 31 % volatile matter on a dry mineral matter free basis."@en,
        <http://purl.obolibrary.org/obo/IAO_0000119> "REGULATION (EC) No 1099/2008 OF THE EUROPEAN PARLIAMENT AND OF THE COUNCIL of 22 October 2008 on energy statistics https://eur-lex.europa.eu/legal-content/EN/TXT/HTML/?uri=CELEX:32008R1099&from=EN"@en
    
    SubClassOf: 
        Coal
    
    
Class: Subgrid

    Annotations: 
        <http://purl.obolibrary.org/obo/IAO_0000115> "A subgrid is a grid component that is a grid itself."@en
    
    SubClassOf: 
        ElectricityGrid,
        has_part some ElectricityGridComponent,
        part_of some ElectricityGrid
    
    
Class: SubsidyAssumption

    Annotations: 
        <http://purl.obolibrary.org/obo/IAO_0000112> "Public subsidies for energy efficient renovation of private buildings."@en,
        <http://purl.obolibrary.org/obo/IAO_0000115> "A subsidy assumption is an assumption about financial support from the government to an economic sector or certain economic entities."@en
    
    SubClassOf: 
        PoliticalAssumption
    
    DisjointWith: 
        RegulationAssumption
    
    
Class: SuperconductingMagneticEnergy

    Annotations: 
        <http://purl.obolibrary.org/obo/IAO_0000115> "Superconducting magnetic energy storage (SMES) systems store energy in the magnetic field created by the flow of direct current in a superconducting coil which has been cryogenically cooled to a temperature below its superconducting critical temperature.
          A typical SMES system includes three parts: superconducting coil, power conditioning system and cryogenically cooled refrigerator. Once the superconducting coil is charged, the current will not decay and the magnetic energy can be stored indefinitely."@en,
        <http://purl.obolibrary.org/obo/IAO_0000119> "https://en.wikipedia.org/w/index.php?title=Superconducting_magnetic_energy_storage&oldid=902190687"
    
    SubClassOf: 
        EnergyStorageTechnology
    
    
Class: Support

    SubClassOf: 
        SoftwareMaintenance
    
    
Class: SynthethicDataset

    Annotations: 
        <http://purl.obolibrary.org/obo/IAO_0000112> "The projected power usage during an idealized model year."@en,
        <http://purl.obolibrary.org/obo/IAO_0000115> "A synthetic dataset is a dataset that is optained by artificially creating data items. It is constructed to be an estimation of a real world dataset."@en
    
    SubClassOf: 
        Dataset
    
    DisjointWith: 
        EmpiricalDataset
    
    
Class: TCSSector

    Annotations: 
        <http://purl.obolibrary.org/obo/IAO_0000115> "A TCS sector is a demand sector that includes the energy consumption from trade, commerce and services."@en
    
    SubClassOf: 
        DemandSector
    
    
Class: Technical

    SubClassOf: 
        Type
    
    
Class: TechnicalDataWind

    SubClassOf: 
        WindEntityData,
        part_of some WindEntity
    
    
Class: TechnologicalAssumption

    Annotations: 
        <http://purl.obolibrary.org/obo/IAO_0000115> "A technological assumption is an assumption about what kind of technologies are available."@en
    
    SubClassOf: 
        Assumption
    
    
Class: Technology

    Annotations: 
        <http://purl.obolibrary.org/obo/IAO_0000115> "A technology is an entity that is created by mental or phisical efford and used to help society?"@en
    
    SubClassOf: 
        <http://purl.obolibrary.org/obo/BFO_0000030>
    
    
Class: TestDataset

    SubClassOf: 
        Dataset
    
    
Class: Thermal

    Annotations: 
        <http://purl.obolibrary.org/obo/IAO_0000115> "Thermal energy storage (TES) is a technology that stocks thermal energy by heating or cooling a storage medium so that the stored energy can be used at a later time for heating and cooling applications and power generation. TES systems are used particularly in buildings and in industrial processes."@en,
        <http://purl.obolibrary.org/obo/IAO_0000119> "Sarbu, Ioan & Sebarchievici, C. (2018). A Comprehensive Review of Thermal Energy Storage. Sustainability (Switzerland). 10. 10.3390/su10010191. "
    
    SubClassOf: 
        EnergyStorageTechnology
    
    
Class: TidalPowerPlant

    Annotations: 
        <http://purl.obolibrary.org/obo/IAO_0000115> "Mechanical energy derived from tidal movement, wave motion or ocean current and exploited for electricity generation."@en,
        <http://purl.obolibrary.org/obo/IAO_0000119> "REGULATION (EC) No 1099/2008 OF THE EUROPEAN PARLIAMENT AND OF THE COUNCIL of 22 October 2008 on energy statistics https://eur-lex.europa.eu/legal-content/EN/TXT/HTML/?uri=CELEX:32008R1099&from=EN"@en
    
    SubClassOf: 
        OceanPowerplant,
        uses some Tide
    
    DisjointWith: 
        RunOfRiverPowerplant
    
    
Class: TidalStreamGenerator

    Annotations: 
        <http://purl.obolibrary.org/obo/IAO_0000115> "A tidal stream generator uses tidal movement, wave motion or water current for electricity generation."@en
    
    SubClassOf: 
        EnergyGeneratorTechnology,
        has_physical_output some Power,
        has_physical_input only TideWaveOcean
    
    
Class: TidalStreamPowerplant

    Annotations: 
        <http://purl.obolibrary.org/obo/IAO_0000115> "A tidal stream generator uses tidal movement, wave motion or water current for electricity generation."@en
    
    SubClassOf: 
        HydroelectricPowerplant
    
    
Class: Tide

    SubClassOf: 
        Ocean
    
    
Class: TideWaveOcean

    Annotations: 
        <http://purl.obolibrary.org/obo/IAO_0000115> "Mechanical energy derived from tidal movement, wave motion or ocean current and exploited for electricity generation."@en,
        <http://purl.obolibrary.org/obo/IAO_0000119> "REGULATION (EC) No 1099/2008 OF THE EUROPEAN PARLIAMENT AND OF THE COUNCIL of 22 October 2008 on energy statistics https://eur-lex.europa.eu/legal-content/EN/TXT/HTML/?uri=CELEX:32008R1099&from=EN"@en
    
    SubClassOf: 
        Hydropower
    
    
Class: TimeHorizon

    SubClassOf: 
        ModelVariable
    
    
Class: TimeSeries

    SubClassOf: 
        ModelVariable
    
    
Class: TimeStep

    SubClassOf: 
        ModelVariable
    
    
Class: TimeUnit

    Annotations: 
        <http://purl.obolibrary.org/obo/IAO_0000112> "second"@en,
        <http://purl.obolibrary.org/obo/IAO_0000115> "A time unit is a unit of measurement used to express the duration of a process."@en
    
    SubClassOf: 
        UnitOfMeasurement
    
    
Class: Title

    Annotations: 
        <http://purl.obolibrary.org/obo/IAO_0000115> "A titel is a name for a information artifact."@en
    
    SubClassOf: 
        Identifier
    
    
Class: TrafficSector

    Annotations: 
        <http://purl.obolibrary.org/obo/IAO_0000115> "A traffic sector is a demand sector that includes the energy consumption from traffic."@en
    
    SubClassOf: 
        DemandSector
    
    
Class: Transformation

    Annotations: 
        definition "A transformation is a process that transforms one or more inputs into at least one output."@en
    
    SubClassOf: 
        <http://purl.obolibrary.org/obo/BFO_0000015>
    
    
Class: Transformer

    Annotations: 
        <http://purl.obolibrary.org/obo/IAO_0000115> "1. A transformer is an electrical device that transfers electrical energy between two or more circuits through electromagnetic induction. A varying current in one coil of the transformer produces a varying magnetic field, which in turn induces a voltage in a second coil. Transformers are used to increase or decrease the alternating voltages in electric power applications.
2. A transformer is a static machine used for transforming power from one circuit to another without changing frequency. This is a very basic definition of transformer. Since there is no rotating or moving part so transformer is a static device. Transformer operates on ac supply. Transformer works on the principle of mutual induction.

Source: https://wiki.openmod-initiative.org/wiki/Transformer"@en
    
    SubClassOf: 
        NetworkNode
    
    
Class: TranshipmentModel

    SubClassOf: 
        GridModel
    
    
Class: TransportDemand

    SubClassOf: 
        Demand
    
    
Class: TransportSector

    Annotations: 
        <http://purl.obolibrary.org/obo/IAO_0000115> "Consumption in transport covers all transport activity (in mobile engines) regardless of the economic sector to which it is contributing, and is specified as follows:

* Domestic aviation
* Road: fuels used in road vehicles as well as agricultural and industrial highway use
* Rail, including industrial railways.
* Pipeline transport
* Domestic navigation
* Non-specified: includes all transport not elsewhere specified."@en
    
    SubClassOf: 
        Sector
    
    
Class: Turbine

    Annotations: 
        <http://purl.obolibrary.org/obo/IAO_0000115> "A turbine [...] is a rotary mechanical device that extracts energy from a fluid flow and converts it into useful work. The work produced by a turbine can be used for generating electrical power when combined with a generator."@en,
        <http://purl.obolibrary.org/obo/IAO_0000119> "https://en.wikipedia.org/w/index.php?title=Turbine&oldid=905470312"
    
    SubClassOf: 
        EnergyGeneratorTechnology
    
    
Class: Type

    SubClassOf: 
        DataDescriptor
    
    
Class: TypeDescription

    SubClassOf: 
        ManufacturerSpecifications
    
    
Class: Uncertainty

    SubClassOf: 
        Validation
    
    
Class: UndergroundHydrogenStorage

    Annotations: 
        <http://purl.obolibrary.org/obo/IAO_0000115> "Underground hydrogen storage is the practice of hydrogen storage in underground caverns,salt domes and depleted oil/gas fields."@en,
        <http://purl.obolibrary.org/obo/IAO_0000119> "https://en.wikipedia.org/w/index.php?title=Underground_hydrogen_storage&oldid=895350780"
    
    SubClassOf: 
        Hydrogen
    
    
Class: UndirectedEdge

    SubClassOf: 
        Link
    
    
Class: Unit

    SubClassOf: 
        ModelVariable
    
    
Class: UnitOfMeasurement

    Annotations: 
        <http://purl.obolibrary.org/obo/IAO_0000115> "A unit of measurement is a specified magnitude of a quantity that is used to express the magnitude of the same kind of quantity."@en
    
    SubClassOf: 
        <http://purl.obolibrary.org/obo/BFO_0000141>
    
    
Class: User

    SubClassOf: 
        Agent
    
    
Class: UserDocumentation

    SubClassOf: 
        Documentation
    
    
Class: V2Grid

    SubClassOf: 
        TransportDemand
    
    
Class: Validation

    SubClassOf: 
        ModelElement
    
    
Class: VariableOperationCost

    SubClassOf: 
        Cost
    
    
Class: VolatileOrganicCompound

    Annotations: 
        <http://purl.obolibrary.org/obo/IAO_0000115> "Volatile organic compounds (VOCs) are organic chemicals that have a high vapor pressure at ordinary room temperature. Their high vapor pressure results from a low boiling point, which causes large numbers of molecules to evaporate or sublimate from the liquid or solid form of the compound and enter the surrounding air, a trait known as volatility.

[...]

VOCs are numerous, varied, and ubiquitous. They include both human-made and naturally occurring chemical compounds.

[...]

Some VOCs are dangerous to human health or cause harm to the environment."@en,
        <http://purl.obolibrary.org/obo/IAO_0000115> "https://en.wikipedia.org/w/index.php?title=Volatile_organic_compound&oldid=880677383"
    
    SubClassOf: 
        AirPollutant
    
    
Class: VoltageUnit

    Annotations: 
        <http://purl.obolibrary.org/obo/IAO_0000115> "A voltage unit is a unit of measurement used to express the difference in electric potential between two points."@en
    
    SubClassOf: 
        UnitOfMeasurement
    
    
Class: Warehouse

    SubClassOf: 
        CommericalDemand
    
    
Class: Waste

    Annotations: 
        <http://purl.obolibrary.org/obo/IAO_0000115> "Waste (or wastes) are unwanted or unusable materials. Waste is any substance which is discarded after primary use, or is worthless, defective and of no use."@en,
        <http://purl.obolibrary.org/obo/IAO_0000119> "https://en.wikipedia.org/w/index.php?title=Waste&oldid=903993587"
    
    SubClassOf: 
        Fuel
    
    
Class: WastePowerplant

    Annotations: 
        <http://purl.obolibrary.org/obo/IAO_0000115> "A waste-to-energy plant is a waste management facility that combusts wastes to produce electricity. This type of power plant is sometimes called a trash-to-energy, municipal waste incineration, energy recovery, or resource recovery plant."@en,
        <http://purl.obolibrary.org/obo/IAO_0000119> "https://en.wikipedia.org/w/index.php?title=Waste-to-energy_plant&oldid=904634168"
    
    SubClassOf: 
        FossilePowerplant,
        has_part some SteamTurbine
    
    
Class: Water

    SubClassOf: 
        EnergyCarrier
    
    
Class: WaterElectricityGenerator

    Annotations: 
        <http://purl.obolibrary.org/obo/IAO_0000115> "A water electricity generator is a renewable energy generator that uses power from water to generate electricity."@en
    
    SubClassOf: 
        RenewableGeneratorTechnology
    
    
Class: WaterTurbine

    Annotations: 
        <http://purl.obolibrary.org/obo/IAO_0000115> "A water turbine is a rotary machine that converts kinetic energy and potential energy of water into mechanical work."@en,
        <http://purl.obolibrary.org/obo/IAO_0000119> "https://en.wikipedia.org/w/index.php?title=Water_turbine&oldid=902161000"
    
    SubClassOf: 
        Turbine,
        has_physical_output some Power,
        has_physical_input only Hydropower
    
    
Class: Wave

    SubClassOf: 
        Ocean
    
    
Class: WavePowerPlant

    SubClassOf: 
        OceanPowerplant,
        uses some Wave
    
    
Class: Weblink

    SubClassOf: 
        Link
    
    
Class: Website

    SubClassOf: 
        CorporateIdentity
    
    
Class: Wind

    Annotations: 
        <http://purl.obolibrary.org/obo/IAO_0000115> "Kinetic energy of wind exploited for electricity generation in wind turbines.",
        <http://purl.obolibrary.org/obo/IAO_0000115> "Kinetic energy of wind exploited for electricity generation in wind turbines."@en,
        <http://purl.obolibrary.org/obo/IAO_0000119> "REGULATION (EC) No 1099/2008 OF THE EUROPEAN PARLIAMENT AND OF THE COUNCIL of 22 October 2008 on energy statistics https://eur-lex.europa.eu/legal-content/EN/TXT/HTML/?uri=CELEX:32008R1099&from=EN"
    
    SubClassOf: 
        Air
    
    
Class: WindElectricityGenerator

    Annotations: 
        <http://purl.obolibrary.org/obo/IAO_0000115> "A wind electricity generator technology uses wind power to generate electricity."@en
    
    SubClassOf: 
        RenewableGeneratorTechnology
    
    
Class: WindEntity

    SubClassOf: 
        ElectricityProductionUnit,
        has_part some Generator,
        has_part some WindEntityData
    
    
Class: WindEntityData

    SubClassOf: 
        InformationArtifact
    
    
Class: WindEntityDataset

    SubClassOf: 
        ElectricityProductionUnit,
        has_part some Generator,
        has_part some WindEntityData
    
    
Class: WindFarm

    Annotations: 
        <http://purl.obolibrary.org/obo/IAO_0000115> "A wind farm uses wind turbines and and wind to generate renewable energy."@en,
        <http://purl.obolibrary.org/obo/IAO_0000119> "https://en.wikipedia.org/w/index.php?title=Wind_turbine&oldid=867838943"
    
    SubClassOf: 
        RegenerativePowerplant,
        WindTurbine,
        has_part some WindTurbine
    
    
Class: WindOffshore

    SubClassOf: 
        WindTurbine,
        has_input some SeaRegion
    
    
Class: WindOnshore

    Annotations: 
        <http://purl.obolibrary.org/obo/IAO_0000115> "Onshore wind power is the complement to Offshore wind power. It is harvested on land."@en
    
    SubClassOf: 
        RegenerativePowerplant,
        has_part some WindTurbine
    
    
Class: WindTurbine

    Annotations: 
        <http://purl.obolibrary.org/obo/IAO_0000115> "A wind turbine is a device that converts the wind's kinetic energy into electrical energy.

Wind turbines are manufactured in a wide range of vertical and horizontal axis. The smallest turbines are used for applications such as battery charging for auxiliary power for boats or caravans or to power traffic warning signs. Slightly larger turbines can be used for making contributions to a domestic power supply while selling unused power back to the utility supplier via the electrical grid. Arrays of large turbines, known as wind farms, are becoming an increasingly important source of intermittent renewable energy and are used by many countries as part of a strategy to reduce their reliance on fossil fuels."@en,
        <http://purl.obolibrary.org/obo/IAO_0000119> "https://en.wikipedia.org/w/index.php?title=Wind_turbine&oldid=867838943"
    
    SubClassOf: 
        Turbine,
        has_physical_output some Power,
        uses some Wind,
        has_physical_input only Wind
    
    
Class: WoodAndOther

    Annotations: 
        <http://purl.obolibrary.org/obo/IAO_0000115> "Purpose-grown energy crops (poplar, willow etc.), a multitude of woody materials generated by an industrial process (wood/paper industry in particular) or provided directly by forestry and agriculture (firewood, wood chips, wood pellets, bark, sawdust, shavings, chips, black liquor etc.) as well as wastes such as straw, rice husks, nut shells, poultry litter, crushed grape dregs etc. Combustion is the preferred technology for these solid wastes. The quantity of fuel used should be reported on a net calorific value basis."@en,
        <http://purl.obolibrary.org/obo/IAO_0000119> "REGULATION (EC) No 1099/2008 OF THE EUROPEAN PARLIAMENT AND OF THE COUNCIL of 22 October 2008 on energy statistics https://eur-lex.europa.eu/legal-content/EN/TXT/HTML/?uri=CELEX:32008R1099&from=EN"@en
    
    SubClassOf: 
        SolidBiomass
    
    
Class: Workshop

    SubClassOf: 
        Support
    
    
Individual: <http://openenergy-platform.org/ontology/oeo/C++>

    Types: 
        Framework
    
    
Individual: <http://openenergy-platform.org/ontology/oeo/MS_Excel/VBA>

    Types: 
        Framework
    
    
Individual: <http://openenergy-platform.org/ontology/oeo/Spatial(GIS)>

    Types: 
        MethodicalFocus
    
    
Individual: Accounting

    Types: 
        MethodicalFocus
    
    
Individual: Active

    Types: 
        Modus
    
    
Individual: AgentBasedProgramming

    Types: 
        MathematicalConcept
    
    
Individual: Ampere

    Annotations: 
        rdfs:comment "Unit symbol: A
SI unit for electric current."@en
    
    Types: 
        ElectricCurrentUnit
    
    
Individual: Appliance

    
Individual: Aviation

    
Individual: BackCasting

    Types: 
        MethodicalFocus
    
    
Individual: BatteryElectric

    
Individual: BottomUp

    Types: 
        AnalyticalApproach
    
    
Individual: CH4

    SameAs: 
        Methane
    
    
Individual: CO2

    Types: 
        Cost
    
    SameAs: 
        Carbon_dioxide
    
    
Individual: CPLEX

    Types: 
        Solver
    
    
Individual: CSV

    Types: 
        DataFormat
    
    
Individual: Carbon_dioxide

    Types: 
        GreenhouseGas
    
    SameAs: 
        CO2
    
    
Individual: Coal

    Annotations: 
        <http://purl.obolibrary.org/obo/IAO_0000115> "Coal is a combustible black or brownish-black sedimentary rock, formed as rock strata called coal seams. Coal is mostly carbon with variable amounts of other elements; chiefly hydrogen, sulfur, oxygen, and nitrogen.Coal is formed if dead plant matter decays into peat and over millions of years the heat and pressure of deep burial converts the peat into coal."@en,
        <http://purl.obolibrary.org/obo/IAO_0000119> "https://en.wikipedia.org/w/index.php?title=Coal&oldid=907331967"
    
    
Individual: Coin-Or_CBC

    Types: 
        Solver
    
    
Individual: Common_year

    Annotations: 
        rdfs:comment "Unit symbol: a, y
1 a = 365 d"@en
    
    Types: 
        TimeUnit
    
    
Individual: Cooking

    Types: 
        ResidentialDemand
    
    
Individual: Coulomb

    Annotations: 
        rdfs:comment "Unit symbol: C
SI unit for electric charge."@en
    
    Types: 
        ElectricChargeUnit
    
    
Individual: DataFrame

    Types: 
        DataFormat
    
    
Individual: Database

    
Individual: Day

    Annotations: 
        rdfs:comment "Unit symbol: d
1 d = 24 h = 1440 min = 86,400 s"@en
    
    Types: 
        TimeUnit
    
    
Individual: Dict

    Types: 
        DataFormat
    
    
Individual: DynamicProgramming

    Types: 
        MathematicalConcept
    
    
Individual: E-101_3500

    Types: 
        WaterTurbine
    
    
Individual: E-115_3000

    Types: 
        WaterTurbine
    
    
Individual: E-115_3200

    Types: 
        WaterTurbine
    
    
Individual: E-126_4200

    Types: 
        WaterTurbine
    
    
Individual: E-141_4200

    Types: 
        WaterTurbine
    
    
Individual: E-82_3000

    Types: 
        WaterTurbine
    
    
Individual: E-92_2350

    Types: 
        WaterTurbine
    
    
Individual: Econometric

    Types: 
        MethodicalFocus
    
    
Individual: EconomicEquilibrium

    Types: 
        MethodicalFocus
    
    
Individual: Eurostat_Energy_Balances

    Annotations: 
        <http://purl.obolibrary.org/obo/IAO_0000115> "The concept of \"energy balance\" is an accounting framework for the compilation and understanding of data on all energy products entering, exiting and being used in a country. The energy balance is the most complete statistical accounting of energy products and their flow in the economy. Columns of the energy balance represent energy products (fuels). Rows represent energy flows.

The energy balance expresses all forms of energy in a common accounting unit. The balance shows the relationships between supply, inputs to the energy transformation processes and their outputs as well as the actual energy consumption by different sectors of end-use.",
        <http://purl.obolibrary.org/obo/IAO_0000116> "This is a general description of an energy balance. A link to a complete Eurostat energy balance is provided under the URL for 'definition source'",
        <http://purl.obolibrary.org/obo/IAO_0000119> "https://ec.europa.eu/eurostat/statistics-explained/index.php/Energy_balance#What_is_an_energy_balance.3F"
    
    Types: 
        SectorConcept
    
    
Individual: False

    Types: 
        BooleanVariable
    
    
Individual: Farad

    Annotations: 
        rdfs:comment "Unit symbol: F
SI derived unit of electrical capacitance."@en
    
    Types: 
        CapacitanceUnit
    
    
Individual: Foot

    Annotations: 
        rdfs:comment "Unit symbol: ft
1 ft = 0.3048 m"@en
    
    Types: 
        LengthUnit
    
    
Individual: Fortran

    Types: 
        Framework
    
    
Individual: FuzzyLogic

    Types: 
        MathematicalConcept
    
    
Individual: GAMS

    Types: 
        Framework
    
    
Individual: GLPK

    Types: 
        Solver
    
    
Individual: GNU

    Types: 
        Framework
    
    
Individual: German_Energy_Balances

    Annotations: 
        <http://purl.obolibrary.org/obo/IAO_0000115> "Das Schema der Energiebilanzen umfasst eine Matrix von 33 Spalten und 68 Zeilen (einschließlich der Summenspalten und -zeilen). In der horizontalen Gliederung (Spalten) werden die Energieträger ausgewiesen, die der energetischen und nichtenergetischen Nutzung dienen. In der vertikalen Gliederung (Zeilen) werden für die jeweiligen Energieträger Aufkommen, Umwandlung und Verwendung erfasst.

Als Energieträger werden alle Quellen oder Stoffe bezeichnet, in denen Energie mechanisch, thermisch, chemisch oder physikalisch gespeichert ist. Fünf Kerngruppe werden bei der Energiebilanz unterschieden:

    Fossile Brennstoffe
    Erneuerbare Energien
    Strom
    Kernbrennstoffe
    Fernwärme

Bilanzebenen
Schematische Darstellung des Bilanzraums der deutschen Arbeitsgemeinschaft Energiebilanzen
Primär- und Endenergie sowie Umwandlungsverluste

Die Abgrenzung erfolgt in drei Bilanzbereichen:

    die Primärenergiebilanz,
    die Umwandlungsbilanz und
    der Endenergieverbrauch.

In der Primärenergiebilanz werden die Energieträger mit ihrem Mengenaufkommen bei der Gewinnung und Anlieferung nach folgenden Kriterien erfasst:

    inländische Gewinnung von Energieträgern,
    Außenhandel mit Energieträgern, unterteilt nach Einfuhr und Ausfuhr,
    Hochseebunkerungen (Heizöl, Dieselkraftstoff und Schmierstoffe für die nationale und internationale Seeschifffahrt in deutschen Häfen. Ohne Lieferungen an Binnen- und Küstenmotorschiffe und Fischerei, die zum Sektor Verkehr (Endenergieverbrauch) zählen.)
    Bestandsveränderungen, getrennt erfasst nach Bestandsentnahmen und -aufstockungen",
        <http://purl.obolibrary.org/obo/IAO_0000116> "The German Energy Balance is managed by the 'AG Energiebilanzen', where aso the energy balances can be found: https://ag-energiebilanzen.de/",
        <http://purl.obolibrary.org/obo/IAO_0000119> "https://de.wikipedia.org/w/index.php?title=Energiebilanz_(Energiewirtschaft)&oldid=176259115"
    
    Types: 
        SectorConcept
    
    
Individual: GigaWattHours

    Annotations: 
        rdfs:comment "Unit symbol: GWh
Used for electricity"@en
    
    Types: 
        EnergyUnit
    
    
Individual: Grain

    Annotations: 
        rdfs:comment "Unit symbol: grain, gr
1 gr = 64,79891 mg"@en
    
    Types: 
        MassUnit
    
    
Individual: Gram

    Annotations: 
        rdfs:comment "Unit symbol: g
SI unit for mass: kg (1 kg = 1000 g)"@en
    
    Types: 
        MassUnit
    
    
Individual: Gurobi

    Types: 
        Solver
    
    
Individual: HFC

    Annotations: 
        <http://purl.obolibrary.org/obo/IAO_0000115> "Hydrofluorocarbons (HFCs) are organic compounds that contain fluorine and hydrogen atoms, and are the most common type of organofluorine compounds. They are frequently used in air conditioning and as refrigerants in place of the older chlorofluorocarbons such as R-12 and hydrochlorofluorocarbons such as R-21."@en,
        <http://purl.obolibrary.org/obo/IAO_0000119> "https://en.wikipedia.org/w/index.php?title=Hydrofluorocarbon&oldid=904556263"@en
    
    Types: 
        FlourinatedGas
    
    Facts:  
     is_equivalent_to  Hydrofluorocarbon
    
    
Individual: HardCoal

    Annotations: 
        <http://purl.obolibrary.org/obo/IAO_0000115> "The term ‘hard coal’ refers to coal of gross calorific value greater than 23 865 kJ/kg (5 700 kcal/kg) on an ashfree but moist basis and with a mean random reflectance of vitrinite of at least 0,6."@en,
        <http://purl.obolibrary.org/obo/IAO_0000119> "REGULATION (EC) No 1099/2008 OF THE EUROPEAN PARLIAMENT AND OF THE COUNCIL of 22 October 2008 on energy statistics https://eur-lex.europa.eu/legal-content/EN/TXT/HTML/?uri=CELEX:32008R1099&from=EN"@en
    
    
Individual: Heat

    Annotations: 
        <http://purl.obolibrary.org/obo/IAO_0000115> "In thermodynamics, heat is energy in transfer to or from a thermodynamic system, by mechanisms other than thermodynamic work or transfer of matter.
       The mechanisms include conduction, through direct contact of immobile bodies, or through a wall or barrier that is impermeable to matter; or radiation between separated bodies; or isochoric mechanical work done by the surroundings on the system of interest; or Joule heating by an electric current driven through the system of interest by an external system; or a combination of these."@en,
        <http://purl.obolibrary.org/obo/IAO_0000119> "https://en.wikipedia.org/w/index.php?title=Heat&oldid=90563031157"@en
    
    Types: 
        ResidentialDemand
    
    
Individual: Hour

    Annotations: 
        rdfs:comment "Unit symbol: h
1h = 60 min = 3600 s"@en
    
    Types: 
        TimeUnit
    
    
Individual: Hybrid

    Types: 
        AnalyticalApproach
    
    
Individual: Hydrofluorocarbon

    Annotations: 
        <http://purl.obolibrary.org/obo/IAO_0000115> "Hydrofluorocarbons (HFCs) are organic compounds that contain fluorine and hydrogen atoms, and are the most common type of organofluorine compounds. They are frequently used in air conditioning and as refrigerants in place of the older chlorofluorocarbons such as R-12 and hydrochlorofluorocarbons such as R-21."@en,
        <http://purl.obolibrary.org/obo/IAO_0000119> "https://en.wikipedia.org/w/index.php?title=Hydrofluorocarbon&oldid=904556263"@en
    
    Types: 
        FlourinatedGas
    
    Facts:  
     is_equivalent_to  HFC
    
    
Individual: Hydrogen

    Annotations: 
        <http://purl.obolibrary.org/obo/IAO_0000115> "Hydrogen is a chemical element with chemical symbol H and atomic number 1. It is used in water electrolysis during the power-to-gas process as a storage medium for excess electricty."@en,
        <http://purl.obolibrary.org/obo/IAO_0000119> "https://wiki.openmod-initiative.org/wiki/Hydrogen"@en
    
    
Individual: IPCC_1996_Guidelines

    Annotations: 
        <http://purl.obolibrary.org/obo/IAO_0000115> "The sectoral approach taken for reporting greenhouse gas inventories under UNFCCC; version of 1996 (revised).",
        <http://purl.obolibrary.org/obo/IAO_0000119> "https://www.ipcc-nggip.iges.or.jp/public/gl/invs6.html"
    
    Types: 
        SectorConcept
    
    
Individual: IPCC_2006_Guidelines

    Annotations: 
        <http://purl.obolibrary.org/obo/IAO_0000115> "The sectoral approach taken for reporting greenhouse gas inventories under UNFCCC; version of 2006.",
        <http://purl.obolibrary.org/obo/IAO_0000119> "https://www.ipcc-nggip.iges.or.jp/public/2006gl/index.html"
    
    Types: 
        SectorConcept
    
    
Individual: Inactive

    Types: 
        Modus
    
    
Individual: Inch

    Annotations: 
        rdfs:comment "Unit symbol: in, \"
1 in = 1\" = 2,54 cm = 0,0254 m"@en
    
    Types: 
        LengthUnit
    
    
Individual: InternalCombustion

    
Individual: InternalcombustionVehicle

    
Individual: Java

    Types: 
        Framework
    
    
Individual: Joule

    Annotations: 
        rdfs:comment "SI unit for energy.
Unit symbol: J
1 J = 1 kg*(m/s)^2"@en
    
    Types: 
        EnergyUnit
    
    
Individual: Julian_year

    Annotations: 
        rdfs:comment "Unit symbol: a, a_jul, y, y_jul
1 a = 365,25 d = 31,557,600 s"@en
    
    Types: 
        TimeUnit
    
    
Individual: Kilowatt_hour

    Annotations: 
        rdfs:comment "Unit symbol: kWh
1 kWh = 3600 kJ
Used for electricity"@en
    
    Types: 
        EnergyUnit
    
    
Individual: Leap_year

    Annotations: 
        rdfs:comment "Unit symbol: a, y
1 a = 366 d"@en
    
    Types: 
        TimeUnit
    
    
Individual: Light

    Types: 
        ResidentialDemand
    
    
Individual: Lignite

    Annotations: 
        <http://purl.obolibrary.org/obo/IAO_0000115> "Non-agglomerating coal with a gross calorific value less than 17 435 kJ/kg (4 165 kcal/kg) and greater than 31 % volatile matter on a dry mineral matter free basis.

Oil shale and tar sands produced and combusted directly should be reported in this category. Oil shale and tar sands used as inputs for other transformation processes should also be reported in this category.

This includes the portion of the oil shale or tar sands consumed in the transformation process."@en,
        <http://purl.obolibrary.org/obo/IAO_0000119> "REGULATION (EC) No 1099/2008 OF THE EUROPEAN PARLIAMENT AND OF THE COUNCIL of 22 October 2008 on energy statistics https://eur-lex.europa.eu/legal-content/EN/TXT/HTML/?uri=CELEX:32008R1099&from=EN"@en
    
    
Individual: LinearProgramming

    Types: 
        MathematicalConcept
    
    
Individual: MOSEK

    Types: 
        Solver
    
    
Individual: MS_Excel

    Types: 
        Framework
    
    
Individual: Macro-Economic

    Types: 
        MethodicalFocus
    
    
Individual: MathProg

    Types: 
        Framework
    
    
Individual: Matlab

    Types: 
        Framework
    
    
Individual: Megawatt

    Annotations: 
        rdfs:comment "Unit symbol: MW
1 MW = 1000W"@en
    
    Types: 
        PowerUnit
    
    
Individual: Methane

    Types: 
        GreenhouseGas,
        VolatileOrganicCompound
    
    SameAs: 
        CH4
    
    
Individual: Metre

    Annotations: 
        rdfs:comment "Unit symbol: m
SI unit for length"@en
    
    Types: 
        LengthUnit
    
    
Individual: Mile

    Annotations: 
        rdfs:comment "Unit symbol: mile
1 mile = 1609.344 m"@en
    
    Types: 
        LengthUnit
    
    
Individual: Minute

    Annotations: 
        rdfs:comment "Unit Symbol: min
1 min = 60s"@en
    
    Types: 
        TimeUnit
    
    
Individual: MixedIntegerLinearProgramming

    Types: 
        MathematicalConcept
    
    
Individual: Modellca

    Types: 
        Framework
    
    
Individual: MonteCarlo

    Types: 
        MethodicalFocus
    
    
Individual: Month

    
Individual: MultiCriteria

    Types: 
        MethodicalFocus
    
    
Individual: N2O

    SameAs: 
        Nitrous_oxide
    
    
Individual: NACE_Sectors

    Annotations: 
        <http://purl.obolibrary.org/obo/IAO_0000115> "The Statistical classification of economic activities in the European Community, abbreviated as NACE, is the classification of economic activities in the European Union (EU); the term NACE is derived from the French Nomenclature statistique des activités économiques dans la Communauté européenne. Various NACE versions have been developed since 1970.

NACE is a four-digit classification providing the framework for collecting and presenting a large range of statistical data according to economic activity in the fields of economic statistics (e.g. production, employment and national accounts) and in other statistical domains developed within the European statistical system (ESS).",
        <http://purl.obolibrary.org/obo/IAO_0000119> "https://ec.europa.eu/eurostat/statistics-explained/index.php?title=Glossary:Statistical_classification_of_economic_activities_in_the_European_Community_(NACE)"
    
    Types: 
        SectorConcept
    
    
Individual: NF3

    SameAs: 
        Nitrogen_trifluoride
    
    
Individual: Nautical_mile

    Annotations: 
        rdfs:comment "Unit symbol: M, NM, nmi, sm
1 M = 1852 m"@en
    
    Types: 
        LengthUnit
    
    
Individual: Newton_metre

    Annotations: 
        rdfs:comment "Unit symbol: Nm
1 Nm = 1 J
Used for torque"@en
    
    Types: 
        EnergyUnit
    
    
Individual: Nitrogen_trifluoride

    Types: 
        GreenhouseGas
    
    SameAs: 
        NF3
    
    
Individual: Nitrous_oxide

    Types: 
        GreenhouseGas
    
    SameAs: 
        N2O
    
    
Individual: NuclearPower

    Annotations: 
        <http://purl.obolibrary.org/obo/IAO_0000115> "Nuclear power is the use of nuclear reactions that release nuclear energy to generate heat, which most frequently is then used in steam turbines to produce electricity in a nuclear power plant. Nuclear power can be obtained from nuclear fission, nuclear decay and nuclear fusion. Presently, the vast majority of electricity from nuclear power is produced by nuclear fission of elements in the actinide series of the periodic table. Nuclear decay processes are used in niche applications such as radioisotope thermoelectric generators. The possibility of generating electricity from nuclear fusion is still at a research phase with no commercial applications. This article mostly deals with nuclear fission power for electricity generation."@en,
        <http://purl.obolibrary.org/obo/IAO_0000119> "https://en.wikipedia.org/w/index.php?title=Nuclear_power&oldid=868476098"@en
    
    
Individual: Ohm

    Annotations: 
        rdfs:comment "Unit symbol: Ω
SI derived unit for electrical resistance"@en
    
    Types: 
        ResistanceUnit
    
    
Individual: Oil

    
Individual: Optimization

    Annotations: 
        <http://purl.obolibrary.org/obo/IAO_0000115> "An optimization is a model calculation with the goal to find a best choice or result for at least one variable or function in the model."@en
    
    Types: 
        MethodicalFocus
    
    
Individual: Other

    Types: 
        AnalyticalApproach
    
    
Individual: Ounce

    Annotations: 
        rdfs:comment "Unit symbol: oz
1 oz = 28.349523125 g (there are other ounces but this is the one that is used the most)"@en
    
    Types: 
        MassUnit
    
    
Individual: PFC

    Annotations: 
        <http://purl.obolibrary.org/obo/IAO_0000115> "Fluorocarbons, sometimes referred to as perfluorocarbons or PFCs, are, strictly speaking, organofluorine compounds with the formula CxFy, i.e. they contain only carbon and fluorine, though the terminology is not strictly followed. Compounds with the prefix perfluoro- are hydrocarbons, including those with heteroatoms, wherein all C-H bonds have been replaced by C-F bonds."@en,
        <http://purl.obolibrary.org/obo/IAO_0000119> "https://en.wikipedia.org/w/index.php?title=Fluorocarbon&oldid=881053361"@en
    
    Types: 
        FlourinatedGas
    
    
Individual: PHP

    Types: 
        Framework
    
    
Individual: Passive

    
Individual: Perfluorocarbon

    Annotations: 
        <http://purl.obolibrary.org/obo/IAO_0000115> "Fluorocarbons, sometimes referred to as perfluorocarbons or PFCs, are, strictly speaking, organofluorine compounds with the formula CxFy, i.e. they contain only carbon and fluorine, though the terminology is not strictly followed. Compounds with the prefix perfluoro- are hydrocarbons, including those with heteroatoms, wherein all C-H bonds have been replaced by C-F bonds."@en,
        <http://purl.obolibrary.org/obo/IAO_0000119> "https://en.wikipedia.org/w/index.php?title=Fluorocarbon&oldid=881053361"@en
    
    Types: 
        FlourinatedGas
    
    
Individual: Plot

    
Individual: Pound

    Annotations: 
        rdfs:comment "Unit symbol: lb
1 lb = 0.45359237 kg"@en
    
    Types: 
        MassUnit
    
    
Individual: Python

    Types: 
        Framework
    
    
Individual: R

    Types: 
        Framework
    
    
Individual: Rail

    
Individual: Renewable_Energy_Directive_Sectors

    Annotations: 
        <http://purl.obolibrary.org/obo/IAO_0000116> "The Renewable Energy Directive has been revised, but this should have had no impacts on the sectoral definitions. Factsheet on revision: https://ec.europa.eu/energy/sites/ener/files/documents/directive_renewable_factsheet.pdf",
        <http://purl.obolibrary.org/obo/IAO_0000119> "https://eur-lex.europa.eu/legal-content/EN/ALL/?uri=CELEX:32009L0028"
    
    Types: 
        SectorConcept
    
    
Individual: Ruby

    Types: 
        Framework
    
    
Individual: SF6

    SameAs: 
        Sulphur_hexafluoride
    
    
Individual: Second

    Annotations: 
        rdfs:comment "Unit symbol: s
SI unit of time"@en
    
    Types: 
        TimeUnit
    
    
Individual: Simulation

    Annotations: 
        <http://purl.obolibrary.org/obo/IAO_0000115> "A simulation is a model calculation that simulates a process or system behavior from the real world."@en
    
    Types: 
        MethodicalFocus
    
    
Individual: SmartMetre

    Types: 
        Appliance
    
    
Individual: Spreadsheet

    Types: 
        MethodicalFocus
    
    
Individual: Stochastic

    Types: 
        MethodicalFocus
    
    
Individual: Sulphur_hexafluoride

    Types: 
        GreenhouseGas
    
    SameAs: 
        SF6
    
    
Individual: TerraWattHours

    Annotations: 
        rdfs:comment "Unit symbol: TWh
Used for electricity"@en
    
    Types: 
        EnergyUnit
    
    
Individual: Therm

    Annotations: 
        rdfs:comment "Unit symbol: thm
1 thm ≈ 105.5 MJ (exact value depending on region)
Used for natural gas"@en
    
    Types: 
        EnergyUnit
    
    
Individual: Tons

    Annotations: 
        rdfs:comment "Unit symbol: t
1 t = 3600 kg"@en
    
    Types: 
        MassUnit
    
    
Individual: Toolbox

    Types: 
        MethodicalFocus
    
    
Individual: TopDown

    Types: 
        AnalyticalApproach
    
    
Individual: True

    Types: 
        BooleanVariable
    
    
Individual: Txt

    Types: 
        DataFormat
    
    
Individual: V2Grid

    
Individual: Volt

    Annotations: 
        rdfs:comment "Unit symbol: V
SI derived unit for voltage."@en
    
    Types: 
        VoltageUnit
    
    
Individual: Water

    
Individual: Watt

    Annotations: 
        rdfs:comment "Unit symbol: W
SI derived unit for power."@en
    
    Types: 
        PowerUnit
    
    
Individual: Week

    Annotations: 
        rdfs:comment "Unit symbol: week
1 week = 7 d"@en
    
    Types: 
        TimeUnit
    
    
Individual: Wind

    Annotations: 
        <http://purl.obolibrary.org/obo/IAO_0000115> "Kinetic energy of wind exploited for electricity generation in wind turbines.",
        <http://purl.obolibrary.org/obo/IAO_0000115> "Kinetic energy of wind exploited for electricity generation in wind turbines."@en,
        <http://purl.obolibrary.org/obo/IAO_0000119> "REGULATION (EC) No 1099/2008 OF THE EUROPEAN PARLIAMENT AND OF THE COUNCIL of 22 October 2008 on energy statistics https://eur-lex.europa.eu/legal-content/EN/TXT/HTML/?uri=CELEX:32008R1099&from=EN"
    
    
Individual: XLSX

    Types: 
        DataFormat
    
    
Individual: XML

    Types: 
        DataFormat
    
    
Individual: Yard

    Annotations: 
        rdfs:comment "Unit symbol: yd
1 yd = 0.9144 m"@en
    
    Types: 
        LengthUnit
    
    
Individual: Year

    
Individual: gaseous

    Annotations: 
        <http://purl.obolibrary.org/obo/IAO_0000115> "The state of being a gas. A portion of matter is in gaseous state if and only if it has has no definite shape and no definite volume and is not electrically conductive."
    
    
Individual: gdx

    Types: 
        DataFormat
    
    
Individual: liquid

    Annotations: 
        <http://purl.obolibrary.org/obo/IAO_0000115> "The state of being liquid. A portion of matter is liquid has has no definite shape but a definite volume (at a given temperature and pressure)."
    
    
Individual: plasmatic

    Annotations: 
        <http://purl.obolibrary.org/obo/IAO_0000115> "The state of being a plasma. A portion of matter is in plasmatic state if and only if it has has no definite shape and no definite volume and is electrically conductive."
    
    
Individual: solid

    Annotations: 
        <http://purl.obolibrary.org/obo/IAO_0000115> "The state being solid. A portion of matter is in solid state if and only if it has a definite shape and volume (at a given temperature and pressure)."
    
    
DisjointClasses: 
    Acronym,DOI,Title

DisjointClasses: 
    BioElectricityGenerator,PhotovoltaicElectricityGenerator,WaterElectricityGenerator,WindElectricityGenerator

DisjointClasses: 
    BiomassPowerplant,CoalPowerplant,GasPowerplant,GeothermalGenerator,HydroPowerplant,NuclearPowerplant,OceanPowerplant,OilPowerplant,PhotovoltaicGenerator,WastePowerplant,WindTurbine

DisjointClasses: 
    Bus,Consumer,Generator,Line,PowerGeneratingUnit,ShuntImpedance,StorageUnit,Subgrid,Transformer

DisjointClasses: 
    CapacitanceUnit,ElectricChargeUnit,ElectricCurrentUnit,EnergyUnit,LengthUnit,MassUnit,PowerUnit,ResistanceUnit,TimeUnit,VoltageUnit

DisjointClasses: 
    CoalElectricityGenerator,NaturalGasGenerator,NuclearPowerGenerator,OilElectricityGenerator

DisjointClasses: 
    CommerceSector,HouseholdSector,IndustrySector

DisjointClasses: 
    DemographicalAssumption,EconomicalAssumption,PoliticalAssumption,TechnologicalAssumption

DisjointClasses: 
    ElectricityGeneratorTechnology,EnergyStorageTechnology,EnergyTransferTechnology

DisjointClasses: 
    ElectricityGeneratorTechnology,EnergyStorageTechnology,EnergyTransferTechnology,HeatGeneratorTechnology

DisjointClasses: 
    ElectricitySector,HeatSector,TransportSector

DisjointClasses: 
    EnergyGeneratorTechnology,EnergyStorageTechnology,EnergyTransferTechnology

DisjointClasses: 
    EnergyUnit,LengthUnit,MassUnit,TimeUnit

DisjointClasses: 
    Fuel,Heat,Hydropower,Nuclear,Solar,Wind

DisjointClasses: 
    Generator,ShuntImpedance,StorageUnit,Subgrid,Transformer

DisjointClasses: 
    HouseholdSector,IndustrySector,TCSSector,TrafficSector

DisjointClasses: 
    LinearOptimalPowerflow,SingleNodeModel,TranshipmentModel

