Prefix: : <http://openenergy-platform.org/ontology/oeo/>
Prefix: dc: <http://purl.org/dc/elements/1.1/>
Prefix: owl: <http://www.w3.org/2002/07/owl#>
Prefix: rdf: <http://www.w3.org/1999/02/22-rdf-syntax-ns#>
Prefix: rdfs: <http://www.w3.org/2000/01/rdf-schema#>
Prefix: skos: <http://www.w3.org/2004/02/skos/core#>
Prefix: xml: <http://www.w3.org/XML/1998/namespace>
Prefix: xsd: <http://www.w3.org/2001/XMLSchema#>



Ontology: <http://openenergy-platform.org/ontology/oeo/oeo-tasks/>
<http://openenergy-platform.org/ontology/oeo/dev/oeo-tasks.omn>
Import: <http://openenergy-platform.org/ontology/oeo/dev/oeo-shared.omn>

Annotations: 
    dc:description "The Open Energy Ontology is an ontology for all aspects of the energy modelling domain. The 'Tasks' module covers energy-related task definitions and their realization steps. It aims to specify common tasks and methodologies that are performed regularly in the scientific process of energy systems analysis.",
    dc:license "http://creativecommons.org/publicdomain/zero/1.0/",
    <http://purl.org/dc/terms/title> "Open Energy Ontology (Task module)"

AnnotationProperty: <http://purl.obolibrary.org/obo/IAO_0000115>

    
AnnotationProperty: <http://purl.org/dc/terms/title>

    
AnnotationProperty: OEO_00020426

    
AnnotationProperty: dc:description

    
AnnotationProperty: dc:license

    
AnnotationProperty: rdfs:comment

    
AnnotationProperty: rdfs:label

    
Datatype: rdf:PlainLiteral

    
Datatype: xsd:string

    
ObjectProperty: <http://purl.obolibrary.org/obo/BFO_0000051>

    
ObjectProperty: <http://purl.obolibrary.org/obo/BFO_0000054>

    
ObjectProperty: <http://purl.obolibrary.org/obo/RO_0000056>

    
ObjectProperty: <http://purl.obolibrary.org/obo/RO_0000057>

    
ObjectProperty: OEO_00390026

    Annotations: 
        OEO_00020426 "Add:
issue: https://github.com/OpenEnergyPlatform/ontology/issues/1891
pull request: https://github.com/OpenEnergyPlatform/ontology/pull/1940",
        <http://purl.obolibrary.org/obo/IAO_0000115> "A relationship between a process and a plan specification, in which the process is predefined or planned by the plan specification.",
        rdfs:label "structured by"@en
    
    SubPropertyOf: 
        <http://purl.obolibrary.org/obo/RO_0000057>
    
    Domain: 
        <http://purl.obolibrary.org/obo/BFO_0000015>
    
    Range: 
        <http://purl.obolibrary.org/obo/IAO_0000104>
    
    
ObjectProperty: owl:topObjectProperty

    
Class: <http://purl.obolibrary.org/obo/BFO_0000015>

    
Class: <http://purl.obolibrary.org/obo/BFO_0000017>

    
Class: <http://purl.obolibrary.org/obo/BFO_0000035>

    
Class: <http://purl.obolibrary.org/obo/IAO_0000005>

    
Class: <http://purl.obolibrary.org/obo/IAO_0000007>

    
Class: <http://purl.obolibrary.org/obo/IAO_0000104>

    
Class: OEO_00020166

    
Class: OEO_00390002

    Annotations: 
        OEO_00020426 "Add:
issue: https://github.com/OpenEnergyPlatform/ontology/issues/1891
pull request: https://github.com/OpenEnergyPlatform/ontology/pull/1940",
        <http://purl.obolibrary.org/obo/IAO_0000115> "Wind characteristics determination method is a methodology with the goal to understand the specific wind characteristics of a predefined region, encompassing data acquisition, modelling, and analytical procedures.",
        rdfs:label "wind characteristics determination method"@en
    
    SubClassOf: 
        OEO_00020166,
        <http://purl.obolibrary.org/obo/BFO_0000051> some OEO_00390004
    
    
Class: OEO_00390003

    Annotations: 
        OEO_00020426 "Add:
issue: https://github.com/OpenEnergyPlatform/ontology/issues/1891
pull request: https://github.com/OpenEnergyPlatform/ontology/pull/1940",
        <http://purl.obolibrary.org/obo/IAO_0000115> "Data preparation is an action specification that describes the steps the bearer takes to acquire raw data and how this data is cleaned, transformed, and structured for subsequent analysis. So it includes the acquisition and pre-processing of data.",
        rdfs:label "data preparation"@en
    
    SubClassOf: 
        OEO_00390035
    
    
Class: OEO_00390004

    Annotations: 
        OEO_00020426 "Add:
issue: https://github.com/OpenEnergyPlatform/ontology/issues/1891
pull request: https://github.com/OpenEnergyPlatform/ontology/pull/1940",
        <http://purl.obolibrary.org/obo/IAO_0000115> "Determined wind characteristics is an object specification that defines the goal of a methodology as a state of understanding the specific wind characteristics of a predefined region.",
        rdfs:label "determined wind characteristics"@en
    
    SubClassOf: 
        <http://purl.obolibrary.org/obo/IAO_0000005>
    
    
Class: OEO_00390005

    Annotations: 
        OEO_00020426 "Add:
issue: https://github.com/OpenEnergyPlatform/ontology/issues/1891
pull request: https://github.com/OpenEnergyPlatform/ontology/pull/1940",
        <http://purl.obolibrary.org/obo/IAO_0000115> "Wind speed calculation is an action specification that describes how wind speed at the hub height of a wind turbine is inferred from measurements taken at a different height. It is extrapolated vertically to the hub height.",
        rdfs:label "wind speed calculation"@en
    
    SubClassOf: 
        OEO_00390035
    
    
Class: OEO_00390007

    Annotations: 
        OEO_00020426 "Add:
issue: https://github.com/OpenEnergyPlatform/ontology/issues/1891
pull request: https://github.com/OpenEnergyPlatform/ontology/pull/1940",
        <http://purl.obolibrary.org/obo/IAO_0000115> "Wind characteristics determination process is a process that follows a determination methodology for wind characteristics to gain knowledge of the specific wind characteristics of a predefined region.",
        rdfs:label "wind characteristics determination process"@en
    
    SubClassOf: 
        <http://purl.obolibrary.org/obo/BFO_0000015>,
        OEO_00390026 some OEO_00390002
    
    
Class: OEO_00390014

    Annotations: 
        OEO_00020426 "Add:
issue: https://github.com/OpenEnergyPlatform/ontology/issues/1891
pull request: https://github.com/OpenEnergyPlatform/ontology/pull/1940",
        <http://purl.obolibrary.org/obo/IAO_0000115> "Air density adjustment is an action specification that describes how variations in air density due to changes in altitude, temperature, and pressure are incorporated into the wind resource calculations.",
        rdfs:label "air density adjustment"@en
    
    SubClassOf: 
        OEO_00390035
    
    
Class: OEO_00390015

    Annotations: 
        OEO_00020426 "Add:
issue: https://github.com/OpenEnergyPlatform/ontology/issues/1891
pull request: https://github.com/OpenEnergyPlatform/ontology/pull/1940",
        <http://purl.obolibrary.org/obo/IAO_0000115> "Wind speed frequency analysis is an action specification that describes the process of calculating the frequency of different wind speed intervals over a set period giving a wind speed frequency distribution.",
        rdfs:label "wind speed frequency analysis"@en
    
    SubClassOf: 
        OEO_00390035
    
    
Class: OEO_00390016

    Annotations: 
        OEO_00020426 "Add:
issue: https://github.com/OpenEnergyPlatform/ontology/issues/1891
pull request: https://github.com/OpenEnergyPlatform/ontology/pull/1940",
        <http://purl.obolibrary.org/obo/IAO_0000115> "Wind variability identification is an action specification that describes the process of identifying variations in wind characteristics—such as speed, direction, frequency, turbulence, and seasonal or diurnal patterns—across temporal scales.",
        rdfs:label "wind variability identification"@en
    
    SubClassOf: 
        OEO_00390035
    
    
Class: OEO_00390017

    Annotations: 
        OEO_00020426 "Add:
issue: https://github.com/OpenEnergyPlatform/ontology/issues/1891
pull request: https://github.com/OpenEnergyPlatform/ontology/pull/1940",
        <http://purl.obolibrary.org/obo/IAO_0000115> "Wind Power Density calculation is an action specification that describes how Wind Power Density (WPD) is calculated to estimate the theoretical wind power potential based on wind speed and air density.",
        rdfs:comment "Wind Power Density calculation",
        rdfs:label "Wind Power Density calculation"@en
    
    SubClassOf: 
        OEO_00390035
    
    
Class: OEO_00390027

    Annotations: 
        OEO_00020426 "Add:
issue: https://github.com/OpenEnergyPlatform/ontology/issues/1891
pull request: https://github.com/OpenEnergyPlatform/ontology/pull/1940",
        <http://purl.obolibrary.org/obo/IAO_0000115> "Improve spatial resolution is an action specification that describes the process of increasing the spatial resolution of wind data across a region to provide finer detail for wind resource assessment. This is done by horizontal interpolation.",
        rdfs:label "improve spatial resolution"@en
    
    SubClassOf: 
        OEO_00390036
    
    
Class: OEO_00390028

    Annotations: 
        OEO_00020426 "Add:
issue: https://github.com/OpenEnergyPlatform/ontology/issues/1891
pull request: https://github.com/OpenEnergyPlatform/ontology/pull/1940",
        <http://purl.obolibrary.org/obo/IAO_0000115> "Select exclusion criteria is an action specification that describes the process of defining physical, environmental, and regulatory criteria that exclude areas from wind farm development, along with the application of buffer zones.",
        rdfs:label "select exclusion criteria"@en
    
    SubClassOf: 
        OEO_00390036
    
    
Class: OEO_00390029

    Annotations: 
        OEO_00020426 "Add:
issue: https://github.com/OpenEnergyPlatform/ontology/issues/1891
pull request: https://github.com/OpenEnergyPlatform/ontology/pull/1940",
        <http://purl.obolibrary.org/obo/IAO_0000115> "Prepare exclusion criteria datasets is an action specification that describes the steps involved in obtaining and preparing datasets that represent exclusion zones for wind farm development, based on predefined criteria. That includes acquiring and processing the data.",
        rdfs:label "prepare exclusion criteria datasets"@en
    
    SubClassOf: 
        OEO_00390036
    
    
Class: OEO_00390030

    Annotations: 
        OEO_00020426 "Add:
issue: https://github.com/OpenEnergyPlatform/ontology/issues/1891
pull request: https://github.com/OpenEnergyPlatform/ontology/pull/1940",
        <http://purl.obolibrary.org/obo/IAO_0000115> "Run Multi-Criteria Decision Analysis is an action specification that describes how a Multi-Criteria Decision Analysis (MCDA) method is applied to areas where exclusions are not absolute (soft exclusion criteria), allowing for weighted decision-making.",
        rdfs:label "run multi-criteria decision analysis"@en
    
    SubClassOf: 
        OEO_00390036
    
    
Class: OEO_00390031

    Annotations: 
        OEO_00020426 "Add:
issue: https://github.com/OpenEnergyPlatform/ontology/issues/1891
pull request: https://github.com/OpenEnergyPlatform/ontology/pull/1940",
        <http://purl.obolibrary.org/obo/IAO_0000115> "Determine development area is an action specification that describes the identification of potential areas where wind farm development is feasible, by iteratively excluding non-available areas based on the processed data and exclusion criteria.",
        rdfs:label "determine development area"@en
    
    SubClassOf: 
        OEO_00390036
    
    
Class: OEO_00390032

    Annotations: 
        OEO_00020426 "Add:
issue: https://github.com/OpenEnergyPlatform/ontology/issues/1891
pull request: https://github.com/OpenEnergyPlatform/ontology/pull/1940",
        <http://purl.obolibrary.org/obo/IAO_0000115> "Determine geographical potential is an action specification that describes the calculation of the total geographical area available for wind farm development after applying exclusion criteria and considering spatial constraints.",
        rdfs:label "determine geographical potential"@en
    
    SubClassOf: 
        OEO_00390036
    
    
Class: OEO_00390033

    Annotations: 
        OEO_00020426 "Add:
issue: https://github.com/OpenEnergyPlatform/ontology/issues/1891
pull request: https://github.com/OpenEnergyPlatform/ontology/pull/1940",
        <http://purl.obolibrary.org/obo/IAO_0000115> "Determined wind farm area is an object specification that defines the goal of a methodology as a state of understanding the available area for wind farm development.",
        rdfs:label "determined wind farm area"@en
    
    SubClassOf: 
        <http://purl.obolibrary.org/obo/IAO_0000005>
    
    
Class: OEO_00390034

    Annotations: 
        OEO_00020426 "Add:
issue: https://github.com/OpenEnergyPlatform/ontology/issues/1891
pull request: https://github.com/OpenEnergyPlatform/ontology/pull/1940",
        <http://purl.obolibrary.org/obo/IAO_0000115> "Wind farm area determination method is a methodology with the goal of identifying and quantifying the area suitable for wind farm development, based on topographical, environmental, and regulatory constraints.",
        rdfs:label "wind farm area determination method"@en
    
    SubClassOf: 
        OEO_00020166,
        <http://purl.obolibrary.org/obo/BFO_0000051> some OEO_00390033
    
    
Class: OEO_00390035

    Annotations: 
        OEO_00020426 "Add:
issue: https://github.com/OpenEnergyPlatform/ontology/issues/1891
pull request: https://github.com/OpenEnergyPlatform/ontology/pull/1940",
        <http://purl.obolibrary.org/obo/IAO_0000115> "Action specification for wind characteristics is an action specification that deals with wind characteristics.",
        rdfs:label "action specification for wind characteristics"@en
    
    SubClassOf: 
        <http://purl.obolibrary.org/obo/IAO_0000007>
    
    
Class: OEO_00390036

    Annotations: 
        OEO_00020426 "Add:
issue: https://github.com/OpenEnergyPlatform/ontology/issues/1891
pull request: https://github.com/OpenEnergyPlatform/ontology/pull/1940",
        <http://purl.obolibrary.org/obo/IAO_0000115> "Action specification for wind farm development area is an action specification that deals with available area for wind farm development.",
        rdfs:label "action specification for wind farm development area"@en
    
    SubClassOf: 
        <http://purl.obolibrary.org/obo/IAO_0000007>
    
    
Class: OEO_00390037

    Annotations: 
        OEO_00020426 "Add:
issue: https://github.com/OpenEnergyPlatform/ontology/issues/1891
pull request: https://github.com/OpenEnergyPlatform/ontology/pull/1940",
        <http://purl.obolibrary.org/obo/IAO_0000115> "Wind farm area determination process is a process that follows a determination methodology for available area to gain knowledge of the available area for wind farm development.",
        rdfs:label "wind farm area determination process"@en
    
    SubClassOf: 
        <http://purl.obolibrary.org/obo/BFO_0000015>,
        OEO_00390026 some OEO_00390034
    
    
Class: OEO_00390038

    Annotations: 
        OEO_00020426 "Add:
issue: https://github.com/OpenEnergyPlatform/ontology/issues/1891
pull request: https://github.com/OpenEnergyPlatform/ontology/pull/1940",
        <http://purl.obolibrary.org/obo/IAO_0000115> "Action specification for the technical wind potential of the available area is an action specification that deals with the technical wind potential of the available area.",
        rdfs:label "action specification for the technical wind potential"@en
    
    SubClassOf: 
        <http://purl.obolibrary.org/obo/IAO_0000007>
    
    
Class: OEO_00390039

    Annotations: 
        OEO_00020426 "Add:
issue: https://github.com/OpenEnergyPlatform/ontology/issues/1891
pull request: https://github.com/OpenEnergyPlatform/ontology/pull/1940",
        <http://purl.obolibrary.org/obo/IAO_0000115> "Select appropriate turbine types is an action specification that describes the process of choosing wind turbine models based on site-specific wind characteristics, hub height, and rotor diameter.",
        rdfs:label "select appropriate turbine types"@en
    
    SubClassOf: 
        OEO_00390038
    
    
Class: OEO_00390040

    Annotations: 
        OEO_00020426 "Add:
issue: https://github.com/OpenEnergyPlatform/ontology/issues/1891
pull request: https://github.com/OpenEnergyPlatform/ontology/pull/1940",
        <http://purl.obolibrary.org/obo/IAO_0000115> "Place turbines within area is an action specification that describes the definition of the spatial arrangement of wind turbines within the designated area, ensuring optimal positioning based on site characteristics and layout constraints.",
        rdfs:label "place turbines within area"@en
    
    SubClassOf: 
        OEO_00390038
    
    
Class: OEO_00390041

    Annotations: 
        OEO_00020426 "Add:
issue: https://github.com/OpenEnergyPlatform/ontology/issues/1891
pull request: https://github.com/OpenEnergyPlatform/ontology/pull/1940",
        <http://purl.obolibrary.org/obo/IAO_0000115> "Account for wake losses is an action specification that describes the inclusion of losses due to wind turbine wake effects, which reduce wind speed and energy yield behind turbines.",
        rdfs:label "account for wake losses"@en
    
    SubClassOf: 
        OEO_00390038
    
    
Class: OEO_00390042

    Annotations: 
        OEO_00020426 "Add:
issue: https://github.com/OpenEnergyPlatform/ontology/issues/1891
pull request: https://github.com/OpenEnergyPlatform/ontology/pull/1940",
        <http://purl.obolibrary.org/obo/IAO_0000115> "Determine annual energy yield is an action specification that describes how a turbine's power curve is combined with the wind speed distribution to calculate the expected annual energy production.",
        rdfs:label "determine annual energy yield"@en
    
    SubClassOf: 
        OEO_00390038
    
    
Class: OEO_00390043

    Annotations: 
        OEO_00020426 "Add:
issue: https://github.com/OpenEnergyPlatform/ontology/issues/1891
pull request: https://github.com/OpenEnergyPlatform/ontology/pull/1940",
        <http://purl.obolibrary.org/obo/IAO_0000115> "Determine capacity factor is an action specification that describes the calculation of the capacity factor (CF), which represents the ratio of actual energy output to the maximum possible output over a given time period.",
        rdfs:label "determine capacity factor"@en
    
    SubClassOf: 
        OEO_00390038
    
    
Class: OEO_00390044

    Annotations: 
        OEO_00020426 "Add:
issue: https://github.com/OpenEnergyPlatform/ontology/issues/1891
pull request: https://github.com/OpenEnergyPlatform/ontology/pull/1940",
        <http://purl.obolibrary.org/obo/IAO_0000115> "Calculate technical potential is an action specification that describes how the total energy production capability of the available area is determined, factoring in turbine placement, capacity density, and wake losses.",
        rdfs:label "calculate technical potential"@en
    
    SubClassOf: 
        OEO_00390038
    
    
Class: OEO_00390045

    Annotations: 
        OEO_00020426 "Add:
issue: https://github.com/OpenEnergyPlatform/ontology/issues/1891
pull request: https://github.com/OpenEnergyPlatform/ontology/pull/1940",
        <http://purl.obolibrary.org/obo/IAO_0000115> "Determined wind potential is an object specification that defines the goal of a methodology as a state of understanding the technical wind potential of the available area.",
        rdfs:label "determined wind potential"@en
    
    SubClassOf: 
        <http://purl.obolibrary.org/obo/IAO_0000005>
    
    
Class: OEO_00390046

    Annotations: 
        OEO_00020426 "Add:
issue: https://github.com/OpenEnergyPlatform/ontology/issues/1891
pull request: https://github.com/OpenEnergyPlatform/ontology/pull/1940",
        <http://purl.obolibrary.org/obo/IAO_0000115> "Wind potential determination method is a methodology with the goal of calculating the technical wind energy potential within the identified suitable area, considering turbine technology, placement, and energy yield factors.",
        rdfs:label "wind potential determination method"@en
    
    SubClassOf: 
        OEO_00020166,
        <http://purl.obolibrary.org/obo/BFO_0000051> some OEO_00390045
    
    
Class: OEO_00390047

    Annotations: 
        OEO_00020426 "Add:
issue: https://github.com/OpenEnergyPlatform/ontology/issues/1891
pull request: https://github.com/OpenEnergyPlatform/ontology/pull/1940",
        <http://purl.obolibrary.org/obo/IAO_0000115> "Wind potential determination processa is a process that follows a determination methodology for wind potential to gain knowledge of the technical wind potential of the available area.",
        rdfs:label "wind potential determination process"@en
    
    SubClassOf: 
        <http://purl.obolibrary.org/obo/BFO_0000015>,
        OEO_00390026 some OEO_00390046
    
    
Class: OEO_00390048

    Annotations: 
        OEO_00020426 "Add:
issue: https://github.com/OpenEnergyPlatform/ontology/issues/1891
pull request: https://github.com/OpenEnergyPlatform/ontology/pull/1940",
        <http://purl.obolibrary.org/obo/IAO_0000115> "Action specification for techno-economic potential is an action specification that deals with techno-economic potential.",
        rdfs:label "action specification for techno-economic potential"@en
    
    SubClassOf: 
        <http://purl.obolibrary.org/obo/IAO_0000007>
    
    
Class: OEO_00390049

    Annotations: 
        OEO_00020426 "Add;
issue: https://github.com/OpenEnergyPlatform/ontology/issues/1891
pull request: https://github.com/OpenEnergyPlatform/ontology/pull/1940",
        <http://purl.obolibrary.org/obo/IAO_0000115> "Determine wind turbine lifetime is an action specification that describes the process of estimating the operational lifespan of a wind turbine, based on design and site-specific conditions.",
        rdfs:label "determine wind turbine lifetime"@en
    
    SubClassOf: 
        OEO_00390048
    
    
Class: OEO_00390050

    Annotations: 
        OEO_00020426 "Add;
issue: https://github.com/OpenEnergyPlatform/ontology/issues/1891
pull request: https://github.com/OpenEnergyPlatform/ontology/pull/1940",
        <http://purl.obolibrary.org/obo/IAO_0000115> "Determine capital expenditures is an action specification that describes the calculation of capital expenditures (CAPEX) required for the installation of wind turbines and associated infrastructure.",
        rdfs:label "determine capital expenditures"@en
    
    SubClassOf: 
        OEO_00390048
    
    
Class: OEO_00390051

    Annotations: 
        OEO_00020426 "Add;
issue: https://github.com/OpenEnergyPlatform/ontology/issues/1891
pull request: https://github.com/OpenEnergyPlatform/ontology/pull/1940",
        <http://purl.obolibrary.org/obo/IAO_0000115> "Determine operational expenditures is an action specification that describes the estimation of ongoing operational expenditures (OPEX) for wind turbines, including routine maintenance and operational management. These include operating and maintenance costs.",
        rdfs:label "determine operational expenditures"@en
    
    SubClassOf: 
        OEO_00390048
    
    
Class: OEO_00390052

    Annotations: 
        OEO_00020426 "Add;
issue: https://github.com/OpenEnergyPlatform/ontology/issues/1891
pull request: https://github.com/OpenEnergyPlatform/ontology/pull/1940",
        <http://purl.obolibrary.org/obo/IAO_0000115> "Determine discount and interest rate is an action specification that describes the selection of financial discount and interest rates, which are used in the economic analysis to account for the time value of money.",
        rdfs:label "determine discount and interest rate"@en
    
    SubClassOf: 
        OEO_00390048
    
    
Class: OEO_00390053

    Annotations: 
        OEO_00020426 "Add;
issue: https://github.com/OpenEnergyPlatform/ontology/issues/1891
pull request: https://github.com/OpenEnergyPlatform/ontology/pull/1940",
        <http://purl.obolibrary.org/obo/IAO_0000115> "Calculate Levelized Cost of Energy is an action specification that describes the computation of the Levelized Cost of Energy (LCOE) either for individual turbines or for sub-regions within the study area by applying a cost model based on the previously calculated economic parameters and the capacity factors.",
        rdfs:label "calculate Levelized Cost of Energy"@en
    
    SubClassOf: 
        OEO_00390048
    
    
Class: OEO_00390054

    Annotations: 
        OEO_00020426 "Add;
issue: https://github.com/OpenEnergyPlatform/ontology/issues/1891
pull request: https://github.com/OpenEnergyPlatform/ontology/pull/1940",
        <http://purl.obolibrary.org/obo/IAO_0000115> "Calculate economic potential is an action specification that describes the determination of the total economic potential of the available area under a maximum threshold LCOE value.",
        rdfs:label "calculate economic potential"@en
    
    SubClassOf: 
        OEO_00390048
    
    
Class: OEO_00390055

    Annotations: 
        OEO_00020426 "Add:
issue: https://github.com/OpenEnergyPlatform/ontology/issues/1891
pull request: https://github.com/OpenEnergyPlatform/ontology/pull/1940",
        <http://purl.obolibrary.org/obo/IAO_0000115> "Determined techno-economic potential is an object specification that defines the goal of a methodology as a state of understanding the techno-economic potential of the available region.",
        rdfs:label "determined techno-economic potential"@en
    
    SubClassOf: 
        <http://purl.obolibrary.org/obo/IAO_0000005>
    
    
Class: OEO_00390056

    Annotations: 
        OEO_00020426 "Add;
issue: https://github.com/OpenEnergyPlatform/ontology/issues/1891
pull request: https://github.com/OpenEnergyPlatform/ontology/pull/1940",
        <http://purl.obolibrary.org/obo/IAO_0000115> "Techno-economic potential determination method is a methodology with the goal of assessing the economic viability of wind energy projects within the available area, based on the technical potential and incorporating cost factors and economic metrics.",
        rdfs:label "techno-economic potential determination method"@en
    
    SubClassOf: 
        OEO_00020166,
        <http://purl.obolibrary.org/obo/BFO_0000051> some OEO_00390055
    
    
Class: OEO_00390057

    Annotations: 
        OEO_00020426 "Add:
issue: https://github.com/OpenEnergyPlatform/ontology/issues/1891
pull request: https://github.com/OpenEnergyPlatform/ontology/pull/1940",
        <http://purl.obolibrary.org/obo/IAO_0000115> "Techno-economic potential determination process is a process that follows a determination methodology for techno-economic potental to gain knowledge of the techno-economic potential of the available region.",
        rdfs:label "techno-economic potential determination process"@en
    
    SubClassOf: 
        <http://purl.obolibrary.org/obo/BFO_0000015>,
        OEO_00390026 some OEO_00390056
    
    
Class: OEO_00390058

    Annotations: 
        OEO_00020426 "Add:
issue: https://github.com/OpenEnergyPlatform/ontology/issues/1891
pull request: https://github.com/OpenEnergyPlatform/ontology/pull/1940",
        <http://purl.obolibrary.org/obo/IAO_0000115> "Action specification for the feasible potential is an action specification that deals with the feasible potential of something.",
        rdfs:label "action specification for the feasible potential"@en
    
    SubClassOf: 
        <http://purl.obolibrary.org/obo/IAO_0000007>
    
    
Class: OEO_00390059

    Annotations: 
        OEO_00020426 "Add:
issue: https://github.com/OpenEnergyPlatform/ontology/issues/1891
pull request: https://github.com/OpenEnergyPlatform/ontology/pull/1940",
        <http://purl.obolibrary.org/obo/IAO_0000115> "Apply constraints for assessment of potential is an action specification that describes the process of integrating non-technical factors, such as social acceptance, land use regulations, or market conditions, into the potential assessment.",
        rdfs:label "apply constraints for assessment of potential"@en
    
    SubClassOf: 
        OEO_00390058
    
    
Class: OEO_00390060

    Annotations: 
        OEO_00020426 "Add:
issue: https://github.com/OpenEnergyPlatform/ontology/issues/1891
pull request: https://github.com/OpenEnergyPlatform/ontology/pull/1940",
        <http://purl.obolibrary.org/obo/IAO_0000115> "Calculate feasible potential is an action specification that describes the calculation of the feasible wind energy potential, considering both technical and socio-economic constraints.",
        rdfs:label "calculate feasible potential"@en
    
    SubClassOf: 
        OEO_00390058
    
    
Class: OEO_00390061

    Annotations: 
        OEO_00020426 "Add:
issue: https://github.com/OpenEnergyPlatform/ontology/issues/1891
pull request: https://github.com/OpenEnergyPlatform/ontology/pull/1940",
        <http://purl.obolibrary.org/obo/IAO_0000115> "Determined feasible potential is an object specification that defines the goal of a methodology as a state of understanding the feasible potential of something.",
        rdfs:label "determined feasible potential"@en
    
    SubClassOf: 
        <http://purl.obolibrary.org/obo/IAO_0000005>
    
    
Class: OEO_00390062

    Annotations: 
        OEO_00020426 "Add:
issue: https://github.com/OpenEnergyPlatform/ontology/issues/1891
pull request: https://github.com/OpenEnergyPlatform/ontology/pull/1940",
        <http://purl.obolibrary.org/obo/IAO_0000115> "Feasible potental determination method is a methodology with the goal of calculating the wind energy potential that remains after applying additional social, regulatory, or market constraints to the available region.",
        rdfs:label "feasible potental determination method"@en
    
    SubClassOf: 
        OEO_00020166,
        (<http://purl.obolibrary.org/obo/BFO_0000051> some OEO_00390059)
         and (<http://purl.obolibrary.org/obo/BFO_0000051> some OEO_00390060),
        <http://purl.obolibrary.org/obo/BFO_0000051> some OEO_00390061
    
    
Class: OEO_00390063

    Annotations: 
        OEO_00020426 "Add:
issue: https://github.com/OpenEnergyPlatform/ontology/issues/1891
pull request: https://github.com/OpenEnergyPlatform/ontology/pull/1940",
        <http://purl.obolibrary.org/obo/IAO_0000115> "Feasible potential determination process al is a process that follows a determination methodology for feasable potential to gain knowledge of the feasible potential of something.",
        rdfs:label "feasible potental determination process"@en
    
    SubClassOf: 
        <http://purl.obolibrary.org/obo/BFO_0000015>,
        OEO_00390026 some OEO_00390062
    
    
Class: OEO_00390066

    Annotations: 
        OEO_00020426 "Add:
issue: https://github.com/OpenEnergyPlatform/ontology/issues/1891
pull request: https://github.com/OpenEnergyPlatform/ontology/pull/1940",
        <http://purl.obolibrary.org/obo/IAO_0000115> "Determine capacity density is an action specification that describes the calculation of the installed capacity per unit area (MW per km²) by assessing the number and power rating of turbines within the available space.",
        rdfs:label "determine capacity density"@en
    
    SubClassOf: 
        OEO_00390038
    
    
