Prefix: : <http://openenergy-platform.org/ontology/oeo/>
Prefix: dc: <http://purl.org/dc/elements/1.1/>
Prefix: owl: <http://www.w3.org/2002/07/owl#>
Prefix: rdf: <http://www.w3.org/1999/02/22-rdf-syntax-ns#>
Prefix: rdfs: <http://www.w3.org/2000/01/rdf-schema#>
Prefix: skos: <http://www.w3.org/2004/02/skos/core#>
Prefix: xml: <http://www.w3.org/XML/1998/namespace>
Prefix: xsd: <http://www.w3.org/2001/XMLSchema#>



Ontology: <http://openenergy-platform.org/ontology/oeo/oeo-tasks/>
<http://openenergy-platform.org/ontology/oeo/dev/oeo-tasks.omn>
Import: <http://openenergy-platform.org/ontology/oeo/dev/oeo-shared.omn>

Annotations: 
    dc:description "The Open Energy Ontology is an ontology for all aspects of the energy modelling domain. The 'Tasks' module covers energy-related task definitions and their realization steps. It aims to identify steps taken in the scientific process of a certain domain.",
    dc:license "http://creativecommons.org/publicdomain/zero/1.0/",
    <http://purl.org/dc/terms/title> "Open Energy Ontology (Task module)"

AnnotationProperty: <http://purl.obolibrary.org/obo/IAO_0000115>

    
AnnotationProperty: <http://purl.org/dc/terms/title>

    
AnnotationProperty: OEO_00020426

    
AnnotationProperty: dc:description

    
AnnotationProperty: dc:license

    
AnnotationProperty: rdfs:label

    
Datatype: rdf:PlainLiteral

    
Datatype: xsd:string

    
ObjectProperty: <http://purl.obolibrary.org/obo/BFO_0000051>

    
ObjectProperty: <http://purl.obolibrary.org/obo/BFO_0000054>

    
ObjectProperty: <http://purl.obolibrary.org/obo/RO_0000056>

    
ObjectProperty: <http://purl.obolibrary.org/obo/RO_0000057>

    
ObjectProperty: OEO_00390026

    Annotations: 
        OEO_00020426 "Add:
issue: https://github.com/OpenEnergyPlatform/ontology/issues/1891
pull request: https://github.com/OpenEnergyPlatform/ontology/pull/1940",
        <http://purl.obolibrary.org/obo/IAO_0000115> "A relationship between a process and a plan specification, in which the process is predefined or planned by the process.",
        rdfs:label "structured by"@en
    
    SubPropertyOf: 
        <http://purl.obolibrary.org/obo/RO_0000057>
    
    Domain: 
        <http://purl.obolibrary.org/obo/BFO_0000015>
    
    Range: 
        <http://purl.obolibrary.org/obo/IAO_0000104>
    
    
ObjectProperty: owl:topObjectProperty

    
Class: <http://purl.obolibrary.org/obo/BFO_0000015>

    
Class: <http://purl.obolibrary.org/obo/BFO_0000017>

    
Class: <http://purl.obolibrary.org/obo/BFO_0000035>

    
Class: <http://purl.obolibrary.org/obo/IAO_0000005>

    
Class: <http://purl.obolibrary.org/obo/IAO_0000007>

    
Class: <http://purl.obolibrary.org/obo/IAO_0000104>

    
Class: OEO_00020166

    
Class: OEO_00390002

    Annotations: 
        OEO_00020426 "Add:
issue: https://github.com/OpenEnergyPlatform/ontology/issues/1891
pull request: https://github.com/OpenEnergyPlatform/ontology/pull/1940",
        <http://purl.obolibrary.org/obo/IAO_0000115> "Determination method for wind characteristics of a region is a methodology with the goal to understand the specific wind characteristics of a predefined region, encompassing data acquisition, modelling, and analytical procedures",
        rdfs:label "determination method for wind characteristics of a region"@en
    
    SubClassOf: 
        OEO_00020166,
        <http://purl.obolibrary.org/obo/BFO_0000051> some OEO_00390004
    
    
Class: OEO_00390003

    Annotations: 
        OEO_00020426 "Add:
issue: https://github.com/OpenEnergyPlatform/ontology/issues/1891
pull request: https://github.com/OpenEnergyPlatform/ontology/pull/1940",
        <http://purl.obolibrary.org/obo/IAO_0000115> "Data acquisition and pre-processing is an action specification that describes the steps the bearer takes to acquire raw data and how this data is cleaned, transformed, and structured for subsequent analysis.",
        rdfs:label "data acquisition and pre-processing"@en
    
    SubClassOf: 
        OEO_00390035
    
    
Class: OEO_00390004

    Annotations: 
        OEO_00020426 "Add:
issue: https://github.com/OpenEnergyPlatform/ontology/issues/1891
pull request: https://github.com/OpenEnergyPlatform/ontology/pull/1940",
        <http://purl.obolibrary.org/obo/IAO_0000115> "Determined wind characteristics of a region is an object specification that defines the goal of a process as a state of understanding the specific wind characteristics of a predefined region.",
        rdfs:label "determined wind characteristics of a region"@en
    
    SubClassOf: 
        <http://purl.obolibrary.org/obo/IAO_0000005>
    
    
Class: OEO_00390005

    Annotations: 
        OEO_00020426 "Add:
issue: https://github.com/OpenEnergyPlatform/ontology/issues/1891
pull request: https://github.com/OpenEnergyPlatform/ontology/pull/1940",
        <http://purl.obolibrary.org/obo/IAO_0000115> "Extrapolate wind speed vertically to hub height is an action specification that describes how wind speed at the hub height of a wind turbine is inferred from measurements taken at a different height.",
        rdfs:label "extrapolate wind speed vertically to hub height"@en
    
    SubClassOf: 
        OEO_00390035
    
    
Class: OEO_00390007

    Annotations: 
        OEO_00020426 "Add:
issue: https://github.com/OpenEnergyPlatform/ontology/issues/1891
pull request: https://github.com/OpenEnergyPlatform/ontology/pull/1940",
        <http://purl.obolibrary.org/obo/IAO_0000115> "Determination process for wind characteristics of a region is a process that follows some kind of methodology to gain knowledge of the specific wind characteristics of a predefined region.",
        rdfs:label "determination process for wind characteristics of a region"@en
    
    SubClassOf: 
        <http://purl.obolibrary.org/obo/BFO_0000015>,
        OEO_00390026 some OEO_00390002
    
    
Class: OEO_00390014

    Annotations: 
        OEO_00020426 "Add:
issue: https://github.com/OpenEnergyPlatform/ontology/issues/1891
pull request: https://github.com/OpenEnergyPlatform/ontology/pull/1940",
        <http://purl.obolibrary.org/obo/IAO_0000115> "Account for air density change is an action specification that describes how variations in air density due to changes in altitude, temperature, and pressure are incorporated into the wind resource calculations.",
        rdfs:label "account for air density change"@en
    
    SubClassOf: 
        OEO_00390035
    
    
Class: OEO_00390015

    Annotations: 
        OEO_00020426 "Add:
issue: https://github.com/OpenEnergyPlatform/ontology/issues/1891
pull request: https://github.com/OpenEnergyPlatform/ontology/pull/1940",
        <http://purl.obolibrary.org/obo/IAO_0000115> "Determine wind speed frequency distribution is an action specification that describes the process of calculating the frequency of different wind speed intervals over a set period.",
        rdfs:label "determine wind speed frequency distribution"@en
    
    SubClassOf: 
        OEO_00390035
    
    
Class: OEO_00390016

    Annotations: 
        OEO_00020426 "Add:
issue: https://github.com/OpenEnergyPlatform/ontology/issues/1891
pull request: https://github.com/OpenEnergyPlatform/ontology/pull/1940",
        <http://purl.obolibrary.org/obo/IAO_0000115> "Determine seasonal/diurnal variability is an action specification that describes the process of identifying variations in wind characteristics across different seasons and times of day.",
        rdfs:label "determine seasonal/diurnal variability"@en
    
    SubClassOf: 
        OEO_00390035
    
    
Class: OEO_00390017

    Annotations: 
        OEO_00020426 "Add:
issue: https://github.com/OpenEnergyPlatform/ontology/issues/1891
pull request: https://github.com/OpenEnergyPlatform/ontology/pull/1940",
        <http://purl.obolibrary.org/obo/IAO_0000115> "Determine the theoretical potential / WPD is an action specification that describes how Wind Power Density (WPD) is calculated to estimate the theoretical wind power potential based on wind speed and air density.",
        rdfs:label "determine the theoretical potential / WPD"@en
    
    SubClassOf: 
        OEO_00390035
    
    
Class: OEO_00390027

    Annotations: 
        OEO_00020426 "Add:
issue: https://github.com/OpenEnergyPlatform/ontology/issues/1891
pull request: https://github.com/OpenEnergyPlatform/ontology/pull/1940",
        <http://purl.obolibrary.org/obo/IAO_0000115> "Interpolate wind data to greater resolution horizontally is an action specification that describes the process of increasing the spatial resolution of wind data across a region to provide finer detail for wind resource assessment",
        rdfs:label "interpolate wind data to greater resolution horizontally"@en
    
    SubClassOf: 
        OEO_00390036
    
    
Class: OEO_00390028

    Annotations: 
        OEO_00020426 "Add:
issue: https://github.com/OpenEnergyPlatform/ontology/issues/1891
pull request: https://github.com/OpenEnergyPlatform/ontology/pull/1940",
        <http://purl.obolibrary.org/obo/IAO_0000115> "Select exclusion criteria and buffer distances is an action specification that describes the process of defining physical, environmental, and regulatory criteria that exclude areas from wind farm development, along with the application of buffer zones",
        rdfs:label "select exclusion criteria and buffer distances"@en
    
    SubClassOf: 
        OEO_00390036
    
    
Class: OEO_00390029

    Annotations: 
        OEO_00020426 "Add:
issue: https://github.com/OpenEnergyPlatform/ontology/issues/1891
pull request: https://github.com/OpenEnergyPlatform/ontology/pull/1940",
        <http://purl.obolibrary.org/obo/IAO_0000115> "Acquisition and processing datasets for exclusion criteria is an action specification that describes the steps involved in obtaining and preparing datasets that represent exclusion zones for wind farm development, based on predefined criteria.",
        rdfs:label "acquisition and processing datasets for exclusion criteria"@en
    
    SubClassOf: 
        OEO_00390036
    
    
Class: OEO_00390030

    Annotations: 
        OEO_00020426 "Add:
issue: https://github.com/OpenEnergyPlatform/ontology/issues/1891
pull request: https://github.com/OpenEnergyPlatform/ontology/pull/1940",
        <http://purl.obolibrary.org/obo/IAO_0000115> "Determine MCDA approach for soft exclusion criteria is an action specification that describes how a Multi-Criteria Decision Analysis (MCDA) method is applied to areas where exclusions are not absolute, allowing for weighted decision-making",
        rdfs:label "determine MCDA approach for soft exclusion criteria"@en
    
    SubClassOf: 
        OEO_00390036
    
    
Class: OEO_00390031

    Annotations: 
        OEO_00020426 "Add:
issue: https://github.com/OpenEnergyPlatform/ontology/issues/1891
pull request: https://github.com/OpenEnergyPlatform/ontology/pull/1940",
        <http://purl.obolibrary.org/obo/IAO_0000115> "Determine area for development is an action specification that describes the identification of potential areas where wind farm development is feasible, by iteratively excluding non-available areas based on the processed data and exclusion criteria",
        rdfs:label "determine area for development"@en
    
    SubClassOf: 
        OEO_00390036
    
    
Class: OEO_00390032

    Annotations: 
        OEO_00020426 "Add:
issue: https://github.com/OpenEnergyPlatform/ontology/issues/1891
pull request: https://github.com/OpenEnergyPlatform/ontology/pull/1940",
        <http://purl.obolibrary.org/obo/IAO_0000115> "Determine geographical potential is an action specification that describes the calculation of the total geographical area available for wind farm development after applying exclusion criteria and considering spatial constraints",
        rdfs:label "determine geographical potential"@en
    
    SubClassOf: 
        OEO_00390036
    
    
Class: OEO_00390033

    Annotations: 
        OEO_00020426 "Add:
issue: https://github.com/OpenEnergyPlatform/ontology/issues/1891
pull request: https://github.com/OpenEnergyPlatform/ontology/pull/1940",
        <http://purl.obolibrary.org/obo/IAO_0000115> "Determined available area for wind farm development is an object specification that defines the goal of a process as a state of understanding the available area for wind farm development.",
        rdfs:label "determined available area for wind farm development"@en
    
    SubClassOf: 
        <http://purl.obolibrary.org/obo/IAO_0000005>
    
    
Class: OEO_00390034

    Annotations: 
        OEO_00020426 "Add:
issue: https://github.com/OpenEnergyPlatform/ontology/issues/1891
pull request: https://github.com/OpenEnergyPlatform/ontology/pull/1940",
        <http://purl.obolibrary.org/obo/IAO_0000115> "Determination method for the available area for wind farm development is a  methodology with the goal of identifying and quantifying the area suitable for wind farm development, based on topographical, environmental, and regulatory constraints",
        rdfs:label "determination method for the available area for wind farm development"@en
    
    SubClassOf: 
        OEO_00020166,
        <http://purl.obolibrary.org/obo/BFO_0000051> some OEO_00390033
    
    
Class: OEO_00390035

    Annotations: 
        OEO_00020426 "Add:
issue: https://github.com/OpenEnergyPlatform/ontology/issues/1891
pull request: https://github.com/OpenEnergyPlatform/ontology/pull/1940",
        <http://purl.obolibrary.org/obo/IAO_0000115> "Action specification for wind characteristics is an action specification that deals with wind characteristics",
        rdfs:label "action specification for wind characteristics"@en
    
    SubClassOf: 
        <http://purl.obolibrary.org/obo/IAO_0000007>
    
    
Class: OEO_00390036

    Annotations: 
        OEO_00020426 "Add:
issue: https://github.com/OpenEnergyPlatform/ontology/issues/1891
pull request: https://github.com/OpenEnergyPlatform/ontology/pull/1940",
        <http://purl.obolibrary.org/obo/IAO_0000115> "Action specification for available area for wind farm development is an action specification that deals with available area for wind farm development",
        rdfs:label "action specification for available area for wind farm development"@en
    
    SubClassOf: 
        <http://purl.obolibrary.org/obo/IAO_0000007>
    
    
Class: OEO_00390037

    Annotations: 
        OEO_00020426 "Add:
issue: https://github.com/OpenEnergyPlatform/ontology/issues/1891
pull request: https://github.com/OpenEnergyPlatform/ontology/pull/1940",
        <http://purl.obolibrary.org/obo/IAO_0000115> "Determination process for the available area for wind farm development is a process that follows some kind of methodology to gain knowledge of the available area for wind farm development.",
        rdfs:label "determination process for the available area for wind farm development"@en
    
    SubClassOf: 
        <http://purl.obolibrary.org/obo/BFO_0000015>,
        OEO_00390026 some OEO_00390034
    
    
Class: OEO_00390038

    Annotations: 
        OEO_00020426 "Add:
issue: https://github.com/OpenEnergyPlatform/ontology/issues/1891
pull request: https://github.com/OpenEnergyPlatform/ontology/pull/1940",
        <http://purl.obolibrary.org/obo/IAO_0000115> "Action specification for the technical wind potential of the available area is an action specification that deals with the technical wind potential of the available area",
        rdfs:label "action specification for for the technical wind potential"@en
    
    SubClassOf: 
        <http://purl.obolibrary.org/obo/IAO_0000007>
    
    
Class: OEO_00390039

    Annotations: 
        OEO_00020426 "Add:
issue: https://github.com/OpenEnergyPlatform/ontology/issues/1891
pull request: https://github.com/OpenEnergyPlatform/ontology/pull/1940",
        <http://purl.obolibrary.org/obo/IAO_0000115> "Select appropriate turbine type(s) is an action specification that describes the process of choosing wind turbine models based on site-specific wind characteristics, hub height, and rotor diameter.",
        rdfs:label "select appropriate turbine type(s)"@en
    
    SubClassOf: 
        OEO_00390038
    
    
Class: OEO_00390040

    Annotations: 
        OEO_00020426 "Add:
issue: https://github.com/OpenEnergyPlatform/ontology/issues/1891
pull request: https://github.com/OpenEnergyPlatform/ontology/pull/1940",
        <http://purl.obolibrary.org/obo/IAO_0000115> "Place turbines in area or determine capacity density is an action specification that describes how turbines are spatially distributed within the available area, or how the capacity density (MW per unit area) is calculated.",
        rdfs:label "place turbines in area or determine capacity density"@en
    
    SubClassOf: 
        OEO_00390038
    
    
Class: OEO_00390041

    Annotations: 
        OEO_00020426 "Add:
issue: https://github.com/OpenEnergyPlatform/ontology/issues/1891
pull request: https://github.com/OpenEnergyPlatform/ontology/pull/1940",
        <http://purl.obolibrary.org/obo/IAO_0000115> "Account for wake losses is an action specification that describes the inclusion of losses due to wind turbine wake effects, which reduce wind speed and energy yield behind turbines.",
        rdfs:label "account for wake losses"@en
    
    SubClassOf: 
        OEO_00390038
    
    
Class: OEO_00390042

    Annotations: 
        OEO_00020426 "Add:
issue: https://github.com/OpenEnergyPlatform/ontology/issues/1891
pull request: https://github.com/OpenEnergyPlatform/ontology/pull/1940",
        <http://purl.obolibrary.org/obo/IAO_0000115> "Use power curve with wind distribution function to determine annual energy yield is an action specification that describes how a turbine's power curve is combined with the wind speed distribution to calculate the expected annual energy production.",
        rdfs:label "use power curve with wind distribution function to determine annual energy yield"@en
    
    SubClassOf: 
        OEO_00390038
    
    
Class: OEO_00390043

    Annotations: 
        OEO_00020426 "Add:
issue: https://github.com/OpenEnergyPlatform/ontology/issues/1891
pull request: https://github.com/OpenEnergyPlatform/ontology/pull/1940",
        <http://purl.obolibrary.org/obo/IAO_0000115> "Determine capacity factor (CF) is an action specification that describes the calculation of the capacity factor, which represents the ratio of actual energy output to the maximum possible output over a given time period.",
        rdfs:label "determine capacity factor (CF)"@en
    
    SubClassOf: 
        OEO_00390038
    
    
Class: OEO_00390044

    Annotations: 
        OEO_00020426 "Add:
issue: https://github.com/OpenEnergyPlatform/ontology/issues/1891
pull request: https://github.com/OpenEnergyPlatform/ontology/pull/1940",
        <http://purl.obolibrary.org/obo/IAO_0000115> "Calculate technical potential is an action specification that describes how the total energy production capability of the available area is determined, factoring in turbine placement, capacity density, and wake losses.",
        rdfs:label "calculate technical potential"@en
    
    SubClassOf: 
        OEO_00390038
    
    
Class: OEO_00390045

    Annotations: 
        OEO_00020426 "Add:
issue: https://github.com/OpenEnergyPlatform/ontology/issues/1891
pull request: https://github.com/OpenEnergyPlatform/ontology/pull/1940",
        <http://purl.obolibrary.org/obo/IAO_0000115> "Determined the technical wind potential of the available area is an object specification that defines the goal of a process as a state of understanding the technical wind potential of the available area",
        rdfs:label "determined the technical wind potential of the available area"@en
    
    SubClassOf: 
        <http://purl.obolibrary.org/obo/IAO_0000005>
    
    
Class: OEO_00390046

    Annotations: 
        OEO_00020426 "Add:
issue: https://github.com/OpenEnergyPlatform/ontology/issues/1891
pull request: https://github.com/OpenEnergyPlatform/ontology/pull/1940",
        <http://purl.obolibrary.org/obo/IAO_0000115> "Determination method for the technical wind potential of the available area is a methodology with the goal of calculating the technical wind energy potential within the identified suitable area, considering turbine technology, placement, and energy yield factors.",
        rdfs:label "determination method for the technical wind potential of the available area"@en
    
    SubClassOf: 
        OEO_00020166,
        <http://purl.obolibrary.org/obo/BFO_0000051> some OEO_00390045
    
    
Class: OEO_00390047

    Annotations: 
        OEO_00020426 "Add:
issue: https://github.com/OpenEnergyPlatform/ontology/issues/1891
pull request: https://github.com/OpenEnergyPlatform/ontology/pull/1940",
        <http://purl.obolibrary.org/obo/IAO_0000115> "Determination process for the technical wind potential of the available area is a process that follows some kind of methodology to gain knowledge of the technical wind potential of the available area",
        rdfs:label "determination process for the technical wind potential of the available area"@en
    
    SubClassOf: 
        <http://purl.obolibrary.org/obo/BFO_0000015>,
        OEO_00390026 some OEO_00390046
    
    
Class: OEO_00390048

    Annotations: 
        OEO_00020426 "Add:
issue: https://github.com/OpenEnergyPlatform/ontology/issues/1891
pull request: https://github.com/OpenEnergyPlatform/ontology/pull/1940",
        <http://purl.obolibrary.org/obo/IAO_0000115> "Action specification for techno-economic potential is an action specification that deals with techno-economic potential",
        rdfs:label "action specification for techno-economic potential"@en
    
    SubClassOf: 
        <http://purl.obolibrary.org/obo/IAO_0000007>
    
    
Class: OEO_00390049

    Annotations: 
        OEO_00020426 "Add;
issue: https://github.com/OpenEnergyPlatform/ontology/issues/1891
pull request: https://github.com/OpenEnergyPlatform/ontology/pull/1940",
        <http://purl.obolibrary.org/obo/IAO_0000115> "Determine wind turbine lifetime is an action specification that describes the process of estimating the operational lifespan of a wind turbine, based on design and site-specific conditions.",
        rdfs:label "determine wind turbine lifetime"@en
    
    SubClassOf: 
        OEO_00390048
    
    
Class: OEO_00390050

    Annotations: 
        OEO_00020426 "Add;
issue: https://github.com/OpenEnergyPlatform/ontology/issues/1891
pull request: https://github.com/OpenEnergyPlatform/ontology/pull/1940",
        <http://purl.obolibrary.org/obo/IAO_0000115> "Determine investment costs is an action specification that describes the calculation of capital expenditures (CAPEX) required for the installation of wind turbines and associated infrastructure.",
        rdfs:label "determine investment costs"@en
    
    SubClassOf: 
        OEO_00390048
    
    
Class: OEO_00390051

    Annotations: 
        OEO_00020426 "Add;
issue: https://github.com/OpenEnergyPlatform/ontology/issues/1891
pull request: https://github.com/OpenEnergyPlatform/ontology/pull/1940",
        <http://purl.obolibrary.org/obo/IAO_0000115> "Determine operating and maintenance costs is an action specification that describes the estimation of ongoing operational expenditures (OPEX) for wind turbines, including routine maintenance and operational management.",
        rdfs:label "determine operating and maintenance costs"@en
    
    SubClassOf: 
        OEO_00390048
    
    
Class: OEO_00390052

    Annotations: 
        OEO_00020426 "Add;
issue: https://github.com/OpenEnergyPlatform/ontology/issues/1891
pull request: https://github.com/OpenEnergyPlatform/ontology/pull/1940",
        <http://purl.obolibrary.org/obo/IAO_0000115> "Determine discount & interest rate is an action specification that describes the selection of financial discount and interest rates, which are used in the economic analysis to account for the time value of money.",
        rdfs:label "determine discount & interest rate"@en
    
    SubClassOf: 
        OEO_00390048
    
    
Class: OEO_00390053

    Annotations: 
        OEO_00020426 "Add;
issue: https://github.com/OpenEnergyPlatform/ontology/issues/1891
pull request: https://github.com/OpenEnergyPlatform/ontology/pull/1940",
        <http://purl.obolibrary.org/obo/IAO_0000115> "Calculate Levelized Cost of Energy is an action specification that describes the computation of the Levelized Cost of Energy (LCOE) either for individual turbines or for sub-regions within the study area by applying a cost model based on the previously calculated economic parameters and the capacity factors.",
        rdfs:label "calculate Levelized Cost of Energy (LCOE)"@en
    
    SubClassOf: 
        OEO_00390048
    
    
Class: OEO_00390054

    Annotations: 
        OEO_00020426 "Add;
issue: https://github.com/OpenEnergyPlatform/ontology/issues/1891
pull request: https://github.com/OpenEnergyPlatform/ontology/pull/1940",
        <http://purl.obolibrary.org/obo/IAO_0000115> "Calculate economic potential for LCOE range is an action specification that describes the determination of the total economic potential of the available area under a maximum threshold LCOE value.",
        rdfs:label "calculate economic potential for LCOE range"@en
    
    SubClassOf: 
        OEO_00390048
    
    
Class: OEO_00390055

    Annotations: 
        OEO_00020426 "Add:
issue: https://github.com/OpenEnergyPlatform/ontology/issues/1891
pull request: https://github.com/OpenEnergyPlatform/ontology/pull/1940",
        <http://purl.obolibrary.org/obo/IAO_0000115> "Determined the techno-economic potential of the available region is an object specification that defines the goal of a process as a state of understanding the techno-economic potential of the available region",
        rdfs:label "determined the techno-economic potential of the available region"@en
    
    SubClassOf: 
        <http://purl.obolibrary.org/obo/IAO_0000005>
    
    
Class: OEO_00390056

    Annotations: 
        OEO_00020426 "Add;
issue: https://github.com/OpenEnergyPlatform/ontology/issues/1891
pull request: https://github.com/OpenEnergyPlatform/ontology/pull/1940",
        <http://purl.obolibrary.org/obo/IAO_0000115> "Determination method for the techno-economic potential of the available region is a methodology with the goal of assessing the economic viability of wind energy projects within the available area, based on the technical potential and incorporating cost factors and economic metrics.",
        rdfs:label "determination method for the techno-economic potential of the available region"@en
    
    SubClassOf: 
        OEO_00020166,
        <http://purl.obolibrary.org/obo/BFO_0000051> some OEO_00390055
    
    
Class: OEO_00390057

    Annotations: 
        OEO_00020426 "Add:
issue: https://github.com/OpenEnergyPlatform/ontology/issues/1891
pull request: https://github.com/OpenEnergyPlatform/ontology/pull/1940",
        <http://purl.obolibrary.org/obo/IAO_0000115> "Determination process for the techno-economic potential of the available regiont is a process that follows some kind of methodology to gain knowledge of the techno-economic potential of the available region",
        rdfs:label "determination process for the techno-economic potential of the available region"@en
    
    SubClassOf: 
        <http://purl.obolibrary.org/obo/BFO_0000015>,
        OEO_00390026 some OEO_00390056
    
    
Class: OEO_00390058

    Annotations: 
        OEO_00020426 "Add:
issue: https://github.com/OpenEnergyPlatform/ontology/issues/1891
pull request: https://github.com/OpenEnergyPlatform/ontology/pull/1940",
        <http://purl.obolibrary.org/obo/IAO_0000115> "Action specification for the feasible potential is an action specification that deals with the feasible potential of something",
        rdfs:label "action specification for the feasible potential"@en
    
    SubClassOf: 
        <http://purl.obolibrary.org/obo/IAO_0000007>
    
    
Class: OEO_00390059

    Annotations: 
        OEO_00020426 "Add:
issue: https://github.com/OpenEnergyPlatform/ontology/issues/1891
pull request: https://github.com/OpenEnergyPlatform/ontology/pull/1940",
        <http://purl.obolibrary.org/obo/IAO_0000115> "Apply additional social/market constraints is an action specification that describes the process of integrating non-technical factors, such as social acceptance, land use regulations, or market conditions, into the potential assessment.",
        rdfs:label "apply additional social/market constraints"@en
    
    SubClassOf: 
        OEO_00390058
    
    
Class: OEO_00390060

    Annotations: 
        OEO_00020426 "Add:
issue: https://github.com/OpenEnergyPlatform/ontology/issues/1891
pull request: https://github.com/OpenEnergyPlatform/ontology/pull/1940",
        <http://purl.obolibrary.org/obo/IAO_0000115> "Calculate feasible potential for the region is an action specification that describes the calculation of the feasible wind energy potential, considering both technical and socio-economic constraints.",
        rdfs:label "calculate feasible potential for the region"@en
    
    SubClassOf: 
        OEO_00390058
    
    
Class: OEO_00390061

    Annotations: 
        OEO_00020426 "Add:
issue: https://github.com/OpenEnergyPlatform/ontology/issues/1891
pull request: https://github.com/OpenEnergyPlatform/ontology/pull/1940",
        <http://purl.obolibrary.org/obo/IAO_0000115> "Determined the feasible potential is an object specification that defines the goal of a process as a state of understanding the the feasible potential of something",
        rdfs:label "determined feasible potential"@en
    
    SubClassOf: 
        <http://purl.obolibrary.org/obo/IAO_0000005>
    
    
Class: OEO_00390062

    Annotations: 
        OEO_00020426 "Add:
issue: https://github.com/OpenEnergyPlatform/ontology/issues/1891
pull request: https://github.com/OpenEnergyPlatform/ontology/pull/1940",
        <http://purl.obolibrary.org/obo/IAO_0000115> "Determination method for the feasible potential is a methodology with the goal of calculating the wind energy potential that remains after applying additional social, regulatory, or market constraints to the available region.",
        rdfs:label "determination method for the feasible potential"@en
    
    SubClassOf: 
        OEO_00020166,
        (<http://purl.obolibrary.org/obo/BFO_0000051> some OEO_00390059)
         and (<http://purl.obolibrary.org/obo/BFO_0000051> some OEO_00390060),
        <http://purl.obolibrary.org/obo/BFO_0000051> some OEO_00390061
    
    
Class: OEO_00390063

    Annotations: 
        OEO_00020426 "Add:
issue: https://github.com/OpenEnergyPlatform/ontology/issues/1891
pull request: https://github.com/OpenEnergyPlatform/ontology/pull/1940",
        <http://purl.obolibrary.org/obo/IAO_0000115> "Determination process for the feasible potential is a process that follows some kind of methodology to gain knowledge of the feasible potential of something",
        rdfs:label "determination process for the feasible potential"@en
    
    SubClassOf: 
        <http://purl.obolibrary.org/obo/BFO_0000015>,
        OEO_00390026 some OEO_00390062
    
    
