Prefix: : <http://openenergy-platform.org/ontology/oeo/>
Prefix: dc: <http://purl.org/dc/elements/1.1/>
Prefix: owl: <http://www.w3.org/2002/07/owl#>
Prefix: rdf: <http://www.w3.org/1999/02/22-rdf-syntax-ns#>
Prefix: rdfs: <http://www.w3.org/2000/01/rdf-schema#>
Prefix: xml: <http://www.w3.org/XML/1998/namespace>
Prefix: xsd: <http://www.w3.org/2001/XMLSchema#>



Ontology: <http://openenergy-platform.org/ontology/oeo/oeo-model/>
<http://openenergy-platform.org/ontology/oeo/dev/oeo-model.omn>
Import: <http://openenergy-platform.org/ontology/oeo/dev/oeo-shared.omn>

Annotations: 
    dc:description "The Open Energy Ontology is an ontology for all aspects of the energy modelling domain. The 'Model' module covers entities for models, assumptions, parameters, data, software and all the processes that transform these, including model execution and data transformation.",
    <http://purl.org/dc/terms/license> "http://creativecommons.org/publicdomain/zero/1.0/",
    <http://purl.org/dc/terms/title> "Open Energy Ontology (Modelling module)"

AnnotationProperty: <http://purl.obolibrary.org/obo/IAO_0000112>

    
AnnotationProperty: <http://purl.obolibrary.org/obo/IAO_0000115>

    
AnnotationProperty: <http://purl.obolibrary.org/obo/IAO_0000116>

    
AnnotationProperty: <http://purl.obolibrary.org/obo/IAO_0000118>

    
AnnotationProperty: <http://purl.obolibrary.org/obo/IAO_0000119>

    
AnnotationProperty: <http://purl.obolibrary.org/obo/IAO_0000233>

    
AnnotationProperty: <http://purl.obolibrary.org/obo/IAO_0006011>

    
AnnotationProperty: <http://purl.org/dc/terms/license>

    
AnnotationProperty: <http://purl.org/dc/terms/title>

    
AnnotationProperty: OEO_00140170

    Annotations: 
        <http://purl.obolibrary.org/obo/IAO_0000115> "Has documentation quality is the relation between a model and a statement about how well it is documented.",
        <http://purl.obolibrary.org/obo/IAO_0000233> "issue: https://github.com/OpenEnergyPlatform/ontology/issues/526
pull request: https://github.com/OpenEnergyPlatform/ontology/pull/825",
        rdfs:label "has documentation quality"@en
    
    Domain: 
        <http://openenergy-platform.org/ontology/oeo/OEO_00000274>
    
    
AnnotationProperty: dc:contributor

    
AnnotationProperty: dc:description

    
AnnotationProperty: rdfs:comment

    
AnnotationProperty: rdfs:isDefinedBy

    
AnnotationProperty: rdfs:label

    
Datatype: rdf:PlainLiteral

    
Datatype: xsd:integer

    
Datatype: xsd:string

    
ObjectProperty: <http://purl.obolibrary.org/obo/BFO_0000050>

    
ObjectProperty: <http://purl.obolibrary.org/obo/BFO_0000051>

    
ObjectProperty: <http://purl.obolibrary.org/obo/IAO_0000136>

    
ObjectProperty: <http://purl.obolibrary.org/obo/RO_0000057>

    
ObjectProperty: <http://purl.obolibrary.org/obo/RO_0000087>

    
ObjectProperty: <http://purl.obolibrary.org/obo/RO_0002233>

    
ObjectProperty: <http://purl.obolibrary.org/obo/RO_0002234>

    
ObjectProperty: <http://purl.obolibrary.org/obo/RO_0002353>

    
ObjectProperty: OEO_00000503

    
ObjectProperty: OEO_00000504

    
ObjectProperty: OEO_00000506

    
ObjectProperty: OEO_00000507

    
ObjectProperty: OEO_00000508

    
ObjectProperty: OEO_00000510

    
ObjectProperty: OEO_00000511

    Annotations: 
        <http://purl.obolibrary.org/obo/IAO_0000115> "A relation that holds between an optimisation and its objective function or objective variable."@en,
        <http://purl.obolibrary.org/obo/IAO_0000233> "correct spelling optimisation and add range 'objective variable'
issue: https://github.com/OpenEnergyPlatform/ontology/issues/848
pull request: https://github.com/OpenEnergyPlatform/ontology/pull/878",
        rdfs:label "has objective"@en
    
    Domain: 
        OEO_00000313
    
    Range: 
        OEO_00000304 or OEO_00240004
    
    
ObjectProperty: OEO_00000512

    Annotations: 
        <http://purl.obolibrary.org/obo/IAO_0000115> "A relation that holds between an optimisation and its objective function."@en,
        rdfs:label "has objective function"@en
    
    SubPropertyOf: 
        OEO_00000511
    
    Domain: 
        OEO_00000313
    
    Range: 
        OEO_00000304
    
    
ObjectProperty: OEO_00000513

    Annotations: 
        <http://purl.obolibrary.org/obo/IAO_0000115> "A relation that holds between an optimisation and its objective variable."@en,
        <http://purl.obolibrary.org/obo/IAO_0000233> "add range 'objective variable'
issue: https://github.com/OpenEnergyPlatform/ontology/issues/848
pull request: https://github.com/OpenEnergyPlatform/ontology/pull/878",
        rdfs:label "has objective variable"@en
    
    SubPropertyOf: 
        OEO_00000511
    
    Domain: 
        OEO_00000313
    
    Range: 
        OEO_00240004
    
    
ObjectProperty: OEO_00000514

    Annotations: 
        <http://purl.obolibrary.org/obo/IAO_0000115> "A relation that holds between a data set and the resolution it depicts."@en,
        <http://purl.obolibrary.org/obo/IAO_0000233> "issue https://github.com/OpenEnergyPlatform/ontology/issues/622
Pull request https://github.com/OpenEnergyPlatform/ontology/pull/626
rework
issue https://github.com/OpenEnergyPlatform/ontology/issues/849
Pull request https://github.com/OpenEnergyPlatform/ontology/pull/912
add domain and range
Pull request https://github.com/OpenEnergyPlatform/ontology/pull/972
rework module structure 
issue: https://github.com/OpenEnergyPlatform/ontology/issues/1592
pull request: https://github.com/OpenEnergyPlatform/ontology/pull/1652",
        rdfs:label "has resolution"@en
    
    Domain: 
        <http://purl.obolibrary.org/obo/IAO_0000100>
    
    Range: 
        OEO_00020121
    
    
ObjectProperty: OEO_00000515

    Annotations: 
        <http://purl.obolibrary.org/obo/IAO_0000115> "A relation between a data set and the spatial resolution it uses."@en,
        <http://purl.obolibrary.org/obo/IAO_0000233> "issue https://github.com/OpenEnergyPlatform/ontology/issues/622
Pull request https://github.com/OpenEnergyPlatform/ontology/pull/626
def and axioms
Pull request https://github.com/OpenEnergyPlatform/ontology/pull/912
add domain and range
Pull request https://github.com/OpenEnergyPlatform/ontology/pull/972
rework module structure 
issue: https://github.com/OpenEnergyPlatform/ontology/issues/1592
pull request: https://github.com/OpenEnergyPlatform/ontology/pull/1652",
        rdfs:label "has spatial resolution"@en
    
    SubPropertyOf: 
        OEO_00000514
    
    Domain: 
        <http://purl.obolibrary.org/obo/IAO_0000100>
    
    Range: 
        OEO_00020123
    
    
ObjectProperty: OEO_00000516

    Annotations: 
        <http://purl.obolibrary.org/obo/IAO_0000115> "A relation that holds between data set and the temporal resolution it uses."@en,
        <http://purl.obolibrary.org/obo/IAO_0000233> "issue https://github.com/OpenEnergyPlatform/ontology/issues/622
Pull request https://github.com/OpenEnergyPlatform/ontology/pull/626
def and axioms
Pull request https://github.com/OpenEnergyPlatform/ontology/pull/912
fix def and add domain and range
Pull request https://github.com/OpenEnergyPlatform/ontology/pull/972
rework module structure 
issue: https://github.com/OpenEnergyPlatform/ontology/issues/1592
pull request: https://github.com/OpenEnergyPlatform/ontology/pull/1652",
        rdfs:label "has temporal resolution"@en
    
    SubPropertyOf: 
        OEO_00000514
    
    Domain: 
        <http://purl.obolibrary.org/obo/IAO_0000100>
    
    Range: 
        OEO_00020122
    
    
ObjectProperty: OEO_00000517

    Annotations: 
        <http://purl.obolibrary.org/obo/IAO_0000115> "A relation that holds between a transformation and the constraints it has to fulfil."@en,
        <http://purl.obolibrary.org/obo/IAO_0000233> "issue: https://github.com/OpenEnergyPlatform/ontology/issues/618
pull request: https://github.com/OpenEnergyPlatform/ontology/pull/716",
        rdfs:label "has constraint"@en
    
    SubPropertyOf: 
        OEO_00140093
    
    Domain: 
        OEO_00000419
    
    Range: 
        OEO_00000104
    
    
ObjectProperty: OEO_00000522

    Domain: 
        OEO_00020011
    
    
ObjectProperty: OEO_00010121

    
ObjectProperty: OEO_00010378

    Annotations: 
        <http://purl.obolibrary.org/obo/IAO_0000115> "An is-about-relation between an information content entity and a spatial region that describes that the information content entity is about a spatial region.",
        <http://purl.obolibrary.org/obo/IAO_0000233> "issue: https://github.com/OpenEnergyPlatform/ontology/issues/1404
pull request: https://github.com/OpenEnergyPlatform/ontology/pull/1441",
        rdfs:label "has spatial region"@en
    
    SubPropertyOf: 
        <http://purl.obolibrary.org/obo/IAO_0000136>
    
    Domain: 
        <http://purl.obolibrary.org/obo/IAO_0000030>
    
    Range: 
        <http://purl.obolibrary.org/obo/BFO_0000006>
    
    
ObjectProperty: OEO_00020056

    
ObjectProperty: OEO_00020188

    
ObjectProperty: OEO_00020189

    
ObjectProperty: OEO_00020190

    
ObjectProperty: OEO_00020220

    Annotations: 
        <http://purl.obolibrary.org/obo/IAO_0000115> "An is-about-relation between a scenario and a study region to indicate the study region of a scenario.",
        <http://purl.obolibrary.org/obo/IAO_0000233> "issue: https://github.com/OpenEnergyPlatform/ontology/issues/1335
pull request: https://github.com/OpenEnergyPlatform/ontology/pull/1347

Make subproperty of 'has spatial region':
issue: https://github.com/OpenEnergyPlatform/ontology/issues/1404
pull request: https://github.com/OpenEnergyPlatform/ontology/pull/1441",
        rdfs:label "has study region"@en
    
    SubPropertyOf: 
        OEO_00010378
    
    Domain: 
        OEO_00000364
    
    Range: 
        OEO_00020032
    
    
ObjectProperty: OEO_00020221

    Annotations: 
        <http://purl.obolibrary.org/obo/IAO_0000115> "An is-about-relation between a scenario and a considered region to indicated a considered region of a scenario.",
        <http://purl.obolibrary.org/obo/IAO_0000233> "issue: https://github.com/OpenEnergyPlatform/ontology/issues/1335
pull request: https://github.com/OpenEnergyPlatform/ontology/pull/1347

Make subproperty of 'has spatial region':
issue: https://github.com/OpenEnergyPlatform/ontology/issues/1404
pull request: https://github.com/OpenEnergyPlatform/ontology/pull/1441",
        rdfs:label "has considered region"@en
    
    SubPropertyOf: 
        OEO_00010378
    
    Domain: 
        OEO_00000364
    
    Range: 
        OEO_00020035
    
    
ObjectProperty: OEO_00020222

    Annotations: 
        <http://purl.obolibrary.org/obo/IAO_0000115> "An is-about-relation between a scenario and an interacting region to indicate an interacting region of a scenario.",
        <http://purl.obolibrary.org/obo/IAO_0000233> "issue: https://github.com/OpenEnergyPlatform/ontology/issues/1335
pull request: https://github.com/OpenEnergyPlatform/ontology/pull/1347

Make subproperty of 'has spatial region':
issue: https://github.com/OpenEnergyPlatform/ontology/issues/1404
pull request: https://github.com/OpenEnergyPlatform/ontology/pull/1441",
        rdfs:label "has interacting region"@en
    
    SubPropertyOf: 
        OEO_00010378
    
    Domain: 
        OEO_00000364
    
    Range: 
        OEO_00020036
    
    
ObjectProperty: OEO_00020223

    Annotations: 
        <http://purl.obolibrary.org/obo/IAO_0000115> "An is-about-relation between a scenario and a study subregion to indicate a study subregion of a scenario.",
        <http://purl.obolibrary.org/obo/IAO_0000233> "issue: https://github.com/OpenEnergyPlatform/ontology/issues/1335
pull request: https://github.com/OpenEnergyPlatform/ontology/pull/1347

Make subproperty of 'has spatial region':
issue: https://github.com/OpenEnergyPlatform/ontology/issues/1404
pull request: https://github.com/OpenEnergyPlatform/ontology/pull/1441",
        rdfs:label "has study subregion"@en
    
    SubPropertyOf: 
        OEO_00010378
    
    Domain: 
        OEO_00000364
    
    Range: 
        OEO_00020034
    
    
ObjectProperty: OEO_00020224

    Annotations: 
        <http://purl.obolibrary.org/obo/IAO_0000115> "An is-about-relation between a scenario and a scenario year to indicate the scenario year of a scenario.",
        <http://purl.obolibrary.org/obo/IAO_0000233> "issue: https://github.com/OpenEnergyPlatform/ontology/issues/1335
pull request: https://github.com/OpenEnergyPlatform/ontology/pull/1347",
        rdfs:label "has scenario year"@en
    
    SubPropertyOf: 
        <http://purl.obolibrary.org/obo/IAO_0000136>
    
    Domain: 
        OEO_00000364
    
    Range: 
        OEO_00020097
    
    
ObjectProperty: OEO_00020226

    Annotations: 
        <http://purl.obolibrary.org/obo/IAO_0000115> "A relation between a scenario study or projection and a scenario, that indicates the scenario that provides the assumptions on which the respective scenario study or projection is based on.",
        <http://purl.obolibrary.org/obo/IAO_0000233> "issue: https://github.com/OpenEnergyPlatform/ontology/issues/1346
pull request: https://github.com/OpenEnergyPlatform/ontology/pull/1391",
        rdfs:label "is based on"@en
    
    SubPropertyOf: 
        <http://purl.obolibrary.org/obo/RO_0000057>
    
    Domain: 
        OEO_00010252 or OEO_00010262
    
    Range: 
        OEO_00000364
    
    
ObjectProperty: OEO_00040010

    
ObjectProperty: OEO_00140002

    
ObjectProperty: OEO_00140008

    
ObjectProperty: OEO_00140093

    
ObjectProperty: OEO_00140094

    
ObjectProperty: OEO_00140095

    Annotations: 
        <http://purl.obolibrary.org/obo/IAO_0000115> "A relation between an algorithm or a software and the typical duration of its execution.",
        <http://purl.obolibrary.org/obo/IAO_0000233> "issue: https://github.com/OpenEnergyPlatform/ontology/issues/527
pull request: https://github.com/OpenEnergyPlatform/ontology/pull/723",
        rdfs:label "has typical computation time"@en
    
    SubPropertyOf: 
        OEO_00140002
    
    Domain: 
        <http://purl.obolibrary.org/obo/IAO_0000010> or <http://purl.obolibrary.org/obo/IAO_0000064>
    
    Range: 
        OEO_00030035
    
    
ObjectProperty: OEO_00140096

    Annotations: 
        <http://purl.obolibrary.org/obo/IAO_0000115> "A relation between an algorithm or a software and the typical hardware used for its execution.",
        <http://purl.obolibrary.org/obo/IAO_0000233> "issue: https://github.com/OpenEnergyPlatform/ontology/issues/527
pull request: https://github.com/OpenEnergyPlatform/ontology/pull/723

move axiom to shared-axioms
issue: https://github.com/OpenEnergyPlatform/ontology/issues/1703
pull request: https://github.com/OpenEnergyPlatform/ontology/pull/1706",
        rdfs:label "has typical computation hardware"@en
    
    SubPropertyOf: 
        OEO_00000503
    
    Domain: 
        <http://purl.obolibrary.org/obo/IAO_0000010> or <http://purl.obolibrary.org/obo/IAO_0000064>
    
    
ObjectProperty: OEO_00140164

    Domain: 
        OEO_00000274
    
    
ObjectProperty: owl:topObjectProperty

    
DataProperty: OEO_00140178

    
Class: <http://purl.obolibrary.org/obo/BFO_0000002>

    
Class: <http://purl.obolibrary.org/obo/BFO_0000003>

    
Class: <http://purl.obolibrary.org/obo/BFO_0000006>

    
Class: <http://purl.obolibrary.org/obo/BFO_0000009>

    
Class: <http://purl.obolibrary.org/obo/BFO_0000015>

    
Class: <http://purl.obolibrary.org/obo/BFO_0000016>

    
Class: <http://purl.obolibrary.org/obo/BFO_0000019>

    
Class: <http://purl.obolibrary.org/obo/BFO_0000023>

    
Class: <http://purl.obolibrary.org/obo/BFO_0000024>

    
Class: <http://purl.obolibrary.org/obo/BFO_0000027>

    
Class: <http://purl.obolibrary.org/obo/BFO_0000029>

    
Class: <http://purl.obolibrary.org/obo/BFO_0000030>

    
Class: <http://purl.obolibrary.org/obo/BFO_0000031>

    
Class: <http://purl.obolibrary.org/obo/BFO_0000038>

    
Class: <http://purl.obolibrary.org/obo/BFO_0000141>

    
Class: <http://purl.obolibrary.org/obo/BFO_0000148>

    
Class: <http://purl.obolibrary.org/obo/IAO_0000010>

    
Class: <http://purl.obolibrary.org/obo/IAO_0000027>

    
Class: <http://purl.obolibrary.org/obo/IAO_0000028>

    
Class: <http://purl.obolibrary.org/obo/IAO_0000030>

    
Class: <http://purl.obolibrary.org/obo/IAO_0000064>

    
Class: <http://purl.obolibrary.org/obo/IAO_0000088>

    
Class: <http://purl.obolibrary.org/obo/IAO_0000100>

    
Class: <http://purl.obolibrary.org/obo/IAO_0000104>

    
Class: <http://purl.obolibrary.org/obo/IAO_0000300>

    
Class: <http://purl.obolibrary.org/obo/IAO_0000310>

    
Class: <http://purl.obolibrary.org/obo/RO_0002577>

    
Class: <http://purl.obolibrary.org/obo/UO_0000003>

    
Class: <http://purl.obolibrary.org/obo/UO_0000033>

    
Class: <http://purl.obolibrary.org/obo/UO_0000036>

    
Class: <http://purl.obolibrary.org/obo/UO_0000046>

    
Class: OEO_00000048

    Annotations: 
        <http://purl.obolibrary.org/obo/IAO_0000115> "An acronym is an abbreviation of the title by using the first letters of each part of the title."@en,
        <http://purl.obolibrary.org/obo/IAO_0000233> "make subclass of abbreviation:
issue: https://github.com/OpenEnergyPlatform/ontology/issues/1039
pull request: https://github.com/OpenEnergyPlatform/ontology/pull/1075",
        rdfs:label "acronym"@en
    
    SubClassOf: 
        OEO_00010247
    
    
Class: OEO_00000059

    Annotations: 
        <http://purl.obolibrary.org/obo/IAO_0000115> "An API (Application Programming interface) is a software interface allowing two Software applications to communicate with each other.",
        rdfs:label "API"@en
    
    SubClassOf: 
        OEO_00000239
    
    DisjointWith: 
        OEO_00000202
    
    
Class: OEO_00000063

    Annotations: 
        <http://purl.obolibrary.org/obo/IAO_0000115> "An assumption is an information content entity about a property of a system or process. It determines a part of a scenario content."@en,
        <http://purl.obolibrary.org/obo/IAO_0000233> "issue: https://github.com/OpenEnergyPlatform/ontology/issues/353
pull request: https://github.com/OpenEnergyPlatform/ontology/pull/525"@en,
        rdfs:label "assumption"@en
    
    SubClassOf: 
        <http://purl.obolibrary.org/obo/IAO_0000030>,
        <http://purl.obolibrary.org/obo/BFO_0000050> some OEO_00000364
    
    
Class: OEO_00000064

    
Class: OEO_00000078

    Annotations: 
        <http://purl.obolibrary.org/obo/IAO_0000115> "A boolean variable is a variable that represents a boolean value."@en,
        <http://purl.obolibrary.org/obo/IAO_0000233> "definition:
issue: https://github.com/OpenEnergyPlatform/ontology/issues/1148
pull request: https://github.com/OpenEnergyPlatform/ontology/pull/1255",
        rdfs:label "boolean variable"@en
    
    SubClassOf: 
        OEO_00000435,
        <http://purl.obolibrary.org/obo/IAO_0000136> some OEO_00010422
    
    DisjointWith: 
        OEO_00240004
    
    
Class: OEO_00000085

    Annotations: 
        <http://purl.obolibrary.org/obo/IAO_0000115> "A citation reference is a reference stating where a citation was taken from.",
        rdfs:label "citation reference"@en
    
    SubClassOf: 
        OEO_00000353
    
    
Class: OEO_00000090

    Annotations: 
        <http://purl.obolibrary.org/obo/IAO_0000115> "A code documentation is a documentation explaining and annotating software code.",
        rdfs:label "code documentation"@en
    
    SubClassOf: 
        OEO_00000380
    
    
Class: OEO_00000091

    Annotations: 
        <http://purl.obolibrary.org/obo/IAO_0000115> "A code source is a data descriptor describing the origin of some code.",
        rdfs:label "code source"@en
    
    SubClassOf: 
        OEO_00000119
    
    
Class: OEO_00000104

    Annotations: 
        <http://purl.obolibrary.org/obo/IAO_0000112> "\"The carbon dioxide emissions in Germany have to be reduced by 95% till 2050.\" is a constraint for a model calculation about the energy system."@en,
        <http://purl.obolibrary.org/obo/IAO_0000115> "A constraint is a condition that has to be fulfilled within a calculation."@en,
        rdfs:label "constraint"@en
    
    SubClassOf: 
        <http://purl.obolibrary.org/obo/IAO_0000030>
    
    
Class: OEO_00000118

    Annotations: 
        <http://purl.obolibrary.org/obo/IAO_0000115> "A database is an information content entity that stores data items and data sets.",
        <http://purl.obolibrary.org/obo/IAO_0000233> "issue: https://github.com/OpenEnergyPlatform/ontology/issues/253
pull request: https://github.com/OpenEnergyPlatform/ontology/pull/272

Add 'has licence' axiom:
issue: https://github.com/OpenEnergyPlatform/ontology/issues/1275
pull request: https://github.com/OpenEnergyPlatform/ontology/pull/1547",
        rdfs:label "database"@en
    
    SubClassOf: 
        <http://purl.obolibrary.org/obo/IAO_0000030>,
        OEO_00020188 some OEO_00020186,
        <http://purl.obolibrary.org/obo/BFO_0000051> some <http://purl.obolibrary.org/obo/IAO_0000027>
    
    
Class: OEO_00000119

    Annotations: 
        <http://purl.obolibrary.org/obo/IAO_0000115> "A data descriptor is an information content entity that contains additional information about some data.",
        <http://purl.obolibrary.org/obo/IAO_0000233> "issue: https://github.com/OpenEnergyPlatform/ontology/issues/612
		pull request: https://github.com/OpenEnergyPlatform/ontology/pull/724
		move to oeo-shared
		issue: https://github.com/OpenEnergyPlatform/ontology/issues/1384
		pull request: https://github.com/OpenEnergyPlatform/ontology/pull/1390
		rework module structure 
		issue: https://github.com/OpenEnergyPlatform/ontology/issues/1592
		pull request: https://github.com/OpenEnergyPlatform/ontology/pull/1652",
        rdfs:label "data descriptor"@en
    
    SubClassOf: 
        <http://purl.obolibrary.org/obo/IAO_0000030>
    
    
Class: OEO_00000120

    Annotations: 
        <http://purl.obolibrary.org/obo/IAO_0000115> "A data format is a data descriptor that specifies the structure in which the data item is encoded.",
        <http://purl.obolibrary.org/obo/IAO_0000233> "issue: https://github.com/OpenEnergyPlatform/ontology/issues/1145
pull request: https://github.com/OpenEnergyPlatform/ontology/pull/1326",
        rdfs:label "data format"@en
    
    SubClassOf: 
        OEO_00000119
    
    DisjointWith: 
        OEO_00000312
    
    
Class: OEO_00000122

    Annotations: 
        <http://purl.obolibrary.org/obo/IAO_0000115> "Data postprocessing is data processing that transforms the output of a model calculation into a form that is suitable for presentation.",
        rdfs:label "data postprocessing"@en
    
    SubClassOf: 
        OEO_00000124
    
    
Class: OEO_00000123

    Annotations: 
        <http://purl.obolibrary.org/obo/IAO_0000115> "Data preprocessing is data processing that transforms the input into a form that is useable for a model calculation.",
        rdfs:label "data preprocessing"@en
    
    SubClassOf: 
        OEO_00000124
    
    
Class: OEO_00000124

    Annotations: 
        <http://purl.obolibrary.org/obo/IAO_0000233> "issue: https://github.com/OpenEnergyPlatform/ontology/issues/252
pull request: https://github.com/OpenEnergyPlatform/ontology/pull/289",
        rdfs:comment "data processing is a transformation in which a data item gets transformed.",
        rdfs:label "data processing"@en
    
    SubClassOf: 
        OEO_00000419,
        <http://purl.obolibrary.org/obo/RO_0000057> some <http://purl.obolibrary.org/obo/IAO_0000027>
    
    
Class: OEO_00000125

    Annotations: 
        <http://purl.obolibrary.org/obo/IAO_0000115> "data processing software is software used in the context of data processing.",
        rdfs:label "data processing software"@en
    
    SubClassOf: 
        <http://purl.obolibrary.org/obo/IAO_0000010>
    
    
Class: OEO_00000133

    Annotations: 
        <http://purl.obolibrary.org/obo/IAO_0000115> "A DOI (digital object identifier) is a persistent identifier or handle used to uniquely identify objects, standardized by the International Organization for Standardization (ISO).
source: https://en.wikipedia.org/wiki/Digital_object_identifier"@en,
        <http://purl.obolibrary.org/obo/IAO_0000118> "digital object identifier",
        rdfs:label "DOI"@en
    
    SubClassOf: 
        <http://purl.obolibrary.org/obo/IAO_0000028>
    
    
Class: OEO_00000149

    Annotations: 
        <http://purl.obolibrary.org/obo/IAO_0000112> "The measurement series of some experiment."@en,
        <http://purl.obolibrary.org/obo/IAO_0000115> "An empirical data set is a dataset that is obtained from observations in the real world."@en,
        <http://purl.obolibrary.org/obo/IAO_0000233> "Move to oeo-shared and harmonise label:
https://github.com/OpenEnergyPlatform/ontology/pull/1463
rework module structure 
issue: https://github.com/OpenEnergyPlatform/ontology/issues/1592
pull request: https://github.com/OpenEnergyPlatform/ontology/pull/1652",
        rdfs:label "empirical data set"@en
    
    SubClassOf: 
        <http://purl.obolibrary.org/obo/IAO_0000100>
    
    DisjointWith: 
        OEO_00000403
    
    
Class: OEO_00000161

    Annotations: 
        <http://purl.obolibrary.org/obo/IAO_0000115> "An external optimiser is a software external to a model that computes an optimisation.",
        <http://purl.obolibrary.org/obo/IAO_0000118> "external optimizer",
        rdfs:label "external optimiser"@en
    
    SubClassOf: 
        <http://purl.obolibrary.org/obo/IAO_0000010>
    
    
Class: OEO_00000162

    Annotations: 
        <http://purl.obolibrary.org/obo/IAO_0000115> "A factsheet is a document that collects information about a specific topic in a structured way.",
        <http://purl.obolibrary.org/obo/IAO_0000233> "issue: https://github.com/OpenEnergyPlatform/ontology/issues/250
pull request: https://github.com/OpenEnergyPlatform/ontology/pull/271

Add 'has licence' axiom:
issue: https://github.com/OpenEnergyPlatform/ontology/issues/1275
pull request: https://github.com/OpenEnergyPlatform/ontology/pull/1547",
        rdfs:comment "this entity is general and not specific to the OEP factsheets.",
        rdfs:label "factsheet"@en
    
    SubClassOf: 
        <http://purl.obolibrary.org/obo/IAO_0000310>,
        OEO_00020188 some OEO_00010412
    
    
Class: OEO_00000172

    Annotations: 
        <http://purl.obolibrary.org/obo/IAO_0000115> "A framework factsheet is a factsheet that contains information about a software framework.",
        <http://purl.obolibrary.org/obo/IAO_0000233> "issue: https://github.com/OpenEnergyPlatform/ontology/issues/414
pull request: https://github.com/OpenEnergyPlatform/ontology/pull/440
pull request: https://github.com/OpenEnergyPlatform/ontology/pull/584",
        rdfs:label "framework factsheet"@en
    
    SubClassOf: 
        OEO_00000162,
        <http://purl.obolibrary.org/obo/IAO_0000136> some OEO_00000382
    
    
Class: OEO_00000202

    Annotations: 
        <http://purl.obolibrary.org/obo/IAO_0000115> "A GUI (Graphical user interface) is a software interface allowing users to communicate with a software application through a graphical window.",
        rdfs:label "GUI"@en
    
    SubClassOf: 
        OEO_00000239
    
    DisjointWith: 
        OEO_00000059
    
    
Class: OEO_00000228

    Annotations: 
        <http://purl.obolibrary.org/obo/IAO_0000115> "An installation guide is a documentation intended to help users install a Software.",
        rdfs:label "installation guide"@en
    
    SubClassOf: 
        OEO_00000380
    
    
Class: OEO_00000239

    Annotations: 
        <http://purl.obolibrary.org/obo/IAO_0000115> "A software interface is a software that enables an agent to interact with it.",
        rdfs:label "software interface"@en
    
    SubClassOf: 
        <http://purl.obolibrary.org/obo/IAO_0000010>
    
    
Class: OEO_00000264

    Annotations: 
        <http://purl.obolibrary.org/obo/IAO_0000115> "An energy market model is a model that is about the energy market.",
        <http://purl.obolibrary.org/obo/IAO_0000233> "issue: https://github.com/OpenEnergyPlatform/ontology/issues/415
pull request: https://github.com/OpenEnergyPlatform/ontology/pull/821

rework module structure 
issue: https://github.com/OpenEnergyPlatform/ontology/issues/1592
pull request: https://github.com/OpenEnergyPlatform/ontology/pull/1652",
        rdfs:label "energy market model"@en
    
    SubClassOf: 
        OEO_00000274
    
    
Class: OEO_00000274

    Annotations: 
        <http://purl.obolibrary.org/obo/IAO_0000115> "A numerical computer model is a mathematical model that is calculated by a computer."@en,
        <http://purl.obolibrary.org/obo/IAO_0000116> "formerly called \"model\"",
        <http://purl.obolibrary.org/obo/IAO_0000233> "issue: https://github.com/OpenEnergyPlatform/ontology/issues/180
pull request: https://github.com/OpenEnergyPlatform/ontology/pull/349

issue: https://github.com/OpenEnergyPlatform/ontology/issues/208
pull request: https://github.com/OpenEnergyPlatform/ontology/pull/287

add axiom to model calculation
pull request: https://github.com/OpenEnergyPlatform/ontology/pull/1113

rework module structure 
issue: https://github.com/OpenEnergyPlatform/ontology/issues/1592
pull request: https://github.com/OpenEnergyPlatform/ontology/pull/1652

rename and reclassify
issue: https://github.com/OpenEnergyPlatform/ontology/issues/1444
pull request: https://github.com/OpenEnergyPlatform/ontology/pull/1707",
        rdfs:label "numerical computer model"@en
    
    SubClassOf: 
        OEO_00020354
    
    
Class: OEO_00000275

    Annotations: 
        <http://purl.obolibrary.org/obo/IAO_0000115> "A model calculation is a process of solving mathematical equations of a model."@en,
        <http://purl.obolibrary.org/obo/IAO_0000233> "issue: https://github.com/OpenEnergyPlatform/ontology/issues/73
pull request: https://github.com/OpenEnergyPlatform/ontology/pull/504
moved to oeo-shared
pull request: https://github.com/OpenEnergyPlatform/ontology/pull/1113
rework module structure 
issue: https://github.com/OpenEnergyPlatform/ontology/issues/1592
pull request: https://github.com/OpenEnergyPlatform/ontology/pull/1652"@en,
        rdfs:label "model calculation"@en
    
    SubClassOf: 
        <http://purl.obolibrary.org/obo/BFO_0000015>,
        OEO_00140093 some OEO_00030029,
        OEO_00140094 some OEO_00030030,
        
            Annotations: <http://purl.obolibrary.org/obo/IAO_0000233> "issue: https://github.com/OpenEnergyPlatform/ontology/issues/850
pull request: https://github.com/OpenEnergyPlatform/ontology/pull/871"
        <http://purl.obolibrary.org/obo/RO_0000057> some OEO_00000274
    
    
Class: OEO_00000276

    Annotations: 
        <http://purl.obolibrary.org/obo/IAO_0000115> "A model component is a generically dependent continuant that is part of a model.",
        <http://purl.obolibrary.org/obo/IAO_0000118> "model element",
        rdfs:label "model component"@en
    
    EquivalentTo: 
        <http://purl.obolibrary.org/obo/BFO_0000050> some OEO_00000274
    
    SubClassOf: 
        <http://purl.obolibrary.org/obo/BFO_0000031>
    
    
Class: OEO_00000277

    Annotations: 
        <http://purl.obolibrary.org/obo/IAO_0000115> "A model factsheet is a model descriptor that contains a brief description of all relevant model information.",
        <http://purl.obolibrary.org/obo/IAO_0000233> "issue: https://github.com/OpenEnergyPlatform/ontology/issues/414
pull request: https://github.com/OpenEnergyPlatform/ontology/pull/440 
pull request: https://github.com/OpenEnergyPlatform/ontology/pull/577
pull request: https://github.com/OpenEnergyPlatform/ontology/pull/584

issue: https://github.com/OpenEnergyPlatform/ontology/issues/851
pull request: https://github.com/OpenEnergyPlatform/ontology/pull/854",
        rdfs:label "model factsheet"@en
    
    SubClassOf: 
        OEO_00000162
         and (<http://purl.obolibrary.org/obo/IAO_0000136> some OEO_00000274)
    
    
Class: OEO_00000279

    Annotations: 
        <http://purl.obolibrary.org/obo/IAO_0000115> "A modelling software is a software used to create and maintain a (mathematical) model.",
        <http://purl.obolibrary.org/obo/IAO_0000118> "modeling software",
        <http://purl.obolibrary.org/obo/IAO_0000233> "issue: https://github.com/OpenEnergyPlatform/ontology/issues/338
pull request: https://github.com/OpenEnergyPlatform/ontology/pull/345

Add 'has licence' axiom:
issue: https://github.com/OpenEnergyPlatform/ontology/issues/1275
pull request: https://github.com/OpenEnergyPlatform/ontology/pull/1547",
        rdfs:label "modelling software"@en
    
    SubClassOf: 
        <http://purl.obolibrary.org/obo/IAO_0000010>,
        OEO_00020188 some OEO_00020187
    
    
Class: OEO_00000281

    Annotations: 
        <http://purl.obolibrary.org/obo/IAO_0000115> "A modus is an information content entity describing the state of activity something has, e.g. active, inactive or passive.",
        rdfs:label "modus"@en
    
    SubClassOf: 
        <http://purl.obolibrary.org/obo/IAO_0000030>
    
    
Class: OEO_00000304

    Annotations: 
        <http://purl.obolibrary.org/obo/IAO_0000115> "An objective function is an information content entity stating the function that should be maximised or minimised to solve a problem.",
        <http://purl.obolibrary.org/obo/IAO_0000233> "issue: https://github.com/OpenEnergyPlatform/ontology/issues/725
pull request: https://github.com/OpenEnergyPlatform/ontology/pull/757",
        rdfs:label "objective function"@en
    
    SubClassOf: 
        <http://purl.obolibrary.org/obo/IAO_0000030>
    
    
Class: OEO_00000312

    Annotations: 
        <http://purl.obolibrary.org/obo/IAO_0000115> "open source is a software descriptor labelling software whose source code is available online for free and can be modified or redistributed.",
        rdfs:label "open source"@en
    
    SubClassOf: 
        OEO_00000378
    
    DisjointWith: 
        OEO_00000120
    
    
Class: OEO_00000313

    Annotations: 
        <http://purl.obolibrary.org/obo/IAO_0000115> "An optimisation is a model calculation with the goal to find a best choice or result for at least one variable or function in the model."@en,
        <http://purl.obolibrary.org/obo/IAO_0000118> "optimization",
        <http://purl.obolibrary.org/obo/IAO_0000233> "Add 'has participant' axiom:
pull request: https://github.com/OpenEnergyPlatform/ontology/pull/1410",
        rdfs:label "optimisation"@en
    
    SubClassOf: 
        OEO_00000275,
        <http://purl.obolibrary.org/obo/RO_0000057> some OEO_00000314
    
    DisjointWith: 
        OEO_00000370
    
    
Class: OEO_00000314

    Annotations: 
        <http://purl.obolibrary.org/obo/IAO_0000115> "An optimisation model is a model that optimises a target function."@en,
        <http://purl.obolibrary.org/obo/IAO_0000118> "optimization model",
        rdfs:label "optimisation model"@en
    
    SubClassOf: 
        OEO_00000274,
        
            Annotations: <http://purl.obolibrary.org/obo/IAO_0000233> "issue: https://github.com/OpenEnergyPlatform/ontology/issues/415
pull request: https://github.com/OpenEnergyPlatform/ontology/pull/821"
        <http://purl.obolibrary.org/obo/BFO_0000051> some OEO_00000304
    
    
Class: OEO_00000323

    
Class: OEO_00000327

    Annotations: 
        <http://purl.obolibrary.org/obo/IAO_0000115> "Plotting is data processing where data is visualised in form of a diagram.",
        rdfs:label "plotting"@en
    
    SubClassOf: 
        OEO_00000124
    
    
Class: OEO_00000328

    Annotations: 
        <http://purl.obolibrary.org/obo/IAO_0000115> "A political assumption is an assumption about political measures taken."@en,
        rdfs:label "political assumption"@en
    
    SubClassOf: 
        OEO_00000063
    
    
Class: OEO_00000339

    Annotations: 
        <http://purl.obolibrary.org/obo/IAO_0000112> "Settings for a random number generator."@en,
        <http://purl.obolibrary.org/obo/IAO_0000115> "A program parameter is a variable in a software."@en,
        <http://purl.obolibrary.org/obo/IAO_0000233> "Rework definition and change parent class:
issue: https://github.com/OpenEnergyPlatform/ontology/issues/1199
pull request: https://github.com/OpenEnergyPlatform/ontology/pull/1274",
        rdfs:label "program parameter"@en
    
    SubClassOf: 
        OEO_00000435,
        <http://purl.obolibrary.org/obo/BFO_0000050> some <http://purl.obolibrary.org/obo/IAO_0000010>
    
    
Class: OEO_00000340

    
Class: OEO_00000350

    
Class: OEO_00000353

    Annotations: 
        <http://purl.obolibrary.org/obo/IAO_0000115> "A reference is an information content entity naming a relevant document, position in a document or address.",
        rdfs:label "reference"@en
    
    SubClassOf: 
        <http://purl.obolibrary.org/obo/IAO_0000030>
    
    
Class: OEO_00000364

    Annotations: 
        <http://purl.obolibrary.org/obo/IAO_0000115> "A scenario is an information content entity that contains statements about a possible future development based on a coherent and internally consistent set of assumptions and their motivation."@en,
        <http://purl.obolibrary.org/obo/IAO_0000118> "narrative",
        <http://purl.obolibrary.org/obo/IAO_0000118> "storyline",
        <http://purl.obolibrary.org/obo/IAO_0000233> "issue: https://github.com/OpenEnergyPlatform/ontology/issues/328
pull request: https://github.com/OpenEnergyPlatform/ontology/pull/344
add is about-relation
pull request: https://github.com/OpenEnergyPlatform/ontology/pull/764

Add 'narrative' and 'storyline' as alternative label
issue: https://github.com/OpenEnergyPlatform/ontology/issues/1232
pull request: https://github.com/OpenEnergyPlatform/ontology/pull/1296

rework module structure 
issue: https://github.com/OpenEnergyPlatform/ontology/issues/1592
pull request: https://github.com/OpenEnergyPlatform/ontology/pull/1652",
        rdfs:label "scenario"@en
    
    SubClassOf: 
        <http://purl.obolibrary.org/obo/IAO_0000030>,
        <http://purl.obolibrary.org/obo/IAO_0000136> some OEO_00020072
    
    
Class: OEO_00000365

    Annotations: 
        <http://purl.obolibrary.org/obo/IAO_0000115> "A scenario factsheet is a factsheet that contains information about a scenario.",
        <http://purl.obolibrary.org/obo/IAO_0000233> "issue: https://github.com/OpenEnergyPlatform/ontology/issues/414
pull request: https://github.com/OpenEnergyPlatform/ontology/pull/440
pull request: https://github.com/OpenEnergyPlatform/ontology/pull/584",
        rdfs:label "scenario factsheet"@en
    
    SubClassOf: 
        OEO_00000162,
        <http://purl.obolibrary.org/obo/IAO_0000136> some OEO_00000364
    
    
Class: OEO_00000370

    Annotations: 
        <http://purl.obolibrary.org/obo/IAO_0000115> "A simulation is a model calculation that simulates a process or system behaviour from the real world."@en,
        <http://purl.obolibrary.org/obo/IAO_0000233> "Add 'has participant' axiom:
pull request: https://github.com/OpenEnergyPlatform/ontology/pull/1410",
        rdfs:label "simulation"@en
    
    SubClassOf: 
        OEO_00000275,
        <http://purl.obolibrary.org/obo/RO_0000057> some OEO_00000371
    
    DisjointWith: 
        OEO_00000313
    
    
Class: OEO_00000371

    Annotations: 
        <http://purl.obolibrary.org/obo/IAO_0000115> "A simulation model is a model that simulates the behaviour of a system without a target function."@en,
        rdfs:label "simulation model"@en
    
    SubClassOf: 
        OEO_00000274,
        
            Annotations: <http://purl.obolibrary.org/obo/IAO_0000233> "issue: https://github.com/OpenEnergyPlatform/ontology/issues/415
pull request: https://github.com/OpenEnergyPlatform/ontology/pull/821"
        not (<http://purl.obolibrary.org/obo/BFO_0000051> some OEO_00000304)
    
    
Class: OEO_00000372

    Annotations: 
        <http://purl.obolibrary.org/obo/IAO_0000115> "A single node model is a model where a region is represented as a single node.",
        <http://purl.obolibrary.org/obo/IAO_0000233> "issue: https://github.com/OpenEnergyPlatform/ontology/issues/337
pull request: https://github.com/OpenEnergyPlatform/ontology/pull/358",
        rdfs:label "single node model"@en
    
    SubClassOf: 
        OEO_00000274
    
    
Class: OEO_00000378

    Annotations: 
        <http://purl.obolibrary.org/obo/IAO_0000115> "A software descriptor is an information content entity that contains additional information about the software.",
        rdfs:label "software descriptor"@en
    
    SubClassOf: 
        <http://purl.obolibrary.org/obo/IAO_0000030>
    
    
Class: OEO_00000380

    Annotations: 
        <http://purl.obolibrary.org/obo/IAO_0000233> "issue: https://github.com/OpenEnergyPlatform/ontology/issues/251
pull request: https://github.com/OpenEnergyPlatform/ontology/pull/285

Add 'has licence' axiom:
issue: https://github.com/OpenEnergyPlatform/ontology/issues/1275
pull request: https://github.com/OpenEnergyPlatform/ontology/pull/1547",
        rdfs:comment "A software documentation is a document containing explanations and tutorials how to use a program and is delivered with that program.",
        rdfs:label "software documentation"@en
    
    SubClassOf: 
        <http://purl.obolibrary.org/obo/IAO_0000310>,
        OEO_00020188 some OEO_00010412
    
    
Class: OEO_00000382

    Annotations: 
        <http://purl.obolibrary.org/obo/IAO_0000115> "A software framework is a Software that is generic and can be adapted to a specific application.",
        <http://purl.obolibrary.org/obo/IAO_0000233> "issue: https://github.com/OpenEnergyPlatform/ontology/issues/262
pull request: https://github.com/OpenEnergyPlatform/ontology/pull/286",
        rdfs:label "software framework"@en
    
    SubClassOf: 
        <http://purl.obolibrary.org/obo/IAO_0000010>
    
    
Class: OEO_00000392

    Annotations: 
        <http://purl.obolibrary.org/obo/IAO_0000115> "A solver is a software that solves a mathematical problem.",
        rdfs:label "solver"@en
    
    SubClassOf: 
        <http://purl.obolibrary.org/obo/IAO_0000010>
    
    
Class: OEO_00000403

    Annotations: 
        <http://purl.obolibrary.org/obo/IAO_0000112> "The projected power usage during an idealised model year."@en,
        <http://purl.obolibrary.org/obo/IAO_0000115> "A synthetic data set is a dataset that is obtained by artificially creating data items. It is constructed to be an estimation of a real-world dataset."@en,
        <http://purl.obolibrary.org/obo/IAO_0000233> "Harmonise label:
https://github.com/OpenEnergyPlatform/ontology/pull/1463

rework module structure 
issue: https://github.com/OpenEnergyPlatform/ontology/issues/1592
pull request: https://github.com/OpenEnergyPlatform/ontology/pull/1652",
        rdfs:label "synthetic data set"@en
    
    SubClassOf: 
        <http://purl.obolibrary.org/obo/IAO_0000100>
    
    DisjointWith: 
        OEO_00000149
    
    
Class: OEO_00000408

    Annotations: 
        <http://purl.obolibrary.org/obo/IAO_0000115> "A test data set is a data set used for testing.",
        <http://purl.obolibrary.org/obo/IAO_0000233> "Harmonise label:
https://github.com/OpenEnergyPlatform/ontology/pull/1463",
        rdfs:label "test data set"@en
    
    SubClassOf: 
        <http://purl.obolibrary.org/obo/IAO_0000100>
    
    
Class: OEO_00000419

    
Class: OEO_00000423

    Annotations: 
        <http://purl.obolibrary.org/obo/IAO_0000115> "An electricity transshipment model is a model that applies the transshipment problem to the electricity grid.",
        <http://purl.obolibrary.org/obo/IAO_0000233> "issue: https://github.com/OpenEnergyPlatform/ontology/issues/337
pull request: https://github.com/OpenEnergyPlatform/ontology/pull/358

rework module structure 
issue: https://github.com/OpenEnergyPlatform/ontology/issues/1592
pull request: https://github.com/OpenEnergyPlatform/ontology/pull/1652",
        rdfs:label "electricity transshipment model"@en
    
    SubClassOf: 
        OEO_00000274
    
    
Class: OEO_00000432

    Annotations: 
        <http://purl.obolibrary.org/obo/IAO_0000115> "A user documentation is a documentation intended to assist users in using the software.",
        rdfs:label "user documentation"@en
    
    SubClassOf: 
        OEO_00000380
    
    
Class: OEO_00000435

    Annotations: 
        <http://purl.obolibrary.org/obo/IAO_0000115> "A variable is an information content entity that represents a changeable value, vector, matrix or function within a mathematical expression."@en,
        rdfs:label "variable"@en
    
    SubClassOf: 
        <http://purl.obolibrary.org/obo/IAO_0000030>
    
    
Class: OEO_00010051

    Annotations: 
        <http://purl.obolibrary.org/obo/IAO_0000115> "A sensitivity analysis is the process of comparing different model calculations based on a variation of input parameters (exogenous data items).",
        <http://purl.obolibrary.org/obo/IAO_0000233> "issue: https://github.com/OpenEnergyPlatform/ontology/issues/483
pull request: https://github.com/OpenEnergyPlatform/ontology/pull/550",
        rdfs:label "sensitivity analysis"@en
    
    SubClassOf: 
        <http://purl.obolibrary.org/obo/BFO_0000015>
    
    
Class: OEO_00010213

    Annotations: 
        <http://purl.obolibrary.org/obo/IAO_0000115> "An emission constraint is a constraint that determines the emissions a model calculation describes.",
        <http://purl.obolibrary.org/obo/IAO_0000118> "decarbonisation pathway",
        <http://purl.obolibrary.org/obo/IAO_0000233> "issue: https://github.com/OpenEnergyPlatform/ontology/issues/831
pull request: https://github.com/OpenEnergyPlatform/ontology/pull/951",
        rdfs:label "emission constraint"@en
    
    SubClassOf: 
        OEO_00000104
    
    
Class: OEO_00010233

    Annotations: 
        <http://purl.obolibrary.org/obo/IAO_0000115> "A forecast error is a quantity value that quantifies the difference between a measured and a forecasted value.",
        <http://purl.obolibrary.org/obo/IAO_0000233> "issue: https://github.com/OpenEnergyPlatform/ontology/issues/907
pull request: https://github.com/OpenEnergyPlatform/ontology/pull/1002",
        rdfs:label "forecast error"@en
    
    SubClassOf: 
        OEO_00000350
    
    
Class: OEO_00010247

    Annotations: 
        <http://purl.obolibrary.org/obo/IAO_0000115> "An abbreviation is a symbol of a textual entity.",
        <http://purl.obolibrary.org/obo/IAO_0000233> "issue: https://github.com/OpenEnergyPlatform/ontology/issues/1039
pull request: https://github.com/OpenEnergyPlatform/ontology/pull/1075",
        rdfs:label "abbreviation"@en
    
    SubClassOf: 
        <http://purl.obolibrary.org/obo/IAO_0000028>,
        <http://purl.obolibrary.org/obo/IAO_0000136> some <http://purl.obolibrary.org/obo/IAO_0000300>
    
    
Class: OEO_00010250

    Annotations: 
        <http://purl.obolibrary.org/obo/IAO_0000115> "A study factsheet is a factsheet that contains information about a scenario study.",
        <http://purl.obolibrary.org/obo/IAO_0000233> "issue: https://github.com/OpenEnergyPlatform/ontology/issues/1069
pull request: https://github.com/OpenEnergyPlatform/ontology/pull/1131",
        rdfs:label "study factsheet"@en
    
    SubClassOf: 
        OEO_00000162,
        <http://purl.obolibrary.org/obo/IAO_0000136> some OEO_00020011
    
    
Class: OEO_00010251

    Annotations: 
        <http://purl.obolibrary.org/obo/IAO_0000115> "An OEP study factsheet is an study factsheet hosted on the Open Energy Platform. It is used to access the Open Energy Knowledge Graph (OEKG).",
        <http://purl.obolibrary.org/obo/IAO_0000233> "issue: https://github.com/OpenEnergyPlatform/ontology/issues/1069
pull request: https://github.com/OpenEnergyPlatform/ontology/pull/1131",
        rdfs:label "OEP study factsheet"@en
    
    SubClassOf: 
        OEO_00010250,
        <http://purl.obolibrary.org/obo/IAO_0000136> some OEO_00010252
    
    
Class: OEO_00010252

    Annotations: 
        <http://purl.obolibrary.org/obo/IAO_0000115> "A scenario study is a study that investigates one or more scenarios.",
        <http://purl.obolibrary.org/obo/IAO_0000233> "issue: https://github.com/OpenEnergyPlatform/ontology/issues/1058
pull request: https://github.com/OpenEnergyPlatform/ontology/pull/1131
add based on axiom
issue: https://github.com/OpenEnergyPlatform/ontology/issues/1346
pull request: https://github.com/OpenEnergyPlatform/ontology/pull/1391",
        rdfs:label "scenario study"@en
    
    SubClassOf: 
        OEO_00020011,
        OEO_00020226 some OEO_00000364
    
    
Class: OEO_00010255

    Annotations: 
        <http://purl.obolibrary.org/obo/IAO_0000115> "A nationally determined contribution (NDC) is a target description of future greenhouse gas emission reductions prepared, communicated and maintained by a party to the Paris Agreement.",
        <http://purl.obolibrary.org/obo/IAO_0000118> "NDC",
        <http://purl.obolibrary.org/obo/IAO_0000233> "issue: https://github.com/OpenEnergyPlatform/ontology/issues/947
pull request: https://github.com/OpenEnergyPlatform/ontology/pull/1151

move axiom to shared-axioms
issue: https://github.com/OpenEnergyPlatform/ontology/issues/1703
pull request: https://github.com/OpenEnergyPlatform/ontology/pull/1706",
        rdfs:label "nationally determined contribution"@en
    
    SubClassOf: 
        OEO_00020093
    
    
Class: OEO_00010260

    Annotations: 
        <http://purl.obolibrary.org/obo/IAO_0000115> "Parameterisation is the process of translating assumptions into exogenous data the model can use.",
        <http://purl.obolibrary.org/obo/IAO_0000118> "parametrise",
        <http://purl.obolibrary.org/obo/IAO_0000233> "issue: https://github.com/OpenEnergyPlatform/ontology/issues/1040
pull request: https://github.com/OpenEnergyPlatform/ontology/pull/1216",
        rdfs:label "parameterisation"@en
    
    SubClassOf: 
        <http://purl.obolibrary.org/obo/BFO_0000015>,
        <http://purl.obolibrary.org/obo/RO_0002233> some OEO_00000063,
        <http://purl.obolibrary.org/obo/RO_0002234> some OEO_00030029
    
    
Class: OEO_00010261

    Annotations: 
        <http://purl.obolibrary.org/obo/IAO_0000115> "Model calibration is a process of varying exogenous data, so that the model reproduces the known data (e.g. historical) as far as possible, and thus a part of validation.",
        <http://purl.obolibrary.org/obo/IAO_0000233> "issue: https://github.com/OpenEnergyPlatform/ontology/issues/1040
pull request: https://github.com/OpenEnergyPlatform/ontology/pull/1216",
        rdfs:label "model calibration"@en
    
    SubClassOf: 
        <http://purl.obolibrary.org/obo/BFO_0000015>,
        <http://purl.obolibrary.org/obo/BFO_0000050> some OEO_00140024,
        <http://purl.obolibrary.org/obo/RO_0000057> some OEO_00000274,
        <http://purl.obolibrary.org/obo/RO_0000057> some OEO_00030029
    
    
Class: OEO_00010262

    Annotations: 
        <http://purl.obolibrary.org/obo/IAO_0000115> "A scenario projection is an intentional process in which output (endogenous) data of interest are quantified for future points in time using one or more model calculation based on a scenario.",
        <http://purl.obolibrary.org/obo/IAO_0000116> "A scenario projection is an intentional process (with human participation): A scenario is either created or selected, its assumptions are translated into data sets. These datasets are quantified and serve as inputs to a model calculation which is applied to quantitatively project one or more variables of interest into the future.
(Intentional: a research question is basis for the projection to be done)",
        <http://purl.obolibrary.org/obo/IAO_0000233> "issue: https://github.com/OpenEnergyPlatform/ontology/issues/970
pull request: https://github.com/OpenEnergyPlatform/ontology/pull/1217
add based on axiom
issue: https://github.com/OpenEnergyPlatform/ontology/issues/1346
pull request: https://github.com/OpenEnergyPlatform/ontology/pull/1391",
        rdfs:label "scenario projection"@en
    
    SubClassOf: 
        <http://purl.obolibrary.org/obo/BFO_0000015>,
        OEO_00020226 some OEO_00000364,
        <http://purl.obolibrary.org/obo/BFO_0000051> some OEO_00000275,
        <http://purl.obolibrary.org/obo/RO_0002234> some OEO_00020013
    
    
Class: OEO_00010296

    Annotations: 
        <http://purl.obolibrary.org/obo/IAO_0000115> "A primary energy consumption calculation method is a methodology to calculate primary energy consumption.",
        <http://purl.obolibrary.org/obo/IAO_0000233> "issue: https://github.com/OpenEnergyPlatform/ontology/issues/1129
pull request: https://github.com/OpenEnergyPlatform/ontology/pull/1306

Move to oeo-shared:
issue: https://github.com/OpenEnergyPlatform/ontology/issues/1400
pull request: https://github.com/OpenEnergyPlatform/ontology/pull/1463

rework module structure 
issue: https://github.com/OpenEnergyPlatform/ontology/issues/1592
pull request: https://github.com/OpenEnergyPlatform/ontology/pull/1652",
        rdfs:label "primary energy consumption calculation method"@en
    
    SubClassOf: 
        OEO_00020166
    
    
Class: OEO_00010297

    Annotations: 
        <http://purl.obolibrary.org/obo/IAO_0000115> "A substitution method is a primary energy consumption calculation method that treats renewable energy carriers as if they have similar conversion losses as a specified fossil reference energy carrier.",
        <http://purl.obolibrary.org/obo/IAO_0000233> "issue: https://github.com/OpenEnergyPlatform/ontology/issues/1129
pull request: https://github.com/OpenEnergyPlatform/ontology/pull/1306
rework module structure 
issue: https://github.com/OpenEnergyPlatform/ontology/issues/1592
pull request: https://github.com/OpenEnergyPlatform/ontology/pull/1652",
        rdfs:label "substitution method"@en
    
    SubClassOf: 
        OEO_00010296
    
    
Class: OEO_00010298

    Annotations: 
        <http://purl.obolibrary.org/obo/IAO_0000115> "A direct equivalent method is a primary energy consumption calculation method that quantifies renewable and nuclear energies using its secondary energy content assuming no conversion losses.",
        <http://purl.obolibrary.org/obo/IAO_0000233> "issue: https://github.com/OpenEnergyPlatform/ontology/issues/1129
pull request: https://github.com/OpenEnergyPlatform/ontology/pull/1306
rework module structure 
issue: https://github.com/OpenEnergyPlatform/ontology/issues/1592
pull request: https://github.com/OpenEnergyPlatform/ontology/pull/1652",
        rdfs:label "direct equivalent method"@en
    
    SubClassOf: 
        OEO_00010296
    
    
Class: OEO_00010299

    Annotations: 
        <http://purl.obolibrary.org/obo/IAO_0000115> "A physical method is a method to calculate primary energy consumption that quantifies renewable and nuclear energies by attributing an efficiency value each.",
        <http://purl.obolibrary.org/obo/IAO_0000233> "issue: https://github.com/OpenEnergyPlatform/ontology/issues/1129
pull request: https://github.com/OpenEnergyPlatform/ontology/pull/1306
rework module structure 
issue: https://github.com/OpenEnergyPlatform/ontology/issues/1592
pull request: https://github.com/OpenEnergyPlatform/ontology/pull/1652",
        rdfs:label "physical method"@en
    
    SubClassOf: 
        OEO_00010296
    
    
Class: OEO_00010404

    Annotations: 
        <http://purl.obolibrary.org/obo/IAO_0000115> "An energy balance data set is an empirical data set that describes a specified set of energy transformations and a specified set of energy carriers in a spatial region for a specific time step (usually a year).",
        <http://purl.obolibrary.org/obo/IAO_0000233> "issue: https://github.com/OpenEnergyPlatform/ontology/issues/1400
pull request: https://github.com/OpenEnergyPlatform/ontology/pull/1463

rework module structure 
issue: https://github.com/OpenEnergyPlatform/ontology/issues/1592
pull request: https://github.com/OpenEnergyPlatform/ontology/pull/1652

change label 
issue: https://github.com/OpenEnergyPlatform/ontology/issues/1549
pull request: https://github.com/OpenEnergyPlatform/ontology/pull/1717",
        rdfs:label "energy balance data set"@en
    
    SubClassOf: 
        OEO_00000149,
        <http://purl.obolibrary.org/obo/IAO_0000136> exactly 1 OEO_00030033,
        <http://purl.obolibrary.org/obo/IAO_0000136> exactly 1 <http://purl.obolibrary.org/obo/BFO_0000006>
    
    
Class: OEO_00010405

    Annotations: 
        <http://purl.obolibrary.org/obo/IAO_0000115> "An energy balance collection is a data set of energy balances for various time steps and/or temporal regions.",
        <http://purl.obolibrary.org/obo/IAO_0000233> "issue: https://github.com/OpenEnergyPlatform/ontology/issues/1400
pull request: https://github.com/OpenEnergyPlatform/ontology/pull/1463",
        rdfs:label "energy balance collection"@en
    
    SubClassOf: 
        <http://purl.obolibrary.org/obo/IAO_0000100>,
        <http://purl.obolibrary.org/obo/BFO_0000051> some OEO_00010404,
        <http://purl.obolibrary.org/obo/IAO_0000136> some OEO_00030033,
        <http://purl.obolibrary.org/obo/IAO_0000136> some <http://purl.obolibrary.org/obo/BFO_0000006>
    
    
Class: OEO_00010406

    Annotations: 
        <http://purl.obolibrary.org/obo/IAO_0000115> "An energy balance calculation method is a methodology to calculate an energy balance.",
        <http://purl.obolibrary.org/obo/IAO_0000233> "issue: https://github.com/OpenEnergyPlatform/ontology/issues/1400
pull request: https://github.com/OpenEnergyPlatform/ontology/pull/1463

rework module structure 
issue: https://github.com/OpenEnergyPlatform/ontology/issues/1592
pull request: https://github.com/OpenEnergyPlatform/ontology/pull/1652",
        rdfs:label "energy balance calculation method"@en
    
    SubClassOf: 
        OEO_00020166,
        <http://purl.obolibrary.org/obo/BFO_0000051> some OEO_00010296,
        <http://purl.obolibrary.org/obo/IAO_0000136> some OEO_00010404
    
    
Class: OEO_00010411

    Annotations: 
        <http://purl.obolibrary.org/obo/IAO_0000115> "A forecast is an information content entity that contains statements about the most probable future development predicted with the help of past and present data.",
        <http://purl.obolibrary.org/obo/IAO_0000233> "issue: https://github.com/OpenEnergyPlatform/ontology/issues/1501
pull request: https://github.com/OpenEnergyPlatform/ontology/pull/1544",
        rdfs:label "forecast"@en
    
    SubClassOf: 
        <http://purl.obolibrary.org/obo/IAO_0000030>
    
    
Class: OEO_00010412

    Annotations: 
        <http://purl.obolibrary.org/obo/IAO_0000115> "A creative work licence is a copyright license that determines ownership and permissions for literary work and multimedia work that combines various media types such as text, audio, images, animations, video and interactive content and its collections.",
        <http://purl.obolibrary.org/obo/IAO_0000118> "creative work license",
        <http://purl.obolibrary.org/obo/IAO_0000233> "issue: https://github.com/OpenEnergyPlatform/ontology/issues/1275
pull request: https://github.com/OpenEnergyPlatform/ontology/pull/1547

rework module structure 
issue: https://github.com/OpenEnergyPlatform/ontology/issues/1592
pull request: https://github.com/OpenEnergyPlatform/ontology/pull/1652",
        rdfs:label "creative work licence"@en
    
    SubClassOf: 
        OEO_00020185
    
    
Class: OEO_00010422

    Annotations: 
        <http://purl.obolibrary.org/obo/IAO_0000115> "A boolean value is an variable information content entity that can only be true or false.",
        <http://purl.obolibrary.org/obo/IAO_0000118> "truth value",
        <http://purl.obolibrary.org/obo/IAO_0000233> "issue: https://github.com/OpenEnergyPlatform/ontology/issues/1148
pull request: https://github.com/OpenEnergyPlatform/ontology/pull/1255",
        rdfs:label "boolean value"@en
    
    SubClassOf: 
        <http://purl.obolibrary.org/obo/IAO_0000030>
    
    
Class: OEO_00020011

    SubClassOf: 
        OEO_00000522 some OEO_00020072
    
    
Class: OEO_00020012

    
Class: OEO_00020013

    Annotations: 
        <http://purl.obolibrary.org/obo/IAO_0000115> "Output data is endogenous data that is determined by a model calculation and presented as a result.",
        <http://purl.obolibrary.org/obo/IAO_0000118> "modelling results",
        <http://purl.obolibrary.org/obo/IAO_0000233> "issue: https://github.com/OpenEnergyPlatform/ontology/issues/520
pull request: https://github.com/OpenEnergyPlatform/ontology/pull/536

add alternative term
pull request: https://github.com/OpenEnergyPlatform/ontology/pull/1113",
        rdfs:label "output data"@en
    
    SubClassOf: 
        OEO_00030030
    
    
Class: OEO_00020015

    
Class: OEO_00020016

    Annotations: 
        <http://purl.obolibrary.org/obo/IAO_0000115> "A model descriptor is an information content entity that contains information about some model."@en,
        <http://purl.obolibrary.org/obo/IAO_0000233> "issue: https://github.com/OpenEnergyPlatform/ontology/issues/82
pull request: https://github.com/OpenEnergyPlatform/ontology/pull/577

Add SubclassOf axiom:
issue: https://github.com/OpenEnergyPlatform/ontology/issues/1386
pull request: https://github.com/OpenEnergyPlatform/ontology/pull/1387

rework module structure 
issue: https://github.com/OpenEnergyPlatform/ontology/issues/1592
pull request: https://github.com/OpenEnergyPlatform/ontology/pull/1652",
        rdfs:label "model descriptor"@en
    
    EquivalentTo: 
        <http://purl.obolibrary.org/obo/IAO_0000030>
         and (<http://purl.obolibrary.org/obo/IAO_0000136> some OEO_00000274)
    
    SubClassOf: 
        <http://purl.obolibrary.org/obo/IAO_0000030>
    
    
Class: OEO_00020017

    Annotations: 
        <http://purl.obolibrary.org/obo/IAO_0000115> "A analytical approach is a model descriptor that contains information about the analysis strategy of a model.",
        <http://purl.obolibrary.org/obo/IAO_0000233> "issue: https://github.com/OpenEnergyPlatform/ontology/issues/82
pull request: https://github.com/OpenEnergyPlatform/ontology/pull/577
fix typo of label
pull request: https://github.com/OpenEnergyPlatform/ontology/pull/981",
        rdfs:label "analytical approach"@en
    
    SubClassOf: 
        OEO_00020016
    
    
Class: OEO_00020018

    Annotations: 
        <http://purl.obolibrary.org/obo/IAO_0000115> "A methodical focus is a model descriptor that specifies the primary calculation method used in a model.",
        <http://purl.obolibrary.org/obo/IAO_0000118> "methodology",
        <http://purl.obolibrary.org/obo/IAO_0000233> "issue: https://github.com/OpenEnergyPlatform/ontology/issues/82
pull request: https://github.com/OpenEnergyPlatform/ontology/pull/577
alternative term
pull request: https://github.com/OpenEnergyPlatform/ontology/pull/1011
rework module structure 
issue: https://github.com/OpenEnergyPlatform/ontology/issues/1592
pull request: https://github.com/OpenEnergyPlatform/ontology/pull/1652",
        rdfs:label "methodical focus"@en
    
    SubClassOf: 
        OEO_00020016,
        <http://purl.obolibrary.org/obo/IAO_0000136> some OEO_00000275
    
    
Class: OEO_00020019

    Annotations: 
        <http://purl.obolibrary.org/obo/IAO_0000115> "A primary modelling purpose is a model descriptor stating the main purpose of a model.",
        <http://purl.obolibrary.org/obo/IAO_0000118> "primary modeling purpose",
        <http://purl.obolibrary.org/obo/IAO_0000233> "issue: https://github.com/OpenEnergyPlatform/ontology/issues/82
pull request: https://github.com/OpenEnergyPlatform/ontology/pull/577",
        rdfs:label "primary modelling purpose"@en
    
    SubClassOf: 
        OEO_00020016
    
    
Class: OEO_00020022

    Annotations: 
        <http://purl.obolibrary.org/obo/IAO_0000233> "A model documentation is a model descriptor that contains a detailed description of a model.",
        <http://purl.obolibrary.org/obo/IAO_0000233> "issue: https://github.com/OpenEnergyPlatform/ontology/issues/82
pull request: https://github.com/OpenEnergyPlatform/ontology/pull/577",
        rdfs:label "model documentation"@en
    
    SubClassOf: 
        OEO_00020016
    
    
Class: OEO_00020023

    Annotations: 
        <http://purl.obolibrary.org/obo/IAO_0000115> "Top down is an analytical approach where design starts from the system as a whole. The system is then divided into smaller sub-applications with more details. Each part again goes through the top down approach till the complete system is designed with all minute details. Top down approach is also termed as breaking the bigger problem into smaller problems and solving them individually in a recursive manner. A top down model is based on a decomposition approach.",
        <http://purl.obolibrary.org/obo/IAO_0000233> "Convert to subclass and add definition:
issue: https://github.com/OpenEnergyPlatform/ontology/issues/1147
pull request: https://github.com/OpenEnergyPlatform/ontology/pull/1302",
        rdfs:label "top down"@en
    
    SubClassOf: 
        OEO_00020017
    
    
Class: OEO_00020024

    Annotations: 
        <http://purl.obolibrary.org/obo/IAO_0000115> "Bottom up is an analytical approach where parts of the system are defined in details. Once these parts are designed and developed, then these parts or components are linked together to prepare a bigger component. This approach is repeated until the complete system is built. A bottom up model is based on a composition approach.",
        <http://purl.obolibrary.org/obo/IAO_0000233> "Convert to subclass and add definition:
issue: https://github.com/OpenEnergyPlatform/ontology/issues/1147
pull request: https://github.com/OpenEnergyPlatform/ontology/pull/1302",
        rdfs:label "bottom up"@en
    
    SubClassOf: 
        OEO_00020017
    
    
Class: OEO_00020026

    Annotations: 
        <http://purl.obolibrary.org/obo/IAO_0000115> "Hybrid is an analytical approach that combines the top down and the bottom up approach. Some parts are based on composition approach while other parts are based on decomposition approach.",
        <http://purl.obolibrary.org/obo/IAO_0000233> "Convert to subclass and add definition:
issue: https://github.com/OpenEnergyPlatform/ontology/issues/1147
pull request: https://github.com/OpenEnergyPlatform/ontology/pull/1302",
        rdfs:label "hybrid"@en
    
    SubClassOf: 
        OEO_00020017
    
    
Class: OEO_00020032

    Annotations: 
        <http://purl.obolibrary.org/obo/IAO_0000112> "In a study, the spatial focus of the investigation lies on one European country, e.g. Germany. This is the study region.
The study region is not modelled as a whole, but several subregions are modelled, e.g. German Federal States. These are study subregions.
In the study, a spatial region outside the study region plays a role. E.g. for modelling the electricity transfer between Germany and its neighbouring countries. In this example, the neighbouring countries represent the interacting / external region.
The union of the study region and the interacting/ external region ist the considered region.",
        <http://purl.obolibrary.org/obo/IAO_0000115> "A study region is a spatial region that is under investigation and consists entirely of one or more subregions.",
        <http://purl.obolibrary.org/obo/IAO_0000233> "issue: https://github.com/OpenEnergyPlatform/ontology/issues/475
pull request: https://github.com/OpenEnergyPlatform/ontology/pull/585

rework module structure 
issue: https://github.com/OpenEnergyPlatform/ontology/issues/1592
pull request: https://github.com/OpenEnergyPlatform/ontology/pull/1652",
        rdfs:label "study region"@en
    
    SubClassOf: 
        <http://purl.obolibrary.org/obo/BFO_0000006>
    
    
Class: OEO_00020033

    Annotations: 
        <http://purl.obolibrary.org/obo/IAO_0000115> "A subregion is a spatial region that is a part of spatial region.",
        <http://purl.obolibrary.org/obo/IAO_0000233> "issue: https://github.com/OpenEnergyPlatform/ontology/issues/475
pull request: https://github.com/OpenEnergyPlatform/ontology/pull/585",
        rdfs:label "subregion"@en
    
    SubClassOf: 
        <http://purl.obolibrary.org/obo/BFO_0000006>
    
    
Class: OEO_00020034

    Annotations: 
        <http://purl.obolibrary.org/obo/IAO_0000112> "In a study, the spatial focus of the investigation lies on one European country, e.g. Germany. This is the study region.
The study region is not modelled as a whole, but several subregions are modelled, e.g. German Federal States. These are study subregions.
In the study, a spatial region outside the study region plays a role. E.g. for modelling the electricity transfer between Germany and its neighbouring countries. In this example, the neighbouring countries represent the interacting / external region.
The union of the study region and the interacting/ external region ist the considered region.",
        <http://purl.obolibrary.org/obo/IAO_0000115> "A study subregion is a subregion of a study region.",
        <http://purl.obolibrary.org/obo/IAO_0000233> "issue: https://github.com/OpenEnergyPlatform/ontology/issues/475
pull request: https://github.com/OpenEnergyPlatform/ontology/pull/585",
        rdfs:label "study subregion"@en
    
    SubClassOf: 
        OEO_00020033
    
    
Class: OEO_00020035

    Annotations: 
        <http://purl.obolibrary.org/obo/IAO_0000112> "In a study, the spatial focus of the investigation lies on one European country, e.g. Germany. This is the study region.
The study region is not modelled as a whole, but several subregions are modelled, e.g. German Federal States. These are study subregions.
In the study, a spatial region outside the study region plays a role. E.g. for modelling the electricity transfer between Germany and its neighbouring countries. In this example, the neighbouring countries represent the interacting / external region.
The union of the study region and the interacting/ external region ist the considered region.",
        <http://purl.obolibrary.org/obo/IAO_0000115> "A considered region is a spatial region that is used in an analysis.",
        <http://purl.obolibrary.org/obo/IAO_0000233> "issue: https://github.com/OpenEnergyPlatform/ontology/issues/475
pull request: https://github.com/OpenEnergyPlatform/ontology/pull/585

rework module structure 
issue: https://github.com/OpenEnergyPlatform/ontology/issues/1592
pull request: https://github.com/OpenEnergyPlatform/ontology/pull/1652",
        rdfs:label "considered region"@en
    
    SubClassOf: 
        <http://purl.obolibrary.org/obo/BFO_0000006>
    
    
Class: OEO_00020036

    Annotations: 
        <http://purl.obolibrary.org/obo/IAO_0000112> "In a study, the spatial focus of the investigation lies on one European country, e.g. Germany. This is the study region.
The study region is not modelled as a whole, but several subregions are modelled, e.g. German Federal States. These are study subregions.
In the study, a spatial region outside the study region plays a role. E.g. for modelling the electricity transfer between Germany and its neighbouring countries. In this example, the neighbouring countries represent the interacting / external region.
The union of the study region and the interacting/ external region ist the considered region.",
        <http://purl.obolibrary.org/obo/IAO_0000115> "An interacting region is a spatial region that interacts with a study region. It is part of a considered region, but not a study region.",
        <http://purl.obolibrary.org/obo/IAO_0000118> "external region",
        <http://purl.obolibrary.org/obo/IAO_0000233> "issue: https://github.com/OpenEnergyPlatform/ontology/issues/475
pull request: https://github.com/OpenEnergyPlatform/ontology/pull/585",
        rdfs:label "interacting region"@en
    
    SubClassOf: 
        <http://purl.obolibrary.org/obo/BFO_0000006>
    
    
Class: OEO_00020072

    Annotations: 
        <http://purl.obolibrary.org/obo/IAO_0000115> "An analysis scope is an information content entity that describes the boundaries of what a study or scenario covers.",
        <http://purl.obolibrary.org/obo/IAO_0000233> "issue: https://github.com/OpenEnergyPlatform/ontology/issues/638
pull request: https://github.com/OpenEnergyPlatform/ontology/pull/764

Add 'is about' axioms:
issue: https://github.com/OpenEnergyPlatform/ontology/issues/1059
pull request: https://github.com/OpenEnergyPlatform/ontology/pull/1286

rework module structure 
issue: https://github.com/OpenEnergyPlatform/ontology/issues/1592
pull request: https://github.com/OpenEnergyPlatform/ontology/pull/1652",
        rdfs:label "analysis scope"@en
    
    SubClassOf: 
        <http://purl.obolibrary.org/obo/IAO_0000030>,
        <http://purl.obolibrary.org/obo/IAO_0000136> some OEO_00020018,
        <http://purl.obolibrary.org/obo/IAO_0000136> some OEO_00020032,
        <http://purl.obolibrary.org/obo/IAO_0000136> some OEO_00020035,
        <http://purl.obolibrary.org/obo/IAO_0000136> some OEO_00020097,
        <http://purl.obolibrary.org/obo/IAO_0000136> some OEO_00020098
    
    
Class: OEO_00020089

    Annotations: 
        <http://purl.obolibrary.org/obo/IAO_0000115> "A typical period is a time series that represents a couple of real time periods that have certain characteristics in common, e.g. seasonal specifications, weekly routines, etc. It doesn't refer to a real date. Typical periods are used to reduce computing time of energy system models.",
        <http://purl.obolibrary.org/obo/IAO_0000119> "Definition adapted from: https://www.enargus.de/pub/bscw.cgi/d13068-2/*/*/Typtag.html?op=Wiki.getwiki&scope=all",
        <http://purl.obolibrary.org/obo/IAO_0000233> "add axiom `uses some 'aggregation type'`:
issue: https://github.com/OpenEnergyPlatform/ontology/issues/880
pull request: https://github.com/OpenEnergyPlatform/ontology/pull/883

issue: https://github.com/OpenEnergyPlatform/ontology/issues/830
pull request: https://github.com/OpenEnergyPlatform/ontology/pull/875",
        rdfs:label "typical period"@en
    
    SubClassOf: 
        OEO_00030034,
        OEO_00000503 some OEO_00140068
    
    
Class: OEO_00020090

    Annotations: 
        <http://purl.obolibrary.org/obo/IAO_0000115> "A typical year is a typical period with the duration of one year.",
        <http://purl.obolibrary.org/obo/IAO_0000233> "issue: https://github.com/OpenEnergyPlatform/ontology/issues/830
pull request: https://github.com/OpenEnergyPlatform/ontology/pull/875
add axiom
pull request: https://github.com/OpenEnergyPlatform/ontology/pull/882",
        rdfs:label "typical year"@en
    
    SubClassOf: 
        OEO_00020089,
        <http://purl.obolibrary.org/obo/BFO_0000051> some 
            (OEO_00030035
             and (OEO_00040010 some <http://purl.obolibrary.org/obo/UO_0000036>)
             and (OEO_00140178 value 1))
    
    DisjointWith: 
        OEO_00020091
    
    
Class: OEO_00020091

    Annotations: 
        <http://purl.obolibrary.org/obo/IAO_0000115> "A typical day is a typical period with the duration of one day.",
        <http://purl.obolibrary.org/obo/IAO_0000233> "issue: https://github.com/OpenEnergyPlatform/ontology/issues/830
pull request: https://github.com/OpenEnergyPlatform/ontology/pull/875
add axiom
pull request: https://github.com/OpenEnergyPlatform/ontology/pull/882",
        rdfs:label "typical day"@en
    
    SubClassOf: 
        OEO_00020089,
        <http://purl.obolibrary.org/obo/BFO_0000051> some 
            (OEO_00030035
             and (OEO_00040010 some <http://purl.obolibrary.org/obo/UO_0000033>)
             and (OEO_00140178 value 1))
    
    DisjointWith: 
        OEO_00020090
    
    
Class: OEO_00020093

    Annotations: 
        <http://purl.obolibrary.org/obo/IAO_0000115> "A target description is an information content entity that contains statements about a desired future state of a system that a person or organisation commits to in a legally binding way.",
        <http://purl.obolibrary.org/obo/IAO_0000233> "issue: https://github.com/OpenEnergyPlatform/ontology/issues/28
pull request: https://github.com/OpenEnergyPlatform/ontology/pull/881",
        rdfs:label "target description"@en
    
    SubClassOf: 
        <http://purl.obolibrary.org/obo/IAO_0000030>
    
    
Class: OEO_00020097

    Annotations: 
        <http://purl.obolibrary.org/obo/IAO_0000115> "A scenario year is a time step that has a duration of one year and is part of a scenario horizon.",
        <http://purl.obolibrary.org/obo/IAO_0000233> "issue: https://github.com/OpenEnergyPlatform/ontology/issues/474
pull request: https://github.com/OpenEnergyPlatform/ontology/pull/882

rework module structure 
issue: https://github.com/OpenEnergyPlatform/ontology/issues/1592
pull request: https://github.com/OpenEnergyPlatform/ontology/pull/1652",
        rdfs:label "scenario year"@en
    
    SubClassOf: 
        OEO_00030033,
        <http://purl.obolibrary.org/obo/BFO_0000050> some OEO_00020098,
        <http://purl.obolibrary.org/obo/BFO_0000051> some 
            (OEO_00030035
             and (OEO_00040010 some <http://purl.obolibrary.org/obo/UO_0000036>)
             and (OEO_00140178 value 1))
    
    
Class: OEO_00020098

    Annotations: 
        <http://purl.obolibrary.org/obo/IAO_0000115> "A scenario horizon is a time step that is under investigation and consists entirely of one or more scenario years.",
        <http://purl.obolibrary.org/obo/IAO_0000233> "issue: https://github.com/OpenEnergyPlatform/ontology/issues/474
pull request: https://github.com/OpenEnergyPlatform/ontology/pull/882

rework module structure 
issue: https://github.com/OpenEnergyPlatform/ontology/issues/1592
pull request: https://github.com/OpenEnergyPlatform/ontology/pull/1652",
        rdfs:label "scenario horizon"@en
    
    SubClassOf: 
        OEO_00030033,
        <http://purl.obolibrary.org/obo/BFO_0000051> some OEO_00020097,
        <http://purl.obolibrary.org/obo/BFO_0000051> some 
            (OEO_00030035
             and (OEO_00040010 some <http://purl.obolibrary.org/obo/UO_0000036>))
    
    
Class: OEO_00020099

    Annotations: 
        <http://purl.obolibrary.org/obo/IAO_0000115> "A meteorological year is a time step in which meteorological data was collected and that has a duration of one year.",
        <http://purl.obolibrary.org/obo/IAO_0000233> "issue: https://github.com/OpenEnergyPlatform/ontology/issues/474
pull request: https://github.com/OpenEnergyPlatform/ontology/pull/882",
        rdfs:label "meteorological year"@en
    
    SubClassOf: 
        OEO_00030033,
        <http://purl.obolibrary.org/obo/BFO_0000051> some 
            (OEO_00030035
             and (OEO_00040010 some <http://purl.obolibrary.org/obo/UO_0000036>)
             and (OEO_00140178 value 1))
    
    
Class: OEO_00020100

    Annotations: 
        <http://purl.obolibrary.org/obo/IAO_0000115> "A weather time series is a time series that contains data about a specific meteorological year.",
        <http://purl.obolibrary.org/obo/IAO_0000118> "meteorological time series",
        <http://purl.obolibrary.org/obo/IAO_0000233> "issue: https://github.com/OpenEnergyPlatform/ontology/issues/474
pull request: https://github.com/OpenEnergyPlatform/ontology/pull/882",
        rdfs:label "weather time series"@en
    
    SubClassOf: 
        OEO_00030034,
        <http://purl.obolibrary.org/obo/IAO_0000136> some OEO_00020099
    
    
Class: OEO_00020101

    Annotations: 
        <http://purl.obolibrary.org/obo/IAO_0000115> "A scenario time series is a time series that contains data about a specific scenario year.",
        <http://purl.obolibrary.org/obo/IAO_0000233> "issue: https://github.com/OpenEnergyPlatform/ontology/issues/474
pull request: https://github.com/OpenEnergyPlatform/ontology/pull/882",
        rdfs:label "scenario time series"@en
    
    SubClassOf: 
        OEO_00030034,
        <http://purl.obolibrary.org/obo/IAO_0000136> some OEO_00020097
    
    
Class: OEO_00020121

    Annotations: 
        <http://purl.obolibrary.org/obo/IAO_0000115> "Resolution is a quality of a dataset that indicates the level of detail of the data.",
        <http://purl.obolibrary.org/obo/IAO_0000233> "issue: https://github.com/OpenEnergyPlatform/ontology/issues/849
pull request: https://github.com/OpenEnergyPlatform/ontology/pull/972

add 'has bearer' axiom
issue: https://github.com/OpenEnergyPlatform/ontology/issues/1305
pull request: https://github.com/OpenEnergyPlatform/ontology/pull/1310

rework module structure 
issue: https://github.com/OpenEnergyPlatform/ontology/issues/1592
pull request: https://github.com/OpenEnergyPlatform/ontology/pull/1652",
        rdfs:label "resolution"@en
    
    SubClassOf: 
        <http://purl.obolibrary.org/obo/BFO_0000019>,
        OEO_00010121 some <http://purl.obolibrary.org/obo/IAO_0000100>
    
    
Class: OEO_00020122

    Annotations: 
        <http://purl.obolibrary.org/obo/IAO_0000115> "Temporal resolution is the resolution of a time series that indicates time-dependent the level of detail.",
        <http://purl.obolibrary.org/obo/IAO_0000233> "issue: https://github.com/OpenEnergyPlatform/ontology/issues/849
pull request: https://github.com/OpenEnergyPlatform/ontology/pull/912

add individuals
pull request: https://github.com/OpenEnergyPlatform/ontology/pull/972

add 'has bearer' axiom
issue: https://github.com/OpenEnergyPlatform/ontology/issues/1305
pull request: https://github.com/OpenEnergyPlatform/ontology/pull/1310

rework module structure 
issue: https://github.com/OpenEnergyPlatform/ontology/issues/1592
pull request: https://github.com/OpenEnergyPlatform/ontology/pull/1652",
        rdfs:label "temporal resolution"@en
    
    SubClassOf: 
        OEO_00020121,
        OEO_00010121 some OEO_00030034
    
    DisjointWith: 
        OEO_00020123
    
    
Class: OEO_00020123

    Annotations: 
        <http://purl.obolibrary.org/obo/IAO_0000115> "Spatial resolution is the resolution of a georeferenced dataset that indicates the geographical level of detail.",
        <http://purl.obolibrary.org/obo/IAO_0000233> "issue: https://github.com/OpenEnergyPlatform/ontology/issues/849
pull request: https://github.com/OpenEnergyPlatform/ontology/pull/912

rework module structure 
issue: https://github.com/OpenEnergyPlatform/ontology/issues/1592
pull request: https://github.com/OpenEnergyPlatform/ontology/pull/1652",
        rdfs:label "spatial resolution"@en
    
    SubClassOf: 
        OEO_00020121
    
    DisjointWith: 
        OEO_00020122
    
    
Class: OEO_00020166

    
Class: OEO_00020185

    Annotations: 
        <http://purl.obolibrary.org/obo/IAO_0000115> "A copyright licence is a licence that states the ownership and contractually sets the rights and obligations to use, copy, and distribute a creative work.",
        <http://purl.obolibrary.org/obo/IAO_0000118> "copyright license",
        <http://purl.obolibrary.org/obo/IAO_0000233> "add relation has copyright license
issue https://github.com/OpenEnergyPlatform/ontology/issues/1061
pull request https://github.com/OpenEnergyPlatform/ontology/pull/1090

Harmonise use of British English:
issue: https://github.com/OpenEnergyPlatform/ontology/issues/1275
pull request: https://github.com/OpenEnergyPlatform/ontology/pull/1547

rework module structure 
issue: https://github.com/OpenEnergyPlatform/ontology/issues/1592
pull request: https://github.com/OpenEnergyPlatform/ontology/pull/1652",
        rdfs:label "copyright licence"@en
    
    SubClassOf: 
        OEO_00020015
    
    
Class: OEO_00020186

    Annotations: 
        <http://purl.obolibrary.org/obo/IAO_0000115> "A data licence is a licence that determines ownership, database protection, and permissions for data.",
        <http://purl.obolibrary.org/obo/IAO_0000118> "data license",
        <http://purl.obolibrary.org/obo/IAO_0000233> "issue https://github.com/OpenEnergyPlatform/ontology/issues/1061
pull request https://github.com/OpenEnergyPlatform/ontology/pull/1090

Harmonise use of British English:
issue: https://github.com/OpenEnergyPlatform/ontology/issues/1275
pull request: https://github.com/OpenEnergyPlatform/ontology/pull/1547

rework module structure 
issue: https://github.com/OpenEnergyPlatform/ontology/issues/1592
pull request: https://github.com/OpenEnergyPlatform/ontology/pull/1652",
        rdfs:label "data licence"@en
    
    SubClassOf: 
        OEO_00020015
    
    
Class: OEO_00020187

    Annotations: 
        <http://purl.obolibrary.org/obo/IAO_0000115> "A software licence is a copyright licence that determines ownership and permissions for software, code, or models.",
        <http://purl.obolibrary.org/obo/IAO_0000118> "software license",
        <http://purl.obolibrary.org/obo/IAO_0000233> "issue https://github.com/OpenEnergyPlatform/ontology/issues/1061
pull request https://github.com/OpenEnergyPlatform/ontology/pull/1090

Harmonise use of British English:
issue: https://github.com/OpenEnergyPlatform/ontology/issues/1275
pull request: https://github.com/OpenEnergyPlatform/ontology/pull/1547

rework module structure 
issue: https://github.com/OpenEnergyPlatform/ontology/issues/1592
pull request: https://github.com/OpenEnergyPlatform/ontology/pull/1652",
        rdfs:label "software licence"@en
    
    SubClassOf: 
        
            Annotations: <http://purl.obolibrary.org/obo/IAO_0000233> "fix wrong classification
issue: https://github.com/OpenEnergyPlatform/ontology/issues/1153
pull request: https://github.com/OpenEnergyPlatform/ontology/pull/1163"
        OEO_00020185
    
    
Class: OEO_00020227

    Annotations: 
        <http://purl.obolibrary.org/obo/IAO_0000115> "A scenario bundle is an information content entity that connects information about a scenario study and the associated scenario projections on the OEP via the OEKG.",
        <http://purl.obolibrary.org/obo/IAO_0000233> "issue: https://github.com/OpenEnergyPlatform/ontology/issues/1343
pull request: https://github.com/OpenEnergyPlatform/ontology/pull/1429",
        rdfs:label "scenario bundle"@en
    
    SubClassOf: 
        <http://purl.obolibrary.org/obo/IAO_0000030>,
        <http://purl.obolibrary.org/obo/IAO_0000136> some OEO_00010252
    
    
Class: OEO_00020247

    Annotations: 
        <http://purl.obolibrary.org/obo/IAO_0000115> "A target driven scenario is a scenario that contains certain target constraints/ statements that in a possible future shall be realized. The path how the targets will be met is not predefined in the scenario.",
        <http://purl.obolibrary.org/obo/IAO_0000233> "issue: https://github.com/OpenEnergyPlatform/ontology/issues/1110
pull request: https://github.com/OpenEnergyPlatform/ontology/pull/1459
make equivalent
issue: https://github.com/OpenEnergyPlatform/ontology/issues/1329
pull request: https://github.com/OpenEnergyPlatform/ontology/pull/1642",
        rdfs:label "target driven scenario"@en
    
    EquivalentTo: 
        OEO_00000364
         and (<http://purl.obolibrary.org/obo/IAO_0000136> some OEO_00020093)
    
    SubClassOf: 
        OEO_00000364
    
    
Class: OEO_00020248

    Annotations: 
        <http://purl.obolibrary.org/obo/IAO_0000115> "An explorative scenario is a scenario that contains certain constraints / statements regarding measures that are taken in the near future / today to explore where these measures will lead to in a later future. The later future is not predefined in the scenario.",
        <http://purl.obolibrary.org/obo/IAO_0000233> "issue: https://github.com/OpenEnergyPlatform/ontology/issues/1110
pull request: https://github.com/OpenEnergyPlatform/ontology/pull/1459
move to oeo-shared
issue: https://github.com/OpenEnergyPlatform/ontology/issues/1329
pull request: https://github.com/OpenEnergyPlatform/ontology/pull/1642
rework module structure 
issue: https://github.com/OpenEnergyPlatform/ontology/issues/1592
pull request: https://github.com/OpenEnergyPlatform/ontology/pull/1652",
        rdfs:label "explorative scenario"@en
    
    SubClassOf: 
        OEO_00000364
    
    
Class: OEO_00020309

    Annotations: 
        <http://purl.obolibrary.org/obo/IAO_0000115> "A policy scenario is a scenario in which certain policy instruments or transformative measures and their impacts are assessed.",
        <http://purl.obolibrary.org/obo/IAO_0000233> "issue: https://github.com/OpenEnergyPlatform/ontology/issues/1329
pull request: https://github.com/OpenEnergyPlatform/ontology/pull/1614
pull request: https://github.com/OpenEnergyPlatform/ontology/pull/1642
rework module structure 
issue: https://github.com/OpenEnergyPlatform/ontology/issues/1592
pull request: https://github.com/OpenEnergyPlatform/ontology/pull/1652",
        rdfs:label "policy scenario"@en
    
    SubClassOf: 
        OEO_00020248
    
    
Class: OEO_00020310

    Annotations: 
        <http://purl.obolibrary.org/obo/IAO_0000115> "A without measures scenario (WOM) is a policy scenario that excludes all policy instruments and transformative measures which are planned, adopted or implemented.",
        <http://purl.obolibrary.org/obo/IAO_0000118> "WOM scenario",
        <http://purl.obolibrary.org/obo/IAO_0000118> "baseline scenario",
        <http://purl.obolibrary.org/obo/IAO_0000119> "Derived from https://eur-lex.europa.eu/legal-content/EN/TXT/HTML/?uri=CELEX:32018R1999&from=EN#d1e968-1-1 Article 2",
        <http://purl.obolibrary.org/obo/IAO_0000233> "issue: https://github.com/OpenEnergyPlatform/ontology/issues/1329
pull request: https://github.com/OpenEnergyPlatform/ontology/pull/1614

rework module structure 
issue: https://github.com/OpenEnergyPlatform/ontology/issues/1592
pull request: https://github.com/OpenEnergyPlatform/ontology/pull/1652",
        rdfs:label "without measures scenario"@en
    
    SubClassOf: 
        OEO_00020309
    
    
Class: OEO_00020311

    Annotations: 
        <http://purl.obolibrary.org/obo/IAO_0000115> "A with existing measures scenario (WEM) is a policy scenario that includes policy instruments and transformative measures that have been adopted and implemented.",
        <http://purl.obolibrary.org/obo/IAO_0000118> "WEM scenario",
        <http://purl.obolibrary.org/obo/IAO_0000118> "baseline scenario",
        <http://purl.obolibrary.org/obo/IAO_0000119> "Derived from https://eur-lex.europa.eu/legal-content/EN/TXT/HTML/?uri=CELEX:32018R1999&from=EN#d1e968-1-1 Article 2",
        <http://purl.obolibrary.org/obo/IAO_0000233> "issue: https://github.com/OpenEnergyPlatform/ontology/issues/1329
pull request: https://github.com/OpenEnergyPlatform/ontology/pull/1614

rework module structure 
issue: https://github.com/OpenEnergyPlatform/ontology/issues/1592
pull request: https://github.com/OpenEnergyPlatform/ontology/pull/1652",
        rdfs:label "with existing measures scenario"@en
    
    SubClassOf: 
        OEO_00020309
    
    
Class: OEO_00020312

    Annotations: 
        <http://purl.obolibrary.org/obo/IAO_0000115> "A with additional measures scenario (WAM) is a policy scenario that includes policy instruments and transformative measures which have been adopted and implemented to mitigate climate change or meet energy objectives, as well as policy instruments and transformative measures which are planned for that purpose.",
        <http://purl.obolibrary.org/obo/IAO_0000118> "WAM scenario",
        <http://purl.obolibrary.org/obo/IAO_0000119> "Derived from https://eur-lex.europa.eu/legal-content/EN/TXT/HTML/?uri=CELEX:32018R1999&from=EN#d1e968-1-1 Article 2",
        <http://purl.obolibrary.org/obo/IAO_0000233> "issue: https://github.com/OpenEnergyPlatform/ontology/issues/1329
pull request: https://github.com/OpenEnergyPlatform/ontology/pull/1614

rework module structure 
issue: https://github.com/OpenEnergyPlatform/ontology/issues/1592
pull request: https://github.com/OpenEnergyPlatform/ontology/pull/1652",
        rdfs:label "with additional measures scenario"@en
    
    SubClassOf: 
        OEO_00020309
    
    
Class: OEO_00020313

    Annotations: 
        <http://purl.obolibrary.org/obo/IAO_0000115> "A role of an information content entity, that indicates a benchmark, e.g. in a comparison.",
        <http://purl.obolibrary.org/obo/IAO_0000116> "Although contradicting to BFO2, we add the reference role to the generically dependent \"information content entity\", aware of the ongoing discussion.",
        <http://purl.obolibrary.org/obo/IAO_0000233> "issue: https://github.com/OpenEnergyPlatform/ontology/issues/1329
pull request: https://github.com/OpenEnergyPlatform/ontology/pull/1614

rework module structure 
issue: https://github.com/OpenEnergyPlatform/ontology/issues/1592
pull request: https://github.com/OpenEnergyPlatform/ontology/pull/1652",
        rdfs:label "reference role"@en
    
    SubClassOf: 
        <http://purl.obolibrary.org/obo/BFO_0000023>
    
    
Class: OEO_00020314

    Annotations: 
        <http://purl.obolibrary.org/obo/IAO_0000115> "A reference scenario is a scenario that is used as a reference, e.g. in a scenario comparison. It has the reference role.",
        <http://purl.obolibrary.org/obo/IAO_0000233> "issue: https://github.com/OpenEnergyPlatform/ontology/issues/1329
pull request: https://github.com/OpenEnergyPlatform/ontology/pull/1614

rework module structure 
issue: https://github.com/OpenEnergyPlatform/ontology/issues/1592
pull request: https://github.com/OpenEnergyPlatform/ontology/pull/1652",
        rdfs:label "reference scenario"@en
    
    EquivalentTo: 
        OEO_00000364
         and (<http://purl.obolibrary.org/obo/RO_0000087> some OEO_00020313)
    
    SubClassOf: 
        OEO_00000364
    
    
Class: OEO_00020317

    Annotations: 
        <http://purl.obolibrary.org/obo/IAO_0000115> "A greenhouse gas emission scenario is an emission scenario that describes a possible greenhouse gas emission trajectory.",
        <http://purl.obolibrary.org/obo/IAO_0000233> "issue: https://github.com/OpenEnergyPlatform/ontology/issues/1329
pull request: https://github.com/OpenEnergyPlatform/ontology/pull/1615

rework module structure 
issue: https://github.com/OpenEnergyPlatform/ontology/issues/1592
pull request: https://github.com/OpenEnergyPlatform/ontology/pull/1652",
        rdfs:label "greenhouse gas emission scenario"@en
    
    SubClassOf: 
        OEO_00030009
    
    
Class: OEO_00020321

    Annotations: 
        <http://purl.obolibrary.org/obo/IAO_0000115> "A CO2 emission scenario is an emission scenario that describes a possible CO2 emission trajectory.",
        <http://purl.obolibrary.org/obo/IAO_0000233> "issue: https://github.com/OpenEnergyPlatform/ontology/issues/1329
pull request: https://github.com/OpenEnergyPlatform/ontology/pull/1615

rework module structure 
issue: https://github.com/OpenEnergyPlatform/ontology/issues/1592
pull request: https://github.com/OpenEnergyPlatform/ontology/pull/1652",
        rdfs:label "CO2 emission scenario"@en
    
    SubClassOf: 
        OEO_00030009
    
    
Class: OEO_00020345

    Annotations: 
        <http://purl.obolibrary.org/obo/IAO_0000115> "A sufficiency scenario is a scenario that comprises sufficiency strategies.",
        <http://purl.obolibrary.org/obo/IAO_0000233> "issue: https://github.com/OpenEnergyPlatform/ontology/issues/1329
pull request: https://github.com/OpenEnergyPlatform/ontology/pull/1642

Make equivalent class
issue: https://github.com/OpenEnergyPlatform/ontology/issues/1553
pull request: https://github.com/OpenEnergyPlatform/ontology/pull/1648",
        rdfs:label "sufficiency scenario"@en
    
    SubClassOf: 
        OEO_00000364
    
    
Class: OEO_00020352

    
Class: OEO_00020353

    
Class: OEO_00020354

    Annotations: 
        <http://purl.obolibrary.org/obo/IAO_0000115> "A mathematical model is a information content artifact that represents a system and its behaviours mathematically.",
        <http://purl.obolibrary.org/obo/IAO_0000233> "issue:https://github.com/OpenEnergyPlatform/ontology/issues/1444
pull request: https://github.com/OpenEnergyPlatform/ontology/pull/1707",
        rdfs:label "mathematical model"@en
    
    SubClassOf: 
        <http://purl.obolibrary.org/obo/IAO_0000030>,
        <http://purl.obolibrary.org/obo/RO_0000087> some OEO_00020353
    
    
Class: OEO_00020355

    Annotations: 
        <http://purl.obolibrary.org/obo/IAO_0000115> "A scale model is model comprising of a spatial pattern of components arranged in such a way for them to represent a system.",
        <http://purl.obolibrary.org/obo/IAO_0000233> "issue:https://github.com/OpenEnergyPlatform/ontology/issues/1444
pull request: https://github.com/OpenEnergyPlatform/ontology/pull/1707",
        rdfs:label "scale model"@en
    
    SubClassOf: 
        OEO_00020352
    
    
Class: OEO_00030007

    Annotations: 
        <http://purl.obolibrary.org/obo/IAO_0000115> "A climate scenario is a scenario that describes a possible future state of a climate system.",
        <http://purl.obolibrary.org/obo/IAO_0000233> "issue: https://github.com/OpenEnergyPlatform/ontology/issues/328
pull request: https://github.com/OpenEnergyPlatform/ontology/pull/344

issue: https://github.com/OpenEnergyPlatform/ontology/issues/1329
pull request: https://github.com/OpenEnergyPlatform/ontology/pull/1615

move axiom to shared-axioms
issue: https://github.com/OpenEnergyPlatform/ontology/issues/1703
pull request: https://github.com/OpenEnergyPlatform/ontology/pull/1706",
        rdfs:label "climate scenario"@en
    
    SubClassOf: 
        OEO_00000364
    
    
Class: OEO_00030008

    Annotations: 
        <http://purl.obolibrary.org/obo/IAO_0000115> "An economic scenario is a scenario that describes a possible future state of economic systems.",
        <http://purl.obolibrary.org/obo/IAO_0000233> "issue: https://github.com/OpenEnergyPlatform/ontology/issues/328
pull request: https://github.com/OpenEnergyPlatform/ontology/pull/344 
make equivalent
issue: https://github.com/OpenEnergyPlatform/ontology/issues/1329
pull request: https://github.com/OpenEnergyPlatform/ontology/pull/1642",
        rdfs:label "economic scenario"@en
    
    SubClassOf: 
        OEO_00000364
    
    
Class: OEO_00030009

    Annotations: 
        <http://purl.obolibrary.org/obo/IAO_0000115> "An emission scenario is a scenario that describes a possible emission trajectory.",
        <http://purl.obolibrary.org/obo/IAO_0000233> "issue: https://github.com/OpenEnergyPlatform/ontology/issues/328
pull request: https://github.com/OpenEnergyPlatform/ontology/pull/344

move to oeo-share
issue: https://github.com/OpenEnergyPlatform/ontology/issues/1329
pull request: https://github.com/OpenEnergyPlatform/ontology/pull/1615

rework module structure 
issue: https://github.com/OpenEnergyPlatform/ontology/issues/1592
pull request: https://github.com/OpenEnergyPlatform/ontology/pull/1652",
        rdfs:label "emission scenario"@en
    
    SubClassOf: 
        OEO_00000364
    
    
Class: OEO_00030010

    Annotations: 
        <http://purl.obolibrary.org/obo/IAO_0000115> "An energy scenario is a scenario that describes a possible future state of an energy system.",
        <http://purl.obolibrary.org/obo/IAO_0000233> "issue: https://github.com/OpenEnergyPlatform/ontology/issues/328
pull request: https://github.com/OpenEnergyPlatform/ontology/pull/344

make equivalent
issue: https://github.com/OpenEnergyPlatform/ontology/issues/1329
pull request: https://github.com/OpenEnergyPlatform/ontology/pull/1615

move axiom to shared-axioms
issue: https://github.com/OpenEnergyPlatform/ontology/issues/1703
pull request: https://github.com/OpenEnergyPlatform/ontology/pull/1706",
        rdfs:label "energy scenario"@en
    
    SubClassOf: 
        OEO_00000364
    
    
Class: OEO_00030015

    Annotations: 
        <http://purl.obolibrary.org/obo/IAO_0000115> "An energy system model is a model of an energy system.",
        <http://purl.obolibrary.org/obo/IAO_0000233> "issue: https://github.com/OpenEnergyPlatform/ontology/issues/337
pull request: https://github.com/OpenEnergyPlatform/ontology/pull/358
rework module structure 
issue: https://github.com/OpenEnergyPlatform/ontology/issues/1592
pull request: https://github.com/OpenEnergyPlatform/ontology/pull/1652",
        rdfs:label "energy system model"@en
    
    SubClassOf: 
        OEO_00000274
    
    
Class: OEO_00030029

    Annotations: 
        <http://purl.obolibrary.org/obo/IAO_0000115> "Exogenous data is a data item whose quantity value is determined outside of a model and is imposed on a model.",
        <http://purl.obolibrary.org/obo/IAO_0000118> "input data",
        <http://purl.obolibrary.org/obo/IAO_0000233> "issue: https://github.com/OpenEnergyPlatform/ontology/issues/482
pull request: https://github.com/OpenEnergyPlatform/ontology/pull/500

make equivalent class
pull request: https://github.com/OpenEnergyPlatform/ontology/pull/1113

add relation to quantity value:
pull request: https://github.com/OpenEnergyPlatform/ontology/pull/1216

rework module structure 
issue: https://github.com/OpenEnergyPlatform/ontology/issues/1592
pull request: https://github.com/OpenEnergyPlatform/ontology/pull/1652",
        rdfs:label "exogenous data"@en
    
    EquivalentTo: 
        <http://purl.obolibrary.org/obo/IAO_0000027>
         and (OEO_00020189 some OEO_00000275)
    
    SubClassOf: 
        <http://purl.obolibrary.org/obo/IAO_0000027>,
        <http://purl.obolibrary.org/obo/IAO_0000136> some OEO_00000350
    
    
Class: OEO_00030030

    Annotations: 
        <http://purl.obolibrary.org/obo/IAO_0000115> "Endogenous data is a data item whose quantity value is determined by a model.",
        <http://purl.obolibrary.org/obo/IAO_0000233> "issue: https://github.com/OpenEnergyPlatform/ontology/issues/482
pull request: https://github.com/OpenEnergyPlatform/ontology/pull/500

make equivalent class
pull request: https://github.com/OpenEnergyPlatform/ontology/pull/1113

add relation to quantity value:
pull request: https://github.com/OpenEnergyPlatform/ontology/pull/1216

rework module structure 
issue: https://github.com/OpenEnergyPlatform/ontology/issues/1592
pull request: https://github.com/OpenEnergyPlatform/ontology/pull/1652",
        rdfs:label "endogenous data"@en
    
    EquivalentTo: 
        <http://purl.obolibrary.org/obo/IAO_0000027>
         and (OEO_00020190 some OEO_00000275)
    
    SubClassOf: 
        <http://purl.obolibrary.org/obo/IAO_0000027>,
        <http://purl.obolibrary.org/obo/IAO_0000136> some OEO_00000350
    
    
Class: OEO_00030031

    Annotations: 
        <http://purl.obolibrary.org/obo/IAO_0000115> "A start time is a zero-dimensional temporal region that indicates the beginning of a one-dimensional temporal region.",
        <http://purl.obolibrary.org/obo/IAO_0000233> "issue: https://github.com/OpenEnergyPlatform/ontology/issues/267
pull request: https://github.com/OpenEnergyPlatform/ontology/pull/538

rework module structure 
issue: https://github.com/OpenEnergyPlatform/ontology/issues/1592
pull request: https://github.com/OpenEnergyPlatform/ontology/pull/1652",
        rdfs:label "start time"@en
    
    SubClassOf: 
        <http://purl.obolibrary.org/obo/BFO_0000148>
    
    
Class: OEO_00030032

    Annotations: 
        <http://purl.obolibrary.org/obo/IAO_0000115> "An ending time is a zero-dimensional temporal region that indicates the end of a one-dimensional temporal region.",
        <http://purl.obolibrary.org/obo/IAO_0000233> "issue: https://github.com/OpenEnergyPlatform/ontology/issues/267
pull request: https://github.com/OpenEnergyPlatform/ontology/pull/538

rework module structure 
issue: https://github.com/OpenEnergyPlatform/ontology/issues/1592
pull request: https://github.com/OpenEnergyPlatform/ontology/pull/1652",
        rdfs:label "ending time"@en
    
    SubClassOf: 
        <http://purl.obolibrary.org/obo/BFO_0000148>
    
    
Class: OEO_00030033

    Annotations: 
        <http://purl.obolibrary.org/obo/IAO_0000115> "A time step is a one-dimensional temporal region that has a start time and an ending time and thus a finite duration.",
        <http://purl.obolibrary.org/obo/IAO_0000233> "issue: https://github.com/OpenEnergyPlatform/ontology/issues/267
pull request: https://github.com/OpenEnergyPlatform/ontology/pull/538
pull request: https://github.com/OpenEnergyPlatform/ontology/pull/570

move to oeo-shared:
issue: https://github.com/OpenEnergyPlatform/ontology/issues/1384
pull request: https://github.com/OpenEnergyPlatform/ontology/pull/1390

rework module structure 
issue: https://github.com/OpenEnergyPlatform/ontology/issues/1592
pull request: https://github.com/OpenEnergyPlatform/ontology/pull/1652",
        rdfs:label "time step"@en
    
    SubClassOf: 
        <http://purl.obolibrary.org/obo/BFO_0000038>,
        ((<http://purl.obolibrary.org/obo/BFO_0000051> some OEO_00030031)
         and (<http://purl.obolibrary.org/obo/BFO_0000051> some OEO_00030032)) or ((<http://purl.obolibrary.org/obo/BFO_0000051> some OEO_00030035)
         and (<http://purl.obolibrary.org/obo/BFO_0000051> some OEO_00140043)
         and (<http://purl.obolibrary.org/obo/BFO_0000051> some OEO_00140044))
    
    
Class: OEO_00030034

    Annotations: 
        <http://purl.obolibrary.org/obo/IAO_0000115> "A time series is a data set that references to a set of time steps or zero-dimensional temporal regions.",
        <http://purl.obolibrary.org/obo/IAO_0000233> "issue: https://github.com/OpenEnergyPlatform/ontology/issues/267
pull request: https://github.com/OpenEnergyPlatform/ontology/pull/538

move to oeo-shared:
issue: https://github.com/OpenEnergyPlatform/ontology/issues/1384
pull request: https://github.com/OpenEnergyPlatform/ontology/pull/1390

rework module structure 
issue: https://github.com/OpenEnergyPlatform/ontology/issues/1592
pull request: https://github.com/OpenEnergyPlatform/ontology/pull/1652",
        
            Annotations: <http://purl.obolibrary.org/obo/IAO_0000233> "issue: https://github.com/OpenEnergyPlatform/ontology/issues/636
pull request: https://github.com/OpenEnergyPlatform/ontology/pull/810"
        <http://purl.obolibrary.org/obo/IAO_0006011> "http://purl.obolibrary.org/obo/IAO_0000584",
        rdfs:label "time series"@en
    
    SubClassOf: 
        <http://purl.obolibrary.org/obo/IAO_0000100>,
        <http://purl.obolibrary.org/obo/BFO_0000051> some OEO_00030031,
        <http://purl.obolibrary.org/obo/BFO_0000051> some OEO_00030032,
        <http://purl.obolibrary.org/obo/BFO_0000051> some OEO_00030035,
        <http://purl.obolibrary.org/obo/IAO_0000136> some 
            (OEO_00030033 or <http://purl.obolibrary.org/obo/BFO_0000148>)
    
    
Class: OEO_00030035

    
Class: OEO_00140024

    Annotations: 
        <http://purl.obolibrary.org/obo/IAO_0000115> "Validation is the process of checking if something works correctly.",
        <http://purl.obolibrary.org/obo/IAO_0000233> "issue: https://github.com/OpenEnergyPlatform/ontology/issues/487
pull request: https://github.com/OpenEnergyPlatform/ontology/pull/565",
        rdfs:label "validation"@en
    
    SubClassOf: 
        <http://purl.obolibrary.org/obo/BFO_0000015>
    
    
Class: OEO_00140025

    Annotations: 
        <http://purl.obolibrary.org/obo/IAO_0000115> "Cross-checking against other models is a validation where a model gets cross-checked against other models of the domain.",
        <http://purl.obolibrary.org/obo/IAO_0000233> "issue: https://github.com/OpenEnergyPlatform/ontology/issues/487
pull request: https://github.com/OpenEnergyPlatform/ontology/pull/565",
        rdfs:label "cross-checking against other models"@en
    
    SubClassOf: 
        OEO_00140024
    
    
Class: OEO_00140026

    Annotations: 
        <http://purl.obolibrary.org/obo/IAO_0000115> "Checking against measurements is a validation where something gets checked by using relevant measurements.",
        <http://purl.obolibrary.org/obo/IAO_0000233> "issue: https://github.com/OpenEnergyPlatform/ontology/issues/487
pull request: https://github.com/OpenEnergyPlatform/ontology/pull/565",
        rdfs:label "checking against measurements"@en
    
    SubClassOf: 
        OEO_00140024
    
    
Class: OEO_00140027

    Annotations: 
        <http://purl.obolibrary.org/obo/IAO_0000115> "Checking against empirical data is a validation where something gets checked against empirical data.",
        <http://purl.obolibrary.org/obo/IAO_0000233> "issue: https://github.com/OpenEnergyPlatform/ontology/issues/487
pull request: https://github.com/OpenEnergyPlatform/ontology/pull/565",
        rdfs:label "checking against empirical data"@en
    
    SubClassOf: 
        OEO_00140024
    
    
Class: OEO_00140043

    Annotations: 
        <http://purl.obolibrary.org/obo/IAO_0000115> "A time stamp is a zero-dimensional temporal region that is used to describe a time step.",
        <http://purl.obolibrary.org/obo/IAO_0000233> "issue: https://github.com/OpenEnergyPlatform/ontology/issues/267
pull request: https://github.com/OpenEnergyPlatform/ontology/pull/570

move to oeo-shared:
issue: https://github.com/OpenEnergyPlatform/ontology/issues/1384
pull request: https://github.com/OpenEnergyPlatform/ontology/pull/1390

rework module structure 
issue: https://github.com/OpenEnergyPlatform/ontology/issues/1592
pull request: https://github.com/OpenEnergyPlatform/ontology/pull/1652",
        rdfs:label "time stamp"@en
    
    SubClassOf: 
        <http://purl.obolibrary.org/obo/BFO_0000148>
    
    
Class: OEO_00140044

    Annotations: 
        <http://purl.obolibrary.org/obo/IAO_0000115> "A time stamp alignment is a data descriptor that indicates the position of a time stamp in a time step.",
        <http://purl.obolibrary.org/obo/IAO_0000233> "issue: https://github.com/OpenEnergyPlatform/ontology/issues/267
pull request: https://github.com/OpenEnergyPlatform/ontology/pull/570

move to oeo-shared:
issue: https://github.com/OpenEnergyPlatform/ontology/issues/1384
pull request: https://github.com/OpenEnergyPlatform/ontology/pull/1390

rework module structure 
issue: https://github.com/OpenEnergyPlatform/ontology/issues/1592
pull request: https://github.com/OpenEnergyPlatform/ontology/pull/1652",
        rdfs:label "time stamp alignment"@en
    
    SubClassOf: 
        OEO_00000119
    
    
Class: OEO_00140068

    Annotations: 
        <http://purl.obolibrary.org/obo/IAO_0000112> "aggregation of a data set with spatial references",
        <http://purl.obolibrary.org/obo/IAO_0000112> "temporal aggregation of continuous measurements for a discrete time series",
        <http://purl.obolibrary.org/obo/IAO_0000115> "An aggregation type is a data descriptor that contains information on the aggregation method applied on a data set.",
        <http://purl.obolibrary.org/obo/IAO_0000233> "add axiom `'is about' some 'typical period'`:
issue: https://github.com/OpenEnergyPlatform/ontology/issues/880
pull request: https://github.com/OpenEnergyPlatform/ontology/pull/883

issue: https://github.com/OpenEnergyPlatform/ontology/issues/571
pull request: https://github.com/OpenEnergyPlatform/ontology/pull/610",
        rdfs:label "aggregation type"@en
    
    SubClassOf: 
        OEO_00000119,
        <http://purl.obolibrary.org/obo/IAO_0000136> some OEO_00020089
    
    
Class: OEO_00140098

    Annotations: 
        <http://purl.obolibrary.org/obo/IAO_0000115> "A quality control flag is a data descriptor that describes the measurement quality of a data set, e.g. a time series.",
        <http://purl.obolibrary.org/obo/IAO_0000233> "issue: https://github.com/OpenEnergyPlatform/ontology/issues/612
pull request: https://github.com/OpenEnergyPlatform/ontology/pull/724",
        rdfs:label "quality control flag"@en
    
    SubClassOf: 
        OEO_00000119,
        <http://purl.obolibrary.org/obo/IAO_0000136> some <http://purl.obolibrary.org/obo/IAO_0000100>
    
    
Class: OEO_00140099

    Annotations: 
        <http://purl.obolibrary.org/obo/IAO_0000115> "A goal description is an information content entity that contains statements about a desired future state of a system that a person or organisation envisions or plans, or to which it commits.",
        <http://purl.obolibrary.org/obo/IAO_0000233> "issue: https://github.com/OpenEnergyPlatform/ontology/issues/28
pull request: https://github.com/OpenEnergyPlatform/ontology/pull/729",
        rdfs:label "goal description"@en
    
    SubClassOf: 
        <http://purl.obolibrary.org/obo/IAO_0000030>
    
    
Class: OEO_00140138

    Annotations: 
        <http://purl.obolibrary.org/obo/IAO_0000233> "A generation time series is a time series that describes the specific electricity generation of a particular power plant.",
        <http://purl.obolibrary.org/obo/IAO_0000233> "issue: https://github.com/OpenEnergyPlatform/ontology/issues/256
pull request: https://github.com/OpenEnergyPlatform/ontology/pull/793

Add 'is about' axiom:
pull request: https://github.com/OpenEnergyPlatform/ontology/pull/1410

move axiom to shared-axioms
issue: https://github.com/OpenEnergyPlatform/ontology/issues/1703
pull request: https://github.com/OpenEnergyPlatform/ontology/pull/1706",
        rdfs:label "generation time series"@en
    
    SubClassOf: 
        OEO_00030034
    
    
Class: OEO_00140139

    Annotations: 
        <http://purl.obolibrary.org/obo/IAO_0000115> "A yield profile is a generation time series of a particular renewable power plant.",
        <http://purl.obolibrary.org/obo/IAO_0000233> "issue: https://github.com/OpenEnergyPlatform/ontology/issues/256
pull request: https://github.com/OpenEnergyPlatform/ontology/pull/793

Add 'is about' axiom:
issue:https://github.com/OpenEnergyPlatform/ontology/issues/1423
pull request: https://github.com/OpenEnergyPlatform/ontology/pull/1437

move axiom to shared-axioms
issue: https://github.com/OpenEnergyPlatform/ontology/issues/1703
pull request: https://github.com/OpenEnergyPlatform/ontology/pull/1706",
        rdfs:label "yield profile"@en
    
    SubClassOf: 
        OEO_00140138
    
    
Class: OEO_00140161

    Annotations: 
        <http://purl.obolibrary.org/obo/IAO_0000115> "Cooperative programming is the process of two or more people working on program code together at the same time (according to a specified routine).",
        <http://purl.obolibrary.org/obo/IAO_0000118> "collaborative programming",
        <http://purl.obolibrary.org/obo/IAO_0000233> "issue: https://github.com/OpenEnergyPlatform/ontology/issues/254
pull request: https://github.com/OpenEnergyPlatform/ontology/pull/808

add 'has participant axiom':
issue: https://github.com/OpenEnergyPlatform/ontology/issues/1327
pull request: https://github.com/OpenEnergyPlatform/ontology/pull/1395",
        rdfs:label "cooperative programming"@en
    
    SubClassOf: 
        <http://purl.obolibrary.org/obo/BFO_0000015>,
        <http://purl.obolibrary.org/obo/RO_0000057> min 2 OEO_00000323
    
    
Class: OEO_00140167

    Annotations: 
        <http://purl.obolibrary.org/obo/IAO_0000115> "An uncertainty approach is a model descriptor that specifies how a model deals with uncertainty.",
        <http://purl.obolibrary.org/obo/IAO_0000233> "issue: https://github.com/OpenEnergyPlatform/ontology/issues/183
pull request: https://github.com/OpenEnergyPlatform/ontology/pull/824",
        rdfs:label "uncertainty approach"@en
    
    SubClassOf: 
        OEO_00020016
    
    
Class: OEO_00240004

    Annotations: 
        <http://purl.obolibrary.org/obo/IAO_0000115> "An objective variable is a variable that should be maximised or minimised to solve a problem."@en,
        <http://purl.obolibrary.org/obo/IAO_0000233> "issue: https://github.com/OpenEnergyPlatform/ontology/issues/848
pull request: https://github.com/OpenEnergyPlatform/ontology/pull/878",
        rdfs:label "objective variable"@en
    
    SubClassOf: 
        OEO_00000435
    
    DisjointWith: 
        OEO_00000078
    
    
Class: OEO_00280000

    Annotations: 
        <http://purl.obolibrary.org/obo/IAO_0000115> "A file format is a data format that describes how data is structured in a file.",
        <http://purl.obolibrary.org/obo/IAO_0000233> "issue: https://github.com/OpenEnergyPlatform/ontology/issues/1145
pull request: https://github.com/OpenEnergyPlatform/ontology/pull/1326",
        rdfs:label "data file format"@en
    
    SubClassOf: 
        OEO_00000120
    
    
Class: OEO_00280001

    Annotations: 
        <http://purl.obolibrary.org/obo/IAO_0000115> "A text file format is a file format that is structured as a sequence of lines of electronic text.",
        <http://purl.obolibrary.org/obo/IAO_0000233> "issue: https://github.com/OpenEnergyPlatform/ontology/issues/1145
pull request: https://github.com/OpenEnergyPlatform/ontology/pull/1326

Add DisjointWith axiom:
pull request: https://github.com/OpenEnergyPlatform/ontology/pull/1410",
        rdfs:label "text file format"@en
    
    SubClassOf: 
        OEO_00280000
    
    DisjointWith: 
        OEO_00280004
    
    
Class: OEO_00280002

    Annotations: 
        <http://purl.obolibrary.org/obo/IAO_0000115> "A delimiter separated file format is a text file format that uses delimiter-separated values (also DSV) to store two-dimensional arrays of data by separating the values in each row with specific delimiter characters.",
        <http://purl.obolibrary.org/obo/IAO_0000118> "DSV",
        <http://purl.obolibrary.org/obo/IAO_0000233> "issue: https://github.com/OpenEnergyPlatform/ontology/issues/1145
pull request: https://github.com/OpenEnergyPlatform/ontology/pull/1326",
        rdfs:label "delimiter separated file format"@en
    
    SubClassOf: 
        OEO_00280001
    
    
Class: OEO_00280003

    Annotations: 
        <http://purl.obolibrary.org/obo/IAO_0000115> "A comma separated file format is a delimiter separated file format that uses comma (,) as delimiter.",
        <http://purl.obolibrary.org/obo/IAO_0000118> "CSV",
        <http://purl.obolibrary.org/obo/IAO_0000233> "issue: https://github.com/OpenEnergyPlatform/ontology/issues/1145
pull request: https://github.com/OpenEnergyPlatform/ontology/pull/1326",
        rdfs:label "comma separated file format"@en
    
    SubClassOf: 
        OEO_00280002
    
    
Class: OEO_00280004

    Annotations: 
        <http://purl.obolibrary.org/obo/IAO_0000115> "A binary file format is a file format that is not a text format.",
        <http://purl.obolibrary.org/obo/IAO_0000233> "issue: https://github.com/OpenEnergyPlatform/ontology/issues/1145
pull request: https://github.com/OpenEnergyPlatform/ontology/pull/1326

Add DisjointWith axiom:
pull request: https://github.com/OpenEnergyPlatform/ontology/pull/1410",
        rdfs:label "binary file format"@en
    
    SubClassOf: 
        OEO_00280000
    
    DisjointWith: 
        OEO_00280001
    
    
Class: OEO_00280005

    Annotations: 
        <http://purl.obolibrary.org/obo/IAO_0000115> "A source code file format is a text file format that is source code in a programming language.",
        <http://purl.obolibrary.org/obo/IAO_0000233> "Issue: https://github.com/OpenEnergyPlatform/ontology/issues/1145
pull request: https://github.com/OpenEnergyPlatform/ontology/pull/1326

Make subclass of 'text file format`:
pull request: https://github.com/OpenEnergyPlatform/ontology/pull/1410",
        rdfs:label "source code file format"@en
    
    SubClassOf: 
        OEO_00280001
    
    
Class: OEO_00340006

    Annotations: 
        <http://purl.obolibrary.org/obo/IAO_0000115> "Regionalisation is a methodology to calculate spatially distributed energy producers and consumers with the aim to highlight regional differences in energy supply and potentials, particularly related to renewable energies.",
        <http://purl.obolibrary.org/obo/IAO_0000233> "issue: https://github.com/OpenEnergyPlatform/ontology/issues/1554
pull request: https://github.com/OpenEnergyPlatform/ontology/pull/1639",
        rdfs:label "regionalisation"@en
    
    SubClassOf: 
        OEO_00010250
    
    
Class: OEO_00360002

    Annotations: 
        <http://purl.obolibrary.org/obo/IAO_0000115> "A model intercomparison study is a scenario study that performs a comparison of several models using a reference scenario."@en,
        <http://purl.obolibrary.org/obo/IAO_0000233> "issue: https://github.com/OpenEnergyPlatform/ontology/issues/1640
pull request: https://github.com/OpenEnergyPlatform/ontology/pull/1711",
        rdfs:label "model intercomparison study"@en
    
    SubClassOf: 
        OEO_00010252
    
    
Class: OEO_00360003

    Annotations: 
        <http://purl.obolibrary.org/obo/IAO_0000115> "A scenario comparison study is a scenario study that performs a scenario projection comparison"@en,
        <http://purl.obolibrary.org/obo/IAO_0000233> "issue: https://github.com/OpenEnergyPlatform/ontology/issues/1640
pull request: https://github.com/OpenEnergyPlatform/ontology/pull/1711",
        rdfs:label "scenario projection comparison"@en
    
    SubClassOf: 
        OEO_00010252
    
    
Individual: OEO_00000049

    Annotations: 
        rdfs:label "active"@en
    
    Types: 
        OEO_00000281
    
    
Individual: OEO_00000081

    Annotations: 
        rdfs:label "c++"@en
    
    Types: 
        OEO_00000382
    
    
Individual: OEO_00000092

    Annotations: 
        rdfs:label "coin- or_cbc"@en
    
    Types: 
        OEO_00000392
    
    
Individual: OEO_00000114

    Annotations: 
        rdfs:label "cplex"@en
    
    Types: 
        OEO_00000392
    
    
Individual: OEO_00000121

    Annotations: 
        rdfs:label "data frame"@en
    
    Types: 
        OEO_00000120
    
    
Individual: OEO_00000130

    Annotations: 
        rdfs:label "dict"@en
    
    Types: 
        OEO_00000120
    
    
Individual: OEO_00000163

    Annotations: 
        <http://purl.obolibrary.org/obo/IAO_0000115> "False is a boolean value which is intended to represent the truth value false (denoted by 0, by -, the falsum , or falsch (F) in German).",
        <http://purl.obolibrary.org/obo/IAO_0000118> "falsch"@de,
        <http://purl.obolibrary.org/obo/IAO_0000233> "definition:
issue: https://github.com/OpenEnergyPlatform/ontology/issues/1148
pull request: https://github.com/OpenEnergyPlatform/ontology/pull/1255",
        rdfs:label "false"@en
    
    Types: 
        OEO_00010422
    
    DifferentFrom: 
        OEO_00000424
    
    
Individual: OEO_00000170

    Annotations: 
        rdfs:label "fortran"@en
    
    Types: 
        OEO_00000382
    
    
Individual: OEO_00000180

    Annotations: 
        rdfs:label "gams"@en
    
    Types: 
        OEO_00000382
    
    
Individual: OEO_00000187

    Annotations: 
        rdfs:label "gdx"@en
    
    Types: 
        OEO_00000120
    
    
Individual: OEO_00000195

    Annotations: 
        rdfs:label "glpk"@en
    
    Types: 
        OEO_00000392
    
    
Individual: OEO_00000196

    Annotations: 
        rdfs:label "gnu"@en
    
    Types: 
        OEO_00000382
    
    
Individual: OEO_00000203

    Annotations: 
        rdfs:label "gurobi"@en
    
    Types: 
        OEO_00000392
    
    
Individual: OEO_00000225

    Annotations: 
        rdfs:label "inactive"@en
    
    Types: 
        OEO_00000281
    
    
Individual: OEO_00000244

    Annotations: 
        rdfs:label "java"@en
    
    Types: 
        OEO_00000382
    
    
Individual: OEO_00000266

    Annotations: 
        rdfs:label "math prog"@en
    
    Types: 
        OEO_00000382
    
    
Individual: OEO_00000267

    Annotations: 
        rdfs:label "matlab"@en
    
    Types: 
        OEO_00000382
    
    
Individual: OEO_00000280

    Annotations: 
        rdfs:label "modelica"@en
    
    Types: 
        OEO_00000382
    
    
Individual: OEO_00000285

    Annotations: 
        rdfs:label "mosek"@en
    
    Types: 
        OEO_00000392
    
    
Individual: OEO_00000287

    Annotations: 
        rdfs:label "ms_ excel"@en
    
    Types: 
        OEO_00000382
    
    
Individual: OEO_00000288

    Annotations: 
        rdfs:label "vba"@en
    
    Types: 
        OEO_00000382
    
    
Individual: OEO_00000319

    Annotations: 
        rdfs:label "passive"@en
    
    Types: 
        OEO_00000281
    
    
Individual: OEO_00000325

    Annotations: 
        rdfs:label "php"@en
    
    Types: 
        OEO_00000382
    
    
Individual: OEO_00000349

    Annotations: 
        rdfs:label "python"@en
    
    Types: 
        OEO_00000382
    
    
Individual: OEO_00000351

    Annotations: 
        rdfs:label "r"@en
    
    Types: 
        OEO_00000382
    
    
Individual: OEO_00000362

    Annotations: 
        rdfs:label "ruby"@en
    
    Types: 
        OEO_00000382
    
    
Individual: OEO_00000424

    Annotations: 
        <http://purl.obolibrary.org/obo/IAO_0000115> "True is a boolean value which is intended to represent the truth value true (denoted by 1, by +, the verum , or wahr (W) in German).",
        <http://purl.obolibrary.org/obo/IAO_0000118> "wahr"@de,
        <http://purl.obolibrary.org/obo/IAO_0000233> "definition:
issue: https://github.com/OpenEnergyPlatform/ontology/issues/1148
pull request: https://github.com/OpenEnergyPlatform/ontology/pull/1255",
        rdfs:label "true"@en
    
    Types: 
        OEO_00010422
    
    DifferentFrom: 
        OEO_00000163
    
    
Individual: OEO_00000450

    Annotations: 
        rdfs:label "xlsx"@en
    
    Types: 
        OEO_00000120
    
    
Individual: OEO_00000451

    Annotations: 
        rdfs:label "xml"@en
    
    Types: 
        OEO_00000120
    
    
Individual: OEO_00020027

    Annotations: 
        rdfs:label "spreadsheet"@en
    
    Types: 
        OEO_00020018
    
    
Individual: OEO_00020028

    Annotations: 
        rdfs:label "monte carlo"@en
    
    Types: 
        OEO_00020018
    
    
Individual: OEO_00020029

    Annotations: 
        rdfs:label "econometric"@en
    
    Types: 
        OEO_00020018
    
    
Individual: OEO_00020161

    Annotations: 
        <http://purl.obolibrary.org/obo/IAO_0000115> "one value per year",
        <http://purl.obolibrary.org/obo/IAO_0000233> "rework module structure 
issue: https://github.com/OpenEnergyPlatform/ontology/issues/1592
pull request: https://github.com/OpenEnergyPlatform/ontology/pull/1652",
        rdfs:label "annual"@en
    
    Types: 
        OEO_00020122
    
    
Individual: OEO_00020162

    Annotations: 
        <http://purl.obolibrary.org/obo/IAO_0000115> "one value per week",
        <http://purl.obolibrary.org/obo/IAO_0000233> "rework module structure 
issue: https://github.com/OpenEnergyPlatform/ontology/issues/1592
pull request: https://github.com/OpenEnergyPlatform/ontology/pull/1652",
        rdfs:label "weekly"@en
    
    Types: 
        OEO_00020122
    
    
Individual: OEO_00020163

    Annotations: 
        <http://purl.obolibrary.org/obo/IAO_0000115> "one value per day",
        <http://purl.obolibrary.org/obo/IAO_0000233> "rework module structure 
issue: https://github.com/OpenEnergyPlatform/ontology/issues/1592
pull request: https://github.com/OpenEnergyPlatform/ontology/pull/1652",
        rdfs:label "daily"@en
    
    Types: 
        OEO_00020122
    
    
Individual: OEO_00020164

    Annotations: 
        <http://purl.obolibrary.org/obo/IAO_0000115> "one value per hour",
        <http://purl.obolibrary.org/obo/IAO_0000233> "rework module structure 
issue: https://github.com/OpenEnergyPlatform/ontology/issues/1592
pull request: https://github.com/OpenEnergyPlatform/ontology/pull/1652",
        rdfs:label "hourly"@en
    
    Types: 
        OEO_00020122
    
    
Individual: OEO_00020165

    Annotations: 
        <http://purl.obolibrary.org/obo/IAO_0000115> "one value per month",
        <http://purl.obolibrary.org/obo/IAO_0000233> "rework module structure 
issue: https://github.com/OpenEnergyPlatform/ontology/issues/1592
pull request: https://github.com/OpenEnergyPlatform/ontology/pull/1652",
        rdfs:label "monthly"@en
    
    Types: 
        OEO_00020122
    
    
Individual: OEO_00140045

    Annotations: 
        <http://purl.obolibrary.org/obo/IAO_0000115> "A start alignment is a time stamp alignment indicating that the time stamp marks the start of the time step.",
        <http://purl.obolibrary.org/obo/IAO_0000118> "left alignment",
        <http://purl.obolibrary.org/obo/IAO_0000233> "issue: https://github.com/OpenEnergyPlatform/ontology/issues/267
pull request: https://github.com/OpenEnergyPlatform/ontology/pull/570",
        rdfs:label "start alignment"@en
    
    Types: 
        OEO_00140044
    
    
Individual: OEO_00140046

    Annotations: 
        <http://purl.obolibrary.org/obo/IAO_0000115> "A middle alignment is a time stamp alignment indicating that the time stamp marks the middle of the time step.",
        <http://purl.obolibrary.org/obo/IAO_0000118> "center alignment",
        <http://purl.obolibrary.org/obo/IAO_0000118> "centre alignment",
        <http://purl.obolibrary.org/obo/IAO_0000233> "issue: https://github.com/OpenEnergyPlatform/ontology/issues/267
pull request: https://github.com/OpenEnergyPlatform/ontology/pull/570",
        rdfs:label "middle alignment"@en
    
    Types: 
        OEO_00140044
    
    
Individual: OEO_00140047

    Annotations: 
        <http://purl.obolibrary.org/obo/IAO_0000115> "An end alignment is a time stamp alignment indicating that the time stamp marks the end of the time step.",
        <http://purl.obolibrary.org/obo/IAO_0000118> "right alignment",
        <http://purl.obolibrary.org/obo/IAO_0000233> "issue: https://github.com/OpenEnergyPlatform/ontology/issues/267
pull request: https://github.com/OpenEnergyPlatform/ontology/pull/570",
        rdfs:label "end alignment"@en
    
    Types: 
        OEO_00140044
    
    
Individual: OEO_00140069

    Annotations: 
        <http://purl.obolibrary.org/obo/IAO_0000115> "value measured at or modelled for exactly one 0-dim temporal region, referenced by a time stamp, e.g. to represent a time step in a time series",
        <http://purl.obolibrary.org/obo/IAO_0000233> "issue: https://github.com/OpenEnergyPlatform/ontology/issues/571
pull request: https://github.com/OpenEnergyPlatform/ontology/pull/610",
        rdfs:label "instantaneous"@en
    
    Types: 
        OEO_00140068
    
    
Individual: OEO_00140070

    Annotations: 
        <http://purl.obolibrary.org/obo/IAO_0000115> "sum or integral of values, e.g. within a time step or a spatial region",
        <http://purl.obolibrary.org/obo/IAO_0000233> "issue: https://github.com/OpenEnergyPlatform/ontology/issues/571
pull request: https://github.com/OpenEnergyPlatform/ontology/pull/610",
        rdfs:label "integral"@en
    
    Types: 
        OEO_00140068
    
    
Individual: OEO_00140071

    Annotations: 
        <http://purl.obolibrary.org/obo/IAO_0000115> "average value calculated by arithmetic mean over a set of data values, e.g. within a time step or spatial region",
        <http://purl.obolibrary.org/obo/IAO_0000233> "issue: https://github.com/OpenEnergyPlatform/ontology/issues/571
pull request: https://github.com/OpenEnergyPlatform/ontology/pull/610",
        rdfs:label "arithmetic mean"@en
    
    Types: 
        OEO_00140068
    
    
Individual: OEO_00140072

    Annotations: 
        <http://purl.obolibrary.org/obo/IAO_0000115> "minimum value within a set of data values, e.g. in a time step or spatial region",
        <http://purl.obolibrary.org/obo/IAO_0000233> "issue: https://github.com/OpenEnergyPlatform/ontology/issues/571
pull request: https://github.com/OpenEnergyPlatform/ontology/pull/610",
        rdfs:label "minimum"@en
    
    Types: 
        OEO_00140068
    
    
Individual: OEO_00140073

    Annotations: 
        <http://purl.obolibrary.org/obo/IAO_0000115> "maximum value within a set of data values, e.g. in a time step or spatial region",
        <http://purl.obolibrary.org/obo/IAO_0000233> "issue: https://github.com/OpenEnergyPlatform/ontology/issues/571
pull request: https://github.com/OpenEnergyPlatform/ontology/pull/610",
        rdfs:label "maximum"@en
    
    Types: 
        OEO_00140068
    
    
Individual: OEO_00140168

    Annotations: 
        <http://purl.obolibrary.org/obo/IAO_0000233> "issue: https://github.com/OpenEnergyPlatform/ontology/issues/183
pull request: https://github.com/OpenEnergyPlatform/ontology/pull/824",
        rdfs:label "stochastic"@en
    
    Types: 
        OEO_00140167
    
    
Individual: OEO_00140169

    Annotations: 
        <http://purl.obolibrary.org/obo/IAO_0000233> "issue: https://github.com/OpenEnergyPlatform/ontology/issues/183
pull request: https://github.com/OpenEnergyPlatform/ontology/pull/824",
        rdfs:label "deterministic"@en
    
    Types: 
        OEO_00140167
    
    
