Prefix: : <http://openenergy-platform.org/ontology/oeo/>
Prefix: dc: <http://purl.org/dc/elements/1.1/>
Prefix: owl: <http://www.w3.org/2002/07/owl#>
Prefix: rdf: <http://www.w3.org/1999/02/22-rdf-syntax-ns#>
Prefix: rdfs: <http://www.w3.org/2000/01/rdf-schema#>
Prefix: xml: <http://www.w3.org/XML/1998/namespace>
Prefix: xsd: <http://www.w3.org/2001/XMLSchema#>



Ontology: <http://openenergy-platform.org/ontology/oeo/oeo-shared-axioms>
<http://openenergy-platform.org/ontology/oeo/dev/oeo-shared-axioms.omn>
Import: <http://openenergy-platform.org/ontology/oeo/dev/oeo-model.omn>
Import: <http://openenergy-platform.org/ontology/oeo/dev/oeo-physical.omn>
Import: <http://openenergy-platform.org/ontology/oeo/dev/oeo-social.omn>

Annotations: 
    dc:description "The Open Energy Ontology is an ontology for all aspects of the energy modelling domain. The \"oeo-shared-axioms\" module covers axioms that connect classes from more than one thematic module.",
    dc:license "http://creativecommons.org/publicdomain/zero/1.0/",
    <http://purl.org/dc/terms/title> "Open Energy Ontology (Shared axioms module)"

AnnotationProperty: <http://purl.obolibrary.org/obo/IAO_0000112>

    
AnnotationProperty: <http://purl.obolibrary.org/obo/IAO_0000115>

    
AnnotationProperty: <http://purl.obolibrary.org/obo/IAO_0000116>

    
AnnotationProperty: <http://purl.obolibrary.org/obo/IAO_0000118>

    Annotations: 
        rdfs:comment "In the OEO, we don't follow the definition strictly. We use alternative term for synonyms and ambiguous terms as well. See https://github.com/OpenEnergyPlatform/ontology/wiki/Handling-ambiguous-terms"
    
    
AnnotationProperty: <http://purl.obolibrary.org/obo/IAO_0000119>

    
AnnotationProperty: <http://purl.obolibrary.org/obo/IAO_0000233>

    
AnnotationProperty: <http://purl.obolibrary.org/obo/IAO_0006011>

    
AnnotationProperty: <http://purl.org/dc/terms/license>

    
AnnotationProperty: <http://purl.org/dc/terms/title>

    
AnnotationProperty: <http://www.geneontology.org/formats/oboInOwl#hasExactSynonym>

    
AnnotationProperty: OEO_00010037

    
AnnotationProperty: OEO_00040001

    
AnnotationProperty: OEO_00110012

    Annotations: 
        <http://purl.obolibrary.org/obo/IAO_0000115> "A mathematical expression is an annotation property that describes the class with a mathematical formula in LaTeX syntax."@en,
        <http://purl.obolibrary.org/obo/IAO_0000233> "issue: https://github.com/OpenEnergyPlatform/ontology/issues/987
pull request: https://github.com/OpenEnergyPlatform/ontology/pull/990"@en,
        rdfs:label "mathematical expression"@en
    
    
AnnotationProperty: dc:description

    
AnnotationProperty: dc:identifier

    
AnnotationProperty: dc:license

    
AnnotationProperty: rdfs:comment

    
AnnotationProperty: rdfs:isDefinedBy

    
AnnotationProperty: rdfs:label

    
AnnotationProperty: rdfs:seeAlso

    
Datatype: rdf:PlainLiteral

    
Datatype: xsd:integer

    
Datatype: xsd:string

    
ObjectProperty: <http://openenergy-platform.org/ontology/oeo/oeo-physical/OEO_00010238>

    Annotations: 
        <http://purl.obolibrary.org/obo/IAO_0000115> "A relation between an artificial object or a process and an energy, where the energy is used in the artificial object or process.",
        <http://purl.obolibrary.org/obo/IAO_0000233> "issue: https://github.com/OpenEnergyPlatform/ontology/issues/994
pull request: https://github.com/OpenEnergyPlatform/ontology/pull/1006

move to oeo-shared:
issue: https://github.com/OpenEnergyPlatform/ontology/issues/1384
pull request: https://github.com/OpenEnergyPlatform/ontology/pull/1390",
        rdfs:label "has energy participant"@en
    
    Domain: 
        OEO_00000061 or <http://purl.obolibrary.org/obo/BFO_0000015>
    
    Range: 
        OEO_00000150
    
    InverseOf: 
        OEO_00020182
    
    
ObjectProperty: <http://purl.obolibrary.org/obo/BFO_0000050>

    Annotations: 
        <http://purl.obolibrary.org/obo/IAO_0000233> "issue https://github.com/OpenEnergyPlatform/ontology/issues/596
Pull request https://github.com/OpenEnergyPlatform/ontology/pull/599
Pull request https://github.com/OpenEnergyPlatform/ontology/pull/603"
    
    Characteristics: 
        Transitive
    
    
ObjectProperty: <http://purl.obolibrary.org/obo/BFO_0000051>

    Annotations: 
        <http://purl.obolibrary.org/obo/IAO_0000233> "issue https://github.com/OpenEnergyPlatform/ontology/issues/596
Pull request https://github.com/OpenEnergyPlatform/ontology/pull/599
Pull request https://github.com/OpenEnergyPlatform/ontology/pull/603

fix duplicate implementation of `Inverse Of`
issue https://github.com/OpenEnergyPlatform/ontology/issues/979
pull request https://github.com/OpenEnergyPlatform/ontology/pull/1086"
    
    Characteristics: 
        Transitive
    
    
ObjectProperty: <http://purl.obolibrary.org/obo/BFO_0000054>

    
ObjectProperty: <http://purl.obolibrary.org/obo/IAO_0000136>

    InverseOf: 
        OEO_00010231
    
    
ObjectProperty: <http://purl.obolibrary.org/obo/RO_0000053>

    Annotations: 
        <http://purl.obolibrary.org/obo/IAO_0000118> "has characteristic"
    
    Domain: 
        
            Annotations: <http://purl.obolibrary.org/obo/IAO_0000233> "issue: https://github.com/OpenEnergyPlatform/ontology/issues/973
pull request: https://github.com/OpenEnergyPlatform/ontology/pull/985"
        OEO_00000150 or <http://purl.obolibrary.org/obo/BFO_0000004>
    
    Range: 
        <http://purl.obolibrary.org/obo/BFO_0000020>
    
    InverseOf: 
        OEO_00010121
    
    
ObjectProperty: <http://purl.obolibrary.org/obo/RO_0000056>

    Domain: 
        <http://purl.obolibrary.org/obo/BFO_0000002>
    
    Range: 
        <http://purl.obolibrary.org/obo/BFO_0000003>
    
    
ObjectProperty: <http://purl.obolibrary.org/obo/RO_0000057>

    Domain: 
        <http://purl.obolibrary.org/obo/BFO_0000003>
    
    
ObjectProperty: <http://purl.obolibrary.org/obo/RO_0000085>

    Domain: 
        <http://purl.obolibrary.org/obo/BFO_0000004>
    
    Range: 
        <http://purl.obolibrary.org/obo/BFO_0000034>
    
    
ObjectProperty: <http://purl.obolibrary.org/obo/RO_0000086>

    Domain: 
        <http://purl.obolibrary.org/obo/BFO_0000002>
    
    
ObjectProperty: <http://purl.obolibrary.org/obo/RO_0000087>

    Annotations: 
        <http://purl.obolibrary.org/obo/IAO_0000116> "In contrast to the original RO class, the domain was extended to independent continuant or energy. This is due to the special role that energy plays for the OEO and the difficulty of classifying it properly.",
        <http://purl.obolibrary.org/obo/IAO_0000233> "extend domain / definition
issue: https://github.com/OpenEnergyPlatform/ontology/issues/1030
pull request: https://github.com/OpenEnergyPlatform/ontology/pull/1101"
    
    Domain: 
        OEO_00000150 or <http://purl.obolibrary.org/obo/BFO_0000004>
    
    Range: 
        <http://purl.obolibrary.org/obo/BFO_0000023>
    
    
ObjectProperty: <http://purl.obolibrary.org/obo/RO_0000091>

    Domain: 
        <http://purl.obolibrary.org/obo/BFO_0000004>
    
    Range: 
        <http://purl.obolibrary.org/obo/BFO_0000016>
    
    
ObjectProperty: <http://purl.obolibrary.org/obo/RO_0001015>

    
ObjectProperty: <http://purl.obolibrary.org/obo/RO_0001025>

    
ObjectProperty: <http://purl.obolibrary.org/obo/RO_0002222>

    Domain: 
        <http://purl.obolibrary.org/obo/BFO_0000003>
    
    Range: 
        <http://purl.obolibrary.org/obo/BFO_0000003>
    
    
ObjectProperty: <http://purl.obolibrary.org/obo/RO_0002223>

    
ObjectProperty: <http://purl.obolibrary.org/obo/RO_0002224>

    
ObjectProperty: <http://purl.obolibrary.org/obo/RO_0002229>

    
ObjectProperty: <http://purl.obolibrary.org/obo/RO_0002230>

    
ObjectProperty: <http://purl.obolibrary.org/obo/RO_0002233>

    Domain: 
        <http://purl.obolibrary.org/obo/BFO_0000015>
    
    
ObjectProperty: <http://purl.obolibrary.org/obo/RO_0002234>

    
ObjectProperty: <http://purl.obolibrary.org/obo/RO_0002328>

    
ObjectProperty: <http://purl.obolibrary.org/obo/RO_0002352>

    
ObjectProperty: <http://purl.obolibrary.org/obo/RO_0002353>

    
ObjectProperty: <http://purl.obolibrary.org/obo/RO_0002410>

    Domain: 
        
            Annotations: <http://purl.obolibrary.org/obo/IAO_0000233> "add domain and range
issue: https://github.com/OpenEnergyPlatform/ontology/issues/1079
pull-request: https://github.com/OpenEnergyPlatform/ontology/pull/1136"
        <http://purl.obolibrary.org/obo/BFO_0000015> or <http://purl.obolibrary.org/obo/BFO_0000040>
    
    Range: 
        
            Annotations: <http://purl.obolibrary.org/obo/IAO_0000233> "add domain and range
issue: https://github.com/OpenEnergyPlatform/ontology/issues/1079
pull-request: https://github.com/OpenEnergyPlatform/ontology/pull/1136"
        <http://purl.obolibrary.org/obo/BFO_0000015> or <http://purl.obolibrary.org/obo/BFO_0000040>
    
    
ObjectProperty: <http://purl.obolibrary.org/obo/RO_0002418>

    
ObjectProperty: <http://purl.obolibrary.org/obo/RO_0002427>

    
ObjectProperty: <http://purl.obolibrary.org/obo/RO_0002501>

    Domain: 
        
            Annotations: <http://purl.obolibrary.org/obo/IAO_0000233> "add domain and range
issue: https://github.com/OpenEnergyPlatform/ontology/issues/1079
pull-request: https://github.com/OpenEnergyPlatform/ontology/pull/1136"
        <http://purl.obolibrary.org/obo/BFO_0000015>
    
    Range: 
        
            Annotations: <http://purl.obolibrary.org/obo/IAO_0000233> "add domain and range
issue: https://github.com/OpenEnergyPlatform/ontology/issues/1079
pull-request: https://github.com/OpenEnergyPlatform/ontology/pull/1136"
        <http://purl.obolibrary.org/obo/BFO_0000015>
    
    
ObjectProperty: <http://purl.obolibrary.org/obo/RO_0003000>

    Annotations: 
        
            Annotations: <http://purl.obolibrary.org/obo/IAO_0000233> "issue: https://github.com/OpenEnergyPlatform/ontology/issues/994
pull request: https://github.com/OpenEnergyPlatform/ontology/pull/1006"
        <http://purl.obolibrary.org/obo/IAO_0000116> "As produces relates to an material entity, but energy is a quality in the OEO, produces cannot be used to describe the energy output of a process. Use 'has energy output' instead."
    
    
ObjectProperty: <http://purl.obolibrary.org/obo/uo#is_unit_of>

    Annotations: 
        <http://purl.obolibrary.org/obo/IAO_0000115> "A relation to connect a unit to a quantifiable entity that it is the unit of.",
        rdfs:comment "This relation has been imported from UO.",
        rdfs:label "is unit of"
    
    Domain: 
        <http://purl.obolibrary.org/obo/UO_0000000>
    
    
ObjectProperty: OEO_00000500

    Annotations: 
        <http://purl.obolibrary.org/obo/IAO_0000233> "A relation between a process and a process attribute that existentially depends on it.",
        <http://purl.obolibrary.org/obo/IAO_0000233> "issue: https://github.com/OpenEnergyPlatform/ontology/issues/66
pull requests: https://github.com/OpenEnergyPlatform/ontology/pull/472

issue: https://github.com/OpenEnergyPlatform/ontology/issues/205
pull request: https://github.com/OpenEnergyPlatform/ontology/pull/386

add domain and range; move to oeo-shared
issue: https://github.com/OpenEnergyPlatform/ontology/issues/850
pull request: https://github.com/OpenEnergyPlatform/ontology/pull/871",
        rdfs:label "has process attribute"
    
    Domain: 
        <http://purl.obolibrary.org/obo/BFO_0000015>
    
    Range: 
        OEO_00030019
    
    InverseOf: 
        OEO_00000502
    
    
ObjectProperty: OEO_00000501

    Annotations: 
        <http://purl.obolibrary.org/obo/IAO_0000115> "A relation that holds between a continuant c1 and a continuant c2, where c1 is required by c2 as input to work.",
        rdfs:comment "issue: https://github.com/OpenEnergyPlatform/ontology/issues/66
pull requests: https://github.com/OpenEnergyPlatform/ontology/pull/472
add def and domain and range
issue: https://github.com/OpenEnergyPlatform/ontology/issues/1117
pull requests: https://github.com/OpenEnergyPlatform/ontology/pull/1508",
        rdfs:label "is used by"
    
    Domain: 
        <http://purl.obolibrary.org/obo/BFO_0000002>
    
    Range: 
        <http://purl.obolibrary.org/obo/BFO_0000002>
    
    InverseOf: 
        OEO_00000503
    
    
ObjectProperty: OEO_00000502

    Annotations: 
        <http://purl.obolibrary.org/obo/IAO_0000233> "A relation between a process attribute and the process it existentially depends on.",
        <http://purl.obolibrary.org/obo/IAO_0000233> "issue: https://github.com/OpenEnergyPlatform/ontology/issues/66
pull requests: https://github.com/OpenEnergyPlatform/ontology/pull/472

issue: https://github.com/OpenEnergyPlatform/ontology/issues/205
pull request: https://github.com/OpenEnergyPlatform/ontology/pull/386

add domains and ranges:
issue: https://github.com/OpenEnergyPlatform/ontology/issues/973
issue: https://github.com/OpenEnergyPlatform/ontology/pull/1085",
        rdfs:label "process attribute of"
    
    Domain: 
        OEO_00030019
    
    Range: 
        <http://purl.obolibrary.org/obo/BFO_0000015>
    
    InverseOf: 
        OEO_00000500
    
    
ObjectProperty: OEO_00000503

    Annotations: 
        <http://purl.obolibrary.org/obo/IAO_0000115> "A relation that holds between a continuant c1 and a continuant c2, where c1 requires c2 as input to work.",
        <http://purl.obolibrary.org/obo/IAO_0000233> "issue: https://github.com/OpenEnergyPlatform/ontology/issues/66
pull requests: https://github.com/OpenEnergyPlatform/ontology/pull/452 (delete unused subclass)
https://github.com/OpenEnergyPlatform/ontology/pull/472 (move to oeo-shared)
https://github.com/OpenEnergyPlatform/ontology/pull/478 (add definition)
https://github.com/OpenEnergyPlatform/ontology/pull/871 (add domain and range)
change def
issue: https://github.com/OpenEnergyPlatform/ontology/issues/1117
pull requests: https://github.com/OpenEnergyPlatform/ontology/pull/1508",
        rdfs:label "uses"
    
    Domain: 
        <http://purl.obolibrary.org/obo/BFO_0000002>
    
    Range: 
        <http://purl.obolibrary.org/obo/BFO_0000002>
    
    InverseOf: 
        OEO_00000501
    
    
ObjectProperty: OEO_00000504

    Annotations: 
        <http://purl.obolibrary.org/obo/IAO_0000115> "A relation between a continuant (A) and a continuant or occurent (B) in which (A) determines the semantic of (B)",
        <http://purl.obolibrary.org/obo/IAO_0000233> "issue: https://github.com/OpenEnergyPlatform/ontology/issues/460
pull request: https://github.com/OpenEnergyPlatform/ontology/pull/480/

domain:
issue: https://github.com/OpenEnergyPlatform/ontology/issues/850
pull request: https://github.com/OpenEnergyPlatform/ontology/pull/871

adapt domains and ranges:
issue: https://github.com/OpenEnergyPlatform/ontology/issues/973
issue: https://github.com/OpenEnergyPlatform/ontology/pull/1085

Move to oeo-shared:
issue: https://github.com/OpenEnergyPlatform/ontology/issues/1400
pull request: https://github.com/OpenEnergyPlatform/ontology/pull/1463",
        rdfs:label "is defined by"
    
    Range: 
        <http://purl.obolibrary.org/obo/BFO_0000002>
    
    
ObjectProperty: OEO_00000505

    Annotations: 
        <http://purl.obolibrary.org/obo/IAO_0000115> "A relation that holds between a study and the sector it covers."@en,
        <http://purl.obolibrary.org/obo/IAO_0000233> "update definition
issue: https://github.com/OpenEnergyPlatform/ontology/issues/846
pull request: https://github.com/OpenEnergyPlatform/ontology/pull/852",
        rdfs:label "covers sector"
    
    SubPropertyOf: 
        OEO_00000522
    
    Domain: 
        OEO_00020011
    
    Range: 
        OEO_00000367
    
    
ObjectProperty: OEO_00000506

    Annotations: 
        <http://purl.obolibrary.org/obo/IAO_0000115> "A relation that holds between an information content entity / model and its author."@en,
        <http://purl.obolibrary.org/obo/IAO_0000116> "The construct 'has author' some ('has role' some author) is necessary, because 'has author' has the range 'has role some author' (PR https://github.com/OpenEnergyPlatform/ontology/pull/871). That is an independent continuant, i.e. a person, that takes over writing a text and as such the role of an author.",
        <http://purl.obolibrary.org/obo/IAO_0000233> "pull request: https://github.com/OpenEnergyPlatform/ontology/pull/626 (extend def for information content entity)
pull request: https://github.com/OpenEnergyPlatform/ontology/pull/871 (domain and range; move to oeo-shared)",
        rdfs:label "has author"
    
    SubPropertyOf: 
        OEO_00140008
    
    Domain: 
        OEO_00000274 or <http://purl.obolibrary.org/obo/IAO_0000030>
    
    Range: 
        <http://purl.obolibrary.org/obo/RO_0000087> some OEO_00000064
    
    
ObjectProperty: OEO_00000507

    Annotations: 
        <http://purl.obolibrary.org/obo/IAO_0000115> "A relation that holds between an information content entity / model and the client that requested its creation."@en,
        <http://purl.obolibrary.org/obo/IAO_0000233> "pull request: https://github.com/OpenEnergyPlatform/ontology/pull/626 (extend def for information content entity)
pull request: https://github.com/OpenEnergyPlatform/ontology/pull/871 (domain and range; move to oeo-shared)",
        rdfs:label "has client"
    
    SubPropertyOf: 
        OEO_00140008
    
    Domain: 
        OEO_00000274 or <http://purl.obolibrary.org/obo/IAO_0000030>
    
    Range: 
        <http://purl.obolibrary.org/obo/RO_0000087> some OEO_00000087
    
    
ObjectProperty: OEO_00000508

    Annotations: 
        <http://purl.obolibrary.org/obo/IAO_0000115> "A relation that holds between an information content entity / model and the person to contact with issues about it."@en,
        <http://purl.obolibrary.org/obo/IAO_0000233> "pull request: https://github.com/OpenEnergyPlatform/ontology/pull/626 (extend def for information content entity)
pull request: https://github.com/OpenEnergyPlatform/ontology/pull/871 (domain and range; move to oeo-shared)",
        rdfs:label "has contact person"
    
    SubPropertyOf: 
        OEO_00140008
    
    Domain: 
        OEO_00000274 or <http://purl.obolibrary.org/obo/IAO_0000030>
    
    Range: 
        <http://purl.obolibrary.org/obo/RO_0000087> some OEO_00000107
    
    
ObjectProperty: OEO_00000509

    Annotations: 
        <http://purl.obolibrary.org/obo/IAO_0000115> "A relation that holds between an entity and its source of funding."@en,
        <http://purl.obolibrary.org/obo/IAO_0000233> "issue: https://github.com/OpenEnergyPlatform/ontology/issues/530
pull request: https://github.com/OpenEnergyPlatform/ontology/pull/556",
        rdfs:label "has funding source"
    
    SubPropertyOf: 
        owl:topObjectProperty
    
    Range: 
        
            Annotations: rdfs:comment "issue: https://github.com/OpenEnergyPlatform/ontology/issues/850
pull request: https://github.com/OpenEnergyPlatform/ontology/pull/871"
        <http://purl.obolibrary.org/obo/RO_0000087> some OEO_00090001
    
    
ObjectProperty: OEO_00000510

    Annotations: 
        <http://purl.obolibrary.org/obo/IAO_0000115> "A relation that holds between an information content entity or model and the organisation in which it was created."@en,
        <http://purl.obolibrary.org/obo/IAO_0000233> "pull request: https://github.com/OpenEnergyPlatform/ontology/pull/626 (extend def for information content entity)
pull request: https://github.com/OpenEnergyPlatform/ontology/pull/871 (domain and range; move to oeo-shared)

improve definition:
https://github.com/OpenEnergyPlatform/ontology/issues/1038
https://github.com/OpenEnergyPlatform/ontology/pull/1042

Relabel to `has organisation`
issue: https://github.com/OpenEnergyPlatform/ontology/issues/1161
pull request: https://github.com/OpenEnergyPlatform/ontology/pull/1226",
        rdfs:label "has organisation"
    
    SubPropertyOf: 
        OEO_00140008
    
    Domain: 
        OEO_00000274 or <http://purl.obolibrary.org/obo/IAO_0000030>
    
    Range: 
        
            Annotations: <http://purl.obolibrary.org/obo/IAO_0000233> "Replace `institution` as range by `organisation role`
issue: https://github.com/OpenEnergyPlatform/ontology/issues/1161
pull request: https://github.com/OpenEnergyPlatform/ontology/pull/1200"
        <http://purl.obolibrary.org/obo/RO_0000087> some OEO_00000315
    
    
ObjectProperty: OEO_00000514

    
ObjectProperty: OEO_00000515

    
ObjectProperty: OEO_00000516

    
ObjectProperty: OEO_00000522

    Annotations: 
        <http://purl.obolibrary.org/obo/IAO_0000115> "A relation that holds between a study and the thing it covers.",
        <http://purl.obolibrary.org/obo/IAO_0000233> "issue: https://github.com/OpenEnergyPlatform/ontology/issues/66
pull requests: https://github.com/OpenEnergyPlatform/ontology/pull/452 (delete unused subclasses)
pull requests: https://github.com/OpenEnergyPlatform/ontology/pull/584
pull requests: https://github.com/OpenEnergyPlatform/ontology/pull/626 (extend for study)
issue: https://github.com/OpenEnergyPlatform/ontology/issues/415
pull request: https://github.com/OpenEnergyPlatform/ontology/pull/821 (restrict to study)",
        rdfs:label "covers"
    
    
ObjectProperty: OEO_00000523

    Annotations: 
        <http://purl.obolibrary.org/obo/IAO_0000115> "A relation that holds between a study and the energy carrier it covers.",
        <http://purl.obolibrary.org/obo/IAO_0000233> "change range
issue: https://github.com/OpenEnergyPlatform/ontology/pull/721
pull request: https://github.com/OpenEnergyPlatform/ontology/pull/722

update definition
issue: https://github.com/OpenEnergyPlatform/ontology/issues/846
pull request: https://github.com/OpenEnergyPlatform/ontology/pull/852",
        rdfs:label "covers energy carrier"
    
    SubPropertyOf: 
        OEO_00000522
    
    Domain: 
        OEO_00020011
    
    Range: 
        OEO_00020039
    
    
ObjectProperty: OEO_00000524

    Annotations: 
        <http://purl.obolibrary.org/obo/IAO_0000115> "A relation between a greenhouse gas and the global warming potential it has.",
        <http://purl.obolibrary.org/obo/IAO_0000233> "issue: https://github.com/OpenEnergyPlatform/ontology/issues/66
pull request: https://github.com/OpenEnergyPlatform/ontology/pull/478
issue: https://github.com/OpenEnergyPlatform/ontology/issues/420
pull request: https://github.com/OpenEnergyPlatform/ontology/pull/651
issue: https://github.com/OpenEnergyPlatform/ontology/issues/420
pull request: https://github.com/OpenEnergyPlatform/ontology/pull/683

move to oeo-shared:
https://github.com/OpenEnergyPlatform/ontology/pull/1410",
        rdfs:label "has global warming potential"
    
    SubPropertyOf: 
        
            Annotations: <http://purl.obolibrary.org/obo/IAO_0000233> "issue: https://github.com/OpenEnergyPlatform/ontology/issues/858
pull request: https://github.com/OpenEnergyPlatform/ontology/pull/965"
        OEO_00140002
    
    Domain: 
        OEO_00000020
    
    Range: 
        OEO_00010078
    
    
ObjectProperty: OEO_00000529

    Annotations: 
        <http://purl.obolibrary.org/obo/IAO_0000115> "x has normal state of matter y if and only if a portion of x occurs in state y under normal pressure (1 bar) and normal temperature (0°C)",
        <http://purl.obolibrary.org/obo/IAO_0000233> "make subproperty of 'has state of matter'
issue: https://github.com/OpenEnergyPlatform/ontology/issues/989
pull request: https://github.com/OpenEnergyPlatform/ontology/pull/1001

move to oeo-shared:
issue: https://github.com/OpenEnergyPlatform/ontology/issues/1384
pull request: https://github.com/OpenEnergyPlatform/ontology/pull/1390",
        rdfs:label "has normal state of matter"
    
    SubPropertyOf: 
        OEO_00000531
    
    Domain: 
        OEO_00000331
    
    Range: 
        OEO_00000395
    
    
ObjectProperty: OEO_00000530

    Annotations: 
        <http://purl.obolibrary.org/obo/IAO_0000115> "x has the origin of y",
        <http://purl.obolibrary.org/obo/IAO_0000233> "move to oeo-shared:
issue: https://github.com/OpenEnergyPlatform/ontology/issues/1384
pull request: https://github.com/OpenEnergyPlatform/ontology/pull/1390",
        rdfs:label "has origin"
    
    SubPropertyOf: 
        <http://purl.obolibrary.org/obo/RO_0000086>
    
    Domain: 
        
            Annotations: <http://purl.obolibrary.org/obo/IAO_0000233> "add energy
issue: https://github.com/OpenEnergyPlatform/ontology/issues/728
pull request: https://github.com/OpenEnergyPlatform/ontology/pull/742"
        OEO_00000150 or OEO_00000331
    
    Range: 
        OEO_00000316
    
    
ObjectProperty: OEO_00000531

    Annotations: 
        <http://purl.obolibrary.org/obo/IAO_0000115> "A relation between a portion of matter (x) and a state of matter (y) that indicates the state y of matter x under certain given conditions.",
        <http://purl.obolibrary.org/obo/IAO_0000233> "issue: https://github.com/OpenEnergyPlatform/ontology/issues/989
pull request: https://github.com/OpenEnergyPlatform/ontology/pull/1001",
        rdfs:label "has state of matter"
    
    SubPropertyOf: 
        <http://purl.obolibrary.org/obo/RO_0000086>
    
    Domain: 
        OEO_00000331
    
    Range: 
        OEO_00000395
    
    
ObjectProperty: OEO_00000532

    Annotations: 
        <http://purl.obolibrary.org/obo/IAO_0000115> "p has physical input c iff: p has input c, and c is a material entity"@en,
        <http://purl.obolibrary.org/obo/IAO_0000233> "issue: https://github.com/OpenEnergyPlatform/ontology/issues/664
pull request: https://github.com/OpenEnergyPlatform/ontology/pull/702

restrict range to 'material entity':
https://github.com/OpenEnergyPlatform/ontology/issues/994
https://github.com/OpenEnergyPlatform/ontology/pull/1041

move to oeo-shared:
issue: https://github.com/OpenEnergyPlatform/ontology/issues/1384
pull request: https://github.com/OpenEnergyPlatform/ontology/pull/1390",
        rdfs:label "has physical input"
    
    SubPropertyOf: 
        <http://purl.obolibrary.org/obo/RO_0002233>
    
    Domain: 
        <http://purl.obolibrary.org/obo/BFO_0000015>
    
    Range: 
        <http://purl.obolibrary.org/obo/BFO_0000040>
    
    
ObjectProperty: OEO_00000533

    Annotations: 
        <http://purl.obolibrary.org/obo/IAO_0000115> "p has physical output c iff: p has output c, and c is a material entity"@en,
        <http://purl.obolibrary.org/obo/IAO_0000233> "issue: https://github.com/OpenEnergyPlatform/ontology/issues/618
pull request: https://github.com/OpenEnergyPlatform/ontology/pull/716

restrict range to 'material entity':
issue: https://github.com/OpenEnergyPlatform/ontology/issues/994
pull request: https://github.com/OpenEnergyPlatform/ontology/pull/1041

move to oeo-shared:
issue: https://github.com/OpenEnergyPlatform/ontology/issues/1384
pull request: https://github.com/OpenEnergyPlatform/ontology/pull/1390",
        rdfs:label "has physical output"
    
    SubPropertyOf: 
        <http://purl.obolibrary.org/obo/RO_0002234>
    
    Domain: 
        
            Annotations: <http://purl.obolibrary.org/obo/IAO_0000233> "issue: https://github.com/OpenEnergyPlatform/ontology/issues/394
pull request: https://github.com/OpenEnergyPlatform/ontology/pull/838"
        <http://purl.obolibrary.org/obo/BFO_0000015>
    
    Range: 
        
            Annotations: <http://purl.obolibrary.org/obo/IAO_0000233> "issue: https://github.com/OpenEnergyPlatform/ontology/issues/394
pull request: https://github.com/OpenEnergyPlatform/ontology/pull/838"
        <http://purl.obolibrary.org/obo/BFO_0000040>
    
    InverseOf: 
        OEO_00240025
    
    
ObjectProperty: OEO_00010119

    Annotations: 
        <http://purl.obolibrary.org/obo/IAO_0000115> "A relation between a policy instrument and a transformative measure where a policy instrument guides a transformative measure.",
        <http://purl.obolibrary.org/obo/IAO_0000233> "issue: https://github.com/OpenEnergyPlatform/ontology/issues/444
pull request: https://github.com/OpenEnergyPlatform/ontology/pull/853

Make subproperty of 'is about':
issue: https://github.com/OpenEnergyPlatform/ontology/issues/1507
pull request: https://github.com/OpenEnergyPlatform/ontology/pull/1563

move to oeo-shared
issue: https://github.com/OpenEnergyPlatform/ontology/issues/1329
pull request: https://github.com/OpenEnergyPlatform/ontology/pull/1614",
        rdfs:label "guides"@en
    
    SubPropertyOf: 
        <http://purl.obolibrary.org/obo/IAO_0000136>
    
    Domain: 
        OEO_00140151
    
    Range: 
        OEO_00140149
    
    
ObjectProperty: OEO_00010121

    Annotations: 
        <http://purl.obolibrary.org/obo/IAO_0000115> "A relation between a specifically dependent continuant (the dependent) and an independent continuant or energy (the bearer), in which the dependent is specifically reliant on the bearer for its existence",
        <http://purl.obolibrary.org/obo/IAO_0000233> "issue: https://github.com/OpenEnergyPlatform/ontology/issues/444
pull request: issue: https://github.com/OpenEnergyPlatform/ontology/pull/853

add domains and ranges:
issue: https://github.com/OpenEnergyPlatform/ontology/issues/973
pull request: https://github.com/OpenEnergyPlatform/ontology/pull/985

extend range to energy:
issue: https://github.com/OpenEnergyPlatform/ontology/issues/973
pull request: https://github.com/OpenEnergyPlatform/ontology/pull/985

correct definition with respect to energy:
issue: https://github.com/OpenEnergyPlatform/ontology/issues/1305
pull request: https://github.com/OpenEnergyPlatform/ontology/pull/1484",
        rdfs:label "has bearer"@en
    
    Domain: 
        <http://purl.obolibrary.org/obo/BFO_0000020>
    
    Range: 
        OEO_00000150 or <http://purl.obolibrary.org/obo/BFO_0000004>
    
    InverseOf: 
        <http://purl.obolibrary.org/obo/RO_0000053>
    
    
ObjectProperty: OEO_00010231

    Annotations: 
        <http://purl.obolibrary.org/obo/IAO_0000115> "A relation between an entity and an information artifact.",
        <http://purl.obolibrary.org/obo/IAO_0000233> "issue: https://github.com/OpenEnergyPlatform/ontology/issues/858
pull request: https://github.com/OpenEnergyPlatform/ontology/pull/965
",
        rdfs:label "has information content entity"@en
    
    Range: 
        <http://purl.obolibrary.org/obo/IAO_0000030>
    
    InverseOf: 
        <http://purl.obolibrary.org/obo/IAO_0000136>
    
    
ObjectProperty: OEO_00010234

    Annotations: 
        <http://purl.obolibrary.org/obo/IAO_0000115> "A relation between an artificial object or a process and an energy, where the energy is an input of the artificial object or process.",
        <http://purl.obolibrary.org/obo/IAO_0000233> "issue: https://github.com/OpenEnergyPlatform/ontology/issues/994
pull request: https://github.com/OpenEnergyPlatform/ontology/pull/1006

move to oeo-shared:
issue: https://github.com/OpenEnergyPlatform/ontology/issues/1384
pull request: https://github.com/OpenEnergyPlatform/ontology/pull/1390",
        rdfs:label "has energy input"@en
    
    SubPropertyOf: 
        <http://openenergy-platform.org/ontology/oeo/oeo-physical/OEO_00010238>
    
    Domain: 
        OEO_00000061 or <http://purl.obolibrary.org/obo/BFO_0000015>
    
    Range: 
        OEO_00000150
    
    
ObjectProperty: OEO_00010235

    Annotations: 
        <http://purl.obolibrary.org/obo/IAO_0000115> "A relation between an artificial object or a process and an energy, where the energy is an output of the artificial object or process.",
        <http://purl.obolibrary.org/obo/IAO_0000233> "issue: https://github.com/OpenEnergyPlatform/ontology/issues/994
pull request: https://github.com/OpenEnergyPlatform/ontology/pull/1006

move to oeo-shared:
issue: https://github.com/OpenEnergyPlatform/ontology/issues/1384
pull request: https://github.com/OpenEnergyPlatform/ontology/pull/1390",
        rdfs:label "has energy output"@en
    
    SubPropertyOf: 
        <http://openenergy-platform.org/ontology/oeo/oeo-physical/OEO_00010238>
    
    Domain: 
        OEO_00000061 or <http://purl.obolibrary.org/obo/BFO_0000015>
    
    Range: 
        OEO_00000150
    
    
ObjectProperty: OEO_00010312

    Annotations: 
        <http://purl.obolibrary.org/obo/IAO_0000115> "A relation that holds between a sector and the processes or material entities it covers.",
        <http://purl.obolibrary.org/obo/IAO_0000233> "issue: https://github.com/OpenEnergyPlatform/ontology/issues/864
pull request: https://github.com/OpenEnergyPlatform/ontology/pull/1321",
        rdfs:label "is sector of"@en
    
    Domain: 
        OEO_00000367
    
    Range: 
        <http://purl.obolibrary.org/obo/BFO_0000015> or <http://purl.obolibrary.org/obo/BFO_0000040>
    
    
ObjectProperty: OEO_00020056

    Annotations: 
        <http://purl.obolibrary.org/obo/IAO_0000115> "A relation that relates a quantity value to its entity in reality.",
        <http://purl.obolibrary.org/obo/IAO_0000233> "issue: https://github.com/OpenEnergyPlatform/ontology/issues/700
pull request: https://github.com/OpenEnergyPlatform/ontology/pull/710",
        rdfs:label "quantity value of"
    
    SubPropertyOf: 
        <http://purl.obolibrary.org/obo/IAO_0000136>
    
    InverseOf: 
        OEO_00140002
    
    
ObjectProperty: OEO_00020071

    
ObjectProperty: OEO_00020179

    Annotations: 
        <http://purl.obolibrary.org/obo/IAO_0000115> "A relation that relates an economic value to a related entity in reality.",
        <http://purl.obolibrary.org/obo/IAO_0000233> "issue: https://github.com/OpenEnergyPlatform/ontology/issues/958
pull request: https://github.com/OpenEnergyPlatform/ontology/pull/1034

Make subproperty of 'quantity value of' and add domain:
issue: https://github.com/OpenEnergyPlatform/ontology/issues/1411
pull request: https://github.com/OpenEnergyPlatform/ontology/pull/1422",
        rdfs:label "economic value of"
    
    SubPropertyOf: 
        OEO_00020056
    
    Domain: 
        OEO_00140012
    
    
ObjectProperty: OEO_00020180

    
ObjectProperty: OEO_00020182

    Annotations: 
        <http://purl.obolibrary.org/obo/IAO_0000115> "A relation between an energy and an artificial object or a process, where the energy is used in the artificial object or process.",
        <http://purl.obolibrary.org/obo/IAO_0000233> "issue: https://github.com/OpenEnergyPlatform/ontology/issues/1057
pull request: https://github.com/OpenEnergyPlatform/ontology/pull/1065

move to oeo-shared:
issue: https://github.com/OpenEnergyPlatform/ontology/issues/1384
pull request: https://github.com/OpenEnergyPlatform/ontology/pull/1390",
        rdfs:label "is energy participant of"
    
    Domain: 
        OEO_00000150
    
    Range: 
        OEO_00000061 or <http://purl.obolibrary.org/obo/BFO_0000015>
    
    InverseOf: 
        <http://openenergy-platform.org/ontology/oeo/oeo-physical/OEO_00010238>
    
    
ObjectProperty: OEO_00020188

    Annotations: 
        <http://purl.obolibrary.org/obo/IAO_0000115> "A relation that holds between an information content entity and a licence.",
        <http://purl.obolibrary.org/obo/IAO_0000118> "has license",
        <http://purl.obolibrary.org/obo/IAO_0000233> "issue https://github.com/OpenEnergyPlatform/ontology/issues/1061
pull request https://github.com/OpenEnergyPlatform/ontology/pull/1090

Relabel, redefine and add domain and range:
issue: https://github.com/OpenEnergyPlatform/ontology/issues/1275
pull request: https://github.com/OpenEnergyPlatform/ontology/pull/1547",
        rdfs:label "has licence"
    
    SubPropertyOf: 
        OEO_00010231
    
    Domain: 
        <http://purl.obolibrary.org/obo/IAO_0000030>
    
    Range: 
        OEO_00020015
    
    
ObjectProperty: OEO_00020189

    Annotations: 
        <http://purl.obolibrary.org/obo/IAO_0000115> "c is an information input of p iff: c is an input of p, and c is an information content entity",
        <http://purl.obolibrary.org/obo/IAO_0000233> "issue: https://github.com/OpenEnergyPlatform/ontology/issues/1091
pull request: https://github.com/OpenEnergyPlatform/ontology/pull/1113",
        rdfs:label "information input of"
    
    SubPropertyOf: 
        <http://purl.obolibrary.org/obo/RO_0002352>
    
    Domain: 
        <http://purl.obolibrary.org/obo/IAO_0000030>
    
    Range: 
        <http://purl.obolibrary.org/obo/BFO_0000015>
    
    
ObjectProperty: OEO_00020190

    Annotations: 
        <http://purl.obolibrary.org/obo/IAO_0000115> "c is an information output of p iff: c is an output of p, and c is an information content entity",
        <http://purl.obolibrary.org/obo/IAO_0000233> "issue: https://github.com/OpenEnergyPlatform/ontology/issues/1091
pull request: https://github.com/OpenEnergyPlatform/ontology/pull/1113",
        rdfs:label "information output of"
    
    SubPropertyOf: 
        <http://purl.obolibrary.org/obo/RO_0002353>
    
    Domain: 
        <http://purl.obolibrary.org/obo/IAO_0000030>
    
    Range: 
        <http://purl.obolibrary.org/obo/BFO_0000015>
    
    
ObjectProperty: OEO_00040010

    Annotations: 
        <http://purl.obolibrary.org/obo/IAO_0000115> "A property that links a quantity value to a unit in which the quantity value has been expressed.",
        rdfs:label "has unit"@en
    
    Domain: 
        OEO_00000350
    
    Range: 
        <http://purl.obolibrary.org/obo/UO_0000000>
    
    
ObjectProperty: OEO_00140002

    InverseOf: 
        OEO_00020056
    
    
ObjectProperty: OEO_00140008

    Annotations: 
        <http://purl.obolibrary.org/obo/IAO_0000115> "A relation between an information content entity / model and a continuant, in which the continuant is somehow involved in the creation of the information content entity / model.",
        <http://purl.obolibrary.org/obo/IAO_0000233> "issue: https://github.com/OpenEnergyPlatform/ontology/issues/530
pull request: https://github.com/OpenEnergyPlatform/ontology/pull/556
pull request: https://github.com/OpenEnergyPlatform/ontology/pull/626 (extend def for information content entity)
pull request: https://github.com/OpenEnergyPlatform/ontology/pull/871 (domain and range; move to oeo-shared)",
        rdfs:label "has contributor"@en
    
    Domain: 
        OEO_00000274 or <http://purl.obolibrary.org/obo/IAO_0000030>
    
    Range: 
        <http://purl.obolibrary.org/obo/BFO_0000002>
    
    
ObjectProperty: OEO_00140093

    Annotations: 
        <http://purl.obolibrary.org/obo/IAO_0000115> "p has information input c iff: p has input c, and c is an information content entity",
        <http://purl.obolibrary.org/obo/IAO_0000233> "issue: https://github.com/OpenEnergyPlatform/ontology/issues/618
pull request: https://github.com/OpenEnergyPlatform/ontology/pull/716
moved to oeo-shared
pull request: https://github.com/OpenEnergyPlatform/ontology/pull/1113",
        rdfs:label "has information input"@en
    
    SubPropertyOf: 
        <http://purl.obolibrary.org/obo/RO_0002233>
    
    Domain: 
        <http://purl.obolibrary.org/obo/BFO_0000015>
    
    Range: 
        <http://purl.obolibrary.org/obo/IAO_0000030>
    
    
ObjectProperty: OEO_00140094

    Annotations: 
        <http://purl.obolibrary.org/obo/IAO_0000115> "p has information output c iff: p has output c, and c is an information content entity",
        <http://purl.obolibrary.org/obo/IAO_0000233> "issue: https://github.com/OpenEnergyPlatform/ontology/issues/618
pull request: https://github.com/OpenEnergyPlatform/ontology/pull/716
moved to oeo-shared
pull request: https://github.com/OpenEnergyPlatform/ontology/pull/1113",
        rdfs:label "has information output"@en
    
    SubPropertyOf: 
        <http://purl.obolibrary.org/obo/RO_0002234>
    
    Domain: 
        <http://purl.obolibrary.org/obo/BFO_0000015>
    
    Range: 
        <http://purl.obolibrary.org/obo/IAO_0000030>
    
    
ObjectProperty: OEO_00140164

    Annotations: 
        <http://purl.obolibrary.org/obo/IAO_0000115> "A relation between a model and the thing it reproduces.",
        <http://purl.obolibrary.org/obo/IAO_0000233> "issue: https://github.com/OpenEnergyPlatform/ontology/issues/415
pull request: https://github.com/OpenEnergyPlatform/ontology/pull/821",
        rdfs:label "models"@en
    
    Domain: 
        OEO_00000274
    
    Range: 
        <http://purl.obolibrary.org/obo/BFO_0000004>
    
    
ObjectProperty: OEO_00240025

    Annotations: 
        <http://purl.obolibrary.org/obo/IAO_0000115> "c is physical output of p iff: c output of p, and c is a material entity"@en,
        <http://purl.obolibrary.org/obo/IAO_0000233> "issue: https://github.com/OpenEnergyPlatform/ontology/issues/1053
pull request: https://github.com/OpenEnergyPlatform/ontology/pull/1082

move to oeo-shared:
issue: https://github.com/OpenEnergyPlatform/ontology/issues/1384
pull request: https://github.com/OpenEnergyPlatform/ontology/pull/1390",
        rdfs:label "physical output of"
    
    SubPropertyOf: 
        <http://purl.obolibrary.org/obo/RO_0002353>
    
    Domain: 
        <http://purl.obolibrary.org/obo/BFO_0000040>
    
    Range: 
        <http://purl.obolibrary.org/obo/BFO_0000015>
    
    InverseOf: 
        OEO_00000533
    
    
ObjectProperty: owl:topObjectProperty

    
DataProperty: OEO_00140178

    
Class: <http://purl.obolibrary.org/obo/BFO_0000002>

    
Class: <http://purl.obolibrary.org/obo/BFO_0000003>

    
Class: <http://purl.obolibrary.org/obo/BFO_0000004>

    
Class: <http://purl.obolibrary.org/obo/BFO_0000006>

    
Class: <http://purl.obolibrary.org/obo/BFO_0000009>

    
Class: <http://purl.obolibrary.org/obo/BFO_0000015>

    
Class: <http://purl.obolibrary.org/obo/BFO_0000016>

    
Class: <http://purl.obolibrary.org/obo/BFO_0000017>

    
Class: <http://purl.obolibrary.org/obo/BFO_0000019>

    
Class: <http://purl.obolibrary.org/obo/BFO_0000020>

    
Class: <http://purl.obolibrary.org/obo/BFO_0000023>

    
Class: <http://purl.obolibrary.org/obo/BFO_0000027>

    
Class: <http://purl.obolibrary.org/obo/BFO_0000030>

    
Class: <http://purl.obolibrary.org/obo/BFO_0000031>

    
Class: <http://purl.obolibrary.org/obo/BFO_0000034>

    
Class: <http://purl.obolibrary.org/obo/BFO_0000038>

    
Class: <http://purl.obolibrary.org/obo/BFO_0000040>

    
Class: <http://purl.obolibrary.org/obo/BFO_0000141>

    
Class: <http://purl.obolibrary.org/obo/BFO_0000148>

    
Class: <http://purl.obolibrary.org/obo/IAO_0000027>

    Annotations: 
        
            Annotations: <http://purl.obolibrary.org/obo/IAO_0000233> "issue: https://github.com/OpenEnergyPlatform/ontology/issues/823
pull request: https://github.com/OpenEnergyPlatform/ontology/pull/826"
        <http://purl.obolibrary.org/obo/IAO_0000115> "A data item is an information content entity that is intended to be a truthful statement about something (modulo, e.g., measurement precision or other systematic errors) and is constructed/acquired by a method which reliably tends to produce (approximately) truthful statements.",
        <http://purl.obolibrary.org/obo/IAO_0000119> "http://www.ontobee.org/ontology/IAO?iri=http://purl.obolibrary.org/obo/IAO_0000027"
    
    
Class: <http://purl.obolibrary.org/obo/IAO_0000030>

    Annotations: 
        <http://purl.obolibrary.org/obo/IAO_0000233> "add axiom has copyright license
issue https://github.com/OpenEnergyPlatform/ontology/issues/1061
pull request https://github.com/OpenEnergyPlatform/ontology/pull/1090

Delete axiom has (copyright) licence:
issue: https://github.com/OpenEnergyPlatform/ontology/issues/1275
pull request: https://github.com/OpenEnergyPlatform/ontology/pull/1547"
    
    
Class: <http://purl.obolibrary.org/obo/IAO_0000088>

    SubClassOf: 
        OEO_00020188 some OEO_00010412
    
    
Class: <http://purl.obolibrary.org/obo/IAO_0000100>

    SubClassOf: 
        OEO_00000514 some OEO_00020121,
        OEO_00020188 some OEO_00020186
    
    
Class: <http://purl.obolibrary.org/obo/IAO_0000104>

    
Class: <http://purl.obolibrary.org/obo/IAO_0000310>

    SubClassOf: 
        OEO_00020188 some OEO_00010412
    
    
Class: <http://purl.obolibrary.org/obo/RO_0002577>

    
Class: <http://purl.obolibrary.org/obo/UO_0000000>

    Annotations: 
        <http://purl.obolibrary.org/obo/IAO_0000233> "issue: https://github.com/OpenEnergyPlatform/ontology/issues/533
pull request: https://github.com/OpenEnergyPlatform/ontology/pull/537
renaming
pull request: https://github.com/OpenEnergyPlatform/ontology/pull/895",
        rdfs:comment "The original definition from UO is \"A unit of measurement is a standardized quantity of a physical quality.\". It was adjusted for OEO purposes such that currencies can also be defined as units."
    
    SubClassOf: 
        <http://purl.obolibrary.org/obo/BFO_0000031>
    
    
Class: <http://purl.obolibrary.org/obo/UO_0000001>

    
Class: <http://purl.obolibrary.org/obo/UO_0000002>

    
Class: <http://purl.obolibrary.org/obo/UO_0000003>

    
Class: <http://purl.obolibrary.org/obo/UO_0000036>

    
Class: <http://purl.obolibrary.org/obo/UO_0000046>

    SubClassOf: 
        <http://purl.obolibrary.org/obo/BFO_0000141>
    
    
Class: <http://purl.obolibrary.org/obo/UO_0000047>

    
Class: <http://purl.obolibrary.org/obo/UO_0000111>

    
Class: <http://purl.obolibrary.org/obo/UO_0000224>

    Annotations: 
        <http://purl.obolibrary.org/obo/IAO_0000118> "kilowatt hours",
        <http://purl.obolibrary.org/obo/IAO_0000233> "add eurostat alternative term and has_exact_synonym:
issue: https://github.com/OpenEnergyPlatform/ontology/issues/920
pull request: https://github.com/OpenEnergyPlatform/ontology/pull/924",
        <http://www.geneontology.org/formats/oboInOwl#hasExactSynonym> "kWh",
        rdfs:comment "The original term from UO had neither an alternative term nor has_exact_synonym. It was added for OEO purposes to include the Eurostat spellings."@en
    
    
Class: <http://purl.obolibrary.org/obo/UO_0010006>

    
Class: <http://www.openenergy-platform.org/ontology/oeo/OEO_00330023>

    Annotations: 
        <http://purl.obolibrary.org/obo/IAO_0000115> "A life cycle assessment is a methodology to calculate and analyse environmental impacts of the life cycle of a material entity or process.",
        <http://purl.obolibrary.org/obo/IAO_0000118> "LCA"@en,
        <http://purl.obolibrary.org/obo/IAO_0000118> "Lebenszyklusanalyse"@de,
        <http://purl.obolibrary.org/obo/IAO_0000118> "life cycle analysis"@en,
        <http://purl.obolibrary.org/obo/IAO_0000118> "Ökobilanz"@de,
        <http://purl.obolibrary.org/obo/IAO_0000233> "issue: https://github.com/OpenEnergyPlatform/ontology/issues/1551
pull request: https://github.com/OpenEnergyPlatform/ontology/pull/1576",
        rdfs:label "life cycle assessment"@en
    
    SubClassOf: 
        OEO_00020166
    
    
Class: OEO_00000001

    
Class: OEO_00000006

    
Class: OEO_00000007

    
Class: OEO_00000011

    
Class: OEO_00000014

    
Class: OEO_00000020

    
Class: OEO_00000031

    
Class: OEO_00000051

    
Class: OEO_00000061

    
Class: OEO_00000064

    
Class: OEO_00000087

    
Class: OEO_00000097

    
Class: OEO_00000099

    
Class: OEO_00000107

    
Class: OEO_00000115

    
Class: OEO_00000119

    
Class: OEO_00000139

    
Class: OEO_00000143

    
Class: OEO_00000144

    
Class: OEO_00000147

    
Class: OEO_00000148

    
Class: OEO_00000149

    
Class: OEO_00000150

    
Class: OEO_00000151

    
Class: OEO_00000173

    
Class: OEO_00000188

    
Class: OEO_00000198

    
Class: OEO_00000199

    
Class: OEO_00000200

    
Class: OEO_00000206

    
Class: OEO_00000207

    
Class: OEO_00000238

    
Class: OEO_00000253

    
Class: OEO_00000255

    
Class: OEO_00000264

    SubClassOf: 
        
            Annotations: <http://purl.obolibrary.org/obo/IAO_0000233> "issue: https://github.com/OpenEnergyPlatform/ontology/issues/415
pull request: https://github.com/OpenEnergyPlatform/ontology/pull/821"
        OEO_00140164 some OEO_00020065
    
    
Class: OEO_00000274

    
Class: OEO_00000275

    
Class: OEO_00000315

    DisjointWith: 
        OEO_00000323
    
    
Class: OEO_00000316

    
Class: OEO_00000323

    DisjointWith: 
        OEO_00000315
    
    
Class: OEO_00000331

    
Class: OEO_00000333

    
Class: OEO_00000334

    
Class: OEO_00000340

    Annotations: 
        OEO_00040001 "http://openenergy-platform.org/ontology/oeo/oeo-shared",
        <http://purl.obolibrary.org/obo/IAO_0000115> "A project is a process to achieve a specified goal that is unique in the sum of its conditions like its goal, time and cost budget and its organisation.",
        <http://purl.obolibrary.org/obo/IAO_0000233> "issue: https://github.com/OpenEnergyPlatform/ontology/issues/247
pull request: https://github.com/OpenEnergyPlatform/ontology/pull/418
move to oeo-shared
issue: https://github.com/OpenEnergyPlatform/ontology/issues/862
pull request: https://github.com/OpenEnergyPlatform/ontology/pull/869",
        rdfs:label "project"
    
    SubClassOf: 
        <http://purl.obolibrary.org/obo/BFO_0000015>
    
    
Class: OEO_00000350

    Annotations: 
        OEO_00040001 "http://openenergy-platform.org/ontology/oeo/oeo-shared",
        <http://purl.obolibrary.org/obo/IAO_0000115> "A quantity value is an information content entity defined by a numeral together with a unit of measurement to quantify an entity."@en,
        <http://purl.obolibrary.org/obo/IAO_0000233> "issue: https://github.com/OpenEnergyPlatform/ontology/issues/205
pull request: https://github.com/OpenEnergyPlatform/ontology/pull/386

issue: https://github.com/OpenEnergyPlatform/ontology/issues/495
pull request: https://github.com/OpenEnergyPlatform/ontology/pull/496

issue: https://github.com/OpenEnergyPlatform/ontology/issues/505
pull request: https://github.com/OpenEnergyPlatform/ontology/pull/518

issue: https://github.com/OpenEnergyPlatform/ontology/issues/1405
pull request: https://github.com/OpenEnergyPlatform/ontology/pull/1606",
        
            Annotations: <http://purl.obolibrary.org/obo/IAO_0000233> "issue: https://github.com/OpenEnergyPlatform/ontology/issues/636
pull request: https://github.com/OpenEnergyPlatform/ontology/pull/810"
        <http://purl.obolibrary.org/obo/IAO_0006011> "http://purl.obolibrary.org/obo/IAO_0000032",
        rdfs:label "quantity value"
    
    SubClassOf: 
        <http://purl.obolibrary.org/obo/IAO_0000030>
    
    
Class: OEO_00000364

    
Class: OEO_00000367

    
Class: OEO_00000368

    
Class: OEO_00000395

    
Class: OEO_00000403

    
Class: OEO_00000407

    Annotations: 
        OEO_00040001 "http://openenergy-platform.org/ontology/oeo/oeo-shared",
        <http://purl.obolibrary.org/obo/IAO_0000115> "A technology is a plan specification that describes how to combine artificial objects or other material entities and processes in a specific way."@en,
        <http://purl.obolibrary.org/obo/IAO_0000233> "issue: https://github.com/OpenEnergyPlatform/ontology/issues/136
pull request: https://github.com/OpenEnergyPlatform/ontology/pull/334
moved to oeo-shared, change definition, reclassify, add axiom
issue: https://github.com/OpenEnergyPlatform/ontology/issues/1572
pull request: https://github.com/OpenEnergyPlatform/ontology/pull/1591",
        rdfs:label "technology"
    
    SubClassOf: 
        <http://purl.obolibrary.org/obo/IAO_0000104>,
        <http://purl.obolibrary.org/obo/IAO_0000136> some 
            (OEO_00000061
             and (<http://purl.obolibrary.org/obo/RO_0000056> some <http://purl.obolibrary.org/obo/BFO_0000015>))
    
    
Class: OEO_00000419

    Annotations: 
        OEO_00040001 "http://openenergy-platform.org/ontology/oeo/oeo-shared",
        <http://purl.obolibrary.org/obo/IAO_0000115> "A transformation is a process that transforms one or more inputs into at least one output."@en,
        <http://purl.obolibrary.org/obo/IAO_0000233> "issue: https://github.com/OpenEnergyPlatform/ontology/issues/435
pull request: https://github.com/OpenEnergyPlatform/ontology/pull/450

input and output axioms:
issue: https://github.com/OpenEnergyPlatform/ontology/issues/1167
pull request: https://github.com/OpenEnergyPlatform/ontology/pull/1178",
        rdfs:label "transformation"
    
    SubClassOf: 
        <http://purl.obolibrary.org/obo/BFO_0000015>,
        <http://purl.obolibrary.org/obo/RO_0002233> some <http://purl.obolibrary.org/obo/BFO_0000002>,
        <http://purl.obolibrary.org/obo/RO_0002234> some <http://purl.obolibrary.org/obo/BFO_0000002>
    
    
Class: OEO_00000423

    SubClassOf: 
        
            Annotations: <http://purl.obolibrary.org/obo/IAO_0000233> "issue: https://github.com/OpenEnergyPlatform/ontology/issues/415
pull request: https://github.com/OpenEnergyPlatform/ontology/pull/821"
        OEO_00140164 some OEO_00000143
    
    
Class: OEO_00010023

    
Class: OEO_00010078

    
Class: OEO_00010079

    SubClassOf: 
        OEO_00020056 some OEO_00020063
    
    
Class: OEO_00010082

    
Class: OEO_00010083

    
Class: OEO_00010114

    
Class: OEO_00010115

    
Class: OEO_00010116

    
Class: OEO_00010117

    Annotations: 
        OEO_00040001 "http://openenergy-platform.org/ontology/oeo/oeo-shared",
        <http://purl.obolibrary.org/obo/IAO_0000115> "The role of an independent continuant or energy over which ownership rights can be established, whose ownership can be passed from one party to another by engaging in transactions, and that is not money.",
        <http://purl.obolibrary.org/obo/IAO_0000119> "https://spec.edmcouncil.org/fibo/ontology/FND/ProductsAndServices/ProductsAndServices/Good",
        <http://purl.obolibrary.org/obo/IAO_0000233> "issue: https://github.com/OpenEnergyPlatform/ontology/issues/832
pull request: https://github.com/OpenEnergyPlatform/ontology/pull/843
add relation to monetary price
pull request: https://github.com/OpenEnergyPlatform/ontology/pull/1034

update definition:
pull request: https://github.com/OpenEnergyPlatform/ontology/pull/1127

add 'has bearer' axiom
issue: https://github.com/OpenEnergyPlatform/ontology/issues/1305
pull request: https://github.com/OpenEnergyPlatform/ontology/pull/1310
pull request: https://github.com/OpenEnergyPlatform/ontology/pull/1485",
        rdfs:label "good role"@en
    
    SubClassOf: 
        <http://purl.obolibrary.org/obo/BFO_0000023>,
        OEO_00010121 some 
            (OEO_00000139 or <http://purl.obolibrary.org/obo/BFO_0000004>),
        OEO_00020180 some OEO_00040003
    
    
Class: OEO_00010127

    
Class: OEO_00010210

    
Class: OEO_00010211

    
Class: OEO_00010263

    
Class: OEO_00010264

    
Class: OEO_00010265

    
Class: OEO_00010266

    
Class: OEO_00010268

    
Class: OEO_00010269

    
Class: OEO_00010270

    
Class: OEO_00010271

    
Class: OEO_00010296

    SubClassOf: 
        <http://purl.obolibrary.org/obo/IAO_0000136> some OEO_00050018
    
    
Class: OEO_00010315

    
Class: OEO_00010316

    
Class: OEO_00010361

    
Class: OEO_00010362

    
Class: OEO_00010385

    
Class: OEO_00010386

    
Class: OEO_00010388

    
Class: OEO_00010404

    SubClassOf: 
        <http://purl.obolibrary.org/obo/IAO_0000136> some OEO_00020039
    
    
Class: OEO_00010406

    
Class: OEO_00010407

    SubClassOf: 
        OEO_00000504 some OEO_00010406
    
    
Class: OEO_00010412

    
Class: OEO_00020003

    
Class: OEO_00020006

    
Class: OEO_00020011

    Annotations: 
        OEO_00040001 "http://openenergy-platform.org/ontology/oeo/oeo-shared",
        <http://purl.obolibrary.org/obo/IAO_0000115> "A study is a project with the goal to investigate something."@en,
        <http://purl.obolibrary.org/obo/IAO_0000116> "The construct 'has funding source' some ('has role' some funder) is necessary, because has funding source has the range has role some funder. This range comes from issue https://github.com/OpenEnergyPlatform/ontology/issues/850 : funding source is some kind of independent continuant, i.e. a organisation or person, that does something special (giving money). So it is anything that has role some funder.",
        <http://purl.obolibrary.org/obo/IAO_0000233> "issue: https://github.com/OpenEnergyPlatform/ontology/issues/247
pull request: https://github.com/OpenEnergyPlatform/ontology/pull/497
add covers-relation (oeo-model)
pull request: https://github.com/OpenEnergyPlatform/ontology/pull/764
move to oeo-shared
issue: https://github.com/OpenEnergyPlatform/ontology/issues/862
pull request: https://github.com/OpenEnergyPlatform/ontology/pull/869
add axiom (study report)
issue: https://github.com/OpenEnergyPlatform/ontology/issues/971
pull request: https://github.com/OpenEnergyPlatform/ontology/pull/1011
add etitor note
pull request: https://github.com/OpenEnergyPlatform/ontology/pull/1025"@en,
        rdfs:label "study"@en
    
    SubClassOf: 
        OEO_00000340,
        
            Annotations: <http://purl.obolibrary.org/obo/IAO_0000233> "issue: https://github.com/OpenEnergyPlatform/ontology/issues/473
pull request: https://github.com/OpenEnergyPlatform/ontology/pull/557"
        OEO_00000509 some (<http://purl.obolibrary.org/obo/RO_0000087> some OEO_00090001),
        <http://purl.obolibrary.org/obo/RO_0000057> some <http://purl.obolibrary.org/obo/IAO_0000100>,
        <http://purl.obolibrary.org/obo/RO_0002234> some OEO_00020012
    
    
Class: OEO_00020012

    Annotations: 
        OEO_00040001 "http://openenergy-platform.org/ontology/oeo/oeo-shared",
        <http://purl.obolibrary.org/obo/IAO_0000115> "A study report is a report that is the output from some study."@en,
        <http://purl.obolibrary.org/obo/IAO_0000233> "issue: https://github.com/OpenEnergyPlatform/ontology/issues/247
pull request: https://github.com/OpenEnergyPlatform/ontology/pull/497
add etitor note
pull request: https://github.com/OpenEnergyPlatform/ontology/pull/1025"@en,
        rdfs:label "study report"@en
    
    SubClassOf: 
        <http://purl.obolibrary.org/obo/IAO_0000088>,
        
            Annotations: <http://purl.obolibrary.org/obo/IAO_0000233> "issue: https://github.com/OpenEnergyPlatform/ontology/issues/473
pull request: https://github.com/OpenEnergyPlatform/ontology/pull/557

issue: https://github.com/OpenEnergyPlatform/ontology/issues/850
pull request: https://github.com/OpenEnergyPlatform/ontology/pull/871"
        OEO_00000506 some (<http://purl.obolibrary.org/obo/RO_0000087> some OEO_00000064),
        <http://purl.obolibrary.org/obo/IAO_0000136> some <http://purl.obolibrary.org/obo/IAO_0000100>,
        <http://purl.obolibrary.org/obo/RO_0002353> some OEO_00020011
    
    
Class: OEO_00020015

    
Class: OEO_00020016

    
Class: OEO_00020018

    
Class: OEO_00020032

    
Class: OEO_00020035

    
Class: OEO_00020039

    Annotations: 
        OEO_00040001 "http://openenergy-platform.org/ontology/oeo/oeo-shared",
        <http://purl.obolibrary.org/obo/IAO_0000115> "An energy carrier is a material entity that has an energy carrier disposition.",
        <http://purl.obolibrary.org/obo/IAO_0000233> "issue: https://github.com/OpenEnergyPlatform/ontology/issues/407
pull request: https://github.com/OpenEnergyPlatform/ontology/pull/627
move to oeo-shared
pull request: https://github.com/OpenEnergyPlatform/ontology/pull/869
improve definition:
issue: https://github.com/OpenEnergyPlatform/ontology/issues/1169
pull request: https://github.com/OpenEnergyPlatform/ontology/pull/1173",
        rdfs:label "energy carrier"
    
    EquivalentTo: 
        <http://purl.obolibrary.org/obo/BFO_0000040>
         and (<http://purl.obolibrary.org/obo/RO_0000091> some OEO_00000151)
    
    SubClassOf: 
        <http://purl.obolibrary.org/obo/BFO_0000040>
    
    
Class: OEO_00020060

    Annotations: 
        OEO_00040001 "http://openenergy-platform.org/ontology/oeo/oeo-shared",
        <http://purl.obolibrary.org/obo/IAO_0000115> "A fuel market exchange is an energy market exchange where fuels like oil, coal, renewable fuels, and natural gas are traded.",
        <http://purl.obolibrary.org/obo/IAO_0000233> "issue https://github.com/OpenEnergyPlatform/ontology/issues/677
pull request https://github.com/OpenEnergyPlatform/ontology/pull/740
pull request https://github.com/OpenEnergyPlatform/ontology/pull/748

Move to oeo-shared:
issue: https://github.com/OpenEnergyPlatform/ontology/issues/1458
pull request: https://github.com/OpenEnergyPlatform/ontology/pull/1478",
        rdfs:label "fuel market exchange"
    
    SubClassOf: 
        OEO_00020065,
        OEO_00020071 some (<http://purl.obolibrary.org/obo/RO_0000087> some OEO_00020066)
    
    
Class: OEO_00020063

    
Class: OEO_00020065

    Annotations: 
        OEO_00040001 "http://openenergy-platform.org/ontology/oeo/oeo-shared",
        <http://purl.obolibrary.org/obo/IAO_0000115> "An energy market exchange is a market exchange in which energy commodities are traded.",
        <http://purl.obolibrary.org/obo/IAO_0000233> "issue https://github.com/OpenEnergyPlatform/ontology/issues/256
pull request https://github.com/OpenEnergyPlatform/ontology/pull/748

Move to oeo-shared:
issue: https://github.com/OpenEnergyPlatform/ontology/issues/1458
pull request: https://github.com/OpenEnergyPlatform/ontology/pull/1478",
        rdfs:label "energy market exchange"
    
    SubClassOf: 
        OEO_00020069
    
    
Class: OEO_00020066

    Annotations: 
        OEO_00040001 "http://openenergy-platform.org/ontology/oeo/oeo-shared",
        <http://purl.obolibrary.org/obo/IAO_0000115> "Fuel commodity role is the commodity role of fuels.",
        <http://purl.obolibrary.org/obo/IAO_0000233> "https://github.com/OpenEnergyPlatform/ontology/issues/256
https://github.com/OpenEnergyPlatform/ontology/pull/748",
        rdfs:label "fuel commodity role"
    
    SubClassOf: 
        OEO_00040011
    
    
Class: OEO_00020067

    Annotations: 
        OEO_00040001 "http://openenergy-platform.org/ontology/oeo/oeo-shared",
        <http://purl.obolibrary.org/obo/IAO_0000115> "A commodity is a good that bears the commodity role.",
        <http://purl.obolibrary.org/obo/IAO_0000233> "issue: https://github.com/OpenEnergyPlatform/ontology/issues/302
pull request: https://github.com/OpenEnergyPlatform/ontology/pull/748
add alternative term
pull request: https://github.com/OpenEnergyPlatform/ontology/pull/800
subclass of good
pull request: https://github.com/OpenEnergyPlatform/ontology/pull/843
change axiom
pull request: https://github.com/OpenEnergyPlatform/ontology/pull/869",
        rdfs:label "commodity"
    
    EquivalentTo: 
        OEO_00010116
         and (<http://purl.obolibrary.org/obo/RO_0000087> some OEO_00040011)
    
    SubClassOf: 
        OEO_00010116
    
    
Class: OEO_00020068

    Annotations: 
        OEO_00040001 "http://openenergy-platform.org/ontology/oeo/oeo-shared",
        <http://purl.obolibrary.org/obo/IAO_0000115> "A fuel commodity is a commodity that is a fuel.",
        <http://purl.obolibrary.org/obo/IAO_0000233> "issue: https://github.com/OpenEnergyPlatform/ontology/issues/302
pull request: https://github.com/OpenEnergyPlatform/ontology/pull/748",
        rdfs:label "fuel commodity"
    
    EquivalentTo: 
        <http://purl.obolibrary.org/obo/RO_0000087> some OEO_00020066
    
    SubClassOf: 
        OEO_00020067
    
    
Class: OEO_00020069

    
Class: OEO_00020072

    SubClassOf: 
        <http://purl.obolibrary.org/obo/IAO_0000136> some OEO_00000367
    
    
Class: OEO_00020085

    Annotations: 
        OEO_00040001 "http://openenergy-platform.org/ontology/oeo/oeo-shared",
        <http://purl.obolibrary.org/obo/IAO_0000115> "A renewable energy is an energy that has renewable origin.",
        <http://purl.obolibrary.org/obo/IAO_0000233> "issue: https://github.com/OpenEnergyPlatform/ontology/issues/741
pull request: https://github.com/OpenEnergyPlatform/ontology/pull/861

Move to oeo-shared:
issue:https://github.com/OpenEnergyPlatform/ontology/issues/1423
pull request: https://github.com/OpenEnergyPlatform/ontology/pull/1437",
        rdfs:label "renewable energy"
    
    EquivalentTo: 
        OEO_00000150
         and (OEO_00000530 some OEO_00030004)
    
    SubClassOf: 
        OEO_00000150
    
    
Class: OEO_00020097

    
Class: OEO_00020098

    
Class: OEO_00020102

    Annotations: 
        OEO_00040001 "http://openenergy-platform.org/ontology/oeo/oeo-shared",
        <http://purl.obolibrary.org/obo/IAO_0000115> "An energy transformation unit is an artificial object that transforms, changes or transfers a certain type of energy.",
        <http://purl.obolibrary.org/obo/IAO_0000233> "issue: https://github.com/OpenEnergyPlatform/ontology/issues/465
pull request: https://github.com/OpenEnergyPlatform/ontology/pull/895

move to oeo-shared:
issue: https://github.com/OpenEnergyPlatform/ontology/issues/1384
pull request: https://github.com/OpenEnergyPlatform/ontology/pull/1390",
        rdfs:label "energy transformation unit"
    
    SubClassOf: 
        OEO_00000061,
        OEO_00010235 some OEO_00010114,
        
            Annotations: <http://purl.obolibrary.org/obo/IAO_0000233> "issue: https://github.com/OpenEnergyPlatform/ontology/issues/980
pull request: https://github.com/OpenEnergyPlatform/ontology/pull/1010"
        <http://purl.obolibrary.org/obo/BFO_0000051> some OEO_00000011,
        <http://purl.obolibrary.org/obo/RO_0000056> some OEO_00020003,
        <http://purl.obolibrary.org/obo/RO_0000056> some OEO_00020104
    
    
Class: OEO_00020104

    Annotations: 
        OEO_00040001 "http://openenergy-platform.org/ontology/oeo/oeo-physical",
        <http://purl.obolibrary.org/obo/IAO_0000115> "An outage is a process during which an artificial object cannot perform or operate.",
        <http://purl.obolibrary.org/obo/IAO_0000233> "issue: https://github.com/OpenEnergyPlatform/ontology/issues/887
pull request: https://github.com/OpenEnergyPlatform/ontology/pull/897

move to oeo-shared:
issue: https://github.com/OpenEnergyPlatform/ontology/issues/1384
pull request: https://github.com/OpenEnergyPlatform/ontology/pull/1390",
        rdfs:label "outage"
    
    SubClassOf: 
        <http://purl.obolibrary.org/obo/BFO_0000015>,
        <http://purl.obolibrary.org/obo/RO_0000057> some OEO_00020102
    
    
Class: OEO_00020107

    Annotations: 
        OEO_00040001 "http://openenergy-platform.org/ontology/oeo/oeo-physical",
        <http://purl.obolibrary.org/obo/IAO_0000115> "Curtailment is a process in which a power generating unit is forced to reduce its output, in order to balance energy supply and demand or due to transmission constraints.",
        <http://purl.obolibrary.org/obo/IAO_0000233> "issue: https://github.com/OpenEnergyPlatform/ontology/issues/888
pull request: https://github.com/OpenEnergyPlatform/ontology/pull/897",
        rdfs:label "curtailment"
    
    SubClassOf: 
        <http://purl.obolibrary.org/obo/BFO_0000015>,
        <http://purl.obolibrary.org/obo/RO_0000057> some OEO_00000334
    
    
Class: OEO_00020121

    
Class: OEO_00020122

    DisjointWith: 
        OEO_00020123
    
    
Class: OEO_00020123

    DisjointWith: 
        OEO_00020122
    
    
Class: OEO_00020136

    Annotations: 
        OEO_00040001 "http://openenergy-platform.org/ontology/oeo/oeo-shared",
        <http://purl.obolibrary.org/obo/IAO_0000115> "A space requirement is a two-dimensional spatial region that covers the area needed by an object or object aggregate.",
        <http://purl.obolibrary.org/obo/IAO_0000118> "land use",
        <http://purl.obolibrary.org/obo/IAO_0000233> "issue: https://github.com/OpenEnergyPlatform/ontology/issues/889
pull request: https://github.com/OpenEnergyPlatform/ontology/pull/933

extend definition and add alternative term
issue: https://github.com/OpenEnergyPlatform/ontology/issues/1051
pull request: https://github.com/OpenEnergyPlatform/ontology/pull/1084",
        rdfs:label "space requirement"
    
    SubClassOf: 
        <http://purl.obolibrary.org/obo/BFO_0000009>
    
    
Class: OEO_00020140

    Annotations: 
        OEO_00040001 "http://openenergy-platform.org/ontology/oeo/oeo-shared",
        <http://purl.obolibrary.org/obo/IAO_0000115> "An area per power unit is a unit which is a measure for an area per nameplate capacity.",
        <http://purl.obolibrary.org/obo/IAO_0000233> "issue: https://github.com/OpenEnergyPlatform/ontology/issues/889
pull request: https://github.com/OpenEnergyPlatform/ontology/pull/930",
        rdfs:label "area per power unit"
    
    SubClassOf: 
        <http://purl.obolibrary.org/obo/UO_0000000>
    
    
Class: OEO_00020142

    Annotations: 
        OEO_00040001 "http://openenergy-platform.org/ontology/oeo/oeo-shared",
        <http://purl.obolibrary.org/obo/IAO_0000115> "An area unit which is equal to one million square meters or 10^[6] m^[2].",
        <http://purl.obolibrary.org/obo/IAO_0000118> "km^[2]",
        <http://purl.obolibrary.org/obo/IAO_0000118> "square km",
        <http://purl.obolibrary.org/obo/IAO_0000233> "issue: https://github.com/OpenEnergyPlatform/ontology/issues/889
pull request: https://github.com/OpenEnergyPlatform/ontology/pull/933",
        rdfs:label "square kilometer"
    
    SubClassOf: 
        <http://purl.obolibrary.org/obo/UO_0000047>
    
    
Class: OEO_00020143

    Annotations: 
        OEO_00040001 "http://openenergy-platform.org/ontology/oeo/oeo-shared",
        <http://purl.obolibrary.org/obo/IAO_0000115> "An area value is a quantity value indicating the size of a two-dimensional spatial region.",
        <http://purl.obolibrary.org/obo/IAO_0000233> "issue: https://github.com/OpenEnergyPlatform/ontology/issues/889
pull request: https://github.com/OpenEnergyPlatform/ontology/pull/933",
        rdfs:label "area value"
    
    SubClassOf: 
        OEO_00000350,
        OEO_00020056 some <http://purl.obolibrary.org/obo/BFO_0000009>,
        OEO_00040010 some <http://purl.obolibrary.org/obo/UO_0000047>
    
    
Class: OEO_00020154

    
Class: OEO_00020155

    Annotations: 
        OEO_00040001 "http://openenergy-platform.org/ontology/oeo/oeo-shared",
        <http://purl.obolibrary.org/obo/IAO_0000115> "Social cost of carbon emission is the cost the society bears for a greenhouse gas emission value.",
        <http://purl.obolibrary.org/obo/IAO_0000118> "social cost of CO2",
        <http://purl.obolibrary.org/obo/IAO_0000233> "issue: https://github.com/OpenEnergyPlatform/ontology/issues/866
pull request: https://github.com/OpenEnergyPlatform/ontology/pull/956
add axiom to emission value, add new parent class and relabel
pull request: https://github.com/OpenEnergyPlatform/ontology/pull/1034",
        rdfs:label "social cost of carbon emission"
    
    SubClassOf: 
        OEO_00020181,
        OEO_00020179 some OEO_00140081,
        <http://purl.obolibrary.org/obo/IAO_0000136> some OEO_00140081
    
    
Class: OEO_00020166

    Annotations: 
        OEO_00040001 "http://openenergy-platform.org/ontology/oeo/oeo-shared",
        <http://purl.obolibrary.org/obo/IAO_0000115> "A methodology is a plan specification that describes processes that are part of a study.",
        <http://purl.obolibrary.org/obo/IAO_0000233> "issue: https://github.com/OpenEnergyPlatform/ontology/issues/971
pull request: https://github.com/OpenEnergyPlatform/ontology/pull/1011

move to oeo-shared:
issue: https://github.com/OpenEnergyPlatform/ontology/issues/1129
pull request: https://github.com/OpenEnergyPlatform/ontology/pull/1306"@en,
        rdfs:label "methodology"
    
    SubClassOf: 
        <http://purl.obolibrary.org/obo/IAO_0000104>,
        <http://purl.obolibrary.org/obo/BFO_0000050> some OEO_00020011
    
    
Class: OEO_00020175

    Annotations: 
        OEO_00040001 "http://openenergy-platform.org/ontology/oeo/oeo-shared",
        <http://purl.obolibrary.org/obo/IAO_0000115> "A life time is a time span of an artificial object that measures the time during which the artificial object exists.",
        <http://purl.obolibrary.org/obo/IAO_0000233> "issue: https://github.com/OpenEnergyPlatform/ontology/issues/894
pull request: https://github.com/OpenEnergyPlatform/ontology/pull/1026",
        rdfs:label "life time"
    
    SubClassOf: 
        OEO_00030035,
        OEO_00020056 some OEO_00000061
    
    
Class: OEO_00020176

    Annotations: 
        OEO_00040001 "http://openenergy-platform.org/ontology/oeo/oeo-shared",
        <http://purl.obolibrary.org/obo/IAO_0000115> "A construction time is a time span that measures the time that is needed to construct an artificial object.",
        <http://purl.obolibrary.org/obo/IAO_0000233> "issue: https://github.com/OpenEnergyPlatform/ontology/issues/894
pull request: https://github.com/OpenEnergyPlatform/ontology/pull/1026",
        rdfs:label "construction time"
    
    SubClassOf: 
        OEO_00030035,
        OEO_00020056 some OEO_00000061
    
    
Class: OEO_00020177

    
Class: OEO_00020178

    
Class: OEO_00020181

    Annotations: 
        OEO_00040001 "http://openenergy-platform.org/ontology/oeo/oeo-shared",
        <http://purl.obolibrary.org/obo/IAO_0000115> "Social cost of emission is the cost the society bears for an emission value.",
        <http://purl.obolibrary.org/obo/IAO_0000233> "issue: https://github.com/OpenEnergyPlatform/ontology/issues/958
pull request: https://github.com/OpenEnergyPlatform/ontology/pull/1034",
        rdfs:label "social cost of emission"
    
    SubClassOf: 
        OEO_00040009,
        OEO_00020179 some OEO_00140081,
        <http://purl.obolibrary.org/obo/IAO_0000136> some OEO_00140081
    
    
Class: OEO_00020185

    Annotations: 
        <http://purl.obolibrary.org/obo/IAO_0000118> "copyright license"
    
    
Class: OEO_00020186

    
Class: OEO_00020187

    
Class: OEO_00020201

    Annotations: 
        OEO_00040001 "http://openenergy-platform.org/ontology/oeo/oeo-shared",
        <http://purl.obolibrary.org/obo/IAO_0000115> "Import is the process of purchasing goods or services abroad and their delivery to the domestic market.",
        <http://purl.obolibrary.org/obo/IAO_0000233> "add class
issue: https://github.com/OpenEnergyPlatform/ontology/issues/998
pull request: https://github.com/OpenEnergyPlatform/ontology/pull/1221

add 'has participant axiom':
issue: https://github.com/OpenEnergyPlatform/ontology/issues/1327
pull request: https://github.com/OpenEnergyPlatform/ontology/pull/1395",
        rdfs:label "import"
    
    SubClassOf: 
        <http://purl.obolibrary.org/obo/BFO_0000015>,
        (<http://purl.obolibrary.org/obo/RO_0000057> some OEO_00010116) or (<http://purl.obolibrary.org/obo/RO_0002410> some OEO_00140124)
    
    
Class: OEO_00020202

    Annotations: 
        OEO_00040001 "http://openenergy-platform.org/ontology/oeo/oeo-shared",
        <http://purl.obolibrary.org/obo/IAO_0000115> "Export is the process of selling goods or services abroad and their delivery to a foreign market.",
        <http://purl.obolibrary.org/obo/IAO_0000233> "add class
issue: https://github.com/OpenEnergyPlatform/ontology/issues/998
pull request: https://github.com/OpenEnergyPlatform/ontology/pull/1221

add 'has participant axiom':
issue: https://github.com/OpenEnergyPlatform/ontology/issues/1327
pull request: https://github.com/OpenEnergyPlatform/ontology/pull/1395",
        rdfs:label "export"
    
    SubClassOf: 
        <http://purl.obolibrary.org/obo/BFO_0000015>,
        (<http://purl.obolibrary.org/obo/RO_0000057> some OEO_00010116) or (<http://purl.obolibrary.org/obo/RO_0002410> some OEO_00140124)
    
    
Class: OEO_00020204

    
Class: OEO_00020205

    
Class: OEO_00020206

    
Class: OEO_00020207

    
Class: OEO_00020208

    
Class: OEO_00020248

    
Class: OEO_00020252

    
Class: OEO_00020264

    
Class: OEO_00020267

    
Class: OEO_00020309

    EquivalentTo: 
        OEO_00020248
         and (<http://purl.obolibrary.org/obo/IAO_0000136> some 
            (OEO_00140149 or OEO_00140151))
    
    
Class: OEO_00020310

    
Class: OEO_00020311

    
Class: OEO_00020312

    
Class: OEO_00020313

    
Class: OEO_00020314

    
Class: OEO_00020317

    EquivalentTo: 
        OEO_00000364
         and (<http://purl.obolibrary.org/obo/IAO_0000136> some OEO_00000199)
    
    
Class: OEO_00020321

    EquivalentTo: 
        OEO_00000364
         and (<http://purl.obolibrary.org/obo/IAO_0000136> some OEO_00260007)
    
    
Class: OEO_00030002

    
Class: OEO_00030003

    
Class: OEO_00030004

    
Class: OEO_00030008

    EquivalentTo: 
        OEO_00000364
         and (<http://purl.obolibrary.org/obo/IAO_0000136> some OEO_00010115)
    
    
Class: OEO_00030009

    EquivalentTo: 
        OEO_00000364
         and (<http://purl.obolibrary.org/obo/IAO_0000136> some OEO_00000147)
    
    
Class: OEO_00030015

    
Class: OEO_00030019

    Annotations: 
        OEO_00040001 "http://openenergy-platform.org/ontology/oeo/oeo-shared",
        <http://purl.obolibrary.org/obo/IAO_0000115> "A process attribute is a dependent occurrent that existentially depends on a process.",
        <http://purl.obolibrary.org/obo/IAO_0000233> "issue: https://github.com/OpenEnergyPlatform/ontology/issues/205
pull request: https://github.com/OpenEnergyPlatform/ontology/pull/386",
        rdfs:label "process attribute"
    
    SubClassOf: 
        <http://purl.obolibrary.org/obo/BFO_0000003>
    
    
Class: OEO_00030022

    
Class: OEO_00030024

    
Class: OEO_00030025

    
Class: OEO_00030029

    
Class: OEO_00030030

    
Class: OEO_00030031

    
Class: OEO_00030032

    
Class: OEO_00030033

    
Class: OEO_00030034

    
Class: OEO_00030035

    
Class: OEO_00040002

    Annotations: 
        OEO_00040001 "http://openenergy-platform.org/ontology/oeo/oeo-shared",
        <http://purl.obolibrary.org/obo/IAO_0000115> "A role of an organisation, association, or group of persons, whether incorporated or unincorporated, which constitutes, maintains, or provides a facility for bringing together purchasers and sellers of financial instruments, commodities, or other products, services, or goods, and includes the market place and facilities maintained by the exchange",
        <http://purl.obolibrary.org/obo/IAO_0000118> "exchange",
        <http://purl.obolibrary.org/obo/IAO_0000118> "market",
        <http://purl.obolibrary.org/obo/IAO_0000119> "fibo-fbc-fct-mkt:Exchange",
        <http://purl.obolibrary.org/obo/IAO_0000233> "https://github.com/OpenEnergyPlatform/ontology/issues/341
https://github.com/OpenEnergyPlatform/ontology/pull/639

https://github.com/OpenEnergyPlatform/ontology/issues/677
https://github.com/OpenEnergyPlatform/ontology/pull/740

change label to market exchange role
https://github.com/OpenEnergyPlatform/ontology/pull/748

Move to oeo-shared:
issue: https://github.com/OpenEnergyPlatform/ontology/issues/1458
pull request: https://github.com/OpenEnergyPlatform/ontology/pull/1478",
        rdfs:label "market exchange role"@en,
        rdfs:seeAlso "https://spec.edmcouncil.org/fibo/ontology/FBC/FunctionalEntities/Markets/Exchange"
    
    SubClassOf: 
        <http://purl.obolibrary.org/obo/BFO_0000023>
    
    
Class: OEO_00040003

    Annotations: 
        OEO_00040001 "http://openenergy-platform.org/ontology/oeo/oeo-shared",
        <http://purl.obolibrary.org/obo/IAO_0000115> "A monetary price is an economic value that describes the amount of money requested, expected, required or given in exchange for something else.",
        <http://purl.obolibrary.org/obo/IAO_0000119> "fibo-fnd-acc-cur:MonetaryPrice",
        <http://purl.obolibrary.org/obo/IAO_0000233> "issue: https://github.com/OpenEnergyPlatform/ontology/issues/331
pull request: https://github.com/OpenEnergyPlatform/ontology/pull/640
move to oeo-shared
pull request: https://github.com/OpenEnergyPlatform/ontology/pull/956
add relation to good
pull request: https://github.com/OpenEnergyPlatform/ontology/pull/1034",
        rdfs:label "monetary price"@en,
        rdfs:seeAlso "https://spec.edmcouncil.org/fibo/ontology/FND/Accounting/CurrencyAmount/MonetaryPrice"
    
    SubClassOf: 
        OEO_00140012,
        OEO_00020179 some OEO_00010117,
        OEO_00040010 some OEO_00040004
    
    
Class: OEO_00040004

    Annotations: 
        OEO_00040001 "http://openenergy-platform.org/ontology/oeo/oeo-shared",
        <http://purl.obolibrary.org/obo/IAO_0000112> "The currency used in France in 2020 was Euro.",
        <http://purl.obolibrary.org/obo/IAO_0000115> "A unit which is a measure of the medium of an exchange value, defined by reference to the geographical location of the monetary authorities responsible for it.",
        <http://purl.obolibrary.org/obo/IAO_0000119> "fibo-fnd-acc-cur:Currency",
        <http://purl.obolibrary.org/obo/IAO_0000233> "https://github.com/OpenEnergyPlatform/ontology/issues/331
https://github.com/OpenEnergyPlatform/ontology/pull/640
add comment and example
https://github.com/OpenEnergyPlatform/ontology/pull/910
moved to oeo-shared
https://github.com/OpenEnergyPlatform/ontology/pull/956",
        rdfs:comment "Currency is the unit of monetary value as defined by each country.",
        rdfs:label "currency"@en,
        rdfs:seeAlso "https://spec.edmcouncil.org/fibo/ontology/FND/Accounting/CurrencyAmount/Currency"
    
    SubClassOf: 
        <http://purl.obolibrary.org/obo/UO_0000000>
    
    
Class: OEO_00040009

    Annotations: 
        OEO_00040001 "http://openenergy-platform.org/ontology/oeo/oeo-shared",
        <http://purl.obolibrary.org/obo/IAO_0000115> "Cost is an economic value that describes the amount of money needed to buy, make, or do a thing.",
        <http://purl.obolibrary.org/obo/IAO_0000119> "https://dictionary.cambridge.org/dictionary/english/cost",
        <http://purl.obolibrary.org/obo/IAO_0000233> "issue: https://github.com/OpenEnergyPlatform/ontology/issues/268
pull request: https://github.com/OpenEnergyPlatform/ontology/pull/643
move to oeo-shared
pull request: https://github.com/OpenEnergyPlatform/ontology/pull/956
delete cost in oeo-social
issue: https://github.com/OpenEnergyPlatform/ontology/issues/975
pull request: https://github.com/OpenEnergyPlatform/ontology/pull/977",
        rdfs:label "cost"@en
    
    SubClassOf: 
        OEO_00140012,
        OEO_00040010 some OEO_00040004
    
    
Class: OEO_00040011

    Annotations: 
        OEO_00040001 "http://openenergy-platform.org/ontology/oeo/oeo-shared",
        <http://purl.obolibrary.org/obo/IAO_0000115> "A commodity role is a good role that inheres in something that is used in commerce and is exchangeable with other commodities of the same type.",
        <http://purl.obolibrary.org/obo/IAO_0000119> "fibo-fnd-pas-pas:Commodity",
        <http://purl.obolibrary.org/obo/IAO_0000233> "https://github.com/OpenEnergyPlatform/ontology/issues/339
https://github.com/OpenEnergyPlatform/ontology/pull/644
moved to oeo-shared and renamed
https://github.com/OpenEnergyPlatform/ontology/pull/748
made subclass of good role
pull request: https://github.com/OpenEnergyPlatform/ontology/pull/843",
        rdfs:label "commodity role"@en,
        rdfs:seeAlso "https://spec.edmcouncil.org/fibo/ontology/FND/ProductsAndServices/ProductsAndServices/Commodity"
    
    SubClassOf: 
        OEO_00010117
    
    
Class: OEO_00050018

    
Class: OEO_00050019

    Annotations: 
        OEO_00040001 "http://openenergy-platform.org/ontology/oeo/oeo-shared",
        <http://purl.obolibrary.org/obo/IAO_0000115> "An energy amount value is a quantity value that has an energy unit as unit."@en,
        <http://purl.obolibrary.org/obo/IAO_0000118> "energy quantity value",
        <http://purl.obolibrary.org/obo/IAO_0000233> "issue: https://github.com/OpenEnergyPlatform/ontology/issues/576
pull request: https://github.com/OpenEnergyPlatform/ontology/pull/613
moved to oeo-shared
issue: https://github.com/OpenEnergyPlatform/ontology/issues/998
pull request: https://github.com/OpenEnergyPlatform/ontology/pull/1221",
        rdfs:label "energy amount value"@en
    
    SubClassOf: 
        OEO_00000350,
        OEO_00040010 some <http://purl.obolibrary.org/obo/UO_0000111>
    
    
Class: OEO_00090001

    Annotations: 
        OEO_00040001 "http://openenergy-platform.org/ontology/oeo/oeo-shared",
        <http://purl.obolibrary.org/obo/IAO_0000115> "A funder is a sponsor that supports by giving money.",
        <http://purl.obolibrary.org/obo/IAO_0000233> "issue: https://github.com/OpenEnergyPlatform/ontology/issues/246
pull request: https://github.com/OpenEnergyPlatform/ontology/pull/776",
        rdfs:label "funder"@en
    
    SubClassOf: 
        OEO_00140009
    
    
Class: OEO_00140003

    Annotations: 
        OEO_00040001 "http://openenergy-platform.org/ontology/oeo/oeo-shared",
        <http://purl.obolibrary.org/obo/IAO_0000115> "Transport is the process of moving people or goods from one place to another.",
        <http://purl.obolibrary.org/obo/IAO_0000233> "issue: https://github.com/OpenEnergyPlatform/ontology/issues/503
pull request: https://github.com/OpenEnergyPlatform/ontology/pull/517

add performance axiom
issue: https://github.com/OpenEnergyPlatform/ontology/issues/1272
pull-request: https://github.com/OpenEnergyPlatform/ontology/pull/1289

add has participant axiom
issue: https://github.com/OpenEnergyPlatform/ontology/issues/1271
pull request: https://github.com/OpenEnergyPlatform/ontology/pull/1309",
        
            Annotations: <http://purl.obolibrary.org/obo/IAO_0000233> "issue: https://github.com/OpenEnergyPlatform/ontology/issues/636
pull request: https://github.com/OpenEnergyPlatform/ontology/pull/810"
        <http://purl.obolibrary.org/obo/IAO_0006011> "http://purl.obolibrary.org/obo/ENVO_02000125",
        rdfs:label "transport"@en
    
    SubClassOf: 
        <http://purl.obolibrary.org/obo/BFO_0000015>,
        OEO_00140002 some OEO_00320000,
        <http://purl.obolibrary.org/obo/RO_0000057> some 
            (OEO_00000323 or OEO_00010116)
    
    
Class: OEO_00140004

    Annotations: 
        OEO_00040001 "http://openenergy-platform.org/ontology/oeo/oeo-shared",
        <http://purl.obolibrary.org/obo/IAO_0000115> "International transport is a transport process between different countries or within the same country via another country.",
        <http://purl.obolibrary.org/obo/IAO_0000233> "issue: https://github.com/OpenEnergyPlatform/ontology/issues/503
pull request: https://github.com/OpenEnergyPlatform/ontology/pull/517",
        rdfs:label "international transport"@en
    
    SubClassOf: 
        OEO_00140003
    
    
Class: OEO_00140005

    Annotations: 
        OEO_00040001 "http://openenergy-platform.org/ontology/oeo/oeo-shared",
        <http://purl.obolibrary.org/obo/IAO_0000115> "Freight transport is a transport process which moves goods from one place to another.",
        <http://purl.obolibrary.org/obo/IAO_0000233> "issue: https://github.com/OpenEnergyPlatform/ontology/issues/503
pull request: https://github.com/OpenEnergyPlatform/ontology/pull/517

Add axiom for goods as participant:
issue: https://github.com/OpenEnergyPlatform/ontology/issues/1269
pull request: https://github.com/OpenEnergyPlatform/ontology/pull/1299",
        rdfs:label "freight transport"@en
    
    SubClassOf: 
        OEO_00140003,
        <http://purl.obolibrary.org/obo/RO_0000057> some OEO_00010116
    
    
Class: OEO_00140006

    Annotations: 
        OEO_00040001 "http://openenergy-platform.org/ontology/oeo/oeo-shared",
        <http://purl.obolibrary.org/obo/IAO_0000115> "A private transport is a passenger transport in which people use their own vehicle for movement e.g. bicycle, motorcycle and cars.",
        <http://purl.obolibrary.org/obo/IAO_0000233> "issue: https://github.com/OpenEnergyPlatform/ontology/issues/503
pull request: https://github.com/OpenEnergyPlatform/ontology/pull/517

Make subclass of 'passenger transport'
issue: https://github.com/OpenEnergyPlatform/ontology/issues/1055
pull request: https://github.com/OpenEnergyPlatform/ontology/pull/1234",
        rdfs:label "private transport"
    
    SubClassOf: 
        OEO_00010263
    
    
Class: OEO_00140007

    Annotations: 
        OEO_00040001 "http://openenergy-platform.org/ontology/oeo/oeo-shared",
        <http://purl.obolibrary.org/obo/IAO_0000115> "A public transport is a passenger transport in which a number of passengers share a common vehicle.",
        <http://purl.obolibrary.org/obo/IAO_0000233> "issue: https://github.com/OpenEnergyPlatform/ontology/issues/503
pull request: https://github.com/OpenEnergyPlatform/ontology/pull/517

Make subclass of 'passenger transport'
issue: https://github.com/OpenEnergyPlatform/ontology/issues/1055
pull request: https://github.com/OpenEnergyPlatform/ontology/pull/1234",
        rdfs:label "public transport"
    
    SubClassOf: 
        OEO_00010263
    
    
Class: OEO_00140009

    
Class: OEO_00140012

    Annotations: 
        OEO_00040001 "http://openenergy-platform.org/ontology/oeo/oeo-shared",
        <http://purl.obolibrary.org/obo/IAO_0000115> "An economic value is a quantity value that is economically relevant.",
        <http://purl.obolibrary.org/obo/IAO_0000233> "issue: https://github.com/OpenEnergyPlatform/ontology/issues/454
pull request: https://github.com/OpenEnergyPlatform/ontology/pull/559
move to oeo-shared
pull request: https://github.com/OpenEnergyPlatform/ontology/pull/956",
        rdfs:label "economic value"@en
    
    SubClassOf: 
        OEO_00000350
    
    
Class: OEO_00140033

    Annotations: 
        OEO_00040001 "http://openenergy-platform.org/ontology/oeo/oeo-shared",
        <http://purl.obolibrary.org/obo/IAO_0000115> "A chemical reaction is a transformation that involves the interconversion of chemical species.",
        <http://purl.obolibrary.org/obo/IAO_0000233> "issue: https://github.com/OpenEnergyPlatform/ontology/issues/449
pull request: https://github.com/OpenEnergyPlatform/ontology/pull/568

move to oeo-shared:
issue: https://github.com/OpenEnergyPlatform/ontology/issues/1384
pull request: https://github.com/OpenEnergyPlatform/ontology/pull/1390

add 'has participant axiom':
issue: https://github.com/OpenEnergyPlatform/ontology/issues/1327
pull request: https://github.com/OpenEnergyPlatform/ontology/pull/1395",
        rdfs:label "chemical reaction"@en
    
    SubClassOf: 
        OEO_00000419,
        <http://purl.obolibrary.org/obo/RO_0000057> some <http://purl.obolibrary.org/obo/BFO_0000040>
    
    
Class: OEO_00140039

    Annotations: 
        OEO_00040001 "http://openenergy-platform.org/ontology/oeo/oeo-shared",
        <http://purl.obolibrary.org/obo/IAO_0000115> "Consumption is the process of using something and thereby reducing its amount.",
        <http://purl.obolibrary.org/obo/IAO_0000233> "issue: https://github.com/OpenEnergyPlatform/ontology/issues/140
pull request: https://github.com/OpenEnergyPlatform/ontology/pull/569",
        rdfs:label "consumption"@en
    
    SubClassOf: 
        <http://purl.obolibrary.org/obo/BFO_0000015>
    
    
Class: OEO_00140040

    Annotations: 
        OEO_00040001 "http://openenergy-platform.org/ontology/oeo/oeo-shared",
        <http://purl.obolibrary.org/obo/IAO_0000115> "A demand is a realizable entity that is characterised by a person, organisation or object needing it for a specific purpose.",
        <http://purl.obolibrary.org/obo/IAO_0000233> "issue: https://github.com/OpenEnergyPlatform/ontology/issues/140
pull request: https://github.com/OpenEnergyPlatform/ontology/pull/569

add 'has bearer' axiom
issue: https://github.com/OpenEnergyPlatform/ontology/issues/1305
pull request: https://github.com/OpenEnergyPlatform/ontology/pull/1310
pull request: https://github.com/OpenEnergyPlatform/ontology/pull/1485",
        rdfs:label "demand"@en
    
    SubClassOf: 
        <http://purl.obolibrary.org/obo/BFO_0000017>,
        OEO_00010121 some 
            (OEO_00030022 or <http://purl.obolibrary.org/obo/BFO_0000030>)
    
    
Class: OEO_00140043

    
Class: OEO_00140044

    
Class: OEO_00140049

    Annotations: 
        OEO_00040001 "http://openenergy-platform.org/ontology/oeo/oeo-shared",
        <http://purl.obolibrary.org/obo/IAO_0000115> "Energy conversion efficiency is a process attribute describing the ratio between the input of an energy transformation and the outputs that are used.",
        <http://purl.obolibrary.org/obo/IAO_0000233> "issue: https://github.com/OpenEnergyPlatform/ontology/issues/434
pull request: https://github.com/OpenEnergyPlatform/ontology/pull/591

moved to oeo-shared:
issue: https://github.com/OpenEnergyPlatform/ontology/issues/1543
pull request: https://github.com/OpenEnergyPlatform/ontology/pull/1625",
        rdfs:label "energy conversion efficiency"@en
    
    SubClassOf: 
        OEO_00030019,
        OEO_00000502 some OEO_00020003,
        OEO_00140002 some OEO_00140050
    
    
Class: OEO_00140050

    Annotations: 
        OEO_00040001 "http://openenergy-platform.org/ontology/oeo/oeo-physical",
        <http://purl.obolibrary.org/obo/IAO_0000115> "An efficiency value is a quantity value stating the ratio between a process's inputs and the outputs that are used.",
        
            Annotations: <http://purl.obolibrary.org/obo/IAO_0000233> "issue: https://github.com/OpenEnergyPlatform/ontology/issues/256
pull request: https://github.com/OpenEnergyPlatform/ontology/pull/779"
        <http://purl.obolibrary.org/obo/IAO_0000118> "efficiency",
        <http://purl.obolibrary.org/obo/IAO_0000233> "issue: https://github.com/OpenEnergyPlatform/ontology/issues/434
pull request: https://github.com/OpenEnergyPlatform/ontology/pull/591

moved to oeo-shared:
issue: https://github.com/OpenEnergyPlatform/ontology/issues/1543
pull request: https://github.com/OpenEnergyPlatform/ontology/pull/1625",
        rdfs:label "efficiency value"@en
    
    SubClassOf: 
        OEO_00000350,
        OEO_00040010 some <http://purl.obolibrary.org/obo/UO_0010006>
    
    
Class: OEO_00140075

    Annotations: 
        OEO_00040001 "http://openenergy-platform.org/ontology/oeo/oeo-shared",
        <http://purl.obolibrary.org/obo/IAO_0000112> "coals, cruide oil, natural gas, wood or moving air (wind) have the disposition of being primary energy carriers",
        <http://purl.obolibrary.org/obo/IAO_0000115> "Primary energy carrier disposition is an energy carrier disposition of material entities that are extracted directly from natural resources or that are natural energy flows.",
        <http://purl.obolibrary.org/obo/IAO_0000233> "issue: https://github.com/OpenEnergyPlatform/ontology/issues/575
pull request: https://github.com/OpenEnergyPlatform/ontology/pull/633

move to oeo-shared:
issue: https://github.com/OpenEnergyPlatform/ontology/issues/1384
pull request: https://github.com/OpenEnergyPlatform/ontology/pull/1390",
        rdfs:label "primary energy carrier disposition"@en
    
    SubClassOf: 
        OEO_00000151
    
    
Class: OEO_00140076

    Annotations: 
        OEO_00040001 "http://openenergy-platform.org/ontology/oeo/oeo-physical",
        <http://purl.obolibrary.org/obo/IAO_0000112> "blast furnace gas, coke oven gas, cokes, motor gasoline or electricity have the disposition to be a secondary energy carrier",
        <http://purl.obolibrary.org/obo/IAO_0000115> "Secondary energy carrier disposition is an energy carrier disposition of material entities that are manufactured from primary energy carriers or from a different form of secondary energy carriers.",
        <http://purl.obolibrary.org/obo/IAO_0000233> "issue: https://github.com/OpenEnergyPlatform/ontology/issues/575
pull request: https://github.com/OpenEnergyPlatform/ontology/pull/633

Move to oeo-shared:
issue: https://github.com/OpenEnergyPlatform/ontology/issues/1522
pull request: https://github.com/OpenEnergyPlatform/ontology/pull/1531",
        rdfs:label "secondary energy carrier disposition"@en
    
    SubClassOf: 
        OEO_00000151
    
    
Class: OEO_00140079

    Annotations: 
        OEO_00040001 "http://openenergy-platform.org/ontology/oeo/oeo-physical",
        <http://purl.obolibrary.org/obo/IAO_0000115> "A secondary energy carrier is an energy carrier that has the secondary energy carrier disposition.",
        <http://purl.obolibrary.org/obo/IAO_0000233> "issue: https://github.com/OpenEnergyPlatform/ontology/issues/575
pull request: https://github.com/OpenEnergyPlatform/ontology/pull/633
fix error in definition
issue: https://github.com/OpenEnergyPlatform/ontology/issues/669
pull request: https://github.com/OpenEnergyPlatform/ontology/pull/678

Move to oeo-shared:
issue: https://github.com/OpenEnergyPlatform/ontology/issues/1522
pull request: https://github.com/OpenEnergyPlatform/ontology/pull/1531",
        rdfs:label "secondary energy carrier"@en
    
    EquivalentTo: 
        <http://purl.obolibrary.org/obo/BFO_0000040>
         and (<http://purl.obolibrary.org/obo/RO_0000091> some OEO_00140076)
    
    SubClassOf: 
        OEO_00020039
    
    
Class: OEO_00140081

    
Class: OEO_00140124

    Annotations: 
        OEO_00040001 "http://openenergy-platform.org/ontology/oeo/oeo-social",
        <http://purl.obolibrary.org/obo/IAO_0000115> "A service is a process that is an intangible activity performed by some agent for the benefit of another agent.",
        <http://purl.obolibrary.org/obo/IAO_0000119> "https://spec.edmcouncil.org/fibo/ontology/FND/ProductsAndServices/ProductsAndServices/Service (adapted)",
        <http://purl.obolibrary.org/obo/IAO_0000233> "issue: https://github.com/OpenEnergyPlatform/ontology/issues/376
pull request: https://github.com/OpenEnergyPlatform/ontology/pull/778

add 'has participant axiom' and move to oeo-shared:
issue: https://github.com/OpenEnergyPlatform/ontology/issues/1327
pull request: https://github.com/OpenEnergyPlatform/ontology/pull/1395",
        rdfs:label "service"@en
    
    SubClassOf: 
        <http://purl.obolibrary.org/obo/BFO_0000015>,
        <http://purl.obolibrary.org/obo/RO_0000057> some OEO_00000051
    
    
Class: OEO_00140149

    Annotations: 
        OEO_00040001 "http://openenergy-platform.org/ontology/oeo/oeo-shared",
        <http://purl.obolibrary.org/obo/IAO_0000115> "A transformative measure is a process that is an activity that has a direct impact on a specific variable in question.",
        <http://purl.obolibrary.org/obo/IAO_0000118> "policies and measures",
        <http://purl.obolibrary.org/obo/IAO_0000233> "issue: https://github.com/OpenEnergyPlatform/ontology/issues/444
pull request: https://github.com/OpenEnergyPlatform/ontology/pull/797

move to oeo-shared, alternative label
issue: https://github.com/OpenEnergyPlatform/ontology/issues/1329
pull request: https://github.com/OpenEnergyPlatform/ontology/pull/1614",
        rdfs:label "transformative measure"@en
    
    SubClassOf: 
        <http://purl.obolibrary.org/obo/BFO_0000015>
    
    
Class: OEO_00140151

    Annotations: 
        OEO_00040001 "http://openenergy-platform.org/ontology/oeo/oeo-shared",
        <http://purl.obolibrary.org/obo/IAO_0000115> "A policy instrument is a plan specification of an organisation (e.g. a government) that promotes transformative measures.",
        <http://purl.obolibrary.org/obo/IAO_0000118> "policies and measures",
        <http://purl.obolibrary.org/obo/IAO_0000233> "issue: https://github.com/OpenEnergyPlatform/ontology/issues/444
pull request: https://github.com/OpenEnergyPlatform/ontology/pull/797

Redefine as 'plan specification' and add axiom:
issue: https://github.com/OpenEnergyPlatform/ontology/issues/1507
pull request: https://github.com/OpenEnergyPlatform/ontology/pull/1563

move to oeo-shared, alternative label
issue: https://github.com/OpenEnergyPlatform/ontology/issues/1329
pull request: https://github.com/OpenEnergyPlatform/ontology/pull/1614",
        rdfs:label "policy instrument"@en
    
    SubClassOf: 
        <http://purl.obolibrary.org/obo/IAO_0000104>,
        
            Annotations: <http://purl.obolibrary.org/obo/IAO_0000233> "issue: https://github.com/OpenEnergyPlatform/ontology/issues/444
pull request: https://github.com/OpenEnergyPlatform/ontology/pull/853"
        OEO_00010119 some OEO_00140149,
        <http://purl.obolibrary.org/obo/IAO_0000136> some OEO_00030022
    
    
Class: OEO_00140159

    
Class: OEO_00240003

    
Class: OEO_00240014

    
Class: OEO_00240019

    
Class: OEO_00240022

    
Class: OEO_00240024

    
Class: OEO_00240038

    
Class: OEO_00260007

    
Class: OEO_00320000

    
Class: OEO_00320001

    
Class: OEO_00320002

    
Class: OEO_00320003

    
Class: OEO_00320041

    
Class: OEO_00320061

    
Class: OEO_00320073

    Annotations: 
        <http://purl.obolibrary.org/obo/IAO_0000115> "An amortisation time is the time span in which the investment costs are refinanced from the annual profits and depreciation of the investment.",
        <http://purl.obolibrary.org/obo/IAO_0000233> "issue: https://github.com/OpenEnergyPlatform/ontology/issues/1380
pull request: https://github.com/OpenEnergyPlatform/ontology/pull/1436",
        rdfs:label "amortisation time"
    
    SubClassOf: 
        OEO_00030035
    
    
Class: OEO_00320074

    Annotations: 
        <http://purl.obolibrary.org/obo/IAO_0000115> "An economic life time is the operational life time during which an artificial object is profitable to the owner.",
        <http://purl.obolibrary.org/obo/IAO_0000233> "issue: https://github.com/OpenEnergyPlatform/ontology/issues/1380
pull request: https://github.com/OpenEnergyPlatform/ontology/pull/1436",
        rdfs:label "economic life time"
    
    SubClassOf: 
        OEO_00020178
    
    
Class: OEO_00340004

    
Class: OEO_00340005

    
Individual: OEO_00000182

    
Individual: OEO_00000256

    
Individual: OEO_00020161

    
Individual: OEO_00020162

    
Individual: OEO_00020163

    
Individual: OEO_00020164

    
Individual: OEO_00020165

    
