Prefix: : <http://openenergy-platform.org/ontology/oeo/>
Prefix: dc: <http://purl.org/dc/elements/1.1/>
Prefix: owl: <http://www.w3.org/2002/07/owl#>
Prefix: rdf: <http://www.w3.org/1999/02/22-rdf-syntax-ns#>
Prefix: rdfs: <http://www.w3.org/2000/01/rdf-schema#>
Prefix: xml: <http://www.w3.org/XML/1998/namespace>
Prefix: xsd: <http://www.w3.org/2001/XMLSchema#>



Ontology: <http://openenergy-platform.org/ontology/oeo/oeo-shared/>
<http://openenergy-platform.org/ontology/oeo/dev/oeo-shared.omn>
Import: <http://openenergy-platform.org/ontology/oeo/dev/imports/iao-module.owl>
Import: <http://openenergy-platform.org/ontology/oeo/dev/imports/ro-module.owl>
Import: <http://openenergy-platform.org/ontology/oeo/dev/imports/uo-module.owl>
Import: <http://purl.obolibrary.org/obo/omo.owl>
Import: <https://raw.githubusercontent.com/BFO-ontology/BFO/v2.0/bfo.owl>

Annotations: 
    dc:description "The Open Energy Ontology is an ontology for all aspects of the energy modelling domain. The \"Shared\" module covers all entities that are relevant for all our other modules. This includes shared imports like the BFO, IAO- and RO- module.",
    <http://purl.org/dc/terms/license> "http://creativecommons.org/publicdomain/zero/1.0/",
    <http://purl.org/dc/terms/title> "Open Energy Ontology (Shared module)"

AnnotationProperty: <http://purl.obolibrary.org/obo/IAO_0000112>

    
AnnotationProperty: <http://purl.obolibrary.org/obo/IAO_0000115>

    
AnnotationProperty: <http://purl.obolibrary.org/obo/IAO_0000116>

    
AnnotationProperty: <http://purl.obolibrary.org/obo/IAO_0000118>

    Annotations: 
        rdfs:comment "In the OEO, we don't follow the definition strictly. We use alternative term for synonyms and ambiguous terms as well. See https://github.com/OpenEnergyPlatform/ontology/wiki/Handling-ambiguous-terms"
    
    
AnnotationProperty: <http://purl.obolibrary.org/obo/IAO_0000119>

    
AnnotationProperty: <http://purl.obolibrary.org/obo/IAO_0000233>

    
AnnotationProperty: <http://purl.org/dc/terms/license>

    
AnnotationProperty: <http://purl.org/dc/terms/title>

    
AnnotationProperty: <http://www.geneontology.org/formats/oboInOwl#hasExactSynonym>

    
AnnotationProperty: OEO_00010037

    Annotations: 
        <http://purl.obolibrary.org/obo/IAO_0000115> "A unique individual identifier is an identifier that is unique for one individual of a class. Unique individual identifiers follow usually a structure defined e.g. by a sector division.",
        <http://purl.obolibrary.org/obo/IAO_0000233> "issue: https://github.com/OpenEnergyPlatform/ontology/issues/461
pull request: https://github.com/OpenEnergyPlatform/ontology/pull/523",
        rdfs:label "unique individual identifier"
    
    SubPropertyOf: 
        dc:identifier
    
    
AnnotationProperty: OEO_00040001

    Annotations: 
        rdfs:label "belongs to module"
    
    
AnnotationProperty: OEO_00110012

    Annotations: 
        <http://purl.obolibrary.org/obo/IAO_0000115> "A mathematical expression is an annotation property that describes the class with a mathematical formula in LaTeX syntax."@en,
        <http://purl.obolibrary.org/obo/IAO_0000233> "issue: https://github.com/OpenEnergyPlatform/ontology/issues/987
pull request: https://github.com/OpenEnergyPlatform/ontology/pull/990"@en,
        rdfs:label "mathematical expression"@en
    
    
AnnotationProperty: dc:description

    
AnnotationProperty: dc:identifier

    
AnnotationProperty: owl:equivalentClass

    
AnnotationProperty: rdfs:comment

    
AnnotationProperty: rdfs:label

    
AnnotationProperty: rdfs:seeAlso

    
Datatype: rdf:PlainLiteral

    
Datatype: xsd:string

    
ObjectProperty: <http://purl.obolibrary.org/obo/BFO_0000050>

    Annotations: 
        <http://purl.obolibrary.org/obo/IAO_0000233> "issue https://github.com/OpenEnergyPlatform/ontology/issues/596
Pull request https://github.com/OpenEnergyPlatform/ontology/pull/599
Pull request https://github.com/OpenEnergyPlatform/ontology/pull/603"
    
    Characteristics: 
        Transitive
    
    
ObjectProperty: <http://purl.obolibrary.org/obo/BFO_0000051>

    Annotations: 
        <http://purl.obolibrary.org/obo/IAO_0000233> "issue https://github.com/OpenEnergyPlatform/ontology/issues/596
Pull request https://github.com/OpenEnergyPlatform/ontology/pull/599
Pull request https://github.com/OpenEnergyPlatform/ontology/pull/603

fix duplicate implementation of `Inverse Of`
issue https://github.com/OpenEnergyPlatform/ontology/issues/979
pull request https://github.com/OpenEnergyPlatform/ontology/pull/1086"
    
    Characteristics: 
        Transitive
    
    
ObjectProperty: <http://purl.obolibrary.org/obo/BFO_0000054>

    
ObjectProperty: <http://purl.obolibrary.org/obo/IAO_0000136>

    InverseOf: 
        OEO_00010231
    
    
ObjectProperty: <http://purl.obolibrary.org/obo/RO_0000053>

    Annotations: 
        <http://purl.obolibrary.org/obo/IAO_0000118> "has characteristic"
    
    Domain: 
        
            Annotations: <http://purl.obolibrary.org/obo/IAO_0000233> "issue: https://github.com/OpenEnergyPlatform/ontology/issues/973
pull request: https://github.com/OpenEnergyPlatform/ontology/pull/985"
        OEO_00000150 or <http://purl.obolibrary.org/obo/BFO_0000004>
    
    Range: 
        <http://purl.obolibrary.org/obo/BFO_0000020>
    
    InverseOf: 
        OEO_00010121
    
    
ObjectProperty: <http://purl.obolibrary.org/obo/RO_0000056>

    Domain: 
        <http://purl.obolibrary.org/obo/BFO_0000002>
    
    Range: 
        <http://purl.obolibrary.org/obo/BFO_0000003>
    
    
ObjectProperty: <http://purl.obolibrary.org/obo/RO_0000057>

    Domain: 
        <http://purl.obolibrary.org/obo/BFO_0000003>
    
    
ObjectProperty: <http://purl.obolibrary.org/obo/RO_0000085>

    Domain: 
        <http://purl.obolibrary.org/obo/BFO_0000004>
    
    Range: 
        <http://purl.obolibrary.org/obo/BFO_0000034>
    
    
ObjectProperty: <http://purl.obolibrary.org/obo/RO_0000086>

    Domain: 
        <http://purl.obolibrary.org/obo/BFO_0000002>
    
    
ObjectProperty: <http://purl.obolibrary.org/obo/RO_0000087>

    Annotations: 
        <http://purl.obolibrary.org/obo/IAO_0000116> "In contrast to the original RO class, the domain was extended to independent continuant or energy. This is due to the special role that energy plays for the OEO and the difficulty of classifying it properly.",
        <http://purl.obolibrary.org/obo/IAO_0000233> "extend domain / definition
issue: https://github.com/OpenEnergyPlatform/ontology/issues/1030
pull request: https://github.com/OpenEnergyPlatform/ontology/pull/1101"
    
    Domain: 
        OEO_00000150 or <http://purl.obolibrary.org/obo/BFO_0000004>
    
    Range: 
        <http://purl.obolibrary.org/obo/BFO_0000023>
    
    
ObjectProperty: <http://purl.obolibrary.org/obo/RO_0000091>

    Domain: 
        <http://purl.obolibrary.org/obo/BFO_0000004>
    
    Range: 
        <http://purl.obolibrary.org/obo/BFO_0000016>
    
    
ObjectProperty: <http://purl.obolibrary.org/obo/RO_0001025>

    Domain: 
        <http://purl.obolibrary.org/obo/BFO_0000004>
    
    Range: 
        <http://purl.obolibrary.org/obo/BFO_0000004>
    
    
ObjectProperty: <http://purl.obolibrary.org/obo/RO_0002222>

    Domain: 
        <http://purl.obolibrary.org/obo/BFO_0000003>
    
    Range: 
        <http://purl.obolibrary.org/obo/BFO_0000003>
    
    
ObjectProperty: <http://purl.obolibrary.org/obo/RO_0002233>

    Domain: 
        <http://purl.obolibrary.org/obo/BFO_0000015>
    
    
ObjectProperty: <http://purl.obolibrary.org/obo/RO_0002234>

    
ObjectProperty: <http://purl.obolibrary.org/obo/RO_0002328>

    
ObjectProperty: <http://purl.obolibrary.org/obo/RO_0002352>

    
ObjectProperty: <http://purl.obolibrary.org/obo/RO_0002353>

    
ObjectProperty: <http://purl.obolibrary.org/obo/RO_0002410>

    Domain: 
        
            Annotations: <http://purl.obolibrary.org/obo/IAO_0000233> "add domain and range
issue: https://github.com/OpenEnergyPlatform/ontology/issues/1079
pull-request: https://github.com/OpenEnergyPlatform/ontology/pull/1136"
        <http://purl.obolibrary.org/obo/BFO_0000015> or <http://purl.obolibrary.org/obo/BFO_0000040>
    
    Range: 
        
            Annotations: <http://purl.obolibrary.org/obo/IAO_0000233> "add domain and range
issue: https://github.com/OpenEnergyPlatform/ontology/issues/1079
pull-request: https://github.com/OpenEnergyPlatform/ontology/pull/1136"
        <http://purl.obolibrary.org/obo/BFO_0000015> or <http://purl.obolibrary.org/obo/BFO_0000040>
    
    
ObjectProperty: <http://purl.obolibrary.org/obo/RO_0002501>

    Domain: 
        
            Annotations: <http://purl.obolibrary.org/obo/IAO_0000233> "add domain and range
issue: https://github.com/OpenEnergyPlatform/ontology/issues/1079
pull-request: https://github.com/OpenEnergyPlatform/ontology/pull/1136"
        <http://purl.obolibrary.org/obo/BFO_0000015>
    
    Range: 
        
            Annotations: <http://purl.obolibrary.org/obo/IAO_0000233> "add domain and range
issue: https://github.com/OpenEnergyPlatform/ontology/issues/1079
pull-request: https://github.com/OpenEnergyPlatform/ontology/pull/1136"
        <http://purl.obolibrary.org/obo/BFO_0000015>
    
    
ObjectProperty: <http://purl.obolibrary.org/obo/RO_0003000>

    Annotations: 
        
            Annotations: <http://purl.obolibrary.org/obo/IAO_0000233> "issue: https://github.com/OpenEnergyPlatform/ontology/issues/994
pull request: https://github.com/OpenEnergyPlatform/ontology/pull/1006"
        <http://purl.obolibrary.org/obo/IAO_0000116> "As produces relates to an material entity, but energy is a quality in the OEO, produces cannot be used to describe the energy output of a process. Use 'has energy output' instead."
    
    
ObjectProperty: <http://purl.obolibrary.org/obo/uo#is_unit_of>

    Annotations: 
        <http://purl.obolibrary.org/obo/IAO_0000115> "A relation to connect a unit to a quantifiable entity that it is the unit of.",
        rdfs:comment "This relation has been imported from UO.",
        rdfs:label "is unit of"
    
    Domain: 
        <http://purl.obolibrary.org/obo/UO_0000000>
    
    
ObjectProperty: OEO_00000500

    Annotations: 
        <http://purl.obolibrary.org/obo/IAO_0000233> "A relation between a process and a process attribute that existentially depends on it.",
        <http://purl.obolibrary.org/obo/IAO_0000233> "issue: https://github.com/OpenEnergyPlatform/ontology/issues/66
pull requests: https://github.com/OpenEnergyPlatform/ontology/pull/472

issue: https://github.com/OpenEnergyPlatform/ontology/issues/205
pull request: https://github.com/OpenEnergyPlatform/ontology/pull/386

add domain and range; move to oeo-shared
issue: https://github.com/OpenEnergyPlatform/ontology/issues/850
pull request: https://github.com/OpenEnergyPlatform/ontology/pull/871",
        rdfs:label "has process attribute"
    
    Domain: 
        <http://purl.obolibrary.org/obo/BFO_0000015>
    
    Range: 
        OEO_00030019
    
    InverseOf: 
        OEO_00000502
    
    
ObjectProperty: OEO_00000501

    Annotations: 
        rdfs:comment "issue: https://github.com/OpenEnergyPlatform/ontology/issues/66
pull requests: https://github.com/OpenEnergyPlatform/ontology/pull/472",
        rdfs:label "is used by"
    
    InverseOf: 
        OEO_00000503
    
    
ObjectProperty: OEO_00000502

    Annotations: 
        <http://purl.obolibrary.org/obo/IAO_0000233> "A relation between a process attribute and the process it existentially depends on.",
        <http://purl.obolibrary.org/obo/IAO_0000233> "issue: https://github.com/OpenEnergyPlatform/ontology/issues/66
pull requests: https://github.com/OpenEnergyPlatform/ontology/pull/472

issue: https://github.com/OpenEnergyPlatform/ontology/issues/205
pull request: https://github.com/OpenEnergyPlatform/ontology/pull/386

add domains and ranges:
issue: https://github.com/OpenEnergyPlatform/ontology/issues/973
issue: https://github.com/OpenEnergyPlatform/ontology/pull/1085",
        rdfs:label "process attribute of"
    
    Domain: 
        OEO_00030019
    
    Range: 
        <http://purl.obolibrary.org/obo/BFO_0000015>
    
    InverseOf: 
        OEO_00000500
    
    
ObjectProperty: OEO_00000503

    Annotations: 
        <http://purl.obolibrary.org/obo/IAO_0000115> "A relation that holds between a continuant and another continuant it requires to function.",
        <http://purl.obolibrary.org/obo/IAO_0000233> "issue: https://github.com/OpenEnergyPlatform/ontology/issues/66
pull requests: https://github.com/OpenEnergyPlatform/ontology/pull/452 (delete unused subclass)
https://github.com/OpenEnergyPlatform/ontology/pull/472 (move to oeo-shared)
https://github.com/OpenEnergyPlatform/ontology/pull/478 (add definition)
https://github.com/OpenEnergyPlatform/ontology/pull/871 (add domain and range)",
        rdfs:label "uses"
    
    Domain: 
        <http://purl.obolibrary.org/obo/BFO_0000002>
    
    Range: 
        <http://purl.obolibrary.org/obo/BFO_0000002>
    
    InverseOf: 
        OEO_00000501
    
    
ObjectProperty: OEO_00000505

    Annotations: 
        <http://purl.obolibrary.org/obo/IAO_0000115> "A relation that holds between a study and the sector it covers."@en,
        <http://purl.obolibrary.org/obo/IAO_0000233> "update definition
issue: https://github.com/OpenEnergyPlatform/ontology/issues/846
pull request: https://github.com/OpenEnergyPlatform/ontology/pull/852",
        rdfs:label "covers sector"
    
    SubPropertyOf: 
        OEO_00000522
    
    Domain: 
        OEO_00020011
    
    Range: 
        OEO_00000367
    
    
ObjectProperty: OEO_00000506

    Annotations: 
        <http://purl.obolibrary.org/obo/IAO_0000115> "A relation that holds between an information content entity / model and its author."@en,
        <http://purl.obolibrary.org/obo/IAO_0000116> "The construct 'has auther' some ('has role' some author) is necessary, because has author has the range has role some author (PR https://github.com/OpenEnergyPlatform/ontology/pull/871). That is an idependent continuant, i.e. a person, that takes over writing a text and as such the role of an author.",
        <http://purl.obolibrary.org/obo/IAO_0000233> "pull request: https://github.com/OpenEnergyPlatform/ontology/pull/626 (extend def for information content entity)
pull request: https://github.com/OpenEnergyPlatform/ontology/pull/871 (domain and range; move to oeo-shared)",
        rdfs:label "has author"
    
    SubPropertyOf: 
        OEO_00140008
    
    Domain: 
        OEO_00000274 or <http://purl.obolibrary.org/obo/IAO_0000030>
    
    Range: 
        <http://purl.obolibrary.org/obo/RO_0000087> some OEO_00000064
    
    
ObjectProperty: OEO_00000507

    Annotations: 
        <http://purl.obolibrary.org/obo/IAO_0000115> "A relation that holds between an information content entity / model and the client that requested its creation."@en,
        <http://purl.obolibrary.org/obo/IAO_0000233> "pull request: https://github.com/OpenEnergyPlatform/ontology/pull/626 (extend def for information content entity)
pull request: https://github.com/OpenEnergyPlatform/ontology/pull/871 (domain and range; move to oeo-shared)",
        rdfs:label "has client"
    
    SubPropertyOf: 
        OEO_00140008
    
    Domain: 
        OEO_00000274 or <http://purl.obolibrary.org/obo/IAO_0000030>
    
    Range: 
        <http://purl.obolibrary.org/obo/RO_0000087> some OEO_00000087
    
    
ObjectProperty: OEO_00000508

    Annotations: 
        <http://purl.obolibrary.org/obo/IAO_0000115> "A relation that holds between an information content entity / model and the person to contact with issues about it."@en,
        <http://purl.obolibrary.org/obo/IAO_0000233> "pull request: https://github.com/OpenEnergyPlatform/ontology/pull/626 (extend def for information content entity)
pull request: https://github.com/OpenEnergyPlatform/ontology/pull/871 (domain and range; move to oeo-shared)",
        rdfs:label "has contact person"
    
    SubPropertyOf: 
        OEO_00140008
    
    Domain: 
        OEO_00000274 or <http://purl.obolibrary.org/obo/IAO_0000030>
    
    Range: 
        <http://purl.obolibrary.org/obo/RO_0000087> some OEO_00000107
    
    
ObjectProperty: OEO_00000509

    Annotations: 
        <http://purl.obolibrary.org/obo/IAO_0000115> "A relation that holds between an entity and its source of funding."@en,
        <http://purl.obolibrary.org/obo/IAO_0000233> "issue: https://github.com/OpenEnergyPlatform/ontology/issues/530
pull request: https://github.com/OpenEnergyPlatform/ontology/pull/556",
        rdfs:label "has funding source"
    
    SubPropertyOf: 
        owl:topObjectProperty
    
    Range: 
        
            Annotations: rdfs:comment "issue: https://github.com/OpenEnergyPlatform/ontology/issues/850
pull request: https://github.com/OpenEnergyPlatform/ontology/pull/871"
        <http://purl.obolibrary.org/obo/RO_0000087> some OEO_00090001
    
    
ObjectProperty: OEO_00000510

    Annotations: 
        <http://purl.obolibrary.org/obo/IAO_0000115> "A relation that holds between an information content entity or model and the organisation in which it was created."@en,
        <http://purl.obolibrary.org/obo/IAO_0000233> "pull request: https://github.com/OpenEnergyPlatform/ontology/pull/626 (extend def for information content entity)
pull request: https://github.com/OpenEnergyPlatform/ontology/pull/871 (domain and range; move to oeo-shared)

improve definition:
https://github.com/OpenEnergyPlatform/ontology/issues/1038
https://github.com/OpenEnergyPlatform/ontology/pull/1042

Relabel to `has organisation`
issue: https://github.com/OpenEnergyPlatform/ontology/issues/1161
pull request: https://github.com/OpenEnergyPlatform/ontology/pull/1226",
        rdfs:label "has organisation"
    
    SubPropertyOf: 
        OEO_00140008
    
    Domain: 
        OEO_00000274 or <http://purl.obolibrary.org/obo/IAO_0000030>
    
    Range: 
        
            Annotations: <http://purl.obolibrary.org/obo/IAO_0000233> "Replace `institution` as range by `organisation role`
issue: https://github.com/OpenEnergyPlatform/ontology/issues/1161
pull request: https://github.com/OpenEnergyPlatform/ontology/pull/1200"
        <http://purl.obolibrary.org/obo/RO_0000087> some OEO_00000315
    
    
ObjectProperty: OEO_00000514

    Annotations: 
        <http://purl.obolibrary.org/obo/IAO_0000115> "A relation that holds between a data set and the resolution it depicts."@en,
        <http://purl.obolibrary.org/obo/IAO_0000233> "issue https://github.com/OpenEnergyPlatform/ontology/issues/622
Pull request https://github.com/OpenEnergyPlatform/ontology/pull/626
rework
issue https://github.com/OpenEnergyPlatform/ontology/issues/849
Pull request https://github.com/OpenEnergyPlatform/ontology/pull/912
add domain and range
Pull request https://github.com/OpenEnergyPlatform/ontology/pull/972",
        rdfs:label "has resolution"
    
    Domain: 
        <http://purl.obolibrary.org/obo/IAO_0000100>
    
    Range: 
        OEO_00020121
    
    
ObjectProperty: OEO_00000515

    Annotations: 
        <http://purl.obolibrary.org/obo/IAO_0000115> "A relation between a data set and the spatial resolution it uses."@en,
        <http://purl.obolibrary.org/obo/IAO_0000233> "issue https://github.com/OpenEnergyPlatform/ontology/issues/622
Pull request https://github.com/OpenEnergyPlatform/ontology/pull/626
def and axioms
Pull request https://github.com/OpenEnergyPlatform/ontology/pull/912
add domain and range
Pull request https://github.com/OpenEnergyPlatform/ontology/pull/972",
        rdfs:label "has spatial resolution"
    
    SubPropertyOf: 
        OEO_00000514
    
    Domain: 
        <http://purl.obolibrary.org/obo/IAO_0000100>
    
    Range: 
        OEO_00020123
    
    
ObjectProperty: OEO_00000516

    Annotations: 
        <http://purl.obolibrary.org/obo/IAO_0000115> "A relation that holds between data set and the temporal resolution it uses."@en,
        <http://purl.obolibrary.org/obo/IAO_0000233> "issue https://github.com/OpenEnergyPlatform/ontology/issues/622
Pull request https://github.com/OpenEnergyPlatform/ontology/pull/626
def and axioms
Pull request https://github.com/OpenEnergyPlatform/ontology/pull/912
fix def and add domain and range
Pull request https://github.com/OpenEnergyPlatform/ontology/pull/972",
        rdfs:label "has temporal resolution"
    
    SubPropertyOf: 
        OEO_00000514
    
    Domain: 
        <http://purl.obolibrary.org/obo/IAO_0000100>
    
    Range: 
        OEO_00020122
    
    
ObjectProperty: OEO_00000522

    Annotations: 
        <http://purl.obolibrary.org/obo/IAO_0000115> "A relation that holds between a study and the thing it covers.",
        <http://purl.obolibrary.org/obo/IAO_0000233> "issue: https://github.com/OpenEnergyPlatform/ontology/issues/66
pull requests: https://github.com/OpenEnergyPlatform/ontology/pull/452 (delete unused subclasses)
pull requests: https://github.com/OpenEnergyPlatform/ontology/pull/584
pull requests: https://github.com/OpenEnergyPlatform/ontology/pull/626 (extend for study)
issue: https://github.com/OpenEnergyPlatform/ontology/issues/415
pull request: https://github.com/OpenEnergyPlatform/ontology/pull/821 (restrict to study)",
        rdfs:label "covers"
    
    
ObjectProperty: OEO_00000523

    Annotations: 
        <http://purl.obolibrary.org/obo/IAO_0000115> "A relation that holds between a study and the energy carrier it covers.",
        <http://purl.obolibrary.org/obo/IAO_0000233> "change range
issue: https://github.com/OpenEnergyPlatform/ontology/pull/721
pull request: https://github.com/OpenEnergyPlatform/ontology/pull/722

update definition
issue: https://github.com/OpenEnergyPlatform/ontology/issues/846
pull request: https://github.com/OpenEnergyPlatform/ontology/pull/852",
        rdfs:label "covers energy carrier"
    
    SubPropertyOf: 
        OEO_00000522
    
    Domain: 
        OEO_00020011
    
    Range: 
        OEO_00020039
    
    
ObjectProperty: OEO_00000530

    
ObjectProperty: OEO_00010121

    Annotations: 
        <http://purl.obolibrary.org/obo/IAO_0000115> "A relation between a specifically dependent continuant or energy (the dependent) and an independent continuant (the bearer), in which the dependent is specifically reliant on the bearer for its existence",
        <http://purl.obolibrary.org/obo/IAO_0000233> "issue: https://github.com/OpenEnergyPlatform/ontology/issues/444
pull request: issue: https://github.com/OpenEnergyPlatform/ontology/pull/853

add domains and ranges:
issue: https://github.com/OpenEnergyPlatform/ontology/issues/973
pull request: https://github.com/OpenEnergyPlatform/ontology/pull/985

extend range to energy:
issue: https://github.com/OpenEnergyPlatform/ontology/issues/973
pull request: https://github.com/OpenEnergyPlatform/ontology/pull/985",
        rdfs:label "has bearer"@en
    
    Domain: 
        <http://purl.obolibrary.org/obo/BFO_0000020>
    
    Range: 
        OEO_00000150 or <http://purl.obolibrary.org/obo/BFO_0000004>
    
    InverseOf: 
        <http://purl.obolibrary.org/obo/RO_0000053>
    
    
ObjectProperty: OEO_00010231

    Annotations: 
        <http://purl.obolibrary.org/obo/IAO_0000115> "A relation between an entity and an information artifact.",
        <http://purl.obolibrary.org/obo/IAO_0000233> "issue: https://github.com/OpenEnergyPlatform/ontology/issues/858
pull request: https://github.com/OpenEnergyPlatform/ontology/pull/965
",
        rdfs:label "has information content entity"@en
    
    Range: 
        <http://purl.obolibrary.org/obo/IAO_0000030>
    
    InverseOf: 
        <http://purl.obolibrary.org/obo/IAO_0000136>
    
    
ObjectProperty: OEO_00020056

    Annotations: 
        <http://purl.obolibrary.org/obo/IAO_0000115> "A relation that relates a quantity value to its entity in reality.",
        <http://purl.obolibrary.org/obo/IAO_0000233> "issue: https://github.com/OpenEnergyPlatform/ontology/issues/700
pull request: https://github.com/OpenEnergyPlatform/ontology/pull/710",
        rdfs:label "quantity value of"
    
    SubPropertyOf: 
        <http://purl.obolibrary.org/obo/IAO_0000136>
    
    InverseOf: 
        OEO_00140002
    
    
ObjectProperty: OEO_00020179

    Annotations: 
        <http://purl.obolibrary.org/obo/IAO_0000115> "A relation that relates an economic value to a related entity in reality.",
        <http://purl.obolibrary.org/obo/IAO_0000233> "issue: https://github.com/OpenEnergyPlatform/ontology/issues/958
pull request: https://github.com/OpenEnergyPlatform/ontology/pull/1034",
        rdfs:label "economic value of"
    
    SubPropertyOf: 
        <http://purl.obolibrary.org/obo/IAO_0000136>
    
    
ObjectProperty: OEO_00020180

    Annotations: 
        <http://purl.obolibrary.org/obo/IAO_0000115> "A relation between an entity and an economic value.",
        <http://purl.obolibrary.org/obo/IAO_0000233> "issue: https://github.com/OpenEnergyPlatform/ontology/issues/958
pull request: https://github.com/OpenEnergyPlatform/ontology/pull/1034",
        rdfs:label "has economic value"
    
    SubPropertyOf: 
        OEO_00010231
    
    
ObjectProperty: OEO_00020188

    Annotations: 
        <http://purl.obolibrary.org/obo/IAO_0000115> "A relation that holds between an information content entity and a copyright licence.",
        <http://purl.obolibrary.org/obo/IAO_0000233> "issue https://github.com/OpenEnergyPlatform/ontology/issues/1061
pull request https://github.com/OpenEnergyPlatform/ontology/pull/1090",
        rdfs:label "has copyright license"
    
    SubPropertyOf: 
        OEO_00010231
    
    
ObjectProperty: OEO_00020189

    Annotations: 
        <http://purl.obolibrary.org/obo/IAO_0000115> "c is an information input of p iff: c is an input of p, and c is an information content entity",
        <http://purl.obolibrary.org/obo/IAO_0000233> "issue: https://github.com/OpenEnergyPlatform/ontology/issues/1091
pull request: https://github.com/OpenEnergyPlatform/ontology/pull/1113",
        rdfs:label "information input of"
    
    SubPropertyOf: 
        <http://purl.obolibrary.org/obo/RO_0002352>
    
    Domain: 
        <http://purl.obolibrary.org/obo/IAO_0000030>
    
    Range: 
        <http://purl.obolibrary.org/obo/BFO_0000015>
    
    
ObjectProperty: OEO_00020190

    Annotations: 
        <http://purl.obolibrary.org/obo/IAO_0000115> "c is an information ouput of p iff: c is an output of p, and c is an information content entity",
        <http://purl.obolibrary.org/obo/IAO_0000233> "issue: https://github.com/OpenEnergyPlatform/ontology/issues/1091
pull request: https://github.com/OpenEnergyPlatform/ontology/pull/1113",
        rdfs:label "information output of"
    
    SubPropertyOf: 
        <http://purl.obolibrary.org/obo/RO_0002353>
    
    Domain: 
        <http://purl.obolibrary.org/obo/IAO_0000030>
    
    Range: 
        <http://purl.obolibrary.org/obo/BFO_0000015>
    
    
ObjectProperty: OEO_00040010

    Annotations: 
        <http://purl.obolibrary.org/obo/IAO_0000115> "A property that links a quantity value to a unit in which the quantity value has been expressed.",
        rdfs:label "has unit"@en
    
    Domain: 
        OEO_00000350
    
    Range: 
        <http://purl.obolibrary.org/obo/UO_0000000>
    
    
ObjectProperty: OEO_00140002

    Annotations: 
        <http://purl.obolibrary.org/obo/IAO_0000115> "A relation between an entity and a quantity value.",
        <http://purl.obolibrary.org/obo/IAO_0000233> "issue: https://github.com/OpenEnergyPlatform/ontology/issues/505
pull request: https://github.com/OpenEnergyPlatform/ontology/pull/509",
        rdfs:label "has quantity value"@en
    
    SubPropertyOf: 
        
            Annotations: <http://purl.obolibrary.org/obo/IAO_0000233> "issue: https://github.com/OpenEnergyPlatform/ontology/issues/858
pull request: https://github.com/OpenEnergyPlatform/ontology/pull/965"
        OEO_00010231
    
    Range: 
        
            Annotations: rdfs:comment "issue: https://github.com/OpenEnergyPlatform/ontology/issues/850
pull request: https://github.com/OpenEnergyPlatform/ontology/pull/871"
        OEO_00000350
    
    InverseOf: 
        OEO_00020056
    
    
ObjectProperty: OEO_00140008

    Annotations: 
        <http://purl.obolibrary.org/obo/IAO_0000115> "A relation between an information content entity / model and a continuant, in which the continuant is somehow involved in the creation of the information content entity / model.",
        <http://purl.obolibrary.org/obo/IAO_0000233> "issue: https://github.com/OpenEnergyPlatform/ontology/issues/530
pull request: https://github.com/OpenEnergyPlatform/ontology/pull/556
pull request: https://github.com/OpenEnergyPlatform/ontology/pull/626 (extend def for information content entity)
pull request: https://github.com/OpenEnergyPlatform/ontology/pull/871 (domain and range; move to oeo-shared)",
        rdfs:label "has contributor"@en
    
    Domain: 
        OEO_00000274 or <http://purl.obolibrary.org/obo/IAO_0000030>
    
    Range: 
        <http://purl.obolibrary.org/obo/BFO_0000002>
    
    
ObjectProperty: OEO_00140093

    Annotations: 
        <http://purl.obolibrary.org/obo/IAO_0000115> "p has information input c iff: p has input c, and c is an information content entity",
        <http://purl.obolibrary.org/obo/IAO_0000233> "issue: https://github.com/OpenEnergyPlatform/ontology/issues/618
pull request: https://github.com/OpenEnergyPlatform/ontology/pull/716
moved to oeo-shared
pull request: https://github.com/OpenEnergyPlatform/ontology/pull/1113",
        rdfs:label "has information input"@en
    
    SubPropertyOf: 
        <http://purl.obolibrary.org/obo/RO_0002233>
    
    Domain: 
        <http://purl.obolibrary.org/obo/BFO_0000015>
    
    Range: 
        <http://purl.obolibrary.org/obo/IAO_0000030>
    
    
ObjectProperty: OEO_00140094

    Annotations: 
        <http://purl.obolibrary.org/obo/IAO_0000115> "p has information output c iff: p has output c, and c is an information content entity",
        <http://purl.obolibrary.org/obo/IAO_0000233> "issue: https://github.com/OpenEnergyPlatform/ontology/issues/618
pull request: https://github.com/OpenEnergyPlatform/ontology/pull/716
moved to oeo-shared
pull request: https://github.com/OpenEnergyPlatform/ontology/pull/1113",
        rdfs:label "has information output"@en
    
    SubPropertyOf: 
        <http://purl.obolibrary.org/obo/RO_0002234>
    
    Domain: 
        <http://purl.obolibrary.org/obo/BFO_0000015>
    
    Range: 
        <http://purl.obolibrary.org/obo/IAO_0000030>
    
    
ObjectProperty: OEO_00140164

    Annotations: 
        <http://purl.obolibrary.org/obo/IAO_0000115> "A relation between a model and the thing it reproduces.",
        <http://purl.obolibrary.org/obo/IAO_0000233> "issue: https://github.com/OpenEnergyPlatform/ontology/issues/415
pull request: https://github.com/OpenEnergyPlatform/ontology/pull/821",
        rdfs:label "models"@en
    
    Domain: 
        OEO_00000274
    
    Range: 
        <http://purl.obolibrary.org/obo/BFO_0000004>
    
    
ObjectProperty: owl:topObjectProperty

    
DataProperty: OEO_00140178

    Annotations: 
        <http://purl.obolibrary.org/obo/IAO_0000115> "Has number is a data property that links a quantity value to a number that defines the quantity value.",
        <http://purl.obolibrary.org/obo/IAO_0000233> "issue: https://github.com/OpenEnergyPlatform/ontology/issues/829
pull request: https://github.com/OpenEnergyPlatform/ontology/pull/840",
        rdfs:label "has number"@en
    
    Domain: 
        OEO_00000350
    
    
Class: <http://purl.obolibrary.org/obo/BFO_0000002>

    
Class: <http://purl.obolibrary.org/obo/BFO_0000003>

    
Class: <http://purl.obolibrary.org/obo/BFO_0000004>

    
Class: <http://purl.obolibrary.org/obo/BFO_0000009>

    SubClassOf: 
        OEO_00140002 some OEO_00020143
    
    
Class: <http://purl.obolibrary.org/obo/BFO_0000015>

    
Class: <http://purl.obolibrary.org/obo/BFO_0000016>

    
Class: <http://purl.obolibrary.org/obo/BFO_0000017>

    
Class: <http://purl.obolibrary.org/obo/BFO_0000019>

    
Class: <http://purl.obolibrary.org/obo/BFO_0000020>

    
Class: <http://purl.obolibrary.org/obo/BFO_0000023>

    
Class: <http://purl.obolibrary.org/obo/BFO_0000027>

    
Class: <http://purl.obolibrary.org/obo/BFO_0000030>

    
Class: <http://purl.obolibrary.org/obo/BFO_0000031>

    
Class: <http://purl.obolibrary.org/obo/BFO_0000034>

    
Class: <http://purl.obolibrary.org/obo/BFO_0000038>

    
Class: <http://purl.obolibrary.org/obo/BFO_0000040>

    
Class: <http://purl.obolibrary.org/obo/BFO_0000141>

    
Class: <http://purl.obolibrary.org/obo/BFO_0000148>

    
Class: <http://purl.obolibrary.org/obo/IAO_0000027>

    Annotations: 
        
            Annotations: <http://purl.obolibrary.org/obo/IAO_0000233> "issue: https://github.com/OpenEnergyPlatform/ontology/issues/823
pull request: https://github.com/OpenEnergyPlatform/ontology/pull/826"
        <http://purl.obolibrary.org/obo/IAO_0000115> "A data item is an information content entity that is intended to be a truthful statement about something (modulo, e.g., measurement precision or other systematic errors) and is constructed/acquired by a method which reliably tends to produce (approximately) truthful statements.",
        <http://purl.obolibrary.org/obo/IAO_0000119> "http://www.ontobee.org/ontology/IAO?iri=http://purl.obolibrary.org/obo/IAO_0000027"
    
    
Class: <http://purl.obolibrary.org/obo/IAO_0000030>

    Annotations: 
        <http://purl.obolibrary.org/obo/IAO_0000233> "add axiom has copyright license
issue https://github.com/OpenEnergyPlatform/ontology/issues/1061
pull request https://github.com/OpenEnergyPlatform/ontology/pull/1090"
    
    SubClassOf: 
        OEO_00020188 some OEO_00020185
    
    
Class: <http://purl.obolibrary.org/obo/IAO_0000088>

    
Class: <http://purl.obolibrary.org/obo/IAO_0000100>

    Annotations: 
        <http://purl.obolibrary.org/obo/IAO_0000233> "add axiom
pull request: https://github.com/OpenEnergyPlatform/ontology/pull/912"
    
    SubClassOf: 
        OEO_00000514 some OEO_00020121
    
    
Class: <http://purl.obolibrary.org/obo/RO_0002577>

    
Class: <http://purl.obolibrary.org/obo/UO_0000000>

    Annotations: 
        <http://purl.obolibrary.org/obo/IAO_0000233> "issue: https://github.com/OpenEnergyPlatform/ontology/issues/533
pull request: https://github.com/OpenEnergyPlatform/ontology/pull/537
renaming
pull request: https://github.com/OpenEnergyPlatform/ontology/pull/895",
        rdfs:comment "The original definition from UO is \"A unit of measurement is a standardized quantity of a physical quality.\". It was adjusted for OEO purposes such that currencies can also be defined as units."
    
    SubClassOf: 
        <http://purl.obolibrary.org/obo/BFO_0000031>
    
    
Class: <http://purl.obolibrary.org/obo/UO_0000001>

    
Class: <http://purl.obolibrary.org/obo/UO_0000002>

    
Class: <http://purl.obolibrary.org/obo/UO_0000003>

    
Class: <http://purl.obolibrary.org/obo/UO_0000046>

    SubClassOf: 
        <http://purl.obolibrary.org/obo/BFO_0000141>
    
    
Class: <http://purl.obolibrary.org/obo/UO_0000047>

    
Class: <http://purl.obolibrary.org/obo/UO_0000111>

    
Class: <http://purl.obolibrary.org/obo/UO_0000224>

    Annotations: 
        <http://purl.obolibrary.org/obo/IAO_0000118> "kilowatt hours",
        <http://purl.obolibrary.org/obo/IAO_0000233> "add eurostat alternative term and has_exact_synonym:
issue: https://github.com/OpenEnergyPlatform/ontology/issues/920
pull request: https://github.com/OpenEnergyPlatform/ontology/pull/924",
        <http://www.geneontology.org/formats/oboInOwl#hasExactSynonym> "kWh",
        rdfs:comment "The original term from UO had neither an alternative term nor has_exact_synonym. It was added for OEO purposes to include the Eurostat spellings."@en
    
    
Class: OEO_00000051

    Annotations: 
        OEO_00040001 "http://openenergy-platform.org/ontology/oeo/oeo-shared"^^xsd:string,
        <http://purl.obolibrary.org/obo/IAO_0000115> "Agent is a role of a person or organisation that directs its activity towards achieving goals."@en,
        <http://purl.obolibrary.org/obo/IAO_0000233> "issue:https://github.com/OpenEnergyPlatform/ontology/issues/148
pull request: https://github.com/OpenEnergyPlatform/ontology/pull/210",
        rdfs:label "agent"
    
    SubClassOf: 
        <http://purl.obolibrary.org/obo/BFO_0000023>
    
    
Class: OEO_00000061

    Annotations: 
        OEO_00040001 "http://openenergy-platform.org/ontology/oeo/oeo-shared"^^xsd:string,
        <http://purl.obolibrary.org/obo/IAO_0000115> "An artificial object is an object that was deliberately manufactured by humans to address a particular purpose.",
        <http://purl.obolibrary.org/obo/IAO_0000233> "issue: https://github.com/OpenEnergyPlatform/ontology/issues/86
pull requests: https://github.com/OpenEnergyPlatform/ontology/pull/121 (artificial object definition)
subclasses
https://github.com/OpenEnergyPlatform/ontology/pull/128
relation to space requirement
https://github.com/OpenEnergyPlatform/ontology/pull/933",
        rdfs:label "artificial object"
    
    SubClassOf: 
        <http://purl.obolibrary.org/obo/BFO_0000030>,
        <http://purl.obolibrary.org/obo/RO_0002328> some OEO_00020136
    
    
Class: OEO_00000064

    Annotations: 
        OEO_00040001 "http://openenergy-platform.org/ontology/oeo/oeo-shared"^^xsd:string,
        <http://purl.obolibrary.org/obo/IAO_0000115> "An author is an agent that creates or has created written work.",
        rdfs:label "author"
    
    SubClassOf: 
        OEO_00000051
    
    
Class: OEO_00000087

    Annotations: 
        OEO_00040001 "http://openenergy-platform.org/ontology/oeo/oeo-shared"^^xsd:string,
        <http://purl.obolibrary.org/obo/IAO_0000115> "A client is an agent that receives a product or service.",
        rdfs:label "client"
    
    SubClassOf: 
        OEO_00000051
    
    
Class: OEO_00000107

    Annotations: 
        OEO_00040001 "http://openenergy-platform.org/ontology/oeo/oeo-shared"^^xsd:string,
        <http://purl.obolibrary.org/obo/IAO_0000115> "A contact person is an agent that can be contacted for help or information about a specific service or good.",
        rdfs:label "contact person"
    
    SubClassOf: 
        OEO_00000051
    
    
Class: OEO_00000147

    Annotations: 
        OEO_00040001 "http://openenergy-platform.org/ontology/oeo/oeo-shared"^^xsd:string,
        <http://purl.obolibrary.org/obo/IAO_0000115> "emission is a process releasing byproducts from human activity (e.g. production, distribution or consumption) into the environment."@en,
        <http://purl.obolibrary.org/obo/IAO_0000233> "issue: https://github.com/OpenEnergyPlatform/ontology/issues/56
pull request: https://github.com/OpenEnergyPlatform/ontology/pull/234
moved to oeo-shared
https://github.com/OpenEnergyPlatform/ontology/pull/956",
        rdfs:label "emission"
    
    SubClassOf: 
        <http://purl.obolibrary.org/obo/BFO_0000015>,
        OEO_00000500 some OEO_00000148
    
    
Class: OEO_00000148

    Annotations: 
        OEO_00040001 "http://openenergy-platform.org/ontology/oeo/oeo-shared"^^xsd:string,
        <http://purl.obolibrary.org/obo/IAO_0000115> "An emission factor is a process attribute that quantifies the emissions or removals of a gas per unit activity.",
        <http://purl.obolibrary.org/obo/IAO_0000233> "issue: https://github.com/OpenEnergyPlatform/ontology/issues/243
pull request: https://github.com/OpenEnergyPlatform/ontology/pull/581
moved to oeo-shared
https://github.com/OpenEnergyPlatform/ontology/pull/956",
        rdfs:label "emission factor"
    
    SubClassOf: 
        OEO_00030019,
        OEO_00000502 some OEO_00000147,
        OEO_00000502 some <http://purl.obolibrary.org/obo/BFO_0000015>
    
    
Class: OEO_00000150

    Annotations: 
        OEO_00040001 "http://openenergy-platform.org/ontology/oeo/oeo-shared"^^xsd:string,
        <http://purl.obolibrary.org/obo/IAO_0000115> "Energy is a quality of material entities which manifests as a capacity to perform work (such as causing motion or the interaction of molecules)",
        <http://purl.obolibrary.org/obo/IAO_0000119> "Derived from https://www.lexico.com/en/definition/energy",
        <http://purl.obolibrary.org/obo/IAO_0000233> "issue: https://github.com/OpenEnergyPlatform/ontology/issues/224
pull request: https://github.com/OpenEnergyPlatform/ontology/pull/364
fix grammar error:
pull request: https://github.com/OpenEnergyPlatform/ontology/pull/657
update definition
issue: https://github.com/OpenEnergyPlatform/ontology/issues/660
pull request: https://github.com/OpenEnergyPlatform/ontology/pull/665
move to oeo-shared
issue: https://github.com/OpenEnergyPlatform/ontology/issues/1030
pull request: https://github.com/OpenEnergyPlatform/ontology/pull/1101
adjust definition
pull request: https://github.com/OpenEnergyPlatform/ontology/pull/1165

Axiomatise relations between origin, energy and portion of matter:
issue: https://github.com/OpenEnergyPlatform/ontology/issues/1183
pull request: https://github.com/OpenEnergyPlatform/ontology/pull/1192",
        rdfs:comment "Energy is power integrated over time.",
        rdfs:label "energy",
        
            Annotations: <http://purl.obolibrary.org/obo/IAO_0000233> "issue: https://github.com/OpenEnergyPlatform/ontology/issues/636
pull request: https://github.com/OpenEnergyPlatform/ontology/pull/810"
        owl:equivalentClass "http://purl.obolibrary.org/obo/ENVO_2000015"
    
    SubClassOf: 
        <http://purl.obolibrary.org/obo/BFO_0000019>,
        OEO_00000530 some OEO_00000316
    
    
Class: OEO_00000151

    Annotations: 
        OEO_00040001 "http://openenergy-platform.org/ontology/oeo/oeo-shared"^^xsd:string,
        <http://purl.obolibrary.org/obo/IAO_0000115> "An energy carrier disposition is a disposition of an material entity that contains energy for conversion as usable energy."@en,
        <http://purl.obolibrary.org/obo/IAO_0000233> "issue: https://github.com/OpenEnergyPlatform/ontology/issues/209
pull request: https://github.com/OpenEnergyPlatform/ontology/pull/276
issue: https://github.com/OpenEnergyPlatform/ontology/issues/407
pull request: https://github.com/OpenEnergyPlatform/ontology/pull/627
move to oeo-shared
pull request: https://github.com/OpenEnergyPlatform/ontology/pull/869

add has bearer axiom:
issue: https://github.com/OpenEnergyPlatform/ontology/issues/1167
pull request: https://github.com/OpenEnergyPlatform/ontology/pull/1178",
        rdfs:label "energy carrier disposition"
    
    SubClassOf: 
        <http://purl.obolibrary.org/obo/BFO_0000016>,
        OEO_00010121 some <http://purl.obolibrary.org/obo/BFO_0000040>
    
    
Class: OEO_00000206

    Annotations: 
        OEO_00040001 "http://openenergy-platform.org/ontology/oeo/oeo-shared"^^xsd:string,
        <http://purl.obolibrary.org/obo/IAO_0000115> "Hardware is an artificial object that is part of an electronic system.",
        <http://purl.obolibrary.org/obo/IAO_0000233> "issue: https://github.com/OpenEnergyPlatform/ontology/issues/319
pull request: https://github.com/OpenEnergyPlatform/ontology/pull/350",
        rdfs:label "hardware"
    
    SubClassOf: 
        OEO_00000061
    
    
Class: OEO_00000238

    Annotations: 
        OEO_00040001 "http://openenergy-platform.org/ontology/oeo/oeo-shared"^^xsd:string,
        <http://purl.obolibrary.org/obo/IAO_0000115> "An institution is an organisation that serves a social purpose."@en,
        <http://purl.obolibrary.org/obo/IAO_0000233> "moved term to oeo-shared:
pull request: https://github.com/OpenEnergyPlatform/ontology/pull/871",
        rdfs:label "institution"
    
    SubClassOf: 
        OEO_00030022
    
    
Class: OEO_00000264

    Annotations: 
        OEO_00040001 "http://openenergy-platform.org/ontology/oeo/oeo-shared"^^xsd:string,
        <http://purl.obolibrary.org/obo/IAO_0000115> "An energy market model is a model that is about the energy market."^^xsd:string,
        <http://purl.obolibrary.org/obo/IAO_0000233> "issue: https://github.com/OpenEnergyPlatform/ontology/issues/415
pull request: https://github.com/OpenEnergyPlatform/ontology/pull/821",
        rdfs:label "energy market model"
    
    SubClassOf: 
        OEO_00000274
    
    
Class: OEO_00000274

    Annotations: 
        OEO_00040001 "http://openenergy-platform.org/ontology/oeo/oeo-shared"^^xsd:string,
        <http://purl.obolibrary.org/obo/IAO_0000115> "A model is a generically dependent continuant that is used for computing an idealised reproduction of a system and its behaviours."@en,
        <http://purl.obolibrary.org/obo/IAO_0000233> "issue: https://github.com/OpenEnergyPlatform/ontology/issues/180
pull request: https://github.com/OpenEnergyPlatform/ontology/pull/349

issue: https://github.com/OpenEnergyPlatform/ontology/issues/208
pull request: https://github.com/OpenEnergyPlatform/ontology/pull/287

add axiom to model calculation
pull request: https://github.com/OpenEnergyPlatform/ontology/pull/1113",
        rdfs:label "model"
    
    SubClassOf: 
        <http://purl.obolibrary.org/obo/BFO_0000031>,
        
            Annotations: <http://purl.obolibrary.org/obo/IAO_0000233> "issue: https://github.com/OpenEnergyPlatform/ontology/issues/415
pull request: https://github.com/OpenEnergyPlatform/ontology/pull/821"
        OEO_00140164 some <http://purl.obolibrary.org/obo/BFO_0000004>,
        <http://purl.obolibrary.org/obo/RO_0000056> some OEO_00000275
    
    
Class: OEO_00000275

    Annotations: 
        OEO_00040001 "http://openenergy-platform.org/ontology/oeo/oeo-shared"^^xsd:string,
        <http://purl.obolibrary.org/obo/IAO_0000115> "A model calculation is a process of solving mathematical equations of a model."@en,
        <http://purl.obolibrary.org/obo/IAO_0000233> "issue: https://github.com/OpenEnergyPlatform/ontology/issues/73
pull request: https://github.com/OpenEnergyPlatform/ontology/pull/504
moved to oeo-shared
pull request: https://github.com/OpenEnergyPlatform/ontology/pull/1113"@en,
        rdfs:label "model calculation"
    
    SubClassOf: 
        <http://purl.obolibrary.org/obo/BFO_0000015>,
        OEO_00140093 some OEO_00030029,
        OEO_00140094 some OEO_00030030,
        
            Annotations: <http://purl.obolibrary.org/obo/IAO_0000233> "issue: https://github.com/OpenEnergyPlatform/ontology/issues/850
pull request: https://github.com/OpenEnergyPlatform/ontology/pull/871"
        <http://purl.obolibrary.org/obo/RO_0000057> some OEO_00000274
    
    
Class: OEO_00000315

    Annotations: 
        OEO_00040001 "http://openenergy-platform.org/ontology/oeo/oeo-shared"^^xsd:string,
        <http://purl.obolibrary.org/obo/IAO_0000115> "An organisation role is a role of an aggregate of people that has a collective goal and a set of organisation rules.",
        <http://purl.obolibrary.org/obo/IAO_0000118> "organization role",
        <http://purl.obolibrary.org/obo/IAO_0000233> "issue: https://github.com/OpenEnergyPlatform/ontology/issues/314
pull request: https://github.com/OpenEnergyPlatform/ontology/pull/370",
        rdfs:label "organisation role"
    
    SubClassOf: 
        <http://purl.obolibrary.org/obo/BFO_0000023>
    
    DisjointWith: 
        OEO_00000323
    
    
Class: OEO_00000316

    Annotations: 
        OEO_00040001 "http://openenergy-platform.org/ontology/oeo/oeo-shared"^^xsd:string,
        <http://purl.obolibrary.org/obo/IAO_0000115> "Origin is a quality of a portion of matter or energy based on where it comes from. It is inherited from its primary sources.",
        <http://purl.obolibrary.org/obo/IAO_0000233> "issue: https://github.com/OpenEnergyPlatform/ontology/issues/108
pull request: https://github.com/OpenEnergyPlatform/ontology/pull/130

change def
issue: https://github.com/OpenEnergyPlatform/ontology/issues/741
pull request: https://github.com/OpenEnergyPlatform/ontology/pull/861

change definition and add comment with examples:
issue: https://github.com/OpenEnergyPlatform/ontology/issues/974
pull request: https://github.com/OpenEnergyPlatform/ontology/pull/976

Axiomatise relations between origin, energy and portion of matter:
issue: https://github.com/OpenEnergyPlatform/ontology/issues/1183
pull request: https://github.com/OpenEnergyPlatform/ontology/pull/1192

Move to oeo-shared:
issue: https://github.com/OpenEnergyPlatform/ontology/issues/1218
pull request: https://github.com/OpenEnergyPlatform/ontology/pull/1219",
        rdfs:comment "* Biomass has a biogenic origin and if it is converted to biogas, the biogas inherits the the biogenic origin.
* Hard coal has a fossil origin and if it is used in a coal power plant to generate electrical energy, the electrical energy inherits the fossil origin.
* Wind energy has renewable origin and if it is converted to electrical energy using a wind turbine, the electrical energy inherits the renewable origin",
        rdfs:label "origin"
    
    SubClassOf: 
        <http://purl.obolibrary.org/obo/BFO_0000019>,
        OEO_00010121 some 
            (OEO_00000150 or OEO_00000331)
    
    
Class: OEO_00000323

    Annotations: 
        OEO_00040001 "http://openenergy-platform.org/ontology/oeo/oeo-shared"^^xsd:string,
        <http://purl.obolibrary.org/obo/IAO_0000115> "A person is a human being."@en,
        rdfs:label "person"
    
    SubClassOf: 
        <http://purl.obolibrary.org/obo/BFO_0000030>
    
    DisjointWith: 
        OEO_00000315
    
    
Class: OEO_00000331

    Annotations: 
        OEO_00040001 "http://openenergy-platform.org/ontology/oeo/oeo-shared"^^xsd:string,
        <http://purl.obolibrary.org/obo/IAO_0000115> "A portion of matter is an aggregate of material entities that have a state of matter."@en,
        <http://purl.obolibrary.org/obo/IAO_0000116> "Portions of matter describe mass nouns like e.g. water, air and fuel. Mass nouns are uncountable, but portions of these can be quantified, like 1 glass of water, 1 m of air or 1 barrel of fuel. For further explanation please refer to: https://github.com/OpenEnergyPlatform/ontology/wiki/Explanation-on-mass-nouns",
        <http://purl.obolibrary.org/obo/IAO_0000233> "issue: https://github.com/OpenEnergyPlatform/ontology/issues/227
pull request: https://github.com/OpenEnergyPlatform/ontology/pull/279

definition update and editor note:
issue: https://github.com/OpenEnergyPlatform/ontology/issues/738
pull request: https://github.com/OpenEnergyPlatform/ontology/pull/759

Axiomatise relations between origin, energy and portion of matter:
issue: https://github.com/OpenEnergyPlatform/ontology/issues/1183
pull request: https://github.com/OpenEnergyPlatform/ontology/pull/1192

Move to oeo-shared:
issue: https://github.com/OpenEnergyPlatform/ontology/issues/1218
pull request: https://github.com/OpenEnergyPlatform/ontology/pull/1219",
        rdfs:comment "wiki page: https://github.com/OpenEnergyPlatform/ontology/wiki/Explanation-on-mass-nouns",
        rdfs:label "portion of matter"
    
    SubClassOf: 
        <http://purl.obolibrary.org/obo/BFO_0000027>,
        OEO_00000530 some OEO_00000316
    
    
Class: OEO_00000340

    Annotations: 
        OEO_00040001 "http://openenergy-platform.org/ontology/oeo/oeo-shared"^^xsd:string,
        <http://purl.obolibrary.org/obo/IAO_0000115> "A project is a process to achieve a specified goal that is unique in the sum of its conditions like its goal, time and cost budget and its organisation.",
        <http://purl.obolibrary.org/obo/IAO_0000233> "issue: https://github.com/OpenEnergyPlatform/ontology/issues/247
pull request: https://github.com/OpenEnergyPlatform/ontology/pull/418
move to oeo-shared
issue: https://github.com/OpenEnergyPlatform/ontology/issues/862
pull request: https://github.com/OpenEnergyPlatform/ontology/pull/869",
        rdfs:label "project"
    
    SubClassOf: 
        <http://purl.obolibrary.org/obo/BFO_0000015>
    
    
Class: OEO_00000350

    Annotations: 
        OEO_00040001 "http://openenergy-platform.org/ontology/oeo/oeo-shared"^^xsd:string,
        <http://purl.obolibrary.org/obo/IAO_0000115> "A quantity value is an information content entity defined by a numeral together with a unit of measurement to quantify an entity."@en,
        <http://purl.obolibrary.org/obo/IAO_0000233> "issue: https://github.com/OpenEnergyPlatform/ontology/issues/205
pull request: https://github.com/OpenEnergyPlatform/ontology/pull/386

issue: https://github.com/OpenEnergyPlatform/ontology/issues/495

pull request: https://github.com/OpenEnergyPlatform/ontology/pull/496

issue: https://github.com/OpenEnergyPlatform/ontology/issues/505
pull request: https://github.com/OpenEnergyPlatform/ontology/pull/518",
        rdfs:label "quantity value",
        
            Annotations: <http://purl.obolibrary.org/obo/IAO_0000233> "issue: https://github.com/OpenEnergyPlatform/ontology/issues/636
pull request: https://github.com/OpenEnergyPlatform/ontology/pull/810"
        owl:equivalentClass "http://purl.obolibrary.org/obo/IAO_0000032"
    
    SubClassOf: 
        <http://purl.obolibrary.org/obo/IAO_0000030>,
        OEO_00040010 some <http://purl.obolibrary.org/obo/UO_0000000>
    
    
Class: OEO_00000367

    Annotations: 
        OEO_00040001 "http://openenergy-platform.org/ontology/oeo/oeo-shared"^^xsd:string,
        <http://purl.obolibrary.org/obo/IAO_0000115> "A sector is generically dependent continuant that is a subdivision of a system."@en,
        <http://purl.obolibrary.org/obo/IAO_0000233> "issue: https://github.com/OpenEnergyPlatform/ontology/issues/30
pull request: https://github.com/OpenEnergyPlatform/ontology/pull/477
moved to oeo-shared
pull request: https://github.com/OpenEnergyPlatform/ontology/pull/764",
        rdfs:label "sector"
    
    SubClassOf: 
        <http://purl.obolibrary.org/obo/BFO_0000031>
    
    
Class: OEO_00000419

    Annotations: 
        OEO_00040001 "http://openenergy-platform.org/ontology/oeo/oeo-shared"^^xsd:string,
        <http://purl.obolibrary.org/obo/IAO_0000115> "A transformation is a process that transforms one or more inputs into at least one output."@en,
        <http://purl.obolibrary.org/obo/IAO_0000233> "issue: https://github.com/OpenEnergyPlatform/ontology/issues/435
pull request: https://github.com/OpenEnergyPlatform/ontology/pull/450

input and output axioms:
issue: https://github.com/OpenEnergyPlatform/ontology/issues/1167
pull request: https://github.com/OpenEnergyPlatform/ontology/pull/1178",
        rdfs:label "transformation"
    
    SubClassOf: 
        <http://purl.obolibrary.org/obo/BFO_0000015>,
        <http://purl.obolibrary.org/obo/RO_0002233> some <http://purl.obolibrary.org/obo/BFO_0000002>,
        <http://purl.obolibrary.org/obo/RO_0002234> some <http://purl.obolibrary.org/obo/BFO_0000002>
    
    
Class: OEO_00000423

    Annotations: 
        OEO_00040001 "http://openenergy-platform.org/ontology/oeo/oeo-shared"^^xsd:string,
        <http://purl.obolibrary.org/obo/IAO_0000115> "An electricity transshipment model is a model that applies the transshipment problem to the electricity grid.",
        <http://purl.obolibrary.org/obo/IAO_0000233> "issue: https://github.com/OpenEnergyPlatform/ontology/issues/337
pull request: https://github.com/OpenEnergyPlatform/ontology/pull/358",
        rdfs:label "electricity transshipment model"
    
    SubClassOf: 
        OEO_00000274
    
    
Class: OEO_00010023

    Annotations: 
        OEO_00040001 "http://openenergy-platform.org/ontology/oeo/oeo-shared"^^xsd:string,
        <http://purl.obolibrary.org/obo/IAO_0000115> "A vehicle is an artificial object that is used for transporting people or goods.",
        <http://purl.obolibrary.org/obo/IAO_0000233> "issue: https://github.com/OpenEnergyPlatform/ontology/issues/425
pull request: https://github.com/OpenEnergyPlatform/ontology/pull/431",
        rdfs:label "vehicle",
        
            Annotations: <http://purl.obolibrary.org/obo/IAO_0000233> "issue: https://github.com/OpenEnergyPlatform/ontology/issues/636
pull request: https://github.com/OpenEnergyPlatform/ontology/pull/810"
        owl:equivalentClass "http://purl.obolibrary.org/obo/ENVO_01000604"
    
    SubClassOf: 
        OEO_00000061
    
    
Class: OEO_00010079

    Annotations: 
        OEO_00040001 "http://openenergy-platform.org/ontology/oeo/oeo-shared"^^xsd:string,
        <http://purl.obolibrary.org/obo/IAO_0000115> "An emission quantity value is a quantity value that has a mass unit as unit. It is the quantity value of an emission value."@en,
        <http://purl.obolibrary.org/obo/IAO_0000233> "issue: https://github.com/OpenEnergyPlatform/ontology/issues/695
pull request: https://github.com/OpenEnergyPlatform/ontology/pull/697",
        rdfs:label "emission quantity value"@en
    
    SubClassOf: 
        OEO_00000350,
        OEO_00040010 some <http://purl.obolibrary.org/obo/UO_0000002>
    
    
Class: OEO_00010116

    Annotations: 
        OEO_00040001 "http://openenergy-platform.org/ontology/oeo/oeo-shared"^^xsd:string,
        <http://purl.obolibrary.org/obo/IAO_0000115> "A good is a continuant that has the good role.",
        <http://purl.obolibrary.org/obo/IAO_0000233> "issue: https://github.com/OpenEnergyPlatform/ontology/issues/832
pull request: https://github.com/OpenEnergyPlatform/ontology/pull/843
move to oeo-shared
pull request: https://github.com/OpenEnergyPlatform/ontology/pull/869

make good a continuant:
pull request: https://github.com/OpenEnergyPlatform/ontology/pull/1127",
        rdfs:label "good"@en
    
    EquivalentTo: 
        <http://purl.obolibrary.org/obo/BFO_0000002>
         and (<http://purl.obolibrary.org/obo/RO_0000087> some OEO_00010117)
    
    SubClassOf: 
        <http://purl.obolibrary.org/obo/BFO_0000002>
    
    
Class: OEO_00010117

    Annotations: 
        OEO_00040001 "http://openenergy-platform.org/ontology/oeo/oeo-shared"^^xsd:string,
        <http://purl.obolibrary.org/obo/IAO_0000115> "The role of a continuant over which ownership rights can be established, whose ownership can be passed from one party to another by engaging in transactions, and that is not money.",
        <http://purl.obolibrary.org/obo/IAO_0000119> "https://spec.edmcouncil.org/fibo/ontology/FND/ProductsAndServices/ProductsAndServices/Good",
        <http://purl.obolibrary.org/obo/IAO_0000233> "issue: https://github.com/OpenEnergyPlatform/ontology/issues/832
pull request: https://github.com/OpenEnergyPlatform/ontology/pull/843
add relation to monetary price
pull request: https://github.com/OpenEnergyPlatform/ontology/pull/1034

update definition:
pull request: https://github.com/OpenEnergyPlatform/ontology/pull/1127",
        rdfs:label "good role"@en
    
    SubClassOf: 
        <http://purl.obolibrary.org/obo/BFO_0000023>,
        OEO_00020180 some OEO_00040003
    
    
Class: OEO_00010263

    Annotations: 
        OEO_00040001 "http://openenergy-platform.org/ontology/oeo/oeo-shared"^^xsd:string,
        <http://purl.obolibrary.org/obo/IAO_0000115> "A passenger transport is a transport process in which people are moved in a vehicle from one place to another.",
        <http://purl.obolibrary.org/obo/IAO_0000233> "issue: https://github.com/OpenEnergyPlatform/ontology/issues/1055
pull request: https://github.com/OpenEnergyPlatform/ontology/pull/1234",
        rdfs:label "passenger transport"
    
    SubClassOf: 
        OEO_00140003,
        <http://purl.obolibrary.org/obo/RO_0000057> some OEO_00010023,
        <http://purl.obolibrary.org/obo/RO_0000057> some 
            (OEO_00000323
             and (<http://purl.obolibrary.org/obo/RO_0000087> some OEO_00010264))
    
    
Class: OEO_00010264

    Annotations: 
        OEO_00040001 "http://openenergy-platform.org/ontology/oeo/oeo-shared"^^xsd:string,
        <http://purl.obolibrary.org/obo/IAO_0000115> "A passenger is an agent who travels in a vehicle.",
        <http://purl.obolibrary.org/obo/IAO_0000233> "issue: https://github.com/OpenEnergyPlatform/ontology/issues/1055
pull request: https://github.com/OpenEnergyPlatform/ontology/pull/1234",
        rdfs:label "passenger"
    
    SubClassOf: 
        OEO_00000051,
        OEO_00010121 some OEO_00000323
    
    
Class: OEO_00010265

    Annotations: 
        OEO_00040001 "http://openenergy-platform.org/ontology/oeo/oeo-shared"^^xsd:string,
        <http://purl.obolibrary.org/obo/IAO_0000115> "Energy service demand for passenger-kilometre is the energy service demand that is consumed to transport one person over a distance of one kilometre.",
        <http://purl.obolibrary.org/obo/IAO_0000233> "issue: https://github.com/OpenEnergyPlatform/ontology/issues/1055
pull request: https://github.com/OpenEnergyPlatform/ontology/pull/1234",
        rdfs:label "energy service demand for passenger-kilometre"
    
    SubClassOf: 
        OEO_00240024,
        <http://purl.obolibrary.org/obo/BFO_0000054> some OEO_00010263
    
    
Class: OEO_00010266

    Annotations: 
        OEO_00040001 "http://openenergy-platform.org/ontology/oeo/oeo-shared"^^xsd:string,
        <http://purl.obolibrary.org/obo/IAO_0000115> "Energy service demand for ton-kilometre is the energy service demand that is consumed to transport one metric ton over a distance of one kilometre.",
        <http://purl.obolibrary.org/obo/IAO_0000233> "issue: https://github.com/OpenEnergyPlatform/ontology/issues/1055
pull request: https://github.com/OpenEnergyPlatform/ontology/pull/1234",
        rdfs:label "energy service demand for ton-kilometre"
    
    SubClassOf: 
        OEO_00240024,
        <http://purl.obolibrary.org/obo/BFO_0000054> some OEO_00140005
    
    
Class: OEO_00020011

    Annotations: 
        OEO_00040001 "http://openenergy-platform.org/ontology/oeo/oeo-shared"^^xsd:string,
        <http://purl.obolibrary.org/obo/IAO_0000115> "A study is a project with the goal to investigate something."@en,
        <http://purl.obolibrary.org/obo/IAO_0000116> "The construct 'has funding source' some ('has role' some funder) is necessary, because has funding source has the range has role some funder. This range comes from issue https://github.com/OpenEnergyPlatform/ontology/issues/850 : funding source is some kind of independent continuant, i.e. a organisation or person, that does something special (giving money). So it is anything that has role some funder.",
        <http://purl.obolibrary.org/obo/IAO_0000233> "issue: https://github.com/OpenEnergyPlatform/ontology/issues/247
pull request: https://github.com/OpenEnergyPlatform/ontology/pull/497
add covers-relation (oeo-model)
pull request: https://github.com/OpenEnergyPlatform/ontology/pull/764
move to oeo-shared
issue: https://github.com/OpenEnergyPlatform/ontology/issues/862
pull request: https://github.com/OpenEnergyPlatform/ontology/pull/869
add axiom (study report)
issue: https://github.com/OpenEnergyPlatform/ontology/issues/971
pull request: https://github.com/OpenEnergyPlatform/ontology/pull/1011
add etitor note
pull request: https://github.com/OpenEnergyPlatform/ontology/pull/1025"@en,
        rdfs:label "study"@en
    
    SubClassOf: 
        OEO_00000340,
        
            Annotations: <http://purl.obolibrary.org/obo/IAO_0000233> "issue: https://github.com/OpenEnergyPlatform/ontology/issues/473
pull request: https://github.com/OpenEnergyPlatform/ontology/pull/557"
        OEO_00000509 some (<http://purl.obolibrary.org/obo/RO_0000087> some OEO_00090001),
        <http://purl.obolibrary.org/obo/RO_0000057> some <http://purl.obolibrary.org/obo/IAO_0000100>,
        <http://purl.obolibrary.org/obo/RO_0002234> some OEO_00020012
    
    
Class: OEO_00020012

    Annotations: 
        OEO_00040001 "http://openenergy-platform.org/ontology/oeo/oeo-shared"^^xsd:string,
        <http://purl.obolibrary.org/obo/IAO_0000115> "A study report is a report that is the output from some study."@en,
        <http://purl.obolibrary.org/obo/IAO_0000233> "issue: https://github.com/OpenEnergyPlatform/ontology/issues/247
pull request: https://github.com/OpenEnergyPlatform/ontology/pull/497
add etitor note
pull request: https://github.com/OpenEnergyPlatform/ontology/pull/1025"@en,
        rdfs:label "study report"@en
    
    SubClassOf: 
        <http://purl.obolibrary.org/obo/IAO_0000088>,
        
            Annotations: <http://purl.obolibrary.org/obo/IAO_0000233> "issue: https://github.com/OpenEnergyPlatform/ontology/issues/473
pull request: https://github.com/OpenEnergyPlatform/ontology/pull/557

issue: https://github.com/OpenEnergyPlatform/ontology/issues/850
pull request: https://github.com/OpenEnergyPlatform/ontology/pull/871"
        OEO_00000506 some (<http://purl.obolibrary.org/obo/RO_0000087> some OEO_00000064),
        <http://purl.obolibrary.org/obo/IAO_0000136> some <http://purl.obolibrary.org/obo/IAO_0000100>,
        <http://purl.obolibrary.org/obo/RO_0002353> some OEO_00020011
    
    
Class: OEO_00020015

    Annotations: 
        OEO_00040001 "http://openenergy-platform.org/ontology/oeo/oeo-shared"^^xsd:string,
        <http://purl.obolibrary.org/obo/IAO_0000115> "A licence is an information content entity that contains an official permission or permit to do, use or own something.",
        <http://purl.obolibrary.org/obo/IAO_0000118> "license",
        <http://purl.obolibrary.org/obo/IAO_0000233> "issue https://github.com/OpenEnergyPlatform/ontology/issues/31
pull request https://github.com/OpenEnergyPlatform/ontology/pull/561
move to oeo-shared
pull request https://github.com/OpenEnergyPlatform/ontology/pull/740",
        rdfs:label "licence"
    
    SubClassOf: 
        <http://purl.obolibrary.org/obo/IAO_0000030>
    
    
Class: OEO_00020039

    Annotations: 
        OEO_00040001 "http://openenergy-platform.org/ontology/oeo/oeo-shared"^^xsd:string,
        <http://purl.obolibrary.org/obo/IAO_0000115> "An energy carrier is a material entity that has an energy carrier disposition.",
        <http://purl.obolibrary.org/obo/IAO_0000233> "issue: https://github.com/OpenEnergyPlatform/ontology/issues/407
pull request: https://github.com/OpenEnergyPlatform/ontology/pull/627
move to oeo-shared
pull request: https://github.com/OpenEnergyPlatform/ontology/pull/869
improve definition:
issue: https://github.com/OpenEnergyPlatform/ontology/issues/1169
pull request: https://github.com/OpenEnergyPlatform/ontology/pull/1173",
        rdfs:label "energy carrier"
    
    EquivalentTo: 
        <http://purl.obolibrary.org/obo/BFO_0000040>
         and (<http://purl.obolibrary.org/obo/RO_0000091> some OEO_00000151)
    
    SubClassOf: 
        <http://purl.obolibrary.org/obo/BFO_0000040>
    
    
Class: OEO_00020063

    Annotations: 
        OEO_00040001 "http://openenergy-platform.org/ontology/oeo/oeo-shared"^^xsd:string,
        <http://purl.obolibrary.org/obo/IAO_0000115> "An emission certificate is a licence that permits its holder/owner a specific emission value. An emission certificate can be traded at a CO2 market exchange.",
        <http://purl.obolibrary.org/obo/IAO_0000233> "issue https://github.com/OpenEnergyPlatform/ontology/issues/677
pull request https://github.com/OpenEnergyPlatform/ontology/pull/740
moved to oeo-shared
pull request https://github.com/OpenEnergyPlatform/ontology/pull/956
add axiom to emission quantity value and emission certificate price
pull request https://github.com/OpenEnergyPlatform/ontology/pull/1034",
        rdfs:label "emission certificate"
    
    SubClassOf: 
        OEO_00020015,
        OEO_00020180 some OEO_00020154,
        OEO_00140002 some OEO_00010079
    
    
Class: OEO_00020066

    Annotations: 
        OEO_00040001 "http://openenergy-platform.org/ontology/oeo/oeo-shared"^^xsd:string,
        <http://purl.obolibrary.org/obo/IAO_0000115> "Fuel commodity role is the commodity role of fuels.",
        <http://purl.obolibrary.org/obo/IAO_0000233> "https://github.com/OpenEnergyPlatform/ontology/issues/256
https://github.com/OpenEnergyPlatform/ontology/pull/748",
        rdfs:label "fuel commodity role"
    
    SubClassOf: 
        OEO_00040011
    
    
Class: OEO_00020067

    Annotations: 
        OEO_00040001 "http://openenergy-platform.org/ontology/oeo/oeo-shared"^^xsd:string,
        <http://purl.obolibrary.org/obo/IAO_0000115> "A commodity is a good that bears the commodity role.",
        <http://purl.obolibrary.org/obo/IAO_0000233> "issue: https://github.com/OpenEnergyPlatform/ontology/issues/302
pull request: https://github.com/OpenEnergyPlatform/ontology/pull/748
add alternative term
pull request: https://github.com/OpenEnergyPlatform/ontology/pull/800
subclass of good
pull request: https://github.com/OpenEnergyPlatform/ontology/pull/843
change axiom
pull request: https://github.com/OpenEnergyPlatform/ontology/pull/869",
        rdfs:label "commodity"
    
    EquivalentTo: 
        OEO_00010116
         and (<http://purl.obolibrary.org/obo/RO_0000087> some OEO_00040011)
    
    SubClassOf: 
        OEO_00010116
    
    
Class: OEO_00020068

    Annotations: 
        OEO_00040001 "http://openenergy-platform.org/ontology/oeo/oeo-shared"^^xsd:string,
        <http://purl.obolibrary.org/obo/IAO_0000115> "A fuel commodity is a commodity that is a fuel.",
        <http://purl.obolibrary.org/obo/IAO_0000233> "issue: https://github.com/OpenEnergyPlatform/ontology/issues/302
pull request: https://github.com/OpenEnergyPlatform/ontology/pull/748",
        rdfs:label "fuel commodity"
    
    EquivalentTo: 
        <http://purl.obolibrary.org/obo/RO_0000087> some OEO_00020066
    
    SubClassOf: 
        OEO_00020067
    
    
Class: OEO_00020121

    Annotations: 
        OEO_00040001 "http://openenergy-platform.org/ontology/oeo/oeo-shared"^^xsd:string,
        <http://purl.obolibrary.org/obo/IAO_0000115> "Resolution is a quality of a dataset that indicates the level of detail of the data.",
        <http://purl.obolibrary.org/obo/IAO_0000233> "issue: https://github.com/OpenEnergyPlatform/ontology/issues/849
pull request: https://github.com/OpenEnergyPlatform/ontology/pull/972",
        rdfs:label "resolution"
    
    SubClassOf: 
        <http://purl.obolibrary.org/obo/BFO_0000019>
    
    
Class: OEO_00020122

    Annotations: 
        OEO_00040001 "http://openenergy-platform.org/ontology/oeo/oeo-shared"^^xsd:string,
        <http://purl.obolibrary.org/obo/IAO_0000115> "Temporal resolution is the resolution of a time series that indicates time-dependent the level of detail.",
        <http://purl.obolibrary.org/obo/IAO_0000233> "issue: https://github.com/OpenEnergyPlatform/ontology/issues/849
pull request: https://github.com/OpenEnergyPlatform/ontology/pull/912
add individuals
pull request: https://github.com/OpenEnergyPlatform/ontology/pull/972",
        rdfs:label "temporal resolution"
    
    SubClassOf: 
        OEO_00020121
    
    DisjointWith: 
        OEO_00020123
    
    
Class: OEO_00020123

    Annotations: 
        OEO_00040001 "http://openenergy-platform.org/ontology/oeo/oeo-shared"^^xsd:string,
        <http://purl.obolibrary.org/obo/IAO_0000115> "Spatial resolution is the resolution of a georeferenced dataset that indicates the geographical level of detail.",
        <http://purl.obolibrary.org/obo/IAO_0000233> "issue: https://github.com/OpenEnergyPlatform/ontology/issues/849
pull request: https://github.com/OpenEnergyPlatform/ontology/pull/912",
        rdfs:label "spatial resolution"
    
    SubClassOf: 
        OEO_00020121
    
    DisjointWith: 
        OEO_00020122
    
    
Class: OEO_00020136

    Annotations: 
        OEO_00040001 "http://openenergy-platform.org/ontology/oeo/oeo-shared"^^xsd:string,
        <http://purl.obolibrary.org/obo/IAO_0000115> "A space requirement is a two-dimensional spatial region that covers the area needed by an object or object aggregate.",
        <http://purl.obolibrary.org/obo/IAO_0000118> "land use",
        <http://purl.obolibrary.org/obo/IAO_0000233> "issue: https://github.com/OpenEnergyPlatform/ontology/issues/889
pull request: https://github.com/OpenEnergyPlatform/ontology/pull/933

extend definition and add alternative term
issue: https://github.com/OpenEnergyPlatform/ontology/issues/1051
pull request: https://github.com/OpenEnergyPlatform/ontology/pull/1084",
        rdfs:label "space requirement"
    
    SubClassOf: 
        <http://purl.obolibrary.org/obo/BFO_0000009>
    
    
Class: OEO_00020140

    Annotations: 
        OEO_00040001 "http://openenergy-platform.org/ontology/oeo/oeo-shared"^^xsd:string,
        <http://purl.obolibrary.org/obo/IAO_0000115> "An area per power unit is a unit which is a measure for an area per nameplate capacity.",
        <http://purl.obolibrary.org/obo/IAO_0000233> "issue: https://github.com/OpenEnergyPlatform/ontology/issues/889
pull request: https://github.com/OpenEnergyPlatform/ontology/pull/930",
        rdfs:label "area per power unit"
    
    SubClassOf: 
        <http://purl.obolibrary.org/obo/UO_0000000>
    
    
Class: OEO_00020142

    Annotations: 
        OEO_00040001 "http://openenergy-platform.org/ontology/oeo/oeo-shared"^^xsd:string,
        <http://purl.obolibrary.org/obo/IAO_0000115> "An area unit which is equal to one million square meters or 10^[6] m^[2].",
        <http://purl.obolibrary.org/obo/IAO_0000118> "km^[2]",
        <http://purl.obolibrary.org/obo/IAO_0000118> "square km",
        <http://purl.obolibrary.org/obo/IAO_0000233> "issue: https://github.com/OpenEnergyPlatform/ontology/issues/889
pull request: https://github.com/OpenEnergyPlatform/ontology/pull/933",
        rdfs:label "square kilometer"
    
    SubClassOf: 
        <http://purl.obolibrary.org/obo/UO_0000047>
    
    
Class: OEO_00020143

    Annotations: 
        OEO_00040001 "http://openenergy-platform.org/ontology/oeo/oeo-shared"^^xsd:string,
        <http://purl.obolibrary.org/obo/IAO_0000115> "An area value is a quantity value indicating the size of a two-dimensional spatial region.",
        <http://purl.obolibrary.org/obo/IAO_0000233> "issue: https://github.com/OpenEnergyPlatform/ontology/issues/889
pull request: https://github.com/OpenEnergyPlatform/ontology/pull/933",
        rdfs:label "area value"
    
    SubClassOf: 
        OEO_00000350,
        OEO_00020056 some <http://purl.obolibrary.org/obo/BFO_0000009>,
        OEO_00040010 some <http://purl.obolibrary.org/obo/UO_0000047>
    
    
Class: OEO_00020154

    Annotations: 
        OEO_00040001 "http://openenergy-platform.org/ontology/oeo/oeo-shared"^^xsd:string,
        <http://purl.obolibrary.org/obo/IAO_0000115> "Emission certificate price is a monetary price of an emission certificate that allows the emission of a certain emission value.",
        <http://purl.obolibrary.org/obo/IAO_0000118> "CO2 price",
        <http://purl.obolibrary.org/obo/IAO_0000233> "issue: https://github.com/OpenEnergyPlatform/ontology/issues/866
pull request: https://github.com/OpenEnergyPlatform/ontology/pull/956
add relation to emission certificate
pull request: https://github.com/OpenEnergyPlatform/ontology/pull/1034",
        rdfs:label "emission certificate price"
    
    SubClassOf: 
        OEO_00040003,
        OEO_00020179 some OEO_00020063
    
    
Class: OEO_00020155

    Annotations: 
        OEO_00040001 "http://openenergy-platform.org/ontology/oeo/oeo-shared"^^xsd:string,
        <http://purl.obolibrary.org/obo/IAO_0000115> "Social cost of carbon emission is the cost the society bears for a greenhouse gas emission value.",
        <http://purl.obolibrary.org/obo/IAO_0000118> "social cost of CO2",
        <http://purl.obolibrary.org/obo/IAO_0000233> "issue: https://github.com/OpenEnergyPlatform/ontology/issues/866
pull request: https://github.com/OpenEnergyPlatform/ontology/pull/956
add axiom to emission value, add new parent class and relable
pull request: https://github.com/OpenEnergyPlatform/ontology/pull/1034",
        rdfs:label "social cost of carbon emission"
    
    SubClassOf: 
        OEO_00020181,
        OEO_00020179 some OEO_00140081,
        <http://purl.obolibrary.org/obo/IAO_0000136> some OEO_00140081
    
    
Class: OEO_00020175

    Annotations: 
        OEO_00040001 "http://openenergy-platform.org/ontology/oeo/oeo-shared"^^xsd:string,
        <http://purl.obolibrary.org/obo/IAO_0000115> "A life time is a time span of an artificial object that measures the time during which the artificial object exists.",
        <http://purl.obolibrary.org/obo/IAO_0000233> "issue: https://github.com/OpenEnergyPlatform/ontology/issues/894
pull request: https://github.com/OpenEnergyPlatform/ontology/pull/1026",
        rdfs:label "life time"
    
    SubClassOf: 
        OEO_00030035,
        OEO_00020056 some OEO_00000061
    
    
Class: OEO_00020176

    Annotations: 
        OEO_00040001 "http://openenergy-platform.org/ontology/oeo/oeo-shared"^^xsd:string,
        <http://purl.obolibrary.org/obo/IAO_0000115> "A construction time is a time span that measures the time that is needed to construct an artificial object.",
        <http://purl.obolibrary.org/obo/IAO_0000233> "issue: https://github.com/OpenEnergyPlatform/ontology/issues/894
pull request: https://github.com/OpenEnergyPlatform/ontology/pull/1026",
        rdfs:label "construction time"
    
    SubClassOf: 
        OEO_00030035,
        OEO_00020056 some OEO_00000061
    
    
Class: OEO_00020177

    Annotations: 
        OEO_00040001 "http://openenergy-platform.org/ontology/oeo/oeo-shared"^^xsd:string,
        <http://purl.obolibrary.org/obo/IAO_0000115> "A decommissioning time is a time span that measures the time that is needed to decommission an artificial object.",
        <http://purl.obolibrary.org/obo/IAO_0000233> "issue: https://github.com/OpenEnergyPlatform/ontology/issues/894
pull request: https://github.com/OpenEnergyPlatform/ontology/pull/1026",
        rdfs:label "decommissioning time"
    
    SubClassOf: 
        OEO_00030035,
        OEO_00020056 some OEO_00000061
    
    
Class: OEO_00020178

    Annotations: 
        OEO_00040001 "http://openenergy-platform.org/ontology/oeo/oeo-shared"^^xsd:string,
        <http://purl.obolibrary.org/obo/IAO_0000115> "An operational life time is the lifetime of an artificial object. It is measured from the end of construction time to the start of decommissioning time.",
        <http://purl.obolibrary.org/obo/IAO_0000233> "issue: https://github.com/OpenEnergyPlatform/ontology/issues/894
pull request: https://github.com/OpenEnergyPlatform/ontology/pull/1026",
        rdfs:label "operational life time"
    
    SubClassOf: 
        OEO_00020175
    
    
Class: OEO_00020181

    Annotations: 
        OEO_00040001 "http://openenergy-platform.org/ontology/oeo/oeo-shared"^^xsd:string,
        <http://purl.obolibrary.org/obo/IAO_0000115> "Social cost of emission is the cost the society bears for an emission value.",
        <http://purl.obolibrary.org/obo/IAO_0000233> "issue: https://github.com/OpenEnergyPlatform/ontology/issues/958
pull request: https://github.com/OpenEnergyPlatform/ontology/pull/1034",
        rdfs:label "social cost of emission"
    
    SubClassOf: 
        OEO_00040009,
        OEO_00020179 some OEO_00140081,
        <http://purl.obolibrary.org/obo/IAO_0000136> some OEO_00140081
    
    
Class: OEO_00020185

    Annotations: 
        OEO_00040001 "http://openenergy-platform.org/ontology/oeo/oeo-shared"^^xsd:string,
        <http://purl.obolibrary.org/obo/IAO_0000115> "A copyright license is a license that states the ownership and contractually sets the rights and obligations to use, copy, and distribute a creative work.",
        <http://purl.obolibrary.org/obo/IAO_0000233> "add relation has copyright license",
        <http://purl.obolibrary.org/obo/IAO_0000233> "issue https://github.com/OpenEnergyPlatform/ontology/issues/1061
pull request https://github.com/OpenEnergyPlatform/ontology/pull/1090",
        rdfs:label "copyright license"
    
    SubClassOf: 
        OEO_00020015
    
    
Class: OEO_00020186

    Annotations: 
        OEO_00040001 "http://openenergy-platform.org/ontology/oeo/oeo-shared"^^xsd:string,
        <http://purl.obolibrary.org/obo/IAO_0000115> "A data license is a license that determines ownership, database protection, and permissions for data.",
        <http://purl.obolibrary.org/obo/IAO_0000233> "issue https://github.com/OpenEnergyPlatform/ontology/issues/1061
pull request https://github.com/OpenEnergyPlatform/ontology/pull/1090",
        rdfs:label "data license"
    
    SubClassOf: 
        OEO_00020015
    
    
Class: OEO_00020187

    Annotations: 
        OEO_00040001 "http://openenergy-platform.org/ontology/oeo/oeo-shared"^^xsd:string,
        <http://purl.obolibrary.org/obo/IAO_0000115> "A software license is a copyright license that determines ownership and permissions for software, code, or models.",
        <http://purl.obolibrary.org/obo/IAO_0000233> "issue https://github.com/OpenEnergyPlatform/ontology/issues/1061
pull request https://github.com/OpenEnergyPlatform/ontology/pull/1090",
        rdfs:label "software license"
    
    SubClassOf: 
        
            Annotations: <http://purl.obolibrary.org/obo/IAO_0000233> "fix wrong classification
issue: https://github.com/OpenEnergyPlatform/ontology/issues/1153
pull request: https://github.com/OpenEnergyPlatform/ontology/pull/1163"
        OEO_00020185
    
    
Class: OEO_00020201

    Annotations: 
        OEO_00040001 "http://openenergy-platform.org/ontology/oeo/oeo-shared"^^xsd:string,
        <http://purl.obolibrary.org/obo/IAO_0000115> "Import is the process of purchasing goods or services abroad and their delivery to the domestic market.",
        <http://purl.obolibrary.org/obo/IAO_0000233> "add class
issue: https://github.com/OpenEnergyPlatform/ontology/issues/998
pull request: https://github.com/OpenEnergyPlatform/ontology/pull/1221",
        rdfs:label "import"
    
    SubClassOf: 
        <http://purl.obolibrary.org/obo/BFO_0000015>
    
    
Class: OEO_00020202

    Annotations: 
        OEO_00040001 "http://openenergy-platform.org/ontology/oeo/oeo-shared"^^xsd:string,
        <http://purl.obolibrary.org/obo/IAO_0000115> "Export is the process of selling goods or services abroad and their delivery to a foreign market.",
        <http://purl.obolibrary.org/obo/IAO_0000233> "add class
issue: https://github.com/OpenEnergyPlatform/ontology/issues/998
pull request: https://github.com/OpenEnergyPlatform/ontology/pull/1221",
        rdfs:label "export"
    
    SubClassOf: 
        <http://purl.obolibrary.org/obo/BFO_0000015>
    
    
Class: OEO_00020204

    Annotations: 
        OEO_00040001 "http://openenergy-platform.org/ontology/oeo/oeo-shared"^^xsd:string,
        <http://purl.obolibrary.org/obo/IAO_0000115> "An electrical energy amount value is an energy amount value that measures a quantity of electrical energy.",
        <http://purl.obolibrary.org/obo/IAO_0000233> "issue: https://github.com/OpenEnergyPlatform/ontology/issues/998
pull request: https://github.com/OpenEnergyPlatform/ontology/pull/1221",
        rdfs:label "electrical energy amount value"
    
    SubClassOf: 
        OEO_00050019
    
    
Class: OEO_00020205

    Annotations: 
        OEO_00040001 "http://openenergy-platform.org/ontology/oeo/oeo-shared"^^xsd:string,
        <http://purl.obolibrary.org/obo/IAO_0000115> "An electricity export value is an electrical energy amount value that measures the export of electrical energy.",
        <http://purl.obolibrary.org/obo/IAO_0000233> "issue: https://github.com/OpenEnergyPlatform/ontology/issues/998
pull request: https://github.com/OpenEnergyPlatform/ontology/pull/1221",
        rdfs:label "electricity import value"
    
    SubClassOf: 
        OEO_00020204,
        <http://purl.obolibrary.org/obo/IAO_0000136> some OEO_00020207
    
    
Class: OEO_00020206

    Annotations: 
        OEO_00040001 "http://openenergy-platform.org/ontology/oeo/oeo-shared"^^xsd:string,
        <http://purl.obolibrary.org/obo/IAO_0000115> "An electricity import value is an electrical energy amount value that measures the import of electrical energy.",
        <http://purl.obolibrary.org/obo/IAO_0000233> "issue: https://github.com/OpenEnergyPlatform/ontology/issues/998
pull request: https://github.com/OpenEnergyPlatform/ontology/pull/1221",
        rdfs:label "electricity export value"
    
    SubClassOf: 
        OEO_00020204,
        <http://purl.obolibrary.org/obo/IAO_0000136> some OEO_00020208
    
    
Class: OEO_00020207

    Annotations: 
        OEO_00040001 "http://openenergy-platform.org/ontology/oeo/oeo-shared"^^xsd:string,
        <http://purl.obolibrary.org/obo/IAO_0000115> "Electricity import is the import of electrical energy.",
        <http://purl.obolibrary.org/obo/IAO_0000233> "add class
issue: https://github.com/OpenEnergyPlatform/ontology/issues/998
pull request: https://github.com/OpenEnergyPlatform/ontology/pull/1221",
        rdfs:label "electricity import"
    
    SubClassOf: 
        OEO_00020201,
        OEO_00140002 some OEO_00020205
    
    
Class: OEO_00020208

    Annotations: 
        OEO_00040001 "http://openenergy-platform.org/ontology/oeo/oeo-shared"^^xsd:string,
        <http://purl.obolibrary.org/obo/IAO_0000115> "Electricity export is the export of electrical energy.",
        <http://purl.obolibrary.org/obo/IAO_0000233> "add class
issue: https://github.com/OpenEnergyPlatform/ontology/issues/998
pull request: https://github.com/OpenEnergyPlatform/ontology/pull/1221",
        rdfs:label "electricity export"
    
    SubClassOf: 
        OEO_00020202,
        OEO_00140002 some OEO_00020206
    
    
Class: OEO_00030015

    Annotations: 
        OEO_00040001 "http://openenergy-platform.org/ontology/oeo/oeo-shared"^^xsd:string,
        <http://purl.obolibrary.org/obo/IAO_0000115> "An energy system model is a model of an energy system.",
        <http://purl.obolibrary.org/obo/IAO_0000233> "issue: https://github.com/OpenEnergyPlatform/ontology/issues/337
pull request: https://github.com/OpenEnergyPlatform/ontology/pull/358",
        rdfs:label "energy system model"@en
    
    SubClassOf: 
        OEO_00000274
    
    
Class: OEO_00030019

    Annotations: 
        OEO_00040001 "http://openenergy-platform.org/ontology/oeo/oeo-shared"^^xsd:string,
        <http://purl.obolibrary.org/obo/IAO_0000115> "A process attribute is a dependent occurrent that existentially depends on a process.",
        <http://purl.obolibrary.org/obo/IAO_0000233> "issue: https://github.com/OpenEnergyPlatform/ontology/issues/205
pull request: https://github.com/OpenEnergyPlatform/ontology/pull/386",
        rdfs:label "process attribute"
    
    SubClassOf: 
        <http://purl.obolibrary.org/obo/BFO_0000003>
    
    
Class: OEO_00030022

    Annotations: 
        OEO_00040001 "http://openenergy-platform.org/ontology/oeo/oeo-shared"^^xsd:string,
        <http://purl.obolibrary.org/obo/IAO_0000115> "An organisation is an immaterial entity that has the organisation role and there exists some sort of legal framework that recognises the entity and its continued existence.",
        <http://purl.obolibrary.org/obo/IAO_0000118> "organization",
        <http://purl.obolibrary.org/obo/IAO_0000233> "issue: https://github.com/OpenEnergyPlatform/ontology/issues/416
pull request: https://github.com/OpenEnergyPlatform/ontology/pull/421
added term in oeo-shared:
pull request: https://github.com/OpenEnergyPlatform/ontology/pull/871
deleted term in oeo-social:
issue: https://github.com/OpenEnergyPlatform/ontology/issues/983
pull request: https://github.com/OpenEnergyPlatform/ontology/pull/992",
        rdfs:label "organisation"
    
    SubClassOf: 
        <http://purl.obolibrary.org/obo/BFO_0000141>,
        <http://purl.obolibrary.org/obo/RO_0000087> some OEO_00000315
    
    
Class: OEO_00030029

    Annotations: 
        OEO_00040001 "http://openenergy-platform.org/ontology/oeo/oeo-shared"^^xsd:string,
        <http://purl.obolibrary.org/obo/IAO_0000115> "Exogenous data is a data item whose quantity value is determined outside of a model and is imposed on a model.",
        <http://purl.obolibrary.org/obo/IAO_0000118> "input data",
        <http://purl.obolibrary.org/obo/IAO_0000233> "issue: https://github.com/OpenEnergyPlatform/ontology/issues/482
pull request: https://github.com/OpenEnergyPlatform/ontology/pull/500

make equivalent class
pull request: https://github.com/OpenEnergyPlatform/ontology/pull/1113

add relation to quantity value:
pull request: https://github.com/OpenEnergyPlatform/ontology/pull/1216",
        rdfs:label "exogenous data"
    
    EquivalentTo: 
        <http://purl.obolibrary.org/obo/IAO_0000027>
         and (OEO_00020189 some OEO_00000275)
    
    SubClassOf: 
        <http://purl.obolibrary.org/obo/IAO_0000027>,
        <http://purl.obolibrary.org/obo/IAO_0000136> some OEO_00000350
    
    
Class: OEO_00030030

    Annotations: 
        OEO_00040001 "http://openenergy-platform.org/ontology/oeo/oeo-shared"^^xsd:string,
        <http://purl.obolibrary.org/obo/IAO_0000115> "Endogenous data is a data item whose quantity value is determined by a model.",
        <http://purl.obolibrary.org/obo/IAO_0000233> "issue: https://github.com/OpenEnergyPlatform/ontology/issues/482
pull request: https://github.com/OpenEnergyPlatform/ontology/pull/500

make equivalent class
pull request: https://github.com/OpenEnergyPlatform/ontology/pull/1113

add relation to quantity value:
pull request: https://github.com/OpenEnergyPlatform/ontology/pull/1216",
        rdfs:label "endogenous data"
    
    EquivalentTo: 
        <http://purl.obolibrary.org/obo/IAO_0000027>
         and (OEO_00020190 some OEO_00000275)
    
    SubClassOf: 
        <http://purl.obolibrary.org/obo/IAO_0000027>,
        <http://purl.obolibrary.org/obo/IAO_0000136> some OEO_00000350
    
    
Class: OEO_00030031

    Annotations: 
        OEO_00040001 "http://openenergy-platform.org/ontology/oeo/oeo-shared"^^xsd:string,
        <http://purl.obolibrary.org/obo/IAO_0000115> "A start time is a zero-dimensional temporal region that indicates the beginning of a one-dimensional temporal region.",
        <http://purl.obolibrary.org/obo/IAO_0000233> "issue: https://github.com/OpenEnergyPlatform/ontology/issues/267
pull request: https://github.com/OpenEnergyPlatform/ontology/pull/538",
        rdfs:label "start time"
    
    SubClassOf: 
        <http://purl.obolibrary.org/obo/BFO_0000148>
    
    
Class: OEO_00030032

    Annotations: 
        OEO_00040001 "http://openenergy-platform.org/ontology/oeo/oeo-shared"^^xsd:string,
        <http://purl.obolibrary.org/obo/IAO_0000115> "An ending time is a zero-dimensional temporal region that indicates the end of a one-dimensional temporal region.",
        <http://purl.obolibrary.org/obo/IAO_0000233> "issue: https://github.com/OpenEnergyPlatform/ontology/issues/267
pull request: https://github.com/OpenEnergyPlatform/ontology/pull/538",
        rdfs:label "ending time"
    
    SubClassOf: 
        <http://purl.obolibrary.org/obo/BFO_0000148>
    
    
Class: OEO_00030035

    Annotations: 
        OEO_00040001 "http://openenergy-platform.org/ontology/oeo/oeo-shared"^^xsd:string,
        <http://purl.obolibrary.org/obo/IAO_0000115> "A time span is a quantity value indicating the duration of a one-dimensional temporal region, measured in a time unit.",
        <http://purl.obolibrary.org/obo/IAO_0000118> "duration",
        <http://purl.obolibrary.org/obo/IAO_0000233> "issue: https://github.com/OpenEnergyPlatform/ontology/issues/267
pull request: https://github.com/OpenEnergyPlatform/ontology/pull/538
change duration to time span (def, label, alternative term)
pull request: https://github.com/OpenEnergyPlatform/ontology/pull/1017",
        rdfs:label "time span"
    
    SubClassOf: 
        OEO_00000350,
        OEO_00020056 some <http://purl.obolibrary.org/obo/BFO_0000038>,
        OEO_00040010 some <http://purl.obolibrary.org/obo/UO_0000003>
    
    
Class: OEO_00040003

    Annotations: 
        OEO_00040001 "http://openenergy-platform.org/ontology/oeo/oeo-shared"^^xsd:string,
        <http://purl.obolibrary.org/obo/IAO_0000115> "A monetary price is an economic value that describes the amount of money requested, expected, required or given in exchange for something else.",
        <http://purl.obolibrary.org/obo/IAO_0000119> "fibo-fnd-acc-cur:MonetaryPrice",
        <http://purl.obolibrary.org/obo/IAO_0000233> "issue: https://github.com/OpenEnergyPlatform/ontology/issues/331
pull request: https://github.com/OpenEnergyPlatform/ontology/pull/640
move to oeo-shared
pull request: https://github.com/OpenEnergyPlatform/ontology/pull/956
add relation to good
pull request: https://github.com/OpenEnergyPlatform/ontology/pull/1034",
        rdfs:label "monetary price"@en,
        rdfs:seeAlso "https://spec.edmcouncil.org/fibo/ontology/FND/Accounting/CurrencyAmount/MonetaryPrice"
    
    SubClassOf: 
        OEO_00140012,
        OEO_00020179 some OEO_00010117,
        OEO_00040010 some OEO_00040004
    
    
Class: OEO_00040004

    Annotations: 
        OEO_00040001 "http://openenergy-platform.org/ontology/oeo/oeo-shared"^^xsd:string,
        <http://purl.obolibrary.org/obo/IAO_0000112> "The currency used in France in 2020 was Euro.",
        <http://purl.obolibrary.org/obo/IAO_0000115> "A unit which is a measure of the medium of an exchange value, defined by reference to the geographical location of the monetary authorities responsible for it.",
        <http://purl.obolibrary.org/obo/IAO_0000119> "fibo-fnd-acc-cur:Currency",
        <http://purl.obolibrary.org/obo/IAO_0000233> "https://github.com/OpenEnergyPlatform/ontology/issues/331
https://github.com/OpenEnergyPlatform/ontology/pull/640
add comment and example
https://github.com/OpenEnergyPlatform/ontology/pull/910
moved to oeo-shared
https://github.com/OpenEnergyPlatform/ontology/pull/956",
        rdfs:comment "Currency is the unit of monetary value as defined by each country.",
        rdfs:label "currency"@en,
        rdfs:seeAlso "https://spec.edmcouncil.org/fibo/ontology/FND/Accounting/CurrencyAmount/Currency"
    
    SubClassOf: 
        <http://purl.obolibrary.org/obo/UO_0000000>
    
    
Class: OEO_00040009

    Annotations: 
        OEO_00040001 "http://openenergy-platform.org/ontology/oeo/oeo-shared"^^xsd:string,
        <http://purl.obolibrary.org/obo/IAO_0000115> "Cost is an economic value that describes the amount of money needed to buy, make, or do a thing.",
        <http://purl.obolibrary.org/obo/IAO_0000119> "https://dictionary.cambridge.org/dictionary/english/cost",
        <http://purl.obolibrary.org/obo/IAO_0000233> "issue: https://github.com/OpenEnergyPlatform/ontology/issues/268
pull request: https://github.com/OpenEnergyPlatform/ontology/pull/643
move to oeo-shared
pull request: https://github.com/OpenEnergyPlatform/ontology/pull/956
delete cost in oeo-social
issue: https://github.com/OpenEnergyPlatform/ontology/issues/975
pull request: https://github.com/OpenEnergyPlatform/ontology/pull/977",
        rdfs:label "cost"@en
    
    SubClassOf: 
        OEO_00140012,
        OEO_00040010 some OEO_00040004
    
    
Class: OEO_00040011

    Annotations: 
        OEO_00040001 "http://openenergy-platform.org/ontology/oeo/oeo-shared"^^xsd:string,
        <http://purl.obolibrary.org/obo/IAO_0000115> "A commodity role is a good role that inheres in something that is used in commerce and is exchangeable with other commodities of the same type.",
        <http://purl.obolibrary.org/obo/IAO_0000119> "fibo-fnd-pas-pas:Commodity",
        <http://purl.obolibrary.org/obo/IAO_0000233> "https://github.com/OpenEnergyPlatform/ontology/issues/339
https://github.com/OpenEnergyPlatform/ontology/pull/644
moved to oeo-shared and renamed
https://github.com/OpenEnergyPlatform/ontology/pull/748
made subclass of good role
pull request: https://github.com/OpenEnergyPlatform/ontology/pull/843",
        rdfs:label "commodity role"@en,
        rdfs:seeAlso "https://spec.edmcouncil.org/fibo/ontology/FND/ProductsAndServices/ProductsAndServices/Commodity"
    
    SubClassOf: 
        OEO_00010117
    
    
Class: OEO_00050016

    Annotations: 
        OEO_00040001 "http://openenergy-platform.org/ontology/oeo/oeo-shared"^^xsd:string,
        <http://purl.obolibrary.org/obo/IAO_0000115> "Final energy consumption is the consumption of energy delivered to and consumed by end users."@en,
        <http://purl.obolibrary.org/obo/IAO_0000233> "issue: https://github.com/OpenEnergyPlatform/ontology/issues/576
pull request: https://github.com/OpenEnergyPlatform/ontology/pull/613",
        rdfs:label "final energy consumption"@en
    
    SubClassOf: 
        OEO_00140039
    
    
Class: OEO_00050019

    Annotations: 
        OEO_00040001 "http://openenergy-platform.org/ontology/oeo/oeo-shared"^^xsd:string,
        <http://purl.obolibrary.org/obo/IAO_0000115> "An energy amount value is a quantity value that has an energy unit as unit."@en,
        <http://purl.obolibrary.org/obo/IAO_0000118> "energy quantity value",
        <http://purl.obolibrary.org/obo/IAO_0000233> "issue: https://github.com/OpenEnergyPlatform/ontology/issues/576
pull request: https://github.com/OpenEnergyPlatform/ontology/pull/613
moved to oeo-shared
issue: https://github.com/OpenEnergyPlatform/ontology/issues/998
pull request: https://github.com/OpenEnergyPlatform/ontology/pull/1221",
        rdfs:label "energy amount value"@en
    
    SubClassOf: 
        OEO_00000350,
        OEO_00040010 some <http://purl.obolibrary.org/obo/UO_0000111>
    
    
Class: OEO_00090001

    Annotations: 
        OEO_00040001 "http://openenergy-platform.org/ontology/oeo/oeo-shared"^^xsd:string,
        <http://purl.obolibrary.org/obo/IAO_0000115> "A funder is a sponsor that supports by giving money.",
        <http://purl.obolibrary.org/obo/IAO_0000233> "issue: https://github.com/OpenEnergyPlatform/ontology/issues/246
pull request: https://github.com/OpenEnergyPlatform/ontology/pull/776",
        rdfs:label "funder"@en
    
    SubClassOf: 
        OEO_00140009
    
    
Class: OEO_00140003

    Annotations: 
        OEO_00040001 "http://openenergy-platform.org/ontology/oeo/oeo-shared"^^xsd:string,
        <http://purl.obolibrary.org/obo/IAO_0000115> "Transport is the process of moving people or goods from one place to another.",
        <http://purl.obolibrary.org/obo/IAO_0000233> "issue: https://github.com/OpenEnergyPlatform/ontology/issues/503
pull request: https://github.com/OpenEnergyPlatform/ontology/pull/517",
        rdfs:label "transport"@en,
        
            Annotations: <http://purl.obolibrary.org/obo/IAO_0000233> "issue: https://github.com/OpenEnergyPlatform/ontology/issues/636
pull request: https://github.com/OpenEnergyPlatform/ontology/pull/810"
        owl:equivalentClass "http://purl.obolibrary.org/obo/ENVO_02000125"
    
    SubClassOf: 
        <http://purl.obolibrary.org/obo/BFO_0000015>
    
    
Class: OEO_00140004

    Annotations: 
        OEO_00040001 "http://openenergy-platform.org/ontology/oeo/oeo-shared"^^xsd:string,
        <http://purl.obolibrary.org/obo/IAO_0000115> "International transport is a transport process between different countries or within the same country via another country.",
        <http://purl.obolibrary.org/obo/IAO_0000233> "issue: https://github.com/OpenEnergyPlatform/ontology/issues/503
pull request: https://github.com/OpenEnergyPlatform/ontology/pull/517",
        rdfs:label "international transport"@en
    
    SubClassOf: 
        OEO_00140003
    
    
Class: OEO_00140005

    Annotations: 
        OEO_00040001 "http://openenergy-platform.org/ontology/oeo/oeo-shared"^^xsd:string,
        <http://purl.obolibrary.org/obo/IAO_0000115> "Freight transport is a transport process which moves goods from one place to another.",
        <http://purl.obolibrary.org/obo/IAO_0000233> "issue: https://github.com/OpenEnergyPlatform/ontology/issues/503
pull request: https://github.com/OpenEnergyPlatform/ontology/pull/517",
        rdfs:label "freight transport"@en
    
    SubClassOf: 
        OEO_00140003
    
    
Class: OEO_00140006

    Annotations: 
        OEO_00040001 "http://openenergy-platform.org/ontology/oeo/oeo-shared"^^xsd:string,
        <http://purl.obolibrary.org/obo/IAO_0000115> "A private transport is a passenger transport in which people use their own vehicle for movement e.g. bicycle, motorcycle and cars.",
        <http://purl.obolibrary.org/obo/IAO_0000233> "issue: https://github.com/OpenEnergyPlatform/ontology/issues/503
pull request: https://github.com/OpenEnergyPlatform/ontology/pull/517

Make subclass of 'passenger transport'
issue: https://github.com/OpenEnergyPlatform/ontology/issues/1055
pull request: https://github.com/OpenEnergyPlatform/ontology/pull/1234",
        rdfs:label "private transport"
    
    SubClassOf: 
        OEO_00010263
    
    
Class: OEO_00140007

    Annotations: 
        OEO_00040001 "http://openenergy-platform.org/ontology/oeo/oeo-shared"^^xsd:string,
        <http://purl.obolibrary.org/obo/IAO_0000115> "A public transport is a passenger transport in which a number of passengers share a common vehicle.",
        <http://purl.obolibrary.org/obo/IAO_0000233> "issue: https://github.com/OpenEnergyPlatform/ontology/issues/503
pull request: https://github.com/OpenEnergyPlatform/ontology/pull/517

Make subclass of 'passenger transport'
issue: https://github.com/OpenEnergyPlatform/ontology/issues/1055
pull request: https://github.com/OpenEnergyPlatform/ontology/pull/1234",
        rdfs:label "public transport"
    
    SubClassOf: 
        OEO_00010263
    
    
Class: OEO_00140009

    Annotations: 
        OEO_00040001 "http://openenergy-platform.org/ontology/oeo/oeo-shared"^^xsd:string,
        <http://purl.obolibrary.org/obo/IAO_0000115> "A sponsor is an agent that supports a person, organisation, or project by giving money, allowance of kind, services or other help.",
        <http://purl.obolibrary.org/obo/IAO_0000233> "issue: https://github.com/OpenEnergyPlatform/ontology/issues/473
pull request: https://github.com/OpenEnergyPlatform/ontology/pull/557",
        rdfs:label "sponsor"@en
    
    SubClassOf: 
        OEO_00000051
    
    
Class: OEO_00140012

    Annotations: 
        OEO_00040001 "http://openenergy-platform.org/ontology/oeo/oeo-shared"^^xsd:string,
        <http://purl.obolibrary.org/obo/IAO_0000115> "An economic value is a quantity value that is economically relevant.",
        <http://purl.obolibrary.org/obo/IAO_0000233> "issue: https://github.com/OpenEnergyPlatform/ontology/issues/454
pull request: https://github.com/OpenEnergyPlatform/ontology/pull/559
move to oeo-shared
pull request: https://github.com/OpenEnergyPlatform/ontology/pull/956",
        rdfs:label "economic value"@en
    
    SubClassOf: 
        OEO_00000350
    
    
Class: OEO_00140039

    Annotations: 
        OEO_00040001 "http://openenergy-platform.org/ontology/oeo/oeo-shared"^^xsd:string,
        <http://purl.obolibrary.org/obo/IAO_0000115> "Consumption is the process of using something and thereby reducing its amount.",
        <http://purl.obolibrary.org/obo/IAO_0000233> "issue: https://github.com/OpenEnergyPlatform/ontology/issues/140
pull request: https://github.com/OpenEnergyPlatform/ontology/pull/569",
        rdfs:label "consumption"@en
    
    SubClassOf: 
        <http://purl.obolibrary.org/obo/BFO_0000015>
    
    
Class: OEO_00140040

    Annotations: 
        OEO_00040001 "http://openenergy-platform.org/ontology/oeo/oeo-shared"^^xsd:string,
        <http://purl.obolibrary.org/obo/IAO_0000115> "A demand is a realizable entity that is characterised by a person, organisation or object needing it for a specific purpose.",
        <http://purl.obolibrary.org/obo/IAO_0000233> "issue: https://github.com/OpenEnergyPlatform/ontology/issues/140
pull request: https://github.com/OpenEnergyPlatform/ontology/pull/569",
        rdfs:label "demand"@en
    
    SubClassOf: 
        <http://purl.obolibrary.org/obo/BFO_0000017>
    
    
Class: OEO_00140081

    Annotations: 
        OEO_00040001 "http://openenergy-platform.org/ontology/oeo/oeo-shared"^^xsd:string,
        <http://purl.obolibrary.org/obo/IAO_0000115> "An emission value is a process attribute that quantifies the output of an emission process. It can be calculated using the emission factor of that emission process.",
        <http://purl.obolibrary.org/obo/IAO_0000233> "class:
issue: https://github.com/OpenEnergyPlatform/ontology/issues/420
pull request: https://github.com/OpenEnergyPlatform/ontology/pull/651
has quantity value axiom:
issue: https://github.com/OpenEnergyPlatform/ontology/issues/695
pull request: https://github.com/OpenEnergyPlatform/ontology/pull/697
moved to oeo-shared
https://github.com/OpenEnergyPlatform/ontology/pull/956
add axiom to social cost of carbon
pull request: https://github.com/OpenEnergyPlatform/ontology/pull/1034",
        rdfs:label "emission value"@en
    
    SubClassOf: 
        OEO_00030019,
        OEO_00000502 some OEO_00000147,
        OEO_00020180 some OEO_00020181,
        OEO_00140002 some OEO_00010079
    
    
Class: OEO_00240003

    Annotations: 
        OEO_00040001 "http://openenergy-platform.org/ontology/oeo/oeo-shared"^^xsd:string,
        <http://purl.obolibrary.org/obo/IAO_0000115> "Production is the process of combining various inputs in order to create an output that has value and can be used by other processes."@en,
        <http://purl.obolibrary.org/obo/IAO_0000233> "issue: https://github.com/OpenEnergyPlatform/ontology/issues/835
pull request: https://github.com/OpenEnergyPlatform/ontology/pull/845",
        rdfs:label "production"
    
    SubClassOf: 
        <http://purl.obolibrary.org/obo/BFO_0000015>
    
    
Class: OEO_00240022

    Annotations: 
        OEO_00040001 "http://openenergy-platform.org/ontology/oeo/oeo-shared"^^xsd:string,
        <http://purl.obolibrary.org/obo/IAO_0000115> "A protected area is a two-dimensional spatial region recognised, dedicated and managed, through legal or other effective means, to achieve the long term conservation of nature with associated ecosystem services and cultural values."@en,
        <http://purl.obolibrary.org/obo/IAO_0000233> "issue: https://github.com/OpenEnergyPlatform/ontology/issues/1052
pull request: https://github.com/OpenEnergyPlatform/ontology/pull/1078"@en,
        rdfs:label "protected area"
    
    SubClassOf: 
        <http://purl.obolibrary.org/obo/BFO_0000009>
    
    
Class: OEO_00240024

    Annotations: 
        OEO_00040001 "http://openenergy-platform.org/ontology/oeo/oeo-shared"^^xsd:string,
        <http://purl.obolibrary.org/obo/IAO_0000115> "An energy service demand is a demand of an agent to use energy as a means to obtain or facilitate desired end services or states."@en,
        <http://purl.obolibrary.org/obo/IAO_0000116> "An example is the transport demand for goods or persons (e.g. in person/tonne-kilometres). An other example is the demand for room heating or cooling."@en,
        <http://purl.obolibrary.org/obo/IAO_0000233> "issue: https://github.com/OpenEnergyPlatform/ontology/issues/1054
pull request: https://github.com/OpenEnergyPlatform/ontology/pull/1080",
        rdfs:label "energy service demand"
    
    SubClassOf: 
        OEO_00140040,
        OEO_00010121 some (<http://purl.obolibrary.org/obo/RO_0000087> some OEO_00000051)
    
    
Class: OEO_00240038

    Annotations: 
        OEO_00040001 "http://openenergy-platform.org/ontology/oeo/oeo-shared"^^xsd:string,
        <http://purl.obolibrary.org/obo/IAO_0000115> "A personal living space is a space requirement that one person uses for living."@en,
        <http://purl.obolibrary.org/obo/IAO_0000233> "issue: https://github.com/OpenEnergyPlatform/ontology/issues/1056
pull request: https://github.com/OpenEnergyPlatform/ontology/pull/1084",
        rdfs:label "personal living space"
    
    SubClassOf: 
        OEO_00020136
    
    
Individual: OEO_00020161

    Annotations: 
        OEO_00040001 "http://openenergy-platform.org/ontology/oeo/oeo-shared"^^xsd:string,
        <http://purl.obolibrary.org/obo/IAO_0000115> "one value per year",
        rdfs:label "annual"
    
    Types: 
        OEO_00020122
    
    
Individual: OEO_00020162

    Annotations: 
        OEO_00040001 "http://openenergy-platform.org/ontology/oeo/oeo-shared"^^xsd:string,
        <http://purl.obolibrary.org/obo/IAO_0000115> "one value per week",
        rdfs:label "weekly"
    
    Types: 
        OEO_00020122
    
    
Individual: OEO_00020163

    Annotations: 
        OEO_00040001 "http://openenergy-platform.org/ontology/oeo/oeo-shared"^^xsd:string,
        <http://purl.obolibrary.org/obo/IAO_0000115> "one value per day",
        rdfs:label "daily"
    
    Types: 
        OEO_00020122
    
    
Individual: OEO_00020164

    Annotations: 
        OEO_00040001 "http://openenergy-platform.org/ontology/oeo/oeo-shared"^^xsd:string,
        <http://purl.obolibrary.org/obo/IAO_0000115> "one value per hour",
        rdfs:label "hourly"
    
    Types: 
        OEO_00020122
    
    
Individual: OEO_00020165

    Annotations: 
        OEO_00040001 "http://openenergy-platform.org/ontology/oeo/oeo-shared"^^xsd:string,
        <http://purl.obolibrary.org/obo/IAO_0000115> "one value per month",
        rdfs:label "monthly"
    
    Types: 
        OEO_00020122
    
    
