Prefix: : <http://openenergy-platform.org/ontology/oeo/>
Prefix: bfo: <http://purl.obolibrary.org/obo/bfo.owl#>
Prefix: dc: <http://purl.org/dc/elements/1.1/>
Prefix: obda: <https://w3id.org/obda/vocabulary#>
Prefix: owl: <http://www.w3.org/2002/07/owl#>
Prefix: rdf: <http://www.w3.org/1999/02/22-rdf-syntax-ns#>
Prefix: rdfs: <http://www.w3.org/2000/01/rdf-schema#>
Prefix: xml: <http://www.w3.org/XML/1998/namespace>
Prefix: xsd: <http://www.w3.org/2001/XMLSchema#>



Ontology: <http://openenergy-platform.org/ontology/oeo/oeo-social/>
<http://openenergy-platform.org/ontology/oeo/dev/oeo-social.omn>
Import: <http://openenergy-platform.org/ontology/oeo/dev/oeo-shared.omn>

Annotations: 
    dc:description "The Open Energy Ontology is an ontology for all aspects of the energy modelling domain. The 'Social' module covers entities that relate to people and the social, organisational and economic environment in which energy is produced and consumed, including sector, organisation, and various roles.",
    <http://purl.org/dc/terms/license> "http://creativecommons.org/publicdomain/zero/1.0/",
    <http://purl.org/dc/terms/title> "Open Energy Ontology (social module)"

AnnotationProperty: <http://purl.obolibrary.org/obo/IAO_0000112>

    
AnnotationProperty: <http://purl.obolibrary.org/obo/IAO_0000115>

    
AnnotationProperty: <http://purl.obolibrary.org/obo/IAO_0000116>

    
AnnotationProperty: <http://purl.obolibrary.org/obo/IAO_0000118>

    
AnnotationProperty: <http://purl.obolibrary.org/obo/IAO_0000119>

    
AnnotationProperty: <http://purl.obolibrary.org/obo/IAO_0000233>

    
AnnotationProperty: <http://purl.org/dc/terms/license>

    
AnnotationProperty: <http://purl.org/dc/terms/source>

    
AnnotationProperty: <http://purl.org/dc/terms/title>

    
AnnotationProperty: OEO_00010037

    
AnnotationProperty: dc:contributor

    
AnnotationProperty: dc:description

    
AnnotationProperty: dc:identifier

    
AnnotationProperty: rdfs:comment

    
AnnotationProperty: rdfs:isDefinedBy

    
AnnotationProperty: rdfs:label

    
AnnotationProperty: rdfs:seeAlso

    
Datatype: rdf:PlainLiteral

    
ObjectProperty: <http://purl.obolibrary.org/obo/BFO_0000050>

    
ObjectProperty: <http://purl.obolibrary.org/obo/BFO_0000051>

    
ObjectProperty: <http://purl.obolibrary.org/obo/IAO_0000136>

    
ObjectProperty: <http://purl.obolibrary.org/obo/RO_0000056>

    
ObjectProperty: <http://purl.obolibrary.org/obo/RO_0000057>

    
ObjectProperty: <http://purl.obolibrary.org/obo/RO_0000086>

    
ObjectProperty: <http://purl.obolibrary.org/obo/RO_0000087>

    
ObjectProperty: OEO_00000503

    
ObjectProperty: OEO_00000504

    Annotations: 
        <http://purl.obolibrary.org/obo/IAO_0000115> "A relation between a continuant (A) and a continuant or occurent (B) in which (A) determines the semantic of (B)",
        <http://purl.obolibrary.org/obo/IAO_0000233> "issue: https://github.com/OpenEnergyPlatform/ontology/issues/460
pull request: https://github.com/OpenEnergyPlatform/ontology/pull/480/

domain:
issue: https://github.com/OpenEnergyPlatform/ontology/issues/850
pull request: https://github.com/OpenEnergyPlatform/ontology/pull/871

adapt domains and ranges:
issue: https://github.com/OpenEnergyPlatform/ontology/issues/973
issue: https://github.com/OpenEnergyPlatform/ontology/pull/1085",
        rdfs:label "is defined by"
    
    Range: 
        <http://purl.obolibrary.org/obo/BFO_0000002>
    
    
ObjectProperty: OEO_00000505

    
ObjectProperty: OEO_00000506

    
ObjectProperty: OEO_00000507

    
ObjectProperty: OEO_00000508

    
ObjectProperty: OEO_00000509

    
ObjectProperty: OEO_00000510

    
ObjectProperty: OEO_00000522

    
ObjectProperty: OEO_00010119

    Annotations: 
        <http://purl.obolibrary.org/obo/IAO_0000115> "A relation between a policy instrument and a transformative measure where a policy instrument guides a transformative measure.",
        <http://purl.obolibrary.org/obo/IAO_0000233> "issue: https://github.com/OpenEnergyPlatform/ontology/issues/444
pull request: https://github.com/OpenEnergyPlatform/ontology/pull/853",
        rdfs:label "guides"@en
    
    SubPropertyOf: 
        <http://purl.obolibrary.org/obo/RO_0000056>
    
    Domain: 
        OEO_00140151
    
    Range: 
        OEO_00140149
    
    
ObjectProperty: OEO_00010121

    
ObjectProperty: OEO_00010128

    Annotations: 
        <http://purl.obolibrary.org/obo/IAO_0000115> "A relation that holds between a policy or policy instrument and the thing it governs.",
        <http://purl.obolibrary.org/obo/IAO_0000233> "issue: https://github.com/OpenEnergyPlatform/ontology/issues/855
pull request: https://github.com/OpenEnergyPlatform/ontology/pull/868",
        rdfs:label "governs"@en
    
    Domain: 
        OEO_00140150 or OEO_00140151
    
    
ObjectProperty: OEO_00010231

    
ObjectProperty: OEO_00010232

    Annotations: 
        <http://purl.obolibrary.org/obo/IAO_0000115> "A relation between a sector and a memo item.",
        <http://purl.obolibrary.org/obo/IAO_0000233> "issue: https://github.com/OpenEnergyPlatform/ontology/issues/858
pull request: https://github.com/OpenEnergyPlatform/ontology/pull/965",
        rdfs:label "has memo item"
    
    SubPropertyOf: 
        OEO_00010231
    
    Domain: 
        OEO_00000367
    
    Range: 
        OEO_00010227
    
    
ObjectProperty: OEO_00020056

    
ObjectProperty: OEO_00020070

    Annotations: 
        <http://purl.obolibrary.org/obo/IAO_0000115> "Is traded at is a relation that holds between a market exchange and the financial instruments, commodities, or other products, services, or goods which are traded there.",
        <http://purl.obolibrary.org/obo/IAO_0000233> "pull request: https://github.com/OpenEnergyPlatform/ontology/pull/748

change range: 
issue: https://github.com/OpenEnergyPlatform/ontology/issues/791
pull request: https://github.com/OpenEnergyPlatform/ontology/pull/842

add domain:
issue: https://github.com/OpenEnergyPlatform/ontology/issues/973
pull request: https://github.com/OpenEnergyPlatform/ontology/pull/1127",
        rdfs:label "is traded at"
    
    SubPropertyOf: 
        owl:topObjectProperty
    
    Domain: 
        
            Annotations: <http://purl.obolibrary.org/obo/IAO_0000116> "Extension of domain to financial instrument and other products planned"
        OEO_00010116 or OEO_00020067 or OEO_00140124
    
    Range: 
        <http://purl.obolibrary.org/obo/RO_0000087> some OEO_00040002
    
    InverseOf: 
        OEO_00020071
    
    
ObjectProperty: OEO_00020071

    Annotations: 
        <http://purl.obolibrary.org/obo/IAO_0000115> "A relation that holds between financial instruments, commodities, or other products, services, or goods and a market exchange.",
        <http://purl.obolibrary.org/obo/IAO_0000233> "pull request: https://github.com/OpenEnergyPlatform/ontology/pull/748

add domain and range:
issue: https://github.com/OpenEnergyPlatform/ontology/issues/973
pull request: https://github.com/OpenEnergyPlatform/ontology/pull/1127",
        rdfs:label "trades"
    
    SubPropertyOf: 
        owl:topObjectProperty
    
    Domain: 
        <http://purl.obolibrary.org/obo/RO_0000087> some OEO_00040002
    
    Range: 
        
            Annotations: <http://purl.obolibrary.org/obo/IAO_0000116> "Extension of range to financial instrument and other products planned"
        OEO_00010116 or OEO_00020067 or OEO_00140124
    
    InverseOf: 
        OEO_00020070
    
    
ObjectProperty: OEO_00040010

    
ObjectProperty: OEO_00140008

    
ObjectProperty: OEO_00140017

    Annotations: 
        <http://purl.obolibrary.org/obo/IAO_0000115> "A relation between a person and an organisation where the person is a member of the organisation.",
        <http://purl.obolibrary.org/obo/IAO_0000233> "issue: https://github.com/OpenEnergyPlatform/ontology/issues/486
pull request: https://github.com/OpenEnergyPlatform/ontology/pull/562",
        rdfs:label "member of"@en
    
    Domain: 
        OEO_00000323
    
    Range: 
        OEO_00030022
    
    
ObjectProperty: OEO_00140018

    Annotations: 
        <http://purl.obolibrary.org/obo/IAO_0000115> "A relation between an organisation and a person where the person is a member of the organisation.",
        <http://purl.obolibrary.org/obo/IAO_0000233> "issue: https://github.com/OpenEnergyPlatform/ontology/issues/486
pull request: https://github.com/OpenEnergyPlatform/ontology/pull/562",
        rdfs:label "has member"@en
    
    SubPropertyOf: 
        owl:topObjectProperty
    
    Domain: 
        OEO_00030022
    
    Range: 
        OEO_00000323
    
    
ObjectProperty: OEO_00140164

    
ObjectProperty: owl:topObjectProperty

    
Class: <http://purl.obolibrary.org/obo/BFO_0000002>

    
Class: <http://purl.obolibrary.org/obo/BFO_0000003>

    
Class: <http://purl.obolibrary.org/obo/BFO_0000004>

    
Class: <http://purl.obolibrary.org/obo/BFO_0000006>

    
Class: <http://purl.obolibrary.org/obo/BFO_0000009>

    
Class: <http://purl.obolibrary.org/obo/BFO_0000015>

    
Class: <http://purl.obolibrary.org/obo/BFO_0000016>

    
Class: <http://purl.obolibrary.org/obo/BFO_0000017>

    
Class: <http://purl.obolibrary.org/obo/BFO_0000019>

    
Class: <http://purl.obolibrary.org/obo/BFO_0000020>

    
Class: <http://purl.obolibrary.org/obo/BFO_0000023>

    
Class: <http://purl.obolibrary.org/obo/BFO_0000024>

    
Class: <http://purl.obolibrary.org/obo/BFO_0000027>

    
Class: <http://purl.obolibrary.org/obo/BFO_0000029>

    
Class: <http://purl.obolibrary.org/obo/BFO_0000030>

    
Class: <http://purl.obolibrary.org/obo/BFO_0000031>

    
Class: <http://purl.obolibrary.org/obo/BFO_0000038>

    
Class: <http://purl.obolibrary.org/obo/BFO_0000040>

    
Class: <http://purl.obolibrary.org/obo/BFO_0000141>

    
Class: <http://purl.obolibrary.org/obo/BFO_0000148>

    
Class: <http://purl.obolibrary.org/obo/IAO_0000030>

    
Class: <http://purl.obolibrary.org/obo/IAO_0000104>

    
Class: <http://purl.obolibrary.org/obo/IAO_0000310>

    
Class: <http://purl.obolibrary.org/obo/RO_0002577>

    
Class: <http://purl.obolibrary.org/obo/UO_0000000>

    
Class: <http://purl.obolibrary.org/obo/UO_0000187>

    
Class: <http://purl.obolibrary.org/obo/UO_0000190>

    
Class: <http://purl.obolibrary.org/obo/UO_0010006>

    
Class: OEO_00000045

    Annotations: 
        <http://purl.obolibrary.org/obo/IAO_0000115> "A producer is an agent that makes goods.",
        <http://purl.obolibrary.org/obo/IAO_0000233> "issue: https://github.com/OpenEnergyPlatform/ontology/issues/835
pull request: https://github.com/OpenEnergyPlatform/ontology/pull/845

issue: https://github.com/OpenEnergyPlatform/ontology/issues/314
pull request: https://github.com/OpenEnergyPlatform/ontology/pull/370",
        rdfs:label "producer"
    
    SubClassOf: 
        OEO_00000051,
        <http://purl.obolibrary.org/obo/RO_0000056> some OEO_00240003
    
    
Class: OEO_00000051

    
Class: OEO_00000064

    
Class: OEO_00000087

    
Class: OEO_00000105

    Annotations: 
        <http://purl.obolibrary.org/obo/IAO_0000115> "A consumer is a user of a commercial product or service."@en,
        rdfs:label "consumer"
    
    SubClassOf: 
        OEO_00000431
    
    
Class: OEO_00000107

    
Class: OEO_00000128

    Annotations: 
        <http://purl.obolibrary.org/obo/IAO_0000115> "An energy demand sector is a sector that covers energy consumers."@en,
        
            Annotations: <http://purl.obolibrary.org/obo/IAO_0000233> "issue: https://github.com/OpenEnergyPlatform/ontology/issues/1014
pull request: https://github.com/OpenEnergyPlatform/ontology/pull/1015"
        <http://purl.obolibrary.org/obo/IAO_0000118> "final energy sector",
        <http://purl.obolibrary.org/obo/IAO_0000233> "issue: https://github.com/OpenEnergyPlatform/ontology/issues/30
pull request: https://github.com/OpenEnergyPlatform/ontology/pull/484",
        rdfs:label "energy demand sector"
    
    SubClassOf: 
        OEO_00000367
    
    
Class: OEO_00000145

    Annotations: 
        <http://purl.obolibrary.org/obo/IAO_0000115> "An electricity sector is a transformation sector that covers electricity generation and transport of electrical energy to consumers of electrical energy."@en,
        <http://purl.obolibrary.org/obo/IAO_0000233> "issue: https://github.com/OpenEnergyPlatform/ontology/issues/30
pull request: https://github.com/OpenEnergyPlatform/ontology/pull/484",
        rdfs:label "electricity sector"
    
    SubClassOf: 
        OEO_00000158
    
    
Class: OEO_00000158

    Annotations: 
        <http://purl.obolibrary.org/obo/IAO_0000115> "An energy transformation sector is a sector that covers energy production, energy transformation from primary to secondary energy and transport of energy to the demand sector.",
        <http://purl.obolibrary.org/obo/IAO_0000118> "energy industry sector",
        <http://purl.obolibrary.org/obo/IAO_0000118> "energy sector",
        <http://purl.obolibrary.org/obo/IAO_0000233> "issue: https://github.com/OpenEnergyPlatform/ontology/issues/30
pull request: https://github.com/OpenEnergyPlatform/ontology/pull/484",
        rdfs:label "energy transformation sector"
    
    SubClassOf: 
        OEO_00000367
    
    
Class: OEO_00000213

    Annotations: 
        <http://purl.obolibrary.org/obo/IAO_0000115> "A heating and cooling sector is a sector that covers heating and cooling activities."@en,
        <http://purl.obolibrary.org/obo/IAO_0000118> "H&C sector",
        <http://purl.obolibrary.org/obo/IAO_0000233> "issue: https://github.com/OpenEnergyPlatform/ontology/issues/30
pull request: https://github.com/OpenEnergyPlatform/ontology/pull/484",
        rdfs:label "heating and cooling sector"
    
    SubClassOf: 
        OEO_00000128
    
    
Class: OEO_00000214

    Annotations: 
        <http://purl.obolibrary.org/obo/IAO_0000115> "A household sector is a sector that covers households."@en,
        <http://purl.obolibrary.org/obo/IAO_0000118> "private household sector",
        <http://purl.obolibrary.org/obo/IAO_0000233> "issue: https://github.com/OpenEnergyPlatform/ontology/issues/30
pull request: https://github.com/OpenEnergyPlatform/ontology/pull/484",
        rdfs:label "household sector"
    
    SubClassOf: 
        OEO_00000128
    
    
Class: OEO_00000227

    Annotations: 
        <http://purl.obolibrary.org/obo/IAO_0000115> "An industry sector is a sector that covers industrial activities with other main purposes of energy transformation."@en,
        <http://purl.obolibrary.org/obo/IAO_0000233> "issue: https://github.com/OpenEnergyPlatform/ontology/issues/30
pull request: https://github.com/OpenEnergyPlatform/ontology/pull/484",
        rdfs:label "industry sector"
    
    SubClassOf: 
        OEO_00000367
    
    
Class: OEO_00000238

    
Class: OEO_00000264

    SubClassOf: 
        
            Annotations: <http://purl.obolibrary.org/obo/IAO_0000233> "issue: https://github.com/OpenEnergyPlatform/ontology/issues/415
pull request: https://github.com/OpenEnergyPlatform/ontology/pull/821"
        OEO_00140164 some OEO_00020065
    
    
Class: OEO_00000315

    
Class: OEO_00000323

    
Class: OEO_00000329

    Annotations: 
        <http://purl.obolibrary.org/obo/IAO_0000115> "A political party is a organisation of a group of people with common views or goals that wants to have influence in politics."@en,
        rdfs:label "political party"
    
    SubClassOf: 
        OEO_00030022
    
    
Class: OEO_00000341

    Annotations: 
        <http://purl.obolibrary.org/obo/IAO_0000115> "A prosumer is an agent who is producer and consumer at the same time."@en,
        rdfs:label "prosumer"
    
    SubClassOf: 
        OEO_00000051
    
    
Class: OEO_00000350

    
Class: OEO_00000367

    
Class: OEO_00000368

    Annotations: 
        <http://purl.obolibrary.org/obo/IAO_0000115> "A sector division is a specific way to subdivide a system."@en,
        <http://purl.obolibrary.org/obo/IAO_0000233> "issue: https://github.com/OpenEnergyPlatform/ontology/issues/30",
        rdfs:label "sector division"
    
    SubClassOf: 
        <http://purl.obolibrary.org/obo/BFO_0000031>
    
    
Class: OEO_00000379

    Annotations: 
        <http://purl.obolibrary.org/obo/IAO_0000115> "A software developer is an agent that creates computer software.",
        rdfs:label "software developer"
    
    SubClassOf: 
        OEO_00000051
    
    
Class: OEO_00000405

    Annotations: 
        <http://purl.obolibrary.org/obo/IAO_0000115> "A commercial sector is a sector that covers non-industrial commercial activities."@en,
        <http://purl.obolibrary.org/obo/IAO_0000118> "TCS sector",
        <http://purl.obolibrary.org/obo/IAO_0000118> "service sector",
        <http://purl.obolibrary.org/obo/IAO_0000118> "trading, commerce and service sector",
        <http://purl.obolibrary.org/obo/IAO_0000233> "issue: https://github.com/OpenEnergyPlatform/ontology/issues/30
pull request: https://github.com/OpenEnergyPlatform/ontology/pull/484",
        rdfs:label "commercial sector"
    
    SubClassOf: 
        OEO_00000128
    
    
Class: OEO_00000422

    Annotations: 
        <http://purl.obolibrary.org/obo/IAO_0000115> "A transport sector is a sector that covers transport of people and/or goods."@en,
        <http://purl.obolibrary.org/obo/IAO_0000118> "traffic sector",
        <http://purl.obolibrary.org/obo/IAO_0000233> "issue: https://github.com/OpenEnergyPlatform/ontology/issues/30
pull request: https://github.com/OpenEnergyPlatform/ontology/pull/484",
        rdfs:label "transport sector"
    
    SubClassOf: 
        OEO_00000128
    
    
Class: OEO_00000431

    Annotations: 
        <http://purl.obolibrary.org/obo/IAO_0000115> "A user is an agent that employs an aid, tool or information system to achieve a goal/benefit.",
        rdfs:label "user"
    
    SubClassOf: 
        OEO_00000051
    
    
Class: OEO_00010034

    Annotations: 
        <http://purl.obolibrary.org/obo/IAO_0000115> "A building sector is a sector that covers buildings.",
        <http://purl.obolibrary.org/obo/IAO_0000233> "issue: https://github.com/OpenEnergyPlatform/ontology/issues/30
pull request: https://github.com/OpenEnergyPlatform/ontology/pull/484",
        rdfs:label "building sector"
    
    SubClassOf: 
        OEO_00000128
    
    
Class: OEO_00010035

    Annotations: 
        <http://purl.obolibrary.org/obo/IAO_0000115> "A agriculture, forestry and land use (AFOLU) sector is a sector that covers activities and natural processes from agriculture, forestry, land use and land use change.",
        <http://purl.obolibrary.org/obo/IAO_0000118> "AFOLU sector",
        <http://purl.obolibrary.org/obo/IAO_0000233> "issue: https://github.com/OpenEnergyPlatform/ontology/issues/30
pull request: https://github.com/OpenEnergyPlatform/ontology/pull/484",
        rdfs:label "agriculture, forestry and land use sector"
    
    SubClassOf: 
        OEO_00000367
    
    
Class: OEO_00010036

    Annotations: 
        <http://purl.obolibrary.org/obo/IAO_0000115> "A waste and wastewater sector is a sector that covers activities related the collection and treatment of waste and wastewater.",
        <http://purl.obolibrary.org/obo/IAO_0000233> "issue: https://github.com/OpenEnergyPlatform/ontology/issues/30
pull request: https://github.com/OpenEnergyPlatform/ontology/pull/484",
        rdfs:label "waste and wastewater sector"
    
    SubClassOf: 
        OEO_00000367
    
    
Class: OEO_00010055

    Annotations: 
        <http://purl.obolibrary.org/obo/IAO_0000115> "The common reporting format (CRF) is a sector division used for compiling national inventory reports on greenhouse gas emissions and providing emission relevant data in so called CRF tables.",
        <http://purl.obolibrary.org/obo/IAO_0000118> "CRF",
        <http://purl.obolibrary.org/obo/IAO_0000233> "issue: https://github.com/OpenEnergyPlatform/ontology/issues/461
pull request: https://github.com/OpenEnergyPlatform/ontology/pull/578",
        rdfs:label "common reporting format"
    
    SubClassOf: 
        OEO_00000368
    
    
Class: OEO_00010079

    SubClassOf: 
        OEO_00020056 some OEO_00020063
    
    
Class: OEO_00010082

    Annotations: 
        <http://purl.obolibrary.org/obo/IAO_0000115> "A trade is a process in which one commodity or service is exchanged for another commodity or service.",
        <http://purl.obolibrary.org/obo/IAO_0000233> "issue: https://github.com/OpenEnergyPlatform/ontology/issues/307
pull request: https://github.com/OpenEnergyPlatform/ontology/pull/745",
        rdfs:label "trade"@en
    
    SubClassOf: 
        <http://purl.obolibrary.org/obo/BFO_0000015>,
        <http://purl.obolibrary.org/obo/RO_0000057> some OEO_00040011
    
    
Class: OEO_00010083

    Annotations: 
        <http://purl.obolibrary.org/obo/IAO_0000115> "A market participant is an agent who participates in trading in a market exchange.",
        <http://purl.obolibrary.org/obo/IAO_0000233> "issue: https://github.com/OpenEnergyPlatform/ontology/issues/330
pull request: https://github.com/OpenEnergyPlatform/ontology/pull/745

update definition and improve axiom:
https://github.com/OpenEnergyPlatform/ontology/issues/617
https://github.com/OpenEnergyPlatform/ontology/pull/1019",
        rdfs:label "market participant"@en
    
    SubClassOf: 
        OEO_00000051,
        <http://purl.obolibrary.org/obo/RO_0000056> some OEO_00010082
    
    
Class: OEO_00010115

    Annotations: 
        <http://purl.obolibrary.org/obo/IAO_0000115> "An economy is a system of production, distribution, trade and consumption of goods and services.",
        <http://purl.obolibrary.org/obo/IAO_0000233> "issue: https://github.com/OpenEnergyPlatform/ontology/issues/832
pull request: https://github.com/OpenEnergyPlatform/ontology/pull/843",
        rdfs:label "economy"@en
    
    SubClassOf: 
        <http://purl.obolibrary.org/obo/RO_0002577>
    
    
Class: OEO_00010116

    
Class: OEO_00010117

    
Class: OEO_00010123

    Annotations: 
        <http://purl.obolibrary.org/obo/IAO_0000115> "Effort sharing is a policy instrument that sets a common emission reduction goal for a number of countries. Each country has a national reduction goal. Under- or overachievement of that goal can be compensated by trading emission certificates.",
        <http://purl.obolibrary.org/obo/IAO_0000233> "issue: https://github.com/OpenEnergyPlatform/ontology/issues/834
pull request: https://github.com/OpenEnergyPlatform/ontology/pull/857",
        rdfs:label "effort sharing"@en
    
    SubClassOf: 
        OEO_00140151,
        OEO_00000503 some OEO_00020063
    
    
Class: OEO_00010126

    Annotations: 
        <http://purl.obolibrary.org/obo/IAO_0000115> "An Annual Emission Allocation (AEA) is an emission certificate used in the Effort Sharing Decision (ESD) and the Effort Sharing Regulation (ESR). It permits the emission of a CO2 equivalent quantity of 1 tonne.",
        <http://purl.obolibrary.org/obo/IAO_0000118> "AEA",
        <http://purl.obolibrary.org/obo/IAO_0000233> "issue: https://github.com/OpenEnergyPlatform/ontology/issues/834
pull request: https://github.com/OpenEnergyPlatform/ontology/pull/857",
        rdfs:label "Annual Emission Allocation"@en
    
    SubClassOf: 
        OEO_00020063
    
    
Class: OEO_00010136

    Annotations: 
        <http://purl.obolibrary.org/obo/IAO_0000115> "Distribution is the process of delivering goods and services to agents",
        <http://purl.obolibrary.org/obo/IAO_0000233> "issue: https://github.com/OpenEnergyPlatform/ontology/issues/836
pull request: https://github.com/OpenEnergyPlatform/ontology/pull/876",
        rdfs:label "distribution"@en
    
    SubClassOf: 
        <http://purl.obolibrary.org/obo/BFO_0000015>
    
    
Class: OEO_00010212

    Annotations: 
        <http://purl.obolibrary.org/obo/IAO_0000115> "A decarbonisation pathway is a policy that aims at long-term emissions reductions.",
        <http://purl.obolibrary.org/obo/IAO_0000233> "issue: https://github.com/OpenEnergyPlatform/ontology/issues/831
pull request: https://github.com/OpenEnergyPlatform/ontology/pull/951",
        rdfs:label "decarbonisation pathway"@en
    
    SubClassOf: 
        OEO_00140150
    
    
Class: OEO_00010227

    Annotations: 
        <http://purl.obolibrary.org/obo/IAO_0000115> "A memo item is an information content entity about a sector that describes that the sector is excluded from some kind of total and only reported to provide further information (memo).",
        <http://purl.obolibrary.org/obo/IAO_0000233> "issue: https://github.com/OpenEnergyPlatform/ontology/issues/858
pull request: https://github.com/OpenEnergyPlatform/ontology/pull/965",
        rdfs:label "memo item"@en
    
    SubClassOf: 
        <http://purl.obolibrary.org/obo/IAO_0000030>,
        <http://purl.obolibrary.org/obo/IAO_0000136> some OEO_00000367
    
    
Class: OEO_00020015

    
Class: OEO_00020060

    Annotations: 
        <http://purl.obolibrary.org/obo/IAO_0000115> "A fuel market exchange is an energy market exchange where fuels like oil, coal, renewable fuels, and natural gas are traded.",
        <http://purl.obolibrary.org/obo/IAO_0000233> "issue https://github.com/OpenEnergyPlatform/ontology/issues/677
pull request https://github.com/OpenEnergyPlatform/ontology/pull/740
pull request https://github.com/OpenEnergyPlatform/ontology/pull/748",
        rdfs:label "fuel market exchange"
    
    SubClassOf: 
        OEO_00020065,
        OEO_00020071 some (<http://purl.obolibrary.org/obo/RO_0000087> some OEO_00020066)
    
    
Class: OEO_00020063

    
Class: OEO_00020064

    Annotations: 
        <http://purl.obolibrary.org/obo/IAO_0000115> "An EU Allowance (EUA) is an emission certificate used in the European Union Emissions Trading System (EU ETS). It permits the emission of a CO2 equivalent quantity of 1 tonne.",
        <http://purl.obolibrary.org/obo/IAO_0000118> "EUA",
        <http://purl.obolibrary.org/obo/IAO_0000233> "issue https://github.com/OpenEnergyPlatform/ontology/issues/677
pull request https://github.com/OpenEnergyPlatform/ontology/pull/740",
        rdfs:label "EU allowance"
    
    SubClassOf: 
        OEO_00020063
    
    
Class: OEO_00020065

    Annotations: 
        <http://purl.obolibrary.org/obo/IAO_0000115> "An energy market exchange is a market exchange in which energy commodities are traded.",
        <http://purl.obolibrary.org/obo/IAO_0000233> "issue https://github.com/OpenEnergyPlatform/ontology/issues/256
pull request https://github.com/OpenEnergyPlatform/ontology/pull/748",
        rdfs:label "energy market exchange"
    
    SubClassOf: 
        OEO_00020069
    
    
Class: OEO_00020066

    
Class: OEO_00020067

    Annotations: 
        <http://purl.obolibrary.org/obo/IAO_0000118> "product"
    
    SubClassOf: 
        OEO_00020070 some OEO_00020069
    
    
Class: OEO_00020068

    SubClassOf: 
        OEO_00020070 some OEO_00020060
    
    
Class: OEO_00020069

    Annotations: 
        <http://purl.obolibrary.org/obo/IAO_0000115> "A market exchange is an organisation that has the market exchange role.",
        <http://purl.obolibrary.org/obo/IAO_0000233> "pull request: https://github.com/OpenEnergyPlatform/ontology/pull/748",
        rdfs:label "market exchange"
    
    EquivalentTo: 
        <http://purl.obolibrary.org/obo/RO_0000087> some OEO_00040002
    
    SubClassOf: 
        OEO_00030022,
        
            Annotations: <http://purl.obolibrary.org/obo/IAO_0000233> "https://github.com/OpenEnergyPlatform/ontology/issues/617
https://github.com/OpenEnergyPlatform/ontology/pull/1019"
        <http://purl.obolibrary.org/obo/RO_0000056> some 
            (OEO_00010082
             and (<http://purl.obolibrary.org/obo/RO_0000057> some OEO_00010083))
    
    
Class: OEO_00020075

    Annotations: 
        <http://purl.obolibrary.org/obo/IAO_0000115> "An emission market exchange is a market exchange where emission certificates are traded",
        <http://purl.obolibrary.org/obo/IAO_0000233> "issue https://github.com/OpenEnergyPlatform/ontology/issues/302
pull request https://github.com/OpenEnergyPlatform/ontology/pull/781",
        rdfs:label "emission market exchange"
    
    SubClassOf: 
        OEO_00020069,
        OEO_00020071 some OEO_00020063
    
    
Class: OEO_00020076

    Annotations: 
        <http://purl.obolibrary.org/obo/IAO_0000115> "A markup is an economic value that indicates a virtual amount added to an assumed or historical price to predict a price in a different context.",
        <http://purl.obolibrary.org/obo/IAO_0000233> "https://github.com/OpenEnergyPlatform/ontology/issues/256
https://github.com/OpenEnergyPlatform/ontology/pull/800",
        rdfs:label "markup"
    
    SubClassOf: 
        OEO_00140012,
        OEO_00040010 some OEO_00040004
    
    
Class: OEO_00020077

    Annotations: 
        <http://purl.obolibrary.org/obo/IAO_0000115> "A markdown is an economic value that indicates a virtual amount deducted from an assumed or historical price to predict a price in a different context.",
        <http://purl.obolibrary.org/obo/IAO_0000233> "https://github.com/OpenEnergyPlatform/ontology/issues/256
https://github.com/OpenEnergyPlatform/ontology/pull/800",
        rdfs:label "markdown"
    
    SubClassOf: 
        OEO_00140012,
        OEO_00040010 some OEO_00040004
    
    
Class: OEO_00020108

    Annotations: 
        <http://purl.obolibrary.org/obo/IAO_0000115> "A feed-in tariff is a policy instrument designed to stimulate investment in renewable energy technologies by offering long-term contracts to agents who are producers of renewable energy.",
        <http://purl.obolibrary.org/obo/IAO_0000233> "issue: https://github.com/OpenEnergyPlatform/ontology/issues/839
issue: https://github.com/OpenEnergyPlatform/ontology/issues/898
pull request: https://github.com/OpenEnergyPlatform/ontology/pull/909",
        rdfs:comment "Feed-in tariffs provide cost-based compensation to renewable energy producers, leading to price certainty and long-term contracts that help finance energy transformation units, e.g. power plants",
        rdfs:label "feed-in tariff"
    
    SubClassOf: 
        OEO_00140151
    
    
Class: OEO_00020109

    Annotations: 
        <http://purl.obolibrary.org/obo/IAO_0000115> "A market premium is a policy instrument that ensures a guaranteed remuneration, e.g. a fixed feed-in tariff, by paying to the producing agent the difference between a guaranteed return on a good/product and the monetary price for which the good/product is traded on the market",
        <http://purl.obolibrary.org/obo/IAO_0000233> "issue: https://github.com/OpenEnergyPlatform/ontology/issues/839
issue: https://github.com/OpenEnergyPlatform/ontology/issues/899
pull request: https://github.com/OpenEnergyPlatform/ontology/pull/909",
        rdfs:label "market premium"
    
    SubClassOf: 
        OEO_00140151
    
    
Class: OEO_00020110

    Annotations: 
        <http://purl.obolibrary.org/obo/IAO_0000115> "A levy is a policy instrument that consists of a compulsory financial charge imposed on an agent or institution by a governmental organisation.",
        <http://purl.obolibrary.org/obo/IAO_0000233> "issue: https://github.com/OpenEnergyPlatform/ontology/issues/839
issue: https://github.com/OpenEnergyPlatform/ontology/issues/900
pull request: https://github.com/OpenEnergyPlatform/ontology/pull/909",
        rdfs:label "levy"
    
    SubClassOf: 
        OEO_00140151
    
    
Class: OEO_00020111

    Annotations: 
        <http://purl.obolibrary.org/obo/IAO_0000115> "A capacity premium is a market premium that guarantees remuneration for reserving capacity of energy transformation units to be available for unexpected events.",
        <http://purl.obolibrary.org/obo/IAO_0000233> "issue: https://github.com/OpenEnergyPlatform/ontology/issues/839
issue: https://github.com/OpenEnergyPlatform/ontology/issues/903
pull request: https://github.com/OpenEnergyPlatform/ontology/pull/909",
        rdfs:label "capacity premium"
    
    SubClassOf: 
        OEO_00020109
    
    
Class: OEO_00020112

    Annotations: 
        <http://purl.obolibrary.org/obo/IAO_0000115> "A tax is a levy whose returns are used by the government to finance expenditures for the common welfare.",
        <http://purl.obolibrary.org/obo/IAO_0000233> "issue: https://github.com/OpenEnergyPlatform/ontology/issues/839
issue: https://github.com/OpenEnergyPlatform/ontology/issues/901
pull request: https://github.com/OpenEnergyPlatform/ontology/pull/909",
        rdfs:label "tax"
    
    SubClassOf: 
        OEO_00020110
    
    
Class: OEO_00020113

    Annotations: 
        <http://purl.obolibrary.org/obo/IAO_0000115> "Inflation rate is an economic value reprensenting the ratio between the monetary price for a good at two different points in time that equalises differences in monetary price levels between these two points in time.",
        <http://purl.obolibrary.org/obo/IAO_0000233> "https://github.com/OpenEnergyPlatform/ontology/issues/335
https://github.com/OpenEnergyPlatform/ontology/pull/910",
        rdfs:label "inflation rate"
    
    SubClassOf: 
        OEO_00140012,
        OEO_00040010 some <http://purl.obolibrary.org/obo/UO_0010006>
    
    
Class: OEO_00020114

    Annotations: 
        <http://purl.obolibrary.org/obo/IAO_0000112> "The exchange rate between USD and EUR on March 15, 2020 was X.X.",
        <http://purl.obolibrary.org/obo/IAO_0000115> "The exchange rate is an economic value representing the ratio at which one currency can be exchanged for another.",
        <http://purl.obolibrary.org/obo/IAO_0000118> "market exchange rate",
        <http://purl.obolibrary.org/obo/IAO_0000233> "https://github.com/OpenEnergyPlatform/ontology/issues/335
https://github.com/OpenEnergyPlatform/ontology/pull/910",
        rdfs:comment "The ratio at which one can exchange one currency for another can differ over time therefore it is necessary to specify a time point when referring to an exchange rate.",
        rdfs:label "exchange rate"
    
    SubClassOf: 
        OEO_00140012,
        OEO_00040010 some <http://purl.obolibrary.org/obo/UO_0010006>
    
    
Class: OEO_00020115

    Annotations: 
        <http://purl.obolibrary.org/obo/IAO_0000115> "Purchasing power parity is an economic value reprensenting the ratio between currencies that equalises differences in monetary price levels between countries for the same set of goods.",
        <http://purl.obolibrary.org/obo/IAO_0000118> "PPP",
        <http://purl.obolibrary.org/obo/IAO_0000233> "https://github.com/OpenEnergyPlatform/ontology/issues/867
https://github.com/OpenEnergyPlatform/ontology/pull/910",
        <http://purl.org/dc/terms/source> "https://www.oecd.org/sdd/prices-ppp/purchasingpowerparities-frequentlyaskedquestionsfaqs.htm#FAQ1",
        rdfs:label "purchasing power parity"
    
    SubClassOf: 
        OEO_00140012,
        OEO_00040010 some <http://purl.obolibrary.org/obo/UO_0010006>
    
    
Class: OEO_00020116

    Annotations: 
        <http://purl.obolibrary.org/obo/IAO_0000115> "System cost are total costs of a system.",
        <http://purl.obolibrary.org/obo/IAO_0000233> "issue: https://github.com/OpenEnergyPlatform/ontology/issues/335
pull request: https://github.com/OpenEnergyPlatform/ontology/pull/910",
        rdfs:label "system cost"
    
    SubClassOf: 
        OEO_00040009
    
    
Class: OEO_00020117

    Annotations: 
        <http://purl.obolibrary.org/obo/IAO_0000112> "The electricity price is Y EUR per megawatt-hour.",
        <http://purl.obolibrary.org/obo/IAO_0000115> "Electricity price is the monetary price per energy unit of electricity.",
        <http://purl.obolibrary.org/obo/IAO_0000233> "issue: https://github.com/OpenEnergyPlatform/ontology/issues/335
pull request: https://github.com/OpenEnergyPlatform/ontology/pull/910",
        rdfs:comment "has unit some \"currency per energy unit\"",
        rdfs:label "electricity price"
    
    SubClassOf: 
        OEO_00040003
    
    
Class: OEO_00020124

    Annotations: 
        <http://purl.obolibrary.org/obo/IAO_0000115> "A due is an economic value that represents a payment that an agent makes to belong to an organisation.",
        <http://purl.obolibrary.org/obo/IAO_0000233> "issue: https://github.com/OpenEnergyPlatform/ontology/issues/904
pull request: https://github.com/OpenEnergyPlatform/ontology/pull/913",
        rdfs:label "due"
    
    SubClassOf: 
        OEO_00140012,
        OEO_00040010 some OEO_00040004
    
    
Class: OEO_00020125

    Annotations: 
        <http://purl.obolibrary.org/obo/IAO_0000115> "A remuneration is an economic value that describes a financial compensation provided in exchange for services performed.",
        <http://purl.obolibrary.org/obo/IAO_0000233> "issue: https://github.com/OpenEnergyPlatform/ontology/issues/902
pull request: https://github.com/OpenEnergyPlatform/ontology/pull/913",
        rdfs:label "remuneration"
    
    SubClassOf: 
        OEO_00140012,
        OEO_00040010 some OEO_00040004
    
    
Class: OEO_00020126

    Annotations: 
        <http://purl.obolibrary.org/obo/IAO_0000115> "A fee is an economic value that represents an amount of money paid for a  particular piece of work or for a particular right or service.",
        <http://purl.obolibrary.org/obo/IAO_0000233> "issue: https://github.com/OpenEnergyPlatform/ontology/issues/905
pull request: https://github.com/OpenEnergyPlatform/ontology/pull/913",
        rdfs:label "fee"
    
    SubClassOf: 
        OEO_00140012,
        OEO_00040010 some OEO_00040004
    
    
Class: OEO_00020127

    Annotations: 
        <http://purl.obolibrary.org/obo/IAO_0000115> "Levelised cost of electricity are the net cost of converting energy to electricity / electric energy over the lifetime of an energy transformation unit. They are calculated considering all relevant costs including investment, operation, maintenance and fuel cost, etc.",
        <http://purl.obolibrary.org/obo/IAO_0000118> "LCOE",
        <http://purl.obolibrary.org/obo/IAO_0000233> "issue: https://github.com/OpenEnergyPlatform/ontology/issues/906
pull request: https://github.com/OpenEnergyPlatform/ontology/pull/913",
        rdfs:comment "Since over the lifetime of an energy transformation unit different costs exhibit different relevance or vary over time, the LCOE differ over the course of the lifetime.",
        rdfs:label "levelised cost of electricity"
    
    SubClassOf: 
        OEO_00040009
    
    
Class: OEO_00020128

    Annotations: 
        <http://purl.obolibrary.org/obo/IAO_0000115> "Market revenue is an economic value that represents the income from a trade at a market exchange.",
        <http://purl.obolibrary.org/obo/IAO_0000233> "add term
https://github.com/OpenEnergyPlatform/ontology/issues/908
https://github.com/OpenEnergyPlatform/ontology/pull/929",
        rdfs:label "market revenue"
    
    SubClassOf: 
        OEO_00140012,
        OEO_00040010 some OEO_00040004
    
    
Class: OEO_00020145

    Annotations: 
        <http://purl.obolibrary.org/obo/IAO_0000115> "Variable costs are costs that depend on an amount of goods or services.",
        <http://purl.obolibrary.org/obo/IAO_0000118> "unit-level cost",
        <http://purl.obolibrary.org/obo/IAO_0000233> "issue: https://github.com/OpenEnergyPlatform/ontology/issues/891
pull request: https://github.com/OpenEnergyPlatform/ontology/pull/953",
        rdfs:label "variable cost"
    
    SubClassOf: 
        OEO_00040009
    
    
Class: OEO_00020146

    Annotations: 
        <http://purl.obolibrary.org/obo/IAO_0000112> "An example for variable cost are costs incurred for raw materials (of which more are needed if production is increased).",
        <http://purl.obolibrary.org/obo/IAO_0000115> "Variable costs are costs that depend on the amount of goods or services produced and which are payed by the producer.",
        <http://purl.obolibrary.org/obo/IAO_0000233> "issue: https://github.com/OpenEnergyPlatform/ontology/issues/891
pull request: https://github.com/OpenEnergyPlatform/ontology/pull/953",
        rdfs:label "variable production cost"
    
    SubClassOf: 
        OEO_00020145
    
    
Class: OEO_00020156

    Annotations: 
        <http://purl.obolibrary.org/obo/IAO_0000115> "Carbon tax is a tax for emitting CO2 or other greenhouse gases (measured in CO2 equivalent values).",
        <http://purl.obolibrary.org/obo/IAO_0000118> "CO2 tax",
        <http://purl.obolibrary.org/obo/IAO_0000233> "issue: https://github.com/OpenEnergyPlatform/ontology/issues/866
pull request: https://github.com/OpenEnergyPlatform/ontology/pull/956",
        rdfs:label "carbon tax"
    
    SubClassOf: 
        OEO_00020112
    
    
Class: OEO_00020167

    Annotations: 
        <http://purl.obolibrary.org/obo/IAO_0000115> "Investment costs are costs of a long-term commitment of financial resources in tangible or intangible assets.",
        <http://purl.obolibrary.org/obo/IAO_0000118> "capital investment cost",
        <http://purl.obolibrary.org/obo/IAO_0000118> "fixed investment cost",
        <http://purl.obolibrary.org/obo/IAO_0000118> "investment",
        <http://purl.obolibrary.org/obo/IAO_0000119> "FIBO definition of investment relates to property only: https://spec.edmcouncil.org/fibo/ontology?searchBoxQuery=investment, 

Gabler on Investition: langfristige Bindung finanzieller Mittel in materiellen oder in immateriellen Vermögensgegenständen (https://wirtschaftslexikon.gabler.de/definition/investition-39454)",
        <http://purl.obolibrary.org/obo/IAO_0000233> "issue: https://github.com/OpenEnergyPlatform/ontology/issues/891
pull request: https://github.com/OpenEnergyPlatform/ontology/pull/1022",
        rdfs:label "investment cost"
    
    SubClassOf: 
        OEO_00040009
    
    
Class: OEO_00020168

    Annotations: 
        <http://purl.obolibrary.org/obo/IAO_0000112> "rent, regular technical maintenance cost, staff cost, certification cost",
        <http://purl.obolibrary.org/obo/IAO_0000115> "Fixed costs are costs for operation and mantainance that do not vary with the amount of goods or services produced.",
        <http://purl.obolibrary.org/obo/IAO_0000118> "fixed operation and maintanance cost",
        <http://purl.obolibrary.org/obo/IAO_0000119> "oemof-Model: https://oemof-solph.readthedocs.io/en/latest/_modules/oemof/solph/options.html?highlight=fix%20costs

Fixe Kosten: Kosten, die von der jeweils betrachteten Einflussgröße bzw. Entscheidung unabhängig sind, d.h. Kosten, die sich nicht mit der jeweils betrachteten Einflussgröße ändern. (https://wirtschaftslexikon.gabler.de/definition/fixe-kosten-33359)",
        <http://purl.obolibrary.org/obo/IAO_0000233> "issue: https://github.com/OpenEnergyPlatform/ontology/issues/891
pull request: https://github.com/OpenEnergyPlatform/ontology/pull/1022",
        rdfs:label "fixed cost"
    
    SubClassOf: 
        OEO_00040009
    
    
Class: OEO_00020169

    Annotations: 
        <http://purl.obolibrary.org/obo/IAO_0000115> "Equipment costs are investment costs for acquisition of the components and machinery including environmental facilities.",
        <http://purl.obolibrary.org/obo/IAO_0000233> "issue: https://github.com/OpenEnergyPlatform/ontology/issues/891
pull request: https://github.com/OpenEnergyPlatform/ontology/pull/1022",
        rdfs:label "equipment cost"
    
    SubClassOf: 
        OEO_00020167
    
    
Class: OEO_00020170

    Annotations: 
        <http://purl.obolibrary.org/obo/IAO_0000112> "costs that occur for becoming operational",
        <http://purl.obolibrary.org/obo/IAO_0000115> "Installation and development cost are investment costs incurred for setting up the installation.",
        <http://purl.obolibrary.org/obo/IAO_0000118> "installation and development cost",
        <http://purl.obolibrary.org/obo/IAO_0000118> "site development cost",
        <http://purl.obolibrary.org/obo/IAO_0000233> "issue: https://github.com/OpenEnergyPlatform/ontology/issues/891
pull request: https://github.com/OpenEnergyPlatform/ontology/pull/1022",
        rdfs:label "installation cost"
    
    SubClassOf: 
        OEO_00020167
    
    
Class: OEO_00020171

    Annotations: 
        <http://purl.obolibrary.org/obo/IAO_0000115> "Grid connection costs are investment costs for establishing the grid connection from the energy generating device to point of connection to national grid.",
        <http://purl.obolibrary.org/obo/IAO_0000233> "issue: https://github.com/OpenEnergyPlatform/ontology/issues/891
pull request: https://github.com/OpenEnergyPlatform/ontology/pull/1022",
        rdfs:label "grid connection cost"
    
    SubClassOf: 
        OEO_00020167
    
    
Class: OEO_00020172

    Annotations: 
        <http://purl.obolibrary.org/obo/IAO_0000115> "Property costs are investment costs arising from the acquisition of a property.",
        <http://purl.obolibrary.org/obo/IAO_0000118> "land cost",
        <http://purl.obolibrary.org/obo/IAO_0000233> "issue: https://github.com/OpenEnergyPlatform/ontology/issues/891
pull request: https://github.com/OpenEnergyPlatform/ontology/pull/1022",
        rdfs:label "property cost"
    
    SubClassOf: 
        OEO_00020167
    
    
Class: OEO_00020173

    Annotations: 
        <http://purl.obolibrary.org/obo/IAO_0000115> "Decommissioning costs are investment costs arising from the decommissioning of a technological device at the end of its lifetime.",
        <http://purl.obolibrary.org/obo/IAO_0000233> "issue: https://github.com/OpenEnergyPlatform/ontology/issues/891
pull request: https://github.com/OpenEnergyPlatform/ontology/pull/1022",
        rdfs:label "decommissioning cost"
    
    SubClassOf: 
        OEO_00020167
    
    
Class: OEO_00020174

    Annotations: 
        <http://purl.obolibrary.org/obo/IAO_0000115> "Delivery costs are costs for a product or service that refer to the total unit cost of a product or commodity delivered to a certain market, city or customer. It is normally composed of all associated transport costs and the unit cost of production for that product.",
        <http://purl.obolibrary.org/obo/IAO_0000233> "issue: https://github.com/OpenEnergyPlatform/ontology/issues/891
pull request: https://github.com/OpenEnergyPlatform/ontology/pull/1022",
        rdfs:label "delivery cost"
    
    SubClassOf: 
        OEO_00040009
    
    
Class: OEO_00030016

    Annotations: 
        <http://purl.obolibrary.org/obo/IAO_0000115> "An organisational energy producer is an organisation that undertakes the generation of electricity and/or heat.\"",
        <http://purl.obolibrary.org/obo/IAO_0000118> "organisational energy producer",
        <http://purl.obolibrary.org/obo/IAO_0000119> "inspired by https://ec.europa.eu/eurostat/documents/38154/41386/Ele_AQ_documentation.pdf/a06bf650-1830-4fcb-9376-7be1f8ab080c",
        <http://purl.obolibrary.org/obo/IAO_0000233> "issue: https://github.com/OpenEnergyPlatform/ontology/issues/314
pull request: https://github.com/OpenEnergyPlatform/ontology/pull/370",
        rdfs:label "organisational energy producer"
    
    SubClassOf: 
        OEO_00030022,
        <http://purl.obolibrary.org/obo/RO_0000087> some OEO_00000045
    
    
Class: OEO_00030017

    Annotations: 
        <http://purl.obolibrary.org/obo/IAO_0000115> "An energy autoproducer is an organisational energy producer who produces electrical energy and/or heat wholly or partly for their own use as an activity which supports their primary activity.",
        <http://purl.obolibrary.org/obo/IAO_0000119> "inspired by https://ec.europa.eu/eurostat/documents/38154/41386/Ele_AQ_documentation.pdf/a06bf650-1830-4fcb-9376-7be1f8ab080c",
        <http://purl.obolibrary.org/obo/IAO_0000233> "issue: https://github.com/OpenEnergyPlatform/ontology/issues/314
pull request: https://github.com/OpenEnergyPlatform/ontology/pull/370",
        rdfs:comment "They may be privately or publicly owned.",
        rdfs:label "energy autoproducer"
    
    SubClassOf: 
        OEO_00030016
    
    
Class: OEO_00030018

    Annotations: 
        <http://purl.obolibrary.org/obo/IAO_0000115> "A main activity energy producer is an organisational energy producer whose primary activity is electrical energy and/or heat production.",
        <http://purl.obolibrary.org/obo/IAO_0000119> "inspired by https://ec.europa.eu/eurostat/documents/38154/41386/Ele_AQ_documentation.pdf/a06bf650-1830-4fcb-9376-7be1f8ab080c",
        <http://purl.obolibrary.org/obo/IAO_0000233> "issue: https://github.com/OpenEnergyPlatform/ontology/issues/314
pull request: https://github.com/OpenEnergyPlatform/ontology/pull/370",
        rdfs:comment "They may be privately or publicly owned. Note that the sale need not take place through the public grid.",
        rdfs:label "main activity energy producer"
    
    SubClassOf: 
        OEO_00030016
    
    
Class: OEO_00030022

    
Class: OEO_00030035

    
Class: OEO_00040002

    Annotations: 
        <http://purl.obolibrary.org/obo/IAO_0000115> "A role of an organisation, association, or group of persons, whether incorporated or unincorporated, which constitutes, maintains, or provides a facility for bringing together purchasers and sellers of financial instruments, commodities, or other products, services, or goods, and includes the market place and facilities maintained by the exchange",
        <http://purl.obolibrary.org/obo/IAO_0000118> "exchange",
        <http://purl.obolibrary.org/obo/IAO_0000118> "market",
        <http://purl.obolibrary.org/obo/IAO_0000119> "fibo-fbc-fct-mkt:Exchange",
        <http://purl.obolibrary.org/obo/IAO_0000233> "https://github.com/OpenEnergyPlatform/ontology/issues/341
https://github.com/OpenEnergyPlatform/ontology/pull/639

https://github.com/OpenEnergyPlatform/ontology/issues/677
https://github.com/OpenEnergyPlatform/ontology/pull/740

change label to market exchange role
https://github.com/OpenEnergyPlatform/ontology/pull/748",
        rdfs:label "market exchange role"@en,
        rdfs:seeAlso "https://spec.edmcouncil.org/fibo/ontology/FBC/FunctionalEntities/Markets/Exchange"
    
    SubClassOf: 
        <http://purl.obolibrary.org/obo/BFO_0000023>
    
    
Class: OEO_00040003

    
Class: OEO_00040004

    
Class: OEO_00040005

    Annotations: 
        <http://purl.obolibrary.org/obo/IAO_0000115> "A trader is a market participant that engages in the transfer of financial assets in any financial market on behalf of a client or a financial services provider.",
        <http://purl.obolibrary.org/obo/IAO_0000119> "fibo-fbc-pas-fpas:Trader",
        <http://purl.obolibrary.org/obo/IAO_0000233> "Implement in line with FIBO:
issue: https://github.com/OpenEnergyPlatform/ontology/issues/377
pull request: https://github.com/OpenEnergyPlatform/ontology/pull/641

Make trader subclass of market participant:
issue: https://github.com/OpenEnergyPlatform/ontology/issues/330
https://github.com/OpenEnergyPlatform/ontology/pull/745",
        rdfs:label "trader"@en,
        rdfs:seeAlso "https://spec.edmcouncil.org/fibo/ontology/FBC/ProductsAndServices/FinancialProductsAndServices/Trader"
    
    SubClassOf: 
        OEO_00010083
    
    
Class: OEO_00040006

    Annotations: 
        <http://purl.obolibrary.org/obo/IAO_0000115> "A request is a process whereby an agent asks another agent for something or to do something.",
        <http://purl.obolibrary.org/obo/IAO_0000119> "https://spec.edmcouncil.org/fibo/ontology/FND/Arrangements/Communications/Request",
        <http://purl.obolibrary.org/obo/IAO_0000233> "https://github.com/OpenEnergyPlatform/ontology/issues/376
https://github.com/OpenEnergyPlatform/ontology/pull/642",
        rdfs:label "request"@en
    
    SubClassOf: 
        <http://purl.obolibrary.org/obo/BFO_0000015>
    
    
Class: OEO_00040007

    Annotations: 
        <http://purl.obolibrary.org/obo/IAO_0000115> "A price request is a request in which an agent asks another agent for a price.",
        <http://purl.obolibrary.org/obo/IAO_0000233> "https://github.com/OpenEnergyPlatform/ontology/issues/376
https://github.com/OpenEnergyPlatform/ontology/pull/642",
        rdfs:label "price request"@en
    
    SubClassOf: 
        OEO_00040006
    
    
Class: OEO_00040008

    Annotations: 
        <http://purl.obolibrary.org/obo/IAO_0000115> "Marginal cost is the economic value that corresponds to the change in the total cost that arises when the quantity produced is incremented by one unit; that is, it is the cost of producing one more unit of a good.",
        <http://purl.obolibrary.org/obo/IAO_0000119> "O'Sullivan, Arthur; Sheffrin, Steven M. (2003). Economics: Principles in Action.",
        <http://purl.obolibrary.org/obo/IAO_0000233> "https://github.com/OpenEnergyPlatform/ontology/issues/376
https://github.com/OpenEnergyPlatform/ontology/pull/642",
        rdfs:label "marginal cost"@en
    
    SubClassOf: 
        OEO_00140012
    
    
Class: OEO_00040009

    
Class: OEO_00040011

    
Class: OEO_00090001

    
Class: OEO_00090002

    Annotations: 
        <http://purl.obolibrary.org/obo/IAO_0000115> "A public funder is a funder that gives public money.",
        <http://purl.obolibrary.org/obo/IAO_0000233> "issue: https://github.com/OpenEnergyPlatform/ontology/issues/246
pull request: https://github.com/OpenEnergyPlatform/ontology/pull/776",
        rdfs:label "public funder"@en
    
    SubClassOf: 
        OEO_00090001
    
    
Class: OEO_00090003

    Annotations: 
        <http://purl.obolibrary.org/obo/IAO_0000115> "A private funder is a funder that gives private money.",
        <http://purl.obolibrary.org/obo/IAO_0000233> "issue: https://github.com/OpenEnergyPlatform/ontology/issues/246
pull request: https://github.com/OpenEnergyPlatform/ontology/pull/776",
        rdfs:label "private funder"@en
    
    SubClassOf: 
        OEO_00090001
    
    
Class: OEO_00140009

    
Class: OEO_00140012

    
Class: OEO_00140013

    Annotations: 
        <http://purl.obolibrary.org/obo/IAO_0000115> "A gross domestic product is an economic value that represents the broadest measure of aggregate economic activity, measuring the total unduplicated market value of all final goods and services produced within a statistical area in a period.",
        <http://purl.obolibrary.org/obo/IAO_0000118> "GDP",
        <http://purl.obolibrary.org/obo/IAO_0000233> "issue: https://github.com/OpenEnergyPlatform/ontology/issues/454
pull request: https://github.com/OpenEnergyPlatform/ontology/pull/559
alternative term:
https://github.com/OpenEnergyPlatform/ontology/issues/675
https://github.com/OpenEnergyPlatform/ontology/pull/676",
        rdfs:label "gross domestic product"@en
    
    SubClassOf: 
        OEO_00140012
    
    
Class: OEO_00140023

    Annotations: 
        <http://purl.obolibrary.org/obo/IAO_0000115> "Gross value added is an economic value that is the value of goods and services produced in a sector of an economy, measuring that sector's contribution to gross domestic product (GDP). It is calculated as the monetary value of products and services produced, less the value of intermediate consumption.",
        <http://purl.obolibrary.org/obo/IAO_0000118> "GVA",
        <http://purl.obolibrary.org/obo/IAO_0000233> "issue: https://github.com/OpenEnergyPlatform/ontology/issues/455
pull request: https://github.com/OpenEnergyPlatform/ontology/pull/563
alternative term:
https://github.com/OpenEnergyPlatform/ontology/issues/675
https://github.com/OpenEnergyPlatform/ontology/pull/676",
        rdfs:label "gross value added"@en
    
    SubClassOf: 
        OEO_00140012
    
    
Class: OEO_00140040
    
    
Class: OEO_00140109

    Annotations: 
        <http://purl.obolibrary.org/obo/IAO_0000115> "A contract is a document that contains an agreement between two or more competent agents to which those agents agree to be legally bound.",
        <http://purl.obolibrary.org/obo/IAO_0000119> "https://spec.edmcouncil.org/fibo/ontology/FND/Agreements/Contracts/Contract",
        <http://purl.obolibrary.org/obo/IAO_0000233> "issue: https://github.com/OpenEnergyPlatform/ontology/issues/376
pull request: https://github.com/OpenEnergyPlatform/ontology/pull/756",
        rdfs:label "contract"@en
    
    SubClassOf: 
        <http://purl.obolibrary.org/obo/IAO_0000310>
    
    
Class: OEO_00140117

    Annotations: 
        <http://purl.obolibrary.org/obo/IAO_0000115> "Delivery time is a one-dimensional temporal region expressing the amount of time that it takes for goods that have been bought to arrive at the place where they are wanted.",
        <http://purl.obolibrary.org/obo/IAO_0000233> "issue: https://github.com/OpenEnergyPlatform/ontology/issues/376
pull request: https://github.com/OpenEnergyPlatform/ontology/pull/778",
        rdfs:label "delivery time"@en
    
    SubClassOf: 
        <http://purl.obolibrary.org/obo/BFO_0000038>
    
    
Class: OEO_00140118

    Annotations: 
        <http://purl.obolibrary.org/obo/IAO_0000115> "A delivery time point is a zero-dimensional temporal region expressing the point in time when goods that have been bought arrive at the place where they are wanted.",
        <http://purl.obolibrary.org/obo/IAO_0000233> "issue: https://github.com/OpenEnergyPlatform/ontology/issues/376
pull request: https://github.com/OpenEnergyPlatform/ontology/pull/778",
        rdfs:label "delivery time point"@en
    
    SubClassOf: 
        <http://purl.obolibrary.org/obo/BFO_0000148>
    
    
Class: OEO_00140119

    Annotations: 
        <http://purl.obolibrary.org/obo/IAO_0000115> "A sender is an agent who initiates a communication.",
        <http://purl.obolibrary.org/obo/IAO_0000233> "issue: https://github.com/OpenEnergyPlatform/ontology/issues/376
pull request: https://github.com/OpenEnergyPlatform/ontology/pull/778",
        rdfs:label "sender"@en
    
    SubClassOf: 
        OEO_00000051
    
    
Class: OEO_00140120

    Annotations: 
        <http://purl.obolibrary.org/obo/IAO_0000115> "A receiver is an agent who obtains information from a sender.",
        <http://purl.obolibrary.org/obo/IAO_0000233> "issue: https://github.com/OpenEnergyPlatform/ontology/issues/376
pull request: https://github.com/OpenEnergyPlatform/ontology/pull/778",
        rdfs:label "receiver"@en
    
    SubClassOf: 
        OEO_00000051
    
    
Class: OEO_00140121

    Annotations: 
        <http://purl.obolibrary.org/obo/IAO_0000115> "A bid is a document describing an offer made by an agent to another agent in an effort to exchange commodities or services via terms relating to price and quantity which will be part of the resulting contract.",
        <http://purl.obolibrary.org/obo/IAO_0000233> "issue: https://github.com/OpenEnergyPlatform/ontology/issues/376
pull request: https://github.com/OpenEnergyPlatform/ontology/pull/778",
        rdfs:label "bid"@en
    
    SubClassOf: 
        <http://purl.obolibrary.org/obo/IAO_0000310>
    
    
Class: OEO_00140122

    Annotations: 
        <http://purl.obolibrary.org/obo/IAO_0000115> "An award is a document that signifies that a supplier for a particular commodity or service specified in a bid has been accepted.",
        <http://purl.obolibrary.org/obo/IAO_0000233> "issue: https://github.com/OpenEnergyPlatform/ontology/issues/376
pull request: https://github.com/OpenEnergyPlatform/ontology/pull/778",
        rdfs:label "award"@en
    
    SubClassOf: 
        <http://purl.obolibrary.org/obo/IAO_0000310>
    
    
Class: OEO_00140123

    Annotations: 
        <http://purl.obolibrary.org/obo/IAO_0000115> "A provider is an agent that transfers commodities or services to other agents.",
        <http://purl.obolibrary.org/obo/IAO_0000119> "https://spec.edmcouncil.org/fibo/ontology/FND/ProductsAndServices/ProductsAndServices/ServiceProvider (adapted)",
        <http://purl.obolibrary.org/obo/IAO_0000233> "issue: https://github.com/OpenEnergyPlatform/ontology/issues/376
pull request: https://github.com/OpenEnergyPlatform/ontology/pull/778",
        rdfs:comment "The transfer is typically defined in a contract.",
        rdfs:label "provider"@en
    
    SubClassOf: 
        OEO_00000051
    
    
Class: OEO_00140124

    Annotations: 
        <http://purl.obolibrary.org/obo/IAO_0000115> "A service is a process that is an intangible actitvity performed by some agent for the benefit of another agent.",
        <http://purl.obolibrary.org/obo/IAO_0000119> "https://spec.edmcouncil.org/fibo/ontology/FND/ProductsAndServices/ProductsAndServices/Service (adapted)",
        <http://purl.obolibrary.org/obo/IAO_0000233> "issue: https://github.com/OpenEnergyPlatform/ontology/issues/376
pull request: https://github.com/OpenEnergyPlatform/ontology/pull/778",
        rdfs:label "service"@en
    
    SubClassOf: 
        <http://purl.obolibrary.org/obo/BFO_0000015>
    
    
Class: OEO_00140125

    Annotations: 
        <http://purl.obolibrary.org/obo/IAO_0000115> "A delivery interval is the duration between repeated deliveries of services or commodities.",
        <http://purl.obolibrary.org/obo/IAO_0000233> "issue: https://github.com/OpenEnergyPlatform/ontology/issues/256
pull request: https://github.com/OpenEnergyPlatform/ontology/pull/779",
        rdfs:comment "This duration is often contractually fixed and regular.",
        rdfs:label "delivery interval"@en
    
    SubClassOf: 
        OEO_00030035
    
    
Class: OEO_00140130

    Annotations: 
        <http://purl.obolibrary.org/obo/IAO_0000115> "A power plant operator is an agent that operates an electric utility generation station.",
        <http://purl.obolibrary.org/obo/IAO_0000233> "issue: https://github.com/OpenEnergyPlatform/ontology/issues/256
pull request: https://github.com/OpenEnergyPlatform/ontology/pull/779",
        rdfs:label "power plant operator"@en
    
    SubClassOf: 
        OEO_00000051
    
    
Class: OEO_00140131

    Annotations: 
        <http://purl.obolibrary.org/obo/IAO_0000115> "A trader that trades the power of fossil fuel power plants.",
        <http://purl.obolibrary.org/obo/IAO_0000233> "issue: https://github.com/OpenEnergyPlatform/ontology/issues/256
pull request: https://github.com/OpenEnergyPlatform/ontology/pull/779",
        rdfs:label "conventional trader"@en
    
    SubClassOf: 
        OEO_00040005
    
    
Class: OEO_00140136

    Annotations: 
        <http://purl.obolibrary.org/obo/IAO_0000115> "Dispatch assignment is a plan specification that refers to resource planning at a power plant (usually by the plant’s operator).",
        <http://purl.obolibrary.org/obo/IAO_0000233> "issue: https://github.com/OpenEnergyPlatform/ontology/issues/376
pull request: https://github.com/OpenEnergyPlatform/ontology/pull/792",
        rdfs:label "dispatch assignment"@en
    
    SubClassOf: 
        <http://purl.obolibrary.org/obo/IAO_0000104>
    
    
Class: OEO_00140137

    Annotations: 
        <http://purl.obolibrary.org/obo/IAO_0000115> "A power plant portfolio is an information content entity that describes a particular combination or mix of different power plants, e.g. renewables and fossil plants within one business unit or company or trader.",
        <http://purl.obolibrary.org/obo/IAO_0000233> "issue: https://github.com/OpenEnergyPlatform/ontology/issues/376
pull request: https://github.com/OpenEnergyPlatform/ontology/pull/792",
        rdfs:label "power plant portfolio"@en
    
    SubClassOf: 
        <http://purl.obolibrary.org/obo/IAO_0000030>
    
    
Class: OEO_00140140

    Annotations: 
        <http://purl.obolibrary.org/obo/IAO_0000115> "A demand trader is a trader that deals specifically with energy demand.",
        <http://purl.obolibrary.org/obo/IAO_0000233> "issue: https://github.com/OpenEnergyPlatform/ontology/issues/256
pull request: https://github.com/OpenEnergyPlatform/ontology/pull/793",
        rdfs:label "demand trader"@en
    
    SubClassOf: 
        OEO_00040005
    
    
Class: OEO_00140141

    Annotations: 
        <http://purl.obolibrary.org/obo/IAO_0000115> "A merit order is a plan specification that describes the dispatch ranking of power plants (electrical generation) based on ascending order of price.",
        <http://purl.obolibrary.org/obo/IAO_0000233> "issue: https://github.com/OpenEnergyPlatform/ontology/issues/256
pull request: https://github.com/OpenEnergyPlatform/ontology/pull/793",
        rdfs:label "merit order"@en
    
    SubClassOf: 
        <http://purl.obolibrary.org/obo/IAO_0000104>
    
    
Class: OEO_00140143

    Annotations: 
        <http://purl.obolibrary.org/obo/IAO_0000115> "A direct marketer is a trader who is the relay between the energy exchange and power plant operators.",
        <http://purl.obolibrary.org/obo/IAO_0000233> "issue: https://github.com/OpenEnergyPlatform/ontology/issues/256
pull request: https://github.com/OpenEnergyPlatform/ontology/pull/793",
        rdfs:label "direct marketer"@en
    
    SubClassOf: 
        OEO_00040005
    
    
Class: OEO_00140146

    Annotations: 
        <http://purl.obolibrary.org/obo/IAO_0000115> "Energy demand is a demand for energy.",
        <http://purl.obolibrary.org/obo/IAO_0000233> "issue: https://github.com/OpenEnergyPlatform/ontology/issues/794
pull request: https://github.com/OpenEnergyPlatform/ontology/pull/796",
        rdfs:label "energy demand"@en
    
    SubClassOf: 
        OEO_00140040
    
    
Class: OEO_00140149

    Annotations: 
        <http://purl.obolibrary.org/obo/IAO_0000115> "A transformative measure is a process that is an activity that has a direct impact on a specific variable in question.",
        <http://purl.obolibrary.org/obo/IAO_0000233> "issue: https://github.com/OpenEnergyPlatform/ontology/issues/444
pull request: https://github.com/OpenEnergyPlatform/ontology/pull/797",
        rdfs:label "transformative measure"@en
    
    SubClassOf: 
        <http://purl.obolibrary.org/obo/BFO_0000015>
    
    
Class: OEO_00140150

    Annotations: 
        <http://purl.obolibrary.org/obo/IAO_0000115> "A policy is a specifically dependent continuant that is a deliberate system of principles, rules and guidelines, adopted by an organisation to guide decision making with respect to particular situations and implemented to achieve stated goals.",
        <http://purl.obolibrary.org/obo/IAO_0000233> "issue: https://github.com/OpenEnergyPlatform/ontology/issues/444
pull request: https://github.com/OpenEnergyPlatform/ontology/pull/797

relations:
issue: https://github.com/OpenEnergyPlatform/ontology/issues/444
pull request: https://github.com/OpenEnergyPlatform/ontology/pull/853",
        rdfs:label "policy"@en
    
    SubClassOf: 
        <http://purl.obolibrary.org/obo/BFO_0000020>,
        OEO_00010121 some OEO_00030022,
        <http://purl.obolibrary.org/obo/BFO_0000051> some OEO_00140151
    
    
Class: OEO_00140151

    Annotations: 
        <http://purl.obolibrary.org/obo/IAO_0000115> "A policy instrument is a specifically dependent continuant that is an action by the government that is intended to promote the adoption of a (transformative) measure.",
        <http://purl.obolibrary.org/obo/IAO_0000233> "issue: https://github.com/OpenEnergyPlatform/ontology/issues/444
pull request: https://github.com/OpenEnergyPlatform/ontology/pull/797",
        rdfs:label "policy instrument"@en
    
    SubClassOf: 
        <http://purl.obolibrary.org/obo/BFO_0000020>,
        
            Annotations: <http://purl.obolibrary.org/obo/IAO_0000233> "issue: https://github.com/OpenEnergyPlatform/ontology/issues/444
pull request: https://github.com/OpenEnergyPlatform/ontology/pull/853"
        OEO_00010119 some OEO_00140149
    
    
Class: OEO_00140171

    Annotations: 
        <http://purl.obolibrary.org/obo/IAO_0000115> "An email address is an information content entity that identifies an email box to which messages are delivered.",
        <http://purl.obolibrary.org/obo/IAO_0000233> "issue: https://github.com/OpenEnergyPlatform/ontology/issues/818
pull request: https://github.com/OpenEnergyPlatform/ontology/pull/827",
        rdfs:label "email address"@en
    
    SubClassOf: 
        <http://purl.obolibrary.org/obo/IAO_0000030>
    
    
Class: OEO_00230013

    Annotations: 
        <http://purl.obolibrary.org/obo/IAO_0000115> "A population is an aggregate of people in a spatial region."@en,
        <http://purl.obolibrary.org/obo/IAO_0000233> "issue: https://github.com/OpenEnergyPlatform/ontology/issues/479
https://github.com/OpenEnergyPlatform/ontology/issues/301
pull request: https://github.com/OpenEnergyPlatform/ontology/pull/491"@en,
        rdfs:label "population"@en
    
    SubClassOf: 
        <http://purl.obolibrary.org/obo/BFO_0000027>
    
    
Class: OEO_00230014

    Annotations: 
        <http://purl.obolibrary.org/obo/IAO_0000115> "An urban population is a population living in urban areas, as defined by national statistical offices."@en,
        <http://purl.obolibrary.org/obo/IAO_0000119> "United Nations Population Division. World Urbanization Prospects: 2018 Revision."@en,
        <http://purl.obolibrary.org/obo/IAO_0000233> "issue: https://github.com/OpenEnergyPlatform/ontology/issues/479
https://github.com/OpenEnergyPlatform/ontology/issues/301
pull request: https://github.com/OpenEnergyPlatform/ontology/pull/491"@en,
        rdfs:label "urban population"@en
    
    SubClassOf: 
        OEO_00230013
    
    DisjointWith: 
        OEO_00230015
    
    
Class: OEO_00230015

    Annotations: 
        <http://purl.obolibrary.org/obo/IAO_0000115> "A rural population is a population living in rural areas, as defined by national statistical offices."@en,
        <http://purl.obolibrary.org/obo/IAO_0000119> "United Nations Population Division. World Urbanization Prospects: 2018 Revision."@en,
        <http://purl.obolibrary.org/obo/IAO_0000233> "issue: https://github.com/OpenEnergyPlatform/ontology/issues/301
https://github.com/OpenEnergyPlatform/ontology/issues/479
pull request: https://github.com/OpenEnergyPlatform/ontology/pull/491"@en,
        rdfs:label "rural population"@en
    
    SubClassOf: 
        OEO_00230013
    
    DisjointWith: 
        OEO_00230014
    
    
Class: OEO_00230016

    Annotations: 
        <http://purl.obolibrary.org/obo/IAO_0000115> "The labour force is the population of people ages 15 and older who supply labour to the production of goods and services.  It includes people who are currently employed and people who are unemployed but seeking work as well as first-time job-seekers."@en,
        <http://purl.obolibrary.org/obo/IAO_0000118> "labor force",
        <http://purl.obolibrary.org/obo/IAO_0000119> "https://databank.worldbank.org/reports.aspx?source=2&type=metadata&series=SL.TLF.TOTL.IN"@en,
        <http://purl.obolibrary.org/obo/IAO_0000233> "issue: https://github.com/OpenEnergyPlatform/ontology/issues/479
https://github.com/OpenEnergyPlatform/ontology/issues/301
pull request: https://github.com/OpenEnergyPlatform/ontology/pull/491"@en,
        rdfs:label "labour force"@en
    
    SubClassOf: 
        OEO_00230013
    
    
Class: OEO_00230017

    Annotations: 
        <http://purl.obolibrary.org/obo/IAO_0000115> "The working age population is the population of people aged 15 to 65."@en,
        <http://purl.obolibrary.org/obo/IAO_0000233> "issue: https://github.com/OpenEnergyPlatform/ontology/issues/301
https://github.com/OpenEnergyPlatform/ontology/issues/479
pull request: https://github.com/OpenEnergyPlatform/ontology/pull/491"@en,
        rdfs:label "working age population"@en
    
    SubClassOf: 
        OEO_00230013
    
    
Class: OEO_00240003

    
Class: OEO_00240021

    Annotations: 
        <http://purl.obolibrary.org/obo/IAO_0000115> "A discount rate is an economic value with the unit percent that refers to the interest rate used in discounted cash flow (DCF) analysis to determine the present value of future cash flows."@en,
        <http://purl.obolibrary.org/obo/IAO_0000233> "issue: https://github.com/OpenEnergyPlatform/ontology/issues/1049
pull request: https://github.com/OpenEnergyPlatform/ontology/pull/1077"@en,
        rdfs:label "discount rate"
    
    SubClassOf: 
        OEO_00140012,
        OEO_00040010 some <http://purl.obolibrary.org/obo/UO_0000187>
    
    
Class: OEO_00240036

    Annotations: 
        <http://purl.obolibrary.org/obo/IAO_0000115> "An import price is the monetary price for the import of a material entity."@en,
        <http://purl.obolibrary.org/obo/IAO_0000233> "issue: https://github.com/OpenEnergyPlatform/ontology/issues/1050
pull request: https://github.com/OpenEnergyPlatform/ontology/pull/1083",
        rdfs:label "import price"
    
    SubClassOf: 
        OEO_00040003
    
    
Class: OEO_00240037

    Annotations: 
        <http://purl.obolibrary.org/obo/IAO_0000115> "An export price is the monetary price for the export of a material entity."@en,
        <http://purl.obolibrary.org/obo/IAO_0000233> "issue: https://github.com/OpenEnergyPlatform/ontology/issues/1050
pull request: https://github.com/OpenEnergyPlatform/ontology/pull/1083",
        rdfs:label "export price"
    
    SubClassOf: 
        OEO_00040003
    
    
Individual: OEO_00000160

    Annotations: 
        <http://purl.obolibrary.org/obo/IAO_0000115> "The concept of \"energy balance\" is an accounting framework for the compilation and understanding of data on all energy products entering, exiting and being used in a country. The energy balance is the most complete statistical accounting of energy products and their flow in the economy. Columns of the energy balance represent energy products (fuels). Rows represent energy flows.

The energy balance expresses all forms of energy in a common accounting unit. The balance shows the relationships between supply, inputs to the energy transformation processes and their outputs as well as the actual energy consumption by different sectors of end-use.",
        <http://purl.obolibrary.org/obo/IAO_0000116> "This is a general description of an energy balance. A link to a complete Eurostat energy balance is provided under the URL for 'definition source'",
        <http://purl.obolibrary.org/obo/IAO_0000119> "https://ec.europa.eu/eurostat/statistics-explained/index.php/Energy_balance#What_is_an_energy_balance.3F",
        rdfs:label "eurostat energy balances"
    
    Types: 
        OEO_00000368
    
    
Individual: OEO_00000193

    Annotations: 
        <http://purl.obolibrary.org/obo/IAO_0000115> "Das Schema der Energiebilanzen umfasst eine Matrix von 33 Spalten und 68 Zeilen (einschließlich der Summenspalten und -zeilen). In der horizontalen Gliederung (Spalten) werden die Energieträger ausgewiesen, die der energetischen und nichtenergetischen Nutzung dienen. In der vertikalen Gliederung (Zeilen) werden für die jeweiligen Energieträger Aufkommen, Umwandlung und Verwendung erfasst.

Als Energieträger werden alle Quellen oder Stoffe bezeichnet, in denen Energie mechanisch, thermisch, chemisch oder physikalisch gespeichert ist. Fünf Kerngruppe werden bei der Energiebilanz unterschieden:

    Fossile Brennstoffe
    Erneuerbare Energien
    Strom
    Kernbrennstoffe
    Fernwärme

Bilanzebenen
Schematische Darstellung des Bilanzraums der deutschen Arbeitsgemeinschaft Energiebilanzen
Primär- und Endenergie sowie Umwandlungsverluste

Die Abgrenzung erfolgt in drei Bilanzbereichen:

    die Primärenergiebilanz,
    die Umwandlungsbilanz und
    der Endenergieverbrauch.

In der Primärenergiebilanz werden die Energieträger mit ihrem Mengenaufkommen bei der Gewinnung und Anlieferung nach folgenden Kriterien erfasst:

    inländische Gewinnung von Energieträgern,
    Außenhandel mit Energieträgern, unterteilt nach Einfuhr und Ausfuhr,
    Hochseebunkerungen (Heizöl, Dieselkraftstoff und Schmierstoffe für die nationale und internationale Seeschifffahrt in deutschen Häfen. Ohne Lieferungen an Binnen- und Küstenmotorschiffe und Fischerei, die zum Sektor Verkehr (Endenergieverbrauch) zählen.)
    Bestandsveränderungen, getrennt erfasst nach Bestandsentnahmen und -aufstockungen",
        <http://purl.obolibrary.org/obo/IAO_0000116> "The German Energy Balance is managed by the 'AG Energiebilanzen', where aso the energy balances can be found: https://ag-energiebilanzen.de/",
        <http://purl.obolibrary.org/obo/IAO_0000119> "https://de.wikipedia.org/w/index.php?title=Energiebilanz_(Energiewirtschaft)&oldid=176259115",
        rdfs:label "german energy balances"
    
    Types: 
        OEO_00000368
    
    
Individual: OEO_00000242

    Annotations: 
        <http://purl.obolibrary.org/obo/IAO_0000115> "CRF sectors (IPCC 2006) is a version of the common reporting format that was used for national greenhouse gas inventories since the year 2015. It implements the 2006 IPCC Guidelines for National Greenhouse Gas Inventories (with some deviations).",
        <http://purl.obolibrary.org/obo/IAO_0000233> "issue: https://github.com/OpenEnergyPlatform/ontology/issues/461
pull request: https://github.com/OpenEnergyPlatform/ontology/pull/578",
        rdfs:label "CRF sectors (IPCC 2006)"
    
    Types: 
        OEO_00010055
    
    Facts:  
     OEO_00000504  OEO_00000242
    
    
Individual: OEO_00000243

    Annotations: 
        <http://purl.obolibrary.org/obo/IAO_0000115> "CRF sectors (IPCC 1996) is a version of the common reporting format that was used for national greenhouse gas inventories until the year 2014. It implements the Revised 1996 IPCC Guidelines for National Greenhouse Gas Inventories (with some deviations).",
        <http://purl.obolibrary.org/obo/IAO_0000233> "issue: https://github.com/OpenEnergyPlatform/ontology/issues/461
pull request: https://github.com/OpenEnergyPlatform/ontology/pull/578",
        rdfs:label "CRF sectors (IPCC 1996)"
    
    Types: 
        OEO_00010055
    
    
Individual: OEO_00000291

    Annotations: 
        <http://purl.obolibrary.org/obo/IAO_0000115> "The Statistical classification of economic activities in the European Community, abbreviated as NACE, is the classification of economic activities in the European Union (EU); the term NACE is derived from the French Nomenclature statistique des activités économiques dans la Communauté européenne. Various NACE versions have been developed since 1970.

NACE is a four-digit classification providing the framework for collecting and presenting a large range of statistical data according to economic activity in the fields of economic statistics (e.g. production, employment and national accounts) and in other statistical domains developed within the European statistical system (ESS).",
        <http://purl.obolibrary.org/obo/IAO_0000119> "https://ec.europa.eu/eurostat/statistics-explained/index.php?title=Glossary:Statistical_classification_of_economic_activities_in_the_European_Community_(NACE)",
        rdfs:label "nace_ sectors"
    
    Types: 
        OEO_00000368
    
    
Individual: OEO_00000355

    Annotations: 
        <http://purl.obolibrary.org/obo/IAO_0000116> "The Renewable energy Directive has been revised, but this should have had no impacts on the sectoral definitions. Factsheet on revision: https://ec.europa.eu/energy/sites/ener/files/documents/directive_renewable_factsheet.pdf",
        <http://purl.obolibrary.org/obo/IAO_0000119> "https://eur-lex.europa.eu/legal-content/EN/ALL/?uri=CELEX:32009L0028",
        rdfs:label "renewable_ energy_ directive_ sectors"
    
    Types: 
        OEO_00000368
    
    
Individual: OEO_00010038

    Annotations: 
        OEO_00010037 "CRF 1",
        <http://purl.obolibrary.org/obo/IAO_0000115> "The CRF sector (IPCC 2006) energy is a sector defined by the 2006 IPCC Guidelines for National Greenhouse Gas Inventories:
All GHG emissions arising from combustion and fugitive releases of fuels. Emissions from the non-energy uses of fuels are generally not included here, but reported under Industrial Processes and Product Use.",
        <http://purl.obolibrary.org/obo/IAO_0000119> "2006 IPCC Guidelines for National Greenhouse Gas Inventories, Volume 2, Chapter 2.2, https://www.ipcc-nggip.iges.or.jp/public/2006gl/",
        <http://purl.obolibrary.org/obo/IAO_0000233> "issue: https://github.com/OpenEnergyPlatform/ontology/issues/461
pull request: https://github.com/OpenEnergyPlatform/ontology/pull/523",
        rdfs:label "CRF sector (IPCC 2006): energy"
    
    Types: 
        OEO_00000367
    
    Facts:  
     OEO_00000504  OEO_00000242,
     <http://purl.obolibrary.org/obo/BFO_0000051>  OEO_00010040,
     <http://purl.obolibrary.org/obo/BFO_0000051>  OEO_00010041,
     <http://purl.obolibrary.org/obo/BFO_0000051>  OEO_00010042,
     <http://purl.obolibrary.org/obo/BFO_0000051>  OEO_00010043,
     <http://purl.obolibrary.org/obo/BFO_0000051>  OEO_00010044
    
    
Individual: OEO_00010039

    Annotations: 
        OEO_00010037 "CRF 1.A",
        <http://purl.obolibrary.org/obo/IAO_0000115> "The CRF sector (IPCC 2006) 'fuel combustion' is a sector defined by the 2006 IPCC Guidelines for National Greenhouse Gas Inventories:
Emissions from the intentional oxidation of materials within an apparatus that is designed to raise heat and provide it either as heat or as mechanical work to a process or for use away from the apparatus.",
        <http://purl.obolibrary.org/obo/IAO_0000119> "2006 IPCC Guidelines for National Greenhouse Gas Inventories, Volume 2, Chapter 2.2, https://www.ipcc-nggip.iges.or.jp/public/2006gl/",
        <http://purl.obolibrary.org/obo/IAO_0000233> "issue: https://github.com/OpenEnergyPlatform/ontology/issues/461
pull request: https://github.com/OpenEnergyPlatform/ontology/pull/523",
        rdfs:label "CRF sector (IPCC 2006): fuel combustion"
    
    Types: 
        OEO_00000367
    
    Facts:  
     OEO_00000504  OEO_00000242,
     <http://purl.obolibrary.org/obo/BFO_0000050>  OEO_00010038
    
    
Individual: OEO_00010040

    Annotations: 
        OEO_00010037 "CRF 1.A.1",
        <http://purl.obolibrary.org/obo/IAO_0000115> "The CRF sector (IPCC 2006) 'energy industry' is an energy transformation sector defined by the 2006 IPCC Guidelines for National Greenhouse Gas Inventories:
Comprises emissions from fuels combusted by the fuel extraction or energy-producing industries.",
        <http://purl.obolibrary.org/obo/IAO_0000119> "2006 IPCC Guidelines for National Greenhouse Gas Inventories, Volume 2, Chapter 2.2, https://www.ipcc-nggip.iges.or.jp/public/2006gl/",
        <http://purl.obolibrary.org/obo/IAO_0000233> "issue: https://github.com/OpenEnergyPlatform/ontology/issues/461
pull request: https://github.com/OpenEnergyPlatform/ontology/pull/523

add has part relations:
issue: https://github.com/OpenEnergyPlatform/ontology/issues/858
pull request: https://github.com/OpenEnergyPlatform/ontology/pull/941",
        rdfs:label "CRF sector (IPCC 2006): energy industry"
    
    Types: 
        OEO_00000158
    
    Facts:  
     OEO_00000504  OEO_00000242,
     <http://purl.obolibrary.org/obo/BFO_0000050>  OEO_00010039,
     <http://purl.obolibrary.org/obo/BFO_0000051>  OEO_00010158,
     <http://purl.obolibrary.org/obo/BFO_0000051>  OEO_00010159,
     <http://purl.obolibrary.org/obo/BFO_0000051>  OEO_00010160
    
    
Individual: OEO_00010041

    Annotations: 
        OEO_00010037 "CRF 1.A.2",
        <http://purl.obolibrary.org/obo/IAO_0000115> "The CRF sector (IPCC 2006) 'manufacturing industries and construction' is an industry sector defined by the 2006 IPCC Guidelines for National Greenhouse Gas Inventories:
Emissions from combustion of fuels in industry. Also includes combustion for the generation of electricity and heat for own use in these industries.",
        <http://purl.obolibrary.org/obo/IAO_0000119> "2006 IPCC Guidelines for National Greenhouse Gas Inventories, Volume 2, Chapter 2.2, https://www.ipcc-nggip.iges.or.jp/public/2006gl/",
        <http://purl.obolibrary.org/obo/IAO_0000233> "issue: https://github.com/OpenEnergyPlatform/ontology/issues/461
pull request: https://github.com/OpenEnergyPlatform/ontology/pull/523",
        rdfs:label "CRF sector (IPCC 2006): manufacturing industries and construction"
    
    Types: 
        OEO_00000227
    
    Facts:  
     OEO_00000504  OEO_00000242,
     <http://purl.obolibrary.org/obo/BFO_0000050>  OEO_00010039
    
    
Individual: OEO_00010042

    Annotations: 
        OEO_00010037 "CRF 1.A.3",
        <http://purl.obolibrary.org/obo/IAO_0000115> "The CRF sector (IPCC 2006) 'transport' is a transport sector defined by the 2006 IPCC Guidelines for National Greenhouse Gas Inventories:
Emissions from the combustion and evaporation of fuel for all transport activity (excluding military transport), regardless of the sector, specifiedby sub-categories below. Emissions from fuel sold to any air or marine vessel engaged in international transport (1 A 3 a i and 1 A 3 d i) should as far as possible be excluded from the totals and subtotals in this category and should be reported separately.",
        <http://purl.obolibrary.org/obo/IAO_0000119> "2006 IPCC Guidelines for National Greenhouse Gas Inventories, Volume 2, Chapter 3.1, https://www.ipcc-nggip.iges.or.jp/public/2006gl/",
        <http://purl.obolibrary.org/obo/IAO_0000233> "issue: https://github.com/OpenEnergyPlatform/ontology/issues/461
pull request: https://github.com/OpenEnergyPlatform/ontology/pull/523",
        rdfs:label "CRF sector (IPCC 2006): transport"
    
    Types: 
        OEO_00000422
    
    Facts:  
     OEO_00000504  OEO_00000242,
     <http://purl.obolibrary.org/obo/BFO_0000050>  OEO_00010039
    
    
Individual: OEO_00010043

    Annotations: 
        OEO_00010037 "CRF 1.A.4",
        <http://purl.obolibrary.org/obo/IAO_0000115> "The CRF sector (IPCC 2006) 'fuel combustion - other sectors' is an energy demand sector defined by the 2006 IPCC Guidelines for National Greenhouse Gas Inventories:
Emissions from combustion activities as described below, including combustion for the generation of electricity and heat for own use in these sectors.",
        <http://purl.obolibrary.org/obo/IAO_0000119> "2006 IPCC Guidelines for National Greenhouse Gas Inventories, Volume 2, Chapter 2.2, https://www.ipcc-nggip.iges.or.jp/public/2006gl/",
        <http://purl.obolibrary.org/obo/IAO_0000233> "issue: https://github.com/OpenEnergyPlatform/ontology/issues/461
pull request: https://github.com/OpenEnergyPlatform/ontology/pull/523",
        rdfs:label "CRF sector (IPCC 2006): fuel combustion - other sectors"
    
    Types: 
        OEO_00000128
    
    Facts:  
     OEO_00000504  OEO_00000242,
     <http://purl.obolibrary.org/obo/BFO_0000050>  OEO_00010039,
     <http://purl.obolibrary.org/obo/BFO_0000051>  OEO_00010052,
     <http://purl.obolibrary.org/obo/BFO_0000051>  OEO_00010053
    
    
Individual: OEO_00010044

    Annotations: 
        OEO_00010037 "CRF 1.A.5",
        <http://purl.obolibrary.org/obo/IAO_0000115> "The CRF sector (IPCC 2006) 'fuel combustion' is a sector defined by the 2006 IPCC Guidelines for National Greenhouse Gas Inventories:
All remaining emissions from fuel combustion that are not specified elsewhere. Include emissions from fuel delivered to the military in the country and delivered to the military of other countries that are not engaged in multilateral operations.",
        <http://purl.obolibrary.org/obo/IAO_0000119> "2006 IPCC Guidelines for National Greenhouse Gas Inventories, Volume 2, Chapter 2.2, https://www.ipcc-nggip.iges.or.jp/public/2006gl/",
        <http://purl.obolibrary.org/obo/IAO_0000233> "issue: https://github.com/OpenEnergyPlatform/ontology/issues/461
pull request: https://github.com/OpenEnergyPlatform/ontology/pull/523",
        rdfs:label "CRF sector (IPCC 2006): fuel combustion - other"
    
    Types: 
        OEO_00000367
    
    Facts:  
     OEO_00000504  OEO_00000242,
     <http://purl.obolibrary.org/obo/BFO_0000050>  OEO_00010039
    
    
Individual: OEO_00010046

    Annotations: 
        OEO_00010037 "CRF 2",
        <http://purl.obolibrary.org/obo/IAO_0000115> "The CRF sector (IPCC 2006) 'energy industrial processes and product use' (IPPU) is an industry sector defined by the 2006 IPCC Guidelines for National Greenhouse Gas Inventories:
It covers greenhouse gas emissions occurring from industrial processes, from the use of greenhouse gases in products, and from non-energy uses of fossil fuel carbon.",
        <http://purl.obolibrary.org/obo/IAO_0000118> "IPPU",
        <http://purl.obolibrary.org/obo/IAO_0000119> "2006 IPCC Guidelines for National Greenhouse Gas Inventories, Volume 3, Chapter 1.1, https://www.ipcc-nggip.iges.or.jp/public/2006gl/",
        <http://purl.obolibrary.org/obo/IAO_0000233> "issue: https://github.com/OpenEnergyPlatform/ontology/issues/461
pull request: https://github.com/OpenEnergyPlatform/ontology/pull/578

add has part relations:
issue: https://github.com/OpenEnergyPlatform/ontology/issues/858
pull request: https://github.com/OpenEnergyPlatform/ontology/pull/941",
        rdfs:label "CRF sector (IPCC 2006): industrial processes and product use"
    
    Types: 
        OEO_00000227
    
    Facts:  
     OEO_00000504  OEO_00000242,
     <http://purl.obolibrary.org/obo/BFO_0000051>  OEO_00010164,
     <http://purl.obolibrary.org/obo/BFO_0000051>  OEO_00010166,
     <http://purl.obolibrary.org/obo/BFO_0000051>  OEO_00010167,
     <http://purl.obolibrary.org/obo/BFO_0000051>  OEO_00010169,
     <http://purl.obolibrary.org/obo/BFO_0000051>  OEO_00010170,
     <http://purl.obolibrary.org/obo/BFO_0000051>  OEO_00010171,
     <http://purl.obolibrary.org/obo/BFO_0000051>  OEO_00010172,
     <http://purl.obolibrary.org/obo/BFO_0000051>  OEO_00010173
    
    
Individual: OEO_00010047

    Annotations: 
        OEO_00010037 "CRF 3",
        <http://purl.obolibrary.org/obo/IAO_0000233> "issue: https://github.com/OpenEnergyPlatform/ontology/issues/461
pull request: https://github.com/OpenEnergyPlatform/ontology/pull/578

add has part axioms:
issue: https://github.com/OpenEnergyPlatform/ontology/issues/858
pull request: https://github.com/OpenEnergyPlatform/ontology/pull/941",
        rdfs:comment "The CRF sector (IPCC 2006) 'agriculture' is an agriculture, forestry and land use sector defined by the 2006 IPCC Guidelines for National Greenhouse Gas Inventories",
        rdfs:label "CRF sector (IPCC 2006): agriculture"
    
    Types: 
        OEO_00010035
    
    Facts:  
     OEO_00000504  OEO_00000242,
     <http://purl.obolibrary.org/obo/BFO_0000051>  OEO_00010179,
     <http://purl.obolibrary.org/obo/BFO_0000051>  OEO_00010180,
     <http://purl.obolibrary.org/obo/BFO_0000051>  OEO_00010181,
     <http://purl.obolibrary.org/obo/BFO_0000051>  OEO_00010182,
     <http://purl.obolibrary.org/obo/BFO_0000051>  OEO_00010183,
     <http://purl.obolibrary.org/obo/BFO_0000051>  OEO_00010184,
     <http://purl.obolibrary.org/obo/BFO_0000051>  OEO_00010185,
     <http://purl.obolibrary.org/obo/BFO_0000051>  OEO_00010186,
     <http://purl.obolibrary.org/obo/BFO_0000051>  OEO_00010187,
     <http://purl.obolibrary.org/obo/BFO_0000051>  OEO_00010188
    
    
Individual: OEO_00010048

    Annotations: 
        OEO_00010037 "CRF 4",
        <http://purl.obolibrary.org/obo/IAO_0000115> "The CRF sector (IPCC 2006) 'land use, land-use change and forestry' (LULUCF) is an agriculture, forestry and land use sector defined by the 2006 IPCC Guidelines for National Greenhouse Gas Inventories",
        <http://purl.obolibrary.org/obo/IAO_0000118> "LULUCF",
        <http://purl.obolibrary.org/obo/IAO_0000233> "issue: https://github.com/OpenEnergyPlatform/ontology/issues/461
pull request: https://github.com/OpenEnergyPlatform/ontology/pull/578

add has part axioms:
issue: https://github.com/OpenEnergyPlatform/ontology/issues/858
pull request: https://github.com/OpenEnergyPlatform/ontology/pull/941",
        rdfs:label "CRF sector (IPCC 2006): land use, land-use change and forestry"
    
    Types: 
        OEO_00010035
    
    Facts:  
     OEO_00000504  OEO_00000242,
     <http://purl.obolibrary.org/obo/BFO_0000051>  OEO_00010189,
     <http://purl.obolibrary.org/obo/BFO_0000051>  OEO_00010190,
     <http://purl.obolibrary.org/obo/BFO_0000051>  OEO_00010192,
     <http://purl.obolibrary.org/obo/BFO_0000051>  OEO_00010193,
     <http://purl.obolibrary.org/obo/BFO_0000051>  OEO_00010194,
     <http://purl.obolibrary.org/obo/BFO_0000051>  OEO_00010195,
     <http://purl.obolibrary.org/obo/BFO_0000051>  OEO_00010196
    
    SameAs: 
        OEO_00010071,
        OEO_00010135
    
    
Individual: OEO_00010049

    Annotations: 
        OEO_00010037 "CRF 5",
        <http://purl.obolibrary.org/obo/IAO_0000115> "The CRF sector (IPCC 2006) 'waste' is a waste and wastewater sector defined by the 2006 IPCC Guidelines for National Greenhouse Gas Inventories:
Carbon dioxide (CO2), methane (CH4) and nitrous oxide (N2O) emissions from following categories: Solid waste disposal, Biological treatment of solid waste, 
Incineration and open burning of waste, Wastewater treatment and discharge.",
        <http://purl.obolibrary.org/obo/IAO_0000119> "2006 IPCC Guidelines for National Greenhouse Gas Inventories, Volume 5, Chapter 1.1, https://www.ipcc-nggip.iges.or.jp/public/2006gl/",
        <http://purl.obolibrary.org/obo/IAO_0000233> "issue: https://github.com/OpenEnergyPlatform/ontology/issues/461
pull request: https://github.com/OpenEnergyPlatform/ontology/pull/578

add has part axioms and improve definition:
issue: https://github.com/OpenEnergyPlatform/ontology/issues/858
pull request: https://github.com/OpenEnergyPlatform/ontology/pull/941",
        rdfs:label "CRF sector (IPCC 2006): waste"
    
    Types: 
        OEO_00010036
    
    Facts:  
     OEO_00000504  OEO_00000242,
     <http://purl.obolibrary.org/obo/BFO_0000051>  OEO_00010174,
     <http://purl.obolibrary.org/obo/BFO_0000051>  OEO_00010175,
     <http://purl.obolibrary.org/obo/BFO_0000051>  OEO_00010176,
     <http://purl.obolibrary.org/obo/BFO_0000051>  OEO_00010177,
     <http://purl.obolibrary.org/obo/BFO_0000051>  OEO_00010178
    
    
Individual: OEO_00010050

    Annotations: 
        OEO_00010037 "CRF 6",
        <http://purl.obolibrary.org/obo/IAO_0000115> "The CRF sector (IPCC 2006) 'other' is a sector defined by the 2006 IPCC Guidelines for National Greenhouse Gas Inventories",
        <http://purl.obolibrary.org/obo/IAO_0000233> "issue: https://github.com/OpenEnergyPlatform/ontology/issues/461
pull request: https://github.com/OpenEnergyPlatform/ontology/pull/578",
        rdfs:label "CRF sector (IPCC 2006): other"
    
    Types: 
        OEO_00000367
    
    Facts:  
     OEO_00000504  OEO_00000242
    
    
Individual: OEO_00010052

    Annotations: 
        OEO_00010037 "CRF 1.A.4.a",
        <http://purl.obolibrary.org/obo/IAO_0000115> "The CRF sector (IPCC 2006) 'commercial and institutional' is a commercial sector defined by the 2006 IPCC Guidelines for National Greenhouse Gas Inventories:
Emissions from fuel combustion in commercial and institutional buildings.",
        <http://purl.obolibrary.org/obo/IAO_0000119> "2006 IPCC Guidelines for National Greenhouse Gas Inventories, Volume 3, Chapter 1.1, https://www.ipcc-nggip.iges.or.jp/public/2006gl/",
        <http://purl.obolibrary.org/obo/IAO_0000233> "issue: https://github.com/OpenEnergyPlatform/ontology/issues/461
pull request: https://github.com/OpenEnergyPlatform/ontology/pull/578",
        rdfs:label "CRF sector (IPCC 2006): commercial and institutional"
    
    Types: 
        OEO_00000405
    
    Facts:  
     OEO_00000504  OEO_00000242,
     <http://purl.obolibrary.org/obo/BFO_0000050>  OEO_00010043
    
    
Individual: OEO_00010053

    Annotations: 
        OEO_00010037 "CRF 1.A.4.b",
        <http://purl.obolibrary.org/obo/IAO_0000115> "The CRF sector (IPCC 2006) 'residential' is a household sector defined by the 2006 IPCC Guidelines for National Greenhouse Gas Inventories:
All emissions from fuel combustion in households.",
        <http://purl.obolibrary.org/obo/IAO_0000119> "2006 IPCC Guidelines for National Greenhouse Gas Inventories, Volume 2, Chapter 2.2, https://www.ipcc-nggip.iges.or.jp/public/2006gl/",
        <http://purl.obolibrary.org/obo/IAO_0000233> "issue: https://github.com/OpenEnergyPlatform/ontology/issues/461
pull request: https://github.com/OpenEnergyPlatform/ontology/pull/578",
        rdfs:label "CRF sector (IPCC 2006): residential"
    
    Types: 
        OEO_00000214
    
    Facts:  
     OEO_00000504  OEO_00000242,
     <http://purl.obolibrary.org/obo/BFO_0000050>  OEO_00010043
    
    
Individual: OEO_00010054

    Annotations: 
        OEO_00010037 "CRF 1.A.4.c",
        <http://purl.obolibrary.org/obo/IAO_0000115> "The CRF sector (IPCC 2006) 'agriculture, forestry and fishing' is an energy demand sector defined by the 2006 IPCC Guidelines for National Greenhouse Gas Inventories:
Emissions from fuel combustion in agriculture, forestry, fishing and fishing industries such as fish farms.",
        <http://purl.obolibrary.org/obo/IAO_0000119> "2006 IPCC Guidelines for National Greenhouse Gas Inventories, Volume 2, Chapter 2.2, https://www.ipcc-nggip.iges.or.jp/public/2006gl/",
        <http://purl.obolibrary.org/obo/IAO_0000233> "issue: https://github.com/OpenEnergyPlatform/ontology/issues/461
pull request: https://github.com/OpenEnergyPlatform/ontology/pull/578",
        rdfs:label "CRF sector (IPCC 2006): agriculture, forestry and fishing"
    
    Types: 
        OEO_00000128
    
    Facts:  
     OEO_00000504  OEO_00000242,
     <http://purl.obolibrary.org/obo/BFO_0000050>  OEO_00010043
    
    
Individual: OEO_00010056

    Annotations: 
        <http://purl.obolibrary.org/obo/IAO_0000115> "The KSG sector division is a sector division defined in annex 1 of the Bundes-Klimaschutzgesetz (KSG).",
        <http://purl.obolibrary.org/obo/IAO_0000233> "issue: https://github.com/OpenEnergyPlatform/ontology/issues/580
pull request: https://github.com/OpenEnergyPlatform/ontology/pull/595",
        rdfs:label "KSG sector division"
    
    Types: 
        OEO_00000368
    
    
Individual: OEO_00010057

    Annotations: 
        OEO_00010037 "CRF 1.B",
        <http://purl.obolibrary.org/obo/IAO_0000115> "The CRF sector (IPCC 2006) 'fugitive emissions from fuels' is a sector defined by the 2006 IPCC Guidelines for National Greenhouse Gas Inventories:
Includes all intentional and unintentional emissions from the extraction, processing, storage and transport of solid fuel to the point of final use.",
        <http://purl.obolibrary.org/obo/IAO_0000119> "2006 IPCC Guidelines for National Greenhouse Gas Inventories, Volume 1, Chapter 8.5, https://www.ipcc-nggip.iges.or.jp/public/2006gl/",
        <http://purl.obolibrary.org/obo/IAO_0000233> "issue: https://github.com/OpenEnergyPlatform/ontology/issues/580
pull request: https://github.com/OpenEnergyPlatform/ontology/pull/595",
        rdfs:label "CRF sector (IPCC 2006): fugitive emissions from fuels"
    
    Types: 
        OEO_00000367
    
    Facts:  
     OEO_00000504  OEO_00000242,
     <http://purl.obolibrary.org/obo/BFO_0000050>  OEO_00010038,
     <http://purl.obolibrary.org/obo/BFO_0000051>  OEO_00010161,
     <http://purl.obolibrary.org/obo/BFO_0000051>  OEO_00010162
    
    
Individual: OEO_00010058

    Annotations: 
        OEO_00010037 "CRF 1.C",
        <http://purl.obolibrary.org/obo/IAO_0000115> "The CRF sector (IPCC 2006) 'CO2 transport and storage' is a sector defined by the 2006 IPCC Guidelines for National Greenhouse Gas Inventories:
Carbon dioxide (CO2) capture and storage (CCS) involves the capture of CO2 from anthropogenic sources, its transport to a storage location and its long-term isolation from the atmosphere. Emissions associated with CO2 transport, injection and storage are covered under category 1C. Emissions (and reductions) associated with CO2 capture should be reported under the IPCC Sector in which capture takes place (e.g. Fuel Combustion or Industrial Activities).",
        <http://purl.obolibrary.org/obo/IAO_0000119> "2006 IPCC Guidelines for National Greenhouse Gas Inventories, Volume 1, Chapter 8.5, https://www.ipcc-nggip.iges.or.jp/public/2006gl/",
        <http://purl.obolibrary.org/obo/IAO_0000233> "issue: https://github.com/OpenEnergyPlatform/ontology/issues/580
pull request: https://github.com/OpenEnergyPlatform/ontology/pull/595",
        rdfs:label "CRF sector (IPCC 2006): CO2 transport and storage"
    
    Types: 
        OEO_00000367
    
    Facts:  
     OEO_00000504  OEO_00000242,
     <http://purl.obolibrary.org/obo/BFO_0000050>  OEO_00010038
    
    DifferentFrom: 
        OEO_00010229
    
    
Individual: OEO_00010059

    Annotations: 
        OEO_00010037 "CRF 1.A.3.a",
        <http://purl.obolibrary.org/obo/IAO_0000115> "The CRF sector (IPCC 2006) 'domestic aviation' is a transport sector defined by the 2006 IPCC Guidelines for National Greenhouse Gas Inventories:
Emissions from civil domestic passenger and freight traffic that departs and arrives in the same country (commercial, private, agriculture, etc.), including take-offs and landings for these flight stages. Note that this may include journeys of considerable length between two airports in a country (e.g. San Francisco to Honolulu). Exclude military, which should be reported under 1 A 5 b.",
        <http://purl.obolibrary.org/obo/IAO_0000119> "2006 IPCC Guidelines for National Greenhouse Gas Inventories, Volume 1, Chapter 8.5, https://www.ipcc-nggip.iges.or.jp/public/2006gl/",
        <http://purl.obolibrary.org/obo/IAO_0000233> "issue: https://github.com/OpenEnergyPlatform/ontology/issues/580
pull request: https://github.com/OpenEnergyPlatform/ontology/pull/595",
        rdfs:label "CRF sector (IPCC 2006): domestic aviation"
    
    Types: 
        OEO_00000422
    
    Facts:  
     OEO_00000504  OEO_00000242,
     <http://purl.obolibrary.org/obo/BFO_0000050>  OEO_00010042
    
    DifferentFrom: 
        OEO_00010201
    
    
Individual: OEO_00010060

    Annotations: 
        OEO_00010037 "CRF 1.A.3.b",
        <http://purl.obolibrary.org/obo/IAO_0000115> "The CRF sector (IPCC 2006) 'road transport' is a transport sector defined by the 2006 IPCC Guidelines for National Greenhouse Gas Inventories:
All combustion and evaporative emissions arising from fuel use in road vehicles, including the use of agricultural vehicles on paved roads.",
        <http://purl.obolibrary.org/obo/IAO_0000119> "2006 IPCC Guidelines for National Greenhouse Gas Inventories, Volume 1, Chapter 8.5, https://www.ipcc-nggip.iges.or.jp/public/2006gl/",
        <http://purl.obolibrary.org/obo/IAO_0000233> "issue: https://github.com/OpenEnergyPlatform/ontology/issues/580
pull request: https://github.com/OpenEnergyPlatform/ontology/pull/595",
        rdfs:label "CRF sector (IPCC 2006): road transportation"
    
    Types: 
        OEO_00000422
    
    Facts:  
     OEO_00000504  OEO_00000242,
     <http://purl.obolibrary.org/obo/BFO_0000050>  OEO_00010042
    
    
Individual: OEO_00010061

    Annotations: 
        OEO_00010037 "CRF 1.A.3.c",
        <http://purl.obolibrary.org/obo/IAO_0000115> "2006 IPCC Guidelines for National Greenhouse Gas Inventories, Volume 1, Chapter 8.5, https://www.ipcc-nggip.iges.or.jp/public/2006gl/",
        <http://purl.obolibrary.org/obo/IAO_0000115> "The CRF sector (IPCC 2006) 'railways' is a transport sector defined by the 2006 IPCC Guidelines for National Greenhouse Gas Inventories:
Emissions from railway transport for both freight and passenger traffic routes.",
        <http://purl.obolibrary.org/obo/IAO_0000115> "issue: https://github.com/OpenEnergyPlatform/ontology/issues/580
pull request: https://github.com/OpenEnergyPlatform/ontology/pull/595",
        rdfs:label "CRF sector (IPCC 2006): railways"
    
    Types: 
        OEO_00000422
    
    Facts:  
     OEO_00000504  OEO_00000242,
     <http://purl.obolibrary.org/obo/BFO_0000050>  OEO_00010042
    
    
Individual: OEO_00010062

    Annotations: 
        OEO_00010037 "CRF 1.A.3.d",
        <http://purl.obolibrary.org/obo/IAO_0000115> "The CRF sector (IPCC 2006) 'domestic navigation' is a transport sector defined by the 2006 IPCC Guidelines for National Greenhouse Gas Inventories:
Emissions from fuels used by vessels of all flags that depart and arrive in the same country (exclude fishing, which should be reported under 1 A 4 c iii, and military, which should be reported under 1 A 5 b). Note that this may include journeys of considerable length between two ports in a country (e.g. San Francisco to Honolulu).",
        <http://purl.obolibrary.org/obo/IAO_0000119> "2006 IPCC Guidelines for National Greenhouse Gas Inventories, Volume 1, Chapter 8.5, https://www.ipcc-nggip.iges.or.jp/public/2006gl/",
        <http://purl.obolibrary.org/obo/IAO_0000233> "issue: https://github.com/OpenEnergyPlatform/ontology/issues/580
pull request: https://github.com/OpenEnergyPlatform/ontology/pull/595",
        rdfs:label "CRF sector (IPCC 2006): domestic navigation"
    
    Types: 
        OEO_00000422
    
    Facts:  
     OEO_00000504  OEO_00000242,
     <http://purl.obolibrary.org/obo/BFO_0000050>  OEO_00010042
    
    DifferentFrom: 
        OEO_00010202
    
    
Individual: OEO_00010063

    Annotations: 
        OEO_00010037 "CRF 1.A.3.e",
        <http://purl.obolibrary.org/obo/IAO_0000115> "The CRF sector (IPCC 2006) 'other transportation' is a transport sector defined by the 2006 IPCC Guidelines for National Greenhouse Gas Inventories:
Combustion emissions from all remaining transport activities including pipeline transportation, ground activities in airports and harbours, and off-road activities not otherwise reported under 1 A 4 c Agriculture or 1 A 2. Manufacturing Industries and Construction. Military transport should be reported under 1 A 5.",
        <http://purl.obolibrary.org/obo/IAO_0000119> "2006 IPCC Guidelines for National Greenhouse Gas Inventories, Volume 1, Chapter 8.5, https://www.ipcc-nggip.iges.or.jp/public/2006gl/",
        <http://purl.obolibrary.org/obo/IAO_0000233> "issue: https://github.com/OpenEnergyPlatform/ontology/issues/580
pull request: https://github.com/OpenEnergyPlatform/ontology/pull/595",
        rdfs:label "CRF sector (IPCC 2006): other transportation"
    
    Types: 
        OEO_00000422
    
    Facts:  
     OEO_00000504  OEO_00000242,
     <http://purl.obolibrary.org/obo/BFO_0000050>  OEO_00010042
    
    
Individual: OEO_00010064

    Annotations: 
        OEO_00010037 "CRF 1.A.3.e.i",
        <http://purl.obolibrary.org/obo/IAO_0000115> "The CRF sector (IPCC 2006) 'pipeline transport' is a transport sector defined by the 2006 IPCC Guidelines for National Greenhouse Gas Inventories:
Combustion related emissions from the operation of pump stations and maintenance of pipelines. Transport via pipelines includes transport of gases  liquids, slurry and other commodities via pipelines. Distribution of natural or manufactured gas, water or steam from the distributor to final users is excluded and should be reported in 1 A 1 c ii or 1 A 4 a.",
        <http://purl.obolibrary.org/obo/IAO_0000119> "2006 IPCC Guidelines for National Greenhouse Gas Inventories, Volume 1, Chapter 8.5, https://www.ipcc-nggip.iges.or.jp/public/2006gl/",
        <http://purl.obolibrary.org/obo/IAO_0000233> "issue: https://github.com/OpenEnergyPlatform/ontology/issues/580
pull request: https://github.com/OpenEnergyPlatform/ontology/pull/595

fix unique individual identfier
issue: https://github.com/OpenEnergyPlatform/ontology/issues/1121
pull request: https://github.com/OpenEnergyPlatform/ontology/pull/1122",
        rdfs:label "CRF sector (IPCC 2006): pipeline transport"
    
    Types: 
        OEO_00000422
    
    Facts:  
     OEO_00000504  OEO_00000242,
     <http://purl.obolibrary.org/obo/BFO_0000050>  OEO_00010063
    
    
Individual: OEO_00010065

    Annotations: 
        <http://purl.obolibrary.org/obo/IAO_0000115> "The KSG sector energy industry is an energy transformation sector defined by the KSG sector division. It is an aggregate of the following three sectors:
- CRF sector (IPCC 2006): energy industry (CRF 1.A.1.a)
- CRF sector (IPCC 2006): other transportation (CRF 1.A.3.e)
- CRF sector (IPCC 2006): fugitive emissions from fuels (CRF 1.B)",
        <http://purl.obolibrary.org/obo/IAO_0000119> "Bundes-Klimaschutzgesetz (KSG), Anlage 1 (zu den §§ 4 und 5) https://www.gesetze-im-internet.de/ksg/anlage_1.html",
        <http://purl.obolibrary.org/obo/IAO_0000233> "issue: https://github.com/OpenEnergyPlatform/ontology/issues/580
pull request: https://github.com/OpenEnergyPlatform/ontology/pull/595",
        rdfs:label "KSG sector energy industry"
    
    Types: 
        OEO_00000158
    
    Facts:  
     OEO_00000504  OEO_00010056,
     <http://purl.obolibrary.org/obo/BFO_0000051>  OEO_00010040,
     <http://purl.obolibrary.org/obo/BFO_0000051>  OEO_00010057,
     <http://purl.obolibrary.org/obo/BFO_0000051>  OEO_00010064
    
    
Individual: OEO_00010066

    Annotations: 
        <http://purl.obolibrary.org/obo/IAO_0000115> "The KSG sector industry is an industry sector defined by the KSG sector division. It is an aggregate of the following three sectors:
- CRF sector (IPCC 2006): manufacturing industries and construction (CRF 1.A.2)
- CRF sector (IPCC 2006): CO2 transport and storage (CRF 1.C)
- CRF sector (IPCC 2006): industrial processes and product use (CRF 2)",
        <http://purl.obolibrary.org/obo/IAO_0000119> "Bundes-Klimaschutzgesetz (KSG), Anlage 1 (zu den §§ 4 und 5) https://www.gesetze-im-internet.de/ksg/anlage_1.html",
        <http://purl.obolibrary.org/obo/IAO_0000233> "issue: https://github.com/OpenEnergyPlatform/ontology/issues/580
pull request: https://github.com/OpenEnergyPlatform/ontology/pull/595",
        rdfs:label "KSG sector industry"
    
    Types: 
        OEO_00000227
    
    Facts:  
     OEO_00000504  OEO_00010056,
     <http://purl.obolibrary.org/obo/BFO_0000051>  OEO_00010041,
     <http://purl.obolibrary.org/obo/BFO_0000051>  OEO_00010046,
     <http://purl.obolibrary.org/obo/BFO_0000051>  OEO_00010058
    
    
Individual: OEO_00010067

    Annotations: 
        <http://purl.obolibrary.org/obo/IAO_0000115> "The KSG sector buildings is a building sector defined by the KSG sector division. It is an aggregate of the following two sectors:
- CRF sector (IPCC 2006): commercial and institutional (CRF 1.A.4.a)
- CRF sector (IPCC 2006): residential (CRF 1.A.4.b)",
        <http://purl.obolibrary.org/obo/IAO_0000119> "Bundes-Klimaschutzgesetz (KSG), Anlage 1 (zu den §§ 4 und 5) https://www.gesetze-im-internet.de/ksg/anlage_1.html",
        <http://purl.obolibrary.org/obo/IAO_0000233> "issue: https://github.com/OpenEnergyPlatform/ontology/issues/580
pull request: https://github.com/OpenEnergyPlatform/ontology/pull/595",
        rdfs:label "KSG sector buildings"
    
    Types: 
        OEO_00010034
    
    Facts:  
     OEO_00000504  OEO_00010056,
     <http://purl.obolibrary.org/obo/BFO_0000051>  OEO_00010052,
     <http://purl.obolibrary.org/obo/BFO_0000051>  OEO_00010053
    
    
Individual: OEO_00010068

    Annotations: 
        <http://purl.obolibrary.org/obo/IAO_0000115> "The KSG sector transport is a transport sector defined by the KSG sector division. It is an aggregate of the following four sectors:
- CRF sector (IPCC 2006): domestic aviation (CRF 1.A.3.a)
- CRF sector (IPCC 2006): road transportation (CRF 1.A.3.b)
- CRF sector (IPCC 2006): railways (CRF 1.A.3.c)
- CRF sector (IPCC 2006): domestic navigation (CRF 1.A.3.d)",
        <http://purl.obolibrary.org/obo/IAO_0000119> "Bundes-Klimaschutzgesetz (KSG), Anlage 1 (zu den §§ 4 und 5) https://www.gesetze-im-internet.de/ksg/anlage_1.html",
        <http://purl.obolibrary.org/obo/IAO_0000233> "issue: https://github.com/OpenEnergyPlatform/ontology/issues/580
pull request: https://github.com/OpenEnergyPlatform/ontology/pull/595",
        rdfs:label "KSG sector transport"
    
    Types: 
        OEO_00000422
    
    Facts:  
     OEO_00000504  OEO_00010056,
     <http://purl.obolibrary.org/obo/BFO_0000051>  OEO_00010059,
     <http://purl.obolibrary.org/obo/BFO_0000051>  OEO_00010060,
     <http://purl.obolibrary.org/obo/BFO_0000051>  OEO_00010061,
     <http://purl.obolibrary.org/obo/BFO_0000051>  OEO_00010062
    
    
Individual: OEO_00010069

    Annotations: 
        <http://purl.obolibrary.org/obo/IAO_0000115> "The KSG sector agriculture is an agriculture, forestry and land use sector defined by the KSG sector division. It is an aggregate of the following two sectors:
- CRF sector (IPCC 2006): agriculture, forestry and fishing (CRF 1.A.4.c)
- CRF sector (IPCC 2006): agriculture (CRF 3)",
        <http://purl.obolibrary.org/obo/IAO_0000119> "Bundes-Klimaschutzgesetz (KSG), Anlage 1 (zu den §§ 4 und 5) https://www.gesetze-im-internet.de/ksg/anlage_1.html",
        <http://purl.obolibrary.org/obo/IAO_0000233> "issue: https://github.com/OpenEnergyPlatform/ontology/issues/580
pull request: https://github.com/OpenEnergyPlatform/ontology/pull/595",
        rdfs:label "KSG sector agriculture"
    
    Types: 
        OEO_00010035
    
    Facts:  
     OEO_00000504  OEO_00010056,
     <http://purl.obolibrary.org/obo/BFO_0000051>  OEO_00010047,
     <http://purl.obolibrary.org/obo/BFO_0000051>  OEO_00010054
    
    
Individual: OEO_00010070

    Annotations: 
        <http://purl.obolibrary.org/obo/IAO_0000115> "The KSG sector waste management and other is a sector defined by the KSG sector division. It is an aggregate of the following two sectors:
- CRF sector (IPCC 2006): waste (CRF 5)
- CRF sector (IPCC 2006): other (CRF 6)",
        <http://purl.obolibrary.org/obo/IAO_0000119> "Bundes-Klimaschutzgesetz (KSG), Anlage 1 (zu den §§ 4 und 5) https://www.gesetze-im-internet.de/ksg/anlage_1.html",
        <http://purl.obolibrary.org/obo/IAO_0000233> "issue: https://github.com/OpenEnergyPlatform/ontology/issues/580
pull request: https://github.com/OpenEnergyPlatform/ontology/pull/595",
        rdfs:label "KSG sector waste management and other"
    
    Types: 
        OEO_00010036
    
    Facts:  
     OEO_00000504  OEO_00010056,
     <http://purl.obolibrary.org/obo/BFO_0000051>  OEO_00010049,
     <http://purl.obolibrary.org/obo/BFO_0000051>  OEO_00010050
    
    
Individual: OEO_00010071

    Annotations: 
        <http://purl.obolibrary.org/obo/IAO_0000115> "The KSG sector land use, land-use change and forestry is an agriculture, forestry and land use sector defined by the KSG sector division.
It is equivalent to the CRF sector (IPCC 2006): land use, land-use change and forestry (CRF 4).",
        <http://purl.obolibrary.org/obo/IAO_0000119> "Bundes-Klimaschutzgesetz (KSG), Anlage 1 (zu den §§ 4 und 5) https://www.gesetze-im-internet.de/ksg/anlage_1.html",
        <http://purl.obolibrary.org/obo/IAO_0000233> "issue: https://github.com/OpenEnergyPlatform/ontology/issues/580
pull request: https://github.com/OpenEnergyPlatform/ontology/pull/595",
        rdfs:label "KSG sector land use, land-use change and forestry"
    
    Types: 
        OEO_00010035
    
    Facts:  
     OEO_00000504  OEO_00010056
    
    SameAs: 
        OEO_00010048
    
    
Individual: OEO_00010122

    Annotations: 
        <http://purl.obolibrary.org/obo/IAO_0000115> "The European Union Emissions Trading System (EU ETS) is a policy instrument that implements an emissions trading system covering the European Union, Norway, Iceland and Liechtenstein.",
        <http://purl.obolibrary.org/obo/IAO_0000118> "EU ETS",
        <http://purl.obolibrary.org/obo/IAO_0000233> "issue: https://github.com/OpenEnergyPlatform/ontology/issues/834
pull request: https://github.com/OpenEnergyPlatform/ontology/pull/857

add axioms:
issue: https://github.com/OpenEnergyPlatform/ontology/issues/928
pull request: https://github.com/OpenEnergyPlatform/ontology/pull/944",
        rdfs:label "European Union Emissions Trading System"@en
    
    Types: 
        OEO_00140151,
        OEO_00000503 some OEO_00020064
    
    Facts:  
     OEO_00010128  OEO_00010131,
     OEO_00010128  OEO_00010132,
     OEO_00010128  OEO_00010133,
     OEO_00010128  OEO_00010205,
     <http://purl.obolibrary.org/obo/BFO_0000050>  OEO_00010129
    
    
Individual: OEO_00010124

    Annotations: 
        <http://purl.obolibrary.org/obo/IAO_0000115> "The Effort Sharing Decision (ESD) is the European effort sharing for the years 2013-2020. It covers the European Union, Norway, Iceland and Liechtenstein and the following greenhouse gases: carbon dioxide, methane, nitrous oxide, hydrofluorocarbons, perfluorocarbons and sulphur hexafluoride. Emission quantities under the ESD are calculated using global warming potentials from the Fourth IPCC Assessment Report.",
        <http://purl.obolibrary.org/obo/IAO_0000118> "ESD",
        <http://purl.obolibrary.org/obo/IAO_0000233> "issue: https://github.com/OpenEnergyPlatform/ontology/issues/834
pull request: https://github.com/OpenEnergyPlatform/ontology/pull/857",
        rdfs:label "Effort Sharing Decision"@en
    
    Types: 
        OEO_00010123,
        OEO_00000503 some OEO_00010126
    
    Facts:  
     <http://purl.obolibrary.org/obo/BFO_0000050>  OEO_00010129
    
    
Individual: OEO_00010125

    Annotations: 
        <http://purl.obolibrary.org/obo/IAO_0000115> "The Effort Sharing Regulation (ESR) is the European effort sharing for the years 2021-2030. It covers the European Union, Norway, Iceland and Liechtenstein and the following greenhouse gases: carbon dioxide, methane, nitrous oxide, hydrofluorocarbons, perfluorocarbons, sulphur hexafluoride and nitrogen trifluoride. Emission quantities under the ESR are calculated using global warming potentials from the Fifth IPCC Assessment Report.",
        <http://purl.obolibrary.org/obo/IAO_0000118> "ESR",
        <http://purl.obolibrary.org/obo/IAO_0000233> "issue: https://github.com/OpenEnergyPlatform/ontology/issues/834
pull request: https://github.com/OpenEnergyPlatform/ontology/pull/857",
        rdfs:label "Effort Sharing Regulation"@en
    
    Types: 
        OEO_00010123,
        OEO_00000503 some OEO_00010126
    
    Facts:  
     <http://purl.obolibrary.org/obo/BFO_0000050>  OEO_00010129
    
    
Individual: OEO_00010129

    Annotations: 
        <http://purl.obolibrary.org/obo/IAO_0000115> "The EU climate policy is the policy of the European Union for reducing greenhouse gas emissions. It uses the EU emission sector division.",
        <http://purl.obolibrary.org/obo/IAO_0000233> "issue: https://github.com/OpenEnergyPlatform/ontology/issues/834
pull request: https://github.com/OpenEnergyPlatform/ontology/pull/857",
        rdfs:label "EU climate policy"@en
    
    Types: 
        OEO_00140150
    
    Facts:  
     OEO_00000503  OEO_00010130
    
    
Individual: OEO_00010130

    Annotations: 
        <http://purl.obolibrary.org/obo/IAO_0000115> "The EU emission sector division is used in the EU climate policy.",
        <http://purl.obolibrary.org/obo/IAO_0000233> "issue: https://github.com/OpenEnergyPlatform/ontology/issues/834
pull request: https://github.com/OpenEnergyPlatform/ontology/pull/857",
        rdfs:label "EU emission sector division"@en
    
    Types: 
        OEO_00000368
    
    Facts:  
     OEO_00000504  OEO_00010129
    
    
Individual: OEO_00010131

    Annotations: 
        <http://purl.obolibrary.org/obo/IAO_0000115> "The EU emission sector ETS is a sector defined by the EU emission sector division that covers greenhouse gas emissions that are regulated by the European Union Emissions Trading System.",
        <http://purl.obolibrary.org/obo/IAO_0000233> "issue: https://github.com/OpenEnergyPlatform/ontology/issues/834
pull request: https://github.com/OpenEnergyPlatform/ontology/pull/857",
        rdfs:label "EU emission sector: ETS"@en
    
    Types: 
        OEO_00000367
    
    Facts:  
     OEO_00000504  OEO_00010130
    
    
Individual: OEO_00010132

    Annotations: 
        <http://purl.obolibrary.org/obo/IAO_0000115> "The EU emission sector ETS stationary is a sector defined by the EU emission sector division that covers greenhouse gas emissions regulated by the European Union Emissions Trading System and that are emitted by stationary installations.",
        <http://purl.obolibrary.org/obo/IAO_0000233> "issue: https://github.com/OpenEnergyPlatform/ontology/issues/834
pull request: https://github.com/OpenEnergyPlatform/ontology/pull/857",
        rdfs:label "EU emission sector: ETS stationary"@en
    
    Types: 
        OEO_00000367
    
    Facts:  
     OEO_00000504  OEO_00010130,
     <http://purl.obolibrary.org/obo/BFO_0000050>  OEO_00010131
    
    
Individual: OEO_00010133

    Annotations: 
        <http://purl.obolibrary.org/obo/IAO_0000115> "The EU emission sector ETS aviation is a transport sector defined by the EU emission sector division that covers greenhouse gas emissions regulated by the European Union Emissions Trading System and that are emitted by stationary installations.",
        <http://purl.obolibrary.org/obo/IAO_0000233> "issue: https://github.com/OpenEnergyPlatform/ontology/issues/834
pull request: https://github.com/OpenEnergyPlatform/ontology/pull/857",
        rdfs:label "EU emission sector: ETS aviation"@en
    
    Types: 
        OEO_00000422
    
    Facts:  
     OEO_00000504  OEO_00010130,
     <http://purl.obolibrary.org/obo/BFO_0000050>  OEO_00010131
    
    
Individual: OEO_00010134

    Annotations: 
        <http://purl.obolibrary.org/obo/IAO_0000115> "The EU emission sector effort sharing is a sector defined by the EU emission sector division that covers greenhouse gas emissions regulated by the Effort Sharing Decision and the Effort Sharing Regulation.",
        <http://purl.obolibrary.org/obo/IAO_0000233> "issue: https://github.com/OpenEnergyPlatform/ontology/issues/834
pull request: https://github.com/OpenEnergyPlatform/ontology/pull/857",
        rdfs:label "EU emission sector: effort sharing"@en
    
    Types: 
        OEO_00000367
    
    Facts:  
     OEO_00000504  OEO_00010130
    
    
Individual: OEO_00010135

    Annotations: 
        <http://purl.obolibrary.org/obo/IAO_0000115> "The EU emission sector ETS stationary is a sector defined by the EU emission sector division that covers greenhouse gas emissions regulated by the European Union Emissions Trading System and that are emitted by stationary installations.",
        <http://purl.obolibrary.org/obo/IAO_0000233> "issue: https://github.com/OpenEnergyPlatform/ontology/issues/834
pull request: https://github.com/OpenEnergyPlatform/ontology/pull/857",
        rdfs:label "EU emission sector: LULUCF"@en
    
    Types: 
        OEO_00010035
    
    Facts:  
     OEO_00000504  OEO_00010130
    
    SameAs: 
        OEO_00010048
    
    
Individual: OEO_00010158

    Annotations: 
        OEO_00010037 "CRF 1.A.1.a",
        <http://purl.obolibrary.org/obo/IAO_0000115> "The CRF sector (IPCC 2006) 'public electricity and heat production' is an energy transformation sector defined by the 2006 IPCC Guidelines for National Greenhouse Gas Inventories:
Sum of emissions from main activity producers of electricity generation, combined heat and power generation, and heat plants.",
        <http://purl.obolibrary.org/obo/IAO_0000119> "2006 IPCC Guidelines for National Greenhouse Gas Inventories, Volume 2, Chapter 2.2, https://www.ipcc-nggip.iges.or.jp/public/2006gl/",
        <http://purl.obolibrary.org/obo/IAO_0000233> "issue: https://github.com/OpenEnergyPlatform/ontology/issues/858
pull request: https://github.com/OpenEnergyPlatform/ontology/pull/941",
        rdfs:label "CRF sector (IPCC 2006): public electricity and heat production"@en
    
    Types: 
        OEO_00000158
    
    Facts:  
     OEO_00000504  OEO_00000242,
     <http://purl.obolibrary.org/obo/BFO_0000050>  OEO_00010040
    
    
Individual: OEO_00010159

    Annotations: 
        OEO_00010037 "CRF 1.A.1.b",
        <http://purl.obolibrary.org/obo/IAO_0000115> "The CRF sector (IPCC 2006) 'petroleum refining' is an energy transformation sector defined by the 2006 IPCC Guidelines for National Greenhouse Gas Inventories:
All combustion activities supporting the refining of petroleum products including on-site combustion for the generation of electricity and heat for own use.",
        <http://purl.obolibrary.org/obo/IAO_0000119> "2006 IPCC Guidelines for National Greenhouse Gas Inventories, Volume 2, Chapter 2.2, https://www.ipcc-nggip.iges.or.jp/public/2006gl/",
        <http://purl.obolibrary.org/obo/IAO_0000233> "issue: https://github.com/OpenEnergyPlatform/ontology/issues/858
pull request: https://github.com/OpenEnergyPlatform/ontology/pull/941",
        rdfs:label "CRF sector (IPCC 2006): petroleum refining"@en
    
    Types: 
        OEO_00000158
    
    Facts:  
     OEO_00000504  OEO_00000242,
     <http://purl.obolibrary.org/obo/BFO_0000050>  OEO_00010040
    
    
Individual: OEO_00010160

    Annotations: 
        OEO_00010037 "CRF 1.A.1.c",
        <http://purl.obolibrary.org/obo/IAO_0000115> "The CRF sector (IPCC 2006) 'manufacture of solid fuels and other energy industries' is an energy transformation sector defined by the 2006 IPCC Guidelines for National Greenhouse Gas Inventories:
Combustion emissions from fuel use during the manufacture of secondary and tertiary products from solid fuels including production of charcoal.",
        <http://purl.obolibrary.org/obo/IAO_0000119> "2006 IPCC Guidelines for National Greenhouse Gas Inventories, Volume 2, Chapter 2.2, https://www.ipcc-nggip.iges.or.jp/public/2006gl/",
        <http://purl.obolibrary.org/obo/IAO_0000233> "issue: https://github.com/OpenEnergyPlatform/ontology/issues/858
pull request: https://github.com/OpenEnergyPlatform/ontology/pull/941",
        rdfs:label "CRF sector (IPCC 2006): manufacture of solid fuels and other energy industries"@en
    
    Types: 
        OEO_00000158
    
    Facts:  
     OEO_00000504  OEO_00000242,
     <http://purl.obolibrary.org/obo/BFO_0000050>  OEO_00010040
    
    
Individual: OEO_00010161

    Annotations: 
        OEO_00010037 "CRF 1.B.1",
        <http://purl.obolibrary.org/obo/IAO_0000115> "The CRF sector (IPCC 2006) 'solid fuels' is a sector defined by the 2006 IPCC Guidelines for National Greenhouse Gas Inventories:
Includes all intentional and unintentional emissions from the extraction, processing, storage and transport of fuel to the point of final use.",
        <http://purl.obolibrary.org/obo/IAO_0000119> "2006 IPCC Guidelines for National Greenhouse Gas Inventories, Volume 1, Chapter 8.5, https://www.ipcc-nggip.iges.or.jp/public/2006gl/",
        <http://purl.obolibrary.org/obo/IAO_0000233> "issue: https://github.com/OpenEnergyPlatform/ontology/issues/858
pull request: https://github.com/OpenEnergyPlatform/ontology/pull/941",
        rdfs:label "CRF sector (IPCC 2006): solid fuels"@en
    
    Types: 
        OEO_00000367
    
    Facts:  
     OEO_00000504  OEO_00000242,
     <http://purl.obolibrary.org/obo/BFO_0000050>  OEO_00010057
    
    
Individual: OEO_00010162

    Annotations: 
        OEO_00010037 "CRF 1.B.2",
        <http://purl.obolibrary.org/obo/IAO_0000115> "The CRF sector (IPCC 2006) 'oil and natural gas' is a sector defined by the 2006 IPCC Guidelines for National Greenhouse Gas Inventories:
Comprises fugitive emissions from all oil and natural gas activities.",
        <http://purl.obolibrary.org/obo/IAO_0000119> "2006 IPCC Guidelines for National Greenhouse Gas Inventories, Volume 1, Chapter 8.5, https://www.ipcc-nggip.iges.or.jp/public/2006gl/",
        <http://purl.obolibrary.org/obo/IAO_0000233> "issue: https://github.com/OpenEnergyPlatform/ontology/issues/858
pull request: https://github.com/OpenEnergyPlatform/ontology/pull/941",
        rdfs:label "CRF sector (IPCC 2006): oil and natural gas"@en
    
    Types: 
        OEO_00000367
    
    Facts:  
     OEO_00000504  OEO_00000242,
     <http://purl.obolibrary.org/obo/BFO_0000050>  OEO_00010057
    
    
Individual: OEO_00010163

    Annotations: 
        <http://purl.obolibrary.org/obo/IAO_0000115> "The GovReg sector division is a sector division defined in Annex XXV, Table 1a of Commission Implementing Regulation (EU) 2020/1208. It uses CRF sectors (IPCC 2006) and adds further sectors.",
        <http://purl.obolibrary.org/obo/IAO_0000116> "Annex XXV, Table 1a of Commission Implementing Regulation (EU) 2020/1208: https://eur-lex.europa.eu/legal-content/EN/TXT/HTML/?uri=CELEX:32020R1208&from=EN#d1e32-98-1",
        <http://purl.obolibrary.org/obo/IAO_0000233> "issue: https://github.com/OpenEnergyPlatform/ontology/issues/858
pull request: https://github.com/OpenEnergyPlatform/ontology/pull/941

relabel:
issue: https://github.com/OpenEnergyPlatform/ontology/issues/928
pull request: https://github.com/OpenEnergyPlatform/ontology/pull/944",
        rdfs:label "GovReg sector division"@en
    
    Types: 
        OEO_00000368
    
    Facts:  
     OEO_00000503  OEO_00000242
    
    
Individual: OEO_00010164

    Annotations: 
        OEO_00010037 "CRF 2.A",
        <http://purl.obolibrary.org/obo/IAO_0000115> "The CRF sector (IPCC 2006) 'mineral industry' is an industry sector defined by the 2006 IPCC Guidelines for National Greenhouse Gas Inventories:
Process-related carbon dioxide (CO2) emissions resulting from the use of carbonate raw materials in the production and use of a variety of mineral industry products.",
        <http://purl.obolibrary.org/obo/IAO_0000119> "2006 IPCC Guidelines for National Greenhouse Gas Inventories, Volume 3, Chapter 2.1, https://www.ipcc-nggip.iges.or.jp/public/2006gl/",
        <http://purl.obolibrary.org/obo/IAO_0000233> "issue: https://github.com/OpenEnergyPlatform/ontology/issues/858
pull request: https://github.com/OpenEnergyPlatform/ontology/pull/941",
        rdfs:label "CRF sector (IPCC 2006): mineral industry"@en
    
    Types: 
        OEO_00000227
    
    Facts:  
     OEO_00000504  OEO_00000242,
     <http://purl.obolibrary.org/obo/BFO_0000050>  OEO_00010046
    
    
Individual: OEO_00010165

    Annotations: 
        OEO_00010037 "CRF 2.A.1",
        <http://purl.obolibrary.org/obo/IAO_0000115> "The CRF sector (IPCC 2006) 'cement production' is an industry sector defined by the 2006 IPCC Guidelines for National Greenhouse Gas Inventories:
Process-related emissions from the production of various types of cement (ISIC: D2694).",
        <http://purl.obolibrary.org/obo/IAO_0000119> "2006 IPCC Guidelines for National Greenhouse Gas Inventories, Volume 1, Chapter 8.5, https://www.ipcc-nggip.iges.or.jp/public/2006gl/",
        <http://purl.obolibrary.org/obo/IAO_0000233> "issue: https://github.com/OpenEnergyPlatform/ontology/issues/858
pull request: https://github.com/OpenEnergyPlatform/ontology/pull/941",
        rdfs:label "CRF sector (IPCC 2006): cement production"@en
    
    Types: 
        OEO_00000227
    
    Facts:  
     OEO_00000504  OEO_00000242,
     <http://purl.obolibrary.org/obo/BFO_0000050>  OEO_00010164
    
    
Individual: OEO_00010166

    Annotations: 
        OEO_00010037 "CRF 2.B",
        <http://purl.obolibrary.org/obo/IAO_0000115> "The CRF sector (IPCC 2006) 'chemical industry' is an industry sector defined by the 2006 IPCC Guidelines for National Greenhouse Gas Inventories:
Greenhouse gas emissions that result from the production of various inorganic and organic chemicals.",
        <http://purl.obolibrary.org/obo/IAO_0000119> "2006 IPCC Guidelines for National Greenhouse Gas Inventories, Volume 3, Chapter 3.1, https://www.ipcc-nggip.iges.or.jp/public/2006gl/",
        <http://purl.obolibrary.org/obo/IAO_0000233> "issue: https://github.com/OpenEnergyPlatform/ontology/issues/858
pull request: https://github.com/OpenEnergyPlatform/ontology/pull/941",
        rdfs:label "CRF sector (IPCC 2006): chemical industry"@en
    
    Types: 
        OEO_00000227
    
    Facts:  
     OEO_00000504  OEO_00000242,
     <http://purl.obolibrary.org/obo/BFO_0000050>  OEO_00010046
    
    
Individual: OEO_00010167

    Annotations: 
        OEO_00010037 "CRF 2.C",
        <http://purl.obolibrary.org/obo/IAO_0000115> "The CRF sector (IPCC 2006) 'metal industry' is an industry sector defined by the 2006 IPCC Guidelines for National Greenhouse Gas Inventories:
Greenhouse gas emissions that result from the production of metals.",
        <http://purl.obolibrary.org/obo/IAO_0000119> "2006 IPCC Guidelines for National Greenhouse Gas Inventories, Volume 3, Chapter 4.1, https://www.ipcc-nggip.iges.or.jp/public/2006gl/",
        <http://purl.obolibrary.org/obo/IAO_0000233> "issue: https://github.com/OpenEnergyPlatform/ontology/issues/858
pull request: https://github.com/OpenEnergyPlatform/ontology/pull/941",
        rdfs:label "CRF sector (IPCC 2006): metal industry"@en
    
    Types: 
        OEO_00000227
    
    Facts:  
     OEO_00000504  OEO_00000242,
     <http://purl.obolibrary.org/obo/BFO_0000050>  OEO_00010046
    
    
Individual: OEO_00010168

    Annotations: 
        OEO_00010037 "CRF 2.C.1",
        <http://purl.obolibrary.org/obo/IAO_0000115> "The CRF sector (IPCC 2006) 'cement production' is an industry sector defined by the 2006 IPCC Guidelines for National Greenhouse Gas Inventories:
Carbon dioxide is the predominant gas emitted from the production of iron and steel. The sources of the carbon dioxide emissions include that from carbon-containing reducing agents such as coke and pulverized coal, and, from minerals such as limestone and dolomite added.",
        <http://purl.obolibrary.org/obo/IAO_0000119> "2006 IPCC Guidelines for National Greenhouse Gas Inventories, Volume 1, Chapter 8.5, https://www.ipcc-nggip.iges.or.jp/public/2006gl/",
        <http://purl.obolibrary.org/obo/IAO_0000233> "issue: https://github.com/OpenEnergyPlatform/ontology/issues/858
pull request: https://github.com/OpenEnergyPlatform/ontology/pull/941",
        rdfs:label "CRF sector (IPCC 2006): iron and steel production"@en
    
    Types: 
        OEO_00000227
    
    Facts:  
     OEO_00000504  OEO_00000242,
     <http://purl.obolibrary.org/obo/BFO_0000050>  OEO_00010167
    
    
Individual: OEO_00010169

    Annotations: 
        OEO_00010037 "CRF 2.D",
        <http://purl.obolibrary.org/obo/IAO_0000115> "The CRF sector (IPCC 2006) 'non-energy products from fuels and solvent use' is an industry sector defined by the 2006 IPCC Guidelines for National Greenhouse Gas Inventories:
The use of oil products and coal-derived oils primarily intended for purposes other than combustion",
        <http://purl.obolibrary.org/obo/IAO_0000119> "2006 IPCC Guidelines for National Greenhouse Gas Inventories, Volume 1, Chapter 8.5, https://www.ipcc-nggip.iges.or.jp/public/2006gl/",
        <http://purl.obolibrary.org/obo/IAO_0000233> "issue: https://github.com/OpenEnergyPlatform/ontology/issues/858
pull request: https://github.com/OpenEnergyPlatform/ontology/pull/941",
        rdfs:label "CRF sector (IPCC 2006): non-energy products from fuels and solvent use"@en
    
    Types: 
        OEO_00000227
    
    Facts:  
     OEO_00000504  OEO_00000242,
     <http://purl.obolibrary.org/obo/BFO_0000050>  OEO_00010046
    
    
Individual: OEO_00010170

    Annotations: 
        OEO_00010037 "CRF 2.E",
        <http://purl.obolibrary.org/obo/IAO_0000115> "The CRF sector (IPCC 2006) 'electronics industry' is an industry sector defined by the 2006 IPCC Guidelines for National Greenhouse Gas Inventories:
Several advanced electronics manufacturing processes utilise fluorinated compounds (FCs) for plasma etching intricate patterns, cleaning reactor chambers, and temperature control. The specific electronic industry sectors include semiconductor, thin-film-transistor flat panel display (TFT-FPD), and photovoltaic (PV) manufacturing (collectively termed ‘electronics industry’).",
        <http://purl.obolibrary.org/obo/IAO_0000119> "2006 IPCC Guidelines for National Greenhouse Gas Inventories, Volume 3, Chapter 6.1, https://www.ipcc-nggip.iges.or.jp/public/2006gl/",
        <http://purl.obolibrary.org/obo/IAO_0000233> "issue: https://github.com/OpenEnergyPlatform/ontology/issues/858
pull request: https://github.com/OpenEnergyPlatform/ontology/pull/941",
        rdfs:label "CRF sector (IPCC 2006): electronics industry"@en
    
    Types: 
        OEO_00000227
    
    Facts:  
     OEO_00000504  OEO_00000242,
     <http://purl.obolibrary.org/obo/BFO_0000050>  OEO_00010046
    
    
Individual: OEO_00010171

    Annotations: 
        OEO_00010037 "CRF 2.F",
        <http://purl.obolibrary.org/obo/IAO_0000115> "The CRF sector (IPCC 2006) 'product uses as substitutes for ozone depleting substances' is an industry sector defined by the 2006 IPCC Guidelines for National Greenhouse Gas Inventories:
Hydrofluorocarbons (HFCs) and, to a very limited extent, perfluorocarbons (PFCs), are serving as alternatives to ozone depleting substances (ODS) being phased out under the Montreal Protocol.",
        <http://purl.obolibrary.org/obo/IAO_0000119> "2006 IPCC Guidelines for National Greenhouse Gas Inventories, Volume 3, Chapter 7.1, https://www.ipcc-nggip.iges.or.jp/public/2006gl/",
        <http://purl.obolibrary.org/obo/IAO_0000233> "issue: https://github.com/OpenEnergyPlatform/ontology/issues/858
pull request: https://github.com/OpenEnergyPlatform/ontology/pull/941",
        rdfs:label "CRF sector (IPCC 2006): product uses as substitutes for ozone depleting substances"@en
    
    Types: 
        OEO_00000227
    
    Facts:  
     OEO_00000504  OEO_00000242,
     <http://purl.obolibrary.org/obo/BFO_0000050>  OEO_00010046
    
    
Individual: OEO_00010172

    Annotations: 
        OEO_00010037 "CRF 2.G",
        <http://purl.obolibrary.org/obo/IAO_0000115> "The CRF sector (IPCC 2006) 'other product manufacture and use' is an industry sector defined by the 2006 IPCC Guidelines for National Greenhouse Gas Inventories:
Emissions of sulphur hexafluoride (SF6) and perfluorocarbons
(PFCs) from the manufacture and use of electrical equipment and a number of other products. It also includes emissions of nitrous oxide (N2O) from several products.",
        <http://purl.obolibrary.org/obo/IAO_0000119> "2006 IPCC Guidelines for National Greenhouse Gas Inventories, Volume 3, Chapter 8.1, https://www.ipcc-nggip.iges.or.jp/public/2006gl/",
        rdfs:label "CRF sector (IPCC 2006): other product manufacture and use"@en
    
    Types: 
        OEO_00000227
    
    Facts:  
     OEO_00000504  OEO_00000242,
     <http://purl.obolibrary.org/obo/BFO_0000050>  OEO_00010046
    
    
Individual: OEO_00010173

    Annotations: 
        OEO_00010037 "CRF 2.H",
        <http://purl.obolibrary.org/obo/IAO_0000115> "The CRF sector (IPCC 2006) 'industrial processes and product use - other' is an industry sector defined by the 2006 IPCC Guidelines for National Greenhouse Gas Inventories",
        <http://purl.obolibrary.org/obo/IAO_0000233> "issue: https://github.com/OpenEnergyPlatform/ontology/issues/858
pull request: https://github.com/OpenEnergyPlatform/ontology/pull/941",
        rdfs:label "CRF sector (IPCC 2006): industrial processes and product use - other"@en
    
    Types: 
        OEO_00000227
    
    Facts:  
     OEO_00000504  OEO_00000242,
     <http://purl.obolibrary.org/obo/BFO_0000050>  OEO_00010046
    
    
Individual: OEO_00010174

    Annotations: 
        OEO_00010037 "CRF 5.A",
        <http://purl.obolibrary.org/obo/IAO_0000115> "The CRF sector (IPCC 2006) 'solid waste disposal' is a waste and wastewater sector defined by the 2006 IPCC Guidelines for National Greenhouse Gas Inventories:
Methane is produced from anaerobic microbial decomposition of organic matter in solid waste disposal sites.",
        <http://purl.obolibrary.org/obo/IAO_0000119> "2006 IPCC Guidelines for National Greenhouse Gas Inventories, Volume 1, Chapter 8.5, https://www.ipcc-nggip.iges.or.jp/public/2006gl/",
        <http://purl.obolibrary.org/obo/IAO_0000233> "issue: https://github.com/OpenEnergyPlatform/ontology/issues/858
pull request: https://github.com/OpenEnergyPlatform/ontology/pull/941",
        rdfs:label "CRF sector (IPCC 2006): solid waste disposal"@en
    
    Types: 
        OEO_00010036
    
    Facts:  
     OEO_00000504  OEO_00000242,
     <http://purl.obolibrary.org/obo/BFO_0000050>  OEO_00010049
    
    
Individual: OEO_00010175

    Annotations: 
        OEO_00010037 "CRF 5.B",
        <http://purl.obolibrary.org/obo/IAO_0000115> "The CRF sector (IPCC 2006) 'biological treatment of solid waste' is a waste and wastewater sector defined by the 2006 IPCC Guidelines for National Greenhouse Gas Inventories:
Solid waste composting and other biological treatment. Emissions from biogas facilities (anaerobic digestion) with energy production are reported in the Energy Sector (1A4).",
        <http://purl.obolibrary.org/obo/IAO_0000119> "2006 IPCC Guidelines for National Greenhouse Gas Inventories, Volume 1, Chapter 8.5, https://www.ipcc-nggip.iges.or.jp/public/2006gl/",
        <http://purl.obolibrary.org/obo/IAO_0000233> "issue: https://github.com/OpenEnergyPlatform/ontology/issues/858
pull request: https://github.com/OpenEnergyPlatform/ontology/pull/941",
        rdfs:label "CRF sector (IPCC 2006): biological treatment of solid waste"@en
    
    Types: 
        OEO_00010036
    
    Facts:  
     OEO_00000504  OEO_00000242,
     <http://purl.obolibrary.org/obo/BFO_0000050>  OEO_00010049
    
    
Individual: OEO_00010176

    Annotations: 
        OEO_00010037 "CRF 5.C",
        <http://purl.obolibrary.org/obo/IAO_0000115> "The CRF sector (IPCC 2006) 'incineration and open burning of waste' is a waste and wastewater sector defined by the 2006 IPCC Guidelines for National Greenhouse Gas Inventories:
Incineration of waste and open burning waste, not including waste-to-energy facilities.",
        <http://purl.obolibrary.org/obo/IAO_0000119> "2006 IPCC Guidelines for National Greenhouse Gas Inventories, Volume 1, Chapter 8.5, https://www.ipcc-nggip.iges.or.jp/public/2006gl/",
        <http://purl.obolibrary.org/obo/IAO_0000233> "issue: https://github.com/OpenEnergyPlatform/ontology/issues/858
pull request: https://github.com/OpenEnergyPlatform/ontology/pull/941",
        rdfs:label "CRF sector (IPCC 2006): incineration and open burning of waste"@en
    
    Types: 
        OEO_00010036
    
    Facts:  
     OEO_00000504  OEO_00000242,
     <http://purl.obolibrary.org/obo/BFO_0000050>  OEO_00010049
    
    
Individual: OEO_00010177

    Annotations: 
        OEO_00010037 "CRF 5.D",
        <http://purl.obolibrary.org/obo/IAO_0000115> "The CRF sector (IPCC 2006) 'waste water treatment and discharge' is a waste and wastewater sector defined by the 2006 IPCC Guidelines for National Greenhouse Gas Inventories:
Methane is produced from anaerobic decomposition of organic matter by bacteria in sewage facilities and from food processing and other industrial facilities during wastewater treatment. N2O is also produced by bacteria
(denitrification and nitrification) in wastewater treatment and discharge.",
        <http://purl.obolibrary.org/obo/IAO_0000119> "2006 IPCC Guidelines for National Greenhouse Gas Inventories, Volume 1, Chapter 8.5, https://www.ipcc-nggip.iges.or.jp/public/2006gl/",
        <http://purl.obolibrary.org/obo/IAO_0000233> "issue: https://github.com/OpenEnergyPlatform/ontology/issues/858
pull request: https://github.com/OpenEnergyPlatform/ontology/pull/941",
        rdfs:label "CRF sector (IPCC 2006): waste water treatment and discharge"@en
    
    Types: 
        OEO_00010036
    
    Facts:  
     OEO_00000504  OEO_00000242,
     <http://purl.obolibrary.org/obo/BFO_0000050>  OEO_00010049
    
    
Individual: OEO_00010178

    Annotations: 
        OEO_00010037 "CRF 5.E",
        <http://purl.obolibrary.org/obo/IAO_0000115> "The CRF sector (IPCC 2006) 'waste - other' is a waste and wastewater sector defined by the 2006 IPCC Guidelines for National Greenhouse Gas Inventories",
        <http://purl.obolibrary.org/obo/IAO_0000119> "2006 IPCC Guidelines for National Greenhouse Gas Inventories, Volume 1, Chapter 8.5, https://www.ipcc-nggip.iges.or.jp/public/2006gl/",
        <http://purl.obolibrary.org/obo/IAO_0000233> "issue: https://github.com/OpenEnergyPlatform/ontology/issues/858
pull request: https://github.com/OpenEnergyPlatform/ontology/pull/941",
        rdfs:label "CRF sector (IPCC 2006): waste - other"@en
    
    Types: 
        OEO_00010036
    
    Facts:  
     OEO_00000504  OEO_00000242,
     <http://purl.obolibrary.org/obo/BFO_0000050>  OEO_00010049
    
    
Individual: OEO_00010179

    Annotations: 
        OEO_00010037 "CRF 3.A",
        <http://purl.obolibrary.org/obo/IAO_0000115> "The CRF sector (IPCC 2006) 'enteric fermentation' is an agriculture, forestry and land use sector defined by the 2006 IPCC Guidelines for National Greenhouse Gas Inventories:
Methane emissions from herbivores as a by-product of enteric fermentation (a digestive process by which carbohydrates are broken down by micro-organisms into simple molecules for absorption into the bloodstream). Ruminant animals (e.g., cattle, sheep) are major sources with moderate amounts produced from non-ruminant animals (e.g., pigs, horses).",
        <http://purl.obolibrary.org/obo/IAO_0000119> "2006 IPCC Guidelines for National Greenhouse Gas Inventories, Volume 1, Chapter 8.5, https://www.ipcc-nggip.iges.or.jp/public/2006gl/",
        <http://purl.obolibrary.org/obo/IAO_0000233> "issue: https://github.com/OpenEnergyPlatform/ontology/issues/858
pull request: https://github.com/OpenEnergyPlatform/ontology/pull/941",
        rdfs:label "CRF sector (IPCC 2006): enteric fermentation"@en
    
    Types: 
        OEO_00010035
    
    Facts:  
     OEO_00000504  OEO_00000242,
     <http://purl.obolibrary.org/obo/BFO_0000050>  OEO_00010047
    
    
Individual: OEO_00010180

    Annotations: 
        OEO_00010037 "CRF 3.B",
        <http://purl.obolibrary.org/obo/IAO_0000115> "The CRF sector (IPCC 2006) 'manure management' is an agriculture, forestry and land use sector defined by the 2006 IPCC Guidelines for National Greenhouse Gas Inventories:
Methane and nitrous oxide emissions from the decomposition of manure under low oxygen or anaerobic conditions.",
        <http://purl.obolibrary.org/obo/IAO_0000119> "2006 IPCC Guidelines for National Greenhouse Gas Inventories, Volume 1, Chapter 8.5, https://www.ipcc-nggip.iges.or.jp/public/2006gl/",
        <http://purl.obolibrary.org/obo/IAO_0000233> "issue: https://github.com/OpenEnergyPlatform/ontology/issues/858
pull request: https://github.com/OpenEnergyPlatform/ontology/pull/941",
        rdfs:label "CRF sector (IPCC 2006): manure management"@en
    
    Types: 
        OEO_00010035
    
    Facts:  
     OEO_00000504  OEO_00000242,
     <http://purl.obolibrary.org/obo/BFO_0000050>  OEO_00010047
    
    
Individual: OEO_00010181

    Annotations: 
        OEO_00010037 "CRF 3.C",
        <http://purl.obolibrary.org/obo/IAO_0000115> "The CRF sector (IPCC 2006) 'rice cultivation' is an agriculture, forestry and land use sector defined by the 2006 IPCC Guidelines for National Greenhouse Gas Inventories:
Methane (CH4) emissions from anaerobic decomposition of organic material in flooded rice fields.",
        <http://purl.obolibrary.org/obo/IAO_0000119> "2006 IPCC Guidelines for National Greenhouse Gas Inventories, Volume 1, Chapter 8.5, https://www.ipcc-nggip.iges.or.jp/public/2006gl/",
        <http://purl.obolibrary.org/obo/IAO_0000233> "issue: https://github.com/OpenEnergyPlatform/ontology/issues/858
pull request: https://github.com/OpenEnergyPlatform/ontology/pull/941",
        rdfs:label "CRF sector (IPCC 2006): rice cultivation"@en
    
    Types: 
        OEO_00010035
    
    Facts:  
     OEO_00000504  OEO_00000242,
     <http://purl.obolibrary.org/obo/BFO_0000050>  OEO_00010047
    
    
Individual: OEO_00010182

    Annotations: 
        OEO_00010037 "CRF 3.D",
        <http://purl.obolibrary.org/obo/IAO_0000115> "The CRF sector (IPCC 2006) 'agricultural soils' is an agriculture, forestry and land use sector defined by the 2006 IPCC Guidelines for National Greenhouse Gas Inventories",
        <http://purl.obolibrary.org/obo/IAO_0000233> "issue: https://github.com/OpenEnergyPlatform/ontology/issues/858
pull request: https://github.com/OpenEnergyPlatform/ontology/pull/941",
        rdfs:label "CRF sector (IPCC 2006): agricultural soils"@en
    
    Types: 
        OEO_00010035
    
    Facts:  
     OEO_00000504  OEO_00000242,
     <http://purl.obolibrary.org/obo/BFO_0000050>  OEO_00010047
    
    
Individual: OEO_00010183

    Annotations: 
        OEO_00010037 "CRF 3.E",
        <http://purl.obolibrary.org/obo/IAO_0000115> "The CRF sector (IPCC 2006) 'prescribed burning of savannas' is an agriculture, forestry and land use sector defined by the 2006 IPCC Guidelines for National Greenhouse Gas Inventories",
        <http://purl.obolibrary.org/obo/IAO_0000233> "issue: https://github.com/OpenEnergyPlatform/ontology/issues/858
pull request: https://github.com/OpenEnergyPlatform/ontology/pull/941",
        rdfs:label "CRF sector (IPCC 2006): prescribed burning of savannas"@en
    
    Types: 
        OEO_00010035
    
    Facts:  
     OEO_00000504  OEO_00000242,
     <http://purl.obolibrary.org/obo/BFO_0000050>  OEO_00010047
    
    
Individual: OEO_00010184

    Annotations: 
        OEO_00010037 "CRF 3.F",
        <http://purl.obolibrary.org/obo/IAO_0000115> "The CRF sector (IPCC 2006) 'field burning of agricultural residues' is an agriculture, forestry and land use sector defined by the 2006 IPCC Guidelines for National Greenhouse Gas Inventories:
CO2 emissions from urea application",
        <http://purl.obolibrary.org/obo/IAO_0000119> "2006 IPCC Guidelines for National Greenhouse Gas Inventories, Volume 1, Chapter 8.5, https://www.ipcc-nggip.iges.or.jp/public/2006gl/",
        <http://purl.obolibrary.org/obo/IAO_0000233> "issue: https://github.com/OpenEnergyPlatform/ontology/issues/858
pull request: https://github.com/OpenEnergyPlatform/ontology/pull/941",
        rdfs:label "CRF sector (IPCC 2006): field burning of agricultural residues"@en
    
    Types: 
        OEO_00010035
    
    Facts:  
     OEO_00000504  OEO_00000242,
     <http://purl.obolibrary.org/obo/BFO_0000050>  OEO_00010047
    
    
Individual: OEO_00010185

    Annotations: 
        OEO_00010037 "CRF 3.G",
        <http://purl.obolibrary.org/obo/IAO_0000115> "The CRF sector (IPCC 2006) 'liming' is an agriculture, forestry and land use sector defined by the 2006 IPCC Guidelines for National Greenhouse Gas Inventories:
CO2 emissions from the use of lime in agricultural soils, managed forest soils or lakes.",
        <http://purl.obolibrary.org/obo/IAO_0000119> "2006 IPCC Guidelines for National Greenhouse Gas Inventories, Volume 1, Chapter 8.5, https://www.ipcc-nggip.iges.or.jp/public/2006gl/",
        <http://purl.obolibrary.org/obo/IAO_0000233> "issue: https://github.com/OpenEnergyPlatform/ontology/issues/858
pull request: https://github.com/OpenEnergyPlatform/ontology/pull/941",
        rdfs:label "CRF sector (IPCC 2006): liming"@en
    
    Types: 
        OEO_00010035
    
    Facts:  
     OEO_00000504  OEO_00000242,
     <http://purl.obolibrary.org/obo/BFO_0000050>  OEO_00010047
    
    
Individual: OEO_00010186

    Annotations: 
        OEO_00010037 "CRF 3.H",
        <http://purl.obolibrary.org/obo/IAO_0000115> "The CRF sector (IPCC 2006) 'urea application' is an agriculture, forestry and land use sector defined by the 2006 IPCC Guidelines for National Greenhouse Gas Inventories",
        <http://purl.obolibrary.org/obo/IAO_0000233> "issue: https://github.com/OpenEnergyPlatform/ontology/issues/858
pull request: https://github.com/OpenEnergyPlatform/ontology/pull/941",
        rdfs:label "CRF sector (IPCC 2006): urea application"@en
    
    Types: 
        OEO_00010035
    
    Facts:  
     OEO_00000504  OEO_00000242,
     <http://purl.obolibrary.org/obo/BFO_0000050>  OEO_00010047
    
    
Individual: OEO_00010187

    Annotations: 
        OEO_00010037 "CRF 3.I",
        <http://purl.obolibrary.org/obo/IAO_0000115> "The CRF sector (IPCC 2006) 'other carbon-containing fertilizers' is an agriculture, forestry and land use sector defined by the 2006 IPCC Guidelines for National Greenhouse Gas Inventories",
        <http://purl.obolibrary.org/obo/IAO_0000233> "issue: https://github.com/OpenEnergyPlatform/ontology/issues/858
pull request: https://github.com/OpenEnergyPlatform/ontology/pull/941",
        rdfs:label "CRF sector (IPCC 2006): other carbon-containing fertilizers"@en
    
    Types: 
        OEO_00010035
    
    Facts:  
     OEO_00000504  OEO_00000242,
     <http://purl.obolibrary.org/obo/BFO_0000050>  OEO_00010047
    
    
Individual: OEO_00010188

    Annotations: 
        OEO_00010037 "CRF 3.J",
        <http://purl.obolibrary.org/obo/IAO_0000115> "The CRF sector (IPCC 2006) 'agriculture - other' is an agriculture, forestry and land use sector defined by the 2006 IPCC Guidelines for National Greenhouse Gas Inventories",
        <http://purl.obolibrary.org/obo/IAO_0000233> "issue: https://github.com/OpenEnergyPlatform/ontology/issues/858
pull request: https://github.com/OpenEnergyPlatform/ontology/pull/941",
        rdfs:label "CRF sector (IPCC 2006): agriculture - other"@en
    
    Types: 
        OEO_00010035
    
    Facts:  
     OEO_00000504  OEO_00000242,
     <http://purl.obolibrary.org/obo/BFO_0000050>  OEO_00010047
    
    
Individual: OEO_00010189

    Annotations: 
        OEO_00010037 "CRF 4.A",
        <http://purl.obolibrary.org/obo/IAO_0000115> "The CRF sector (IPCC 2006) 'forest land' is an agriculture, forestry and land use sector defined by the 2006 IPCC Guidelines for National Greenhouse Gas Inventories:
Emissions and removals from lands with woody vegetation consistent with thresholds used to define forest land in the national GHG inventory, sub-divided into managed and unmanaged, and possibly also by climatic region, soil type and vegetation type as appropriate. It also includes systems with vegetation that currently fall below, but are expected to later exceed, the threshold values used by a country to define the forest land category.",
        <http://purl.obolibrary.org/obo/IAO_0000119> "2006 IPCC Guidelines for National Greenhouse Gas Inventories, Volume 1, Chapter 8.5, https://www.ipcc-nggip.iges.or.jp/public/2006gl/",
        <http://purl.obolibrary.org/obo/IAO_0000233> "issue: https://github.com/OpenEnergyPlatform/ontology/issues/858
pull request: https://github.com/OpenEnergyPlatform/ontology/pull/941",
        rdfs:label "CRF sector (IPCC 2006): forest land"@en
    
    Types: 
        OEO_00010035
    
    Facts:  
     OEO_00000504  OEO_00000242,
     <http://purl.obolibrary.org/obo/BFO_0000050>  OEO_00010048
    
    
Individual: OEO_00010190

    Annotations: 
        OEO_00010037 "CRF 4.B",
        <http://purl.obolibrary.org/obo/IAO_0000115> "The CRF sector (IPCC 2006) 'cropland' is an agriculture, forestry and land use sector defined by the 2006 IPCC Guidelines for National Greenhouse Gas Inventories:
Emissions and removals from arable and tillage land, rice fields, and agro-forestry systems where vegetation falls below the thresholds used for the forest land category.",
        <http://purl.obolibrary.org/obo/IAO_0000119> "2006 IPCC Guidelines for National Greenhouse Gas Inventories, Volume 1, Chapter 8.5, https://www.ipcc-nggip.iges.or.jp/public/2006gl/",
        <http://purl.obolibrary.org/obo/IAO_0000233> "issue: https://github.com/OpenEnergyPlatform/ontology/issues/858
pull request: https://github.com/OpenEnergyPlatform/ontology/pull/941",
        rdfs:label "CRF sector (IPCC 2006): cropland"@en
    
    Types: 
        OEO_00010035
    
    Facts:  
     OEO_00000504  OEO_00000242,
     <http://purl.obolibrary.org/obo/BFO_0000050>  OEO_00010048
    
    
Individual: OEO_00010191

    Annotations: 
        OEO_00010037 "CRF 4.C",
        <http://purl.obolibrary.org/obo/IAO_0000115> "The CRF sector (IPCC 2006) 'grassland' is an agriculture, forestry and land use sector defined by the 2006 IPCC Guidelines for National Greenhouse Gas Inventories:
Emissions and removals from rangelands and pasture land that is not considered cropland. It also includes systems with woody vegetation that fall below the threshold values used in the forest land category and are not expected to exceed them, without human intervention. The category also includes all grassland from wild lands to recreational areas as well as agricultural and silvi-pastural systems, subdivided into managed and unmanaged, consistent with national definitions.",
        <http://purl.obolibrary.org/obo/IAO_0000119> "2006 IPCC Guidelines for National Greenhouse Gas Inventories, Volume 1, Chapter 8.5, https://www.ipcc-nggip.iges.or.jp/public/2006gl/",
        <http://purl.obolibrary.org/obo/IAO_0000233> "issue: https://github.com/OpenEnergyPlatform/ontology/issues/858
pull request: https://github.com/OpenEnergyPlatform/ontology/pull/941",
        rdfs:label "CRF sector (IPCC 2006): grassland"@en
    
    Types: 
        OEO_00010035
    
    Facts:  
     OEO_00000504  OEO_00000242,
     <http://purl.obolibrary.org/obo/BFO_0000050>  OEO_00010048
    
    
Individual: OEO_00010192

    Annotations: 
        OEO_00010037 "CRF 4.D",
        <http://purl.obolibrary.org/obo/IAO_0000115> "The CRF sector (IPCC 2006) 'wetlands' is an agriculture, forestry and land use sector defined by the 2006 IPCC Guidelines for National Greenhouse Gas Inventories:
Emissions from land that is covered or saturated by water for all or part of the year (e.g., peatland) and that does not fall into the forest land, cropland, grassland or settlements categories. The category can be subdivided into managed and unmanaged according to national definitions. It includes reservoirs as a managed sub-division and natural rivers and lakes as unmanaged sub-divisions.",
        <http://purl.obolibrary.org/obo/IAO_0000119> "2006 IPCC Guidelines for National Greenhouse Gas Inventories, Volume 1, Chapter 8.5, https://www.ipcc-nggip.iges.or.jp/public/2006gl/",
        <http://purl.obolibrary.org/obo/IAO_0000233> "issue: https://github.com/OpenEnergyPlatform/ontology/issues/858
pull request: https://github.com/OpenEnergyPlatform/ontology/pull/941",
        rdfs:label "CRF sector (IPCC 2006): wetlands"@en
    
    Types: 
        OEO_00010035
    
    Facts:  
     OEO_00000504  OEO_00000242,
     <http://purl.obolibrary.org/obo/BFO_0000050>  OEO_00010048
    
    
Individual: OEO_00010193

    Annotations: 
        OEO_00010037 "CRF 4.E",
        <http://purl.obolibrary.org/obo/IAO_0000115> "The CRF sector (IPCC 2006) 'settlements' is an agriculture, forestry and land use sector defined by the 2006 IPCC Guidelines for National Greenhouse Gas Inventories:
Emissions and removals from all developed land, including transportation infrastructure and human settlements of any size, unless they are already included under other categories.",
        <http://purl.obolibrary.org/obo/IAO_0000119> "2006 IPCC Guidelines for National Greenhouse Gas Inventories, Volume 1, Chapter 8.5, https://www.ipcc-nggip.iges.or.jp/public/2006gl/",
        <http://purl.obolibrary.org/obo/IAO_0000233> "issue: https://github.com/OpenEnergyPlatform/ontology/issues/858
pull request: https://github.com/OpenEnergyPlatform/ontology/pull/941",
        rdfs:label "CRF sector (IPCC 2006): settlements"@en
    
    Types: 
        OEO_00010035
    
    Facts:  
     OEO_00000504  OEO_00000242,
     <http://purl.obolibrary.org/obo/BFO_0000050>  OEO_00010048
    
    
Individual: OEO_00010194

    Annotations: 
        OEO_00010037 "CRF 4.F",
        <http://purl.obolibrary.org/obo/IAO_0000115> "The CRF sector (IPCC 2006) 'other land' is an agriculture, forestry and land use sector defined by the 2006 IPCC Guidelines for National Greenhouse Gas Inventories:
Emissions and removals from bare soil, rock, ice, and all unmanaged land areas that do not fall into any of the other five categories.",
        <http://purl.obolibrary.org/obo/IAO_0000119> "2006 IPCC Guidelines for National Greenhouse Gas Inventories, Volume 1, Chapter 8.5, https://www.ipcc-nggip.iges.or.jp/public/2006gl/",
        <http://purl.obolibrary.org/obo/IAO_0000233> "issue: https://github.com/OpenEnergyPlatform/ontology/issues/858
pull request: https://github.com/OpenEnergyPlatform/ontology/pull/941",
        rdfs:label "CRF sector (IPCC 2006): other land"@en
    
    Types: 
        OEO_00010035
    
    Facts:  
     OEO_00000504  OEO_00000242,
     <http://purl.obolibrary.org/obo/BFO_0000050>  OEO_00010048
    
    
Individual: OEO_00010195

    Annotations: 
        OEO_00010037 "CRF 4.G",
        <http://purl.obolibrary.org/obo/IAO_0000115> "The CRF sector (IPCC 2006) 'harvested wood products' is an agriculture, forestry and land use sector defined by the 2006 IPCC Guidelines for National Greenhouse Gas Inventories
CO2 net emissions or removals resulting from Harvest Wood Products.",
        <http://purl.obolibrary.org/obo/IAO_0000119> "2006 IPCC Guidelines for National Greenhouse Gas Inventories, Volume 1, Chapter 8.5, https://www.ipcc-nggip.iges.or.jp/public/2006gl/",
        <http://purl.obolibrary.org/obo/IAO_0000233> "issue: https://github.com/OpenEnergyPlatform/ontology/issues/858
pull request: https://github.com/OpenEnergyPlatform/ontology/pull/941",
        rdfs:label "CRF sector (IPCC 2006): harvested wood products"@en
    
    Types: 
        OEO_00010035
    
    Facts:  
     OEO_00000504  OEO_00000242,
     <http://purl.obolibrary.org/obo/BFO_0000050>  OEO_00010048
    
    
Individual: OEO_00010196

    Annotations: 
        OEO_00010037 "CRF 4.H",
        <http://purl.obolibrary.org/obo/IAO_0000115> "The CRF sector (IPCC 2006) 'land use, land-use change and forestry - other' is an agriculture, forestry and land use sector defined by the 2006 IPCC Guidelines for National Greenhouse Gas Inventories",
        <http://purl.obolibrary.org/obo/IAO_0000233> "issue: https://github.com/OpenEnergyPlatform/ontology/issues/858
pull request: https://github.com/OpenEnergyPlatform/ontology/pull/941",
        rdfs:label "CRF sector (IPCC 2006): land use, land-use change and forestry - other"@en
    
    Types: 
        OEO_00010035
    
    Facts:  
     OEO_00000504  OEO_00000242,
     <http://purl.obolibrary.org/obo/BFO_0000050>  OEO_00010048
    
    
Individual: OEO_00010197

    Annotations: 
        <http://purl.obolibrary.org/obo/IAO_0000115> "The CRF sector (IPCC 2006) 'total emissions excluding LULUCF' is a sector defined by the 2006 IPCC Guidelines for National Greenhouse Gas Inventories. It encompasses the following IPCC 2006 sectors: energy; industrial processes and product use; agriculture; waste; and other.",
        
            Annotations: <http://purl.obolibrary.org/obo/IAO_0000116> "Term used by the European Environment Agency (EEA) https://climate-energy.eea.europa.eu/topics/climate-change-mitigation/greenhouse-gas-emissions-inventory/data"
        <http://purl.obolibrary.org/obo/IAO_0000118> "Total emissions: (UNFCCC)",
        <http://purl.obolibrary.org/obo/IAO_0000233> "issue: https://github.com/OpenEnergyPlatform/ontology/issues/928
pull request: https://github.com/OpenEnergyPlatform/ontology/pull/944",
        rdfs:label "CRF sector (IPCC 2006): total emissions excluding LULUCF"@en
    
    Types: 
        OEO_00000367
    
    Facts:  
     OEO_00000504  OEO_00000242,
     <http://purl.obolibrary.org/obo/BFO_0000051>  OEO_00010038,
     <http://purl.obolibrary.org/obo/BFO_0000051>  OEO_00010046,
     <http://purl.obolibrary.org/obo/BFO_0000051>  OEO_00010047,
     <http://purl.obolibrary.org/obo/BFO_0000051>  OEO_00010049,
     <http://purl.obolibrary.org/obo/BFO_0000051>  OEO_00010050
    
    
Individual: OEO_00010198

    Annotations: 
        <http://purl.obolibrary.org/obo/IAO_0000115> "The CRF sector (IPCC 2006) 'total emissions including LULUCF' is a sector defined by the 2006 IPCC Guidelines for National Greenhouse Gas Inventories. It encompasses the following IPCC 2006 sectors: energy; industrial processes and product use; agriculture; land use, land-use change and forestry; waste; and other.",
        
            Annotations: <http://purl.obolibrary.org/obo/IAO_0000116> "Term used by the European Environment Agency (EEA): https://climate-energy.eea.europa.eu/topics/climate-change-mitigation/greenhouse-gas-emissions-inventory/data"
        <http://purl.obolibrary.org/obo/IAO_0000118> "Total net emissions (UNFCCC)",
        <http://purl.obolibrary.org/obo/IAO_0000233> "issue: https://github.com/OpenEnergyPlatform/ontology/issues/928
pull request: https://github.com/OpenEnergyPlatform/ontology/pull/944",
        rdfs:label "CRF sector (IPCC 2006): total emissions including LULUCF"@en
    
    Types: 
        OEO_00000367
    
    Facts:  
     OEO_00000504  OEO_00000242,
     <http://purl.obolibrary.org/obo/BFO_0000051>  OEO_00010038,
     <http://purl.obolibrary.org/obo/BFO_0000051>  OEO_00010046,
     <http://purl.obolibrary.org/obo/BFO_0000051>  OEO_00010047,
     <http://purl.obolibrary.org/obo/BFO_0000051>  OEO_00010048,
     <http://purl.obolibrary.org/obo/BFO_0000051>  OEO_00010049,
     <http://purl.obolibrary.org/obo/BFO_0000051>  OEO_00010050
    
    
Individual: OEO_00010199

    Annotations: 
        OEO_00010037 "CRF 1.D",
        <http://purl.obolibrary.org/obo/IAO_0000115> "The CRF sector (IPCC 2006) international bunkers is a transport sector defined by the 2006 IPCC Guidelines for National Greenhouse Gas Inventories. It encompasses international bunkers and multilateral operation.",
        <http://purl.obolibrary.org/obo/IAO_0000233> "issue: https://github.com/OpenEnergyPlatform/ontology/issues/928
pull request: https://github.com/OpenEnergyPlatform/ontology/pull/944",
        rdfs:label "CRF sector (IPCC 2006): international bunkers and multilateral operations"@en
    
    Types: 
        OEO_00000422,
        
            Annotations: <http://purl.obolibrary.org/obo/IAO_0000233> "issue: https://github.com/OpenEnergyPlatform/ontology/issues/858
pull request: https://github.com/OpenEnergyPlatform/ontology/pull/965"
        OEO_00010232 some OEO_00010227
    
    Facts:  
     OEO_00000504  OEO_00000242,
     <http://purl.obolibrary.org/obo/BFO_0000051>  OEO_00010200,
     <http://purl.obolibrary.org/obo/BFO_0000051>  OEO_00010203
    
    
Individual: OEO_00010200

    Annotations: 
        OEO_00010037 "CRF 1.D.1",
        <http://purl.obolibrary.org/obo/IAO_0000115> "The CRF sector (IPCC 2006) 'international bunkers' is a transport sector defined by the 2006 IPCC Guidelines for National Greenhouse Gas Inventories. It encompasses international aviation and maritime navigation.",
        <http://purl.obolibrary.org/obo/IAO_0000233> "issue: https://github.com/OpenEnergyPlatform/ontology/issues/928
pull request: https://github.com/OpenEnergyPlatform/ontology/pull/944",
        rdfs:label "CRF sector (IPCC 2006): international bunkers"@en
    
    Types: 
        OEO_00000422,
        
            Annotations: <http://purl.obolibrary.org/obo/IAO_0000233> "issue: https://github.com/OpenEnergyPlatform/ontology/issues/858
pull request: https://github.com/OpenEnergyPlatform/ontology/pull/965"
        OEO_00010232 some OEO_00010227
    
    Facts:  
     OEO_00000504  OEO_00000242,
     <http://purl.obolibrary.org/obo/BFO_0000051>  OEO_00010201,
     <http://purl.obolibrary.org/obo/BFO_0000051>  OEO_00010202
    
    
Individual: OEO_00010201

    Annotations: 
        OEO_00010037 "CRF 1.D.1.a",
        <http://purl.obolibrary.org/obo/IAO_0000115> "The CRF sector (IPCC 2006) 'international aviation' is a transport sector defined by the 2006 IPCC Guidelines for National Greenhouse Gas Inventories. It encompasses emissions from flights that depart in one country and arrive in a different country.",
        <http://purl.obolibrary.org/obo/IAO_0000119> "2006 IPCC Guidelines for National Greenhouse Gas Inventories, Volume 1, Chapter 8.5, https://www.ipcc-nggip.iges.or.jp/public/2006gl/",
        <http://purl.obolibrary.org/obo/IAO_0000233> "issue: https://github.com/OpenEnergyPlatform/ontology/issues/928
pull request: https://github.com/OpenEnergyPlatform/ontology/pull/944",
        rdfs:label "CRF sector (IPCC 2006): international aviation"@en
    
    Types: 
        OEO_00000422,
        
            Annotations: <http://purl.obolibrary.org/obo/IAO_0000233> "issue: https://github.com/OpenEnergyPlatform/ontology/issues/858
pull request: https://github.com/OpenEnergyPlatform/ontology/pull/965"
        OEO_00010232 some OEO_00010227
    
    Facts:  
     OEO_00000504  OEO_00000242,
     <http://purl.obolibrary.org/obo/BFO_0000050>  OEO_00010200
    
    DifferentFrom: 
        OEO_00010059
    
    
Individual: OEO_00010202

    Annotations: 
        OEO_00010037 "CRF 1.D.1.b",
        <http://purl.obolibrary.org/obo/IAO_0000115> "The CRF sector (IPCC 2006) 'maritime navigation' is a transport sector defined by the 2006 IPCC Guidelines for National Greenhouse Gas Inventories. Emissions from fuels used by vessels of all flags that are engaged in international water-borne navigation. The international navigation may take place at sea, on inland lakes and waterways and in coastal waters. It includes emissions from journeys that depart in one country and arrive in a different country. It excludes consumption by fishing vessels.",
        <http://purl.obolibrary.org/obo/IAO_0000119> "2006 IPCC Guidelines for National Greenhouse Gas Inventories, Volume 1, Chapter 8.5, https://www.ipcc-nggip.iges.or.jp/public/2006gl/",
        <http://purl.obolibrary.org/obo/IAO_0000233> "issue: https://github.com/OpenEnergyPlatform/ontology/issues/928
pull request: https://github.com/OpenEnergyPlatform/ontology/pull/944",
        rdfs:label "CRF sector (IPCC 2006): maritime navigation"@en
    
    Types: 
        OEO_00000422,
        
            Annotations: <http://purl.obolibrary.org/obo/IAO_0000233> "issue: https://github.com/OpenEnergyPlatform/ontology/issues/858
pull request: https://github.com/OpenEnergyPlatform/ontology/pull/965"
        OEO_00010232 some OEO_00010227
    
    Facts:  
     OEO_00000504  OEO_00000242,
     <http://purl.obolibrary.org/obo/BFO_0000050>  OEO_00010200
    
    DifferentFrom: 
        OEO_00010062
    
    
Individual: OEO_00010203

    Annotations: 
        OEO_00010037 "CRF 1.D.2",
        <http://purl.obolibrary.org/obo/IAO_0000115> "The CRF sector (IPCC 2006) 'multilateral operation' is a transport sector defined by the 2006 IPCC Guidelines for National Greenhouse Gas Inventories:
Emissions from fuels used for aviation and waterborne navigation in multilateral operations pursuant to the Charter of the United Nations.",
        <http://purl.obolibrary.org/obo/IAO_0000119> "2006 IPCC Guidelines for National Greenhouse Gas Inventories, Volume 2, Chapter 3.1, https://www.ipcc-nggip.iges.or.jp/public/2006gl/",
        <http://purl.obolibrary.org/obo/IAO_0000233> "issue: https://github.com/OpenEnergyPlatform/ontology/issues/928
pull request: https://github.com/OpenEnergyPlatform/ontology/pull/944",
        rdfs:label "CRF sector (IPCC 2006): multilateral operations"@en
    
    Types: 
        OEO_00000422,
        
            Annotations: <http://purl.obolibrary.org/obo/IAO_0000233> "issue: https://github.com/OpenEnergyPlatform/ontology/issues/858
pull request: https://github.com/OpenEnergyPlatform/ontology/pull/965"
        OEO_00010232 some OEO_00010227
    
    Facts:  
     OEO_00000504  OEO_00000242,
     <http://purl.obolibrary.org/obo/BFO_0000050>  OEO_00010199
    
    
Individual: OEO_00010204

    Annotations: 
        <http://purl.obolibrary.org/obo/IAO_0000115> "The MMR sector division is a sector division defined in Annex XII, Table 1 of Commission Implementing Regulation (EU) 749/2014. It uses CRF sectors (IPCC 2006) and adds further sectors.",
        <http://purl.obolibrary.org/obo/IAO_0000116> "Annex XII, Table 1 of Commission Implementing Regulation (EU) 749/2014 https://eur-lex.europa.eu/legal-content/EN/TXT/HTML/?uri=CELEX:32014R0749&from=EN#d1e32-67-1",
        <http://purl.obolibrary.org/obo/IAO_0000233> "issue: https://github.com/OpenEnergyPlatform/ontology/issues/928
pull request: https://github.com/OpenEnergyPlatform/ontology/pull/944",
        rdfs:label "MMR sector division"@en
    
    Types: 
        OEO_00000368
    
    Facts:  
     OEO_00000503  OEO_00000242
    
    
Individual: OEO_00010205

    Annotations: 
        <http://purl.obolibrary.org/obo/IAO_0000115> "The MMR sector 'M.International aviation in the EU ETS' is a transport sector that encompasses that part of the international aviation that is regulated by the European Union Emissions Trading System.",
        <http://purl.obolibrary.org/obo/IAO_0000233> "issue: https://github.com/OpenEnergyPlatform/ontology/issues/928
pull request: https://github.com/OpenEnergyPlatform/ontology/pull/944",
        rdfs:label "MMR sector: M.International aviation in the EU ETS"@en
    
    Types: 
        OEO_00000422,
        
            Annotations: <http://purl.obolibrary.org/obo/IAO_0000233> "issue: https://github.com/OpenEnergyPlatform/ontology/issues/858
pull request: https://github.com/OpenEnergyPlatform/ontology/pull/965"
        OEO_00010232 some OEO_00010227
    
    Facts:  
     OEO_00000504  OEO_00010204,
     <http://purl.obolibrary.org/obo/BFO_0000050>  OEO_00010133,
      not  OEO_00000504  OEO_00010163
    
    
Individual: OEO_00010206

    Annotations: 
        <http://purl.obolibrary.org/obo/IAO_0000115> "'Total emissions excluding LULUCF and including international aviation' is a sector that encompasses 'CRF sector (IPCC 2006): total emissions excluding LULUCF' and 'CRF sector (IPCC 2006): international bunkers'.",
        
            Annotations: <http://purl.obolibrary.org/obo/IAO_0000116> "Term used by the European Environment Agency (EEA): https://climate-energy.eea.europa.eu/topics/climate-change-mitigation/greenhouse-gas-emissions-inventory/data"
        <http://purl.obolibrary.org/obo/IAO_0000118> "total emissions with international transport (EEA)",
        rdfs:label "total emissions excluding LULUCF and including international bunkers"@en
    
    Types: 
        OEO_00000367
    
    Facts:  
     OEO_00000503  OEO_00000242,
     <http://purl.obolibrary.org/obo/BFO_0000051>  OEO_00010197,
     <http://purl.obolibrary.org/obo/BFO_0000051>  OEO_00010200
    
    
Individual: OEO_00010207

    Annotations: 
        <http://purl.obolibrary.org/obo/IAO_0000115> "'Total emissions excluding LULUCF and including international aviation' is a sector that 'CRF sector (IPCC 2006): total emissions including LULUCF' and 'CRF sector (IPCC 2006): international bunkers'.",
        
            Annotations: <http://purl.obolibrary.org/obo/IAO_0000116> "Term used by the European Environment Agency (EEA): https://climate-energy.eea.europa.eu/topics/climate-change-mitigation/greenhouse-gas-emissions-inventory/data"
        <http://purl.obolibrary.org/obo/IAO_0000118> "total net emissions with international transport (EEA)",
        rdfs:label "total emissions including LULUCF and including international bunkers"@en
    
    Types: 
        OEO_00000367
    
    Facts:  
     OEO_00000503  OEO_00000242,
     <http://purl.obolibrary.org/obo/BFO_0000051>  OEO_00010198,
     <http://purl.obolibrary.org/obo/BFO_0000051>  OEO_00010200
    
    
Individual: OEO_00010208

    Annotations: 
        <http://purl.obolibrary.org/obo/IAO_0000115> "'Total emissions excluding LULUCF and including international aviation' is a sector that encompasses 'CRF sector (IPCC 2006): total emissions excluding LULUCF' and 'CRF sector (IPCC 2006): international aviation'.",
        <http://purl.obolibrary.org/obo/IAO_0000116> "This definition corresponds to the 2020 emission target of the European Union.",
        
            Annotations: <http://purl.obolibrary.org/obo/IAO_0000116> "Term used by the European Environment Agency (EEA): https://climate-energy.eea.europa.eu/topics/climate-change-mitigation/greenhouse-gas-emissions-inventory/data"
        <http://purl.obolibrary.org/obo/IAO_0000118> "total emissions with international aviation (EU 2020)",
        <http://purl.obolibrary.org/obo/IAO_0000233> "issue: https://github.com/OpenEnergyPlatform/ontology/issues/928
pull request: https://github.com/OpenEnergyPlatform/ontology/pull/944",
        rdfs:label "total emissions excluding LULUCF and including international aviation"@en
    
    Types: 
        OEO_00000367
    
    Facts:  
     OEO_00000503  OEO_00000242,
     <http://purl.obolibrary.org/obo/BFO_0000051>  OEO_00010197,
     <http://purl.obolibrary.org/obo/BFO_0000051>  OEO_00010201
    
    
Individual: OEO_00010209

    Annotations: 
        <http://purl.obolibrary.org/obo/IAO_0000115> "'Total emissions excluding LULUCF and including international aviation' is a sector that 'CRF sector (IPCC 2006): total emissions including LULUCF' and 'CRF sector (IPCC 2006): international aviation'.",
        <http://purl.obolibrary.org/obo/IAO_0000116> "This definition corresponds to the 2030 emission target as specified in the Nationally Determined Contribution (NDC) of the European Union .",
        
            Annotations: <http://purl.obolibrary.org/obo/IAO_0000116> "Term used by the European Environment Agency (EEA): https://climate-energy.eea.europa.eu/topics/climate-change-mitigation/greenhouse-gas-emissions-inventory/data"
        <http://purl.obolibrary.org/obo/IAO_0000118> "total net emissions with international aviation (NDC)",
        <http://purl.obolibrary.org/obo/IAO_0000233> "issue: https://github.com/OpenEnergyPlatform/ontology/issues/928
pull request: https://github.com/OpenEnergyPlatform/ontology/pull/944",
        rdfs:label "total emissions including LULUCF and including international aviation"@en
    
    Types: 
        OEO_00000367
    
    Facts:  
     OEO_00000503  OEO_00000242,
     <http://purl.obolibrary.org/obo/BFO_0000051>  OEO_00010198,
     <http://purl.obolibrary.org/obo/BFO_0000051>  OEO_00010201
    
    
Individual: OEO_00010228

    Annotations: 
        <http://purl.obolibrary.org/obo/IAO_0000115> "The CRF sector (IPCC 2006): 'CO2 emissions from biomass' is a sector defined by the 2006 IPCC Guidelines for National Greenhouse Gas Inventories: CO2 emissions from biomass combustion are not included in national totals, but are recorded as an information item for cross-checking purposes as well as avoiding double counting.",
        <http://purl.obolibrary.org/obo/IAO_0000119> "2006 IPCC Guidelines for National Greenhouse Gas Inventories, Volume 2, Chapter 1, https://www.ipcc-nggip.iges.or.jp/public/2006gl/",
        <http://purl.obolibrary.org/obo/IAO_0000233> "issue: https://github.com/OpenEnergyPlatform/ontology/issues/858
pull request: https://github.com/OpenEnergyPlatform/ontology/pull/965",
        rdfs:label "CRF sector (IPCC 2006): CO2 emissions from biomass"@en
    
    Types: 
        OEO_00000367,
        OEO_00010232 some OEO_00010227
    
    Facts:  
     OEO_00000504  OEO_00000242
    
    
Individual: OEO_00010229

    Annotations: 
        <http://purl.obolibrary.org/obo/IAO_0000115> "The CRF sector (IPCC 2006): 'CO2 captured' is a sector defined by the 2006 IPCC Guidelines for National Greenhouse Gas Inventories: It encompasses the total amount of CO2 captured for storage.",
        <http://purl.obolibrary.org/obo/IAO_0000119> "2006 IPCC Guidelines for National Greenhouse Gas Inventories, Volume 2, Chapter 5.9, https://www.ipcc-nggip.iges.or.jp/public/2006gl/",
        <http://purl.obolibrary.org/obo/IAO_0000233> "issue: https://github.com/OpenEnergyPlatform/ontology/issues/858
pull request: https://github.com/OpenEnergyPlatform/ontology/pull/965",
        rdfs:label "CRF sector (IPCC 2006): CO2 captured"@en
    
    Types: 
        OEO_00000367,
        OEO_00010232 some OEO_00010227
    
    Facts:  
     OEO_00000504  OEO_00000242
    
    DifferentFrom: 
        OEO_00010058
    
    
Individual: OEO_00010230

    Annotations: 
        <http://purl.obolibrary.org/obo/IAO_0000115> "The CRF sector (IPCC 2006): 'indirect CO2' is a sector defined by the 2006 IPCC Guidelines for National Greenhouse Gas Inventories: It encompasses Methane, carbon monoxide (CO) or NMVOC emissions that will eventually be oxidised to CO2 in the atmosphere.",
        <http://purl.obolibrary.org/obo/IAO_0000119> "2006 IPCC Guidelines for National Greenhouse Gas Inventories, Volume 1, Chapter 7.2.1.5, https://www.ipcc-nggip.iges.or.jp/public/2006gl/",
        <http://purl.obolibrary.org/obo/IAO_0000233> "issue: https://github.com/OpenEnergyPlatform/ontology/issues/858
pull request: https://github.com/OpenEnergyPlatform/ontology/pull/965",
        rdfs:label "CRF sector (IPCC 2006): indirect CO2"@en
    
    Types: 
        OEO_00000367,
        OEO_00010232 some OEO_00010227
    
    Facts:  
     OEO_00000504  OEO_00000242
    
    
DisjointClasses: 
    OEO_00000145,OEO_00000213,OEO_00000422

