Prefix: : <http://openenergy-platform.org/ontology/oeo/>
Prefix: bfo: <http://purl.obolibrary.org/obo/bfo.owl#>
Prefix: dc: <http://purl.org/dc/elements/1.1/>
Prefix: obda: <https://w3id.org/obda/vocabulary#>
Prefix: owl: <http://www.w3.org/2002/07/owl#>
Prefix: rdf: <http://www.w3.org/1999/02/22-rdf-syntax-ns#>
Prefix: rdfs: <http://www.w3.org/2000/01/rdf-schema#>
Prefix: xml: <http://www.w3.org/XML/1998/namespace>
Prefix: xsd: <http://www.w3.org/2001/XMLSchema#>



Ontology: <http://openenergy-platform.org/ontology/oeo/oeo-physical/>
<http://openenergy-platform.org/ontology/oeo/releases/v1.2.0/oeo-physical.omn>
Import: <http://openenergy-platform.org/ontology/oeo/releases/v1.2.0/oeo-shared.omn>
Import: <http://openenergy-platform.org/ontology/oeo/releases/v1.2.0/imports/iao-minimal-module.owl>

Annotations: 
    dc:description "The Open Energy Ontology is an ontology for all aspects of the energy modelling domain. The 'Physical' module covers all those aspects of the world that are relevant for the energy systems domain, including physical entities such as generators, power lines, technologies, hardware, portions of matter; attributes of those, such as the energy they carry or release, whether they can be a pollutant, or their origins; representational transformations into maps and measures, such as coordinates, units, quantities; and the processes that modify the physical entities, such as energy production.",
    dc:license "http://creativecommons.org/publicdomain/zero/1.0/",
    <http://purl.org/dc/terms/title> "Open Energy Ontology (Physical module)"

AnnotationProperty: <http://purl.obolibrary.org/obo/IAO_0000112>

    
AnnotationProperty: <http://purl.obolibrary.org/obo/IAO_0000115>

    
AnnotationProperty: <http://purl.obolibrary.org/obo/IAO_0000116>

    
AnnotationProperty: <http://purl.obolibrary.org/obo/IAO_0000118>

    
AnnotationProperty: <http://purl.obolibrary.org/obo/IAO_0000119>

    
AnnotationProperty: <http://purl.obolibrary.org/obo/IAO_0000233>

    
AnnotationProperty: <http://purl.org/dc/terms/title>

    
AnnotationProperty: <http://www.geneontology.org/formats/oboInOwl#hasExactSynonym>

    
AnnotationProperty: dc:contributor

    
AnnotationProperty: dc:description

    
AnnotationProperty: dc:license

    
AnnotationProperty: rdfs:comment

    
AnnotationProperty: rdfs:isDefinedBy

    
AnnotationProperty: rdfs:label

    
Datatype: rdf:PlainLiteral

    
ObjectProperty: <http://purl.obolibrary.org/obo/BFO_0000050>

    
ObjectProperty: <http://purl.obolibrary.org/obo/BFO_0000051>

    
ObjectProperty: <http://purl.obolibrary.org/obo/RO_0000056>

    
ObjectProperty: <http://purl.obolibrary.org/obo/RO_0000057>

    
ObjectProperty: <http://purl.obolibrary.org/obo/RO_0000085>

    
ObjectProperty: <http://purl.obolibrary.org/obo/RO_0000086>

    
ObjectProperty: <http://purl.obolibrary.org/obo/RO_0000087>

    
ObjectProperty: <http://purl.obolibrary.org/obo/RO_0000091>

    
ObjectProperty: <http://purl.obolibrary.org/obo/RO_0002233>

    
ObjectProperty: <http://purl.obolibrary.org/obo/RO_0002234>

    
ObjectProperty: <http://purl.obolibrary.org/obo/uo#is_unit_of>

    
ObjectProperty: OEO_00000500

    
ObjectProperty: OEO_00000501

    
ObjectProperty: OEO_00000502

    
ObjectProperty: OEO_00000503

    
ObjectProperty: OEO_00000521

    Annotations: 
        <http://purl.obolibrary.org/obo/IAO_0000115> "the property of an artificial object to apply to a technology.",
        rdfs:label "applies technology"
    
    Domain: 
        OEO_00000061
    
    Range: 
        OEO_00000407
    
    InverseOf: 
        OEO_00000525
    
    
ObjectProperty: OEO_00000522

    
ObjectProperty: OEO_00000523

    Annotations: 
        rdfs:comment "A relation that holds between a publication/model calculation/model and the energycarrier it covers.",
        rdfs:label "covers energycarrier"
    
    SubPropertyOf: 
        OEO_00000522
    
    Range: 
        OEO_00000151
    
    
ObjectProperty: OEO_00000524

    Annotations: 
        <http://purl.obolibrary.org/obo/IAO_0000115> "A relation between a portion of matter and the global warming potential it has.",
        <http://purl.obolibrary.org/obo/IAO_0000233> "issue: https://github.com/OpenEnergyPlatform/ontology/issues/66
pull requests: https://github.com/OpenEnergyPlatform/ontology/pull/478",
        rdfs:label "has global warming potential"
    
    SubPropertyOf: 
        owl:topObjectProperty
    
    Domain: 
        OEO_00000198
    
    
ObjectProperty: OEO_00000525

    Annotations: 
        <http://purl.obolibrary.org/obo/IAO_0000115> "The property of a technology to be applied to an artificial object.",
        rdfs:label "is applied to object"
    
    Domain: 
        OEO_00000407
    
    Range: 
        OEO_00000061
    
    InverseOf: 
        OEO_00000521
    
    
ObjectProperty: OEO_00000526

    Annotations: 
        <http://purl.obolibrary.org/obo/IAO_0000115> "A relation that holds between two nodes in a graph that are connected to each other through an edge.",
        <http://purl.obolibrary.org/obo/IAO_0000233> "issue: https://github.com/OpenEnergyPlatform/ontology/issues/66
pull requests: https://github.com/OpenEnergyPlatform/ontology/pull/478",
        rdfs:label "is connected to"
    
    SubPropertyOf: 
        owl:topObjectProperty
    
    Characteristics: 
        Symmetric
    
    
ObjectProperty: OEO_00000527

    Annotations: 
        <http://purl.obolibrary.org/obo/IAO_0000115> "A relation that holds between a directed graph and a node in that graph that has edges ending but not starting there.",
        <http://purl.obolibrary.org/obo/IAO_0000233> "issue: https://github.com/OpenEnergyPlatform/ontology/issues/66
pull requests: https://github.com/OpenEnergyPlatform/ontology/pull/478",
        rdfs:label "has sink"
    
    SubPropertyOf: 
        OEO_00000526
    
    DisjointWith: 
        OEO_00000528
    
    
ObjectProperty: OEO_00000528

    Annotations: 
        <http://purl.obolibrary.org/obo/IAO_0000115> "A relation that holds between a directed graph and a node in that graph that has edges starting but not ending there.",
        <http://purl.obolibrary.org/obo/IAO_0000233> "issue: https://github.com/OpenEnergyPlatform/ontology/issues/66
pull requests: https://github.com/OpenEnergyPlatform/ontology/pull/478",
        rdfs:label "has source"
    
    SubPropertyOf: 
        OEO_00000526
    
    DisjointWith: 
        OEO_00000527
    
    
ObjectProperty: OEO_00000529

    Annotations: 
        <http://purl.obolibrary.org/obo/IAO_0000115> "x has normal state of matter y if and only if a portion of x occurs in state y under normal pressure (1 bar) and normal temperature (0Â°C)",
        rdfs:label "has normal state of matter"
    
    SubPropertyOf: 
        <http://purl.obolibrary.org/obo/RO_0000086>
    
    Domain: 
        OEO_00000331
    
    Range: 
        OEO_00000395
    
    
ObjectProperty: OEO_00000530

    Annotations: 
        <http://purl.obolibrary.org/obo/IAO_0000115> "x has the origin of y",
        rdfs:label "has origin"
    
    SubPropertyOf: 
        <http://purl.obolibrary.org/obo/RO_0000086>
    
    Domain: 
        OEO_00000331
    
    Range: 
        OEO_00000316
    
    
ObjectProperty: OEO_00000531

    Annotations: 
        rdfs:label "has state of matter"
    
    SubPropertyOf: 
        <http://purl.obolibrary.org/obo/RO_0000086>
    
    Domain: 
        OEO_00000331
    
    Range: 
        OEO_00000395
    
    
ObjectProperty: OEO_00000532

    Annotations: 
        <http://purl.obolibrary.org/obo/IAO_0000115> "A relation that holds between a transformation and its input."@en,
        rdfs:label "has physical input"
    
    SubPropertyOf: 
        <http://purl.obolibrary.org/obo/RO_0002233>
    
    Characteristics: 
        Functional,
        Irreflexive,
        Asymmetric
    
    Range: 
        <http://purl.obolibrary.org/obo/RO_0000091> some OEO_00000151
    
    
ObjectProperty: OEO_00000533

    Annotations: 
        <http://purl.obolibrary.org/obo/IAO_0000115> "A relation that holds between a transformation and its output."@en,
        rdfs:label "has physical output"
    
    SubPropertyOf: 
        <http://purl.obolibrary.org/obo/RO_0002234>
    
    
ObjectProperty: OEO_00040010

    
ObjectProperty: OEO_00140002

    
ObjectProperty: owl:topObjectProperty

    
Class: <http://purl.obolibrary.org/obo/BFO_0000002>

    
Class: <http://purl.obolibrary.org/obo/BFO_0000003>

    
Class: <http://purl.obolibrary.org/obo/BFO_0000006>

    
Class: <http://purl.obolibrary.org/obo/BFO_0000009>

    
Class: <http://purl.obolibrary.org/obo/BFO_0000015>

    
Class: <http://purl.obolibrary.org/obo/BFO_0000016>

    
Class: <http://purl.obolibrary.org/obo/BFO_0000019>

    
Class: <http://purl.obolibrary.org/obo/BFO_0000023>

    
Class: <http://purl.obolibrary.org/obo/BFO_0000024>

    
Class: <http://purl.obolibrary.org/obo/BFO_0000027>

    
Class: <http://purl.obolibrary.org/obo/BFO_0000029>

    
Class: <http://purl.obolibrary.org/obo/BFO_0000030>

    
Class: <http://purl.obolibrary.org/obo/BFO_0000031>

    
Class: <http://purl.obolibrary.org/obo/BFO_0000034>

    
Class: <http://purl.obolibrary.org/obo/BFO_0000038>

    
Class: <http://purl.obolibrary.org/obo/BFO_0000141>

    
Class: <http://purl.obolibrary.org/obo/BFO_0000144>

    
Class: <http://purl.obolibrary.org/obo/IAO_0000030>

    
Class: <http://purl.obolibrary.org/obo/RO_0002577>

    
Class: <http://purl.obolibrary.org/obo/UO_0000000>

    
Class: <http://purl.obolibrary.org/obo/UO_0000001>

    
Class: <http://purl.obolibrary.org/obo/UO_0000111>

    
Class: <http://purl.obolibrary.org/obo/UO_0010006>

    
Class: OEO_00000001

    Annotations: 
        <http://purl.obolibrary.org/obo/IAO_0000115> "A fuel role is a role of a portion of matter that has the disposition to be an energy carrier and is used in a process that releases the carried energy by transforming the portion of matter into a different kind of portion of matter in a way that releases heat or does work.",
        <http://purl.obolibrary.org/obo/IAO_0000233> "issue: https://github.com/OpenEnergyPlatform/ontology/issues/227
pull request: https://github.com/OpenEnergyPlatform/ontology/pull/279",
        rdfs:label "fuel role"
    
    SubClassOf: 
        <http://purl.obolibrary.org/obo/BFO_0000023>
    
    
Class: OEO_00000003

    Annotations: 
        <http://purl.obolibrary.org/obo/IAO_0000115> "A biofuel power unit is a power generating unit using biofuel.",
        rdfs:label "biofuel power unit"
    
    SubClassOf: 
        OEO_00000334,
        OEO_00000503 some OEO_00000072
    
    
Class: OEO_00000004

    Annotations: 
        <http://purl.obolibrary.org/obo/IAO_0000115> "A biogas powerplant is a biofuel powerplant having an aggregate of biogas powerunits as its power generating units.",
        rdfs:label "biogas powerplant"
    
    SubClassOf: 
        OEO_00000073
    
    
Class: OEO_00000005

    Annotations: 
        <http://purl.obolibrary.org/obo/IAO_0000115> "A biogas power unit is a biofuel power unit using biogas as fuel.",
        rdfs:label "biogas power unit"
    
    SubClassOf: 
        OEO_00000003,
        OEO_00000503 some OEO_00000074
    
    
Class: OEO_00000006

    Annotations: 
        <http://purl.obolibrary.org/obo/IAO_0000115> "Carbon dioxide is a portion of matter with the chemical formula CO2. It has a gaseous normal state of matter. It occurs naturally in the atmosphere as a trace gas and can work as a greenhouse gas.",
        <http://purl.obolibrary.org/obo/IAO_0000118> "CO2",
        rdfs:label "carbon dioxide"
    
    SubClassOf: 
        OEO_00000331,
        <http://purl.obolibrary.org/obo/RO_0000091> some OEO_00000198,
        OEO_00000529 value OEO_00000182
    
    
Class: OEO_00000007

    Annotations: 
        <http://purl.obolibrary.org/obo/IAO_0000115> "Chemical energy is energy that is stored in the chemical bonds of a substance, which can be released by a chemical reaction.",
        <http://purl.obolibrary.org/obo/IAO_0000233> "issue: https://github.com/OpenEnergyPlatform/ontology/issues/174
pull request: https://github.com/OpenEnergyPlatform/ontology/pull/214",
        rdfs:label "chemical energy"
    
    SubClassOf: 
        OEO_00000150
    
    
Class: OEO_00000008

    Annotations: 
        <http://purl.obolibrary.org/obo/IAO_0000115> "A coal power unit is a power generating unit using coal as fuel.",
        rdfs:label "coal power unit"
    
    SubClassOf: 
        OEO_00000334,
        OEO_00000503 some OEO_00000088
    
    
Class: OEO_00000009

    Annotations: 
        rdfs:comment "An electric heat pump is a heat pump that uses electric energy as drive energy.",
        rdfs:label "electric heat pump"
    
    SubClassOf: 
        OEO_00000212
    
    
Class: OEO_00000010

    Annotations: 
        <http://purl.obolibrary.org/obo/IAO_0000115> "An electro motive generator is a generator that converts kinetic energy into electric energy.",
        rdfs:label "electro motive generator"
    
    SubClassOf: 
        OEO_00000188
    
    
Class: OEO_00000011

    Annotations: 
        <http://purl.obolibrary.org/obo/IAO_0000115> "An energy converting device is an artificial object that transforms or changes a certain type of energy.",
        <http://purl.obolibrary.org/obo/IAO_0000233> "issue: https://github.com/OpenEnergyPlatform/ontology/issues/173
pull request: https://github.com/OpenEnergyPlatform/ontology/pull/273",
        rdfs:comment "formerly called energy transformer",
        rdfs:label "energy converting device"
    
    SubClassOf: 
        OEO_00000061
    
    
Class: OEO_00000012

    Annotations: 
        <http://purl.obolibrary.org/obo/IAO_0000115> "Energy storage is a function of an artificial object that has been engineered to contain energy for conversion as usable energy later.",
        <http://purl.obolibrary.org/obo/IAO_0000233> "issue: https://github.com/OpenEnergyPlatform/ontology/issues/209
pull request: https://github.com/OpenEnergyPlatform/ontology/pull/276",
        rdfs:label "energy storage"
    
    SubClassOf: 
        OEO_00000151,
        <http://purl.obolibrary.org/obo/BFO_0000034>
    
    
Class: OEO_00000013

    Annotations: 
        <http://purl.obolibrary.org/obo/IAO_0000115> "A fluorinated greenhouse gas is a greenhouse gas that is produced by fluorination. Hence it contains Fluor (F) atoms and is of anthropogenic origin.",
        rdfs:label "fluorinated greenhouse gas"
    
    EquivalentTo: 
        OEO_00000026 or OEO_00000038 or OEO_00000219 or OEO_00000322
    
    SubClassOf: 
        OEO_00000020
    
    
Class: OEO_00000014

    Annotations: 
        <http://purl.obolibrary.org/obo/IAO_0000115> "A fossil combustion fuel is a combustion fuel with the origin fossil.",
        rdfs:comment "This class is used to implement the subset relationship between origins fossil and geogenic: Every object with the origin fossil also has the origin geogenic.",
        rdfs:label "fossil combustion fuel"
    
    EquivalentTo: 
        OEO_00000099
         and (OEO_00000530 some OEO_00030002)
    
    SubClassOf: 
        OEO_00000530 some OEO_00030003
    
    
Class: OEO_00000016

    Annotations: 
        <http://purl.obolibrary.org/obo/IAO_0000115> "A fuel cell is a generator that converts chemical energy into electricity using redox reactions.",
        rdfs:label "fuel cell"
    
    SubClassOf: 
        OEO_00000188,
        OEO_00000503 some OEO_00000220
    
    
Class: OEO_00000017

    Annotations: 
        <http://purl.obolibrary.org/obo/IAO_0000115> "A gas fired power unit is a power generating unit using gas as fuel.",
        rdfs:label "gas fired power unit"
    
    SubClassOf: 
        OEO_00000334,
        OEO_00000503 some 
            (OEO_00000173
             and (OEO_00000529 value OEO_00000182))
    
    
Class: OEO_00000019

    Annotations: 
        <http://purl.obolibrary.org/obo/IAO_0000115> "A geothermal power unit is a power unit using geothermal heat.",
        rdfs:label "geothermal power unit"
    
    SubClassOf: 
        OEO_00000334
    
    
Class: OEO_00000020

    Annotations: 
        <http://purl.obolibrary.org/obo/IAO_0000115> "A greenhouse gas is a portion of matter that has the disposition to contribute to the greenhouse effect.",
        <http://purl.obolibrary.org/obo/IAO_0000233> "issue: https://github.com/OpenEnergyPlatform/ontology/issues/56
pull request: https://github.com/OpenEnergyPlatform/ontology/pull/234",
        rdfs:label "greenhouse gas"
    
    EquivalentTo: 
        OEO_00000331
         and (<http://purl.obolibrary.org/obo/RO_0000091> some OEO_00000198)
    
    SubClassOf: 
        OEO_00000331,
        OEO_00000529 value OEO_00000182
    
    
Class: OEO_00000021

    Annotations: 
        <http://purl.obolibrary.org/obo/IAO_0000115> "A hard coal power unit is a coal power unit using hard coal as fuel.",
        rdfs:label "hard coal power unit"
    
    SubClassOf: 
        OEO_00000008,
        OEO_00000503 some OEO_00000204
    
    
Class: OEO_00000022

    Annotations: 
        <http://purl.obolibrary.org/obo/IAO_0000115> "A hydrogen power unit is a power generating unit using hydrogen as fuel.",
        rdfs:label "hydrogen power unit"
    
    SubClassOf: 
        OEO_00000334,
        OEO_00000503 some OEO_00000220
    
    
Class: OEO_00000024

    Annotations: 
        <http://purl.obolibrary.org/obo/IAO_0000115> "A lignite power unit is a coal power unit using lignite as fuel.",
        rdfs:label "lignite power unit"
    
    EquivalentTo: 
        OEO_00000503 some OEO_00000251
    
    SubClassOf: 
        OEO_00000008
    
    
Class: OEO_00000025

    Annotations: 
        <http://purl.obolibrary.org/obo/IAO_0000115> "Methane is a portion of matter with the chemical formular CH4. It has a gaseous normal state of matter. It occurs naturally in the atmosphere as a trace gas and can work as a greenhouse gas. As it can be oxidised it can be used as a fuel.",
        <http://purl.obolibrary.org/obo/IAO_0000118> "CH4",
        rdfs:label "methane"
    
    SubClassOf: 
        OEO_00000331,
        <http://purl.obolibrary.org/obo/RO_0000087> some OEO_00000001,
        <http://purl.obolibrary.org/obo/RO_0000091> some OEO_00000097,
        <http://purl.obolibrary.org/obo/RO_0000091> some OEO_00000198,
        <http://purl.obolibrary.org/obo/RO_0000091> some OEO_00010011,
        OEO_00000529 value OEO_00000182
    
    
Class: OEO_00000026

    Annotations: 
        <http://purl.obolibrary.org/obo/IAO_0000115> "Nitrogen trifluoride is a portion of matter with the chemical formula NF3. It has a gaseous normal state of matter. It can work as a potent greenhouse gas and has an anthropogenic origin.",
        <http://purl.obolibrary.org/obo/IAO_0000118> "NF3",
        rdfs:label "nitrogen trifluoride"
    
    SubClassOf: 
        OEO_00000331,
        OEO_00000530 some OEO_00030000,
        OEO_00000529 value OEO_00000182
    
    
Class: OEO_00000027

    Annotations: 
        <http://purl.obolibrary.org/obo/IAO_0000115> "Nitrous oxide is a portion of matter with the chemical formula N2O. It has a gaseous normal state of matter. It occurs naturally in the atmosphere as a trace gas and it can work as a greenhouse gas.",
        <http://purl.obolibrary.org/obo/IAO_0000118> "N2O",
        rdfs:label "nitrous oxide"
    
    SubClassOf: 
        OEO_00000331,
        <http://purl.obolibrary.org/obo/RO_0000091> some OEO_00000198,
        OEO_00000529 value OEO_00000182
    
    
Class: OEO_00000028

    Annotations: 
        <http://purl.obolibrary.org/obo/IAO_0000115> "A nuclear energy carrier is an energy carrier used in nuclear power stations to produce heat for steam turbines. Heat is created when the nuclear fuel undergoes nuclear fission.",
        <http://purl.obolibrary.org/obo/IAO_0000233> "issue: https://github.com/OpenEnergyPlatform/ontology/issues/182
pull request: https://github.com/OpenEnergyPlatform/ontology/pull/237",
        rdfs:label "nuclear energy carrier disposition"
    
    SubClassOf: 
        OEO_00000151
    
    
Class: OEO_00000029

    Annotations: 
        <http://purl.obolibrary.org/obo/IAO_0000115> "A nuclear power unit is a power generating unit using nuclear fuel.",
        rdfs:label "nuclear power unit"
    
    SubClassOf: 
        OEO_00000334,
        OEO_00000503 some OEO_00000302
    
    
Class: OEO_00000030

    Annotations: 
        <http://purl.obolibrary.org/obo/IAO_0000115> "An oil power unit is a power generating unit using oil as fuel.",
        rdfs:label "oil power unit"
    
    SubClassOf: 
        OEO_00000334,
        OEO_00000503 some OEO_00000309
    
    
Class: OEO_00000031

    Annotations: 
        <http://purl.obolibrary.org/obo/IAO_0000115> "A powerplant is an artificial object consisting of power generating units and a grid component that feeds electric energy into an electric grid.",
        <http://purl.obolibrary.org/obo/IAO_0000233> "issue: https://github.com/OpenEnergyPlatform/ontology/issues/588
pull request: https://github.com/OpenEnergyPlatform/ontology/pull/594

issue: https://github.com/OpenEnergyPlatform/ontology/issues/173
pull request: https://github.com/OpenEnergyPlatform/ontology/pull/273",
        rdfs:label "powerplant"
    
    SubClassOf: 
        OEO_00000061,
        <http://purl.obolibrary.org/obo/BFO_0000051> some OEO_00000334,
        <http://purl.obolibrary.org/obo/BFO_0000051> some OEO_00020006
    
    
Class: OEO_00000032

    Annotations: 
        <http://purl.obolibrary.org/obo/IAO_0000115> "A PV cell is a generator that converts light into electrical energy.",
        rdfs:label "PV cell"
    
    SubClassOf: 
        OEO_00000188
    
    
Class: OEO_00000033

    Annotations: 
        <http://purl.obolibrary.org/obo/IAO_0000115> "A renewable fuel is a fuel that has a renewable origin and an energy carrier disposition that is used as a fuel.",
        rdfs:label "renewable fuel"
    
    EquivalentTo: 
        OEO_00000173
         and (OEO_00000530 some OEO_00030004)
    
    SubClassOf: 
        <http://purl.obolibrary.org/obo/RO_0000091> some OEO_00000097
    
    
Class: OEO_00000034

    Annotations: 
        <http://purl.obolibrary.org/obo/IAO_0000115> "A solar power unit is a power generating unit using solar power.",
        rdfs:label "solar power unit"
    
    SubClassOf: 
        OEO_00000334
    
    
Class: OEO_00000035

    Annotations: 
        <http://purl.obolibrary.org/obo/IAO_0000115> "A solar thermal power unit is a solar power unit that has solar thermal collectors as parts.",
        rdfs:label "solar thermal power unit"
    
    SubClassOf: 
        OEO_00000034,
        <http://purl.obolibrary.org/obo/BFO_0000051> some OEO_00000387
    
    
Class: OEO_00000036

    Annotations: 
        <http://purl.obolibrary.org/obo/IAO_0000115> "A solid biomass powerplant is a biomass powerplant having an aggregate of solid biomass power units as its power generating units.",
        rdfs:label "solid biomass powerplant"
    
    SubClassOf: 
        OEO_00000073
    
    
Class: OEO_00000037

    Annotations: 
        <http://purl.obolibrary.org/obo/IAO_0000115> "A solid biomass power unit is a biomass power unit using solid biomass as fuel.",
        rdfs:label "solid biomass power unit"
    
    SubClassOf: 
        OEO_00000003,
        OEO_00000503 some OEO_00000332
    
    
Class: OEO_00000038

    Annotations: 
        <http://purl.obolibrary.org/obo/IAO_0000115> "Sulphur hexafluoride is a portion of matter with the chemical formula SF6. It has a gaseous normal state of matter. It can work as a potent greenhouse gas and has an anthropogenic origin.",
        <http://purl.obolibrary.org/obo/IAO_0000118> "SF6",
        rdfs:label "sulphur hexafluoride"
    
    SubClassOf: 
        OEO_00000331,
        OEO_00000530 some OEO_00030000,
        OEO_00000529 value OEO_00000182
    
    
Class: OEO_00000039

    Annotations: 
        <http://purl.obolibrary.org/obo/IAO_0000115> "A thermal energy storage is an energy storage that stores thermal energy for later use.",
        rdfs:label "thermal energy storage"
    
    SubClassOf: 
        OEO_00000012
    
    
Class: OEO_00000040

    Annotations: 
        <http://purl.obolibrary.org/obo/IAO_0000115> "Uranium is a portion of matter that has the atomic number 92. It is a silver-grey metal.",
        <http://purl.obolibrary.org/obo/IAO_0000233> "issue: https://github.com/OpenEnergyPlatform/ontology/issues/182
pull request: https://github.com/OpenEnergyPlatform/ontology/pull/237",
        rdfs:label "uranium"
    
    SubClassOf: 
        OEO_00000331,
        OEO_00000530 some OEO_00030003,
        <http://purl.obolibrary.org/obo/RO_0000087> some OEO_00000001,
        <http://purl.obolibrary.org/obo/RO_0000091> some OEO_00000028,
        OEO_00000529 value OEO_00000390
    
    
Class: OEO_00000041

    Annotations: 
        <http://purl.obolibrary.org/obo/IAO_0000115> "A waste power unit is a power generating unit using waste as fuel.",
        rdfs:label "waste power unit"
    
    SubClassOf: 
        OEO_00000334,
        OEO_00000503 some OEO_00000439
    
    
Class: OEO_00000042

    Annotations: 
        <http://purl.obolibrary.org/obo/IAO_0000115> "A waste role is a role of an object aggregate that has been discarded after primary use.",
        <http://purl.obolibrary.org/obo/IAO_0000233> "issue: https://github.com/OpenEnergyPlatform/ontology/issues/132
pull request: https://github.com/OpenEnergyPlatform/ontology/pull/207",
        rdfs:label "waste role"
    
    SubClassOf: 
        <http://purl.obolibrary.org/obo/BFO_0000023>
    
    
Class: OEO_00000043

    Annotations: 
        <http://purl.obolibrary.org/obo/IAO_0000115> "Wind is a process of air naturally moving.",
        <http://purl.obolibrary.org/obo/IAO_0000233> "issue: https://github.com/OpenEnergyPlatform/ontology/issues/211
pull request: https://github.com/OpenEnergyPlatform/ontology/pull/225",
        rdfs:label "wind"
    
    SubClassOf: 
        <http://purl.obolibrary.org/obo/BFO_0000015>
    
    
Class: OEO_00000044

    Annotations: 
        <http://purl.obolibrary.org/obo/IAO_0000115> "A wind energy converting unit is a power generating unit that uses wind energy.",
        <http://purl.obolibrary.org/obo/IAO_0000118> "wind turbine",
        rdfs:label "wind energy converting unit"
    
    SubClassOf: 
        OEO_00000334,
        <http://purl.obolibrary.org/obo/BFO_0000051> some OEO_00000425,
        <http://purl.obolibrary.org/obo/RO_0000086> some OEO_00140000
    
    
Class: OEO_00000047

    Annotations: 
        <http://purl.obolibrary.org/obo/IAO_0000115> "An AC-line is a powerline for transferring high voltage alternating current."@en,
        <http://purl.obolibrary.org/obo/IAO_0000233> "issue: https://github.com/OpenEnergyPlatform/ontology/issues/231
pull request: https://github.com/OpenEnergyPlatform/ontology/pull/385",
        rdfs:comment "undirected",
        rdfs:label "AC-line"@en
    
    SubClassOf: 
        OEO_00000253
    
    DisjointWith: 
        OEO_00000126
    
    
Class: OEO_00000054

    Annotations: 
        <http://purl.obolibrary.org/obo/IAO_0000115> "Air is a portion of matter that consists of a composition of gases that forms the Earth's atmosphere."@en,
        <http://purl.obolibrary.org/obo/IAO_0000119> "https://en.wikipedia.org/wiki/Air_(disambiguation)",
        rdfs:label "air"
    
    SubClassOf: 
        OEO_00000331,
        OEO_00000501 some OEO_00000399,
        <http://purl.obolibrary.org/obo/RO_0000091> some OEO_00000151,
        OEO_00000529 value OEO_00000182
    
    
Class: OEO_00000055

    Annotations: 
        <http://purl.obolibrary.org/obo/IAO_0000115> "Air pollution occurs when harmful or excessive quantities of substances including gases, particles, and biological molecules are introduced into Earth's atmosphere."@en,
        <http://purl.obolibrary.org/obo/IAO_0000119> "https://en.wikipedia.org/w/index.php?title=Air_pollution&oldid=877082014"@en,
        <http://purl.obolibrary.org/obo/IAO_0000233> "issue: https://github.com/OpenEnergyPlatform/ontology/issues/406
pull request: https://github.com/OpenEnergyPlatform/ontology/pull/410",
        rdfs:label "air pollution"
    
    SubClassOf: 
        OEO_00000330,
        <http://purl.obolibrary.org/obo/RO_0000057> some OEO_00010012
    
    
Class: OEO_00000056

    Annotations: 
        <http://purl.obolibrary.org/obo/IAO_0000115> "Ambient heat, understood as heat that is naturally around us in its diffuse and extended form, emanates from a diversity of heat sources, including earth, water, or air, and is increasingly attracting the attention of those concerned with energy and sustainability."@en,
        <http://purl.obolibrary.org/obo/IAO_0000119> "Urchueguia, J. F. (2016). Shallow geothermal and ambient heat technologies for renewable heating. In Renewable Heating and Cooling (pp. 89-118). Woodhead Publishing."@en,
        rdfs:label "ambient heat"
    
    SubClassOf: 
        OEO_00000207
    
    
Class: OEO_00000058

    Annotations: 
        <http://purl.obolibrary.org/obo/IAO_0000115> "Anthracite is a hard coal with a high caloric value due to its high carbon content (about 90 % fixed carbon).",
        <http://purl.obolibrary.org/obo/IAO_0000119> "REGULATION (EC) No 1099/2008 OF THE EUROPEAN PARLIAMENT AND OF THE COUNCIL of 22 October 2008 on energy statistics https://eur-lex.europa.eu/legal-content/EN/TXT/HTML/?uri=CELEX:32008R1099&from=EN"@en,
        rdfs:comment "Its gross calorific value is greater than 23 865 kJ/kg (5 700 kcal/kg) on an ash-free but moist basis."@en,
        rdfs:label "anthracite"
    
    SubClassOf: 
        OEO_00000204
    
    
Class: OEO_00000061

    Annotations: 
        <http://purl.obolibrary.org/obo/IAO_0000115> "An artificial object is an object that was deliberately manufactured by humans to address a particular purpose.",
        <http://purl.obolibrary.org/obo/IAO_0000233> "issue: https://github.com/OpenEnergyPlatform/ontology/issues/86
pull requests: https://github.com/OpenEnergyPlatform/ontology/pull/121 (artificial object definition),
 https://github.com/OpenEnergyPlatform/ontology/pull/128 (subclasses)",
        rdfs:label "artificial object"
    
    SubClassOf: 
        <http://purl.obolibrary.org/obo/BFO_0000030>
    
    
Class: OEO_00000062

    Annotations: 
        <http://purl.obolibrary.org/obo/IAO_0000115> "Associated gas is a natural gas that is a byproduct from crude oil exploitation."@en,
        <http://purl.obolibrary.org/obo/IAO_0000119> "REGULATION (EC) No 1099/2008 OF THE EUROPEAN PARLIAMENT AND OF THE COUNCIL of 22 October 2008 on energy statistics https://eur-lex.europa.eu/legal-content/EN/TXT/HTML/?uri=CELEX:32008R1099&from=EN"@en,
        rdfs:label "associated gas"
    
    SubClassOf: 
        OEO_00000292
    
    
Class: OEO_00000066

    Annotations: 
        <http://purl.obolibrary.org/obo/IAO_0000115> "Aviation gasoline is gasoline used as motor spirit and prepared especially for aviation piston engines, with an octane number suited to the engine, a freezing point of -60 Â°C and a distillation range usually within the limits of 30 Â°C and 180 Â°C."@en,
        <http://purl.obolibrary.org/obo/IAO_0000119> "REGULATION (EC) No 1099/2008 OF THE EUROPEAN PARLIAMENT AND OF THE COUNCIL of 22 October 2008 on energy statistics https://eur-lex.europa.eu/legal-content/EN/TXT/HTML/?uri=CELEX:32008R1099&from=EN"@en,
        rdfs:label "aviation gasoline"
    
    SubClassOf: 
        OEO_00000183
    
    
Class: OEO_00000068

    Annotations: 
        <http://purl.obolibrary.org/obo/IAO_0000115> "A battery is a device using different chemical or physical reactions to store energy."@en,
        rdfs:label "battery"
    
    SubClassOf: 
        OEO_00000159,
        <http://purl.obolibrary.org/obo/RO_0000085> some OEO_00000070
    
    
Class: OEO_00000070

    Annotations: 
        <http://purl.obolibrary.org/obo/IAO_0000115> "A battery storage is a energy storage that uses batteries to store energy."@en,
        rdfs:label "battery storage"
    
    SubClassOf: 
        OEO_00000012
    
    DisjointWith: 
        OEO_00000269
    
    
Class: OEO_00000071

    Annotations: 
        <http://purl.obolibrary.org/obo/IAO_0000115> "Biodiesel is a portion of matter that includes bio-diesel (a methyl-ester produced from vegetable or animal oil, of diesel quality), biodimethylether (dimethylether produced from biomass), Fischer-Tropsch (Fischer-Tropsch produced from biomass), cold extracted bio-oil (oil produced from oil seed through mechanical processing only) and all other liquid biofuels which are added to, blended with or used straight as transport diesel.",
        <http://purl.obolibrary.org/obo/IAO_0000119> "REGULATION (EC) No 1099/2008 OF THE EUROPEAN PARLIAMENT AND OF THE COUNCIL of 22 October 2008 on energy statistics https://eur-lex.europa.eu/legal-content/EN/TXT/HTML/?uri=CELEX:32008R1099&from=EN",
        rdfs:label "biodiesel"
    
    SubClassOf: 
        OEO_00000331,
        OEO_00000530 some OEO_00030001,
        <http://purl.obolibrary.org/obo/RO_0000087> some OEO_00000001,
        <http://purl.obolibrary.org/obo/RO_0000091> some OEO_00000097,
        OEO_00000529 value OEO_00000256
    
    
Class: OEO_00000072

    Annotations: 
        <http://purl.obolibrary.org/obo/IAO_0000115> "A biofuel is a fuel that is produced through contemporary biological processes, such as agriculture and anaerobic digestion, rather than a fuel produced by geological processes such as those involved in the formation of fossil fuels, such as coal and petroleum, from prehistoric biological matter.

Biofuels can be derived directly from plants (i.e. energy crops), or indirectly from agricultural, commercial, domestic, and/or industrial wastes.[1] Renewable biofuels generally involve contemporary carbon fixation, such as those that occur in plants or microalgae through the process of photosynthesis. Other renewable biofuels are made through the use or conversion of biomass (referring to recently living organisms, most often referring to plants or plant-derived materials). This biomass can be converted to convenient energy-containing substances in three different ways: thermal conversion, chemical conversion, and biochemical conversion. This biomass conversion can result in fuel in solid, liquid, or gas form. This new biomass can also be used directly for biofuels.",
        <http://purl.obolibrary.org/obo/IAO_0000119> "https://en.wikipedia.org/w/index.php?title=Biofuel&oldid=866432109",
        <http://purl.obolibrary.org/obo/IAO_0000233> "issue: https://github.com/OpenEnergyPlatform/ontology/issues/396
pull request: https://github.com/OpenEnergyPlatform/ontology/pull/400",
        rdfs:label "biofuel"
    
    EquivalentTo: 
        OEO_00000173
         and (OEO_00000530 some OEO_00030001)
    
    SubClassOf: 
        OEO_00000173,
        OEO_00000530 some OEO_00030001,
        OEO_00000530 some OEO_00030004,
        <http://purl.obolibrary.org/obo/RO_0000091> some OEO_00000097
    
    
Class: OEO_00000073

    Annotations: 
        <http://purl.obolibrary.org/obo/IAO_0000115> "A biofuel powerplant is a powerplant having an aggregate of biofuel power units as its power generating units.",
        rdfs:label "biofuel powerplant"
    
    SubClassOf: 
        OEO_00000031,
        <http://purl.obolibrary.org/obo/BFO_0000051> some OEO_00000003
    
    
Class: OEO_00000074

    Annotations: 
        <http://purl.obolibrary.org/obo/IAO_0000115> "A biogas is a biofuel which has a gaseous state and is composed principally of methane and carbon dioxide produced by anaerobic digestion of biomass. It is used as a biofuel.",
        rdfs:label "biogas"
    
    SubClassOf: 
        OEO_00000072,
        OEO_00000530 some OEO_00030001,
        <http://purl.obolibrary.org/obo/RO_0000091> some OEO_00000097,
        OEO_00000529 value OEO_00000182
    
    
Class: OEO_00000075

    Annotations: 
        <http://purl.obolibrary.org/obo/IAO_0000115> "Biogasoline is a portion of matter that includes bioethanol (ethanol produced from biomass and/or the biodegradable fraction of waste), biomethanol (methanol produced from biomass and/or the biodegradable fraction of waste), bioETBE (ethyl-tertio-butyl-ether produced on the basis of bioethanol; the percentage by volume of bioETBE that is calculated as biofuel is 47 %) and bioMTBE (methyl-tertio-butyl-ether produced on the basis of biomethanol: the percentage by volume of bioMTBE that is calculated as biofuel is 36 %)",
        <http://purl.obolibrary.org/obo/IAO_0000118> "Bioethanol"@en,
        <http://purl.obolibrary.org/obo/IAO_0000119> "REGULATION (EC) No 1099/2008 OF THE EUROPEAN PARLIAMENT AND OF THE COUNCIL of 22 October 2008 on energy statistics https://eur-lex.europa.eu/legal-content/EN/TXT/HTML/?uri=CELEX:32008R1099&from=EN",
        <http://purl.obolibrary.org/obo/IAO_0000233> "issue: https://github.com/OpenEnergyPlatform/ontology/issues/439
pull request: https://github.com/OpenEnergyPlatform/ontology/pull/445",
        rdfs:label "biogasoline",
        rdfs:label "biogasoline"@en
    
    SubClassOf: 
        OEO_00000331,
        OEO_00000530 some OEO_00030001,
        <http://purl.obolibrary.org/obo/BFO_0000051> some OEO_00020001,
        <http://purl.obolibrary.org/obo/RO_0000087> some OEO_00000001,
        <http://purl.obolibrary.org/obo/RO_0000091> some OEO_00000097,
        OEO_00000529 value OEO_00000256
    
    
Class: OEO_00000077

    Annotations: 
        <http://purl.obolibrary.org/obo/IAO_0000115> "Blast furnace gas is manufactured coal based gas produced during the combustion of coke in blast furnaces in the iron and steel industry. It is recovered and used as a fuel partly within the plant and partly in other steel industry processes or in power stations equipped to burn it. The quantity of fuel should be reported on a gross calorific value basis."@en,
        <http://purl.obolibrary.org/obo/IAO_0000119> "REGULATION (EC) No 1099/2008 OF THE EUROPEAN PARLIAMENT AND OF THE COUNCIL of 22 October 2008 on energy statistics https://eur-lex.europa.eu/legal-content/EN/TXT/HTML/?uri=CELEX:32008R1099&from=EN"@en,
        rdfs:label "blast furnace gas"
    
    SubClassOf: 
        OEO_00000263
    
    
Class: OEO_00000084

    Annotations: 
        <http://purl.obolibrary.org/obo/IAO_0000115> "Charcoal is a portion of matter consisting of the solid residue of the destructive distillation and pyrolysis of wood and other vegetal material.It is used as a fuel."@en,
        <http://purl.obolibrary.org/obo/IAO_0000119> "REGULATION (EC) No 1099/2008 OF THE EUROPEAN PARLIAMENT AND OF THE COUNCIL of 22 October 2008 on energy statistics https://eur-lex.europa.eu/legal-content/EN/TXT/HTML/?uri=CELEX:32008R1099&from=EN"@en,
        rdfs:label "charcoal"
    
    SubClassOf: 
        OEO_00000331,
        OEO_00000530 some OEO_00030001,
        <http://purl.obolibrary.org/obo/RO_0000087> some OEO_00000001,
        <http://purl.obolibrary.org/obo/RO_0000091> some OEO_00000097,
        OEO_00000529 value OEO_00000390
    
    
Class: OEO_00000088

    Annotations: 
        <http://purl.obolibrary.org/obo/IAO_0000115> "Coal is a portion of matter consisting of combustible black or brownish-black sedimentary rock, formed as rock strata called coal seams. Coal is mostly carbon with variable amounts of other elements; chiefly hydrogen, sulfur, oxygen, and nitrogen.coal is formed if dead plant matter decays into peat and over millions of years the heat and pressure of deep burial converts the peat into coal."@en,
        <http://purl.obolibrary.org/obo/IAO_0000119> "https://en.wikipedia.org/w/index.php?title=Coal&oldid=907331967",
        rdfs:label "coal"
    
    SubClassOf: 
        OEO_00000331,
        OEO_00000530 some OEO_00030002,
        <http://purl.obolibrary.org/obo/RO_0000087> some OEO_00000001,
        <http://purl.obolibrary.org/obo/RO_0000091> some OEO_00000097,
        OEO_00000529 value OEO_00000390
    
    
Class: OEO_00000089

    Annotations: 
        <http://purl.obolibrary.org/obo/IAO_0000115> "A coal powerplant is a powerplant having an aggregate of coal power units as its power generating units."@en,
        rdfs:label "coal powerplant"
    
    SubClassOf: 
        OEO_00000031,
        <http://purl.obolibrary.org/obo/BFO_0000051> some OEO_00000008,
        <http://purl.obolibrary.org/obo/BFO_0000051> some OEO_00000396
    
    
Class: OEO_00000093

    Annotations: 
        <http://purl.obolibrary.org/obo/IAO_0000115> "Coke oven gas is manufactured coal based gas obtained as a by-product of the manufacture of coke oven coke for the production of iron and steel."@en,
        <http://purl.obolibrary.org/obo/IAO_0000119> "REGULATION (EC) No 1099/2008 OF THE EUROPEAN PARLIAMENT AND OF THE COUNCIL of 22 October 2008 on energy statistics https://eur-lex.europa.eu/legal-content/EN/TXT/HTML/?uri=CELEX:32008R1099&from=EN"@en,
        rdfs:label "coke oven gas"
    
    SubClassOf: 
        OEO_00000263
    
    
Class: OEO_00000094

    Annotations: 
        <http://purl.obolibrary.org/obo/IAO_0000115> "Coking coal is hard coal that is bituminous with a quality that allows the production of a coke suitable to support a blast furnace charge. Its gross calorific value is greater than 23 865 kJ/kg (5 700 kcal/kg) on an ash-free but moist basis."@en,
        <http://purl.obolibrary.org/obo/IAO_0000119> "REGULATION (EC) No 1099/2008 OF THE EUROPEAN PARLIAMENT AND OF THE COUNCIL of 22 October 2008 on energy statistics https://eur-lex.europa.eu/legal-content/EN/TXT/HTML/?uri=CELEX:32008R1099&from=EN"@en,
        rdfs:label "coking coal"
    
    SubClassOf: 
        OEO_00000204
    
    
Class: OEO_00000096

    Annotations: 
        <http://purl.obolibrary.org/obo/IAO_0000115> "Colliery gas is natural gas found in coal mines (British English: colliery). The main component is methane. Synonyms are firedamp, mine gas. It is used as a fossil fuel."@en,
        rdfs:label "colliery gas"
    
    SubClassOf: 
        OEO_00000292
    
    
Class: OEO_00000097

    Annotations: 
        <http://purl.obolibrary.org/obo/IAO_0000115> "A combustible energy carrier is an energy carrier that releases energy from a material entity in form of heat or work, by chemical reaction with other substances.",
        rdfs:label "combustible energy carrier disposition"
    
    SubClassOf: 
        OEO_00000151
    
    
Class: OEO_00000099

    Annotations: 
        <http://purl.obolibrary.org/obo/IAO_0000115> "A combustible fuel is a fuel that realizes its fuel role in processes that release energy in the form of heat or work by chemical reaction with other substances.",
        <http://purl.obolibrary.org/obo/IAO_0000233> "issue: https://github.com/OpenEnergyPlatform/ontology/issues/182
pull request: https://github.com/OpenEnergyPlatform/ontology/pull/237",
        rdfs:label "combustion fuel"
    
    EquivalentTo: 
        OEO_00000173
         and (<http://purl.obolibrary.org/obo/RO_0000091> some OEO_00000097)
    
    SubClassOf: 
        OEO_00000173
    
    
Class: OEO_00000102

    Annotations: 
        <http://purl.obolibrary.org/obo/IAO_0000115> "Compressed air is air that has been compressed to store energy. To discharge energy, the air is expanded."@en,
        rdfs:label "compressed air"
    
    SubClassOf: 
        OEO_00000054
    
    
Class: OEO_00000115

    Annotations: 
        <http://purl.obolibrary.org/obo/IAO_0000115> "Crude oil is an oil and petroleum product of natural origin comprising a mixture of hydrocarbons and associated impurities, such as sulphur. It exists in the liquid phase under normal surface temperature and pressure and its physical characteristics (density, viscosity, etc.) are highly variable. This category includes field or lease condensate recovered from associated and non-associated gas where it is commingled with the commercial crude oil stream."@en,
        <http://purl.obolibrary.org/obo/IAO_0000119> "REGULATION (EC) No 1099/2008 OF THE EUROPEAN PARLIAMENT AND OF THE COUNCIL of 22 October 2008 on energy statistics https://eur-lex.europa.eu/legal-content/EN/TXT/HTML/?uri=CELEX:32008R1099&from=EN"@en,
        rdfs:label "crude oil"
    
    SubClassOf: 
        OEO_00000309,
        OEO_00000529 value OEO_00000256
    
    
Class: OEO_00000117

    Annotations: 
        <http://purl.obolibrary.org/obo/IAO_0000115> "A dam is a barrier that stops or restricts the flow of water or underground streams. Reservoirs created by dams not only suppress floods but also provide water for activities such as irrigation, human consumption, industrial use, aquaculture, and navigability. Hydropower is often used in conjunction with dams to generate electricity."@en,
        <http://purl.obolibrary.org/obo/IAO_0000119> "https://en.wikipedia.org/w/index.php?title=Dam&oldid=906014627"@en,
        rdfs:label "dammed water"
    
    SubClassOf: 
        OEO_00000441,
        OEO_00000501 some OEO_00000399
    
    
Class: OEO_00000126

    Annotations: 
        <http://purl.obolibrary.org/obo/IAO_0000115> "An HVDC-line is a powerline for transferring high voltage direct current."@en,
        <http://purl.obolibrary.org/obo/IAO_0000233> "issue: https://github.com/OpenEnergyPlatform/ontology/issues/231
pull request: https://github.com/OpenEnergyPlatform/ontology/pull/385",
        rdfs:comment "directed",
        rdfs:label "HVDC-line"@en
    
    SubClassOf: 
        OEO_00000253
    
    DisjointWith: 
        OEO_00000047
    
    
Class: OEO_00000129

    Annotations: 
        <http://purl.obolibrary.org/obo/IAO_0000115> "Derived heat covers the total heat production in heating plants and in combined heat and power plants. It includes the heat used by the auxiliaries of the installation which use hot fluid (space heating, liquid fuel heating, etc.) And losses in the installation/network heat exchanges. For autoproducing entities (= entities generating electricity and/or heat wholly or partially for their own use as an activity which supports their primary activity) the heat used by the undertaking for its own processes is not included."@en,
        <http://purl.obolibrary.org/obo/IAO_0000119> "https://ec.europa.eu/eurostat/ramon/nomenclatures/index.cfm?TargetUrl=DSP_GLOSSARY_NOM_DTL_VIEW&StrNom=CODED2&StrLanguageCode=EN&IntKey=16452285&RdoSearch=&TxtSearch=&CboTheme=&IntCurrentPage=1"@en,
        rdfs:label "derived heat"
    
    EquivalentTo: 
        OEO_00000132
    
    SubClassOf: 
        OEO_00000207
    
    
Class: OEO_00000131

    Annotations: 
        <http://purl.obolibrary.org/obo/IAO_0000115> "Diesel fuel is gas diesel oil used on-road for diesel compression ignition (cars, trucks, etc.), usually of low sulphur content."@en,
        <http://purl.obolibrary.org/obo/IAO_0000118> "TransportDiesel"@en,
        <http://purl.obolibrary.org/obo/IAO_0000119> "REGULATION (EC) No 1099/2008 OF THE EUROPEAN PARLIAMENT AND OF THE COUNCIL of 22 October 2008 on energy statistics https://eur-lex.europa.eu/legal-content/EN/TXT/HTML/?uri=CELEX:32008R1099&from=EN"@en,
        rdfs:label "diesel fuel",
        rdfs:label "diesel fuel"@en
    
    SubClassOf: 
        OEO_00000181
    
    
Class: OEO_00000132

    Annotations: 
        <http://purl.obolibrary.org/obo/IAO_0000115> "District heating (also known as heat networks or teleheating) is a system for distributing heat generated in a centralized location through a system of insulated pipes for residential and commercial heating requirements such as space heating and water heating. The heat is often obtained from a cogeneration plant burning fossil fuels or biomass, but heat-only boiler stations, geothermal heating, heat pumps and central solar heating are also used, as well as heat waste from nuclear power electricity generation. "@en,
        <http://purl.obolibrary.org/obo/IAO_0000119> "https://en.wikipedia.org/w/index.php?title=District_heating&oldid=906646999"@en,
        rdfs:label "district heat"
    
    EquivalentTo: 
        OEO_00000129
    
    SubClassOf: 
        OEO_00000207
    
    
Class: OEO_00000139

    Annotations: 
        <http://purl.obolibrary.org/obo/IAO_0000115> "Electrical energy is a form of energy derived from the potential or kinetic energy of charged particles."@en,
        <http://purl.obolibrary.org/obo/IAO_0000119> "https://en.wikipedia.org/wiki/Electrical_energy"@en,
        <http://purl.obolibrary.org/obo/IAO_0000233> "issue: https://github.com/OpenEnergyPlatform/ontology/issues/224
pull request:  https://github.com/OpenEnergyPlatform/ontology/pull/524",
        rdfs:label "electrical energy"
    
    SubClassOf: 
        OEO_00000150
    
    
Class: OEO_00000143

    Annotations: 
        <http://purl.obolibrary.org/obo/IAO_0000115> "An electricity grid is a supply grid that distributes electrical energy / electricity."@en,
        <http://purl.obolibrary.org/obo/IAO_0000233> "issue: https://github.com/OpenEnergyPlatform/ontology/issues/138
pull request: https://github.com/OpenEnergyPlatform/ontology/pull/165",
        rdfs:label "electricity grid"
    
    SubClassOf: 
        OEO_00000200,
        <http://purl.obolibrary.org/obo/BFO_0000051> some OEO_00000144,
        <http://purl.obolibrary.org/obo/BFO_0000051> min 1 OEO_00000253
    
    
Class: OEO_00000144

    Annotations: 
        <http://purl.obolibrary.org/obo/IAO_0000115> "An electricity grid component is a grid component that is part of an electricity grid."@en,
        <http://purl.obolibrary.org/obo/IAO_0000233> "issue: https://github.com/OpenEnergyPlatform/ontology/issues/36
pull request: https://github.com/OpenEnergyPlatform/ontology/pull/385",
        rdfs:label "electricity grid component"
    
    EquivalentTo: 
        OEO_00020006
         and (<http://purl.obolibrary.org/obo/BFO_0000050> some OEO_00000143)
    
    SubClassOf: 
        OEO_00020006
    
    
Class: OEO_00000146

    Annotations: 
        <http://purl.obolibrary.org/obo/IAO_0000115> "An electric vehicle (abbreviated as EV) is a vehicle that uses one or more electric motors for propulsion."@en,
        <http://purl.obolibrary.org/obo/IAO_0000118> "EV",
        <http://purl.obolibrary.org/obo/IAO_0000233> "https://github.com/OpenEnergyPlatform/ontology/issues/425
pull request: https://github.com/OpenEnergyPlatform/ontology/pull/431",
        rdfs:label "electric vehicle"
    
    SubClassOf: 
        OEO_00010023,
        OEO_00000503 some OEO_00000139,
        <http://purl.obolibrary.org/obo/BFO_0000051> some OEO_00010028
    
    
Class: OEO_00000147

    Annotations: 
        <http://purl.obolibrary.org/obo/IAO_0000115> "emission is a process releasing byproducts from human activity (e.g. production, distribution or consumption) into the environment."@en,
        <http://purl.obolibrary.org/obo/IAO_0000233> "issue: https://github.com/OpenEnergyPlatform/ontology/issues/56
pull request: https://github.com/OpenEnergyPlatform/ontology/pull/234",
        rdfs:label "emission"
    
    SubClassOf: 
        <http://purl.obolibrary.org/obo/BFO_0000015>,
        OEO_00000500 some OEO_00000148
    
    
Class: OEO_00000148

    Annotations: 
        <http://purl.obolibrary.org/obo/IAO_0000115> "An emission factor is a process attribute that quantifies the emissions or removals of a gas per unit activity.",
        <http://purl.obolibrary.org/obo/IAO_0000233> "issue: https://github.com/OpenEnergyPlatform/ontology/issues/243
pull request: https://github.com/OpenEnergyPlatform/ontology/pull/581",
        rdfs:label "emission factor"
    
    SubClassOf: 
        OEO_00030019,
        OEO_00000502 some OEO_00000147,
        OEO_00000502 some <http://purl.obolibrary.org/obo/BFO_0000015>
    
    
Class: OEO_00000150

    Annotations: 
        <http://purl.obolibrary.org/obo/IAO_0000115> "Energy is a quality of matter and radiation which is manifest as a capacity to perform work (such as causing motion or the interaction of molecules)",
        <http://purl.obolibrary.org/obo/IAO_0000119> "Derived from https://www.lexico.com/en/definition/energy",
        <http://purl.obolibrary.org/obo/IAO_0000233> "issue: https://github.com/OpenEnergyPlatform/ontology/issues/224
pull request: https://github.com/OpenEnergyPlatform/ontology/pull/364",
        rdfs:comment "Energy is power integrated over time.",
        rdfs:label "energy"
    
    SubClassOf: 
        <http://purl.obolibrary.org/obo/BFO_0000019>
    
    
Class: OEO_00000151

    Annotations: 
        <http://purl.obolibrary.org/obo/IAO_0000115> "An energy carrier disposition is a disposition of an object or object aggregate that contains energy for conversion as usable energy."@en,
        <http://purl.obolibrary.org/obo/IAO_0000233> "issue: https://github.com/OpenEnergyPlatform/ontology/issues/209
pull request: https://github.com/OpenEnergyPlatform/ontology/pull/276",
        rdfs:label "energy carrier disposition"
    
    SubClassOf: 
        <http://purl.obolibrary.org/obo/BFO_0000016>
    
    
Class: OEO_00000159

    Annotations: 
        <http://purl.obolibrary.org/obo/IAO_0000115> "An energy storage object is an artificial object that has the function energy storage.",
        <http://purl.obolibrary.org/obo/IAO_0000233> "issue: https://github.com/OpenEnergyPlatform/ontology/issues/209
pull request: https://github.com/OpenEnergyPlatform/ontology/pull/276",
        rdfs:label "energy storage object"
    
    SubClassOf: 
        OEO_00000061
    
    
Class: OEO_00000165

    Annotations: 
        <http://purl.obolibrary.org/obo/IAO_0000115> "A field photovoltaic powerplant (also: solar farm, solar park) is a photovoltaic powerplant that is installed out in the open on the ground."@en,
        <http://purl.obolibrary.org/obo/IAO_0000118> "Solar park",
        rdfs:label "field photovoltaic powerplant"
    
    SubClassOf: 
        OEO_00000324
    
    DisjointWith: 
        OEO_00000361
    
    
Class: OEO_00000169

    Annotations: 
        <http://purl.obolibrary.org/obo/IAO_0000115> "A flow battery, or redox flow battery (after reductionâoxidation), is a type of electrochemical cell where chemical energy is provided by two chemical components dissolved in liquids contained within the system and separated by a membrane. Ion exchange (accompanied by flow of electric current) occurs through the membrane while both liquids circulate in their own respective space."@en,
        <http://purl.obolibrary.org/obo/IAO_0000119> "https://en.wikipedia.org/w/index.php?title=Flow_battery&oldid=907053515"@en,
        rdfs:label "flow battery"
    
    SubClassOf: 
        OEO_00000068
    
    
Class: OEO_00000173

    Annotations: 
        <http://purl.obolibrary.org/obo/IAO_0000115> "A fuel is a portion of matter that has the disposition to be an energy carrier and which has a fuel role that is realised in processes that release the carried energy by transforming the portion of matter into a different kind of portion of matter in a way that releases heat or does work.",
        <http://purl.obolibrary.org/obo/IAO_0000233> "issue: https://github.com/OpenEnergyPlatform/ontology/issues/227
pull request: https://github.com/OpenEnergyPlatform/ontology/pull/279",
        rdfs:label "fuel"
    
    EquivalentTo: 
        (<http://purl.obolibrary.org/obo/RO_0000087> some OEO_00000001)
         and (<http://purl.obolibrary.org/obo/RO_0000091> some OEO_00000151)
    
    SubClassOf: 
        OEO_00000331
    
    
Class: OEO_00000174

    Annotations: 
        <http://purl.obolibrary.org/obo/IAO_0000115> "A fueled powerplant is a powerplant that has fueled power units as parts.",
        <http://purl.obolibrary.org/obo/IAO_0000233> "issue: https://github.com/OpenEnergyPlatform/ontology/issues/292
pull request: https://github.com/OpenEnergyPlatform/ontology/pull/306",
        rdfs:label "fueled powerplant"
    
    EquivalentTo: 
        <http://purl.obolibrary.org/obo/BFO_0000051> some OEO_00000175
    
    SubClassOf: 
        OEO_00000031,
        <http://purl.obolibrary.org/obo/RO_0000056> some OEO_00050001
    
    
Class: OEO_00000175

    Annotations: 
        <http://purl.obolibrary.org/obo/IAO_0000115> "A fueled power unit is a power generating unit that uses fuel.",
        <http://purl.obolibrary.org/obo/IAO_0000233> "issue: https://github.com/OpenEnergyPlatform/ontology/issues/292
pull request: https://github.com/OpenEnergyPlatform/ontology/pull/306",
        rdfs:label "fueled power unit"
    
    EquivalentTo: 
        OEO_00000334
         and (OEO_00000503 some OEO_00000173)
    
    SubClassOf: 
        OEO_00000334,
        <http://purl.obolibrary.org/obo/RO_0000056> some OEO_00050001
    
    
Class: OEO_00000181

    Annotations: 
        <http://purl.obolibrary.org/obo/IAO_0000115> "Gas/diesel oil is an oil and petroleum product that is primarily a medium distillate distilling between 180 Â°C and 380 Â°C. Includes blending components. Several grades are available depending on uses."@en,
        <http://purl.obolibrary.org/obo/IAO_0000119> "REGULATION (EC) No 1099/2008 OF THE EUROPEAN PARLIAMENT AND OF THE COUNCIL of 22 October 2008 on energy statistics https://eur-lex.europa.eu/legal-content/EN/TXT/HTML/?uri=CELEX:32008R1099&from=EN"@en,
        rdfs:label "gas diesel oil"
    
    SubClassOf: 
        OEO_00000309,
        OEO_00000529 value OEO_00000256
    
    
Class: OEO_00000183

    Annotations: 
        <http://purl.obolibrary.org/obo/IAO_0000115> "Gasoline (American English) or petrol (British English) is an oil and petroleum product in the form of a transparent petroleum-derived liquid that is used primarily as a fuel in spark-ignited internal combustion engines. It consists mostly of organic compounds obtained by the fractional distillation of petroleum, enhanced with a variety of additives.",
        <http://purl.obolibrary.org/obo/IAO_0000115> "https://en.wikipedia.org/w/index.php?title=Gasoline&oldid=867948640",
        <http://purl.obolibrary.org/obo/IAO_0000118> "petrol",
        rdfs:label "gasoline"
    
    SubClassOf: 
        OEO_00000309,
        OEO_00000529 value OEO_00000256
    
    
Class: OEO_00000184

    Annotations: 
        <http://purl.obolibrary.org/obo/IAO_0000115> "A gas powerplant is a powerplant having an aggregate of gas fired power units as its power generating units."@en,
        rdfs:label "gas powerplant"
    
    SubClassOf: 
        OEO_00000031,
        <http://purl.obolibrary.org/obo/BFO_0000051> some OEO_00000017
    
    
Class: OEO_00000185

    Annotations: 
        <http://purl.obolibrary.org/obo/IAO_0000115> "A gas turbine is a turbine that converts chemical energy into rotational energy using a continous internal combustion process. Hence it is also called combustion turbine."@en,
        <http://purl.obolibrary.org/obo/IAO_0000118> "Combustion turbine",
        <http://purl.obolibrary.org/obo/IAO_0000233> "issue: https://github.com/OpenEnergyPlatform/ontology/issues/299
pull request: https://github.com/OpenEnergyPlatform/ontology/pull/300",
        rdfs:label "gas turbine"
    
    SubClassOf: 
        OEO_00000425,
        OEO_00000533 some OEO_00000333,
        OEO_00000532 only OEO_00000292
    
    
Class: OEO_00000186

    Annotations: 
        <http://purl.obolibrary.org/obo/IAO_0000115> "Gasworks gas is manufactured coal based gas that covers all types of gases produced in public utility or private plants, whose main purpose is manufacture, transport and distribution of gas. It includes gas produced by carbonisation (including gas produced by coke ovens and transferred to gasworks gas), by total gasification with or without enrichment with oil products (LPG, residual fuel oil, etc.), and by reforming and simple mixing of gases and/or air, reported under the rows âfrom other sourcesâ. Under the transformation sector identify amounts of gasworks gas transferred to blended natural gas which will be distributed and consumed through the natural gas grid.

The production of other coal gases (i.e. coke oven gas, blast furnace gas and oxygen steel furnace gas) should be reported in the columns concerning such gases, and not as production of gasworks gas. The coal gases transferred to gasworks plants should then be reported (in their own column) in the transformation sector in the gasworks plants row. The total amount of gasworks gas resulting from transfers of other coal gases should appear in the production line for gasworks gas."@en,
        <http://purl.obolibrary.org/obo/IAO_0000119> "REGULATION (EC) No 1099/2008 OF THE EUROPEAN PARLIAMENT AND OF THE COUNCIL of 22 October 2008 on energy statistics https://eur-lex.europa.eu/legal-content/EN/TXT/HTML/?uri=CELEX:32008R1099&from=EN"@en,
        rdfs:label "gasworks gas"
    
    SubClassOf: 
        OEO_00000263
    
    
Class: OEO_00000188

    Annotations: 
        <http://purl.obolibrary.org/obo/IAO_0000115> "A generator is an energy converting device that converts other forms of energy into electrical energy."@en,
        <http://purl.obolibrary.org/obo/IAO_0000233> "issue: https://github.com/OpenEnergyPlatform/ontology/issues/173
pull request: https://github.com/OpenEnergyPlatform/ontology/pull/273",
        rdfs:label "generator"
    
    SubClassOf: 
        OEO_00000011,
        OEO_00000533 some OEO_00000139
    
    
Class: OEO_00000189

    Annotations: 
        rdfs:label "geographic coordinate"
    
    SubClassOf: 
        <http://purl.obolibrary.org/obo/BFO_0000141>
    
    
Class: OEO_00000191

    Annotations: 
        <http://purl.obolibrary.org/obo/IAO_0000115> "Energy available as heat emitted from within the earth's crust, usually in the form of hot water or steam. This energy production is the difference between the enthalpy of the fluid produced in the production borehole and that of the fluid eventually disposed of. It is exploited at suitable sites:
â for electricity generation using dry steam or high enthalpy brine after flashing,
â directly as heat for district heating, agriculture etc"@en,
        <http://purl.obolibrary.org/obo/IAO_0000119> "REGULATION (EC) No 1099/2008 OF THE EUROPEAN PARLIAMENT AND OF THE COUNCIL of 22 October 2008 on energy statistics https://eur-lex.europa.eu/legal-content/EN/TXT/HTML/?uri=CELEX:32008R1099&from=EN"@en,
        rdfs:label "geothermal heat"
    
    SubClassOf: 
        OEO_00000207,
        <http://purl.obolibrary.org/obo/RO_0000091> some OEO_00000033
    
    
Class: OEO_00000192

    Annotations: 
        <http://purl.obolibrary.org/obo/IAO_0000115> "A geothermal powerplant is a powerplant having an aggregate of geothermal power units as its power generating units."@en,
        rdfs:label "geothermal powerplant"
    
    SubClassOf: 
        OEO_00000031,
        <http://purl.obolibrary.org/obo/BFO_0000051> some OEO_00000019,
        <http://purl.obolibrary.org/obo/BFO_0000051> some OEO_00000396
    
    
Class: OEO_00000198

    Annotations: 
        <http://purl.obolibrary.org/obo/IAO_0000115> "The greenhouse effect disposition is the disposition of a gas to contribute to the greenhouse effect, when it is emitted into the atmosphere.",
        <http://purl.obolibrary.org/obo/IAO_0000233> "issue: https://github.com/OpenEnergyPlatform/ontology/issues/56
pull request: https://github.com/OpenEnergyPlatform/ontology/pull/234",
        rdfs:label "greenhouse effect disposition"
    
    SubClassOf: 
        <http://purl.obolibrary.org/obo/BFO_0000016>
    
    
Class: OEO_00000199

    Annotations: 
        <http://purl.obolibrary.org/obo/IAO_0000115> "A greenhouse gas emission is an emission that releases a greenhouse gas.",
        <http://purl.obolibrary.org/obo/IAO_0000233> "issue: https://github.com/OpenEnergyPlatform/ontology/issues/406
pull request: https://github.com/OpenEnergyPlatform/ontology/pull/410
issue: https://github.com/OpenEnergyPlatform/ontology/issues/56
pull request: https://github.com/OpenEnergyPlatform/ontology/pull/234",
        rdfs:label "greenhouse gas emission"
    
    SubClassOf: 
        OEO_00000147,
        <http://purl.obolibrary.org/obo/RO_0000057> some OEO_00000020
    
    
Class: OEO_00000200

    Annotations: 
        <http://purl.obolibrary.org/obo/IAO_0000115> "A supply grid is an object aggregate of systematically connected artificial objects that can work as a supply system.",
        <http://purl.obolibrary.org/obo/IAO_0000118> "grid",
        <http://purl.obolibrary.org/obo/IAO_0000118> "network",
        <http://purl.obolibrary.org/obo/IAO_0000233> "issue: https://github.com/OpenEnergyPlatform/ontology/issues/36
pull request: https://github.com/OpenEnergyPlatform/ontology/pull/385

issue: https://github.com/OpenEnergyPlatform/ontology/issues/114
pull request: https://github.com/OpenEnergyPlatform/ontology/pull/137",
        rdfs:label "supply grid"
    
    SubClassOf: 
        <http://purl.obolibrary.org/obo/BFO_0000027>
    
    
Class: OEO_00000204

    Annotations: 
        <http://purl.obolibrary.org/obo/IAO_0000115> "Hard coal is coal with a gross calorific value greater than 23 865 kJ/kg (5 700 kcal/kg) on an ashfree but moist basis and with a mean random reflectance of vitrinite of at least 0,6."@en,
        <http://purl.obolibrary.org/obo/IAO_0000119> "REGULATION (EC) No 1099/2008 OF THE EUROPEAN PARLIAMENT AND OF THE COUNCIL of 22 October 2008 on energy statistics https://eur-lex.europa.eu/legal-content/EN/TXT/HTML/?uri=CELEX:32008R1099&from=EN"@en,
        rdfs:label "hard coal"
    
    SubClassOf: 
        OEO_00000088
    
    DisjointWith: 
        OEO_00000251
    
    
Class: OEO_00000205

    Annotations: 
        <http://purl.obolibrary.org/obo/IAO_0000115> "A hard coal powerplant is a coal powerplant having an aggregate of hard coal power units as its power generating units."@en,
        rdfs:label "hard coal powerplant"
    
    SubClassOf: 
        OEO_00000089,
        <http://purl.obolibrary.org/obo/BFO_0000051> some OEO_00000021
    
    
Class: OEO_00000206

    Annotations: 
        <http://purl.obolibrary.org/obo/IAO_0000115> "Hardware is an artificial object that is part of an electronic system.",
        <http://purl.obolibrary.org/obo/IAO_0000233> "issue: https://github.com/OpenEnergyPlatform/ontology/issues/319
pull request: https://github.com/OpenEnergyPlatform/ontology/pull/350",
        rdfs:label "hardware"
    
    SubClassOf: 
        OEO_00000061
    
    
Class: OEO_00000207

    Annotations: 
        <http://purl.obolibrary.org/obo/IAO_0000115> "Thermal energy is the energy that a material entity contains in the undirected motion of its constituent parts (e.g. molecules and atoms)."@en,
        <http://purl.obolibrary.org/obo/IAO_0000233> "issue: https://github.com/OpenEnergyPlatform/ontology/issues/522
pull request: https://github.com/OpenEnergyPlatform/ontology/pull/609"@en,
        rdfs:label "thermal energy"@en
    
    SubClassOf: 
        OEO_00000150
    
    
Class: OEO_00000210

    Annotations: 
        <http://purl.obolibrary.org/obo/IAO_0000115> "A heater is an energy converting device that converts other forms of energy into useful heat.",
        <http://purl.obolibrary.org/obo/IAO_0000233> "issue: https://github.com/OpenEnergyPlatform/ontology/issues/173
pull request: https://github.com/OpenEnergyPlatform/ontology/pull/273",
        rdfs:label "heater"
    
    SubClassOf: 
        OEO_00000011,
        OEO_00000533 some OEO_00000207
    
    
Class: OEO_00000211

    Annotations: 
        <http://purl.obolibrary.org/obo/IAO_0000115> "Heating oil is gas diesel oil for industrial and commercial uses, marine diesel and diesel used in rail traffic, other gas oil, including heavy gas oils which distil between 380 Â°C and 540 Â°C and which are used as petrochemical feedstocks."@en,
        <http://purl.obolibrary.org/obo/IAO_0000118> "OtherGasOil"@en,
        <http://purl.obolibrary.org/obo/IAO_0000119> "REGULATION (EC) No 1099/2008 OF THE EUROPEAN PARLIAMENT AND OF THE COUNCIL of 22 October 2008 on energy statistics https://eur-lex.europa.eu/legal-content/EN/TXT/HTML/?uri=CELEX:32008R1099&from=EN"@en,
        rdfs:label "heating oil",
        rdfs:label "heating oil"@en
    
    SubClassOf: 
        OEO_00000181
    
    
Class: OEO_00000212

    Annotations: 
        <http://purl.obolibrary.org/obo/IAO_0000115> "A heat pump is a heater that transforms low temperature heat to high temperature heat using external energy."@en,
        rdfs:label "heat pump"
    
    SubClassOf: 
        OEO_00000210
    
    
Class: OEO_00000216

    Annotations: 
        <http://purl.obolibrary.org/obo/IAO_0000115> "Potential and kinetic energy of water converted into electricity in hydroelectric plants.",
        <http://purl.obolibrary.org/obo/IAO_0000119> "REGULATION (EC) No 1099/2008 OF THE EUROPEAN PARLIAMENT AND OF THE COUNCIL of 22 October 2008 on energy statistics https://eur-lex.europa.eu/legal-content/EN/TXT/HTML/?uri=CELEX:32008R1099&from=EN",
        rdfs:label "hydroelectricity"
    
    SubClassOf: 
        OEO_00000218
    
    
Class: OEO_00000218

    Annotations: 
        <http://purl.obolibrary.org/obo/IAO_0000115> "Hydropower or water power [...] is power derived from the energy of falling water or fast running water, which may be harnessed for useful purposes."@en,
        <http://purl.obolibrary.org/obo/IAO_0000119> "https://en.wikipedia.org/w/index.php?title=Hydropower&oldid=906980683"@en,
        <http://purl.obolibrary.org/obo/IAO_0000233> "issue: https://github.com/OpenEnergyPlatform/ontology/issues/211
pull request: https://github.com/OpenEnergyPlatform/ontology/pull/225",
        rdfs:label "hydro energy"
    
    SubClassOf: 
        OEO_00000150
    
    
Class: OEO_00000219

    Annotations: 
        <http://purl.obolibrary.org/obo/IAO_0000115> "Hydrofluorocarbons (HFCs) are portions of matter consisting of organic compounds that contain fluorine and hydrogen atoms, and are the most common type of organofluorine compounds. They are frequently used in air conditioning and as refrigerants in place of the older chlorofluorocarbons such as R-12 and hydrochlorofluorocarbons such as R-21."@en,
        <http://purl.obolibrary.org/obo/IAO_0000118> "HFC",
        <http://purl.obolibrary.org/obo/IAO_0000119> "https://en.wikipedia.org/w/index.php?title=Hydrofluorocarbon&oldid=904556263"@en,
        rdfs:label "hydrofluorocarbon"
    
    SubClassOf: 
        OEO_00000331,
        OEO_00000530 some OEO_00030000
    
    
Class: OEO_00000220

    Annotations: 
        <http://purl.obolibrary.org/obo/IAO_0000115> "Hydrogen is a portion of matter with the chemical formular H2. It has a gaseous normal state of matter. As it can be oxidised it can be used as a fuel."@en,
        <http://purl.obolibrary.org/obo/IAO_0000118> "H2",
        <http://purl.obolibrary.org/obo/IAO_0000233> "issue: https://github.com/OpenEnergyPlatform/ontology/issues/134",
        rdfs:label "hydrogen"
    
    SubClassOf: 
        OEO_00000331,
        <http://purl.obolibrary.org/obo/RO_0000087> some OEO_00000001,
        <http://purl.obolibrary.org/obo/RO_0000091> some OEO_00000097,
        OEO_00000529 value OEO_00000182
    
    
Class: OEO_00000221

    Annotations: 
        <http://purl.obolibrary.org/obo/IAO_0000115> "A hydrogen powerplant is a powerplant having an aggregate of hydrogen power units as its power generating units."@en,
        rdfs:label "hydrogen powerplant"
    
    SubClassOf: 
        OEO_00000031,
        <http://purl.obolibrary.org/obo/BFO_0000051> some OEO_00000022,
        <http://purl.obolibrary.org/obo/BFO_0000051> some OEO_00000222
    
    
Class: OEO_00000222

    Annotations: 
        <http://purl.obolibrary.org/obo/IAO_0000115> "A hydrogen turbine is a gas turbine fueled with hydrogen."@en,
        <http://purl.obolibrary.org/obo/IAO_0000233> "issue: https://github.com/OpenEnergyPlatform/ontology/issues/299
pull request: https://github.com/OpenEnergyPlatform/ontology/pull/300",
        rdfs:label "hydrogen turbine"
    
    SubClassOf: 
        OEO_00000185,
        OEO_00000533 some OEO_00000333,
        OEO_00000532 only OEO_00000220
    
    
Class: OEO_00000226

    Annotations: 
        <http://purl.obolibrary.org/obo/IAO_0000115> "Industrial waste fuel is waste fuel of industrial non-renewable origin (solids or liquids) combusted directly for the production of electricity and/or heat. The quantity of fuel used should be reported on a net calorific value basis. Renewable industrial waste should be reported in the solid biomass, biogas and/or liquid biofuels categories."@en,
        <http://purl.obolibrary.org/obo/IAO_0000119> "REGULATION (EC) No 1099/2008 OF THE EUROPEAN PARLIAMENT AND OF THE COUNCIL of 22 October 2008 on energy statistics https://eur-lex.europa.eu/legal-content/EN/TXT/HTML/?uri=CELEX:32008R1099&from=EN"@en,
        rdfs:label "industrial waste fuel"
    
    SubClassOf: 
        OEO_00000439
    
    
Class: OEO_00000240

    Annotations: 
        <http://purl.obolibrary.org/obo/IAO_0000115> "An internal combustion vehicle is a vehicle powered by an internal combustion engine.",
        <http://purl.obolibrary.org/obo/IAO_0000233> "issue: https://github.com/OpenEnergyPlatform/ontology/issues/425
pull request: https://github.com/OpenEnergyPlatform/ontology/pull/431",
        rdfs:label "internal combustion vehicle"
    
    SubClassOf: 
        OEO_00010023,
        OEO_00000503 some OEO_00000099,
        <http://purl.obolibrary.org/obo/BFO_0000051> some OEO_00010029
    
    
Class: OEO_00000245

    Annotations: 
        <http://purl.obolibrary.org/obo/IAO_0000115> "Jet fuel is kerosene used for aviation turbine power units. It has the same distillation characteristics between 150 Â°C and 300 Â°C (generally not above 250 Â°C) and flash point as kerosene. In addition, it has particular specifications (such as freezing point) which are established by the International air Transport Association (IATA)."@en,
        <http://purl.obolibrary.org/obo/IAO_0000119> "REGULATION (EC) No 1099/2008 OF THE EUROPEAN PARLIAMENT AND OF THE COUNCIL of 22 October 2008 on energy statistics https://eur-lex.europa.eu/legal-content/EN/TXT/HTML/?uri=CELEX:32008R1099&from=EN"@en,
        rdfs:label "KeroseneTypeJetFuel"@en,
        rdfs:label "jet fuel"
    
    SubClassOf: 
        OEO_00000246
    
    
Class: OEO_00000246

    Annotations: 
        <http://purl.obolibrary.org/obo/IAO_0000115> "Kerosene, also known as paraffin, lamp oil, and coal oil (an obsolete term), is an oil and petroleum product consisting of combustible hydrocarbon liquid which is derived from petroleum. It is widely used as a fuel in industry as well as households. It is sometimes spelled kerosine in scientific and industrial usage.
[...]

Kerosene is widely used to power jet engines of aircraft (jet fuel) and some rocket engines and is also commonly used as a cooking and lighting fuel and for fire toys such as poi. In parts of Asia, kerosene is sometimes used as fuel for small outboard motors or even motorcycles.",
        <http://purl.obolibrary.org/obo/IAO_0000119> "https://en.wikipedia.org/w/index.php?title=Kerosene&oldid=867958484",
        rdfs:label "kerosene"
    
    SubClassOf: 
        OEO_00000309,
        OEO_00000529 value OEO_00000256
    
    
Class: OEO_00000248

    Annotations: 
        <http://purl.obolibrary.org/obo/IAO_0000115> "A lithium-ion battery or Li-ion battery (abbreviated as LIB) is a type of rechargeable battery [...] In the batteries lithium ions move from the negative electrode to the positive electrode during discharge and back when charging. Li-ion batteries use an intercalated lithium compound as one electrode material, compared to the metallic lithium used in a non-rechargeable lithium battery. "@en,
        <http://purl.obolibrary.org/obo/IAO_0000119> "https://en.wikipedia.org/w/index.php?title=Lithium-ion_battery&oldid=906786251"@en,
        rdfs:label "lithium-ion battery"
    
    SubClassOf: 
        OEO_00000068
    
    
Class: OEO_00000251

    Annotations: 
        <http://purl.obolibrary.org/obo/IAO_0000115> "Lignite is coal that is non-agglomerating with a gross calorific value less than 17 435 kJ/kg (4 165 kcal/kg) and greater than 31 % volatile matter on a dry mineral matter free basis.	

Oil shale and tar sands produced and combusted directly should be reported in this category. Oil shale and tar sands used as inputs for other transformation processes should also be reported in this category.	

This includes the portion of the oil shale or tar sands consumed in the transformation process."@en,
        <http://purl.obolibrary.org/obo/IAO_0000119> "REGULATION (EC) No 1099/2008 OF THE EUROPEAN PARLIAMENT AND OF THE COUNCIL of 22 October 2008 on energy statistics https://eur-lex.europa.eu/legal-content/EN/TXT/HTML/?uri=CELEX:32008R1099&from=EN"@en,
        rdfs:label "lignite"
    
    SubClassOf: 
        OEO_00000088,
        OEO_00000530 some OEO_00030002,
        OEO_00000529 value OEO_00000390
    
    DisjointWith: 
        OEO_00000204
    
    
Class: OEO_00000252

    Annotations: 
        <http://purl.obolibrary.org/obo/IAO_0000115> "A lignite powerplant is a coal powerplant having an aggregate of lignite power units as its power generating units."@en,
        rdfs:label "lignite powerplant"
    
    SubClassOf: 
        OEO_00000089,
        <http://purl.obolibrary.org/obo/BFO_0000051> some OEO_00000024
    
    
Class: OEO_00000253

    Annotations: 
        <http://purl.obolibrary.org/obo/IAO_0000115> "A powerline is a grid component that is an uninterrupted transmission system between two nodes in an electricity grid."@en,
        <http://purl.obolibrary.org/obo/IAO_0000233> "issue: https://github.com/OpenEnergyPlatform/ontology/issues/231
pull request: https://github.com/OpenEnergyPlatform/ontology/pull/385",
        rdfs:label "power line"@en
    
    SubClassOf: 
        OEO_00000255,
        <http://purl.obolibrary.org/obo/BFO_0000050> some OEO_00000143
    
    
Class: OEO_00000255

    Annotations: 
        <http://purl.obolibrary.org/obo/IAO_0000115> "A grid component link is a grid component that serves as a connection between two other grid components."@en,
        <http://purl.obolibrary.org/obo/IAO_0000233> "issue: https://github.com/OpenEnergyPlatform/ontology/issues/36
pull request: https://github.com/OpenEnergyPlatform/ontology/pull/385"@en,
        rdfs:label "grid component link"
    
    SubClassOf: 
        OEO_00020006
    
    DisjointWith: 
        OEO_00000296
    
    
Class: OEO_00000257

    Annotations: 
        <http://purl.obolibrary.org/obo/IAO_0000115> "Liquid air is air that has been compressed and cooled to store energy until it condenses as a liquid. To discharge energy, the air is expanded."@en,
        rdfs:label "liquid air"
    
    SubClassOf: 
        OEO_00000054
    
    
Class: OEO_00000258

    Annotations: 
        <http://purl.obolibrary.org/obo/IAO_0000115> "A liquid biofuel is a biofuel that has liquid as its normal state of matter.",
        rdfs:label "liquid biofuel"
    
    EquivalentTo: 
        OEO_00000072
         and (OEO_00000529 value OEO_00000256)
    
    SubClassOf: 
        OEO_00000530 some OEO_00030001,
        OEO_00000530 some OEO_00030004,
        OEO_00000529 value OEO_00000256
    
    
Class: OEO_00000259

    Annotations: 
        <http://purl.obolibrary.org/obo/IAO_0000115> "Rechargeable liquid-metal batteries are used for electric vehicles and potentially also for grid energy storage, to balance out intermittent renewable power sources such as solar panels and wind turbines."@en,
        <http://purl.obolibrary.org/obo/IAO_0000119> "https://en.wikipedia.org/w/index.php?title=Molten-salt_battery&oldid=900557096"@en,
        rdfs:label "liquid-metal battery"
    
    SubClassOf: 
        OEO_00000283
    
    
Class: OEO_00000263

    Annotations: 
        <http://purl.obolibrary.org/obo/IAO_0000115> "A manufactured coal based gas is a portion of matter that is gaseous and manufactured from coal. It is used as fossil fuel."@en,
        rdfs:label "manufactured coal based gas"
    
    SubClassOf: 
        OEO_00000331,
        OEO_00000530 some OEO_00030002,
        <http://purl.obolibrary.org/obo/RO_0000087> some OEO_00000001,
        <http://purl.obolibrary.org/obo/RO_0000091> some OEO_00000097,
        OEO_00000529 value OEO_00000182
    
    
Class: OEO_00000269

    Annotations: 
        <http://purl.obolibrary.org/obo/IAO_0000115> "A methanation gas storage is a energy storage that uses carbon dioxide and hydrogen from electrolysis to produce methan and store this. The methan can then be used to produce electricity or heat in a gas generator."@en,
        rdfs:label "methanation gas storage"
    
    SubClassOf: 
        OEO_00000012
    
    DisjointWith: 
        OEO_00000070
    
    
Class: OEO_00000282

    Annotations: 
        <http://purl.obolibrary.org/obo/IAO_0000115> "Molten-salt batteries are a class of battery that uses molten salts as an electrolyte and offers both a high energy density and a high power density."@en,
        <http://purl.obolibrary.org/obo/IAO_0000119> "https://en.wikipedia.org/w/index.php?title=Molten-salt_battery&oldid=900557096"@en,
        rdfs:label "molten-salt battery"
    
    SubClassOf: 
        OEO_00000283
    
    
Class: OEO_00000283

    Annotations: 
        <http://purl.obolibrary.org/obo/IAO_0000115> "Molten-state batteries consist of two molten metal alloys separated by an electrolyte."@en,
        <http://purl.obolibrary.org/obo/IAO_0000115> "Wastes produced by households, hospitals and the tertiary sector incinerated at specific installations, on a net calorific value basis."@en,
        <http://purl.obolibrary.org/obo/IAO_0000119> "REGULATION (EC) No 1099/2008 OF THE EUROPEAN PARLIAMENT AND OF THE COUNCIL of 22 October 2008 on energy statistics https://eur-lex.europa.eu/legal-content/EN/TXT/HTML/?uri=CELEX:32008R1099&from=EN"@en,
        rdfs:label "molten state battery"
    
    SubClassOf: 
        OEO_00000068
    
    
Class: OEO_00000286

    Annotations: 
        <http://purl.obolibrary.org/obo/IAO_0000115> "Motor gasoline is gasoline consisting of a mixture of light hydrocarbons distilling between 35 oC and 215 oC. It is used as a fuel for land based spark ignition engines. Motor gasoline may include additives, oxygenates and octane enhancers, including lead compounds such as TEL and TML.

Includes motor gasoline blending components (excluding additives/oxygenates), e.g. alkylates, isomerate, reformate, cracked gasoline destined for use as finished motor gasoline."@en,
        <http://purl.obolibrary.org/obo/IAO_0000119> "REGULATION (EC) No 1099/2008 OF THE EUROPEAN PARLIAMENT AND OF THE COUNCIL of 22 October 2008 on energy statistics https://eur-lex.europa.eu/legal-content/EN/TXT/HTML/?uri=CELEX:32008R1099&from=EN"@en,
        rdfs:label "motor gasoline"
    
    SubClassOf: 
        OEO_00000183
    
    
Class: OEO_00000290

    Annotations: 
        <http://purl.obolibrary.org/obo/IAO_0000115> "Municipal waste fuel is waste fuel of waste produced by households, hospitals and the tertiary sector incinerated at specific installations, on a net calorific value basis."@en,
        <http://purl.obolibrary.org/obo/IAO_0000119> "REGULATION (EC) No 1099/2008 OF THE EUROPEAN PARLIAMENT AND OF THE COUNCIL of 22 October 2008 on energy statistics https://eur-lex.europa.eu/legal-content/EN/TXT/HTML/?uri=CELEX:32008R1099&from=EN"@en,
        rdfs:label "municipal waste fuel"
    
    SubClassOf: 
        OEO_00000439
    
    
Class: OEO_00000292

    Annotations: 
        <http://purl.obolibrary.org/obo/IAO_0000115> "Natural gas is a portion of matter which comprises gases occurring in underground deposits, whether liquefied or gaseous, consisting mainly of methane.

It includes both ânon-associatedâ gas originating from fields producing hydrocarbons only in gaseous form, and âassociatedâ gas produced in association with crude oil as well as methane recovered from coal mines (colliery gas) or from coal seams (coal seam gas).

It does not include gases created by anaerobic digestion of biomass (e.g. municipal or sewage gas) nor gasworks gas."@en,
        <http://purl.obolibrary.org/obo/IAO_0000119> "REGULATION (EC) No 1099/2008 OF THE EUROPEAN PARLIAMENT AND OF THE COUNCIL of 22 October 2008 on energy statistics https://eur-lex.europa.eu/legal-content/EN/TXT/HTML/?uri=CELEX:32008R1099&from=EN"@en,
        <http://purl.obolibrary.org/obo/IAO_0000233> "issue: https://github.com/OpenEnergyPlatform/ontology/issues/430
pull request: https://github.com/OpenEnergyPlatform/ontology/pull/431",
        rdfs:label "natural gas"
    
    SubClassOf: 
        OEO_00000331,
        OEO_00000530 some OEO_00030002,
        <http://purl.obolibrary.org/obo/BFO_0000051> some OEO_00000025,
        <http://purl.obolibrary.org/obo/RO_0000087> some OEO_00000001,
        <http://purl.obolibrary.org/obo/RO_0000091> some OEO_00000097,
        OEO_00000529 value OEO_00000182
    
    
Class: OEO_00000293

    Annotations: 
        <http://purl.obolibrary.org/obo/IAO_0000115> "Negative emission is the process of absorbing a substance, usually a pollutant that was emitted before.",
        <http://purl.obolibrary.org/obo/IAO_0000233> "issue: https://github.com/OpenEnergyPlatform/ontology/issues/56
pull request: https://github.com/OpenEnergyPlatform/ontology/pull/234",
        rdfs:label "negative emission"
    
    SubClassOf: 
        <http://purl.obolibrary.org/obo/BFO_0000015>
    
    
Class: OEO_00000296

    Annotations: 
        <http://purl.obolibrary.org/obo/IAO_0000115> "A grid node is a grid component of a supply grid where two or more links meet."@en,
        <http://purl.obolibrary.org/obo/IAO_0000233> "issue: https://github.com/OpenEnergyPlatform/ontology/issues/36
pull request: https://github.com/OpenEnergyPlatform/ontology/pull/385"@en,
        rdfs:label "grid node"
    
    SubClassOf: 
        OEO_00020006
    
    DisjointWith: 
        OEO_00000255
    
    
Class: OEO_00000297

    Annotations: 
        <http://purl.obolibrary.org/obo/IAO_0000115> "Non associated gas is natural gas originating from fields producing hydrocarbons only in gaseous form.",
        <http://purl.obolibrary.org/obo/IAO_0000119> "REGULATION (EC) No 1099/2008 OF THE EUROPEAN PARLIAMENT AND OF THE COUNCIL of 22 October 2008 on energy statistics https://eur-lex.europa.eu/legal-content/EN/TXT/HTML/?uri=CELEX:32008R1099&from=EN",
        rdfs:label "non associated gas"
    
    SubClassOf: 
        OEO_00000292
    
    
Class: OEO_00000298

    Annotations: 
        <http://purl.obolibrary.org/obo/IAO_0000115> "A non-methane volatile organic compound (NMVOC) is a volatile organic compound other than methane."@en,
        <http://purl.obolibrary.org/obo/IAO_0000118> "NMVOC",
        <http://purl.obolibrary.org/obo/IAO_0000119> "This definition is partly based on Article 2 of the European Air Quality Directive (2008/50/EC): https://eur-lex.europa.eu/legal-content/EN/TXT/?uri=CELEX:32008L0050",
        <http://purl.obolibrary.org/obo/IAO_0000233> "issue: https://github.com/OpenEnergyPlatform/ontology/issues/263
pull request: https://github.com/OpenEnergyPlatform/ontology/pull/356",
        rdfs:label "non-methane volatile organic compound"
    
    SubClassOf: 
        OEO_00000437
    
    
Class: OEO_00000299

    Annotations: 
        <http://purl.obolibrary.org/obo/IAO_0000115> "Non renewable municipal waste fuel is municipal waste fuel of non-biological origin."@en,
        <http://purl.obolibrary.org/obo/IAO_0000119> "REGULATION (EC) No 1099/2008 OF THE EUROPEAN PARLIAMENT AND OF THE COUNCIL of 22 October 2008 on energy statistics https://eur-lex.europa.eu/legal-content/EN/TXT/HTML/?uri=CELEX:32008R1099&from=EN"@en,
        rdfs:label "non renewable municipal waste fuel"
    
    SubClassOf: 
        OEO_00000290,
        OEO_00000530 some OEO_00030002
    
    
Class: OEO_00000300

    Annotations: 
        <http://purl.obolibrary.org/obo/IAO_0000115> "Nuclear energy is the use of nuclear reactions that release nuclear energy to generate heat, which most frequently is then used in steam turbines to produce electricity in a nuclear power plant. Nuclear power can be obtained from nuclear fission, nuclear decay and nuclear fusion. Presently, the vast majority of electricity from nuclear power is produced by nuclear fission of elements in the actinide series of the periodic table. Nuclear decay processes are used in niche applications such as radioisotope thermoelectric generators. The possibility of generating electricity from nuclear fusion is still at a research phase with no commercial applications. This article mostly deals with nuclear fission power for electricity generation."@en,
        <http://purl.obolibrary.org/obo/IAO_0000119> "https://en.wikipedia.org/w/index.php?title=Nuclear_power&oldid=868476098"@en,
        <http://purl.obolibrary.org/obo/IAO_0000233> "issue: https://github.com/OpenEnergyPlatform/ontology/issues/211
pull request: https://github.com/OpenEnergyPlatform/ontology/pull/225",
        rdfs:label "nuclear energy"
    
    SubClassOf: 
        OEO_00000150
    
    
Class: OEO_00000302

    Annotations: 
        <http://purl.obolibrary.org/obo/IAO_0000115> "A nuclear fuel is a fuel that realizes its fuel role in processes that release energy in the form of heat or work by undergoing nuclear fission.",
        <http://purl.obolibrary.org/obo/IAO_0000233> "issue: https://github.com/OpenEnergyPlatform/ontology/issues/182
pull request: https://github.com/OpenEnergyPlatform/ontology/pull/237",
        rdfs:label "nuclear fuel"
    
    EquivalentTo: 
        OEO_00000173
         and (<http://purl.obolibrary.org/obo/RO_0000091> some OEO_00000028)
    
    SubClassOf: 
        OEO_00000173
    
    
Class: OEO_00000303

    Annotations: 
        <http://purl.obolibrary.org/obo/IAO_0000115> "A nuclear powerplant is a powerplant having an aggregate of nuclear power units as its power generating units.",
        rdfs:label "nuclear powerplant"
    
    SubClassOf: 
        OEO_00000031,
        <http://purl.obolibrary.org/obo/BFO_0000051> some OEO_00000029,
        <http://purl.obolibrary.org/obo/BFO_0000051> some OEO_00000396
    
    
Class: OEO_00000308

    Annotations: 
        <http://purl.obolibrary.org/obo/IAO_0000115> "An offshore wind farm is a wind farm that is build in a body of water, usually the ocean."@en,
        rdfs:label "offshore wind farm"
    
    SubClassOf: 
        OEO_00000447
    
    DisjointWith: 
        OEO_00000311
    
    
Class: OEO_00000309

    Annotations: 
        <http://purl.obolibrary.org/obo/IAO_0000115> "Petroleum (/pÉËtroÊliÉm/) is a naturally occurring, yellowish-black liquid found in geological formations beneath the Earth's surface. It is commonly refined into various types of fuels. Components of petroleum are separated using a technique called fractional distillation, i.e. separation of a liquid mixture into fractions differing in boiling point by means of distillation, typically using a fractionating column.

It consists of hydrocarbons of various molecular weights and other organic compounds. The name petroleum covers both naturally occurring unprocessed crude oil and petroleum products that are made up of refined crude oil. A fossil fuel, petroleum is formed when large quantities of dead organisms, mostly zooplankton and algae, are buried underneath sedimentary rock and subjected to both intense heat and pressure."@en,
        <http://purl.obolibrary.org/obo/IAO_0000119> "https://en.wikipedia.org/w/index.php?title=Petroleum&oldid=868006507"@en,
        rdfs:label "oil and petroleum products"
    
    SubClassOf: 
        OEO_00000331,
        OEO_00000530 some OEO_00030002,
        <http://purl.obolibrary.org/obo/RO_0000087> some OEO_00000001,
        <http://purl.obolibrary.org/obo/RO_0000091> some OEO_00000097
    
    
Class: OEO_00000310

    Annotations: 
        <http://purl.obolibrary.org/obo/IAO_0000115> "An oil powerplant is a powerplant having an aggregate of oil power units as its power generating units.",
        rdfs:label "oil powerplant"
    
    SubClassOf: 
        OEO_00000031,
        <http://purl.obolibrary.org/obo/BFO_0000051> some OEO_00000030,
        <http://purl.obolibrary.org/obo/BFO_0000051> some OEO_00000396
    
    
Class: OEO_00000311

    Annotations: 
        <http://purl.obolibrary.org/obo/IAO_0000115> "An onshore wind farm is a wind farm that is build on land."@en,
        rdfs:label "onshore wind farm"
    
    SubClassOf: 
        OEO_00000447
    
    DisjointWith: 
        OEO_00000308
    
    
Class: OEO_00000316

    Annotations: 
        <http://purl.obolibrary.org/obo/IAO_0000115> "The origin is a quality that indicates where something comes from (its source).",
        <http://purl.obolibrary.org/obo/IAO_0000233> "issue: https://github.com/OpenEnergyPlatform/ontology/issues/108
pull request: https://github.com/OpenEnergyPlatform/ontology/pull/130",
        rdfs:label "origin"
    
    SubClassOf: 
        <http://purl.obolibrary.org/obo/BFO_0000019>
    
    
Class: OEO_00000318

    Annotations: 
        <http://purl.obolibrary.org/obo/IAO_0000115> "Particulate matter is a portion of matter consisting of small particles. It can act as an air pollutant."@en,
        <http://purl.obolibrary.org/obo/IAO_0000118> "PM",
        <http://purl.obolibrary.org/obo/IAO_0000233> "issue: https://github.com/OpenEnergyPlatform/ontology/issues/263
pull request: https://github.com/OpenEnergyPlatform/ontology/pull/356",
        rdfs:label "particulate matter"
    
    SubClassOf: 
        OEO_00000331,
        (OEO_00000529 value OEO_00000256) or (OEO_00000529 value OEO_00000390),
        <http://purl.obolibrary.org/obo/RO_0000056> some OEO_00000055
    
    
Class: OEO_00000320

    Annotations: 
        <http://purl.obolibrary.org/obo/IAO_0000115> "Peat is a portion of matter consisting of combustible soft, porous or compressed, sedimentary deposit of plant origin with high water content (up to 90 % in the raw state), easily cut, of light to dark brown colour. Peat used for non-energy purposes is not included.

This definition is without prejudice to the definition of renewable energy sources in Directive 2001/77/EC and to the 2006 IPCC Guidelines for National Greenhouse Gas Inventories."@en,
        <http://purl.obolibrary.org/obo/IAO_0000119> "REGULATION (EC) No 1099/2008 OF THE EUROPEAN PARLIAMENT AND OF THE COUNCIL of 22 October 2008 on energy statistics https://eur-lex.europa.eu/legal-content/EN/TXT/HTML/?uri=CELEX:32008R1099&from=EN"@en,
        rdfs:label "peat"
    
    SubClassOf: 
        OEO_00000331,
        OEO_00000530 some OEO_00030002,
        <http://purl.obolibrary.org/obo/RO_0000087> some OEO_00000001,
        <http://purl.obolibrary.org/obo/RO_0000091> some OEO_00000097,
        OEO_00000529 value OEO_00000390
    
    
Class: OEO_00000322

    Annotations: 
        <http://purl.obolibrary.org/obo/IAO_0000115> "Perfluorocarbons (PFCs) are portions of matter consisting of organic compounds that contain fluorine atoms but no hydrogen atoms.",
        <http://purl.obolibrary.org/obo/IAO_0000118> "PFC",
        rdfs:label "perfluorocarbon"
    
    SubClassOf: 
        OEO_00000331,
        OEO_00000530 some OEO_00030000
    
    
Class: OEO_00000324

    Annotations: 
        <http://purl.obolibrary.org/obo/IAO_0000115> "A photovoltaic powerplant is a powerplant having an aggregate of PV panels as its power generating units."@en,
        rdfs:label "photovoltaic powerplant"
    
    SubClassOf: 
        OEO_00000386,
        <http://purl.obolibrary.org/obo/BFO_0000051> some OEO_00000348
    
    
Class: OEO_00000330

    Annotations: 
        <http://purl.obolibrary.org/obo/IAO_0000115> "Pollution is an emission with a negative effect on the environment or organisms."@en,
        <http://purl.obolibrary.org/obo/IAO_0000233> "issue: https://github.com/OpenEnergyPlatform/ontology/issues/56
pull request: https://github.com/OpenEnergyPlatform/ontology/pull/234",
        rdfs:label "pollution"
    
    SubClassOf: 
        OEO_00000147
    
    
Class: OEO_00000331

    Annotations: 
        <http://purl.obolibrary.org/obo/IAO_0000115> "A portion of matter is a part of a material entity that has a state_of_matter property."@en,
        <http://purl.obolibrary.org/obo/IAO_0000233> "issue: https://github.com/OpenEnergyPlatform/ontology/issues/227
pull request: https://github.com/OpenEnergyPlatform/ontology/pull/279",
        rdfs:comment "wiki page: https://github.com/OpenEnergyPlatform/ontology/wiki/Explanation-on-mass-nouns",
        rdfs:label "portion of matter"
    
    SubClassOf: 
        <http://purl.obolibrary.org/obo/BFO_0000027>
    
    
Class: OEO_00000332

    Annotations: 
        <http://purl.obolibrary.org/obo/IAO_0000115> "Solid biomass is a portion of matter consisting of organic, non-fossil material of biological origin which may be used as fuel for heat production or electricity generation.",
        <http://purl.obolibrary.org/obo/IAO_0000118> "portion of solid biomass",
        <http://purl.obolibrary.org/obo/IAO_0000118> "solid biomass"@en,
        <http://purl.obolibrary.org/obo/IAO_0000119> "https://eur-lex.europa.eu/legal-content/EN/TXT/HTML/?uri=CELEX:32008R1099&from=EN",
        rdfs:label "solid biofuel"@en
    
    EquivalentTo: 
        OEO_00000072
         and (OEO_00000529 value OEO_00000390)
    
    SubClassOf: 
        OEO_00000530 some OEO_00030001,
        OEO_00000530 some OEO_00030004,
        <http://purl.obolibrary.org/obo/RO_0000087> some OEO_00000001,
        <http://purl.obolibrary.org/obo/RO_0000091> some OEO_00000097,
        OEO_00000529 value OEO_00000390
    
    
Class: OEO_00000333

    Annotations: 
        <http://purl.obolibrary.org/obo/IAO_0000115> "Power is the process attribute that is the amount of energy transformed or transferred per time unit."@en,
        <http://purl.obolibrary.org/obo/IAO_0000233> "classification:
issue: https://github.com/OpenEnergyPlatform/ontology/issues/205
pull request: https://github.com/OpenEnergyPlatform/ontology/pull/386

definition:
issue: https://github.com/OpenEnergyPlatform/ontology/issues/79
pull request: https://github.com/OpenEnergyPlatform/ontology/pull/369",
        rdfs:comment "Power is the derivative of energy transformation over time",
        rdfs:label "power"
    
    SubClassOf: 
        OEO_00030019,
        OEO_00000502 some OEO_00020003
    
    
Class: OEO_00000334

    Annotations: 
        <http://purl.obolibrary.org/obo/IAO_0000115> "A power generating unit is an artificial object that contains a generator, among other parts.",
        <http://purl.obolibrary.org/obo/IAO_0000233> "issue: https://github.com/OpenEnergyPlatform/ontology/issues/173
pull request: https://github.com/OpenEnergyPlatform/ontology/pull/273",
        rdfs:label "power generating unit"
    
    SubClassOf: 
        OEO_00000061,
        <http://purl.obolibrary.org/obo/BFO_0000051> some OEO_00000188
    
    
Class: OEO_00000335

    Annotations: 
        <http://purl.obolibrary.org/obo/IAO_0000115> "a power-to-gas (often abbreviated P2G) system is an energy storage object that converts electrical power to a gas fuel. When using surplus power from wind generation, the concept is sometimes called windgas. There are currently three methods in use; all use electricity to split water into hydrogen and oxygen by means of electrolysis."@en,
        <http://purl.obolibrary.org/obo/IAO_0000118> "P2G",
        <http://purl.obolibrary.org/obo/IAO_0000118> "PtG",
        <http://purl.obolibrary.org/obo/IAO_0000119> "https://en.wikipedia.org/w/index.php?title=Power-to-gas&oldid=907220452"@en,
        rdfs:label "power-to-gas system"
    
    SubClassOf: 
        OEO_00000159
    
    
Class: OEO_00000343

    Annotations: 
        <http://purl.obolibrary.org/obo/IAO_0000115> "A pumped storage (pumped-storage hdyroelectricity) is an energy storage that uses water from a higher reservoir to generate energy."@en,
        rdfs:label "pumped storage"
    
    SubClassOf: 
        OEO_00000012
    
    
Class: OEO_00000345

    Annotations: 
        <http://purl.obolibrary.org/obo/IAO_0000115> "Pumped water is water which was pumped into an upper reservoir and thus contains potential energy."@en,
        rdfs:label "pumped water"
    
    SubClassOf: 
        OEO_00000441,
        OEO_00000501 some OEO_00000399
    
    
Class: OEO_00000348

    Annotations: 
        <http://purl.obolibrary.org/obo/IAO_0000115> "A PV panel (photovoltaic panel) is a solar power unit absorbing sunlight as a source of energy to generate electricity."@en,
        rdfs:comment "A photovoltaic (PV) module is a packaged, connected assembly of typically 6x10 photovoltaic solar cells. Photovoltaic modules constitute the photovoltaic array of a photovoltaic system that generates and supplies solar electricity in commercial and residential applications.",
        rdfs:label "PV panel"
    
    SubClassOf: 
        OEO_00000034,
        OEO_00000533 some OEO_00000333,
        <http://purl.obolibrary.org/obo/BFO_0000051> some OEO_00000032
    
    
Class: OEO_00000350

    
Class: OEO_00000356

    Annotations: 
        <http://purl.obolibrary.org/obo/IAO_0000115> "Renewable municipal waste fuel is municipal waste fuel of biological origin."@en,
        <http://purl.obolibrary.org/obo/IAO_0000119> "REGULATION (EC) No 1099/2008 OF THE EUROPEAN PARLIAMENT AND OF THE COUNCIL of 22 October 2008 on energy statistics https://eur-lex.europa.eu/legal-content/EN/TXT/HTML/?uri=CELEX:32008R1099&from=EN"@en,
        rdfs:label "renewable municipal waste fuel"
    
    SubClassOf: 
        OEO_00000290,
        OEO_00000530 some OEO_00030001,
        OEO_00000530 some OEO_00030004
    
    
Class: OEO_00000361

    Annotations: 
        <http://purl.obolibrary.org/obo/IAO_0000115> "A rooftop photovoltaic powerplant is a photovoltaic powerplant that is installed on top of the roof of a building."@en,
        rdfs:label "rooftop photovoltaic powerplant"
    
    SubClassOf: 
        OEO_00000324
    
    DisjointWith: 
        OEO_00000165
    
    
Class: OEO_00000374

    Annotations: 
        <http://purl.obolibrary.org/obo/IAO_0000115> "Superconducting magnetic energy storage (SMES) systems store energy in the magnetic field created by the flow of direct current in a superconducting coil which has been cryogenically cooled to a temperature below its superconducting critical temperature.
          A typical smes system includes three parts: superconducting coil, power conditioning system and cryogenically cooled refrigerator. Once the superconducting coil is charged, the current will not decay and the magnetic energy can be stored indefinitely."@en,
        <http://purl.obolibrary.org/obo/IAO_0000119> "https://en.wikipedia.org/w/index.php?title=Superconducting_magnetic_energy_storage&oldid=902190687",
        rdfs:label "SMES"
    
    SubClassOf: 
        OEO_00000159
    
    
Class: OEO_00000376

    Annotations: 
        <http://purl.obolibrary.org/obo/IAO_0000115> "Sodium-ion batteries (SIB) are a type of rechargeable metal-ion battery that uses sodium ions as charge carriers."@en,
        <http://purl.obolibrary.org/obo/IAO_0000119> "https://en.wikipedia.org/w/index.php?title=Sodium-ion_battery&oldid=906459441"@en,
        rdfs:label "sodium-ion battery"
    
    SubClassOf: 
        OEO_00000068
    
    
Class: OEO_00000377

    Annotations: 
        <http://purl.obolibrary.org/obo/IAO_0000115> "A sodiumâsulfur battery is a type of molten-salt battery constructed from liquid sodium (Na) and sulfur (S).This type of battery has a high energy density, high efficiency of charge/discharge and long cycle life, and is fabricated from inexpensive materials. The operating temperatures of 300 to 350 Â°C and the highly corrosive nature of the sodium polysulfides, primarily make them suitable for stationary energy storage applications. The cell becomes more economical with increasing size."@en,
        <http://purl.obolibrary.org/obo/IAO_0000119> "https://en.wikipedia.org/w/index.php?title=Sodium%E2%80%93sulfur_battery&oldid=900392594"@en,
        rdfs:label "sodium-sulfur battery"
    
    SubClassOf: 
        OEO_00000283
    
    
Class: OEO_00000384

    Annotations: 
        <http://purl.obolibrary.org/obo/IAO_0000115> "Solar radiation exploited for hot water production and electricity generation. This energy production is the heat available to the heat transfer medium, i.e. the incident solar energy less the optical and collectors' losses. Passive solar energy for the direct heating, cooling and lighting of dwellings or other buildings is not included."@en,
        <http://purl.obolibrary.org/obo/IAO_0000119> "REGULATION (EC) No 1099/2008 OF THE EUROPEAN PARLIAMENT AND OF THE COUNCIL of 22 October 2008 on energy statistics https://eur-lex.europa.eu/legal-content/EN/TXT/HTML/?uri=CELEX:32008R1099&from=EN"@en,
        <http://purl.obolibrary.org/obo/IAO_0000233> "issue: https://github.com/OpenEnergyPlatform/ontology/issues/211
pull request: https://github.com/OpenEnergyPlatform/ontology/pull/225",
        rdfs:label "solar energy"
    
    SubClassOf: 
        OEO_00000150,
        <http://purl.obolibrary.org/obo/RO_0000091> some OEO_00000033
    
    
Class: OEO_00000386

    Annotations: 
        <http://purl.obolibrary.org/obo/IAO_0000115> "A solar powerplant is a powerplant having an aggregate of solar power units as its power generating units."@en,
        rdfs:label "solar power plant"
    
    SubClassOf: 
        OEO_00000031,
        <http://purl.obolibrary.org/obo/BFO_0000051> some OEO_00000348
    
    
Class: OEO_00000387

    Annotations: 
        <http://purl.obolibrary.org/obo/IAO_0000115> "A solar thermal collector is a heater that absorbs solar radiation to convert it into heat."@en,
        <http://purl.obolibrary.org/obo/IAO_0000119> "https://en.wikipedia.org/w/index.php?title=Solar_thermal_collector&oldid=903948846"@en,
        rdfs:label "solar thermal collector"
    
    SubClassOf: 
        OEO_00000210,
        OEO_00000532 only OEO_00000388
    
    
Class: OEO_00000388

    Annotations: 
        <http://purl.obolibrary.org/obo/IAO_0000115> "Heat from solar radiation; can consist of:
(a) solar thermal-electric plants; or
(b) equipment for the production of domestic hot water or for the seasonal heating of swimming pools (e.g. flat plate collectors, mainly of the thermosyphon type)."@en,
        <http://purl.obolibrary.org/obo/IAO_0000119> "REGULATION (EC) No 1099/2008 OF THE EUROPEAN PARLIAMENT AND OF THE COUNCIL of 22 October 2008 on energy statistics https://eur-lex.europa.eu/legal-content/EN/TXT/HTML/?uri=CELEX:32008R1099&from=EN"@en,
        rdfs:label "solar thermal heat"
    
    SubClassOf: 
        OEO_00000207
    
    
Class: OEO_00000389

    Annotations: 
        <http://purl.obolibrary.org/obo/IAO_0000115> "A solar thermal powerplant is a powerplant consisting of solar thermal power units."@en,
        rdfs:label "solar thermal powerplant"
    
    SubClassOf: 
        OEO_00000386,
        <http://purl.obolibrary.org/obo/BFO_0000051> some OEO_00000035,
        <http://purl.obolibrary.org/obo/BFO_0000051> some OEO_00000396
    
    
Class: OEO_00000391

    Annotations: 
        <http://purl.obolibrary.org/obo/IAO_0000115> "Solid fossil fuels are fuels of fossil origin and that have a solid state of matter under normal conditions.",
        <http://purl.obolibrary.org/obo/IAO_0000233> "issue: https://github.com/OpenEnergyPlatform/ontology/issues/106
pull request: https://github.com/OpenEnergyPlatform/ontology/pull/164",
        rdfs:label "solid fossil fuel"
    
    EquivalentTo: 
        (OEO_00000530 some OEO_00030002)
         and (<http://purl.obolibrary.org/obo/RO_0000091> some OEO_00000097)
         and (OEO_00000529 value OEO_00000390)
    
    SubClassOf: 
        OEO_00000173,
        OEO_00000530 some OEO_00030002,
        OEO_00000529 value OEO_00000390
    
    
Class: OEO_00000395

    Annotations: 
        <http://purl.obolibrary.org/obo/IAO_0000115> "In physics, a state of matter is one of the distinct forms in which matter can exist. Four states of matter are observable in everyday life: solid, liquid, gas, and plasma. Many intermediate states are known to exist, such as liquid crystal, and some states only exist under extreme conditions",
        <http://purl.obolibrary.org/obo/IAO_0000119> "https://en.wikipedia.org/w/index.php?title=State_of_matter&oldid=903680856",
        <http://purl.obolibrary.org/obo/IAO_0000233> "issue: https://github.com/OpenEnergyPlatform/ontology/issues/38
pull request: https://github.com/OpenEnergyPlatform/ontology/pull/39",
        rdfs:label "state of matter"
    
    SubClassOf: 
        <http://purl.obolibrary.org/obo/BFO_0000019>
    
    
Class: OEO_00000396

    Annotations: 
        <http://purl.obolibrary.org/obo/IAO_0000115> "A steam turbine is a turbine that converts heat from pressurized steam into rotational energy.",
        rdfs:label "steam turbine"
    
    SubClassOf: 
        OEO_00000425,
        OEO_00000533 some OEO_00000333
    
    
Class: OEO_00000399

    Annotations: 
        <http://purl.obolibrary.org/obo/IAO_0000115> "A storage unit is a grid component that stores energy."@en,
        rdfs:label "storage unit"
    
    SubClassOf: 
        OEO_00020006,
        <http://purl.obolibrary.org/obo/BFO_0000050> some OEO_00000200
    
    
Class: OEO_00000401

    Annotations: 
        <http://purl.obolibrary.org/obo/IAO_0000115> "Sub bituminous coal is coal that is non-agglomerating with a gross calorific value between 17 435 kJ/kg (4 165 kcal/kg) and 23 865 kJ/kg (5 700 kcal/kg) containing more than 31 % volatile matter on a dry mineral matter free basis."@en,
        <http://purl.obolibrary.org/obo/IAO_0000119> "REGULATION (EC) No 1099/2008 OF THE EUROPEAN PARLIAMENT AND OF THE COUNCIL of 22 October 2008 on energy statistics https://eur-lex.europa.eu/legal-content/EN/TXT/HTML/?uri=CELEX:32008R1099&from=EN"@en,
        rdfs:label "sub bituminous coal"
    
    SubClassOf: 
        OEO_00000088
    
    
Class: OEO_00000407

    Annotations: 
        <http://purl.obolibrary.org/obo/IAO_0000115> "A Technology is an information content entity that specifies how to create an artificial object."@en,
        <http://purl.obolibrary.org/obo/IAO_0000233> "issue: https://github.com/OpenEnergyPlatform/ontology/issues/136
pull request: https://github.com/OpenEnergyPlatform/ontology/pull/334",
        rdfs:label "technology"
    
    SubClassOf: 
        <http://purl.obolibrary.org/obo/IAO_0000030>
    
    
Class: OEO_00000419

    
Class: OEO_00000420

    Annotations: 
        <http://purl.obolibrary.org/obo/IAO_0000115> "A transformer is an electricity grid component that passively transfers electrical energy from one electrical circuit to another."@en,
        <http://purl.obolibrary.org/obo/IAO_0000233> "issue: https://github.com/OpenEnergyPlatform/ontology/issues/231
pull request: https://github.com/OpenEnergyPlatform/ontology/pull/385"@en,
        rdfs:comment "Source: https://en.wikipedia.org/wiki/Transformer"@en,
        rdfs:label "transformer"
    
    SubClassOf: 
        OEO_00020006,
        <http://purl.obolibrary.org/obo/BFO_0000050> some OEO_00000143
    
    
Class: OEO_00000425

    Annotations: 
        <http://purl.obolibrary.org/obo/IAO_0000115> "A turbine is an energy converting device that converts energy from a moving fluid flow into rotational energy."@en,
        rdfs:label "turbine"
    
    SubClassOf: 
        OEO_00000011
    
    
Class: OEO_00000429

    Annotations: 
        <http://purl.obolibrary.org/obo/IAO_0000115> "An underground hydrogen storage is an energy storage object that stores hydrogen underground. Examples are underground caverns, salt domes and depleted oil/gas fields."@en,
        <http://purl.obolibrary.org/obo/IAO_0000119> "https://en.wikipedia.org/w/index.php?title=Underground_hydrogen_storage&oldid=895350780",
        <http://purl.obolibrary.org/obo/IAO_0000233> "Issue:https://github.com/OpenEnergyPlatform/ontology/issues/448
Pull request: https://github.com/OpenEnergyPlatform/ontology/pull/462",
        rdfs:label "underground hydrogen storage"
    
    SubClassOf: 
        OEO_00000159,
        OEO_00000503 some OEO_00000220
    
    
Class: OEO_00000437

    Annotations: 
        <http://purl.obolibrary.org/obo/IAO_0000115> "A volatile organic compound (VOC) is a portion of matter consisting of organic compounds that is capable of producing photochemical oxidants by reactions with nitrogen oxides in the presence of sunlight. Hence it can act as an air pollutant."@en,
        <http://purl.obolibrary.org/obo/IAO_0000118> "VOC",
        <http://purl.obolibrary.org/obo/IAO_0000119> "This definition is partly based on Article 2 of the European Air Quality Directive (2008/50/EC): https://eur-lex.europa.eu/legal-content/EN/TXT/?uri=CELEX:32008L0050",
        <http://purl.obolibrary.org/obo/IAO_0000233> "issue: https://github.com/OpenEnergyPlatform/ontology/issues/263
pull request: https://github.com/OpenEnergyPlatform/ontology/pull/356",
        rdfs:label "volatile organic compound"
    
    EquivalentTo: 
        OEO_00000025 or OEO_00000298
    
    SubClassOf: 
        OEO_00000331
         and (<http://purl.obolibrary.org/obo/RO_0000091> some OEO_00010011),
        <http://purl.obolibrary.org/obo/RO_0000056> some OEO_00000055
    
    
Class: OEO_00000439

    Annotations: 
        <http://purl.obolibrary.org/obo/IAO_0000115> "A waste fuel is a fuel in which the material entity is waste."@en,
        <http://purl.obolibrary.org/obo/IAO_0000233> "issue: https://github.com/OpenEnergyPlatform/ontology/issues/132
pull request: https://github.com/OpenEnergyPlatform/ontology/pull/207",
        rdfs:comment "The energy content of waste fuel is typically released by incineration or gasification.",
        rdfs:label "waste fuel"
    
    EquivalentTo: 
        OEO_00000173
         and (<http://purl.obolibrary.org/obo/RO_0000087> some OEO_00000042)
    
    SubClassOf: 
        <http://purl.obolibrary.org/obo/RO_0000091> some OEO_00000097
    
    
Class: OEO_00000440

    Annotations: 
        <http://purl.obolibrary.org/obo/IAO_0000115> "A waste powerplant is a powerplant having an aggregate of waste power units as its power generating units."@en,
        rdfs:label "waste powerplant"
    
    SubClassOf: 
        OEO_00000031,
        <http://purl.obolibrary.org/obo/BFO_0000051> some OEO_00000041,
        <http://purl.obolibrary.org/obo/BFO_0000051> some OEO_00000396
    
    
Class: OEO_00000441

    Annotations: 
        <http://purl.obolibrary.org/obo/IAO_0000115> "Water is a portion of matter that is transparent, tasteless, odorless, and nearly colorless, which is the main constituent of Earth's hydrosphere, and the fluids of most living organisms. It is vital for all known forms of life, even though it provides no calories or organic nutrients. Its chemical formula is H2O, meaning that each of its molecules contains one oxygen and two hydrogen atoms, connected by covalent bonds. Water is the name of the liquid state of H2O at standard ambient temperature and pressure.",
        <http://purl.obolibrary.org/obo/IAO_0000119> "https://en.wikipedia.org/wiki/Water",
        rdfs:label "water"
    
    SubClassOf: 
        OEO_00000331,
        <http://purl.obolibrary.org/obo/RO_0000091> some OEO_00000151,
        OEO_00000529 value OEO_00000256
    
    
Class: OEO_00000442

    Annotations: 
        <http://purl.obolibrary.org/obo/IAO_0000115> "A water turbine is a turbine converting kinetic energy and potential energy of water into rotational energy."@en,
        <http://purl.obolibrary.org/obo/IAO_0000233> "issue: https://github.com/OpenEnergyPlatform/ontology/issues/299
pull request: https://github.com/OpenEnergyPlatform/ontology/pull/300",
        rdfs:label "water turbine"
    
    SubClassOf: 
        OEO_00000425,
        OEO_00000533 some OEO_00000333,
        OEO_00000532 only OEO_00000218
    
    
Class: OEO_00000446

    Annotations: 
        <http://purl.obolibrary.org/obo/IAO_0000115> "Kinetic energy of wind exploited for electricity generation in wind turbines."@en,
        <http://purl.obolibrary.org/obo/IAO_0000119> "REGULATION (EC) No 1099/2008 OF THE EUROPEAN PARLIAMENT AND OF THE COUNCIL of 22 October 2008 on energy statistics https://eur-lex.europa.eu/legal-content/EN/TXT/HTML/?uri=CELEX:32008R1099&from=EN",
        <http://purl.obolibrary.org/obo/IAO_0000233> "issue: https://github.com/OpenEnergyPlatform/ontology/issues/211
pull request: https://github.com/OpenEnergyPlatform/ontology/pull/225",
        rdfs:label "wind energy"
    
    SubClassOf: 
        OEO_00000150,
        OEO_00000503 some OEO_00000043,
        <http://purl.obolibrary.org/obo/RO_0000091> some OEO_00000033
    
    
Class: OEO_00000447

    Annotations: 
        <http://purl.obolibrary.org/obo/IAO_0000115> "A wind farm is a powerplant having an aggregate of wind energy converters as its power generating units."@en,
        rdfs:label "wind farm"
    
    SubClassOf: 
        OEO_00000031,
        <http://purl.obolibrary.org/obo/BFO_0000051> some OEO_00000044
    
    
Class: OEO_00000448

    Annotations: 
        <http://purl.obolibrary.org/obo/IAO_0000115> "A wind rotor (or wind turbine) is a turbine that converts the wind's kinetic energy into rotational energy."@en,
        <http://purl.obolibrary.org/obo/IAO_0000118> "wind turbine",
        <http://purl.obolibrary.org/obo/IAO_0000233> "issue: https://github.com/OpenEnergyPlatform/ontology/issues/299
pull request: https://github.com/OpenEnergyPlatform/ontology/pull/300",
        rdfs:label "wind rotor"
    
    SubClassOf: 
        OEO_00000425,
        OEO_00000503 some OEO_00000446,
        OEO_00000533 some OEO_00000333,
        OEO_00000532 only OEO_00000446
    
    
Class: OEO_00000449

    Annotations: 
        <http://purl.obolibrary.org/obo/IAO_0000115> "Wood and other is solid biomass of purpose-grown energy crops (poplar, willow etc.), a multitude of woody materials generated by an industrial process (wood/paper industry in particular) or provided directly by forestry and agriculture (firewood, wood chips, wood pellets, bark, sawdust, shavings, chips, black liquor etc.) as well as wastes such as straw, rice husks, nut shells, poultry litter, crushed grape dregs etc. Combustion is the preferred technology for these solid wastes. The quantity of fuel used should be reported on a net calorific value basis."@en,
        <http://purl.obolibrary.org/obo/IAO_0000119> "REGULATION (EC) No 1099/2008 OF THE EUROPEAN PARLIAMENT AND OF THE COUNCIL of 22 October 2008 on energy statistics https://eur-lex.europa.eu/legal-content/EN/TXT/HTML/?uri=CELEX:32008R1099&from=EN"@en,
        rdfs:label "wood and other"
    
    SubClassOf: 
        OEO_00000332,
        <http://purl.obolibrary.org/obo/RO_0000087> some OEO_00000001
    
    
Class: OEO_00010000

    Annotations: 
        <http://purl.obolibrary.org/obo/IAO_0000115> "Ammonia is a portion of matter with the chemical formula NH3. It has a gaseous normal state of matter and can act as an air pollutant. Synonyms are trihydridonitrogen and nitrogen trihydride.",
        <http://purl.obolibrary.org/obo/IAO_0000118> "NH3",
        <http://purl.obolibrary.org/obo/IAO_0000233> "issue: https://github.com/OpenEnergyPlatform/ontology/issues/263
pull request: https://github.com/OpenEnergyPlatform/ontology/pull/356",
        rdfs:label "ammonia"@en
    
    SubClassOf: 
        OEO_00000331,
        <http://purl.obolibrary.org/obo/RO_0000056> some OEO_00000055,
        OEO_00000529 value OEO_00000182
    
    
Class: OEO_00010001

    Annotations: 
        <http://purl.obolibrary.org/obo/IAO_0000115> "Carbon monoxide is a portion of matter with the chemical formula CO. It has a gaseous normal state of matter and can act as an air pollutant.",
        <http://purl.obolibrary.org/obo/IAO_0000118> "CO",
        <http://purl.obolibrary.org/obo/IAO_0000233> "issue: https://github.com/OpenEnergyPlatform/ontology/issues/263
pull request: https://github.com/OpenEnergyPlatform/ontology/pull/356",
        rdfs:label "carbon monoxide"@en
    
    SubClassOf: 
        OEO_00000331,
        <http://purl.obolibrary.org/obo/RO_0000056> some OEO_00000055,
        OEO_00000529 value OEO_00000182
    
    
Class: OEO_00010002

    Annotations: 
        <http://purl.obolibrary.org/obo/IAO_0000115> "Nitrogen oxides are a portion of matter consisting of compounds of nitrogen and oxygen. It is a collective term for numerous oxides of nitrogen with a gaseous normal state of matter. They can act as air pollutants.",
        <http://purl.obolibrary.org/obo/IAO_0000118> "NOx",
        <http://purl.obolibrary.org/obo/IAO_0000233> "issue: https://github.com/OpenEnergyPlatform/ontology/issues/263
pull request: https://github.com/OpenEnergyPlatform/ontology/pull/356",
        rdfs:label "nitrogen oxides"@en
    
    SubClassOf: 
        OEO_00000331,
        <http://purl.obolibrary.org/obo/RO_0000056> some OEO_00000055,
        OEO_00000529 value OEO_00000182
    
    
Class: OEO_00010003

    Annotations: 
        <http://purl.obolibrary.org/obo/IAO_0000115> "Nitric oxide is a portion of matter with the chemical formula NO. It is a gas and can act as an air pollutant. Synonyms are nitrogen oxide or nitrogen monoxide.",
        <http://purl.obolibrary.org/obo/IAO_0000118> "NO",
        <http://purl.obolibrary.org/obo/IAO_0000118> "nitrogen monoxide",
        <http://purl.obolibrary.org/obo/IAO_0000118> "nitrogen oxide",
        <http://purl.obolibrary.org/obo/IAO_0000233> "issue: https://github.com/OpenEnergyPlatform/ontology/issues/263
pull request: https://github.com/OpenEnergyPlatform/ontology/pull/356",
        rdfs:label "nitric oxide"@en
    
    SubClassOf: 
        OEO_00010002
    
    
Class: OEO_00010004

    Annotations: 
        <http://purl.obolibrary.org/obo/IAO_0000115> "Nitrogen dioxide is a portion of matter with the chemical formula NO2. It is a gas and can act as an air pollutant.",
        <http://purl.obolibrary.org/obo/IAO_0000118> "NO2",
        <http://purl.obolibrary.org/obo/IAO_0000233> "issue: https://github.com/OpenEnergyPlatform/ontology/issues/263
pull request: https://github.com/OpenEnergyPlatform/ontology/pull/356",
        rdfs:label "nitrogen dioxide"@en
    
    SubClassOf: 
        OEO_00010002
    
    
Class: OEO_00010007

    Annotations: 
        <http://purl.obolibrary.org/obo/IAO_0000115> "Sulphur dioxide is a portion of matter with the chemical formula SO2. It has a gaseous normal state of matter and can act as an air pollutant.",
        <http://purl.obolibrary.org/obo/IAO_0000118> "SO2",
        <http://purl.obolibrary.org/obo/IAO_0000233> "issue: https://github.com/OpenEnergyPlatform/ontology/issues/263
pull request: https://github.com/OpenEnergyPlatform/ontology/pull/356",
        rdfs:label "sulphur dioxide"@en
    
    SubClassOf: 
        OEO_00000331,
        <http://purl.obolibrary.org/obo/RO_0000056> some OEO_00000055,
        OEO_00000529 value OEO_00000182
    
    
Class: OEO_00010009

    Annotations: 
        <http://purl.obolibrary.org/obo/IAO_0000115> "PM10 is particulate matter which passes through a size-selective inlet as defined in the reference method for the sampling and measurement of PM10, EN 12341, with a 50 % efficiency cut-off at 10 Âµm aerodynamic diameter.",
        <http://purl.obolibrary.org/obo/IAO_0000119> "This definition is partly based on Article 2 of the European Air Quality Directive (2008/50/EC): https://eur-lex.europa.eu/legal-content/EN/TXT/?uri=CELEX:32008L0050",
        <http://purl.obolibrary.org/obo/IAO_0000233> "issue: https://github.com/OpenEnergyPlatform/ontology/issues/263
pull request: https://github.com/OpenEnergyPlatform/ontology/pull/356",
        rdfs:label "PM10"@en
    
    SubClassOf: 
        OEO_00000318
    
    
Class: OEO_00010010

    Annotations: 
        <http://purl.obolibrary.org/obo/IAO_0000115> "PM2.5 is particulate matter which passes through a size-selective inlet as defined in the reference method for the sampling and measurement of PM2,5, EN 14907, with a 50 % efficiency cut-off at 2,5 Âµm aerodynamic diameter.",
        <http://purl.obolibrary.org/obo/IAO_0000119> "This definition is partly based on Article 2 of the European Air Quality Directive (2008/50/EC): https://eur-lex.europa.eu/legal-content/EN/TXT/?uri=CELEX:32008L0050",
        <http://purl.obolibrary.org/obo/IAO_0000233> "issue: https://github.com/OpenEnergyPlatform/ontology/issues/263
pull request: https://github.com/OpenEnergyPlatform/ontology/pull/356",
        rdfs:label "PM2.5"@en
    
    SubClassOf: 
        OEO_00000318
    
    
Class: OEO_00010011

    Annotations: 
        <http://purl.obolibrary.org/obo/IAO_0000115> "The volatility disposition is the disposition of a portion of matter to sublimate or evaporate from the solid or liquid form and enter the surrounding air.",
        <http://purl.obolibrary.org/obo/IAO_0000233> "issue: https://github.com/OpenEnergyPlatform/ontology/issues/263
pull request: https://github.com/OpenEnergyPlatform/ontology/pull/356",
        rdfs:label "volatility"@en
    
    SubClassOf: 
        <http://purl.obolibrary.org/obo/BFO_0000016>
    
    
Class: OEO_00010012

    Annotations: 
        <http://purl.obolibrary.org/obo/IAO_0000115> "An air pollutant is a portion of matter that has the disposition to participates in air pollution.",
        <http://purl.obolibrary.org/obo/IAO_0000233> "issue: https://github.com/OpenEnergyPlatform/ontology/issues/263
pull request: https://github.com/OpenEnergyPlatform/ontology/pull/356",
        rdfs:label "air pollutant"@en
    
    EquivalentTo: 
        OEO_00000331
         and (<http://purl.obolibrary.org/obo/RO_0000056> some OEO_00000055)
    
    SubClassOf: 
        OEO_00000331
    
    
Class: OEO_00010015

    Annotations: 
        <http://purl.obolibrary.org/obo/IAO_0000115> "Fossil hydrogen is hydrogen with fossil origin. It is usually produced from fossil fuels applying the steam reforming process.",
        <http://purl.obolibrary.org/obo/IAO_0000233> "issue: https://github.com/OpenEnergyPlatform/ontology/issues/134
pull request: https://github.com/OpenEnergyPlatform/ontology/pull/411",
        rdfs:label "fossil hydrogen"@de
    
    SubClassOf: 
        OEO_00000220,
        OEO_00000530 some OEO_00030002
    
    
Class: OEO_00010016

    Annotations: 
        <http://purl.obolibrary.org/obo/IAO_0000115> "Synthetic hydrogen is hydrogen with synthetic origin. It is usually produced from water applying the water electrolysis process.",
        <http://purl.obolibrary.org/obo/IAO_0000233> "issue: https://github.com/OpenEnergyPlatform/ontology/issues/134
pull request: https://github.com/OpenEnergyPlatform/ontology/pull/411",
        rdfs:label "synthetic hydrogen"@de
    
    SubClassOf: 
        OEO_00000220,
        OEO_00000530 some OEO_00030005
    
    
Class: OEO_00010017

    Annotations: 
        <http://purl.obolibrary.org/obo/IAO_0000115> "A synthetic fuel is a fuel produced from one or more portion(s) of matter using electric energy.",
        <http://purl.obolibrary.org/obo/IAO_0000118> "e-fuel",
        <http://purl.obolibrary.org/obo/IAO_0000118> "electric fuel",
        <http://purl.obolibrary.org/obo/IAO_0000233> "issue: https://github.com/OpenEnergyPlatform/ontology/issues/134
pull request: https://github.com/OpenEnergyPlatform/ontology/pull/411",
        rdfs:label "synthetic fuel"@de
    
    EquivalentTo: 
        OEO_00000173
         and (OEO_00000530 some OEO_00030005)
    
    SubClassOf: 
        <http://purl.obolibrary.org/obo/RO_0000091> some OEO_00000097
    
    
Class: OEO_00010018

    Annotations: 
        <http://purl.obolibrary.org/obo/IAO_0000115> "Synthetic methane is synthetic fuel produced in a power-to-gas system from water and carbon dioxide using electric energy.",
        <http://purl.obolibrary.org/obo/IAO_0000233> "issue: https://github.com/OpenEnergyPlatform/ontology/issues/134
pull request: https://github.com/OpenEnergyPlatform/ontology/pull/411",
        rdfs:label "synthetic methane"@de
    
    SubClassOf: 
        OEO_00000025,
        OEO_00000530 some OEO_00030005
    
    
Class: OEO_00010019

    Annotations: 
        <http://purl.obolibrary.org/obo/IAO_0000115> "Synthetic liquid fuel is synthetic fuel produced in a power-to-liquid system from water and carbon dioxide using electric energy applying.",
        <http://purl.obolibrary.org/obo/IAO_0000233> "issue: https://github.com/OpenEnergyPlatform/ontology/issues/134
pull request: https://github.com/OpenEnergyPlatform/ontology/pull/411",
        rdfs:label "synthetic liquid fuel"@de
    
    EquivalentTo: 
        OEO_00010017
         and (OEO_00000529 value OEO_00000256)
    
    SubClassOf: 
        OEO_00010017
    
    
Class: OEO_00010020

    Annotations: 
        <http://purl.obolibrary.org/obo/IAO_0000115> "A power-to-liquid (often abbreviated P2L or PtL) system is an energy storage object that converts electrical power to a liquid fuel.",
        <http://purl.obolibrary.org/obo/IAO_0000118> "P2L",
        <http://purl.obolibrary.org/obo/IAO_0000118> "PtL",
        <http://purl.obolibrary.org/obo/IAO_0000233> "issue: https://github.com/OpenEnergyPlatform/ontology/issues/134
pull request: https://github.com/OpenEnergyPlatform/ontology/pull/411",
        rdfs:label "power-to-liquid system"
    
    SubClassOf: 
        OEO_00000159
    
    
Class: OEO_00010021

    Annotations: 
        <http://purl.obolibrary.org/obo/IAO_0000115> "A water electrolyser is an energy converting device that uses an electric current to decompose water into hydrogen and oxygen gas. Electric energy is converted into chemical energy (and waste heat).",
        <http://purl.obolibrary.org/obo/IAO_0000233> "issue: https://github.com/OpenEnergyPlatform/ontology/issues/134
pull request: https://github.com/OpenEnergyPlatform/ontology/pull/411",
        rdfs:label "water electrolyser"
    
    SubClassOf: 
        OEO_00000011
    
    
Class: OEO_00010022

    Annotations: 
        <http://purl.obolibrary.org/obo/IAO_0000115> "A steam reformer is an energy converting device that produces syngas from hydrocarbons such as natural gas.",
        <http://purl.obolibrary.org/obo/IAO_0000233> "issue: https://github.com/OpenEnergyPlatform/ontology/issues/134
pull request: https://github.com/OpenEnergyPlatform/ontology/pull/411",
        rdfs:label "steam reformer"
    
    SubClassOf: 
        OEO_00000011
    
    
Class: OEO_00010023

    Annotations: 
        <http://purl.obolibrary.org/obo/IAO_0000115> "A vehicle is an artifical object that is used for transporting people or goods.",
        <http://purl.obolibrary.org/obo/IAO_0000233> "issue: https://github.com/OpenEnergyPlatform/ontology/issues/425
pull request: https://github.com/OpenEnergyPlatform/ontology/pull/431",
        rdfs:label "vehicle"@en
    
    SubClassOf: 
        OEO_00000061
    
    
Class: OEO_00010024

    Annotations: 
        <http://purl.obolibrary.org/obo/IAO_0000118> "BEV",
        <http://purl.obolibrary.org/obo/IAO_0000233> "issue: https://github.com/OpenEnergyPlatform/ontology/issues/425
pull request: https://github.com/OpenEnergyPlatform/ontology/pull/453",
        dc:description "A battery electric vehicle (BEV) is a vehicle that stores energy in an on-board battery.",
        rdfs:label "battery electric vehicle"@en
    
    SubClassOf: 
        OEO_00000146,
        <http://purl.obolibrary.org/obo/BFO_0000051> some OEO_00010026
    
    
Class: OEO_00010025

    Annotations: 
        <http://purl.obolibrary.org/obo/IAO_0000118> "FCEV",
        <http://purl.obolibrary.org/obo/IAO_0000233> "issue: https://github.com/OpenEnergyPlatform/ontology/issues/425
pull request: https://github.com/OpenEnergyPlatform/ontology/pull/453",
        dc:description "A fuel cell electric vehicle (FCEV) is a vehicle that uses electrical energy from a fuel cell.",
        rdfs:label "fuel cell electric vehicle"@en
    
    SubClassOf: 
        OEO_00000146,
        OEO_00000503 some OEO_00000220,
        <http://purl.obolibrary.org/obo/BFO_0000051> some OEO_00000016
    
    
Class: OEO_00010026

    Annotations: 
        <http://purl.obolibrary.org/obo/IAO_0000233> "issue: https://github.com/OpenEnergyPlatform/ontology/issues/425
pull request: https://github.com/OpenEnergyPlatform/ontology/pull/453",
        dc:description "A traction battery is a battery that is used in vehicles for propulsion.",
        rdfs:label "traction battery"@en
    
    SubClassOf: 
        OEO_00000068
    
    
Class: OEO_00010027

    Annotations: 
        <http://purl.obolibrary.org/obo/IAO_0000233> "issue: https://github.com/OpenEnergyPlatform/ontology/issues/425
pull request: https://github.com/OpenEnergyPlatform/ontology/pull/453",
        dc:description "An electric motor is an energy converting device that converts electrical energy into kinetic energy.",
        rdfs:label "electric motor"@en
    
    SubClassOf: 
        OEO_00010032,
        OEO_00000503 some OEO_00000139
    
    
Class: OEO_00010028

    Annotations: 
        <http://purl.obolibrary.org/obo/IAO_0000233> "issue: https://github.com/OpenEnergyPlatform/ontology/issues/425
pull request: https://github.com/OpenEnergyPlatform/ontology/pull/453",
        dc:description "A traction motor is an electric motor used for propulsion.",
        rdfs:label "traction motor"@en
    
    SubClassOf: 
        OEO_00010027
    
    
Class: OEO_00010029

    Annotations: 
        <http://purl.obolibrary.org/obo/IAO_0000233> "issue: https://github.com/OpenEnergyPlatform/ontology/issues/425
pull request: https://github.com/OpenEnergyPlatform/ontology/pull/453",
        dc:description "An internal combustion engine is an energy converting device that converts chemical energy into into rotational energy using a cyclic combustion process.",
        rdfs:label "internal combustion engine"@en
    
    SubClassOf: 
        OEO_00010032,
        OEO_00000503 some OEO_00000099
    
    
Class: OEO_00010030

    Annotations: 
        <http://purl.obolibrary.org/obo/IAO_0000118> "PHEV",
        <http://purl.obolibrary.org/obo/IAO_0000233> "issue: https://github.com/OpenEnergyPlatform/ontology/issues/425
pull request: https://github.com/OpenEnergyPlatform/ontology/pull/453",
        dc:description "A plug-in hybrid electric vehicle (PHEV) is a vehicle that contains both a traction motor and an internal combustion engine and can switch between their usage for propulsion. It contains a traction battery that can be charged with electrical energy from an external supply.",
        rdfs:label "plug-in hybrid electric vehicle"@en
    
    SubClassOf: 
        OEO_00010023,
        OEO_00000503 some OEO_00000099,
        OEO_00000503 some OEO_00000139,
        <http://purl.obolibrary.org/obo/BFO_0000051> some OEO_00010026,
        <http://purl.obolibrary.org/obo/BFO_0000051> some OEO_00010028,
        <http://purl.obolibrary.org/obo/BFO_0000051> some OEO_00010029
    
    
Class: OEO_00010031

    Annotations: 
        <http://purl.obolibrary.org/obo/IAO_0000233> "A grid supplied electric vehicle is an electric vehicle that uses electrical energy via a conductor.",
        <http://purl.obolibrary.org/obo/IAO_0000233> "issue: https://github.com/OpenEnergyPlatform/ontology/issues/425
pull request: https://github.com/OpenEnergyPlatform/ontology/pull/453",
        rdfs:label "grid supplied electric vehicle"@en
    
    SubClassOf: 
        OEO_00000146
    
    
Class: OEO_00010032

    Annotations: 
        <http://purl.obolibrary.org/obo/IAO_0000233> "issue: https://github.com/OpenEnergyPlatform/ontology/issues/425
pull request: https://github.com/OpenEnergyPlatform/ontology/pull/453",
        dc:description "A motor is an energy converting device that converts other forms of energy into rotational kinetic energy.",
        rdfs:label "motor"
    
    SubClassOf: 
        OEO_00000011
    
    
Class: OEO_00020001

    Annotations: 
        <http://purl.obolibrary.org/obo/IAO_0000115> "Ethanol is a portion of matter with the chemical formula C2H6O. It has a liquid normal state of matter and can be used as a combustion fuel."@en,
        <http://purl.obolibrary.org/obo/IAO_0000233> "issue: https://github.com/OpenEnergyPlatform/ontology/issues/439
pull request: https://github.com/OpenEnergyPlatform/ontology/pull/445"@en,
        rdfs:label "ethanol"@en
    
    SubClassOf: 
        OEO_00000331,
        <http://purl.obolibrary.org/obo/BFO_0000050> some OEO_00000075
    
    
Class: OEO_00020003

    Annotations: 
        <http://purl.obolibrary.org/obo/IAO_0000115> "Energy transformation is a process in which one ore more certain types of energy as input result in certain types of energy as output.",
        <http://purl.obolibrary.org/obo/IAO_0000233> "issue: https://github.com/OpenEnergyPlatform/ontology/issues/435
pull request: https://github.com/OpenEnergyPlatform/ontology/pull/450",
        <http://purl.obolibrary.org/obo/IAO_0000233> "issue: https://github.com/OpenEnergyPlatform/ontology/issues/77
pull request: https://github.com/OpenEnergyPlatform/ontology/pull/371",
        rdfs:label "energy transformation"@en
    
    SubClassOf: 
        OEO_00000419
    
    
Class: OEO_00020004

    Annotations: 
        <http://purl.obolibrary.org/obo/IAO_0000115> "A gas grid is a supply grid that distributes gaseous fuel, e.g. methane.",
        <http://purl.obolibrary.org/obo/IAO_0000233> "issue: https://github.com/OpenEnergyPlatform/ontology/issues/36
pull request: https://github.com/OpenEnergyPlatform/ontology/385",
        rdfs:label "gas grid"@en
    
    SubClassOf: 
        OEO_00000200,
        <http://purl.obolibrary.org/obo/BFO_0000051> some OEO_00020007
    
    
Class: OEO_00020005

    Annotations: 
        <http://purl.obolibrary.org/obo/IAO_0000115> "A heating grid is a supply grid that distributes thermal energy via circulating steam or liquids."@en,
        <http://purl.obolibrary.org/obo/IAO_0000233> "issue: https://github.com/OpenEnergyPlatform/ontology/issues/36
pull request: https://github.com/OpenEnergyPlatform/ontology/385",
        rdfs:label "heating grid"@en
    
    SubClassOf: 
        OEO_00000200,
        <http://purl.obolibrary.org/obo/BFO_0000051> some OEO_00020008
    
    
Class: OEO_00020006

    Annotations: 
        <http://purl.obolibrary.org/obo/IAO_0000115> "A grid component is an artificial object that is a discrete part of a supply grid serving a specific purpose."@en,
        <http://purl.obolibrary.org/obo/IAO_0000233> "issue: https://github.com/OpenEnergyPlatform/ontology/issues/36
pull request: https://github.com/OpenEnergyPlatform/ontology/pull/385",
        rdfs:label "grid component"@en
    
    SubClassOf: 
        OEO_00000061,
        <http://purl.obolibrary.org/obo/BFO_0000050> some OEO_00000200
    
    
Class: OEO_00020007

    Annotations: 
        <http://purl.obolibrary.org/obo/IAO_0000115> "A gas grid component is a grid component that is part of a gas grid."@en,
        <http://purl.obolibrary.org/obo/IAO_0000233> "issue: https://github.com/OpenEnergyPlatform/ontology/issues/36
issue: https://github.com/OpenEnergyPlatform/ontology/issues/231
pull request: https://github.com/OpenEnergyPlatform/ontology/pull/385"@en,
        rdfs:label "gas grid component"@en
    
    EquivalentTo: 
        OEO_00020006
         and (<http://purl.obolibrary.org/obo/BFO_0000050> some OEO_00020004)
    
    SubClassOf: 
        OEO_00020006
    
    
Class: OEO_00020008

    Annotations: 
        <http://purl.obolibrary.org/obo/IAO_0000115> "A heating grid component is a grid component that is part of a heating grid."@en,
        <http://purl.obolibrary.org/obo/IAO_0000233> "issue: https://github.com/OpenEnergyPlatform/ontology/issues/36
issue: https://github.com/OpenEnergyPlatform/ontology/issues/231
pull request: https://github.com/OpenEnergyPlatform/ontology/pull/385"@en,
        rdfs:label "heating grid component"@en
    
    EquivalentTo: 
        OEO_00020006
         and (<http://purl.obolibrary.org/obo/BFO_0000050> some OEO_00020005)
    
    SubClassOf: 
        OEO_00020006
    
    
Class: OEO_00020009

    Annotations: 
        <http://purl.obolibrary.org/obo/IAO_0000115> "A switchyard is an electricity grid component that connects different levels of voltage"@en,
        <http://purl.obolibrary.org/obo/IAO_0000233> "issue: https://github.com/OpenEnergyPlatform/ontology/issues/231
pull request: https://github.com/OpenEnergyPlatform/ontology/pull/385"@en,
        rdfs:label "switchyard"@en
    
    SubClassOf: 
        OEO_00020006,
        <http://purl.obolibrary.org/obo/BFO_0000050> some OEO_00000143,
        <http://purl.obolibrary.org/obo/BFO_0000051> some OEO_00000420
    
    
Class: OEO_00020037

    Annotations: 
        <http://purl.obolibrary.org/obo/IAO_0000115> "Radiation is the process of emitting or transmitting energy in the form of waves or particles through a spatial region or a material entity.",
        <http://purl.obolibrary.org/obo/IAO_0000119> "Adaptation of https://en.wikipedia.org/w/index.php?title=Radiation&oldid=986678480",
        <http://purl.obolibrary.org/obo/IAO_0000233> "issue: https://github.com/OpenEnergyPlatform/ontology/issues/362
pull request: https://github.com/OpenEnergyPlatform/ontology/pull/600",
        rdfs:label "radiation"
    
    SubClassOf: 
        <http://purl.obolibrary.org/obo/BFO_0000015>
    
    
Class: OEO_00020038

    Annotations: 
        <http://purl.obolibrary.org/obo/IAO_0000115> "Solar radiation is radiation that is emitted by the sun.",
        <http://purl.obolibrary.org/obo/IAO_0000233> "issue: https://github.com/OpenEnergyPlatform/ontology/issues/362
pull request: https://github.com/OpenEnergyPlatform/ontology/pull/600",
        rdfs:label "solar radiation"
    
    SubClassOf: 
        OEO_00020037
    
    
Class: OEO_00030000

    Annotations: 
        <http://purl.obolibrary.org/obo/IAO_0000115> "anthropogenic is an origin of portions of matter created by human activity.",
        <http://purl.obolibrary.org/obo/IAO_0000233> "issue: https://github.com/OpenEnergyPlatform/ontology/issues/56
pull request: https://github.com/OpenEnergyPlatform/ontology/pull/234",
        rdfs:label "anthropogenic"
    
    SubClassOf: 
        OEO_00000316
    
    
Class: OEO_00030001

    Annotations: 
        <http://purl.obolibrary.org/obo/IAO_0000115> "biogenic is an origin of portions of matter made by or produced from life forms.",
        <http://purl.obolibrary.org/obo/IAO_0000233> "issue: https://github.com/OpenEnergyPlatform/ontology/issues/108
pull request: https://github.com/OpenEnergyPlatform/ontology/pull/130",
        rdfs:label "biogenic"
    
    SubClassOf: 
        OEO_00000316
    
    
Class: OEO_00030002

    Annotations: 
        <http://purl.obolibrary.org/obo/IAO_0000115> "fossil is an origin of portions of matter created from organic material by geolocial processes lasting thousands or millions of years.

In real world, fossils are from biogenic origin some thousands or millions of years ago. However, this is irrelevant in the energy modelling domain.",
        <http://purl.obolibrary.org/obo/IAO_0000233> "issue: https://github.com/OpenEnergyPlatform/ontology/issues/108
pull request: https://github.com/OpenEnergyPlatform/ontology/pull/130",
        rdfs:label "fossil"
    
    SubClassOf: 
        OEO_00030003
    
    
Class: OEO_00030003

    Annotations: 
        <http://purl.obolibrary.org/obo/IAO_0000115> "geogenic is an origin of portions of matter that are the result of geological processes.",
        <http://purl.obolibrary.org/obo/IAO_0000233> "issue: https://github.com/OpenEnergyPlatform/ontology/issues/182
pull request: https://github.com/OpenEnergyPlatform/ontology/pull/237",
        rdfs:label "geogenic"
    
    SubClassOf: 
        OEO_00000316
    
    
Class: OEO_00030004

    Annotations: 
        <http://purl.obolibrary.org/obo/IAO_0000115> "Renewable is an origin of portions of matter that replenish on a human time scale.",
        <http://purl.obolibrary.org/obo/IAO_0000233> "issue: https://github.com/OpenEnergyPlatform/ontology/issues/397
pull request: https://github.com/OpenEnergyPlatform/ontology/pull/398
issue: https://github.com/OpenEnergyPlatform/ontology/issues/108
pull request: https://github.com/OpenEnergyPlatform/ontology/pull/130",
        rdfs:label "renewable"
    
    SubClassOf: 
        OEO_00000316
    
    
Class: OEO_00030005

    Annotations: 
        <http://purl.obolibrary.org/obo/IAO_0000115> "synthetic is an origin of portions of matter created artifically by a chemical process.",
        <http://purl.obolibrary.org/obo/IAO_0000233> "issue: https://github.com/OpenEnergyPlatform/ontology/issues/108
pull request: https://github.com/OpenEnergyPlatform/ontology/pull/130",
        rdfs:label "synthetic"
    
    SubClassOf: 
        OEO_00000316
    
    
Class: OEO_00030019

    Annotations: 
        <http://purl.obolibrary.org/obo/IAO_0000115> "A process attribute is a dependent occurrent that existentially depends on a process.",
        <http://purl.obolibrary.org/obo/IAO_0000233> "issue: https://github.com/OpenEnergyPlatform/ontology/issues/205
pull request: https://github.com/OpenEnergyPlatform/ontology/pull/386",
        rdfs:label "process attribute"
    
    SubClassOf: 
        <http://purl.obolibrary.org/obo/BFO_0000003>
    
    
Class: OEO_00030024

    Annotations: 
        <http://purl.obolibrary.org/obo/IAO_0000115> "An energy system is a system of spatially extended linked energy sources and sinks.",
        <http://purl.obolibrary.org/obo/IAO_0000233> "issue: https://github.com/OpenEnergyPlatform/ontology/issues/432
pull request: https://github.com/OpenEnergyPlatform/ontology/pull/493",
        rdfs:label "energy system"
    
    SubClassOf: 
        <http://purl.obolibrary.org/obo/RO_0002577>
    
    
Class: OEO_00030025

    Annotations: 
        <http://purl.obolibrary.org/obo/IAO_0000115> "A supply system is a system that connects producers and consumers.",
        <http://purl.obolibrary.org/obo/IAO_0000233> "issue: https://github.com/OpenEnergyPlatform/ontology/issues/432
pull request: https://github.com/OpenEnergyPlatform/ontology/pull/493",
        rdfs:label "supply system"
    
    SubClassOf: 
        <http://purl.obolibrary.org/obo/RO_0002577>
    
    
Class: OEO_00030026

    Annotations: 
        <http://purl.obolibrary.org/obo/IAO_0000115> "Primary energy production is a process that prepares raw material for its use as primary energy carrier.",
        <http://purl.obolibrary.org/obo/IAO_0000233> "issue: https://github.com/OpenEnergyPlatform/ontology/issues/77
pull request: https://github.com/OpenEnergyPlatform/ontology/pull/498",
        rdfs:label "primary energy production"
    
    SubClassOf: 
        <http://purl.obolibrary.org/obo/BFO_0000015>
    
    
Class: OEO_00030027

    Annotations: 
        <http://purl.obolibrary.org/obo/IAO_0000115> "Primary energy carrier mining is a primary energy production process that recovers non-renewable energy carriers from its natural site.",
        <http://purl.obolibrary.org/obo/IAO_0000233> "issue: https://github.com/OpenEnergyPlatform/ontology/issues/77
pull request: https://github.com/OpenEnergyPlatform/ontology/pull/498",
        rdfs:label "primary energy carrier mining"
    
    SubClassOf: 
        OEO_00030026
    
    
Class: OEO_00030028

    Annotations: 
        <http://purl.obolibrary.org/obo/IAO_0000115> "Primary energy carrier harvest is a primary energy production process that collects solid biomass from its natural site.",
        <http://purl.obolibrary.org/obo/IAO_0000233> "issue: https://github.com/OpenEnergyPlatform/ontology/issues/77
pull request: https://github.com/OpenEnergyPlatform/ontology/pull/498",
        rdfs:label "primary energy carrier harvest"
    
    SubClassOf: 
        OEO_00030026
    
    
Class: OEO_00050000

    Annotations: 
        <http://purl.obolibrary.org/obo/IAO_0000115> "An industrial process is a process that has output object or object aggregates that are economic goods. An industrial process consists of several subprocesses. Examples of subprocesses that can be involved in an industrial process are energy transformations, mechanical operations and chemical reactions.",
        <http://purl.obolibrary.org/obo/IAO_0000233> "issue: https://github.com/OpenEnergyPlatform/ontology/issues/534
pull request: https://github.com/OpenEnergyPlatform/ontology/pull/589",
        rdfs:label "industrial process"@en
    
    SubClassOf: 
        <http://purl.obolibrary.org/obo/BFO_0000015>,
        <http://purl.obolibrary.org/obo/RO_0002234> some 
            (<http://purl.obolibrary.org/obo/BFO_0000027> or <http://purl.obolibrary.org/obo/BFO_0000030>)
    
    
Class: OEO_00050001

    Annotations: 
        <http://purl.obolibrary.org/obo/IAO_0000115> "Fuel-powered electricity generation is a transformation that contains at least two sub process: An energy transformation of chemical energy from fuel into electrical energy and an emission process.",
        <http://purl.obolibrary.org/obo/IAO_0000233> "issue: https://github.com/OpenEnergyPlatform/ontology/issues/582
pull request: https://github.com/OpenEnergyPlatform/ontology/pull/592",
        rdfs:label "fuel-powered electricity generation"@en
    
    SubClassOf: 
        OEO_00000419,
        OEO_00000500 some OEO_00000148,
        <http://purl.obolibrary.org/obo/BFO_0000051> some OEO_00000147,
        <http://purl.obolibrary.org/obo/BFO_0000051> some OEO_00020003,
        <http://purl.obolibrary.org/obo/RO_0000057> some OEO_00000174,
        <http://purl.obolibrary.org/obo/RO_0000057> some OEO_00000175
    
    
Class: OEO_00050002

    Annotations: 
        <http://purl.obolibrary.org/obo/IAO_0000115> "An energy unit which is equal to 1,000 joules.",
        <http://purl.obolibrary.org/obo/IAO_0000233> "issue: https://github.com/OpenEnergyPlatform/ontology/issues/606
pull request: https://github.com/OpenEnergyPlatform/ontology/pull/608",
        <http://www.geneontology.org/formats/oboInOwl#hasExactSynonym> "kJ",
        rdfs:label "kilojoule"@en
    
    SubClassOf: 
        <http://purl.obolibrary.org/obo/UO_0000111>
    
    
Class: OEO_00050003

    Annotations: 
        <http://purl.obolibrary.org/obo/IAO_0000115> "An energy unit which is equal to 1,000,000 joules.",
        <http://purl.obolibrary.org/obo/IAO_0000233> "issue: https://github.com/OpenEnergyPlatform/ontology/issues/606
pull request: https://github.com/OpenEnergyPlatform/ontology/pull/608",
        <http://www.geneontology.org/formats/oboInOwl#hasExactSynonym> "MJ",
        rdfs:label "megajoule"@en
    
    SubClassOf: 
        <http://purl.obolibrary.org/obo/UO_0000111>
    
    
Class: OEO_00050004

    Annotations: 
        <http://purl.obolibrary.org/obo/IAO_0000115> "An energy unit which is equal to 10^9 joules.",
        <http://purl.obolibrary.org/obo/IAO_0000233> "issue: https://github.com/OpenEnergyPlatform/ontology/issues/606
pull request: https://github.com/OpenEnergyPlatform/ontology/pull/608",
        <http://www.geneontology.org/formats/oboInOwl#hasExactSynonym> "GJ",
        rdfs:label "gigajoule"@en
    
    SubClassOf: 
        <http://purl.obolibrary.org/obo/UO_0000111>
    
    
Class: OEO_00050005

    Annotations: 
        <http://purl.obolibrary.org/obo/IAO_0000115> "An energy unit which is equal to 10^12 joules.",
        <http://purl.obolibrary.org/obo/IAO_0000233> "issue: https://github.com/OpenEnergyPlatform/ontology/issues/606
pull request: https://github.com/OpenEnergyPlatform/ontology/pull/608",
        <http://www.geneontology.org/formats/oboInOwl#hasExactSynonym> "TJ",
        rdfs:label "terajoule"@en
    
    SubClassOf: 
        <http://purl.obolibrary.org/obo/UO_0000111>
    
    
Class: OEO_00050006

    Annotations: 
        <http://purl.obolibrary.org/obo/IAO_0000115> "An energy unit which is equal to 10^15 joules.",
        <http://purl.obolibrary.org/obo/IAO_0000233> "issue: https://github.com/OpenEnergyPlatform/ontology/issues/606
pull request: https://github.com/OpenEnergyPlatform/ontology/pull/608",
        <http://www.geneontology.org/formats/oboInOwl#hasExactSynonym> "PJ",
        rdfs:label "petajoule"@en
    
    SubClassOf: 
        <http://purl.obolibrary.org/obo/UO_0000111>
    
    
Class: OEO_00050007

    Annotations: 
        <http://purl.obolibrary.org/obo/IAO_0000115> "An energy unit which is equal to 10^18 joules.",
        <http://purl.obolibrary.org/obo/IAO_0000233> "issue: https://github.com/OpenEnergyPlatform/ontology/issues/606
pull request: https://github.com/OpenEnergyPlatform/ontology/pull/608",
        <http://www.geneontology.org/formats/oboInOwl#hasExactSynonym> "EJ",
        rdfs:label "exajoule"@en
    
    SubClassOf: 
        <http://purl.obolibrary.org/obo/UO_0000111>
    
    
Class: OEO_00050008

    Annotations: 
        <http://purl.obolibrary.org/obo/IAO_0000115> "An energy unit which is equal to 1,000,000 watt-hours.",
        <http://purl.obolibrary.org/obo/IAO_0000233> "issue: https://github.com/OpenEnergyPlatform/ontology/issues/606
pull request: https://github.com/OpenEnergyPlatform/ontology/pull/608",
        <http://www.geneontology.org/formats/oboInOwl#hasExactSynonym> "MWh",
        rdfs:label "megawatt-hour"@en
    
    SubClassOf: 
        <http://purl.obolibrary.org/obo/UO_0000111>
    
    
Class: OEO_00050009

    Annotations: 
        <http://purl.obolibrary.org/obo/IAO_0000115> "An energy unit which is equal to 10^12 watt-hours.",
        <http://purl.obolibrary.org/obo/IAO_0000233> "issue: https://github.com/OpenEnergyPlatform/ontology/issues/606
pull request: https://github.com/OpenEnergyPlatform/ontology/pull/608",
        <http://www.geneontology.org/formats/oboInOwl#hasExactSynonym> "TWh",
        rdfs:label "terawatt-hour"@en
    
    SubClassOf: 
        <http://purl.obolibrary.org/obo/UO_0000111>
    
    
Class: OEO_00050010

    Annotations: 
        <http://purl.obolibrary.org/obo/IAO_0000115> "An energy unit which is equal to 10^15 watt-hours.",
        <http://purl.obolibrary.org/obo/IAO_0000233> "issue: https://github.com/OpenEnergyPlatform/ontology/issues/606
pull request: https://github.com/OpenEnergyPlatform/ontology/pull/608",
        <http://www.geneontology.org/formats/oboInOwl#hasExactSynonym> "PWh",
        rdfs:label "petawatt-hour"@en
    
    SubClassOf: 
        <http://purl.obolibrary.org/obo/UO_0000111>
    
    
Class: OEO_00050011

    Annotations: 
        <http://purl.obolibrary.org/obo/IAO_0000115> "An energy unit which is equal to 10^9 watt-hours.",
        <http://purl.obolibrary.org/obo/IAO_0000233> "issue: https://github.com/OpenEnergyPlatform/ontology/issues/606
pull request: https://github.com/OpenEnergyPlatform/ontology/pull/608",
        <http://www.geneontology.org/formats/oboInOwl#hasExactSynonym> "GWh",
        rdfs:label "gigawatt-hour"@en
    
    SubClassOf: 
        <http://purl.obolibrary.org/obo/UO_0000111>
    
    
Class: OEO_00140000

    Annotations: 
        <http://purl.obolibrary.org/obo/IAO_0000115> "Hub height is a quality of a wind energy converting unit that measures the distance between surface and center-line of the wind rotor.",
        <http://purl.obolibrary.org/obo/IAO_0000233> "issue: https://github.com/OpenEnergyPlatform/ontology/issues/505
pull request: https://github.com/OpenEnergyPlatform/ontology/pull/509",
        rdfs:label "hub height"@en
    
    SubClassOf: 
        <http://purl.obolibrary.org/obo/BFO_0000019>,
        OEO_00140002 some OEO_00140001
    
    
Class: OEO_00140001

    Annotations: 
        <http://purl.obolibrary.org/obo/IAO_0000115> "Length value is a quantity value that has a length unit as unit.",
        <http://purl.obolibrary.org/obo/IAO_0000233> "issue: https://github.com/OpenEnergyPlatform/ontology/issues/505
pull request: https://github.com/OpenEnergyPlatform/ontology/pull/509",
        rdfs:label "length value"@en
    
    SubClassOf: 
        OEO_00000350,
        <http://purl.obolibrary.org/obo/BFO_0000051> some <http://purl.obolibrary.org/obo/UO_0000001>
    
    
Class: OEO_00140033

    Annotations: 
        <http://purl.obolibrary.org/obo/IAO_0000115> "A chemical reaction is a transformation that involves the interconversion of chemical species.",
        <http://purl.obolibrary.org/obo/IAO_0000233> "issue: https://github.com/OpenEnergyPlatform/ontology/issues/449
pull request: https://github.com/OpenEnergyPlatform/ontology/pull/568",
        rdfs:label "chemical reaction"@en
    
    SubClassOf: 
        OEO_00000419
    
    
Class: OEO_00140034

    Annotations: 
        <http://purl.obolibrary.org/obo/IAO_0000115> "A redox reaction is a chemical reaction in which the oxidation of one reactant is coupled to the reduction of a second reactant.",
        <http://purl.obolibrary.org/obo/IAO_0000118> "oxidation",
        <http://purl.obolibrary.org/obo/IAO_0000233> "issue: https://github.com/OpenEnergyPlatform/ontology/issues/449
pull request: https://github.com/OpenEnergyPlatform/ontology/pull/568",
        rdfs:label "redox reaction"@en
    
    SubClassOf: 
        OEO_00140033
    
    
Class: OEO_00140035

    Annotations: 
        <http://purl.obolibrary.org/obo/IAO_0000115> "Oxidation is a chemical reaction that describes the loss of electrons of an atom, an ion, or of certain atoms in a molecule and is a part of a redox reaction.",
        <http://purl.obolibrary.org/obo/IAO_0000233> "issue: https://github.com/OpenEnergyPlatform/ontology/issues/449
pull request: https://github.com/OpenEnergyPlatform/ontology/pull/568",
        rdfs:label "oxidation"@en
    
    SubClassOf: 
        OEO_00140033
    
    
Class: OEO_00140036

    Annotations: 
        <http://purl.obolibrary.org/obo/IAO_0000115> "Reduction is a chemical reaction that describes the gain of electrons of an atom, an ion, or of certain atoms in a molecule and is a part of a redox reaction.",
        <http://purl.obolibrary.org/obo/IAO_0000233> "issue: https://github.com/OpenEnergyPlatform/ontology/issues/449
pull request: https://github.com/OpenEnergyPlatform/ontology/pull/568",
        rdfs:label "reduction"@en
    
    SubClassOf: 
        OEO_00140033
    
    
Class: OEO_00140037

    Annotations: 
        <http://purl.obolibrary.org/obo/IAO_0000115> "An electrochemical reaction is a chemical reaction that describes the overall reactions of individual redox reactions being separated but connected by an external electric circuit and an intervening electrolyte.",
        <http://purl.obolibrary.org/obo/IAO_0000233> "issue: https://github.com/OpenEnergyPlatform/ontology/issues/449
pull request: https://github.com/OpenEnergyPlatform/ontology/pull/568",
        rdfs:label "electrochemical reaction"@en
    
    SubClassOf: 
        OEO_00140033
    
    
Class: OEO_00140038

    Annotations: 
        <http://purl.obolibrary.org/obo/IAO_0000115> "Combustion is an exothermic redox reaction between a fuel (the reductant) and an oxidant (usually atmospheric oxygen) which is initiated by a ignition source.",
        <http://purl.obolibrary.org/obo/IAO_0000233> "issue: https://github.com/OpenEnergyPlatform/ontology/issues/449
pull request: https://github.com/OpenEnergyPlatform/ontology/pull/568",
        rdfs:label "combustion"@en
    
    SubClassOf: 
        OEO_00140034
    
    
Class: OEO_00140049

    Annotations: 
        <http://purl.obolibrary.org/obo/IAO_0000115> "Energy conversion efficiency is a process attribute describing the ratio between the input of an energy transformation and the outputs that are used.",
        <http://purl.obolibrary.org/obo/IAO_0000233> "issue: https://github.com/OpenEnergyPlatform/ontology/issues/434
pull request: https://github.com/OpenEnergyPlatform/ontology/pull/591",
        rdfs:label "energy conversion efficiency"@en
    
    SubClassOf: 
        OEO_00030019,
        OEO_00000502 some OEO_00020003,
        OEO_00140002 some OEO_00140050
    
    
Class: OEO_00140050

    Annotations: 
        <http://purl.obolibrary.org/obo/IAO_0000115> "An efficiency value is a quantity value stating the ratio between a process's inputs and the outputs that are used.",
        <http://purl.obolibrary.org/obo/IAO_0000233> "issue: https://github.com/OpenEnergyPlatform/ontology/issues/434
pull request: https://github.com/OpenEnergyPlatform/ontology/pull/591",
        rdfs:label "efficiency value"@en
    
    SubClassOf: 
        OEO_00000350,
        OEO_00040010 some <http://purl.obolibrary.org/obo/UO_0010006>
    
    
Class: OEO_00140051

    Annotations: 
        <http://purl.obolibrary.org/obo/IAO_0000115> "A coefficient of performance value is a quantity value stating the ratio between the work input and the total output of an energy conversion process.",
        <http://purl.obolibrary.org/obo/IAO_0000233> "issue: https://github.com/OpenEnergyPlatform/ontology/issues/434
pull request: https://github.com/OpenEnergyPlatform/ontology/pull/591",
        rdfs:label "coefficient of performance value"@en
    
    SubClassOf: 
        OEO_00000350,
        OEO_00040010 some <http://purl.obolibrary.org/obo/UO_0010006>
    
    
Class: OEO_00140052

    Annotations: 
        <http://purl.obolibrary.org/obo/IAO_0000115> "Energy conversion performance is a process attribute describing the ratio between the non-heat input of an energy transformation and the outputs that are used.",
        <http://purl.obolibrary.org/obo/IAO_0000233> "issue: https://github.com/OpenEnergyPlatform/ontology/issues/434
pull request: https://github.com/OpenEnergyPlatform/ontology/pull/591",
        rdfs:label "energy conversion performance"@en
    
    SubClassOf: 
        OEO_00030019,
        OEO_00000502 some OEO_00020003,
        OEO_00140002 some OEO_00140051
    
    
Class: OEO_00140056

    Annotations: 
        <http://purl.obolibrary.org/obo/IAO_0000115> "A flow potential is a quantity value that describes the upper limit of an input or output of a process in a spatial region of reference per unit time.",
        <http://purl.obolibrary.org/obo/IAO_0000233> "issue: https://github.com/OpenEnergyPlatform/ontology/issues/481
pull request: https://github.com/OpenEnergyPlatform/ontology/pull/607",
        rdfs:label "flow potential"@en
    
    SubClassOf: 
        OEO_00000350
    
    
Class: OEO_00140057

    Annotations: 
        <http://purl.obolibrary.org/obo/IAO_0000115> "A theoretical flow potential is a type of flow potential that identifies the physical upper limit of an input or output of a process in a spatial region of reference per unit time.",
        <http://purl.obolibrary.org/obo/IAO_0000233> "issue: https://github.com/OpenEnergyPlatform/ontology/issues/481
pull request: https://github.com/OpenEnergyPlatform/ontology/pull/607",
        rdfs:label "theoretical flow potential"@en
    
    SubClassOf: 
        OEO_00140056
    
    
Class: OEO_00140058

    Annotations: 
        <http://purl.obolibrary.org/obo/IAO_0000115> "A technological flow potential is a type of a flow potential derived from a theoretical flow potential, taking account of the annual efficiency of the respective conversion technology and the additional restrictions regarding the area that is realistically available for energy generation.",
        <http://purl.obolibrary.org/obo/IAO_0000233> "issue: https://github.com/OpenEnergyPlatform/ontology/issues/481
pull request: https://github.com/OpenEnergyPlatform/ontology/pull/607",
        rdfs:label "technological flow potential"@en
    
    SubClassOf: 
        OEO_00140056
    
    
Class: OEO_00140059

    Annotations: 
        <http://purl.obolibrary.org/obo/IAO_0000115> "An economic flow potential is a type of flow potential that identifies the proportion of the technological potential that can be utilized economically (based on economic boundary conditions).",
        <http://purl.obolibrary.org/obo/IAO_0000233> "issue: https://github.com/OpenEnergyPlatform/ontology/issues/481
pull request: https://github.com/OpenEnergyPlatform/ontology/pull/607",
        rdfs:label "economic flow potential"@en
    
    SubClassOf: 
        OEO_00140056
    
    
Class: OEO_00140060

    Annotations: 
        <http://purl.obolibrary.org/obo/IAO_0000115> "A developable flow potential is a type of flow potential that describes the fraction of the economic potential that can be developed under realistic conditions (regulations, environmental and social restrictions).",
        <http://purl.obolibrary.org/obo/IAO_0000233> "issue: https://github.com/OpenEnergyPlatform/ontology/issues/481
pull request: https://github.com/OpenEnergyPlatform/ontology/pull/607",
        rdfs:label "developable flow potential"@en
    
    SubClassOf: 
        OEO_00140056
    
    
Class: OEO_00140061

    Annotations: 
        <http://purl.obolibrary.org/obo/IAO_0000115> "A sustainable flow potential is a type of flow potential that takes into account all aspects of sustainability, which usually requires careful consideration and evaluation of different ecological and socio-economic aspects. The differentiation of the sustainable potential is blurred, since ecological aspects may already have been considered for the technological or economic potential, depending on the author.",
        <http://purl.obolibrary.org/obo/IAO_0000233> "issue: https://github.com/OpenEnergyPlatform/ontology/issues/481
pull request: https://github.com/OpenEnergyPlatform/ontology/pull/607",
        rdfs:label "sustainable flow potential"@en
    
    SubClassOf: 
        OEO_00140056
    
    
Class: OEO_00140062

    Annotations: 
        <http://purl.obolibrary.org/obo/IAO_0000115> "A stock potential is a quantity value that describes the upper limit of a stock of a source or sink in a spatial region of reference.",
        <http://purl.obolibrary.org/obo/IAO_0000233> "issue: https://github.com/OpenEnergyPlatform/ontology/issues/481
pull request: https://github.com/OpenEnergyPlatform/ontology/pull/607",
        rdfs:label "stock potential"@en
    
    SubClassOf: 
        OEO_00000350
    
    
Class: OEO_00140063

    Annotations: 
        <http://purl.obolibrary.org/obo/IAO_0000115> "A theoretical stock potential is a type of stock potential that identifies the physical upper limit of a stock of a source or sink in a spatial region of reference.",
        <http://purl.obolibrary.org/obo/IAO_0000233> "issue: https://github.com/OpenEnergyPlatform/ontology/issues/481
pull request: https://github.com/OpenEnergyPlatform/ontology/pull/607",
        rdfs:label "theoretical stock potential"@en
    
    SubClassOf: 
        OEO_00140062
    
    
Class: OEO_00140064

    Annotations: 
        <http://purl.obolibrary.org/obo/IAO_0000115> "A technological stock potential is a type of a stock potential derived from a theoretical stock potential, taking account of the annual efficiency of the respective conversion technology and the additional restrictions regarding the area that is realistically available for energy generation.",
        <http://purl.obolibrary.org/obo/IAO_0000233> "issue: https://github.com/OpenEnergyPlatform/ontology/issues/481
pull request: https://github.com/OpenEnergyPlatform/ontology/pull/607",
        rdfs:label "technological stock potential"@en
    
    SubClassOf: 
        OEO_00140062
    
    
Class: OEO_00140065

    Annotations: 
        <http://purl.obolibrary.org/obo/IAO_0000115> "An economic stock potential is a type of stock potential that identifies the proportion of the technological potential that can be utilized economically (based on economic boundary conditions).",
        <http://purl.obolibrary.org/obo/IAO_0000233> "issue: https://github.com/OpenEnergyPlatform/ontology/issues/481
pull request: https://github.com/OpenEnergyPlatform/ontology/pull/607",
        rdfs:label "economic stock potential"@en
    
    SubClassOf: 
        OEO_00140062
    
    
Class: OEO_00140066

    Annotations: 
        <http://purl.obolibrary.org/obo/IAO_0000115> "A developable stock potential is a type of stock potential that describes the fraction of the economic potential that can be developed under realistic conditions (regulations, environmental and social restrictions).",
        <http://purl.obolibrary.org/obo/IAO_0000233> "issue: https://github.com/OpenEnergyPlatform/ontology/issues/481
pull request: https://github.com/OpenEnergyPlatform/ontology/pull/607",
        rdfs:label "developable stock potential"@en
    
    SubClassOf: 
        OEO_00140062
    
    
Class: OEO_00140067

    Annotations: 
        <http://purl.obolibrary.org/obo/IAO_0000115> "A sustainable stock potential is a type of stock potential that takes into account all aspects of sustainability, which usually requires careful consideration and evaluation of different ecological and socio-economic aspects. The differentiation of the sustainable potential is blurred, since ecological aspects may already have been considered for the technological or economic potential, depending on the author.",
        <http://purl.obolibrary.org/obo/IAO_0000233> "issue: https://github.com/OpenEnergyPlatform/ontology/issues/481
pull request: https://github.com/OpenEnergyPlatform/ontology/pull/607",
        rdfs:label "sustainable stock potential"@en
    
    SubClassOf: 
        OEO_00140062
    
    
Class: OEO_00230000

    Annotations: 
        <http://purl.obolibrary.org/obo/IAO_0000115> "Storage capacity is the quantity value stating the maximum energy an energy storage object can store.",
        <http://purl.obolibrary.org/obo/IAO_0000233> "issue: https://github.com/OpenEnergyPlatform/ontology/issues/320
pull request: https://github.com/OpenEnergyPlatform/ontology/pull/391",
        rdfs:label "storage capacity"
    
    SubClassOf: 
        OEO_00000350
    
    
Class: OEO_00230001

    Annotations: 
        <http://purl.obolibrary.org/obo/IAO_0000115> "Power rating is the quantity value stating the maximum power an energy converting device can convert.",
        <http://purl.obolibrary.org/obo/IAO_0000233> "issue: https://github.com/OpenEnergyPlatform/ontology/issues/320
pull request: https://github.com/OpenEnergyPlatform/ontology/pull/391",
        rdfs:label "power rating"@en
    
    SubClassOf: 
        OEO_00000350
    
    
Class: OEO_00230002

    Annotations: 
        <http://purl.obolibrary.org/obo/IAO_0000115> "Declared net capacity is the quantity value stating the maximum power a power generating unit or a power plant can deliver to the electrical grid. It equals the sum of the rated powers of all plant generators minus all power used internally within the plant.",
        <http://purl.obolibrary.org/obo/IAO_0000233> "issue: https://github.com/OpenEnergyPlatform/ontology/issues/320
pull request: https://github.com/OpenEnergyPlatform/ontology/pull/391",
        rdfs:label "declared net capacity"@en
    
    SubClassOf: 
        OEO_00000350
    
    
Class: OEO_00230003

    Annotations: 
        <http://purl.obolibrary.org/obo/IAO_0000115> "Nameplate capacity is the quantity value stating the maximum power a power generating unit or a power plant can generate, and the sum of the power ratings of all energy converting devices of that power plant.",
        <http://purl.obolibrary.org/obo/IAO_0000233> "issue: https://github.com/OpenEnergyPlatform/ontology/issues/320
pull request: https://github.com/OpenEnergyPlatform/ontology/pull/391",
        rdfs:label "nameplate capacity"@en
    
    SubClassOf: 
        OEO_00000350
    
    
Class: OEO_00230020

    Annotations: 
        <http://purl.obolibrary.org/obo/IAO_0000115> "Kinetic energy is the energy that a material entity possesses due to its motion. It is defined as the work needed to accelerate a body of a given mass from rest to a stated velocity."@en,
        <http://purl.obolibrary.org/obo/IAO_0000233> "issue: https://github.com/OpenEnergyPlatform/ontology/issues/522
pull request: https://github.com/OpenEnergyPlatform/ontology/pull/609"@en,
        rdfs:label "kinetic energy"@en
    
    SubClassOf: 
        OEO_00000150
    
    
Individual: OEO_00000182

    Annotations: 
        <http://purl.obolibrary.org/obo/IAO_0000115> "The state of being a gas. A portion of matter is in gaseous state if and only if it has has no definite shape and no definite volume and is not electrically conductive.",
        rdfs:label "gaseous"
    
    Types: 
        OEO_00000395
    
    
Individual: OEO_00000256

    Annotations: 
        <http://purl.obolibrary.org/obo/IAO_0000115> "The state of being liquid. A portion of matter is liquid has has no definite shape but a definite volume (at a given temperature and pressure).",
        rdfs:label "liquid"
    
    Types: 
        OEO_00000395
    
    
Individual: OEO_00000326

    Annotations: 
        <http://purl.obolibrary.org/obo/IAO_0000115> "The state of being a plasma. A portion of matter is in plasmatic state if and only if it has has no definite shape and no definite volume and is electrically conductive.",
        rdfs:label "plasmatic"
    
    Types: 
        OEO_00000395
    
    
Individual: OEO_00000390

    Annotations: 
        <http://purl.obolibrary.org/obo/IAO_0000115> "The state being solid. A portion of matter is in solid state if and only if it has a definite shape and volume (at a given temperature and pressure).",
        rdfs:label "solid"
    
    Types: 
        OEO_00000395
    
    
DisjointClasses: 
    OEO_00000188,OEO_00000210,OEO_00000425
