Prefix: : <http://openenergy-platform.org/ontology/oeo/>
Prefix: dc: <http://purl.org/dc/elements/1.1/>
Prefix: owl: <http://www.w3.org/2002/07/owl#>
Prefix: rdf: <http://www.w3.org/1999/02/22-rdf-syntax-ns#>
Prefix: rdfs: <http://www.w3.org/2000/01/rdf-schema#>
Prefix: xml: <http://www.w3.org/XML/1998/namespace>
Prefix: xsd: <http://www.w3.org/2001/XMLSchema#>



Ontology: <http://openenergy-platform.org/ontology/oeo/oeo-sector/>
<http://openenergy-platform.org/ontology/oeo/dev/oeo-sector.omn>
Import: <http://openenergy-platform.org/ontology/oeo/dev/oeo-shared.omn>

Annotations: 
    dc:description "The Open Energy Ontology is an ontology for all aspects of the energy modelling domain. The 'sector' module covers entities that relate to sectors and sector divisions.",
    <http://purl.org/dc/terms/license> "http://creativecommons.org/publicdomain/zero/1.0/",
    <http://purl.org/dc/terms/title> "Open Energy Ontology (sector module)"

AnnotationProperty: <http://purl.obolibrary.org/obo/IAO_0000112>

    
AnnotationProperty: <http://purl.obolibrary.org/obo/IAO_0000115>

    
AnnotationProperty: <http://purl.obolibrary.org/obo/IAO_0000116>

    
AnnotationProperty: <http://purl.obolibrary.org/obo/IAO_0000118>

    
AnnotationProperty: <http://purl.obolibrary.org/obo/IAO_0000119>

    
AnnotationProperty: <http://purl.obolibrary.org/obo/IAO_0000233>

    
AnnotationProperty: <http://purl.obolibrary.org/obo/IAO_0000600>

    
AnnotationProperty: <http://purl.org/dc/terms/license>

    
AnnotationProperty: <http://purl.org/dc/terms/source>

    
AnnotationProperty: <http://purl.org/dc/terms/title>

    
AnnotationProperty: OEO_00010037

    
AnnotationProperty: dc:contributor

    
AnnotationProperty: dc:description

    
AnnotationProperty: dc:identifier

    
AnnotationProperty: rdfs:comment

    
AnnotationProperty: rdfs:isDefinedBy

    
AnnotationProperty: rdfs:label

    
AnnotationProperty: rdfs:seeAlso

    
Datatype: rdf:PlainLiteral

    
Datatype: xsd:string

    
ObjectProperty: <http://purl.obolibrary.org/obo/BFO_0000050>

    
ObjectProperty: <http://purl.obolibrary.org/obo/BFO_0000051>

    
ObjectProperty: <http://purl.obolibrary.org/obo/IAO_0000136>

    
ObjectProperty: <http://purl.obolibrary.org/obo/RO_0000056>

    
ObjectProperty: <http://purl.obolibrary.org/obo/RO_0000057>

    
ObjectProperty: <http://purl.obolibrary.org/obo/RO_0000086>

    
ObjectProperty: <http://purl.obolibrary.org/obo/RO_0000087>

    
ObjectProperty: <http://purl.obolibrary.org/obo/RO_0002410>

    
ObjectProperty: OEO_00000501

    
ObjectProperty: OEO_00000503

    
ObjectProperty: OEO_00000504

    
ObjectProperty: OEO_00000505

    Range: 
        OEO_00000367
    
    
ObjectProperty: OEO_00000506

    
ObjectProperty: OEO_00000507

    
ObjectProperty: OEO_00000508

    
ObjectProperty: OEO_00000509

    
ObjectProperty: OEO_00000510

    
ObjectProperty: OEO_00000522

    
ObjectProperty: OEO_00010121

    
ObjectProperty: OEO_00010231

    
ObjectProperty: OEO_00010232

    Annotations: 
        <http://purl.obolibrary.org/obo/IAO_0000115> "A relation between a sector and a memo item.",
        <http://purl.obolibrary.org/obo/IAO_0000233> "issue: https://github.com/OpenEnergyPlatform/ontology/issues/858
pull request: https://github.com/OpenEnergyPlatform/ontology/pull/967

move to oeo-sector 
issue: https://github.com/OpenEnergyPlatform/ontology/issues/1399
pull request: https://github.com/OpenEnergyPlatform/ontology/pull/1724",
        rdfs:label "has memo item"@en
    
    SubPropertyOf: 
        OEO_00010231
    
    Domain: 
        OEO_00000367
    
    Range: 
        OEO_00010227
    
    
ObjectProperty: OEO_00010312

    Domain: 
        OEO_00000367
    
    
ObjectProperty: OEO_00020056

    
ObjectProperty: OEO_00020179

    
ObjectProperty: OEO_00020180

    
ObjectProperty: OEO_00040010

    
ObjectProperty: OEO_00140002

    
ObjectProperty: OEO_00140008

    
ObjectProperty: OEO_00140017

    Annotations: 
        <http://purl.obolibrary.org/obo/IAO_0000115> "A relation between a person and an organisation where the person is a member of the organisation.",
        <http://purl.obolibrary.org/obo/IAO_0000233> "issue: https://github.com/OpenEnergyPlatform/ontology/issues/486
pull request: https://github.com/OpenEnergyPlatform/ontology/pull/562
move to oeo-sector 
issue: https://github.com/OpenEnergyPlatform/ontology/issues/1399
pull request: https://github.com/OpenEnergyPlatform/ontology/pull/1724",
        rdfs:label "member of"@en
    
    
ObjectProperty: OEO_00140018

    
ObjectProperty: OEO_00140164

    
ObjectProperty: owl:topObjectProperty

    
Class: <http://purl.obolibrary.org/obo/BFO_0000002>

    
Class: <http://purl.obolibrary.org/obo/BFO_0000003>

    
Class: <http://purl.obolibrary.org/obo/BFO_0000004>

    
Class: <http://purl.obolibrary.org/obo/BFO_0000006>

    
Class: <http://purl.obolibrary.org/obo/BFO_0000009>

    
Class: <http://purl.obolibrary.org/obo/BFO_0000015>

    
Class: <http://purl.obolibrary.org/obo/BFO_0000016>

    
Class: <http://purl.obolibrary.org/obo/BFO_0000017>

    
Class: <http://purl.obolibrary.org/obo/BFO_0000019>

    
Class: <http://purl.obolibrary.org/obo/BFO_0000020>

    
Class: <http://purl.obolibrary.org/obo/BFO_0000023>

    
Class: <http://purl.obolibrary.org/obo/BFO_0000024>

    
Class: <http://purl.obolibrary.org/obo/BFO_0000027>

    
Class: <http://purl.obolibrary.org/obo/BFO_0000029>

    
Class: <http://purl.obolibrary.org/obo/BFO_0000030>

    
Class: <http://purl.obolibrary.org/obo/BFO_0000031>

    
Class: <http://purl.obolibrary.org/obo/BFO_0000038>

    
Class: <http://purl.obolibrary.org/obo/BFO_0000040>

    
Class: <http://purl.obolibrary.org/obo/BFO_0000141>

    
Class: <http://purl.obolibrary.org/obo/BFO_0000148>

    
Class: <http://purl.obolibrary.org/obo/IAO_0000030>

    
Class: <http://purl.obolibrary.org/obo/IAO_0000104>

    
Class: <http://purl.obolibrary.org/obo/IAO_0000310>

    
Class: <http://purl.obolibrary.org/obo/RO_0002577>

    
Class: <http://purl.obolibrary.org/obo/UO_0000000>

    
Class: <http://purl.obolibrary.org/obo/UO_0000187>

    
Class: <http://purl.obolibrary.org/obo/UO_0000189>

    
Class: <http://purl.obolibrary.org/obo/UO_0000190>

    
Class: <http://purl.obolibrary.org/obo/UO_0010006>

    
Class: OEO_00000051

    
Class: OEO_00000064

    
Class: OEO_00000107

    
Class: OEO_00000128

    Annotations: 
        <http://purl.obolibrary.org/obo/IAO_0000115> "An energy demand sector is a sector that covers energy consumers."@en,
        
            Annotations: <http://purl.obolibrary.org/obo/IAO_0000233> "issue: https://github.com/OpenEnergyPlatform/ontology/issues/1014
pull request: https://github.com/OpenEnergyPlatform/ontology/pull/1015"
        <http://purl.obolibrary.org/obo/IAO_0000118> "final energy sector",
        <http://purl.obolibrary.org/obo/IAO_0000233> "issue: https://github.com/OpenEnergyPlatform/ontology/issues/30
pull request: https://github.com/OpenEnergyPlatform/ontology/pull/484

move to oeo-sector 
issue: https://github.com/OpenEnergyPlatform/ontology/issues/1399
pull request: https://github.com/OpenEnergyPlatform/ontology/pull/1724",
        rdfs:label "energy demand sector"@en
    
    SubClassOf: 
        OEO_00000367
    
    
Class: OEO_00000145

    Annotations: 
        <http://purl.obolibrary.org/obo/IAO_0000115> "An electricity sector is a transformation sector that covers electricity generation and transport of electrical energy to consumers of electrical energy."@en,
        <http://purl.obolibrary.org/obo/IAO_0000233> "issue: https://github.com/OpenEnergyPlatform/ontology/issues/30
pull request: https://github.com/OpenEnergyPlatform/ontology/pull/484

move to oeo-sector 
issue: https://github.com/OpenEnergyPlatform/ontology/issues/1399
pull request: https://github.com/OpenEnergyPlatform/ontology/pull/1724",
        rdfs:label "electricity sector"@en
    
    SubClassOf: 
        OEO_00000158
    
    
Class: OEO_00000158

    Annotations: 
        <http://purl.obolibrary.org/obo/IAO_0000115> "An energy transformation sector is a sector that covers energy production, energy transformation from primary to secondary energy and transport of energy to the demand sector.",
        <http://purl.obolibrary.org/obo/IAO_0000118> "energy industry sector",
        <http://purl.obolibrary.org/obo/IAO_0000118> "energy sector",
        <http://purl.obolibrary.org/obo/IAO_0000233> "issue: https://github.com/OpenEnergyPlatform/ontology/issues/30
pull request: https://github.com/OpenEnergyPlatform/ontology/pull/484

move to oeo-sector 
issue: https://github.com/OpenEnergyPlatform/ontology/issues/1399
pull request: https://github.com/OpenEnergyPlatform/ontology/pull/1724",
        rdfs:label "energy transformation sector"@en
    
    SubClassOf: 
        OEO_00000367
    
    
Class: OEO_00000213

    Annotations: 
        <http://purl.obolibrary.org/obo/IAO_0000115> "A heating and cooling sector is a sector that covers heating and cooling activities."@en,
        <http://purl.obolibrary.org/obo/IAO_0000118> "H&C sector",
        <http://purl.obolibrary.org/obo/IAO_0000233> "issue: https://github.com/OpenEnergyPlatform/ontology/issues/30
pull request: https://github.com/OpenEnergyPlatform/ontology/pull/484

move to oeo-sector 
issue: https://github.com/OpenEnergyPlatform/ontology/issues/1399
pull request: https://github.com/OpenEnergyPlatform/ontology/pull/1724",
        rdfs:label "heating and cooling sector"@en
    
    SubClassOf: 
        OEO_00000128
    
    
Class: OEO_00000214

    Annotations: 
        <http://purl.obolibrary.org/obo/IAO_0000115> "A household sector is a sector that covers households."@en,
        <http://purl.obolibrary.org/obo/IAO_0000118> "private household sector",
        <http://purl.obolibrary.org/obo/IAO_0000233> "issue: https://github.com/OpenEnergyPlatform/ontology/issues/30
pull request: https://github.com/OpenEnergyPlatform/ontology/pull/484

move to oeo-sector 
issue: https://github.com/OpenEnergyPlatform/ontology/issues/1399
pull request: https://github.com/OpenEnergyPlatform/ontology/pull/1724",
        rdfs:label "household sector"@en
    
    SubClassOf: 
        OEO_00000128
    
    
Class: OEO_00000227

    Annotations: 
        <http://purl.obolibrary.org/obo/IAO_0000115> "An industry sector is a sector that covers industrial activities with other main purposes of energy transformation."@en,
        <http://purl.obolibrary.org/obo/IAO_0000233> "issue: https://github.com/OpenEnergyPlatform/ontology/issues/30
pull request: https://github.com/OpenEnergyPlatform/ontology/pull/484

move to oeo-sector 
issue: https://github.com/OpenEnergyPlatform/ontology/issues/1399
pull request: https://github.com/OpenEnergyPlatform/ontology/pull/1724",
        rdfs:label "industry sector"@en
    
    SubClassOf: 
        OEO_00000367
    
    
Class: OEO_00000323

    
Class: OEO_00000350

    
Class: OEO_00000367

    Annotations: 
        <http://purl.obolibrary.org/obo/IAO_0000115> "A sector is generically dependent continuant that is a subdivision of a system."@en,
        <http://purl.obolibrary.org/obo/IAO_0000233> "issue: https://github.com/OpenEnergyPlatform/ontology/issues/30
pull request: https://github.com/OpenEnergyPlatform/ontology/pull/477
moved to oeo-shared
pull request: https://github.com/OpenEnergyPlatform/ontology/pull/764
rework module structure 
issue: https://github.com/OpenEnergyPlatform/ontology/issues/1592
pull request: https://github.com/OpenEnergyPlatform/ontology/pull/1652
move to oeo-sector 
issue: https://github.com/OpenEnergyPlatform/ontology/issues/1399
pull request: https://github.com/OpenEnergyPlatform/ontology/pull/1724",
        rdfs:label "sector"@en
    
    SubClassOf: 
        <http://purl.obolibrary.org/obo/BFO_0000031>
    
    
Class: OEO_00000368

    Annotations: 
        <http://purl.obolibrary.org/obo/IAO_0000115> "A sector division is a specific way to subdivide a system."@en,
        <http://purl.obolibrary.org/obo/IAO_0000233> "issue: https://github.com/OpenEnergyPlatform/ontology/issues/30

Move to oeo-shared:
issue: https://github.com/OpenEnergyPlatform/ontology/issues/1400
pull request: https://github.com/OpenEnergyPlatform/ontology/pull/1463

Add relation to organisation or person:
issue: https://github.com/OpenEnergyPlatform/ontology/issues/1449
pull request: https://github.com/OpenEnergyPlatform/ontology/pull/1506

rework module structure 
issue: https://github.com/OpenEnergyPlatform/ontology/issues/1592
pull request: https://github.com/OpenEnergyPlatform/ontology/pull/1652

move to oeo-sector 
issue: https://github.com/OpenEnergyPlatform/ontology/issues/1399
pull request: https://github.com/OpenEnergyPlatform/ontology/pull/1724",
        rdfs:label "sector division"@en
    
    SubClassOf: 
        <http://purl.obolibrary.org/obo/BFO_0000031>,
        OEO_00000504 some 
            (OEO_00000323 or OEO_00030022)
    
    
Class: OEO_00000405

    Annotations: 
        <http://purl.obolibrary.org/obo/IAO_0000115> "A commercial sector is a sector that covers non-industrial commercial activities."@en,
        <http://purl.obolibrary.org/obo/IAO_0000118> "TCS sector",
        <http://purl.obolibrary.org/obo/IAO_0000118> "service sector",
        <http://purl.obolibrary.org/obo/IAO_0000118> "trading, commerce and service sector",
        <http://purl.obolibrary.org/obo/IAO_0000233> "issue: https://github.com/OpenEnergyPlatform/ontology/issues/30
pull request: https://github.com/OpenEnergyPlatform/ontology/pull/484

move to oeo-sector 
issue: https://github.com/OpenEnergyPlatform/ontology/issues/1399
pull request: https://github.com/OpenEnergyPlatform/ontology/pull/1724",
        rdfs:label "commercial sector"@en
    
    SubClassOf: 
        OEO_00000128
    
    
Class: OEO_00000422

    Annotations: 
        <http://purl.obolibrary.org/obo/IAO_0000115> "A transport sector is a sector that covers transport of people and/or goods."@en,
        <http://purl.obolibrary.org/obo/IAO_0000118> "traffic sector",
        <http://purl.obolibrary.org/obo/IAO_0000233> "issue: https://github.com/OpenEnergyPlatform/ontology/issues/30
pull request: https://github.com/OpenEnergyPlatform/ontology/pull/484

move to oeo-sector 
issue: https://github.com/OpenEnergyPlatform/ontology/issues/1399
pull request: https://github.com/OpenEnergyPlatform/ontology/pull/1724",
        rdfs:label "transport sector"@en
    
    SubClassOf: 
        OEO_00000128
    
    
Class: OEO_00010034

    Annotations: 
        <http://purl.obolibrary.org/obo/IAO_0000115> "A building sector is a sector that covers buildings.",
        <http://purl.obolibrary.org/obo/IAO_0000233> "issue: https://github.com/OpenEnergyPlatform/ontology/issues/30
pull request: https://github.com/OpenEnergyPlatform/ontology/pull/484

move to oeo-sector 
issue: https://github.com/OpenEnergyPlatform/ontology/issues/1399
pull request: https://github.com/OpenEnergyPlatform/ontology/pull/1724",
        rdfs:label "building sector"@en
    
    SubClassOf: 
        OEO_00000128
    
    
Class: OEO_00010035

    Annotations: 
        <http://purl.obolibrary.org/obo/IAO_0000115> "A agriculture, forestry and land use (AFOLU) sector is a sector that covers activities and natural processes from agriculture, forestry, land use and land use change.",
        <http://purl.obolibrary.org/obo/IAO_0000118> "AFOLU sector",
        <http://purl.obolibrary.org/obo/IAO_0000233> "issue: https://github.com/OpenEnergyPlatform/ontology/issues/30
pull request: https://github.com/OpenEnergyPlatform/ontology/pull/484

move to oeo-sector 
issue: https://github.com/OpenEnergyPlatform/ontology/issues/1399
pull request: https://github.com/OpenEnergyPlatform/ontology/pull/1724",
        rdfs:label "agriculture, forestry and land use sector"@en
    
    SubClassOf: 
        OEO_00000367
    
    
Class: OEO_00010036

    Annotations: 
        <http://purl.obolibrary.org/obo/IAO_0000115> "A waste and wastewater sector is a sector that covers activities related the collection and treatment of waste and wastewater.",
        <http://purl.obolibrary.org/obo/IAO_0000233> "issue: https://github.com/OpenEnergyPlatform/ontology/issues/30
pull request: https://github.com/OpenEnergyPlatform/ontology/pull/484

move to oeo-sector 
issue: https://github.com/OpenEnergyPlatform/ontology/issues/1399
pull request: https://github.com/OpenEnergyPlatform/ontology/pull/1724",
        rdfs:label "waste and wastewater sector"@en
    
    SubClassOf: 
        OEO_00000367
    
    
Class: OEO_00010055

    Annotations: 
        <http://purl.obolibrary.org/obo/IAO_0000115> "The common reporting format (CRF) is a sector division used for compiling national inventory reports on greenhouse gas emissions and providing emission relevant data in so called CRF tables.",
        <http://purl.obolibrary.org/obo/IAO_0000118> "CRF",
        <http://purl.obolibrary.org/obo/IAO_0000118> "NIR sector division",
        <http://purl.obolibrary.org/obo/IAO_0000118> "national inventory report sector division",
        <http://purl.obolibrary.org/obo/IAO_0000233> "issue: https://github.com/OpenEnergyPlatform/ontology/issues/461
pull request: https://github.com/OpenEnergyPlatform/ontology/pull/578

add alternative labels:
issue: https://github.com/OpenEnergyPlatform/ontology/issues/1535
pull request: https://github.com/OpenEnergyPlatform/ontology/pull/1558

move to oeo-sector 
issue: https://github.com/OpenEnergyPlatform/ontology/issues/1399
pull request: https://github.com/OpenEnergyPlatform/ontology/pull/1724",
        rdfs:label "common reporting format"@en
    
    SubClassOf: 
        OEO_00000368
    
    
Class: OEO_00010116

    
Class: OEO_00010117

    
Class: OEO_00010130

    Annotations: 
        <http://purl.obolibrary.org/obo/IAO_0000115> "An EU emission sector division is used in the EU climate policy.",
        <http://purl.obolibrary.org/obo/IAO_0000233> "issue: https://github.com/OpenEnergyPlatform/ontology/issues/834
pull request: https://github.com/OpenEnergyPlatform/ontology/pull/857

Convert to class:
issue: https://github.com/OpenEnergyPlatform/ontology/issues/1449
pull request: https://github.com/OpenEnergyPlatform/ontology/pull/1462

move to oeo-sector 
issue: https://github.com/OpenEnergyPlatform/ontology/issues/1399
pull request: https://github.com/OpenEnergyPlatform/ontology/pull/1724",
        rdfs:label "EU emission sector division"@en
    
    SubClassOf: 
        OEO_00000368
    
    
Class: OEO_00010227

    Annotations: 
        <http://purl.obolibrary.org/obo/IAO_0000115> "A memo item is an information content entity about a sector that describes that the sector is excluded from some kind of total and only reported to provide further information (memo).",
        <http://purl.obolibrary.org/obo/IAO_0000233> "issue: https://github.com/OpenEnergyPlatform/ontology/issues/858
pull request: https://github.com/OpenEnergyPlatform/ontology/pull/967

move to oeo-sector 
issue: https://github.com/OpenEnergyPlatform/ontology/issues/1399
pull request: https://github.com/OpenEnergyPlatform/ontology/pull/1724",
        rdfs:label "memo item"@en
    
    SubClassOf: 
        <http://purl.obolibrary.org/obo/IAO_0000030>,
        <http://purl.obolibrary.org/obo/IAO_0000136> some OEO_00000367
    
    
Class: OEO_00010304

    Annotations: 
        <http://purl.obolibrary.org/obo/IAO_0000115> "The NC/BR sector division is a CRF-based sector division defined by the UNFCCC reporting guidelines on national communications for Parties included in Annex I to the Convention.
(https://unfccc.int/sites/default/files/resource/cp2019_13a01_adv.pdf, 6/CP.25, VI, Table 2)",
        <http://purl.obolibrary.org/obo/IAO_0000233> "issue: https://github.com/OpenEnergyPlatform/ontology/issues/1273
pull request: https://github.com/OpenEnergyPlatform/ontology/pull/1317

Convert to class:
issue: https://github.com/OpenEnergyPlatform/ontology/issues/1449
pull request: https://github.com/OpenEnergyPlatform/ontology/pull/1462

move to oeo-sector 
issue: https://github.com/OpenEnergyPlatform/ontology/issues/1399
pull request: https://github.com/OpenEnergyPlatform/ontology/pull/1724",
        rdfs:label "NC/BR sector division"@en
    
    SubClassOf: 
        OEO_00010402
    
    
Class: OEO_00010319

    Annotations: 
        <http://purl.obolibrary.org/obo/IAO_0000115> "A mineral oil refining sector is an energy transformation sector that covers mineral oil refining.",
        <http://purl.obolibrary.org/obo/IAO_0000233> "issue: https://github.com/OpenEnergyPlatform/ontology/issues/1318
pull request: https://github.com/OpenEnergyPlatform/ontology/pull/1331

move axiom to shared-axioms
issue: https://github.com/OpenEnergyPlatform/ontology/issues/1703
pull request: https://github.com/OpenEnergyPlatform/ontology/pull/1706

move to oeo-sector 
issue: https://github.com/OpenEnergyPlatform/ontology/issues/1399
pull request: https://github.com/OpenEnergyPlatform/ontology/pull/1724",
        rdfs:label "mineral oil refining sector"@en
    
    SubClassOf: 
        OEO_00000158
    
    
Class: OEO_00010320

    Annotations: 
        <http://purl.obolibrary.org/obo/IAO_0000115> "An international transport sector is a transport sector of international transport processes.",
        <http://purl.obolibrary.org/obo/IAO_0000233> "issue: https://github.com/OpenEnergyPlatform/ontology/issues/969
pull request: https://github.com/OpenEnergyPlatform/ontology/pull/1334

move axiom to shared-axioms
issue: https://github.com/OpenEnergyPlatform/ontology/issues/1703
pull request: https://github.com/OpenEnergyPlatform/ontology/pull/1706

move to oeo-sector 
issue: https://github.com/OpenEnergyPlatform/ontology/issues/1399
pull request: https://github.com/OpenEnergyPlatform/ontology/pull/1724",
        rdfs:label "international transport sector"@en
    
    SubClassOf: 
        OEO_00000422
    
    
Class: OEO_00010360

    Annotations: 
        <http://purl.obolibrary.org/obo/IAO_0000115> "A source category is a sector that is defined by a common reporting format.",
        <http://purl.obolibrary.org/obo/IAO_0000118> "CRF sector",
        <http://purl.obolibrary.org/obo/IAO_0000233> "issue: https://github.com/OpenEnergyPlatform/ontology/issues/1426
pull request: https://github.com/OpenEnergyPlatform/ontology/pull/1428

move to oeo-sector 
issue: https://github.com/OpenEnergyPlatform/ontology/issues/1399
pull request: https://github.com/OpenEnergyPlatform/ontology/pull/1724",
        rdfs:label "source category"@en
    
    EquivalentTo: 
        OEO_00000367
         and (OEO_00000504 some OEO_00010055)
    
    SubClassOf: 
        OEO_00000367
    
    
Class: OEO_00010402

    Annotations: 
        <http://purl.obolibrary.org/obo/IAO_0000115> "A CRF-based sector division is a sector division that is derived from a common reporting format.",
        <http://purl.obolibrary.org/obo/IAO_0000233> "issue: https://github.com/OpenEnergyPlatform/ontology/issues/1449
pull request: https://github.com/OpenEnergyPlatform/ontology/pull/1462

move to oeo-sector 
issue: https://github.com/OpenEnergyPlatform/ontology/issues/1399
pull request: https://github.com/OpenEnergyPlatform/ontology/pull/1724",
        rdfs:label "CRF-based sector division"@en
    
    EquivalentTo: 
        OEO_00000368
         and (OEO_00000503 some OEO_00010055)
    
    SubClassOf: 
        OEO_00000368
    
    
Class: OEO_00010403

    Annotations: 
        <http://purl.obolibrary.org/obo/IAO_0000115> "An EU legislation sector division is a sector division that is used in EU legislation.",
        <http://purl.obolibrary.org/obo/IAO_0000233> "issue: https://github.com/OpenEnergyPlatform/ontology/issues/1449
pull request: https://github.com/OpenEnergyPlatform/ontology/pull/1462

move to oeo-sector 
issue: https://github.com/OpenEnergyPlatform/ontology/issues/1399
pull request: https://github.com/OpenEnergyPlatform/ontology/pull/1724",
        rdfs:label "EU legislation sector division"@en
    
    SubClassOf: 
        OEO_00000368
    
    
Class: OEO_00010407

    Annotations: 
        <http://purl.obolibrary.org/obo/IAO_0000115> "An energy balance sector division is a sector division that is defined by an energy balance calculation method.",
        <http://purl.obolibrary.org/obo/IAO_0000233> "issue: https://github.com/OpenEnergyPlatform/ontology/issues/1400
pull request: https://github.com/OpenEnergyPlatform/ontology/pull/1463
rework module structure 
issue: https://github.com/OpenEnergyPlatform/ontology/issues/1592
pull request: https://github.com/OpenEnergyPlatform/ontology/pull/1652
move to oeo-sector 
issue: https://github.com/OpenEnergyPlatform/ontology/issues/1399
pull request: https://github.com/OpenEnergyPlatform/ontology/pull/1724",
        rdfs:label "energy balance sector division"@en
    
    SubClassOf: 
        OEO_00000368
    
    
Class: OEO_00020015

    
Class: OEO_00030022

    
Class: OEO_00030035

    
Class: OEO_00090001

    
Class: OEO_00140009

    
Class: OEO_00140012

    
Individual: OEO_00000160

    Annotations: 
        <http://purl.obolibrary.org/obo/IAO_0000115> "The concept of \"energy balance\" is an accounting framework for the compilation and understanding of data on all energy products entering, exiting and being used in a country. The energy balance is the most complete statistical accounting of energy products and their flow in the economy. Columns of the energy balance represent energy products (fuels). Rows represent energy flows.

The energy balance expresses all forms of energy in a common accounting unit. The balance shows the relationships between supply, inputs to the energy transformation processes and their outputs as well as the actual energy consumption by different sectors of end-use.",
        <http://purl.obolibrary.org/obo/IAO_0000116> "This is a general description of an energy balance. A link to a complete Eurostat energy balance is provided under the URL for 'definition source'",
        <http://purl.obolibrary.org/obo/IAO_0000119> "https://ec.europa.eu/eurostat/statistics-explained/index.php/Energy_balance#What_is_an_energy_balance.3F",
        <http://purl.obolibrary.org/obo/IAO_0000233> "Change type and label:
issue: https://github.com/OpenEnergyPlatform/ontology/issues/1400
pull request: https://github.com/OpenEnergyPlatform/ontology/pull/1463
move to oeo-sector 
issue: https://github.com/OpenEnergyPlatform/ontology/issues/1399
pull request: https://github.com/OpenEnergyPlatform/ontology/pull/1724",
        rdfs:label "Eurostat energy balance sector division"@en
    
    Types: 
        OEO_00010407
    
    
Individual: OEO_00000193

    Annotations: 
        <http://purl.obolibrary.org/obo/IAO_0000115> "Das Schema der Energiebilanzen umfasst eine Matrix von 33 Spalten und 68 Zeilen (einschließlich der Summenspalten und -zeilen). In der horizontalen Gliederung (Spalten) werden die Energieträger ausgewiesen, die der energetischen und nichtenergetischen Nutzung dienen. In der vertikalen Gliederung (Zeilen) werden für die jeweiligen Energieträger Aufkommen, Umwandlung und Verwendung erfasst.

Als Energieträger werden alle Quellen oder Stoffe bezeichnet, in denen Energie mechanisch, thermisch, chemisch oder physikalisch gespeichert ist. Fünf Kerngruppe werden bei der Energiebilanz unterschieden:

    Fossile Brennstoffe
    Erneuerbare Energien
    Strom
    Kernbrennstoffe
    Fernwärme

Bilanzebenen
Schematische Darstellung des Bilanzraums der deutschen Arbeitsgemeinschaft Energiebilanzen
Primär- und Endenergie sowie Umwandlungsverluste

Die Abgrenzung erfolgt in drei Bilanzbereichen:

    die Primärenergiebilanz,
    die Umwandlungsbilanz und
    der Endenergieverbrauch.

In der Primärenergiebilanz werden die Energieträger mit ihrem Mengenaufkommen bei der Gewinnung und Anlieferung nach folgenden Kriterien erfasst:

    inländische Gewinnung von Energieträgern,
    Außenhandel mit Energieträgern, unterteilt nach Einfuhr und Ausfuhr,
    Hochseebunkerungen (Heizöl, Dieselkraftstoff und Schmierstoffe für die nationale und internationale Seeschifffahrt in deutschen Häfen. Ohne Lieferungen an Binnen- und Küstenmotorschiffe und Fischerei, die zum Sektor Verkehr (Endenergieverbrauch) zählen.)
    Bestandsveränderungen, getrennt erfasst nach Bestandsentnahmen und -aufstockungen",
        <http://purl.obolibrary.org/obo/IAO_0000116> "The German Energy Balance is managed by the 'AG Energiebilanzen', where aso the energy balances can be found: https://ag-energiebilanzen.de/",
        <http://purl.obolibrary.org/obo/IAO_0000119> "https://de.wikipedia.org/w/index.php?title=Energiebilanz_(Energiewirtschaft)&oldid=176259115",
        <http://purl.obolibrary.org/obo/IAO_0000233> "Change type and label:
issue: https://github.com/OpenEnergyPlatform/ontology/issues/1400
pull request: https://github.com/OpenEnergyPlatform/ontology/pull/1463

move to oeo-sector 
issue: https://github.com/OpenEnergyPlatform/ontology/issues/1399
pull request: https://github.com/OpenEnergyPlatform/ontology/pull/1724",
        rdfs:label "German energy balance sector division"@en
    
    Types: 
        OEO_00010407
    
    
Individual: OEO_00000242

    Annotations: 
        <http://purl.obolibrary.org/obo/IAO_0000115> "CRF sectors (IPCC 2006) is a version of the common reporting format that was used for national greenhouse gas inventories since the year 2015. It implements the 2006 IPCC Guidelines for National Greenhouse Gas Inventories (with some deviations).",
        <http://purl.obolibrary.org/obo/IAO_0000233> "issue: https://github.com/OpenEnergyPlatform/ontology/issues/461
pull request: https://github.com/OpenEnergyPlatform/ontology/pull/578

move to oeo-sector 
issue: https://github.com/OpenEnergyPlatform/ontology/issues/1399
pull request: https://github.com/OpenEnergyPlatform/ontology/pull/1724",
        rdfs:label "CRF sectors (IPCC 2006)"@en
    
    Types: 
        OEO_00010055
    
    Facts:  
     OEO_00000504  OEO_00000242
    
    
Individual: OEO_00000243

    Annotations: 
        <http://purl.obolibrary.org/obo/IAO_0000115> "CRF sectors (IPCC 1996) is a version of the common reporting format that was used for national greenhouse gas inventories until the year 2014. It implements the Revised 1996 IPCC Guidelines for National Greenhouse Gas Inventories (with some deviations).",
        <http://purl.obolibrary.org/obo/IAO_0000233> "issue: https://github.com/OpenEnergyPlatform/ontology/issues/461
pull request: https://github.com/OpenEnergyPlatform/ontology/pull/578

move to oeo-sector 
issue: https://github.com/OpenEnergyPlatform/ontology/issues/1399
pull request: https://github.com/OpenEnergyPlatform/ontology/pull/1724",
        rdfs:label "CRF sectors (IPCC 1996)"@en
    
    Types: 
        OEO_00010055
    
    
Individual: OEO_00000291

    Annotations: 
        <http://purl.obolibrary.org/obo/IAO_0000115> "The Statistical classification of economic activities in the European Community, abbreviated as NACE, is the classification of economic activities in the European Union (EU); the term NACE is derived from the French Nomenclature statistique des activités économiques dans la Communauté européenne. Various NACE versions have been developed since 1970.

NACE is a four-digit classification providing the framework for collecting and presenting a large range of statistical data according to economic activity in the fields of economic statistics (e.g. production, employment and national accounts) and in other statistical domains developed within the European statistical system (ESS).",
        <http://purl.obolibrary.org/obo/IAO_0000119> "https://ec.europa.eu/eurostat/statistics-explained/index.php?title=Glossary:Statistical_classification_of_economic_activities_in_the_European_Community_(NACE)",
        <http://purl.obolibrary.org/obo/IAO_0000233> "move to oeo-sector issue: https://github.com/OpenEnergyPlatform/ontology/issues/1399
pull request: https://github.com/OpenEnergyPlatform/ontology/pull/1724",
        rdfs:label "nace_ sectors"@en
    
    Types: 
        OEO_00000368
    
    
Individual: OEO_00000355

    Annotations: 
        <http://purl.obolibrary.org/obo/IAO_0000115> "The Renewable Energy Directive sector division is a sector division used in the Renewable Energy Directive of the European Union.",
        <http://purl.obolibrary.org/obo/IAO_0000116> "The Renewable energy Directive has been revised, but this should have had no impacts on the sectoral definitions. Factsheet on revision: https://ec.europa.eu/energy/sites/ener/files/documents/directive_renewable_factsheet.pdf",
        <http://purl.obolibrary.org/obo/IAO_0000119> "https://eur-lex.europa.eu/legal-content/EN/ALL/?uri=CELEX:32009L0028",
        <http://purl.obolibrary.org/obo/IAO_0000233> "Relabel and add definition:
issue: https://github.com/OpenEnergyPlatform/ontology/issues/1443
pull request: https://github.com/OpenEnergyPlatform/ontology/pull/1446

Make instance of 'EU legislation sector division':
issue: https://github.com/OpenEnergyPlatform/ontology/issues/1449
pull request: https://github.com/OpenEnergyPlatform/ontology/pull/1462

move to oeo-sector 
issue: https://github.com/OpenEnergyPlatform/ontology/issues/1399
pull request: https://github.com/OpenEnergyPlatform/ontology/pull/1724",
        rdfs:label "Renewable Energy Directive sector division"@en
    
    Types: 
        OEO_00010403
    
    
Individual: OEO_00010038

    Annotations: 
        OEO_00010037 "CRF 1",
        <http://purl.obolibrary.org/obo/IAO_0000115> "The CRF sector (IPCC 2006) energy is a sector defined by the 2006 IPCC Guidelines for National Greenhouse Gas Inventories:
All GHG emissions arising from combustion and fugitive releases of fuels. Emissions from the non-energy uses of fuels are generally not included here, but reported under Industrial Processes and Product Use.",
        <http://purl.obolibrary.org/obo/IAO_0000119> "2006 IPCC Guidelines for National Greenhouse Gas Inventories, Volume 2, Chapter 2.2, https://www.ipcc-nggip.iges.or.jp/public/2006gl/",
        <http://purl.obolibrary.org/obo/IAO_0000233> "issue: https://github.com/OpenEnergyPlatform/ontology/issues/461
pull request: https://github.com/OpenEnergyPlatform/ontology/pull/523

move to oeo-sector 
issue: https://github.com/OpenEnergyPlatform/ontology/issues/1399
pull request: https://github.com/OpenEnergyPlatform/ontology/pull/1724",
        rdfs:label "CRF sector (IPCC 2006): energy"@en
    
    Types: 
        OEO_00000367
    
    Facts:  
     OEO_00000504  OEO_00000242,
     <http://purl.obolibrary.org/obo/BFO_0000051>  OEO_00010040,
     <http://purl.obolibrary.org/obo/BFO_0000051>  OEO_00010041,
     <http://purl.obolibrary.org/obo/BFO_0000051>  OEO_00010042,
     <http://purl.obolibrary.org/obo/BFO_0000051>  OEO_00010043,
     <http://purl.obolibrary.org/obo/BFO_0000051>  OEO_00010044
    
    
Individual: OEO_00010039

    Annotations: 
        OEO_00010037 "CRF 1.A",
        <http://purl.obolibrary.org/obo/IAO_0000115> "The CRF sector (IPCC 2006) 'fuel combustion' is a sector defined by the 2006 IPCC Guidelines for National Greenhouse Gas Inventories:
Emissions from the intentional oxidation of materials within an apparatus that is designed to raise heat and provide it either as heat or as mechanical work to a process or for use away from the apparatus.",
        <http://purl.obolibrary.org/obo/IAO_0000119> "2006 IPCC Guidelines for National Greenhouse Gas Inventories, Volume 2, Chapter 2.2, https://www.ipcc-nggip.iges.or.jp/public/2006gl/",
        <http://purl.obolibrary.org/obo/IAO_0000233> "issue: https://github.com/OpenEnergyPlatform/ontology/issues/461
pull request: https://github.com/OpenEnergyPlatform/ontology/pull/523

move to oeo-sector 
issue: https://github.com/OpenEnergyPlatform/ontology/issues/1399
pull request: https://github.com/OpenEnergyPlatform/ontology/pull/1724",
        rdfs:label "CRF sector (IPCC 2006): fuel combustion"@en
    
    Types: 
        OEO_00000367
    
    Facts:  
     OEO_00000504  OEO_00000242,
     <http://purl.obolibrary.org/obo/BFO_0000050>  OEO_00010038
    
    
Individual: OEO_00010040

    Annotations: 
        OEO_00010037 "CRF 1.A.1",
        <http://purl.obolibrary.org/obo/IAO_0000115> "The CRF sector (IPCC 2006) 'energy industry' is an energy transformation sector defined by the 2006 IPCC Guidelines for National Greenhouse Gas Inventories:
Comprises emissions from fuels combusted by the fuel extraction or energy-producing industries.",
        <http://purl.obolibrary.org/obo/IAO_0000119> "2006 IPCC Guidelines for National Greenhouse Gas Inventories, Volume 2, Chapter 2.2, https://www.ipcc-nggip.iges.or.jp/public/2006gl/",
        <http://purl.obolibrary.org/obo/IAO_0000233> "issue: https://github.com/OpenEnergyPlatform/ontology/issues/461
pull request: https://github.com/OpenEnergyPlatform/ontology/pull/523

add has part relations:
issue: https://github.com/OpenEnergyPlatform/ontology/issues/858
pull request: https://github.com/OpenEnergyPlatform/ontology/pull/941

move to oeo-sector 
issue: https://github.com/OpenEnergyPlatform/ontology/issues/1399
pull request: https://github.com/OpenEnergyPlatform/ontology/pull/1724",
        rdfs:label "CRF sector (IPCC 2006): energy industry"@en
    
    Types: 
        OEO_00000158
    
    Facts:  
     OEO_00000504  OEO_00000242,
     <http://purl.obolibrary.org/obo/BFO_0000050>  OEO_00010039,
     <http://purl.obolibrary.org/obo/BFO_0000051>  OEO_00010158,
     <http://purl.obolibrary.org/obo/BFO_0000051>  OEO_00010159,
     <http://purl.obolibrary.org/obo/BFO_0000051>  OEO_00010160
    
    
Individual: OEO_00010041

    Annotations: 
        OEO_00010037 "CRF 1.A.2",
        <http://purl.obolibrary.org/obo/IAO_0000115> "The CRF sector (IPCC 2006) 'manufacturing industries and construction' is an industry sector defined by the 2006 IPCC Guidelines for National Greenhouse Gas Inventories:
Emissions from combustion of fuels in industry. Also includes combustion for the generation of electricity and heat for own use in these industries.",
        <http://purl.obolibrary.org/obo/IAO_0000119> "2006 IPCC Guidelines for National Greenhouse Gas Inventories, Volume 2, Chapter 2.2, https://www.ipcc-nggip.iges.or.jp/public/2006gl/",
        <http://purl.obolibrary.org/obo/IAO_0000233> "issue: https://github.com/OpenEnergyPlatform/ontology/issues/461
pull request: https://github.com/OpenEnergyPlatform/ontology/pull/523

move to oeo-sector 
issue: https://github.com/OpenEnergyPlatform/ontology/issues/1399
pull request: https://github.com/OpenEnergyPlatform/ontology/pull/1724",
        rdfs:label "CRF sector (IPCC 2006): manufacturing industries and construction"@en
    
    Types: 
        OEO_00000227
    
    Facts:  
     OEO_00000504  OEO_00000242,
     <http://purl.obolibrary.org/obo/BFO_0000050>  OEO_00010039
    
    
Individual: OEO_00010042

    Annotations: 
        OEO_00010037 "CRF 1.A.3",
        <http://purl.obolibrary.org/obo/IAO_0000115> "The CRF sector (IPCC 2006) 'transport' is a transport sector defined by the 2006 IPCC Guidelines for National Greenhouse Gas Inventories:
Emissions from the combustion and evaporation of fuel for all transport activity (excluding military transport), regardless of the sector, specified by sub-categories below. Emissions from fuel sold to any air or marine vessel engaged in international transport (1 A 3 a i and 1 A 3 d i) should as far as possible be excluded from the totals and subtotals in this category and should be reported separately.",
        <http://purl.obolibrary.org/obo/IAO_0000119> "2006 IPCC Guidelines for National Greenhouse Gas Inventories, Volume 2, Chapter 3.1, https://www.ipcc-nggip.iges.or.jp/public/2006gl/",
        <http://purl.obolibrary.org/obo/IAO_0000233> "issue: https://github.com/OpenEnergyPlatform/ontology/issues/461
pull request: https://github.com/OpenEnergyPlatform/ontology/pull/523

move to oeo-sector 
issue: https://github.com/OpenEnergyPlatform/ontology/issues/1399
pull request: https://github.com/OpenEnergyPlatform/ontology/pull/1724",
        rdfs:label "CRF sector (IPCC 2006): transport"@en
    
    Types: 
        OEO_00000422
    
    Facts:  
     OEO_00000504  OEO_00000242,
     <http://purl.obolibrary.org/obo/BFO_0000050>  OEO_00010039
    
    SameAs: 
        OEO_00010306
    
    
Individual: OEO_00010043

    Annotations: 
        OEO_00010037 "CRF 1.A.4",
        <http://purl.obolibrary.org/obo/IAO_0000115> "The CRF sector (IPCC 2006) 'fuel combustion - other sectors' is an energy demand sector defined by the 2006 IPCC Guidelines for National Greenhouse Gas Inventories:
Emissions from combustion activities as described below, including combustion for the generation of electricity and heat for own use in these sectors.",
        <http://purl.obolibrary.org/obo/IAO_0000119> "2006 IPCC Guidelines for National Greenhouse Gas Inventories, Volume 2, Chapter 2.2, https://www.ipcc-nggip.iges.or.jp/public/2006gl/",
        <http://purl.obolibrary.org/obo/IAO_0000233> "issue: https://github.com/OpenEnergyPlatform/ontology/issues/461
pull request: https://github.com/OpenEnergyPlatform/ontology/pull/523

move to oeo-sector 
issue: https://github.com/OpenEnergyPlatform/ontology/issues/1399
pull request: https://github.com/OpenEnergyPlatform/ontology/pull/1724",
        rdfs:label "CRF sector (IPCC 2006): fuel combustion - other sectors"@en
    
    Types: 
        OEO_00000128
    
    Facts:  
     OEO_00000504  OEO_00000242,
     <http://purl.obolibrary.org/obo/BFO_0000050>  OEO_00010039,
     <http://purl.obolibrary.org/obo/BFO_0000051>  OEO_00010052,
     <http://purl.obolibrary.org/obo/BFO_0000051>  OEO_00010053
    
    
Individual: OEO_00010044

    Annotations: 
        OEO_00010037 "CRF 1.A.5",
        <http://purl.obolibrary.org/obo/IAO_0000115> "The CRF sector (IPCC 2006) 'fuel combustion' is a sector defined by the 2006 IPCC Guidelines for National Greenhouse Gas Inventories:
All remaining emissions from fuel combustion that are not specified elsewhere. Include emissions from fuel delivered to the military in the country and delivered to the military of other countries that are not engaged in multilateral operations.",
        <http://purl.obolibrary.org/obo/IAO_0000119> "2006 IPCC Guidelines for National Greenhouse Gas Inventories, Volume 2, Chapter 2.2, https://www.ipcc-nggip.iges.or.jp/public/2006gl/",
        <http://purl.obolibrary.org/obo/IAO_0000233> "issue: https://github.com/OpenEnergyPlatform/ontology/issues/461
pull request: https://github.com/OpenEnergyPlatform/ontology/pull/523

move to oeo-sector 
issue: https://github.com/OpenEnergyPlatform/ontology/issues/1399
pull request: https://github.com/OpenEnergyPlatform/ontology/pull/1724",
        rdfs:label "CRF sector (IPCC 2006): fuel combustion - other"@en
    
    Types: 
        OEO_00000367
    
    Facts:  
     OEO_00000504  OEO_00000242,
     <http://purl.obolibrary.org/obo/BFO_0000050>  OEO_00010039
    
    
Individual: OEO_00010046

    Annotations: 
        OEO_00010037 "CRF 2",
        <http://purl.obolibrary.org/obo/IAO_0000115> "The CRF sector (IPCC 2006) 'energy industrial processes and product use' (IPPU) is an industry sector defined by the 2006 IPCC Guidelines for National Greenhouse Gas Inventories:
It covers greenhouse gas emissions occurring from industrial processes, from the use of greenhouse gases in products, and from non-energy uses of fossil fuel carbon.",
        <http://purl.obolibrary.org/obo/IAO_0000118> "IPPU",
        <http://purl.obolibrary.org/obo/IAO_0000119> "2006 IPCC Guidelines for National Greenhouse Gas Inventories, Volume 3, Chapter 1.1, https://www.ipcc-nggip.iges.or.jp/public/2006gl/",
        <http://purl.obolibrary.org/obo/IAO_0000233> "issue: https://github.com/OpenEnergyPlatform/ontology/issues/461
pull request: https://github.com/OpenEnergyPlatform/ontology/pull/578

add has part relations:
issue: https://github.com/OpenEnergyPlatform/ontology/issues/858
pull request: https://github.com/OpenEnergyPlatform/ontology/pull/941

move to oeo-sector 
issue: https://github.com/OpenEnergyPlatform/ontology/issues/1399
pull request: https://github.com/OpenEnergyPlatform/ontology/pull/1724",
        rdfs:label "CRF sector (IPCC 2006): industrial processes and product use"@en
    
    Types: 
        OEO_00000227
    
    Facts:  
     OEO_00000504  OEO_00000242,
     <http://purl.obolibrary.org/obo/BFO_0000051>  OEO_00010164,
     <http://purl.obolibrary.org/obo/BFO_0000051>  OEO_00010166,
     <http://purl.obolibrary.org/obo/BFO_0000051>  OEO_00010167,
     <http://purl.obolibrary.org/obo/BFO_0000051>  OEO_00010169,
     <http://purl.obolibrary.org/obo/BFO_0000051>  OEO_00010170,
     <http://purl.obolibrary.org/obo/BFO_0000051>  OEO_00010171,
     <http://purl.obolibrary.org/obo/BFO_0000051>  OEO_00010172,
     <http://purl.obolibrary.org/obo/BFO_0000051>  OEO_00010173
    
    
Individual: OEO_00010047

    Annotations: 
        OEO_00010037 "CRF 3",
        <http://purl.obolibrary.org/obo/IAO_0000233> "issue: https://github.com/OpenEnergyPlatform/ontology/issues/461
pull request: https://github.com/OpenEnergyPlatform/ontology/pull/578

add has part axioms:
issue: https://github.com/OpenEnergyPlatform/ontology/issues/858
pull request: https://github.com/OpenEnergyPlatform/ontology/pull/941

move to oeo-sector 
issue: https://github.com/OpenEnergyPlatform/ontology/issues/1399
pull request: https://github.com/OpenEnergyPlatform/ontology/pull/1724",
        rdfs:comment "The CRF sector (IPCC 2006) 'agriculture' is an agriculture, forestry and land use sector defined by the 2006 IPCC Guidelines for National Greenhouse Gas Inventories",
        rdfs:label "CRF sector (IPCC 2006): agriculture"@en
    
    Types: 
        OEO_00010035
    
    Facts:  
     OEO_00000504  OEO_00000242,
     <http://purl.obolibrary.org/obo/BFO_0000051>  OEO_00010179,
     <http://purl.obolibrary.org/obo/BFO_0000051>  OEO_00010180,
     <http://purl.obolibrary.org/obo/BFO_0000051>  OEO_00010181,
     <http://purl.obolibrary.org/obo/BFO_0000051>  OEO_00010182,
     <http://purl.obolibrary.org/obo/BFO_0000051>  OEO_00010183,
     <http://purl.obolibrary.org/obo/BFO_0000051>  OEO_00010184,
     <http://purl.obolibrary.org/obo/BFO_0000051>  OEO_00010185,
     <http://purl.obolibrary.org/obo/BFO_0000051>  OEO_00010186,
     <http://purl.obolibrary.org/obo/BFO_0000051>  OEO_00010187,
     <http://purl.obolibrary.org/obo/BFO_0000051>  OEO_00010188
    
    SameAs: 
        OEO_00010308
    
    
Individual: OEO_00010048

    Annotations: 
        OEO_00010037 "CRF 4",
        <http://purl.obolibrary.org/obo/IAO_0000115> "The CRF sector (IPCC 2006) 'land use, land-use change and forestry' (LULUCF) is an agriculture, forestry and land use sector defined by the 2006 IPCC Guidelines for National Greenhouse Gas Inventories",
        <http://purl.obolibrary.org/obo/IAO_0000118> "LULUCF",
        <http://purl.obolibrary.org/obo/IAO_0000233> "issue: https://github.com/OpenEnergyPlatform/ontology/issues/461
pull request: https://github.com/OpenEnergyPlatform/ontology/pull/578

add has part axioms:
issue: https://github.com/OpenEnergyPlatform/ontology/issues/858
pull request: https://github.com/OpenEnergyPlatform/ontology/pull/941

move to oeo-sector 
issue: https://github.com/OpenEnergyPlatform/ontology/issues/1399
pull request: https://github.com/OpenEnergyPlatform/ontology/pull/1724",
        rdfs:label "CRF sector (IPCC 2006): land use, land-use change and forestry"@en
    
    Types: 
        OEO_00010035
    
    Facts:  
     OEO_00000504  OEO_00000242,
     <http://purl.obolibrary.org/obo/BFO_0000051>  OEO_00010189,
     <http://purl.obolibrary.org/obo/BFO_0000051>  OEO_00010190,
     <http://purl.obolibrary.org/obo/BFO_0000051>  OEO_00010192,
     <http://purl.obolibrary.org/obo/BFO_0000051>  OEO_00010193,
     <http://purl.obolibrary.org/obo/BFO_0000051>  OEO_00010194,
     <http://purl.obolibrary.org/obo/BFO_0000051>  OEO_00010195,
     <http://purl.obolibrary.org/obo/BFO_0000051>  OEO_00010196
    
    SameAs: 
        OEO_00010071,
        OEO_00010135,
        OEO_00010309
    
    
Individual: OEO_00010049

    Annotations: 
        OEO_00010037 "CRF 5",
        <http://purl.obolibrary.org/obo/IAO_0000115> "The CRF sector (IPCC 2006) 'waste' is a waste and wastewater sector defined by the 2006 IPCC Guidelines for National Greenhouse Gas Inventories:
Carbon dioxide (CO2), methane (CH4) and nitrous oxide (N2O) emissions from following categories: Solid waste disposal, Biological treatment of solid waste,
Incineration and open burning of waste, Wastewater treatment and discharge.",
        <http://purl.obolibrary.org/obo/IAO_0000119> "2006 IPCC Guidelines for National Greenhouse Gas Inventories, Volume 5, Chapter 1.1, https://www.ipcc-nggip.iges.or.jp/public/2006gl/",
        <http://purl.obolibrary.org/obo/IAO_0000233> "issue: https://github.com/OpenEnergyPlatform/ontology/issues/461
pull request: https://github.com/OpenEnergyPlatform/ontology/pull/578

add has part axioms and improve definition:
issue: https://github.com/OpenEnergyPlatform/ontology/issues/858
pull request: https://github.com/OpenEnergyPlatform/ontology/pull/941

move to oeo-sector 
issue: https://github.com/OpenEnergyPlatform/ontology/issues/1399
pull request: https://github.com/OpenEnergyPlatform/ontology/pull/1724",
        rdfs:label "CRF sector (IPCC 2006): waste"@en
    
    Types: 
        OEO_00010036
    
    Facts:  
     OEO_00000504  OEO_00000242,
     <http://purl.obolibrary.org/obo/BFO_0000051>  OEO_00010174,
     <http://purl.obolibrary.org/obo/BFO_0000051>  OEO_00010175,
     <http://purl.obolibrary.org/obo/BFO_0000051>  OEO_00010176,
     <http://purl.obolibrary.org/obo/BFO_0000051>  OEO_00010177,
     <http://purl.obolibrary.org/obo/BFO_0000051>  OEO_00010178
    
    SameAs: 
        OEO_00010310
    
    
Individual: OEO_00010050

    Annotations: 
        OEO_00010037 "CRF 6",
        <http://purl.obolibrary.org/obo/IAO_0000115> "The CRF sector (IPCC 2006) 'other' is a sector defined by the 2006 IPCC Guidelines for National Greenhouse Gas Inventories",
        <http://purl.obolibrary.org/obo/IAO_0000233> "issue: https://github.com/OpenEnergyPlatform/ontology/issues/461
pull request: https://github.com/OpenEnergyPlatform/ontology/pull/578

move to oeo-sector 
issue: https://github.com/OpenEnergyPlatform/ontology/issues/1399
pull request: https://github.com/OpenEnergyPlatform/ontology/pull/1724",
        rdfs:label "CRF sector (IPCC 2006): other"@en
    
    Types: 
        OEO_00000367
    
    Facts:  
     OEO_00000504  OEO_00000242
    
    SameAs: 
        OEO_00010311
    
    
Individual: OEO_00010052

    Annotations: 
        OEO_00010037 "CRF 1.A.4.a",
        <http://purl.obolibrary.org/obo/IAO_0000115> "The CRF sector (IPCC 2006) 'commercial and institutional' is a commercial sector defined by the 2006 IPCC Guidelines for National Greenhouse Gas Inventories:
Emissions from fuel combustion in commercial and institutional buildings.",
        <http://purl.obolibrary.org/obo/IAO_0000119> "2006 IPCC Guidelines for National Greenhouse Gas Inventories, Volume 3, Chapter 1.1, https://www.ipcc-nggip.iges.or.jp/public/2006gl/",
        <http://purl.obolibrary.org/obo/IAO_0000233> "issue: https://github.com/OpenEnergyPlatform/ontology/issues/461
pull request: https://github.com/OpenEnergyPlatform/ontology/pull/578

move to oeo-sector 
issue: https://github.com/OpenEnergyPlatform/ontology/issues/1399
pull request: https://github.com/OpenEnergyPlatform/ontology/pull/1724",
        rdfs:label "CRF sector (IPCC 2006): commercial and institutional"@en
    
    Types: 
        OEO_00000405
    
    Facts:  
     OEO_00000504  OEO_00000242,
     <http://purl.obolibrary.org/obo/BFO_0000050>  OEO_00010043
    
    
Individual: OEO_00010053

    Annotations: 
        OEO_00010037 "CRF 1.A.4.b",
        <http://purl.obolibrary.org/obo/IAO_0000115> "The CRF sector (IPCC 2006) 'residential' is a household sector defined by the 2006 IPCC Guidelines for National Greenhouse Gas Inventories:
All emissions from fuel combustion in households.",
        <http://purl.obolibrary.org/obo/IAO_0000119> "2006 IPCC Guidelines for National Greenhouse Gas Inventories, Volume 2, Chapter 2.2, https://www.ipcc-nggip.iges.or.jp/public/2006gl/",
        <http://purl.obolibrary.org/obo/IAO_0000233> "issue: https://github.com/OpenEnergyPlatform/ontology/issues/461
pull request: https://github.com/OpenEnergyPlatform/ontology/pull/578

move to oeo-sector 
issue: https://github.com/OpenEnergyPlatform/ontology/issues/1399
pull request: https://github.com/OpenEnergyPlatform/ontology/pull/1724",
        rdfs:label "CRF sector (IPCC 2006): residential"@en
    
    Types: 
        OEO_00000214
    
    Facts:  
     OEO_00000504  OEO_00000242,
     <http://purl.obolibrary.org/obo/BFO_0000050>  OEO_00010043
    
    
Individual: OEO_00010054

    Annotations: 
        OEO_00010037 "CRF 1.A.4.c",
        <http://purl.obolibrary.org/obo/IAO_0000115> "The CRF sector (IPCC 2006) 'agriculture, forestry and fishing' is an energy demand sector defined by the 2006 IPCC Guidelines for National Greenhouse Gas Inventories:
Emissions from fuel combustion in agriculture, forestry, fishing and fishing industries such as fish farms.",
        <http://purl.obolibrary.org/obo/IAO_0000119> "2006 IPCC Guidelines for National Greenhouse Gas Inventories, Volume 2, Chapter 2.2, https://www.ipcc-nggip.iges.or.jp/public/2006gl/",
        <http://purl.obolibrary.org/obo/IAO_0000233> "issue: https://github.com/OpenEnergyPlatform/ontology/issues/461
pull request: https://github.com/OpenEnergyPlatform/ontology/pull/578

move to oeo-sector 
issue: https://github.com/OpenEnergyPlatform/ontology/issues/1399
pull request: https://github.com/OpenEnergyPlatform/ontology/pull/1724",
        rdfs:label "CRF sector (IPCC 2006): agriculture, forestry and fishing"@en
    
    Types: 
        OEO_00000128
    
    Facts:  
     OEO_00000504  OEO_00000242,
     <http://purl.obolibrary.org/obo/BFO_0000050>  OEO_00010043
    
    
Individual: OEO_00010056

    Annotations: 
        <http://purl.obolibrary.org/obo/IAO_0000115> "The KSG sector division is a CRF-based sector division defined in annex 1 of the Bundes-Klimaschutzgesetz (KSG).",
        <http://purl.obolibrary.org/obo/IAO_0000233> "issue: https://github.com/OpenEnergyPlatform/ontology/issues/580
pull request: https://github.com/OpenEnergyPlatform/ontology/pull/595

Make instance of 'CRF-based sector division':
issue: https://github.com/OpenEnergyPlatform/ontology/issues/1449
pull request: https://github.com/OpenEnergyPlatform/ontology/pull/1462

move to oeo-sector 
issue: https://github.com/OpenEnergyPlatform/ontology/issues/1399
pull request: https://github.com/OpenEnergyPlatform/ontology/pull/1724",
        rdfs:label "KSG sector division"@en
    
    Types: 
        OEO_00010402
    
    
Individual: OEO_00010057

    Annotations: 
        OEO_00010037 "CRF 1.B",
        <http://purl.obolibrary.org/obo/IAO_0000115> "The CRF sector (IPCC 2006) 'fugitive emissions from fuels' is a sector defined by the 2006 IPCC Guidelines for National Greenhouse Gas Inventories:
Includes all intentional and unintentional emissions from the extraction, processing, storage and transport of solid fuel to the point of final use.",
        <http://purl.obolibrary.org/obo/IAO_0000119> "2006 IPCC Guidelines for National Greenhouse Gas Inventories, Volume 1, Chapter 8.5, https://www.ipcc-nggip.iges.or.jp/public/2006gl/",
        <http://purl.obolibrary.org/obo/IAO_0000233> "issue: https://github.com/OpenEnergyPlatform/ontology/issues/580
pull request: https://github.com/OpenEnergyPlatform/ontology/pull/595

move to oeo-sector 
issue: https://github.com/OpenEnergyPlatform/ontology/issues/1399
pull request: https://github.com/OpenEnergyPlatform/ontology/pull/1724",
        rdfs:label "CRF sector (IPCC 2006): fugitive emissions from fuels"@en
    
    Types: 
        OEO_00000367
    
    Facts:  
     OEO_00000504  OEO_00000242,
     <http://purl.obolibrary.org/obo/BFO_0000050>  OEO_00010038,
     <http://purl.obolibrary.org/obo/BFO_0000051>  OEO_00010161,
     <http://purl.obolibrary.org/obo/BFO_0000051>  OEO_00010162
    
    
Individual: OEO_00010058

    Annotations: 
        OEO_00010037 "CRF 1.C",
        <http://purl.obolibrary.org/obo/IAO_0000115> "The CRF sector (IPCC 2006) 'CO2 transport and storage' is a sector defined by the 2006 IPCC Guidelines for National Greenhouse Gas Inventories:
Carbon dioxide (CO2) capture and storage (CCS) involves the capture of CO2 from anthropogenic sources, its transport to a storage location and its long-term isolation from the atmosphere. Emissions associated with CO2 transport, injection and storage are covered under category 1C. Emissions (and reductions) associated with CO2 capture should be reported under the IPCC Sector in which capture takes place (e.g. Fuel Combustion or Industrial Activities).",
        <http://purl.obolibrary.org/obo/IAO_0000119> "2006 IPCC Guidelines for National Greenhouse Gas Inventories, Volume 1, Chapter 8.5, https://www.ipcc-nggip.iges.or.jp/public/2006gl/",
        <http://purl.obolibrary.org/obo/IAO_0000233> "issue: https://github.com/OpenEnergyPlatform/ontology/issues/580
pull request: https://github.com/OpenEnergyPlatform/ontology/pull/595

move to oeo-sector 
issue: https://github.com/OpenEnergyPlatform/ontology/issues/1399
pull request: https://github.com/OpenEnergyPlatform/ontology/pull/1724",
        rdfs:label "CRF sector (IPCC 2006): CO2 transport and storage"@en
    
    Types: 
        OEO_00000367
    
    Facts:  
     OEO_00000504  OEO_00000242,
     <http://purl.obolibrary.org/obo/BFO_0000050>  OEO_00010038
    
    DifferentFrom: 
        OEO_00010229
    
    
Individual: OEO_00010059

    Annotations: 
        OEO_00010037 "CRF 1.A.3.a",
        <http://purl.obolibrary.org/obo/IAO_0000115> "The CRF sector (IPCC 2006) 'domestic aviation' is a transport sector defined by the 2006 IPCC Guidelines for National Greenhouse Gas Inventories:
Emissions from civil domestic passenger and freight traffic that departs and arrives in the same country (commercial, private, agriculture, etc.), including take-offs and landings for these flight stages. Note that this may include journeys of considerable length between two airports in a country (e.g. San Francisco to Honolulu). Exclude military, which should be reported under 1 A 5 b.",
        <http://purl.obolibrary.org/obo/IAO_0000119> "2006 IPCC Guidelines for National Greenhouse Gas Inventories, Volume 1, Chapter 8.5, https://www.ipcc-nggip.iges.or.jp/public/2006gl/",
        <http://purl.obolibrary.org/obo/IAO_0000233> "issue: https://github.com/OpenEnergyPlatform/ontology/issues/580
pull request: https://github.com/OpenEnergyPlatform/ontology/pull/595

move to oeo-sector 
issue: https://github.com/OpenEnergyPlatform/ontology/issues/1399
pull request: https://github.com/OpenEnergyPlatform/ontology/pull/1724",
        rdfs:label "CRF sector (IPCC 2006): domestic aviation"@en
    
    Types: 
        OEO_00000422
    
    Facts:  
     OEO_00000504  OEO_00000242,
     <http://purl.obolibrary.org/obo/BFO_0000050>  OEO_00010042
    
    DifferentFrom: 
        OEO_00010201
    
    
Individual: OEO_00010060

    Annotations: 
        OEO_00010037 "CRF 1.A.3.b",
        <http://purl.obolibrary.org/obo/IAO_0000115> "The CRF sector (IPCC 2006) 'road transport' is a transport sector defined by the 2006 IPCC Guidelines for National Greenhouse Gas Inventories:
All combustion and evaporative emissions arising from fuel use in road vehicles, including the use of agricultural vehicles on paved roads.",
        <http://purl.obolibrary.org/obo/IAO_0000119> "2006 IPCC Guidelines for National Greenhouse Gas Inventories, Volume 1, Chapter 8.5, https://www.ipcc-nggip.iges.or.jp/public/2006gl/",
        <http://purl.obolibrary.org/obo/IAO_0000233> "issue: https://github.com/OpenEnergyPlatform/ontology/issues/580
pull request: https://github.com/OpenEnergyPlatform/ontology/pull/595

move to oeo-sector 
issue: https://github.com/OpenEnergyPlatform/ontology/issues/1399
pull request: https://github.com/OpenEnergyPlatform/ontology/pull/1724",
        rdfs:label "CRF sector (IPCC 2006): road transportation"@en
    
    Types: 
        OEO_00000422
    
    Facts:  
     OEO_00000504  OEO_00000242,
     <http://purl.obolibrary.org/obo/BFO_0000050>  OEO_00010042
    
    
Individual: OEO_00010061

    Annotations: 
        OEO_00010037 "CRF 1.A.3.c",
        <http://purl.obolibrary.org/obo/IAO_0000115> "2006 IPCC Guidelines for National Greenhouse Gas Inventories, Volume 1, Chapter 8.5, https://www.ipcc-nggip.iges.or.jp/public/2006gl/",
        <http://purl.obolibrary.org/obo/IAO_0000115> "The CRF sector (IPCC 2006) 'railways' is a transport sector defined by the 2006 IPCC Guidelines for National Greenhouse Gas Inventories:
Emissions from railway transport for both freight and passenger traffic routes.",
        <http://purl.obolibrary.org/obo/IAO_0000115> "issue: https://github.com/OpenEnergyPlatform/ontology/issues/580
pull request: https://github.com/OpenEnergyPlatform/ontology/pull/595

move to oeo-sector 
issue: https://github.com/OpenEnergyPlatform/ontology/issues/1399
pull request: https://github.com/OpenEnergyPlatform/ontology/pull/1724",
        rdfs:label "CRF sector (IPCC 2006): railways"@en
    
    Types: 
        OEO_00000422
    
    Facts:  
     OEO_00000504  OEO_00000242,
     <http://purl.obolibrary.org/obo/BFO_0000050>  OEO_00010042
    
    
Individual: OEO_00010062

    Annotations: 
        OEO_00010037 "CRF 1.A.3.d",
        <http://purl.obolibrary.org/obo/IAO_0000115> "The CRF sector (IPCC 2006) 'domestic navigation' is a transport sector defined by the 2006 IPCC Guidelines for National Greenhouse Gas Inventories:
Emissions from fuels used by vessels of all flags that depart and arrive in the same country (exclude fishing, which should be reported under 1 A 4 c iii, and military, which should be reported under 1 A 5 b). Note that this may include journeys of considerable length between two ports in a country (e.g. San Francisco to Honolulu).",
        <http://purl.obolibrary.org/obo/IAO_0000119> "2006 IPCC Guidelines for National Greenhouse Gas Inventories, Volume 1, Chapter 8.5, https://www.ipcc-nggip.iges.or.jp/public/2006gl/",
        <http://purl.obolibrary.org/obo/IAO_0000233> "issue: https://github.com/OpenEnergyPlatform/ontology/issues/580
pull request: https://github.com/OpenEnergyPlatform/ontology/pull/595

move to oeo-sector 
issue: https://github.com/OpenEnergyPlatform/ontology/issues/1399
pull request: https://github.com/OpenEnergyPlatform/ontology/pull/1724",
        rdfs:label "CRF sector (IPCC 2006): domestic navigation"@en
    
    Types: 
        OEO_00000422
    
    Facts:  
     OEO_00000504  OEO_00000242,
     <http://purl.obolibrary.org/obo/BFO_0000050>  OEO_00010042
    
    DifferentFrom: 
        OEO_00010202
    
    
Individual: OEO_00010063

    Annotations: 
        OEO_00010037 "CRF 1.A.3.e",
        <http://purl.obolibrary.org/obo/IAO_0000115> "The CRF sector (IPCC 2006) 'other transportation' is a transport sector defined by the 2006 IPCC Guidelines for National Greenhouse Gas Inventories:
Combustion emissions from all remaining transport activities including pipeline transportation, ground activities in airports and harbours, and off-road activities not otherwise reported under 1 A 4 c Agriculture or 1 A 2. Manufacturing Industries and Construction. Military transport should be reported under 1 A 5.",
        <http://purl.obolibrary.org/obo/IAO_0000119> "2006 IPCC Guidelines for National Greenhouse Gas Inventories, Volume 1, Chapter 8.5, https://www.ipcc-nggip.iges.or.jp/public/2006gl/",
        <http://purl.obolibrary.org/obo/IAO_0000233> "issue: https://github.com/OpenEnergyPlatform/ontology/issues/580
pull request: https://github.com/OpenEnergyPlatform/ontology/pull/595

move to oeo-sector 
issue: https://github.com/OpenEnergyPlatform/ontology/issues/1399
pull request: https://github.com/OpenEnergyPlatform/ontology/pull/1724",
        rdfs:label "CRF sector (IPCC 2006): other transportation"@en
    
    Types: 
        OEO_00000422
    
    Facts:  
     OEO_00000504  OEO_00000242,
     <http://purl.obolibrary.org/obo/BFO_0000050>  OEO_00010042
    
    
Individual: OEO_00010064

    Annotations: 
        OEO_00010037 "CRF 1.A.3.e.i",
        <http://purl.obolibrary.org/obo/IAO_0000115> "The CRF sector (IPCC 2006) 'pipeline transport' is a transport sector defined by the 2006 IPCC Guidelines for National Greenhouse Gas Inventories:
Combustion related emissions from the operation of pump stations and maintenance of pipelines. Transport via pipelines includes transport of gases  liquids, slurry and other commodities via pipelines. Distribution of natural or manufactured gas, water or steam from the distributor to final users is excluded and should be reported in 1 A 1 c ii or 1 A 4 a.",
        <http://purl.obolibrary.org/obo/IAO_0000119> "2006 IPCC Guidelines for National Greenhouse Gas Inventories, Volume 1, Chapter 8.5, https://www.ipcc-nggip.iges.or.jp/public/2006gl/",
        <http://purl.obolibrary.org/obo/IAO_0000233> "issue: https://github.com/OpenEnergyPlatform/ontology/issues/580
pull request: https://github.com/OpenEnergyPlatform/ontology/pull/595

fix unique individual identfier
issue: https://github.com/OpenEnergyPlatform/ontology/issues/1121
pull request: https://github.com/OpenEnergyPlatform/ontology/pull/1122

move to oeo-sector 
issue: https://github.com/OpenEnergyPlatform/ontology/issues/1399
pull request: https://github.com/OpenEnergyPlatform/ontology/pull/1724",
        rdfs:label "CRF sector (IPCC 2006): pipeline transport"@en
    
    Types: 
        OEO_00000422
    
    Facts:  
     OEO_00000504  OEO_00000242,
     <http://purl.obolibrary.org/obo/BFO_0000050>  OEO_00010063
    
    
Individual: OEO_00010065

    Annotations: 
        <http://purl.obolibrary.org/obo/IAO_0000115> "The KSG sector energy industry is an energy transformation sector defined by the KSG sector division. It is an aggregate of the following three sectors:
- CRF sector (IPCC 2006): energy industry (CRF 1.A.1.a)
- CRF sector (IPCC 2006): other transportation (CRF 1.A.3.e)
- CRF sector (IPCC 2006): fugitive emissions from fuels (CRF 1.B)",
        <http://purl.obolibrary.org/obo/IAO_0000119> "Bundes-Klimaschutzgesetz (KSG), Anlage 1 (zu den §§ 4 und 5) https://www.gesetze-im-internet.de/ksg/anlage_1.html",
        <http://purl.obolibrary.org/obo/IAO_0000233> "issue: https://github.com/OpenEnergyPlatform/ontology/issues/580
pull request: https://github.com/OpenEnergyPlatform/ontology/pull/595

move to oeo-sector 
issue: https://github.com/OpenEnergyPlatform/ontology/issues/1399
pull request: https://github.com/OpenEnergyPlatform/ontology/pull/1724",
        rdfs:label "KSG sector energy industry"@en
    
    Types: 
        OEO_00000158
    
    Facts:  
     OEO_00000504  OEO_00010056,
     <http://purl.obolibrary.org/obo/BFO_0000051>  OEO_00010040,
     <http://purl.obolibrary.org/obo/BFO_0000051>  OEO_00010057,
     <http://purl.obolibrary.org/obo/BFO_0000051>  OEO_00010064
    
    
Individual: OEO_00010066

    Annotations: 
        <http://purl.obolibrary.org/obo/IAO_0000115> "The KSG sector industry is an industry sector defined by the KSG sector division. It is an aggregate of the following three sectors:
- CRF sector (IPCC 2006): manufacturing industries and construction (CRF 1.A.2)
- CRF sector (IPCC 2006): CO2 transport and storage (CRF 1.C)
- CRF sector (IPCC 2006): industrial processes and product use (CRF 2)",
        <http://purl.obolibrary.org/obo/IAO_0000119> "Bundes-Klimaschutzgesetz (KSG), Anlage 1 (zu den §§ 4 und 5) https://www.gesetze-im-internet.de/ksg/anlage_1.html",
        <http://purl.obolibrary.org/obo/IAO_0000233> "issue: https://github.com/OpenEnergyPlatform/ontology/issues/580
pull request: https://github.com/OpenEnergyPlatform/ontology/pull/595

move to oeo-sector 
issue: https://github.com/OpenEnergyPlatform/ontology/issues/1399
pull request: https://github.com/OpenEnergyPlatform/ontology/pull/1724",
        rdfs:label "KSG sector industry"@en
    
    Types: 
        OEO_00000227
    
    Facts:  
     OEO_00000504  OEO_00010056,
     <http://purl.obolibrary.org/obo/BFO_0000051>  OEO_00010041,
     <http://purl.obolibrary.org/obo/BFO_0000051>  OEO_00010046,
     <http://purl.obolibrary.org/obo/BFO_0000051>  OEO_00010058
    
    
Individual: OEO_00010067

    Annotations: 
        <http://purl.obolibrary.org/obo/IAO_0000115> "The KSG sector buildings is a building sector defined by the KSG sector division. It is an aggregate of the following two sectors:
- CRF sector (IPCC 2006): commercial and institutional (CRF 1.A.4.a)
- CRF sector (IPCC 2006): residential (CRF 1.A.4.b)
- CRF sector (IPCC 2006): fuel combustion - other",
        <http://purl.obolibrary.org/obo/IAO_0000119> "Bundes-Klimaschutzgesetz (KSG), Anlage 1 (zu den §§ 4 und 5) https://www.gesetze-im-internet.de/ksg/anlage_1.html",
        <http://purl.obolibrary.org/obo/IAO_0000233> "issue: https://github.com/OpenEnergyPlatform/ontology/issues/580
pull request: https://github.com/OpenEnergyPlatform/ontology/pull/595

Add axiom to 1.A.5 and extend definition:
issue: https://github.com/OpenEnergyPlatform/ontology/issues/1194
pull request: https://github.com/OpenEnergyPlatform/ontology/pull/1198

move to oeo-sector 
issue: https://github.com/OpenEnergyPlatform/ontology/issues/1399
pull request: https://github.com/OpenEnergyPlatform/ontology/pull/1724",
        rdfs:label "KSG sector buildings"@en
    
    Types: 
        OEO_00010034
    
    Facts:  
     OEO_00000504  OEO_00010056,
     <http://purl.obolibrary.org/obo/BFO_0000051>  OEO_00010044,
     <http://purl.obolibrary.org/obo/BFO_0000051>  OEO_00010052,
     <http://purl.obolibrary.org/obo/BFO_0000051>  OEO_00010053
    
    
Individual: OEO_00010068

    Annotations: 
        <http://purl.obolibrary.org/obo/IAO_0000115> "The KSG sector transport is a transport sector defined by the KSG sector division. It is an aggregate of the following four sectors:
- CRF sector (IPCC 2006): domestic aviation (CRF 1.A.3.a)
- CRF sector (IPCC 2006): road transportation (CRF 1.A.3.b)
- CRF sector (IPCC 2006): railways (CRF 1.A.3.c)
- CRF sector (IPCC 2006): domestic navigation (CRF 1.A.3.d)",
        <http://purl.obolibrary.org/obo/IAO_0000119> "Bundes-Klimaschutzgesetz (KSG), Anlage 1 (zu den §§ 4 und 5) https://www.gesetze-im-internet.de/ksg/anlage_1.html",
        <http://purl.obolibrary.org/obo/IAO_0000233> "issue: https://github.com/OpenEnergyPlatform/ontology/issues/580
pull request: https://github.com/OpenEnergyPlatform/ontology/pull/595

move to oeo-sector 
issue: https://github.com/OpenEnergyPlatform/ontology/issues/1399
pull request: https://github.com/OpenEnergyPlatform/ontology/pull/1724",
        rdfs:label "KSG sector transport"@en
    
    Types: 
        OEO_00000422
    
    Facts:  
     OEO_00000504  OEO_00010056,
     <http://purl.obolibrary.org/obo/BFO_0000051>  OEO_00010059,
     <http://purl.obolibrary.org/obo/BFO_0000051>  OEO_00010060,
     <http://purl.obolibrary.org/obo/BFO_0000051>  OEO_00010061,
     <http://purl.obolibrary.org/obo/BFO_0000051>  OEO_00010062
    
    
Individual: OEO_00010069

    Annotations: 
        <http://purl.obolibrary.org/obo/IAO_0000115> "The KSG sector agriculture is an agriculture, forestry and land use sector defined by the KSG sector division. It is an aggregate of the following two sectors:
- CRF sector (IPCC 2006): agriculture, forestry and fishing (CRF 1.A.4.c)
- CRF sector (IPCC 2006): agriculture (CRF 3)",
        <http://purl.obolibrary.org/obo/IAO_0000119> "Bundes-Klimaschutzgesetz (KSG), Anlage 1 (zu den §§ 4 und 5) https://www.gesetze-im-internet.de/ksg/anlage_1.html",
        <http://purl.obolibrary.org/obo/IAO_0000233> "issue: https://github.com/OpenEnergyPlatform/ontology/issues/580
pull request: https://github.com/OpenEnergyPlatform/ontology/pull/595

move to oeo-sector 
issue: https://github.com/OpenEnergyPlatform/ontology/issues/1399
pull request: https://github.com/OpenEnergyPlatform/ontology/pull/1724",
        rdfs:label "KSG sector agriculture"@en
    
    Types: 
        OEO_00010035
    
    Facts:  
     OEO_00000504  OEO_00010056,
     <http://purl.obolibrary.org/obo/BFO_0000051>  OEO_00010047,
     <http://purl.obolibrary.org/obo/BFO_0000051>  OEO_00010054
    
    
Individual: OEO_00010070

    Annotations: 
        <http://purl.obolibrary.org/obo/IAO_0000115> "The KSG sector waste management and other is a sector defined by the KSG sector division. It is an aggregate of the following two sectors:
- CRF sector (IPCC 2006): waste (CRF 5)
- CRF sector (IPCC 2006): other (CRF 6)",
        <http://purl.obolibrary.org/obo/IAO_0000119> "Bundes-Klimaschutzgesetz (KSG), Anlage 1 (zu den §§ 4 und 5) https://www.gesetze-im-internet.de/ksg/anlage_1.html",
        <http://purl.obolibrary.org/obo/IAO_0000233> "issue: https://github.com/OpenEnergyPlatform/ontology/issues/580
pull request: https://github.com/OpenEnergyPlatform/ontology/pull/595

move to oeo-sector 
issue: https://github.com/OpenEnergyPlatform/ontology/issues/1399
pull request: https://github.com/OpenEnergyPlatform/ontology/pull/1724",
        rdfs:label "KSG sector waste management and other"@en
    
    Types: 
        OEO_00010036
    
    Facts:  
     OEO_00000504  OEO_00010056,
     <http://purl.obolibrary.org/obo/BFO_0000051>  OEO_00010049,
     <http://purl.obolibrary.org/obo/BFO_0000051>  OEO_00010050
    
    
Individual: OEO_00010071

    Annotations: 
        <http://purl.obolibrary.org/obo/IAO_0000115> "The KSG sector land use, land-use change and forestry is an agriculture, forestry and land use sector defined by the KSG sector division.
It is equivalent to the CRF sector (IPCC 2006): land use, land-use change and forestry (CRF 4).",
        <http://purl.obolibrary.org/obo/IAO_0000119> "Bundes-Klimaschutzgesetz (KSG), Anlage 1 (zu den §§ 4 und 5) https://www.gesetze-im-internet.de/ksg/anlage_1.html",
        <http://purl.obolibrary.org/obo/IAO_0000233> "issue: https://github.com/OpenEnergyPlatform/ontology/issues/580
pull request: https://github.com/OpenEnergyPlatform/ontology/pull/595

move to oeo-sector 
issue: https://github.com/OpenEnergyPlatform/ontology/issues/1399
pull request: https://github.com/OpenEnergyPlatform/ontology/pull/1724",
        rdfs:label "KSG sector land use, land-use change and forestry"@en
    
    Types: 
        OEO_00010035
    
    Facts:  
     OEO_00000504  OEO_00010056
    
    SameAs: 
        OEO_00010048
    
    
Individual: OEO_00010131

    Annotations: 
        <http://purl.obolibrary.org/obo/IAO_0000115> "The EU emission sector ETS is a sector defined by an EU emission sector division that covers greenhouse gas emissions that are regulated by the European Union Emissions Trading System.",
        <http://purl.obolibrary.org/obo/IAO_0000233> "issue: https://github.com/OpenEnergyPlatform/ontology/issues/834
pull request: https://github.com/OpenEnergyPlatform/ontology/pull/857

Improve axioms and definition:
issue: https://github.com/OpenEnergyPlatform/ontology/issues/1449
pull request: https://github.com/OpenEnergyPlatform/ontology/pull/1462

move to oeo-sector 
issue: https://github.com/OpenEnergyPlatform/ontology/issues/1399
pull request: https://github.com/OpenEnergyPlatform/ontology/pull/1724",
        rdfs:label "EU emission sector: ETS"@en
    
    Types: 
        OEO_00000367,
        OEO_00000504 some OEO_00010403
    
    
Individual: OEO_00010132

    Annotations: 
        <http://purl.obolibrary.org/obo/IAO_0000115> "The EU emission sector ETS stationary is a sector defined by an EU emission sector division that covers greenhouse gas emissions regulated by the European Union Emissions Trading System and that are emitted by stationary installations.",
        <http://purl.obolibrary.org/obo/IAO_0000233> "issue: https://github.com/OpenEnergyPlatform/ontology/issues/834
pull request: https://github.com/OpenEnergyPlatform/ontology/pull/857

Improve axioms and definition:
issue: https://github.com/OpenEnergyPlatform/ontology/issues/1449
pull request: https://github.com/OpenEnergyPlatform/ontology/pull/1462

move to oeo-sector 
issue: https://github.com/OpenEnergyPlatform/ontology/issues/1399
pull request: https://github.com/OpenEnergyPlatform/ontology/pull/1724",
        rdfs:label "EU emission sector: ETS stationary"@en
    
    Types: 
        OEO_00000367,
        OEO_00000504 some OEO_00010403
    
    Facts:  
     <http://purl.obolibrary.org/obo/BFO_0000050>  OEO_00010131
    
    
Individual: OEO_00010133

    Annotations: 
        <http://purl.obolibrary.org/obo/IAO_0000115> "The EU emission sector ETS aviation is a transport sector defined by an EU emission sector division that covers greenhouse gas emissions regulated by the European Union Emissions Trading System and that are emitted by stationary installations.",
        <http://purl.obolibrary.org/obo/IAO_0000233> "issue: https://github.com/OpenEnergyPlatform/ontology/issues/834
pull request: https://github.com/OpenEnergyPlatform/ontology/pull/857

Improve axioms and definition:
issue: https://github.com/OpenEnergyPlatform/ontology/issues/1449
pull request: https://github.com/OpenEnergyPlatform/ontology/pull/1462

move to oeo-sector 
issue: https://github.com/OpenEnergyPlatform/ontology/issues/1399
pull request: https://github.com/OpenEnergyPlatform/ontology/pull/1724",
        rdfs:label "EU emission sector: ETS aviation"@en
    
    Types: 
        OEO_00000422,
        OEO_00000504 some OEO_00010403
    
    Facts:  
     <http://purl.obolibrary.org/obo/BFO_0000050>  OEO_00010131
    
    
Individual: OEO_00010134

    Annotations: 
        <http://purl.obolibrary.org/obo/IAO_0000115> "The EU emission sector effort sharing is a sector defined by the EU emission sector division that covers greenhouse gas emissions regulated by the Effort Sharing Decision and the Effort Sharing Regulation.",
        <http://purl.obolibrary.org/obo/IAO_0000233> "issue: https://github.com/OpenEnergyPlatform/ontology/issues/834
pull request: https://github.com/OpenEnergyPlatform/ontology/pull/857

Improve axioms:
issue: https://github.com/OpenEnergyPlatform/ontology/issues/1449
pull request: https://github.com/OpenEnergyPlatform/ontology/pull/1462

move to oeo-sector 
issue: https://github.com/OpenEnergyPlatform/ontology/issues/1399
pull request: https://github.com/OpenEnergyPlatform/ontology/pull/1724",
        rdfs:label "EU emission sector: effort sharing"@en
    
    Types: 
        OEO_00000367,
        OEO_00000504 some OEO_00010403
    
    
Individual: OEO_00010135

    Annotations: 
        <http://purl.obolibrary.org/obo/IAO_0000115> "The EU emission sector ETS stationary is a sector defined by an EU emission sector division that covers greenhouse gas emissions regulated by the European Union Emissions Trading System and that are emitted by stationary installations.",
        <http://purl.obolibrary.org/obo/IAO_0000233> "issue: https://github.com/OpenEnergyPlatform/ontology/issues/834
pull request: https://github.com/OpenEnergyPlatform/ontology/pull/857

Improve axioms and definition:
issue: https://github.com/OpenEnergyPlatform/ontology/issues/1449
pull request: https://github.com/OpenEnergyPlatform/ontology/pull/1462

move to oeo-sector 
issue: https://github.com/OpenEnergyPlatform/ontology/issues/1399
pull request: https://github.com/OpenEnergyPlatform/ontology/pull/1724",
        rdfs:label "EU emission sector: LULUCF"@en
    
    Types: 
        OEO_00010035,
        OEO_00000504 some OEO_00010403
    
    SameAs: 
        OEO_00010048
    
    
Individual: OEO_00010158

    Annotations: 
        OEO_00010037 "CRF 1.A.1.a",
        <http://purl.obolibrary.org/obo/IAO_0000115> "The CRF sector (IPCC 2006) 'public electricity and heat production' is an energy transformation sector defined by the 2006 IPCC Guidelines for National Greenhouse Gas Inventories:
Sum of emissions from main activity producers of electricity generation, combined heat and power generation, and heat plants.",
        <http://purl.obolibrary.org/obo/IAO_0000119> "2006 IPCC Guidelines for National Greenhouse Gas Inventories, Volume 2, Chapter 2.2, https://www.ipcc-nggip.iges.or.jp/public/2006gl/",
        <http://purl.obolibrary.org/obo/IAO_0000233> "issue: https://github.com/OpenEnergyPlatform/ontology/issues/858
pull request: https://github.com/OpenEnergyPlatform/ontology/pull/941

move to oeo-sector 
issue: https://github.com/OpenEnergyPlatform/ontology/issues/1399
pull request: https://github.com/OpenEnergyPlatform/ontology/pull/1724",
        rdfs:label "CRF sector (IPCC 2006): public electricity and heat production"@en
    
    Types: 
        OEO_00000158
    
    Facts:  
     OEO_00000504  OEO_00000242,
     <http://purl.obolibrary.org/obo/BFO_0000050>  OEO_00010040
    
    
Individual: OEO_00010159

    Annotations: 
        OEO_00010037 "CRF 1.A.1.b",
        <http://purl.obolibrary.org/obo/IAO_0000115> "The CRF sector (IPCC 2006) 'petroleum refining' is an energy transformation sector defined by the 2006 IPCC Guidelines for National Greenhouse Gas Inventories:
All combustion activities supporting the refining of petroleum products including on-site combustion for the generation of electricity and heat for own use.",
        <http://purl.obolibrary.org/obo/IAO_0000119> "2006 IPCC Guidelines for National Greenhouse Gas Inventories, Volume 2, Chapter 2.2, https://www.ipcc-nggip.iges.or.jp/public/2006gl/",
        <http://purl.obolibrary.org/obo/IAO_0000233> "issue: https://github.com/OpenEnergyPlatform/ontology/issues/858
pull request: https://github.com/OpenEnergyPlatform/ontology/pull/941

Make individual of 'mineral oil refining sector':
issue: https://github.com/OpenEnergyPlatform/ontology/issues/1318
pull request: https://github.com/OpenEnergyPlatform/ontology/pull/1331

move to oeo-sector 
issue: https://github.com/OpenEnergyPlatform/ontology/issues/1399
pull request: https://github.com/OpenEnergyPlatform/ontology/pull/1724",
        rdfs:label "CRF sector (IPCC 2006): petroleum refining"@en
    
    Types: 
        OEO_00010319
    
    Facts:  
     OEO_00000504  OEO_00000242,
     <http://purl.obolibrary.org/obo/BFO_0000050>  OEO_00010040
    
    
Individual: OEO_00010160

    Annotations: 
        OEO_00010037 "CRF 1.A.1.c",
        <http://purl.obolibrary.org/obo/IAO_0000115> "The CRF sector (IPCC 2006) 'manufacture of solid fuels and other energy industries' is an energy transformation sector defined by the 2006 IPCC Guidelines for National Greenhouse Gas Inventories:
Combustion emissions from fuel use during the manufacture of secondary and tertiary products from solid fuels including production of charcoal.",
        <http://purl.obolibrary.org/obo/IAO_0000119> "2006 IPCC Guidelines for National Greenhouse Gas Inventories, Volume 2, Chapter 2.2, https://www.ipcc-nggip.iges.or.jp/public/2006gl/",
        <http://purl.obolibrary.org/obo/IAO_0000233> "issue: https://github.com/OpenEnergyPlatform/ontology/issues/858
pull request: https://github.com/OpenEnergyPlatform/ontology/pull/941

move to oeo-sector 
issue: https://github.com/OpenEnergyPlatform/ontology/issues/1399
pull request: https://github.com/OpenEnergyPlatform/ontology/pull/1724",
        rdfs:label "CRF sector (IPCC 2006): manufacture of solid fuels and other energy industries"@en
    
    Types: 
        OEO_00000158
    
    Facts:  
     OEO_00000504  OEO_00000242,
     <http://purl.obolibrary.org/obo/BFO_0000050>  OEO_00010040
    
    
Individual: OEO_00010161

    Annotations: 
        OEO_00010037 "CRF 1.B.1",
        <http://purl.obolibrary.org/obo/IAO_0000115> "The CRF sector (IPCC 2006) 'solid fuels' is a sector defined by the 2006 IPCC Guidelines for National Greenhouse Gas Inventories:
Includes all intentional and unintentional emissions from the extraction, processing, storage and transport of fuel to the point of final use.",
        <http://purl.obolibrary.org/obo/IAO_0000119> "2006 IPCC Guidelines for National Greenhouse Gas Inventories, Volume 1, Chapter 8.5, https://www.ipcc-nggip.iges.or.jp/public/2006gl/",
        <http://purl.obolibrary.org/obo/IAO_0000233> "issue: https://github.com/OpenEnergyPlatform/ontology/issues/858
pull request: https://github.com/OpenEnergyPlatform/ontology/pull/941

move to oeo-sector 
issue: https://github.com/OpenEnergyPlatform/ontology/issues/1399
pull request: https://github.com/OpenEnergyPlatform/ontology/pull/1724",
        rdfs:label "CRF sector (IPCC 2006): solid fuels"@en
    
    Types: 
        OEO_00000367
    
    Facts:  
     OEO_00000504  OEO_00000242,
     <http://purl.obolibrary.org/obo/BFO_0000050>  OEO_00010057
    
    
Individual: OEO_00010162

    Annotations: 
        OEO_00010037 "CRF 1.B.2",
        <http://purl.obolibrary.org/obo/IAO_0000115> "The CRF sector (IPCC 2006) 'oil and natural gas' is a sector defined by the 2006 IPCC Guidelines for National Greenhouse Gas Inventories:
Comprises fugitive emissions from all oil and natural gas activities.",
        <http://purl.obolibrary.org/obo/IAO_0000119> "2006 IPCC Guidelines for National Greenhouse Gas Inventories, Volume 1, Chapter 8.5, https://www.ipcc-nggip.iges.or.jp/public/2006gl/",
        <http://purl.obolibrary.org/obo/IAO_0000233> "issue: https://github.com/OpenEnergyPlatform/ontology/issues/858
pull request: https://github.com/OpenEnergyPlatform/ontology/pull/941

move to oeo-sector 
issue: https://github.com/OpenEnergyPlatform/ontology/issues/1399
pull request: https://github.com/OpenEnergyPlatform/ontology/pull/1724",
        rdfs:label "CRF sector (IPCC 2006): oil and natural gas"@en
    
    Types: 
        OEO_00000367
    
    Facts:  
     OEO_00000504  OEO_00000242,
     <http://purl.obolibrary.org/obo/BFO_0000050>  OEO_00010057
    
    
Individual: OEO_00010163

    Annotations: 
        <http://purl.obolibrary.org/obo/IAO_0000115> "The GovReg sector division is a sector division defined in Annex XXV, Table 1a of Commission Implementing Regulation (EU) 2020/1208. It uses CRF sectors (IPCC 2006) and adds further sectors.",
        <http://purl.obolibrary.org/obo/IAO_0000116> "Annex XXV, Table 1a of Commission Implementing Regulation (EU) 2020/1208: https://eur-lex.europa.eu/legal-content/EN/TXT/HTML/?uri=CELEX:32020R1208&from=EN#d1e32-98-1",
        <http://purl.obolibrary.org/obo/IAO_0000233> "issue: https://github.com/OpenEnergyPlatform/ontology/issues/858
pull request: https://github.com/OpenEnergyPlatform/ontology/pull/941

relabel:
issue: https://github.com/OpenEnergyPlatform/ontology/issues/928
pull request: https://github.com/OpenEnergyPlatform/ontology/pull/944

Make instance of 'EU emission sector division':
issue: https://github.com/OpenEnergyPlatform/ontology/issues/1449
pull request: https://github.com/OpenEnergyPlatform/ontology/pull/1462

move to oeo-sector 
issue: https://github.com/OpenEnergyPlatform/ontology/issues/1399
pull request: https://github.com/OpenEnergyPlatform/ontology/pull/1724",
        rdfs:label "GovReg sector division"@en
    
    Types: 
        OEO_00010130
    
    Facts:  
     OEO_00000503  OEO_00000242
    
    
Individual: OEO_00010164

    Annotations: 
        OEO_00010037 "CRF 2.A",
        <http://purl.obolibrary.org/obo/IAO_0000115> "The CRF sector (IPCC 2006) 'mineral industry' is an industry sector defined by the 2006 IPCC Guidelines for National Greenhouse Gas Inventories:
Process-related carbon dioxide (CO2) emissions resulting from the use of carbonate raw materials in the production and use of a variety of mineral industry products.",
        <http://purl.obolibrary.org/obo/IAO_0000119> "2006 IPCC Guidelines for National Greenhouse Gas Inventories, Volume 3, Chapter 2.1, https://www.ipcc-nggip.iges.or.jp/public/2006gl/",
        <http://purl.obolibrary.org/obo/IAO_0000233> "issue: https://github.com/OpenEnergyPlatform/ontology/issues/858
pull request: https://github.com/OpenEnergyPlatform/ontology/pull/941

move to oeo-sector 
issue: https://github.com/OpenEnergyPlatform/ontology/issues/1399
pull request: https://github.com/OpenEnergyPlatform/ontology/pull/1724",
        rdfs:label "CRF sector (IPCC 2006): mineral industry"@en
    
    Types: 
        OEO_00000227
    
    Facts:  
     OEO_00000504  OEO_00000242,
     <http://purl.obolibrary.org/obo/BFO_0000050>  OEO_00010046
    
    
Individual: OEO_00010165

    Annotations: 
        OEO_00010037 "CRF 2.A.1",
        <http://purl.obolibrary.org/obo/IAO_0000115> "The CRF sector (IPCC 2006) 'cement production' is an industry sector defined by the 2006 IPCC Guidelines for National Greenhouse Gas Inventories:
Process-related emissions from the production of various types of cement (ISIC: D2694).",
        <http://purl.obolibrary.org/obo/IAO_0000119> "2006 IPCC Guidelines for National Greenhouse Gas Inventories, Volume 1, Chapter 8.5, https://www.ipcc-nggip.iges.or.jp/public/2006gl/",
        <http://purl.obolibrary.org/obo/IAO_0000233> "issue: https://github.com/OpenEnergyPlatform/ontology/issues/858
pull request: https://github.com/OpenEnergyPlatform/ontology/pull/941

move to oeo-sector 
issue: https://github.com/OpenEnergyPlatform/ontology/issues/1399
pull request: https://github.com/OpenEnergyPlatform/ontology/pull/1724",
        rdfs:label "CRF sector (IPCC 2006): cement production"@en
    
    Types: 
        OEO_00000227
    
    Facts:  
     OEO_00000504  OEO_00000242,
     <http://purl.obolibrary.org/obo/BFO_0000050>  OEO_00010164
    
    
Individual: OEO_00010166

    Annotations: 
        OEO_00010037 "CRF 2.B",
        <http://purl.obolibrary.org/obo/IAO_0000115> "The CRF sector (IPCC 2006) 'chemical industry' is an industry sector defined by the 2006 IPCC Guidelines for National Greenhouse Gas Inventories:
Greenhouse gas emissions that result from the production of various inorganic and organic chemicals.",
        <http://purl.obolibrary.org/obo/IAO_0000119> "2006 IPCC Guidelines for National Greenhouse Gas Inventories, Volume 3, Chapter 3.1, https://www.ipcc-nggip.iges.or.jp/public/2006gl/",
        <http://purl.obolibrary.org/obo/IAO_0000233> "issue: https://github.com/OpenEnergyPlatform/ontology/issues/858
pull request: https://github.com/OpenEnergyPlatform/ontology/pull/941

move to oeo-sector 
issue: https://github.com/OpenEnergyPlatform/ontology/issues/1399
pull request: https://github.com/OpenEnergyPlatform/ontology/pull/1724",
        rdfs:label "CRF sector (IPCC 2006): chemical industry"@en
    
    Types: 
        OEO_00000227
    
    Facts:  
     OEO_00000504  OEO_00000242,
     <http://purl.obolibrary.org/obo/BFO_0000050>  OEO_00010046
    
    
Individual: OEO_00010167

    Annotations: 
        OEO_00010037 "CRF 2.C",
        <http://purl.obolibrary.org/obo/IAO_0000115> "The CRF sector (IPCC 2006) 'metal industry' is an industry sector defined by the 2006 IPCC Guidelines for National Greenhouse Gas Inventories:
Greenhouse gas emissions that result from the production of metals.",
        <http://purl.obolibrary.org/obo/IAO_0000119> "2006 IPCC Guidelines for National Greenhouse Gas Inventories, Volume 3, Chapter 4.1, https://www.ipcc-nggip.iges.or.jp/public/2006gl/",
        <http://purl.obolibrary.org/obo/IAO_0000233> "issue: https://github.com/OpenEnergyPlatform/ontology/issues/858
pull request: https://github.com/OpenEnergyPlatform/ontology/pull/941

move to oeo-sector 
issue: https://github.com/OpenEnergyPlatform/ontology/issues/1399
pull request: https://github.com/OpenEnergyPlatform/ontology/pull/1724",
        rdfs:label "CRF sector (IPCC 2006): metal industry"@en
    
    Types: 
        OEO_00000227
    
    Facts:  
     OEO_00000504  OEO_00000242,
     <http://purl.obolibrary.org/obo/BFO_0000050>  OEO_00010046
    
    
Individual: OEO_00010168

    Annotations: 
        OEO_00010037 "CRF 2.C.1",
        <http://purl.obolibrary.org/obo/IAO_0000115> "The CRF sector (IPCC 2006) 'iron and steel production' is an industry sector defined by the 2006 IPCC Guidelines for National Greenhouse Gas Inventories:
Carbon dioxide is the predominant gas emitted from the production of iron and steel. The sources of the carbon dioxide emissions include that from carbon-containing reducing agents such as coke and pulverized coal, and, from minerals such as limestone and dolomite added.",
        <http://purl.obolibrary.org/obo/IAO_0000119> "2006 IPCC Guidelines for National Greenhouse Gas Inventories, Volume 1, Chapter 8.5, https://www.ipcc-nggip.iges.or.jp/public/2006gl/",
        <http://purl.obolibrary.org/obo/IAO_0000233> "issue: https://github.com/OpenEnergyPlatform/ontology/issues/858
pull request: https://github.com/OpenEnergyPlatform/ontology/pull/941

Fix definition:
issue: https://github.com/OpenEnergyPlatform/ontology/issues/1401
pull request: https://github.com/OpenEnergyPlatform/ontology/pull/1440

move to oeo-sector 
issue: https://github.com/OpenEnergyPlatform/ontology/issues/1399
pull request: https://github.com/OpenEnergyPlatform/ontology/pull/1724",
        rdfs:label "CRF sector (IPCC 2006): iron and steel production"@en
    
    Types: 
        OEO_00000227
    
    Facts:  
     OEO_00000504  OEO_00000242,
     <http://purl.obolibrary.org/obo/BFO_0000050>  OEO_00010167
    
    
Individual: OEO_00010169

    Annotations: 
        OEO_00010037 "CRF 2.D",
        <http://purl.obolibrary.org/obo/IAO_0000115> "The CRF sector (IPCC 2006) 'non-energy products from fuels and solvent use' is an industry sector defined by the 2006 IPCC Guidelines for National Greenhouse Gas Inventories:
The use of oil products and coal-derived oils primarily intended for purposes other than combustion",
        <http://purl.obolibrary.org/obo/IAO_0000119> "2006 IPCC Guidelines for National Greenhouse Gas Inventories, Volume 1, Chapter 8.5, https://www.ipcc-nggip.iges.or.jp/public/2006gl/",
        <http://purl.obolibrary.org/obo/IAO_0000233> "issue: https://github.com/OpenEnergyPlatform/ontology/issues/858
pull request: https://github.com/OpenEnergyPlatform/ontology/pull/941

move to oeo-sector 
issue: https://github.com/OpenEnergyPlatform/ontology/issues/1399
pull request: https://github.com/OpenEnergyPlatform/ontology/pull/1724",
        rdfs:label "CRF sector (IPCC 2006): non-energy products from fuels and solvent use"@en
    
    Types: 
        OEO_00000227
    
    Facts:  
     OEO_00000504  OEO_00000242,
     <http://purl.obolibrary.org/obo/BFO_0000050>  OEO_00010046
    
    
Individual: OEO_00010170

    Annotations: 
        OEO_00010037 "CRF 2.E",
        <http://purl.obolibrary.org/obo/IAO_0000115> "The CRF sector (IPCC 2006) 'electronics industry' is an industry sector defined by the 2006 IPCC Guidelines for National Greenhouse Gas Inventories:
Several advanced electronics manufacturing processes utilise fluorinated compounds (FCs) for plasma etching intricate patterns, cleaning reactor chambers, and temperature control. The specific electronic industry sectors include semiconductor, thin-film-transistor flat panel display (TFT-FPD), and photovoltaic (PV) manufacturing (collectively termed ‘electronics industry’).",
        <http://purl.obolibrary.org/obo/IAO_0000119> "2006 IPCC Guidelines for National Greenhouse Gas Inventories, Volume 3, Chapter 6.1, https://www.ipcc-nggip.iges.or.jp/public/2006gl/",
        <http://purl.obolibrary.org/obo/IAO_0000233> "issue: https://github.com/OpenEnergyPlatform/ontology/issues/858
pull request: https://github.com/OpenEnergyPlatform/ontology/pull/941

move to oeo-sector 
issue: https://github.com/OpenEnergyPlatform/ontology/issues/1399
pull request: https://github.com/OpenEnergyPlatform/ontology/pull/1724",
        rdfs:label "CRF sector (IPCC 2006): electronics industry"@en
    
    Types: 
        OEO_00000227
    
    Facts:  
     OEO_00000504  OEO_00000242,
     <http://purl.obolibrary.org/obo/BFO_0000050>  OEO_00010046
    
    
Individual: OEO_00010171

    Annotations: 
        OEO_00010037 "CRF 2.F",
        <http://purl.obolibrary.org/obo/IAO_0000115> "The CRF sector (IPCC 2006) 'product uses as substitutes for ozone depleting substances' is an industry sector defined by the 2006 IPCC Guidelines for National Greenhouse Gas Inventories:
Hydrofluorocarbons (HFCs) and, to a very limited extent, perfluorocarbons (PFCs), are serving as alternatives to ozone depleting substances (ODS) being phased out under the Montreal Protocol.",
        <http://purl.obolibrary.org/obo/IAO_0000119> "2006 IPCC Guidelines for National Greenhouse Gas Inventories, Volume 3, Chapter 7.1, https://www.ipcc-nggip.iges.or.jp/public/2006gl/",
        <http://purl.obolibrary.org/obo/IAO_0000233> "issue: https://github.com/OpenEnergyPlatform/ontology/issues/858
pull request: https://github.com/OpenEnergyPlatform/ontology/pull/941

move to oeo-sector 
issue: https://github.com/OpenEnergyPlatform/ontology/issues/1399
pull request: https://github.com/OpenEnergyPlatform/ontology/pull/1724",
        rdfs:label "CRF sector (IPCC 2006): product uses as substitutes for ozone depleting substances"@en
    
    Types: 
        OEO_00000227
    
    Facts:  
     OEO_00000504  OEO_00000242,
     <http://purl.obolibrary.org/obo/BFO_0000050>  OEO_00010046
    
    
Individual: OEO_00010172

    Annotations: 
        OEO_00010037 "CRF 2.G",
        <http://purl.obolibrary.org/obo/IAO_0000115> "The CRF sector (IPCC 2006) 'other product manufacture and use' is an industry sector defined by the 2006 IPCC Guidelines for National Greenhouse Gas Inventories:
Emissions of sulphur hexafluoride (SF6) and perfluorocarbons
(PFCs) from the manufacture and use of electrical equipment and a number of other products. It also includes emissions of nitrous oxide (N2O) from several products.",
        <http://purl.obolibrary.org/obo/IAO_0000119> "2006 IPCC Guidelines for National Greenhouse Gas Inventories, Volume 3, Chapter 8.1, https://www.ipcc-nggip.iges.or.jp/public/2006gl/",
        <http://purl.obolibrary.org/obo/IAO_0000233> "move to oeo-sector: issue: https://github.com/OpenEnergyPlatform/ontology/issues/1399
pull request: https://github.com/OpenEnergyPlatform/ontology/pull/1724",
        rdfs:label "CRF sector (IPCC 2006): other product manufacture and use"@en
    
    Types: 
        OEO_00000227
    
    Facts:  
     OEO_00000504  OEO_00000242,
     <http://purl.obolibrary.org/obo/BFO_0000050>  OEO_00010046
    
    
Individual: OEO_00010173

    Annotations: 
        OEO_00010037 "CRF 2.H",
        <http://purl.obolibrary.org/obo/IAO_0000115> "The CRF sector (IPCC 2006) 'industrial processes and product use - other' is an industry sector defined by the 2006 IPCC Guidelines for National Greenhouse Gas Inventories",
        <http://purl.obolibrary.org/obo/IAO_0000233> "issue: https://github.com/OpenEnergyPlatform/ontology/issues/858
pull request: https://github.com/OpenEnergyPlatform/ontology/pull/941

move to oeo-sector 
issue: https://github.com/OpenEnergyPlatform/ontology/issues/1399
pull request: https://github.com/OpenEnergyPlatform/ontology/pull/1724",
        rdfs:label "CRF sector (IPCC 2006): industrial processes and product use - other"@en
    
    Types: 
        OEO_00000227
    
    Facts:  
     OEO_00000504  OEO_00000242,
     <http://purl.obolibrary.org/obo/BFO_0000050>  OEO_00010046
    
    
Individual: OEO_00010174

    Annotations: 
        OEO_00010037 "CRF 5.A",
        <http://purl.obolibrary.org/obo/IAO_0000115> "The CRF sector (IPCC 2006) 'solid waste disposal' is a waste and wastewater sector defined by the 2006 IPCC Guidelines for National Greenhouse Gas Inventories:
Methane is produced from anaerobic microbial decomposition of organic matter in solid waste disposal sites.",
        <http://purl.obolibrary.org/obo/IAO_0000119> "2006 IPCC Guidelines for National Greenhouse Gas Inventories, Volume 1, Chapter 8.5, https://www.ipcc-nggip.iges.or.jp/public/2006gl/",
        <http://purl.obolibrary.org/obo/IAO_0000233> "issue: https://github.com/OpenEnergyPlatform/ontology/issues/858
pull request: https://github.com/OpenEnergyPlatform/ontology/pull/941

move to oeo-sector 
issue: https://github.com/OpenEnergyPlatform/ontology/issues/1399
pull request: https://github.com/OpenEnergyPlatform/ontology/pull/1724",
        rdfs:label "CRF sector (IPCC 2006): solid waste disposal"@en
    
    Types: 
        OEO_00010036
    
    Facts:  
     OEO_00000504  OEO_00000242,
     <http://purl.obolibrary.org/obo/BFO_0000050>  OEO_00010049
    
    
Individual: OEO_00010175

    Annotations: 
        OEO_00010037 "CRF 5.B",
        <http://purl.obolibrary.org/obo/IAO_0000115> "The CRF sector (IPCC 2006) 'biological treatment of solid waste' is a waste and wastewater sector defined by the 2006 IPCC Guidelines for National Greenhouse Gas Inventories:
Solid waste composting and other biological treatment. Emissions from biogas facilities (anaerobic digestion) with energy production are reported in the Energy Sector (1A4).",
        <http://purl.obolibrary.org/obo/IAO_0000119> "2006 IPCC Guidelines for National Greenhouse Gas Inventories, Volume 1, Chapter 8.5, https://www.ipcc-nggip.iges.or.jp/public/2006gl/",
        <http://purl.obolibrary.org/obo/IAO_0000233> "issue: https://github.com/OpenEnergyPlatform/ontology/issues/858
pull request: https://github.com/OpenEnergyPlatform/ontology/pull/941

move to oeo-sector 
issue: https://github.com/OpenEnergyPlatform/ontology/issues/1399
pull request: https://github.com/OpenEnergyPlatform/ontology/pull/1724",
        rdfs:label "CRF sector (IPCC 2006): biological treatment of solid waste"@en
    
    Types: 
        OEO_00010036
    
    Facts:  
     OEO_00000504  OEO_00000242,
     <http://purl.obolibrary.org/obo/BFO_0000050>  OEO_00010049
    
    
Individual: OEO_00010176

    Annotations: 
        OEO_00010037 "CRF 5.C",
        <http://purl.obolibrary.org/obo/IAO_0000115> "The CRF sector (IPCC 2006) 'incineration and open burning of waste' is a waste and wastewater sector defined by the 2006 IPCC Guidelines for National Greenhouse Gas Inventories:
Incineration of waste and open burning waste, not including waste-to-energy facilities.",
        <http://purl.obolibrary.org/obo/IAO_0000119> "2006 IPCC Guidelines for National Greenhouse Gas Inventories, Volume 1, Chapter 8.5, https://www.ipcc-nggip.iges.or.jp/public/2006gl/",
        <http://purl.obolibrary.org/obo/IAO_0000233> "issue: https://github.com/OpenEnergyPlatform/ontology/issues/858
pull request: https://github.com/OpenEnergyPlatform/ontology/pull/941

move to oeo-sector 
issue: https://github.com/OpenEnergyPlatform/ontology/issues/1399
pull request: https://github.com/OpenEnergyPlatform/ontology/pull/1724",
        rdfs:label "CRF sector (IPCC 2006): incineration and open burning of waste"@en
    
    Types: 
        OEO_00010036
    
    Facts:  
     OEO_00000504  OEO_00000242,
     <http://purl.obolibrary.org/obo/BFO_0000050>  OEO_00010049
    
    
Individual: OEO_00010177

    Annotations: 
        OEO_00010037 "CRF 5.D",
        <http://purl.obolibrary.org/obo/IAO_0000115> "The CRF sector (IPCC 2006) 'waste water treatment and discharge' is a waste and wastewater sector defined by the 2006 IPCC Guidelines for National Greenhouse Gas Inventories:
Methane is produced from anaerobic decomposition of organic matter by bacteria in sewage facilities and from food processing and other industrial facilities during wastewater treatment. N2O is also produced by bacteria
(denitrification and nitrification) in wastewater treatment and discharge.",
        <http://purl.obolibrary.org/obo/IAO_0000119> "2006 IPCC Guidelines for National Greenhouse Gas Inventories, Volume 1, Chapter 8.5, https://www.ipcc-nggip.iges.or.jp/public/2006gl/",
        <http://purl.obolibrary.org/obo/IAO_0000233> "issue: https://github.com/OpenEnergyPlatform/ontology/issues/858
pull request: https://github.com/OpenEnergyPlatform/ontology/pull/941

move to oeo-sector 
issue: https://github.com/OpenEnergyPlatform/ontology/issues/1399
pull request: https://github.com/OpenEnergyPlatform/ontology/pull/1724",
        rdfs:label "CRF sector (IPCC 2006): waste water treatment and discharge"@en
    
    Types: 
        OEO_00010036
    
    Facts:  
     OEO_00000504  OEO_00000242,
     <http://purl.obolibrary.org/obo/BFO_0000050>  OEO_00010049
    
    
Individual: OEO_00010178

    Annotations: 
        OEO_00010037 "CRF 5.E",
        <http://purl.obolibrary.org/obo/IAO_0000115> "The CRF sector (IPCC 2006) 'waste - other' is a waste and wastewater sector defined by the 2006 IPCC Guidelines for National Greenhouse Gas Inventories",
        <http://purl.obolibrary.org/obo/IAO_0000119> "2006 IPCC Guidelines for National Greenhouse Gas Inventories, Volume 1, Chapter 8.5, https://www.ipcc-nggip.iges.or.jp/public/2006gl/",
        <http://purl.obolibrary.org/obo/IAO_0000233> "issue: https://github.com/OpenEnergyPlatform/ontology/issues/858
pull request: https://github.com/OpenEnergyPlatform/ontology/pull/941

move to oeo-sector 
issue: https://github.com/OpenEnergyPlatform/ontology/issues/1399
pull request: https://github.com/OpenEnergyPlatform/ontology/pull/1724",
        rdfs:label "CRF sector (IPCC 2006): waste - other"@en
    
    Types: 
        OEO_00010036
    
    Facts:  
     OEO_00000504  OEO_00000242,
     <http://purl.obolibrary.org/obo/BFO_0000050>  OEO_00010049
    
    
Individual: OEO_00010179

    Annotations: 
        OEO_00010037 "CRF 3.A",
        <http://purl.obolibrary.org/obo/IAO_0000115> "The CRF sector (IPCC 2006) 'enteric fermentation' is an agriculture, forestry and land use sector defined by the 2006 IPCC Guidelines for National Greenhouse Gas Inventories:
Methane emissions from herbivores as a by-product of enteric fermentation (a digestive process by which carbohydrates are broken down by micro-organisms into simple molecules for absorption into the bloodstream). Ruminant animals (e.g., cattle, sheep) are major sources with moderate amounts produced from non-ruminant animals (e.g., pigs, horses).",
        <http://purl.obolibrary.org/obo/IAO_0000119> "2006 IPCC Guidelines for National Greenhouse Gas Inventories, Volume 1, Chapter 8.5, https://www.ipcc-nggip.iges.or.jp/public/2006gl/",
        <http://purl.obolibrary.org/obo/IAO_0000233> "issue: https://github.com/OpenEnergyPlatform/ontology/issues/858
pull request: https://github.com/OpenEnergyPlatform/ontology/pull/941

move to oeo-sector 
issue: https://github.com/OpenEnergyPlatform/ontology/issues/1399
pull request: https://github.com/OpenEnergyPlatform/ontology/pull/1724",
        rdfs:label "CRF sector (IPCC 2006): enteric fermentation"@en
    
    Types: 
        OEO_00010035
    
    Facts:  
     OEO_00000504  OEO_00000242,
     <http://purl.obolibrary.org/obo/BFO_0000050>  OEO_00010047
    
    
Individual: OEO_00010180

    Annotations: 
        OEO_00010037 "CRF 3.B",
        <http://purl.obolibrary.org/obo/IAO_0000115> "The CRF sector (IPCC 2006) 'manure management' is an agriculture, forestry and land use sector defined by the 2006 IPCC Guidelines for National Greenhouse Gas Inventories:
Methane and nitrous oxide emissions from the decomposition of manure under low oxygen or anaerobic conditions.",
        <http://purl.obolibrary.org/obo/IAO_0000119> "2006 IPCC Guidelines for National Greenhouse Gas Inventories, Volume 1, Chapter 8.5, https://www.ipcc-nggip.iges.or.jp/public/2006gl/",
        <http://purl.obolibrary.org/obo/IAO_0000233> "issue: https://github.com/OpenEnergyPlatform/ontology/issues/858
pull request: https://github.com/OpenEnergyPlatform/ontology/pull/941

move to oeo-sector 
issue: https://github.com/OpenEnergyPlatform/ontology/issues/1399
pull request: https://github.com/OpenEnergyPlatform/ontology/pull/1724",
        rdfs:label "CRF sector (IPCC 2006): manure management"@en
    
    Types: 
        OEO_00010035
    
    Facts:  
     OEO_00000504  OEO_00000242,
     <http://purl.obolibrary.org/obo/BFO_0000050>  OEO_00010047
    
    
Individual: OEO_00010181

    Annotations: 
        OEO_00010037 "CRF 3.C",
        <http://purl.obolibrary.org/obo/IAO_0000115> "The CRF sector (IPCC 2006) 'rice cultivation' is an agriculture, forestry and land use sector defined by the 2006 IPCC Guidelines for National Greenhouse Gas Inventories:
Methane (CH4) emissions from anaerobic decomposition of organic material in flooded rice fields.",
        <http://purl.obolibrary.org/obo/IAO_0000119> "2006 IPCC Guidelines for National Greenhouse Gas Inventories, Volume 1, Chapter 8.5, https://www.ipcc-nggip.iges.or.jp/public/2006gl/",
        <http://purl.obolibrary.org/obo/IAO_0000233> "issue: https://github.com/OpenEnergyPlatform/ontology/issues/858
pull request: https://github.com/OpenEnergyPlatform/ontology/pull/941

move to oeo-sector 
issue: https://github.com/OpenEnergyPlatform/ontology/issues/1399
pull request: https://github.com/OpenEnergyPlatform/ontology/pull/1724",
        rdfs:label "CRF sector (IPCC 2006): rice cultivation"@en
    
    Types: 
        OEO_00010035
    
    Facts:  
     OEO_00000504  OEO_00000242,
     <http://purl.obolibrary.org/obo/BFO_0000050>  OEO_00010047
    
    
Individual: OEO_00010182

    Annotations: 
        OEO_00010037 "CRF 3.D",
        <http://purl.obolibrary.org/obo/IAO_0000115> "The CRF sector (IPCC 2006) 'agricultural soils' is an agriculture, forestry and land use sector defined by the 2006 IPCC Guidelines for National Greenhouse Gas Inventories",
        <http://purl.obolibrary.org/obo/IAO_0000233> "issue: https://github.com/OpenEnergyPlatform/ontology/issues/858
pull request: https://github.com/OpenEnergyPlatform/ontology/pull/941

move to oeo-sector 
issue: https://github.com/OpenEnergyPlatform/ontology/issues/1399
pull request: https://github.com/OpenEnergyPlatform/ontology/pull/1724",
        rdfs:label "CRF sector (IPCC 2006): agricultural soils"@en
    
    Types: 
        OEO_00010035
    
    Facts:  
     OEO_00000504  OEO_00000242,
     <http://purl.obolibrary.org/obo/BFO_0000050>  OEO_00010047
    
    
Individual: OEO_00010183

    Annotations: 
        OEO_00010037 "CRF 3.E",
        <http://purl.obolibrary.org/obo/IAO_0000115> "The CRF sector (IPCC 2006) 'prescribed burning of savannas' is an agriculture, forestry and land use sector defined by the 2006 IPCC Guidelines for National Greenhouse Gas Inventories",
        <http://purl.obolibrary.org/obo/IAO_0000233> "issue: https://github.com/OpenEnergyPlatform/ontology/issues/858
pull request: https://github.com/OpenEnergyPlatform/ontology/pull/941

move to oeo-sector 
issue: https://github.com/OpenEnergyPlatform/ontology/issues/1399
pull request: https://github.com/OpenEnergyPlatform/ontology/pull/1724",
        rdfs:label "CRF sector (IPCC 2006): prescribed burning of savannas"@en
    
    Types: 
        OEO_00010035
    
    Facts:  
     OEO_00000504  OEO_00000242,
     <http://purl.obolibrary.org/obo/BFO_0000050>  OEO_00010047
    
    
Individual: OEO_00010184

    Annotations: 
        OEO_00010037 "CRF 3.F",
        <http://purl.obolibrary.org/obo/IAO_0000115> "The CRF sector (IPCC 2006) 'field burning of agricultural residues' is an agriculture, forestry and land use sector defined by the 2006 IPCC Guidelines for National Greenhouse Gas Inventories:
CO2 emissions from urea application",
        <http://purl.obolibrary.org/obo/IAO_0000119> "2006 IPCC Guidelines for National Greenhouse Gas Inventories, Volume 1, Chapter 8.5, https://www.ipcc-nggip.iges.or.jp/public/2006gl/",
        <http://purl.obolibrary.org/obo/IAO_0000233> "issue: https://github.com/OpenEnergyPlatform/ontology/issues/858
pull request: https://github.com/OpenEnergyPlatform/ontology/pull/941

move to oeo-sector 
issue: https://github.com/OpenEnergyPlatform/ontology/issues/1399
pull request: https://github.com/OpenEnergyPlatform/ontology/pull/1724",
        rdfs:label "CRF sector (IPCC 2006): field burning of agricultural residues"@en
    
    Types: 
        OEO_00010035
    
    Facts:  
     OEO_00000504  OEO_00000242,
     <http://purl.obolibrary.org/obo/BFO_0000050>  OEO_00010047
    
    
Individual: OEO_00010185

    Annotations: 
        OEO_00010037 "CRF 3.G",
        <http://purl.obolibrary.org/obo/IAO_0000115> "The CRF sector (IPCC 2006) 'liming' is an agriculture, forestry and land use sector defined by the 2006 IPCC Guidelines for National Greenhouse Gas Inventories:
CO2 emissions from the use of lime in agricultural soils, managed forest soils or lakes.",
        <http://purl.obolibrary.org/obo/IAO_0000119> "2006 IPCC Guidelines for National Greenhouse Gas Inventories, Volume 1, Chapter 8.5, https://www.ipcc-nggip.iges.or.jp/public/2006gl/",
        <http://purl.obolibrary.org/obo/IAO_0000233> "issue: https://github.com/OpenEnergyPlatform/ontology/issues/858
pull request: https://github.com/OpenEnergyPlatform/ontology/pull/941

move to oeo-sector 
issue: https://github.com/OpenEnergyPlatform/ontology/issues/1399
pull request: https://github.com/OpenEnergyPlatform/ontology/pull/1724",
        rdfs:label "CRF sector (IPCC 2006): liming"@en
    
    Types: 
        OEO_00010035
    
    Facts:  
     OEO_00000504  OEO_00000242,
     <http://purl.obolibrary.org/obo/BFO_0000050>  OEO_00010047
    
    
Individual: OEO_00010186

    Annotations: 
        OEO_00010037 "CRF 3.H",
        <http://purl.obolibrary.org/obo/IAO_0000115> "The CRF sector (IPCC 2006) 'urea application' is an agriculture, forestry and land use sector defined by the 2006 IPCC Guidelines for National Greenhouse Gas Inventories",
        <http://purl.obolibrary.org/obo/IAO_0000233> "issue: https://github.com/OpenEnergyPlatform/ontology/issues/858
pull request: https://github.com/OpenEnergyPlatform/ontology/pull/941

move to oeo-sector 
issue: https://github.com/OpenEnergyPlatform/ontology/issues/1399
pull request: https://github.com/OpenEnergyPlatform/ontology/pull/1724",
        rdfs:label "CRF sector (IPCC 2006): urea application"@en
    
    Types: 
        OEO_00010035
    
    Facts:  
     OEO_00000504  OEO_00000242,
     <http://purl.obolibrary.org/obo/BFO_0000050>  OEO_00010047
    
    
Individual: OEO_00010187

    Annotations: 
        OEO_00010037 "CRF 3.I",
        <http://purl.obolibrary.org/obo/IAO_0000115> "The CRF sector (IPCC 2006) 'other carbon-containing fertilizers' is an agriculture, forestry and land use sector defined by the 2006 IPCC Guidelines for National Greenhouse Gas Inventories",
        <http://purl.obolibrary.org/obo/IAO_0000233> "issue: https://github.com/OpenEnergyPlatform/ontology/issues/858
pull request: https://github.com/OpenEnergyPlatform/ontology/pull/941

move to oeo-sector 
issue: https://github.com/OpenEnergyPlatform/ontology/issues/1399
pull request: https://github.com/OpenEnergyPlatform/ontology/pull/1724",
        rdfs:label "CRF sector (IPCC 2006): other carbon-containing fertilizers"@en
    
    Types: 
        OEO_00010035
    
    Facts:  
     OEO_00000504  OEO_00000242,
     <http://purl.obolibrary.org/obo/BFO_0000050>  OEO_00010047
    
    
Individual: OEO_00010188

    Annotations: 
        OEO_00010037 "CRF 3.J",
        <http://purl.obolibrary.org/obo/IAO_0000115> "The CRF sector (IPCC 2006) 'agriculture - other' is an agriculture, forestry and land use sector defined by the 2006 IPCC Guidelines for National Greenhouse Gas Inventories",
        <http://purl.obolibrary.org/obo/IAO_0000233> "issue: https://github.com/OpenEnergyPlatform/ontology/issues/858
pull request: https://github.com/OpenEnergyPlatform/ontology/pull/941

move to oeo-sector 
issue: https://github.com/OpenEnergyPlatform/ontology/issues/1399
pull request: https://github.com/OpenEnergyPlatform/ontology/pull/1724",
        rdfs:label "CRF sector (IPCC 2006): agriculture - other"@en
    
    Types: 
        OEO_00010035
    
    Facts:  
     OEO_00000504  OEO_00000242,
     <http://purl.obolibrary.org/obo/BFO_0000050>  OEO_00010047
    
    
Individual: OEO_00010189

    Annotations: 
        OEO_00010037 "CRF 4.A",
        <http://purl.obolibrary.org/obo/IAO_0000115> "The CRF sector (IPCC 2006) 'forest land' is an agriculture, forestry and land use sector defined by the 2006 IPCC Guidelines for National Greenhouse Gas Inventories:
Emissions and removals from lands with woody vegetation consistent with thresholds used to define forest land in the national GHG inventory, sub-divided into managed and unmanaged, and possibly also by climatic region, soil type and vegetation type as appropriate. It also includes systems with vegetation that currently fall below, but are expected to later exceed, the threshold values used by a country to define the forest land category.",
        <http://purl.obolibrary.org/obo/IAO_0000119> "2006 IPCC Guidelines for National Greenhouse Gas Inventories, Volume 1, Chapter 8.5, https://www.ipcc-nggip.iges.or.jp/public/2006gl/",
        <http://purl.obolibrary.org/obo/IAO_0000233> "issue: https://github.com/OpenEnergyPlatform/ontology/issues/858
pull request: https://github.com/OpenEnergyPlatform/ontology/pull/941

move to oeo-sector 
issue: https://github.com/OpenEnergyPlatform/ontology/issues/1399
pull request: https://github.com/OpenEnergyPlatform/ontology/pull/1724",
        rdfs:label "CRF sector (IPCC 2006): forest land"@en
    
    Types: 
        OEO_00010035
    
    Facts:  
     OEO_00000504  OEO_00000242,
     <http://purl.obolibrary.org/obo/BFO_0000050>  OEO_00010048
    
    
Individual: OEO_00010190

    Annotations: 
        OEO_00010037 "CRF 4.B",
        <http://purl.obolibrary.org/obo/IAO_0000115> "The CRF sector (IPCC 2006) 'cropland' is an agriculture, forestry and land use sector defined by the 2006 IPCC Guidelines for National Greenhouse Gas Inventories:
Emissions and removals from arable and tillage land, rice fields, and agro-forestry systems where vegetation falls below the thresholds used for the forest land category.",
        <http://purl.obolibrary.org/obo/IAO_0000119> "2006 IPCC Guidelines for National Greenhouse Gas Inventories, Volume 1, Chapter 8.5, https://www.ipcc-nggip.iges.or.jp/public/2006gl/",
        <http://purl.obolibrary.org/obo/IAO_0000233> "issue: https://github.com/OpenEnergyPlatform/ontology/issues/858
pull request: https://github.com/OpenEnergyPlatform/ontology/pull/941

move to oeo-sector 
issue: https://github.com/OpenEnergyPlatform/ontology/issues/1399
pull request: https://github.com/OpenEnergyPlatform/ontology/pull/1724",
        rdfs:label "CRF sector (IPCC 2006): cropland"@en
    
    Types: 
        OEO_00010035
    
    Facts:  
     OEO_00000504  OEO_00000242,
     <http://purl.obolibrary.org/obo/BFO_0000050>  OEO_00010048
    
    
Individual: OEO_00010191

    Annotations: 
        OEO_00010037 "CRF 4.C",
        <http://purl.obolibrary.org/obo/IAO_0000115> "The CRF sector (IPCC 2006) 'grassland' is an agriculture, forestry and land use sector defined by the 2006 IPCC Guidelines for National Greenhouse Gas Inventories:
Emissions and removals from rangelands and pasture land that is not considered cropland. It also includes systems with woody vegetation that fall below the threshold values used in the forest land category and are not expected to exceed them, without human intervention. The category also includes all grassland from wild lands to recreational areas as well as agricultural and silvi-pastural systems, subdivided into managed and unmanaged, consistent with national definitions.",
        <http://purl.obolibrary.org/obo/IAO_0000119> "2006 IPCC Guidelines for National Greenhouse Gas Inventories, Volume 1, Chapter 8.5, https://www.ipcc-nggip.iges.or.jp/public/2006gl/",
        <http://purl.obolibrary.org/obo/IAO_0000233> "issue: https://github.com/OpenEnergyPlatform/ontology/issues/858
pull request: https://github.com/OpenEnergyPlatform/ontology/pull/941

move to oeo-sector 
issue: https://github.com/OpenEnergyPlatform/ontology/issues/1399
pull request: https://github.com/OpenEnergyPlatform/ontology/pull/1724",
        rdfs:label "CRF sector (IPCC 2006): grassland"@en
    
    Types: 
        OEO_00010035
    
    Facts:  
     OEO_00000504  OEO_00000242,
     <http://purl.obolibrary.org/obo/BFO_0000050>  OEO_00010048
    
    
Individual: OEO_00010192

    Annotations: 
        OEO_00010037 "CRF 4.D",
        <http://purl.obolibrary.org/obo/IAO_0000115> "The CRF sector (IPCC 2006) 'wetlands' is an agriculture, forestry and land use sector defined by the 2006 IPCC Guidelines for National Greenhouse Gas Inventories:
Emissions from land that is covered or saturated by water for all or part of the year (e.g., peatland) and that does not fall into the forest land, cropland, grassland or settlements categories. The category can be subdivided into managed and unmanaged according to national definitions. It includes reservoirs as a managed sub-division and natural rivers and lakes as unmanaged sub-divisions.",
        <http://purl.obolibrary.org/obo/IAO_0000119> "2006 IPCC Guidelines for National Greenhouse Gas Inventories, Volume 1, Chapter 8.5, https://www.ipcc-nggip.iges.or.jp/public/2006gl/",
        <http://purl.obolibrary.org/obo/IAO_0000233> "issue: https://github.com/OpenEnergyPlatform/ontology/issues/858
pull request: https://github.com/OpenEnergyPlatform/ontology/pull/941

move to oeo-sector 
issue: https://github.com/OpenEnergyPlatform/ontology/issues/1399
pull request: https://github.com/OpenEnergyPlatform/ontology/pull/1724",
        rdfs:label "CRF sector (IPCC 2006): wetlands"@en
    
    Types: 
        OEO_00010035
    
    Facts:  
     OEO_00000504  OEO_00000242,
     <http://purl.obolibrary.org/obo/BFO_0000050>  OEO_00010048
    
    
Individual: OEO_00010193

    Annotations: 
        OEO_00010037 "CRF 4.E",
        <http://purl.obolibrary.org/obo/IAO_0000115> "The CRF sector (IPCC 2006) 'settlements' is an agriculture, forestry and land use sector defined by the 2006 IPCC Guidelines for National Greenhouse Gas Inventories:
Emissions and removals from all developed land, including transportation infrastructure and human settlements of any size, unless they are already included under other categories.",
        <http://purl.obolibrary.org/obo/IAO_0000119> "2006 IPCC Guidelines for National Greenhouse Gas Inventories, Volume 1, Chapter 8.5, https://www.ipcc-nggip.iges.or.jp/public/2006gl/",
        <http://purl.obolibrary.org/obo/IAO_0000233> "issue: https://github.com/OpenEnergyPlatform/ontology/issues/858
pull request: https://github.com/OpenEnergyPlatform/ontology/pull/941

move to oeo-sector 
issue: https://github.com/OpenEnergyPlatform/ontology/issues/1399
pull request: https://github.com/OpenEnergyPlatform/ontology/pull/1724",
        rdfs:label "CRF sector (IPCC 2006): settlements"@en
    
    Types: 
        OEO_00010035
    
    Facts:  
     OEO_00000504  OEO_00000242,
     <http://purl.obolibrary.org/obo/BFO_0000050>  OEO_00010048
    
    
Individual: OEO_00010194

    Annotations: 
        OEO_00010037 "CRF 4.F",
        <http://purl.obolibrary.org/obo/IAO_0000115> "The CRF sector (IPCC 2006) 'other land' is an agriculture, forestry and land use sector defined by the 2006 IPCC Guidelines for National Greenhouse Gas Inventories:
Emissions and removals from bare soil, rock, ice, and all unmanaged land areas that do not fall into any of the other five categories.",
        <http://purl.obolibrary.org/obo/IAO_0000119> "2006 IPCC Guidelines for National Greenhouse Gas Inventories, Volume 1, Chapter 8.5, https://www.ipcc-nggip.iges.or.jp/public/2006gl/",
        <http://purl.obolibrary.org/obo/IAO_0000233> "issue: https://github.com/OpenEnergyPlatform/ontology/issues/858
pull request: https://github.com/OpenEnergyPlatform/ontology/pull/941

move to oeo-sector 
issue: https://github.com/OpenEnergyPlatform/ontology/issues/1399
pull request: https://github.com/OpenEnergyPlatform/ontology/pull/1724",
        rdfs:label "CRF sector (IPCC 2006): other land"@en
    
    Types: 
        OEO_00010035
    
    Facts:  
     OEO_00000504  OEO_00000242,
     <http://purl.obolibrary.org/obo/BFO_0000050>  OEO_00010048
    
    
Individual: OEO_00010195

    Annotations: 
        OEO_00010037 "CRF 4.G",
        <http://purl.obolibrary.org/obo/IAO_0000115> "The CRF sector (IPCC 2006) 'harvested wood products' is an agriculture, forestry and land use sector defined by the 2006 IPCC Guidelines for National Greenhouse Gas Inventories
CO2 net emissions or removals resulting from Harvest Wood Products.",
        <http://purl.obolibrary.org/obo/IAO_0000119> "2006 IPCC Guidelines for National Greenhouse Gas Inventories, Volume 1, Chapter 8.5, https://www.ipcc-nggip.iges.or.jp/public/2006gl/",
        <http://purl.obolibrary.org/obo/IAO_0000233> "issue: https://github.com/OpenEnergyPlatform/ontology/issues/858
pull request: https://github.com/OpenEnergyPlatform/ontology/pull/941

move to oeo-sector 
issue: https://github.com/OpenEnergyPlatform/ontology/issues/1399
pull request: https://github.com/OpenEnergyPlatform/ontology/pull/1724",
        rdfs:label "CRF sector (IPCC 2006): harvested wood products"@en
    
    Types: 
        OEO_00010035
    
    Facts:  
     OEO_00000504  OEO_00000242,
     <http://purl.obolibrary.org/obo/BFO_0000050>  OEO_00010048
    
    
Individual: OEO_00010196

    Annotations: 
        OEO_00010037 "CRF 4.H",
        <http://purl.obolibrary.org/obo/IAO_0000115> "The CRF sector (IPCC 2006) 'land use, land-use change and forestry - other' is an agriculture, forestry and land use sector defined by the 2006 IPCC Guidelines for National Greenhouse Gas Inventories",
        <http://purl.obolibrary.org/obo/IAO_0000233> "issue: https://github.com/OpenEnergyPlatform/ontology/issues/858
pull request: https://github.com/OpenEnergyPlatform/ontology/pull/941

move to oeo-sector 
issue: https://github.com/OpenEnergyPlatform/ontology/issues/1399
pull request: https://github.com/OpenEnergyPlatform/ontology/pull/1724",
        rdfs:label "CRF sector (IPCC 2006): land use, land-use change and forestry - other"@en
    
    Types: 
        OEO_00010035
    
    Facts:  
     OEO_00000504  OEO_00000242,
     <http://purl.obolibrary.org/obo/BFO_0000050>  OEO_00010048
    
    
Individual: OEO_00010197

    Annotations: 
        <http://purl.obolibrary.org/obo/IAO_0000115> "The CRF sector (IPCC 2006) 'total emissions excluding LULUCF' is a sector defined by the 2006 IPCC Guidelines for National Greenhouse Gas Inventories. It encompasses the following IPCC 2006 sectors: energy; industrial processes and product use; agriculture; waste; and other.",
        
            Annotations: <http://purl.obolibrary.org/obo/IAO_0000116> "Term used by the European Environment Agency (EEA) https://climate-energy.eea.europa.eu/topics/climate-change-mitigation/greenhouse-gas-emissions-inventory/data"
        <http://purl.obolibrary.org/obo/IAO_0000118> "Total emissions: (UNFCCC)",
        <http://purl.obolibrary.org/obo/IAO_0000233> "issue: https://github.com/OpenEnergyPlatform/ontology/issues/928
pull request: https://github.com/OpenEnergyPlatform/ontology/pull/944

move to oeo-sector 
issue: https://github.com/OpenEnergyPlatform/ontology/issues/1399
pull request: https://github.com/OpenEnergyPlatform/ontology/pull/1724",
        rdfs:label "CRF sector (IPCC 2006): total emissions excluding LULUCF"@en
    
    Types: 
        OEO_00000367
    
    Facts:  
     OEO_00000504  OEO_00000242,
     <http://purl.obolibrary.org/obo/BFO_0000051>  OEO_00010038,
     <http://purl.obolibrary.org/obo/BFO_0000051>  OEO_00010046,
     <http://purl.obolibrary.org/obo/BFO_0000051>  OEO_00010047,
     <http://purl.obolibrary.org/obo/BFO_0000051>  OEO_00010049,
     <http://purl.obolibrary.org/obo/BFO_0000051>  OEO_00010050
    
    
Individual: OEO_00010198

    Annotations: 
        <http://purl.obolibrary.org/obo/IAO_0000115> "The CRF sector (IPCC 2006) 'total emissions including LULUCF' is a sector defined by the 2006 IPCC Guidelines for National Greenhouse Gas Inventories. It encompasses the following IPCC 2006 sectors: energy; industrial processes and product use; agriculture; land use, land-use change and forestry; waste; and other.",
        
            Annotations: <http://purl.obolibrary.org/obo/IAO_0000116> "Term used by the European Environment Agency (EEA): https://climate-energy.eea.europa.eu/topics/climate-change-mitigation/greenhouse-gas-emissions-inventory/data"
        <http://purl.obolibrary.org/obo/IAO_0000118> "Total net emissions (UNFCCC)",
        <http://purl.obolibrary.org/obo/IAO_0000233> "issue: https://github.com/OpenEnergyPlatform/ontology/issues/928
pull request: https://github.com/OpenEnergyPlatform/ontology/pull/944

move to oeo-sector 
issue: https://github.com/OpenEnergyPlatform/ontology/issues/1399
pull request: https://github.com/OpenEnergyPlatform/ontology/pull/1724",
        rdfs:label "CRF sector (IPCC 2006): total emissions including LULUCF"@en
    
    Types: 
        OEO_00000367
    
    Facts:  
     OEO_00000504  OEO_00000242,
     <http://purl.obolibrary.org/obo/BFO_0000051>  OEO_00010038,
     <http://purl.obolibrary.org/obo/BFO_0000051>  OEO_00010046,
     <http://purl.obolibrary.org/obo/BFO_0000051>  OEO_00010047,
     <http://purl.obolibrary.org/obo/BFO_0000051>  OEO_00010048,
     <http://purl.obolibrary.org/obo/BFO_0000051>  OEO_00010049,
     <http://purl.obolibrary.org/obo/BFO_0000051>  OEO_00010050
    
    
Individual: OEO_00010199

    Annotations: 
        OEO_00010037 "CRF 1.D",
        <http://purl.obolibrary.org/obo/IAO_0000115> "The CRF sector (IPCC 2006) international bunkers is a transport sector defined by the 2006 IPCC Guidelines for National Greenhouse Gas Inventories. It encompasses international bunkers and multilateral operation.",
        <http://purl.obolibrary.org/obo/IAO_0000233> "issue: https://github.com/OpenEnergyPlatform/ontology/issues/928
pull request: https://github.com/OpenEnergyPlatform/ontology/pull/944

move to oeo-sector 
issue: https://github.com/OpenEnergyPlatform/ontology/issues/1399
pull request: https://github.com/OpenEnergyPlatform/ontology/pull/1724",
        rdfs:label "CRF sector (IPCC 2006): international bunkers and multilateral operations"@en
    
    Types: 
        OEO_00000422,
        
            Annotations: <http://purl.obolibrary.org/obo/IAO_0000233> "issue: https://github.com/OpenEnergyPlatform/ontology/issues/858
pull request: https://github.com/OpenEnergyPlatform/ontology/pull/967"
        OEO_00010232 some OEO_00010227
    
    Facts:  
     OEO_00000504  OEO_00000242,
     <http://purl.obolibrary.org/obo/BFO_0000051>  OEO_00010200,
     <http://purl.obolibrary.org/obo/BFO_0000051>  OEO_00010203
    
    
Individual: OEO_00010200

    Annotations: 
        OEO_00010037 "CRF 1.D.1",
        <http://purl.obolibrary.org/obo/IAO_0000115> "The CRF sector (IPCC 2006) 'international bunkers' is a transport sector defined by the 2006 IPCC Guidelines for National Greenhouse Gas Inventories. It encompasses international aviation and maritime navigation.",
        <http://purl.obolibrary.org/obo/IAO_0000233> "issue: https://github.com/OpenEnergyPlatform/ontology/issues/928
pull request: https://github.com/OpenEnergyPlatform/ontology/pull/944

Make instance of 'international transport sector':
issue: https://github.com/OpenEnergyPlatform/ontology/issues/969
pull request: https://github.com/OpenEnergyPlatform/ontology/pull/1334

move to oeo-sector 
issue: https://github.com/OpenEnergyPlatform/ontology/issues/1399
pull request: https://github.com/OpenEnergyPlatform/ontology/pull/1724",
        rdfs:label "CRF sector (IPCC 2006): international bunkers"@en
    
    Types: 
        OEO_00010320,
        
            Annotations: <http://purl.obolibrary.org/obo/IAO_0000233> "issue: https://github.com/OpenEnergyPlatform/ontology/issues/858
pull request: https://github.com/OpenEnergyPlatform/ontology/pull/967"
        OEO_00010232 some OEO_00010227
    
    Facts:  
     OEO_00000504  OEO_00000242,
     <http://purl.obolibrary.org/obo/BFO_0000051>  OEO_00010201,
     <http://purl.obolibrary.org/obo/BFO_0000051>  OEO_00010202
    
    
Individual: OEO_00010201

    Annotations: 
        OEO_00010037 "CRF 1.D.1.a",
        <http://purl.obolibrary.org/obo/IAO_0000115> "The CRF sector (IPCC 2006) 'international aviation' is a transport sector defined by the 2006 IPCC Guidelines for National Greenhouse Gas Inventories. It encompasses emissions from flights that depart in one country and arrive in a different country.",
        <http://purl.obolibrary.org/obo/IAO_0000119> "2006 IPCC Guidelines for National Greenhouse Gas Inventories, Volume 1, Chapter 8.5, https://www.ipcc-nggip.iges.or.jp/public/2006gl/",
        <http://purl.obolibrary.org/obo/IAO_0000233> "issue: https://github.com/OpenEnergyPlatform/ontology/issues/928
pull request: https://github.com/OpenEnergyPlatform/ontology/pull/944

Make instance of 'international transport sector':
issue: https://github.com/OpenEnergyPlatform/ontology/issues/969
pull request: https://github.com/OpenEnergyPlatform/ontology/pull/1334

move to oeo-sector 
issue: https://github.com/OpenEnergyPlatform/ontology/issues/1399
pull request: https://github.com/OpenEnergyPlatform/ontology/pull/1724",
        rdfs:label "CRF sector (IPCC 2006): international aviation"@en
    
    Types: 
        OEO_00010320,
        
            Annotations: <http://purl.obolibrary.org/obo/IAO_0000233> "issue: https://github.com/OpenEnergyPlatform/ontology/issues/858
pull request: https://github.com/OpenEnergyPlatform/ontology/pull/967"
        OEO_00010232 some OEO_00010227
    
    Facts:  
     OEO_00000504  OEO_00000242,
     <http://purl.obolibrary.org/obo/BFO_0000050>  OEO_00010200
    
    DifferentFrom: 
        OEO_00010059
    
    
Individual: OEO_00010202

    Annotations: 
        OEO_00010037 "CRF 1.D.1.b",
        <http://purl.obolibrary.org/obo/IAO_0000115> "The CRF sector (IPCC 2006) 'maritime navigation' is a transport sector defined by the 2006 IPCC Guidelines for National Greenhouse Gas Inventories. Emissions from fuels used by vessels of all flags that are engaged in international water-borne navigation. The international navigation may take place at sea, on inland lakes and waterways and in coastal waters. It includes emissions from journeys that depart in one country and arrive in a different country. It excludes consumption by fishing vessels.",
        <http://purl.obolibrary.org/obo/IAO_0000119> "2006 IPCC Guidelines for National Greenhouse Gas Inventories, Volume 1, Chapter 8.5, https://www.ipcc-nggip.iges.or.jp/public/2006gl/",
        <http://purl.obolibrary.org/obo/IAO_0000233> "issue: https://github.com/OpenEnergyPlatform/ontology/issues/928
pull request: https://github.com/OpenEnergyPlatform/ontology/pull/944

Make instance of 'international transport sector':
issue: https://github.com/OpenEnergyPlatform/ontology/issues/969
pull request: https://github.com/OpenEnergyPlatform/ontology/pull/1334

move to oeo-sector 
issue: https://github.com/OpenEnergyPlatform/ontology/issues/1399
pull request: https://github.com/OpenEnergyPlatform/ontology/pull/1724",
        rdfs:label "CRF sector (IPCC 2006): maritime navigation"@en
    
    Types: 
        OEO_00010320,
        
            Annotations: <http://purl.obolibrary.org/obo/IAO_0000233> "issue: https://github.com/OpenEnergyPlatform/ontology/issues/858
pull request: https://github.com/OpenEnergyPlatform/ontology/pull/967"
        OEO_00010232 some OEO_00010227
    
    Facts:  
     OEO_00000504  OEO_00000242,
     <http://purl.obolibrary.org/obo/BFO_0000050>  OEO_00010200
    
    DifferentFrom: 
        OEO_00010062
    
    
Individual: OEO_00010203

    Annotations: 
        OEO_00010037 "CRF 1.D.2",
        <http://purl.obolibrary.org/obo/IAO_0000115> "The CRF sector (IPCC 2006) 'multilateral operation' is a transport sector defined by the 2006 IPCC Guidelines for National Greenhouse Gas Inventories:
Emissions from fuels used for aviation and waterborne navigation in multilateral operations pursuant to the Charter of the United Nations.",
        <http://purl.obolibrary.org/obo/IAO_0000119> "2006 IPCC Guidelines for National Greenhouse Gas Inventories, Volume 2, Chapter 3.1, https://www.ipcc-nggip.iges.or.jp/public/2006gl/",
        <http://purl.obolibrary.org/obo/IAO_0000233> "issue: https://github.com/OpenEnergyPlatform/ontology/issues/928
pull request: https://github.com/OpenEnergyPlatform/ontology/pull/944

move to oeo-sector 
issue: https://github.com/OpenEnergyPlatform/ontology/issues/1399
pull request: https://github.com/OpenEnergyPlatform/ontology/pull/1724",
        rdfs:label "CRF sector (IPCC 2006): multilateral operations"@en
    
    Types: 
        OEO_00000422,
        OEO_00010232 some OEO_00010227,
        
            Annotations: <http://purl.obolibrary.org/obo/IAO_0000233> "issue: https://github.com/OpenEnergyPlatform/ontology/issues/858
pull request: https://github.com/OpenEnergyPlatform/ontology/pull/967"
        OEO_00010232 some OEO_00010227
    
    Facts:  
     OEO_00000504  OEO_00000242,
     <http://purl.obolibrary.org/obo/BFO_0000050>  OEO_00010199
    
    
Individual: OEO_00010204

    Annotations: 
        <http://purl.obolibrary.org/obo/IAO_0000115> "The MMR sector division is a sector division defined in Annex XII, Table 1 of Commission Implementing Regulation (EU) 749/2014. It uses CRF sectors (IPCC 2006) and adds further sectors.",
        <http://purl.obolibrary.org/obo/IAO_0000116> "Annex XII, Table 1 of Commission Implementing Regulation (EU) 749/2014 https://eur-lex.europa.eu/legal-content/EN/TXT/HTML/?uri=CELEX:32014R0749&from=EN#d1e32-67-1",
        <http://purl.obolibrary.org/obo/IAO_0000233> "issue: https://github.com/OpenEnergyPlatform/ontology/issues/928
pull request: https://github.com/OpenEnergyPlatform/ontology/pull/944

move to oeo-sector 
issue: https://github.com/OpenEnergyPlatform/ontology/issues/1399
pull request: https://github.com/OpenEnergyPlatform/ontology/pull/1724",
        rdfs:label "MMR sector division"@en
    
    Types: 
        OEO_00000368
    
    Facts:  
     OEO_00000503  OEO_00000242
    
    
Individual: OEO_00010205

    Annotations: 
        <http://purl.obolibrary.org/obo/IAO_0000115> "The MMR sector 'M.International aviation in the EU ETS' is a transport sector that encompasses that part of the international aviation that is regulated by the European Union Emissions Trading System.",
        <http://purl.obolibrary.org/obo/IAO_0000233> "issue: https://github.com/OpenEnergyPlatform/ontology/issues/928
pull request: https://github.com/OpenEnergyPlatform/ontology/pull/944

Make instance of 'international transport sector':
issue: https://github.com/OpenEnergyPlatform/ontology/issues/969
pull request: https://github.com/OpenEnergyPlatform/ontology/pull/1334

move to oeo-sector 
issue: https://github.com/OpenEnergyPlatform/ontology/issues/1399
pull request: https://github.com/OpenEnergyPlatform/ontology/pull/1724",
        rdfs:label "MMR sector: M.International aviation in the EU ETS"@en
    
    Types: 
        OEO_00010320,
        
            Annotations: <http://purl.obolibrary.org/obo/IAO_0000233> "issue: https://github.com/OpenEnergyPlatform/ontology/issues/858
pull request: https://github.com/OpenEnergyPlatform/ontology/pull/967"
        OEO_00010232 some OEO_00010227
    
    Facts:  
     OEO_00000504  OEO_00010204,
     <http://purl.obolibrary.org/obo/BFO_0000050>  OEO_00010133,
      not  OEO_00000504  OEO_00010163
    
    
Individual: OEO_00010206

    Annotations: 
        <http://purl.obolibrary.org/obo/IAO_0000115> "'Total emissions excluding LULUCF and including international aviation' is a sector that encompasses 'CRF sector (IPCC 2006): total emissions excluding LULUCF' and 'CRF sector (IPCC 2006): international bunkers'.",
        
            Annotations: <http://purl.obolibrary.org/obo/IAO_0000116> "Term used by the European Environment Agency (EEA): https://climate-energy.eea.europa.eu/topics/climate-change-mitigation/greenhouse-gas-emissions-inventory/data"
        <http://purl.obolibrary.org/obo/IAO_0000118> "total emissions with international transport (EEA)",
        <http://purl.obolibrary.org/obo/IAO_0000233> "move to oeo-sector 
issue: https://github.com/OpenEnergyPlatform/ontology/issues/1399
pull request: https://github.com/OpenEnergyPlatform/ontology/pull/1724",
        rdfs:label "total emissions excluding LULUCF and including international bunkers"@en
    
    Types: 
        OEO_00000367
    
    Facts:  
     OEO_00000503  OEO_00000242,
     <http://purl.obolibrary.org/obo/BFO_0000051>  OEO_00010197,
     <http://purl.obolibrary.org/obo/BFO_0000051>  OEO_00010200
    
    
Individual: OEO_00010207

    Annotations: 
        <http://purl.obolibrary.org/obo/IAO_0000115> "'Total emissions excluding LULUCF and including international aviation' is a sector that 'CRF sector (IPCC 2006): total emissions including LULUCF' and 'CRF sector (IPCC 2006): international bunkers'.",
        
            Annotations: <http://purl.obolibrary.org/obo/IAO_0000116> "Term used by the European Environment Agency (EEA): https://climate-energy.eea.europa.eu/topics/climate-change-mitigation/greenhouse-gas-emissions-inventory/data"
        <http://purl.obolibrary.org/obo/IAO_0000118> "total net emissions with international transport (EEA)",
        <http://purl.obolibrary.org/obo/IAO_0000233> "move to oeo-sector 
issue: https://github.com/OpenEnergyPlatform/ontology/issues/1399
pull request: https://github.com/OpenEnergyPlatform/ontology/pull/1724",
        rdfs:label "total emissions including LULUCF and including international bunkers"@en
    
    Types: 
        OEO_00000367
    
    Facts:  
     OEO_00000503  OEO_00000242,
     <http://purl.obolibrary.org/obo/BFO_0000051>  OEO_00010198,
     <http://purl.obolibrary.org/obo/BFO_0000051>  OEO_00010200
    
    
Individual: OEO_00010208

    Annotations: 
        <http://purl.obolibrary.org/obo/IAO_0000115> "'Total emissions excluding LULUCF and including international aviation' is a sector that encompasses 'CRF sector (IPCC 2006): total emissions excluding LULUCF' and 'CRF sector (IPCC 2006): international aviation'.",
        <http://purl.obolibrary.org/obo/IAO_0000116> "This definition corresponds to the 2020 emission target of the European Union.",
        
            Annotations: <http://purl.obolibrary.org/obo/IAO_0000116> "Term used by the European Environment Agency (EEA): https://climate-energy.eea.europa.eu/topics/climate-change-mitigation/greenhouse-gas-emissions-inventory/data"
        <http://purl.obolibrary.org/obo/IAO_0000118> "total emissions with international aviation (EU 2020)",
        <http://purl.obolibrary.org/obo/IAO_0000233> "issue: https://github.com/OpenEnergyPlatform/ontology/issues/928
pull request: https://github.com/OpenEnergyPlatform/ontology/pull/944

move to oeo-sector 
issue: https://github.com/OpenEnergyPlatform/ontology/issues/1399
pull request: https://github.com/OpenEnergyPlatform/ontology/pull/1724",
        rdfs:label "total emissions excluding LULUCF and including international aviation"@en
    
    Types: 
        OEO_00000367
    
    Facts:  
     OEO_00000503  OEO_00000242,
     <http://purl.obolibrary.org/obo/BFO_0000051>  OEO_00010197,
     <http://purl.obolibrary.org/obo/BFO_0000051>  OEO_00010201
    
    
Individual: OEO_00010209

    Annotations: 
        <http://purl.obolibrary.org/obo/IAO_0000115> "'Total emissions excluding LULUCF and including international aviation' is a sector that 'CRF sector (IPCC 2006): total emissions including LULUCF' and 'CRF sector (IPCC 2006): international aviation'.",
        <http://purl.obolibrary.org/obo/IAO_0000116> "This definition corresponds to the 2030 emission target as specified in the Nationally Determined Contribution (NDC) of the European Union .",
        
            Annotations: <http://purl.obolibrary.org/obo/IAO_0000116> "Term used by the European Environment Agency (EEA): https://climate-energy.eea.europa.eu/topics/climate-change-mitigation/greenhouse-gas-emissions-inventory/data"
        <http://purl.obolibrary.org/obo/IAO_0000118> "total net emissions with international aviation (NDC)",
        <http://purl.obolibrary.org/obo/IAO_0000233> "issue: https://github.com/OpenEnergyPlatform/ontology/issues/928
pull request: https://github.com/OpenEnergyPlatform/ontology/pull/944

move to oeo-sector 
issue: https://github.com/OpenEnergyPlatform/ontology/issues/1399
pull request: https://github.com/OpenEnergyPlatform/ontology/pull/1724",
        rdfs:label "total emissions including LULUCF and including international aviation"@en
    
    Types: 
        OEO_00000367
    
    Facts:  
     OEO_00000503  OEO_00000242,
     <http://purl.obolibrary.org/obo/BFO_0000051>  OEO_00010198,
     <http://purl.obolibrary.org/obo/BFO_0000051>  OEO_00010201
    
    
Individual: OEO_00010228

    Annotations: 
        <http://purl.obolibrary.org/obo/IAO_0000115> "The CRF sector (IPCC 2006): 'CO2 emissions from biomass' is a sector defined by the 2006 IPCC Guidelines for National Greenhouse Gas Inventories: CO2 emissions from biomass combustion are not included in national totals, but are recorded as an information item for cross-checking purposes as well as avoiding double counting.",
        <http://purl.obolibrary.org/obo/IAO_0000119> "2006 IPCC Guidelines for National Greenhouse Gas Inventories, Volume 2, Chapter 1, https://www.ipcc-nggip.iges.or.jp/public/2006gl/",
        <http://purl.obolibrary.org/obo/IAO_0000233> "issue: https://github.com/OpenEnergyPlatform/ontology/issues/858
pull request: https://github.com/OpenEnergyPlatform/ontology/pull/967

move to oeo-sector 
issue: https://github.com/OpenEnergyPlatform/ontology/issues/1399
pull request: https://github.com/OpenEnergyPlatform/ontology/pull/1724",
        rdfs:label "CRF sector (IPCC 2006): CO2 emissions from biomass"@en
    
    Types: 
        OEO_00000367,
        OEO_00010232 some OEO_00010227
    
    Facts:  
     OEO_00000504  OEO_00000242
    
    
Individual: OEO_00010229

    Annotations: 
        <http://purl.obolibrary.org/obo/IAO_0000115> "The CRF sector (IPCC 2006): 'CO2 captured' is a sector defined by the 2006 IPCC Guidelines for National Greenhouse Gas Inventories: It encompasses the total amount of CO2 captured for storage.",
        <http://purl.obolibrary.org/obo/IAO_0000119> "2006 IPCC Guidelines for National Greenhouse Gas Inventories, Volume 2, Chapter 5.9, https://www.ipcc-nggip.iges.or.jp/public/2006gl/",
        <http://purl.obolibrary.org/obo/IAO_0000233> "issue: https://github.com/OpenEnergyPlatform/ontology/issues/858
pull request: https://github.com/OpenEnergyPlatform/ontology/pull/967

move to oeo-sector 
issue: https://github.com/OpenEnergyPlatform/ontology/issues/1399
pull request: https://github.com/OpenEnergyPlatform/ontology/pull/1724",
        rdfs:label "CRF sector (IPCC 2006): CO2 captured"@en
    
    Types: 
        OEO_00000367,
        OEO_00010232 some OEO_00010227
    
    Facts:  
     OEO_00000504  OEO_00000242
    
    DifferentFrom: 
        OEO_00010058
    
    
Individual: OEO_00010230

    Annotations: 
        <http://purl.obolibrary.org/obo/IAO_0000115> "The CRF sector (IPCC 2006): 'indirect CO2' is a sector defined by the 2006 IPCC Guidelines for National Greenhouse Gas Inventories: It encompasses Methane, carbon monoxide (CO) or NMVOC emissions that will eventually be oxidised to CO2 in the atmosphere.",
        <http://purl.obolibrary.org/obo/IAO_0000119> "2006 IPCC Guidelines for National Greenhouse Gas Inventories, Volume 1, Chapter 7.2.1.5, https://www.ipcc-nggip.iges.or.jp/public/2006gl/",
        <http://purl.obolibrary.org/obo/IAO_0000233> "issue: https://github.com/OpenEnergyPlatform/ontology/issues/858
pull request: https://github.com/OpenEnergyPlatform/ontology/pull/967

move to oeo-sector 
issue: https://github.com/OpenEnergyPlatform/ontology/issues/1399
pull request: https://github.com/OpenEnergyPlatform/ontology/pull/1724",
        rdfs:label "CRF sector (IPCC 2006): indirect CO2"@en
    
    Types: 
        OEO_00000367,
        OEO_00010232 some OEO_00010227
    
    Facts:  
     OEO_00000504  OEO_00000242
    
    
Individual: OEO_00010305

    Annotations: 
        <http://purl.obolibrary.org/obo/IAO_0000115> "The NC/BR sector \"energy\" is a sector defined by an NC/BR sector division that includes all energy use that is not related to transport or industry. The sector includes:
- CRF sector (IPCC 2006): energy industry
- CRF sector (IPCC 2006): fuel combustion - other sectors
- CRF sector (IPCC 2006): fuel combustion - other
- CRF sector (IPCC 2006): fugitive emissions from fuels
- CRF sector (IPCC 2006): CO2 transport and storage",
        <http://purl.obolibrary.org/obo/IAO_0000233> "issue: https://github.com/OpenEnergyPlatform/ontology/issues/1273
pull request: https://github.com/OpenEnergyPlatform/ontology/pull/1317

Improve definition and axioms:
issue: https://github.com/OpenEnergyPlatform/ontology/issues/1449
pull request: https://github.com/OpenEnergyPlatform/ontology/pull/1462

move to oeo-sector 
issue: https://github.com/OpenEnergyPlatform/ontology/issues/1399
pull request: https://github.com/OpenEnergyPlatform/ontology/pull/1724",
        rdfs:label "NC/BR sector: energy"@en
    
    Types: 
        OEO_00000367,
        OEO_00000504 some OEO_00010304
    
    Facts:  
     <http://purl.obolibrary.org/obo/BFO_0000051>  OEO_00010040,
     <http://purl.obolibrary.org/obo/BFO_0000051>  OEO_00010043,
     <http://purl.obolibrary.org/obo/BFO_0000051>  OEO_00010044,
     <http://purl.obolibrary.org/obo/BFO_0000051>  OEO_00010057,
     <http://purl.obolibrary.org/obo/BFO_0000051>  OEO_00010058
    
    
Individual: OEO_00010306

    Annotations: 
        <http://purl.obolibrary.org/obo/IAO_0000115> "The NC/BR sector \"transport\" is a transport sector defined by an NC/BR sector division. It aligns to the CRF sector (IPCC 2006): transport.",
        <http://purl.obolibrary.org/obo/IAO_0000233> "issue: https://github.com/OpenEnergyPlatform/ontology/issues/1273
pull request: https://github.com/OpenEnergyPlatform/ontology/pull/1317

move to oeo-sector 
issue: https://github.com/OpenEnergyPlatform/ontology/issues/1399
pull request: https://github.com/OpenEnergyPlatform/ontology/pull/1724",
        rdfs:label "NC/BR sector: transport"@en
    
    Types: 
        OEO_00000422,
        OEO_00000504 some OEO_00010304
    
    SameAs: 
        OEO_00010042
    
    
Individual: OEO_00010307

    Annotations: 
        <http://purl.obolibrary.org/obo/IAO_0000115> "The NC/BR sector \"industry/industrial processes and product use\" is an industry sector defined by an NC/BR sector division. The sector includes:
- CRF sector (IPCC 2006): manufacture of solid fuels and other energy industries
- CRF sector (IPCC 2006): industrial processes and product use",
        <http://purl.obolibrary.org/obo/IAO_0000233> "issue: https://github.com/OpenEnergyPlatform/ontology/issues/1273
pull request: https://github.com/OpenEnergyPlatform/ontology/pull/1317

Improve definition and axioms:
issue: https://github.com/OpenEnergyPlatform/ontology/issues/1449
pull request: https://github.com/OpenEnergyPlatform/ontology/pull/1462

move to oeo-sector 
issue: https://github.com/OpenEnergyPlatform/ontology/issues/1399
pull request: https://github.com/OpenEnergyPlatform/ontology/pull/1724",
        rdfs:label "NC/BR sector: industry/industrial processes and product use"@en
    
    Types: 
        OEO_00000227,
        OEO_00000504 some OEO_00010304
    
    Facts:  
     <http://purl.obolibrary.org/obo/BFO_0000051>  OEO_00010046,
     <http://purl.obolibrary.org/obo/BFO_0000051>  OEO_00010160
    
    
Individual: OEO_00010308

    Annotations: 
        <http://purl.obolibrary.org/obo/IAO_0000115> "The NC/BR sector \"agriculture\" is an agriculture, forestry and land use sector defined by an NC/BR sector division. It aligns to the CRF sector (IPCC 2006): agriculture.",
        <http://purl.obolibrary.org/obo/IAO_0000233> "issue: https://github.com/OpenEnergyPlatform/ontology/issues/1273
pull request: https://github.com/OpenEnergyPlatform/ontology/pull/1317

Improve definition and axioms:
issue: https://github.com/OpenEnergyPlatform/ontology/issues/1449
pull request: https://github.com/OpenEnergyPlatform/ontology/pull/1462

move to oeo-sector 
issue: https://github.com/OpenEnergyPlatform/ontology/issues/1399
pull request: https://github.com/OpenEnergyPlatform/ontology/pull/1724",
        rdfs:label "NC/BR sector: agriculture"@en
    
    Types: 
        OEO_00010035,
        OEO_00000504 some OEO_00010304
    
    SameAs: 
        OEO_00010047
    
    
Individual: OEO_00010309

    Annotations: 
        <http://purl.obolibrary.org/obo/IAO_0000115> "The NC/BR sector \"forestry/LULUCF\" is an agriculture, forestry and land use sector defined by an NC/BR sector division. It aligns to the CRF sector (IPCC 2006): land use, land-use change and forestry.",
        <http://purl.obolibrary.org/obo/IAO_0000233> "issue: https://github.com/OpenEnergyPlatform/ontology/issues/1273
pull request: https://github.com/OpenEnergyPlatform/ontology/pull/1317

Improve definition and axioms:
issue: https://github.com/OpenEnergyPlatform/ontology/issues/1449
pull request: https://github.com/OpenEnergyPlatform/ontology/pull/1462

move to oeo-sector 
issue: https://github.com/OpenEnergyPlatform/ontology/issues/1399
pull request: https://github.com/OpenEnergyPlatform/ontology/pull/1724",
        rdfs:label "NC/BR sector: forestry/LULUCF"@en
    
    Types: 
        OEO_00010035,
        OEO_00000504 some OEO_00010304
    
    SameAs: 
        OEO_00010048
    
    
Individual: OEO_00010310

    Annotations: 
        <http://purl.obolibrary.org/obo/IAO_0000115> "The NC/BR sector \"waste management/waste\" is a waste and wastewater sector defined by an NC/BR sector division. It aligns to the CRF sector (IPCC 2006): waste.",
        <http://purl.obolibrary.org/obo/IAO_0000233> "issue: https://github.com/OpenEnergyPlatform/ontology/issues/1273
pull request: https://github.com/OpenEnergyPlatform/ontology/pull/1317

Improve definition and axioms:
issue: https://github.com/OpenEnergyPlatform/ontology/issues/1449
pull request: https://github.com/OpenEnergyPlatform/ontology/pull/1462

move to oeo-sector 
issue: https://github.com/OpenEnergyPlatform/ontology/issues/1399
pull request: https://github.com/OpenEnergyPlatform/ontology/pull/1724",
        rdfs:label "NC/BR sector: waste management/waste"@en
    
    Types: 
        OEO_00010036,
        OEO_00000504 some OEO_00010304
    
    SameAs: 
        OEO_00010049
    
    
Individual: OEO_00010311

    Annotations: 
        <http://purl.obolibrary.org/obo/IAO_0000115> "The NC/BR sector \"other\" is a sector defined by an NC/BR sector division that includes everything that is not included in the other NC/BR sectors. It aligns to the CRF sector (IPCC 2006): other.",
        <http://purl.obolibrary.org/obo/IAO_0000233> "issue: https://github.com/OpenEnergyPlatform/ontology/issues/1273
pull request: https://github.com/OpenEnergyPlatform/ontology/pull/1317

Improve definition and axioms:
issue: https://github.com/OpenEnergyPlatform/ontology/issues/1449
pull request: https://github.com/OpenEnergyPlatform/ontology/pull/1462

move to oeo-sector 
issue: https://github.com/OpenEnergyPlatform/ontology/issues/1399
pull request: https://github.com/OpenEnergyPlatform/ontology/pull/1724",
        rdfs:label "NC/BR sector: other"@en
    
    Types: 
        OEO_00000367,
        OEO_00000504 some OEO_00010304
    
    SameAs: 
        OEO_00010050
    
    
Individual: OEO_00010338

    Annotations: 
        OEO_00010037 "CRF 1.C.1",
        <http://purl.obolibrary.org/obo/IAO_0000115> "The CRF sector (IPCC 2006) 'transport of CO2' is a sector defined by the 2006 IPCC Guidelines for National Greenhouse Gas Inventories:
This comprises fugitive emissions from the systems used to transport captured CO2 from the source to the injection site. These emissions may comprise losses due to fugitive equipment leaks, venting and releases due to pipeline
ruptures or other accidental releases (e.g., temporary storage).",
        <http://purl.obolibrary.org/obo/IAO_0000119> "2006 IPCC Guidelines for National Greenhouse Gas Inventories, Volume 1, Chapter 8.5, https://www.ipcc-nggip.iges.or.jp/public/2006gl/",
        <http://purl.obolibrary.org/obo/IAO_0000233> "move to oeo-sector 
issue: https://github.com/OpenEnergyPlatform/ontology/issues/1399
pull request: https://github.com/OpenEnergyPlatform/ontology/pull/1724",
        rdfs:label "CRF sector (IPCC 2006): transport of CO2"@en
    
    Types: 
        OEO_00000367
    
    Facts:  
     OEO_00000504  OEO_00000242,
     <http://purl.obolibrary.org/obo/BFO_0000050>  OEO_00010058
    
    
Individual: OEO_00010339

    Annotations: 
        OEO_00010037 "CRF 1.C.2",
        <http://purl.obolibrary.org/obo/IAO_0000115> "The CRF sector (IPCC 2006) 'pipelines' is a sector defined by the 2006 IPCC Guidelines for National Greenhouse Gas Inventories:
Fugitive emissions from activities and equipment at the injection site and those from the end containment once the CO2 is placed in storage.",
        <http://purl.obolibrary.org/obo/IAO_0000119> "2006 IPCC Guidelines for National Greenhouse Gas Inventories, Volume 1, Chapter 8.5, https://www.ipcc-nggip.iges.or.jp/public/2006gl/",
        <http://purl.obolibrary.org/obo/IAO_0000233> "move to oeo-sector 
issue: https://github.com/OpenEnergyPlatform/ontology/issues/1399
pull request: https://github.com/OpenEnergyPlatform/ontology/pull/1724",
        rdfs:label "CRF sector (IPCC 2006): injection and storage"@en
    
    Types: 
        OEO_00000367
    
    Facts:  
     OEO_00000504  OEO_00000242,
     <http://purl.obolibrary.org/obo/BFO_0000050>  OEO_00010058
    
    
Individual: OEO_00010340

    Annotations: 
        OEO_00010037 "CRF 1.C.3",
        <http://purl.obolibrary.org/obo/IAO_0000115> "The CRF sector (IPCC 2006) 'CO2 transport and storage' is a sector defined by the 2006 IPCC Guidelines for National Greenhouse Gas Inventories:
Any other emissions from CCS not reported elsewhere.",
        <http://purl.obolibrary.org/obo/IAO_0000119> "2006 IPCC Guidelines for National Greenhouse Gas Inventories, Volume 1, Chapter 8.5, https://www.ipcc-nggip.iges.or.jp/public/2006gl/",
        <http://purl.obolibrary.org/obo/IAO_0000233> "move to oeo-sector 
issue: https://github.com/OpenEnergyPlatform/ontology/issues/1399
pull request: https://github.com/OpenEnergyPlatform/ontology/pull/1724",
        rdfs:label "CRF sector (IPCC 2006): CO2 transport and storage - other"@en
    
    Types: 
        OEO_00000367
    
    Facts:  
     OEO_00000504  OEO_00000242,
     <http://purl.obolibrary.org/obo/BFO_0000050>  OEO_00010058
    
    
Individual: OEO_00010341

    Annotations: 
        OEO_00010037 "CRF 2.A.2",
        <http://purl.obolibrary.org/obo/IAO_0000115> "The CRF sector (IPCC 2006) 'lime production' is an industry sector defined by the 2006 IPCC Guidelines for National Greenhouse Gas Inventories:
Process-related emissions from the production of various types of lime (ISIC: D2694).",
        <http://purl.obolibrary.org/obo/IAO_0000119> "2006 IPCC Guidelines for National Greenhouse Gas Inventories, Volume 1, Chapter 8.5, https://www.ipcc-nggip.iges.or.jp/public/2006gl/",
        <http://purl.obolibrary.org/obo/IAO_0000233> "issue: https://github.com/OpenEnergyPlatform/ontology/issues/1401
pull request: https://github.com/OpenEnergyPlatform/ontology/pull/1440

move to oeo-sector 
issue: https://github.com/OpenEnergyPlatform/ontology/issues/1399
pull request: https://github.com/OpenEnergyPlatform/ontology/pull/1724",
        rdfs:label "CRF sector (IPCC 2006): lime production"@en
    
    Types: 
        OEO_00000227
    
    Facts:  
     OEO_00000504  OEO_00000242,
     <http://purl.obolibrary.org/obo/BFO_0000050>  OEO_00010164
    
    
Individual: OEO_00010342

    Annotations: 
        OEO_00010037 "CRF 2.A.3",
        <http://purl.obolibrary.org/obo/IAO_0000115> "The CRF sector (IPCC 2006) 'glass production' is an industry sector defined by the 2006 IPCC Guidelines for National Greenhouse Gas Inventories:
Process-related emissions from the production of various types of glass (ISIC: D2610).",
        <http://purl.obolibrary.org/obo/IAO_0000119> "2006 IPCC Guidelines for National Greenhouse Gas Inventories, Volume 1, Chapter 8.5, https://www.ipcc-nggip.iges.or.jp/public/2006gl/",
        <http://purl.obolibrary.org/obo/IAO_0000233> "issue: https://github.com/OpenEnergyPlatform/ontology/issues/1401
pull request: https://github.com/OpenEnergyPlatform/ontology/pull/1440

move to oeo-sector 
issue: https://github.com/OpenEnergyPlatform/ontology/issues/1399
pull request: https://github.com/OpenEnergyPlatform/ontology/pull/1724",
        rdfs:label "CRF sector (IPCC 2006): glass production"@en
    
    Types: 
        OEO_00000227
    
    Facts:  
     OEO_00000504  OEO_00000242,
     <http://purl.obolibrary.org/obo/BFO_0000050>  OEO_00010164
    
    
Individual: OEO_00010343

    Annotations: 
        OEO_00010037 "CRF 2.A.4",
        <http://purl.obolibrary.org/obo/IAO_0000115> "The CRF sector (IPCC 2006) 'other process uses of carbonates' is an industry sector defined by the 2006 IPCC Guidelines for National Greenhouse Gas Inventories:
Includes limestone, dolomite and other carbonates etc. Emissions from the use of limestone, dolomite and other carbonates should be included in the industrial source category where they are emitted. Therefore, for example, where a carbonate is used as a flux for iron and steel production, resultant emissions should be reported under 2C1 “Iron and Steel Production” rather than this
subcategory.",
        <http://purl.obolibrary.org/obo/IAO_0000119> "2006 IPCC Guidelines for National Greenhouse Gas Inventories, Volume 1, Chapter 8.5, https://www.ipcc-nggip.iges.or.jp/public/2006gl/",
        <http://purl.obolibrary.org/obo/IAO_0000233> "issue: https://github.com/OpenEnergyPlatform/ontology/issues/1401
pull request: https://github.com/OpenEnergyPlatform/ontology/pull/1440

move to oeo-sector 
issue: https://github.com/OpenEnergyPlatform/ontology/issues/1399
pull request: https://github.com/OpenEnergyPlatform/ontology/pull/1724",
        rdfs:label "CRF sector (IPCC 2006): other process uses of carbonates"@en
    
    Types: 
        OEO_00000227
    
    Facts:  
     OEO_00000504  OEO_00000242,
     <http://purl.obolibrary.org/obo/BFO_0000050>  OEO_00010166
    
    
Individual: OEO_00010344

    Annotations: 
        OEO_00010037 "CRF 2.B.1",
        <http://purl.obolibrary.org/obo/IAO_0000115> "The CRF sector (IPCC 2006) 'ammonia' is an industry sector defined by the 2006 IPCC Guidelines for National Greenhouse Gas Inventories:
Ammonia (NH3) is a major industrial chemical and the most important nitrogenous material produced. Ammonia gas is used directly as a fertilizer, in heat treating, paper pulping, nitric acid and nitrates manufacture, nitric acid ester and nitro compound manufacture, explosives of various types, and as a refrigerant. Amines, amides, and miscellaneous other organic compounds, such as urea, are made from ammonia. The main greenhouse gas emitted from NH3 production is CO2. CO2 used in the production of urea, a downstream process, should be subtracted from the CO2 generated and accounted for in the AFOLU Sector.",
        <http://purl.obolibrary.org/obo/IAO_0000119> "2006 IPCC Guidelines for National Greenhouse Gas Inventories, Volume 1, Chapter 8.5, https://www.ipcc-nggip.iges.or.jp/public/2006gl/",
        <http://purl.obolibrary.org/obo/IAO_0000233> "issue: https://github.com/OpenEnergyPlatform/ontology/issues/1401
pull request: https://github.com/OpenEnergyPlatform/ontology/pull/1440

move to oeo-sector 
issue: https://github.com/OpenEnergyPlatform/ontology/issues/1399
pull request: https://github.com/OpenEnergyPlatform/ontology/pull/1724",
        rdfs:label "CRF sector (IPCC 2006): ammonia production"@en
    
    Types: 
        OEO_00000227
    
    Facts:  
     OEO_00000504  OEO_00000242,
     <http://purl.obolibrary.org/obo/BFO_0000050>  OEO_00010166
    
    
Individual: OEO_00010345

    Annotations: 
        OEO_00010037 "CRF 2.B.2",
        <http://purl.obolibrary.org/obo/IAO_0000115> "The CRF sector (IPCC 2006) 'nitric acid production' is an industry sector defined by the 2006 IPCC Guidelines for National Greenhouse Gas Inventories:
Nitric acid is used as a raw material mainly in the manufacture of nitrogenous-based fertiliser. Nitric acid may also be used in the production of adipic acid and explosives (e.g., dynamite), for metal etching and in the processing of ferrous metals. The main greenhouse gas emitted from HNO3 production is nitrous oxide",
        <http://purl.obolibrary.org/obo/IAO_0000119> "2006 IPCC Guidelines for National Greenhouse Gas Inventories, Volume 1, Chapter 8.5, https://www.ipcc-nggip.iges.or.jp/public/2006gl/",
        <http://purl.obolibrary.org/obo/IAO_0000233> "issue: https://github.com/OpenEnergyPlatform/ontology/issues/1401
pull request: https://github.com/OpenEnergyPlatform/ontology/pull/1440

move to oeo-sector 
issue: https://github.com/OpenEnergyPlatform/ontology/issues/1399
pull request: https://github.com/OpenEnergyPlatform/ontology/pull/1724",
        rdfs:label "CRF sector (IPCC 2006): nitric acid production"@en
    
    Types: 
        OEO_00000227
    
    Facts:  
     OEO_00000504  OEO_00000242,
     <http://purl.obolibrary.org/obo/BFO_0000050>  OEO_00010166
    
    
Individual: OEO_00010346

    Annotations: 
        OEO_00010037 "CRF 2.B.3",
        <http://purl.obolibrary.org/obo/IAO_0000115> "The CRF sector (IPCC 2006) 'adipic acid production is an industry sector defined by the 2006 IPCC Guidelines for National Greenhouse Gas Inventories:
Adipic acid is used in the manufacture of a large number of products including synthetic fibres, coatings, plastics, urethane foams, elastomers and synthetic lubricants. The production of Nylon 6.6 accounts for the bulk of adipic acid
use. The main greenhouse gas emitted from adipic acid production is nitrous oxide.",
        <http://purl.obolibrary.org/obo/IAO_0000119> "2006 IPCC Guidelines for National Greenhouse Gas Inventories, Volume 1, Chapter 8.5, https://www.ipcc-nggip.iges.or.jp/public/2006gl/",
        <http://purl.obolibrary.org/obo/IAO_0000233> "issue: https://github.com/OpenEnergyPlatform/ontology/issues/1401
pull request: https://github.com/OpenEnergyPlatform/ontology/pull/1440

move to oeo-sector 
issue: https://github.com/OpenEnergyPlatform/ontology/issues/1399
pull request: https://github.com/OpenEnergyPlatform/ontology/pull/1724",
        rdfs:label "CRF sector (IPCC 2006): adipic acid production"@en
    
    Types: 
        OEO_00000227
    
    Facts:  
     OEO_00000504  OEO_00000242,
     <http://purl.obolibrary.org/obo/BFO_0000050>  OEO_00010166
    
    
Individual: OEO_00010347

    Annotations: 
        OEO_00010037 "CRF 2.B.4",
        <http://purl.obolibrary.org/obo/IAO_0000115> "The CRF sector (IPCC 2006) 'caprolactam, glyoxal and glyoxylic acid production' is an industry sector defined by the 2006 IPCC Guidelines for National Greenhouse Gas Inventories:
Most of the annual production of caprolactam (NH(CH2)5CO) is consumed as the monomer for nylon-6 fibres and plastics, with a substantial proportion of the fibre used in carpet manufacturing. All commercial processes for the manufacture of caprolactam are based on either toluene or benzene. This subcategory also covers production of glyoxal (ethanedial) and glyoxylic acid production. The main greenhouse gas emitted from this subcategory is nitrous oxide.",
        <http://purl.obolibrary.org/obo/IAO_0000119> "2006 IPCC Guidelines for National Greenhouse Gas Inventories, Volume 1, Chapter 8.5, https://www.ipcc-nggip.iges.or.jp/public/2006gl/",
        <http://purl.obolibrary.org/obo/IAO_0000233> "issue: https://github.com/OpenEnergyPlatform/ontology/issues/1401
pull request: https://github.com/OpenEnergyPlatform/ontology/pull/1440

move to oeo-sector 
issue: https://github.com/OpenEnergyPlatform/ontology/issues/1399
pull request: https://github.com/OpenEnergyPlatform/ontology/pull/1724",
        rdfs:label "CRF sector (IPCC 2006): caprolactam, gloxal and glyoxylic acid production"@en
    
    Types: 
        OEO_00000227
    
    Facts:  
     OEO_00000504  OEO_00000242,
     <http://purl.obolibrary.org/obo/BFO_0000050>  OEO_00010166
    
    
Individual: OEO_00010348

    Annotations: 
        OEO_00010037 "CRF 2.B.5",
        <http://purl.obolibrary.org/obo/IAO_0000115> "The CRF sector (IPCC 2006) 'carbide production' is an industry sector defined by the 2006 IPCC Guidelines for National Greenhouse Gas Inventories:
The production of carbide can result in emissions of CO2, CH4, CO and SO2. Silicon carbide is a significant artificial abrasive. It is produced from silica sand or quartz and petroleum coke. Calcium carbide is used in the production of acetylene, in the manufacture of cyanamide (a minor historical use), and as a reductant in electric arc steel furnaces. It is made from calcium carbonate (limestone) and carbon-containing reductant (petroleum coke).",
        <http://purl.obolibrary.org/obo/IAO_0000119> "2006 IPCC Guidelines for National Greenhouse Gas Inventories, Volume 1, Chapter 8.5, https://www.ipcc-nggip.iges.or.jp/public/2006gl/",
        <http://purl.obolibrary.org/obo/IAO_0000233> "issue: https://github.com/OpenEnergyPlatform/ontology/issues/1401
pull request: https://github.com/OpenEnergyPlatform/ontology/pull/1440

move to oeo-sector 
issue: https://github.com/OpenEnergyPlatform/ontology/issues/1399
pull request: https://github.com/OpenEnergyPlatform/ontology/pull/1724",
        rdfs:label "CRF sector (IPCC 2006): carbide production"@en
    
    Types: 
        OEO_00000227
    
    Facts:  
     OEO_00000504  OEO_00000242,
     <http://purl.obolibrary.org/obo/BFO_0000050>  OEO_00010166
    
    
Individual: OEO_00010349

    Annotations: 
        OEO_00010037 "CRF 2.B.6",
        <http://purl.obolibrary.org/obo/IAO_0000115> "The CRF sector (IPCC 2006) 'titanium dioxide producion' is an industry sector defined by the 2006 IPCC Guidelines for National Greenhouse Gas Inventories:
Titanium dioxide (TiO2) is the most important white pigment. The main use is in paint manufacture followed by paper, plastics, rubber, ceramics, fabrics, floor covering, printing ink, and other miscellaneous uses. The main production process is the chloride route, giving rise to CO2 emissions that are likely to be significant. This category also includes synthetic rutile production using the Becher process, and titanium slag production, both of which are reduction processes using fossil fuels and resulting in CO2 emissions. Synthetic rutile is the major input to TiO2 production using the chloride route.",
        <http://purl.obolibrary.org/obo/IAO_0000119> "2006 IPCC Guidelines for National Greenhouse Gas Inventories, Volume 1, Chapter 8.5, https://www.ipcc-nggip.iges.or.jp/public/2006gl/",
        <http://purl.obolibrary.org/obo/IAO_0000233> "issue: https://github.com/OpenEnergyPlatform/ontology/issues/1401
pull request: https://github.com/OpenEnergyPlatform/ontology/pull/1440

move to oeo-sector 
issue: https://github.com/OpenEnergyPlatform/ontology/issues/1399
pull request: https://github.com/OpenEnergyPlatform/ontology/pull/1724",
        rdfs:label "CRF sector (IPCC 2006): titanium dioxide production"@en
    
    Types: 
        OEO_00000227
    
    Facts:  
     OEO_00000504  OEO_00000242,
     <http://purl.obolibrary.org/obo/BFO_0000050>  OEO_00010166
    
    
Individual: OEO_00010350

    Annotations: 
        OEO_00010037 "CRF 2.B.7",
        <http://purl.obolibrary.org/obo/IAO_0000115> "The CRF sector (IPCC 2006) 'soda ash production' is an industry sector defined by the 2006 IPCC Guidelines for National Greenhouse Gas Inventories:
Soda ash (sodium carbonate, Na2CO3) is a white crystalline solid that is used as a raw material in a large number of industries including glass manufacture, soap and detergents, pulp and paper production and water treatment. Emissions of CO2 from the production of soda ash vary dependent on the manufacturing process. Four different processes may be used to produce soda ash. Three of these processes, monohydrate, sodium sesquicarbonate (trona) and direct carbonation, are referred to as natural processes. The fourth, the Solvay process, is classified as a synthetic process.",
        <http://purl.obolibrary.org/obo/IAO_0000119> "2006 IPCC Guidelines for National Greenhouse Gas Inventories, Volume 1, Chapter 8.5, https://www.ipcc-nggip.iges.or.jp/public/2006gl/",
        <http://purl.obolibrary.org/obo/IAO_0000233> "issue: https://github.com/OpenEnergyPlatform/ontology/issues/1401
pull request: https://github.com/OpenEnergyPlatform/ontology/pull/1440

move to oeo-sector 
issue: https://github.com/OpenEnergyPlatform/ontology/issues/1399
pull request: https://github.com/OpenEnergyPlatform/ontology/pull/1724",
        rdfs:label "CRF sector (IPCC 2006): soda ash production"@en
    
    Types: 
        OEO_00000227
    
    Facts:  
     OEO_00000504  OEO_00000242,
     <http://purl.obolibrary.org/obo/BFO_0000050>  OEO_00010166
    
    
Individual: OEO_00010351

    Annotations: 
        OEO_00010037 "CRF 2.B.8",
        <http://purl.obolibrary.org/obo/IAO_0000115> "The CRF sector (IPCC 2006) 'petrochemical and carbon black production' is an industry sector defined by the 2006 IPCC Guidelines for National Greenhouse Gas Inventories:",
        <http://purl.obolibrary.org/obo/IAO_0000119> "2006 IPCC Guidelines for National Greenhouse Gas Inventories, Volume 1, Chapter 8.5, https://www.ipcc-nggip.iges.or.jp/public/2006gl/",
        <http://purl.obolibrary.org/obo/IAO_0000233> "issue: https://github.com/OpenEnergyPlatform/ontology/issues/1401
pull request: https://github.com/OpenEnergyPlatform/ontology/pull/1440

move to oeo-sector 
issue: https://github.com/OpenEnergyPlatform/ontology/issues/1399
pull request: https://github.com/OpenEnergyPlatform/ontology/pull/1724",
        rdfs:label "CRF sector (IPCC 2006): petrochemical and carbon black production"@en
    
    Types: 
        OEO_00000227
    
    Facts:  
     OEO_00000504  OEO_00000242,
     <http://purl.obolibrary.org/obo/BFO_0000050>  OEO_00010166
    
    
Individual: OEO_00010352

    Annotations: 
        OEO_00010037 "CRF 2.B.9",
        <http://purl.obolibrary.org/obo/IAO_0000115> "The CRF sector (IPCC 2006) 'fluorochemical production' is an industry sector defined by the 2006 IPCC Guidelines for National Greenhouse Gas Inventories:",
        <http://purl.obolibrary.org/obo/IAO_0000119> "2006 IPCC Guidelines for National Greenhouse Gas Inventories, Volume 1, Chapter 8.5, https://www.ipcc-nggip.iges.or.jp/public/2006gl/",
        <http://purl.obolibrary.org/obo/IAO_0000233> "issue: https://github.com/OpenEnergyPlatform/ontology/issues/1401
pull request: https://github.com/OpenEnergyPlatform/ontology/pull/1440

move to oeo-sector 
issue: https://github.com/OpenEnergyPlatform/ontology/issues/1399
pull request: https://github.com/OpenEnergyPlatform/ontology/pull/1724",
        rdfs:label "CRF sector (IPCC 2006): fluorochemical production"@en
    
    Types: 
        OEO_00000227
    
    Facts:  
     OEO_00000504  OEO_00000242,
     <http://purl.obolibrary.org/obo/BFO_0000050>  OEO_00010166
    
    
Individual: OEO_00010353

    Annotations: 
        OEO_00010037 "CRF 2.B.10",
        <http://purl.obolibrary.org/obo/IAO_0000115> "The CRF sector (IPCC 2006) 'chemical industry - other' is an industry sector defined by the 2006 IPCC Guidelines for National Greenhouse Gas Inventories:
For example, gases with global warming potential listed in IPCC assessment reports that do not fall within any categories above could be reported here, if they are estimated.",
        <http://purl.obolibrary.org/obo/IAO_0000119> "2006 IPCC Guidelines for National Greenhouse Gas Inventories, Volume 1, Chapter 8.5, https://www.ipcc-nggip.iges.or.jp/public/2006gl/",
        <http://purl.obolibrary.org/obo/IAO_0000233> "issue: https://github.com/OpenEnergyPlatform/ontology/issues/1401
pull request: https://github.com/OpenEnergyPlatform/ontology/pull/1440

move to oeo-sector 
issue: https://github.com/OpenEnergyPlatform/ontology/issues/1399
pull request: https://github.com/OpenEnergyPlatform/ontology/pull/1724",
        rdfs:label "CRF sector (IPCC 2006): chemical industry - other"@en
    
    Types: 
        OEO_00000227
    
    Facts:  
     OEO_00000504  OEO_00000242,
     <http://purl.obolibrary.org/obo/BFO_0000050>  OEO_00010166
    
    
Individual: OEO_00010354

    Annotations: 
        OEO_00010037 "CRF 2.C.2",
        <http://purl.obolibrary.org/obo/IAO_0000115> "The CRF sector (IPCC 2006) 'ferroalloys' is an industry sector defined by the 2006 IPCC Guidelines for National Greenhouse Gas Inventories:
Ferroalloys production covers emissions from primary metallurgical reduction production of the most common ferroalloys, i.e. ferro-silicon, silicon metal, ferro-manganese, silicon manganese, and ferro-chromium, excluding those
emissions relating to fuel use. From the production of these alloys, carbon dioxide (CO2), nitrous oxide (N2O), and methane (CH4) originating from ore- and reductant raw materials, is emitted.",
        <http://purl.obolibrary.org/obo/IAO_0000119> "2006 IPCC Guidelines for National Greenhouse Gas Inventories, Volume 1, Chapter 8.5, https://www.ipcc-nggip.iges.or.jp/public/2006gl/",
        <http://purl.obolibrary.org/obo/IAO_0000233> "issue: https://github.com/OpenEnergyPlatform/ontology/issues/1401
pull request: https://github.com/OpenEnergyPlatform/ontology/pull/1440

move to oeo-sector 
issue: https://github.com/OpenEnergyPlatform/ontology/issues/1399
pull request: https://github.com/OpenEnergyPlatform/ontology/pull/1724",
        rdfs:label "CRF sector (IPCC 2006): ferroalloys production"@en
    
    Types: 
        OEO_00000227
    
    Facts:  
     OEO_00000504  OEO_00000242,
     <http://purl.obolibrary.org/obo/BFO_0000050>  OEO_00010167
    
    
Individual: OEO_00010355

    Annotations: 
        OEO_00010037 "CRF 2.C.3",
        <http://purl.obolibrary.org/obo/IAO_0000115> "The CRF sector (IPCC 2006) 'aluminium production' is an industry sector defined by the 2006 IPCC Guidelines for National Greenhouse Gas Inventories:
Aluminium Production covers primary production of aluminium, except the emissions related to the use of fuel. Carbon dioxide emissions result from the electrochemical reduction reaction of alumina with a carbon-based anode.
Tetrafluoromethane (CF4) and hexafluoroethane (C2F6) are also produced intermittently. No greenhouse gases are produced in recycling of aluminium other than from the fuels uses for metal remelting. Sulphur hexafluoride (SF6)
emissions are not associated with primary aluminium production; however, casting of some high magnesium containing alloys does result in SF6 emissions and these emissions are accounted for in Section 2C4, Magnesium
Production.",
        <http://purl.obolibrary.org/obo/IAO_0000119> "2006 IPCC Guidelines for National Greenhouse Gas Inventories, Volume 1, Chapter 8.5, https://www.ipcc-nggip.iges.or.jp/public/2006gl/",
        <http://purl.obolibrary.org/obo/IAO_0000233> "issue: https://github.com/OpenEnergyPlatform/ontology/issues/1401
pull request: https://github.com/OpenEnergyPlatform/ontology/pull/1440

move to oeo-sector 
issue: https://github.com/OpenEnergyPlatform/ontology/issues/1399
pull request: https://github.com/OpenEnergyPlatform/ontology/pull/1724",
        rdfs:label "CRF sector (IPCC 2006): aluminium production"@en
    
    Types: 
        OEO_00000227
    
    Facts:  
     OEO_00000504  OEO_00000242,
     <http://purl.obolibrary.org/obo/BFO_0000050>  OEO_00010167
    
    
Individual: OEO_00010356

    Annotations: 
        OEO_00010037 "CRF 2.C.4",
        <http://purl.obolibrary.org/obo/IAO_0000115> "The CRF sector (IPCC 2006) 'magnesium production' is an industry sector defined by the 2006 IPCC Guidelines for National Greenhouse Gas Inventories:
Magnesium production covers GHG emissions related to both primary magnesium production as well as oxidation protection of magnesium metal during processing (recycling and casting), excluding those emissions relating to fuel use. In the primary production of magnesium, carbon dioxide (CO2) is emitted during calcination of dolomite and magnesite raw materials. Primary production of magnesium from non-carbonate raw materials does not emit carbon dioxide. In the processing of liquid magnesium, cover gases containing carbon dioxide (CO2), sulphur hexafluoride (SF6), the hydrofluorocarbon HFC 134a or the fluorinated ketone FK 5-1-12 ( C3F7C(O)C2F5) may be used. Partial
thermal decomposition and/or reaction between these compounds and liquid magnesium generates secondary compounds such as perfluorocarbons (PFCs), which are emitted in addition to unreacted cover gas constituents.",
        <http://purl.obolibrary.org/obo/IAO_0000119> "2006 IPCC Guidelines for National Greenhouse Gas Inventories, Volume 1, Chapter 8.5, https://www.ipcc-nggip.iges.or.jp/public/2006gl/",
        <http://purl.obolibrary.org/obo/IAO_0000233> "issue: https://github.com/OpenEnergyPlatform/ontology/issues/1401
pull request: https://github.com/OpenEnergyPlatform/ontology/pull/1440

move to oeo-sector 
issue: https://github.com/OpenEnergyPlatform/ontology/issues/1399
pull request: https://github.com/OpenEnergyPlatform/ontology/pull/1724",
        rdfs:label "CRF sector (IPCC 2006): magnesium production"@en
    
    Types: 
        OEO_00000227
    
    Facts:  
     OEO_00000504  OEO_00000242,
     <http://purl.obolibrary.org/obo/BFO_0000050>  OEO_00010167
    
    
Individual: OEO_00010357

    Annotations: 
        OEO_00010037 "CRF 2.C.5",
        <http://purl.obolibrary.org/obo/IAO_0000115> "The CRF sector (IPCC 2006) 'lead production' is an industry sector defined by the 2006 IPCC Guidelines for National Greenhouse Gas Inventories:
Lead production covers production by the sintering/smelting process as well as direct smelting. Carbon dioxide emissions result as a product of the use of a variety of carbon-based reducing agents in both production 
processes.",
        <http://purl.obolibrary.org/obo/IAO_0000119> "2006 IPCC Guidelines for National Greenhouse Gas Inventories, Volume 1, Chapter 8.5, https://www.ipcc-nggip.iges.or.jp/public/2006gl/",
        <http://purl.obolibrary.org/obo/IAO_0000233> "issue: https://github.com/OpenEnergyPlatform/ontology/issues/1401
pull request: https://github.com/OpenEnergyPlatform/ontology/pull/1440

move to oeo-sector 
issue: https://github.com/OpenEnergyPlatform/ontology/issues/1399
pull request: https://github.com/OpenEnergyPlatform/ontology/pull/1724",
        rdfs:label "CRF sector (IPCC 2006): lead production"@en
    
    Types: 
        OEO_00000227
    
    Facts:  
     OEO_00000504  OEO_00000242,
     <http://purl.obolibrary.org/obo/BFO_0000050>  OEO_00010167
    
    
Individual: OEO_00010358

    Annotations: 
        OEO_00010037 "CRF 2.C.6",
        <http://purl.obolibrary.org/obo/IAO_0000115> "The CRF sector (IPCC 2006) 'zinc production' is an industry sector defined by the 2006 IPCC Guidelines for National Greenhouse Gas Inventories:
Zinc production covers emissions from both primary production of zinc from ore as well as recovery of zinc from scrap metals, excluding emissions related to fuel use. Following calcination, zinc metal is produced through one of three methods; 1-electro-thermic distillation, 2-pyrometallurgical smelting or 3-electrolysis. If method 1 or 2 is used, carbon dioxide (CO2) is emitted. Method 3 does not result in carbon dioxide emissions. Recovery of zinc from metal scrap often uses the same methods as primary production and may thus produce carbon dioxide emissions, which is included in this section.",
        <http://purl.obolibrary.org/obo/IAO_0000119> "2006 IPCC Guidelines for National Greenhouse Gas Inventories, Volume 1, Chapter 8.5, https://www.ipcc-nggip.iges.or.jp/public/2006gl/",
        <http://purl.obolibrary.org/obo/IAO_0000233> "issue: https://github.com/OpenEnergyPlatform/ontology/issues/1401
pull request: https://github.com/OpenEnergyPlatform/ontology/pull/1440

move to oeo-sector 
issue: https://github.com/OpenEnergyPlatform/ontology/issues/1399
pull request: https://github.com/OpenEnergyPlatform/ontology/pull/1724",
        rdfs:label "CRF sector (IPCC 2006): zinc production"@en
    
    Types: 
        OEO_00000227
    
    Facts:  
     OEO_00000504  OEO_00000242,
     <http://purl.obolibrary.org/obo/BFO_0000050>  OEO_00010167
    
    
Individual: OEO_00010359

    Annotations: 
        OEO_00010037 "CRF 2.C.7",
        <http://purl.obolibrary.org/obo/IAO_0000115> "The CRF sector (IPCC 2006) 'metal industry - other' is an industry sector defined by the 2006 IPCC Guidelines for National Greenhouse Gas Inventories:",
        <http://purl.obolibrary.org/obo/IAO_0000119> "2006 IPCC Guidelines for National Greenhouse Gas Inventories, Volume 1, Chapter 8.5, https://www.ipcc-nggip.iges.or.jp/public/2006gl/",
        <http://purl.obolibrary.org/obo/IAO_0000233> "issue: https://github.com/OpenEnergyPlatform/ontology/issues/1401
pull request: https://github.com/OpenEnergyPlatform/ontology/pull/1440

move to oeo-sector 
issue: https://github.com/OpenEnergyPlatform/ontology/issues/1399
pull request: https://github.com/OpenEnergyPlatform/ontology/pull/1724",
        rdfs:label "CRF sector (IPCC 2006): metal industry - other"@en
    
    Types: 
        OEO_00000227
    
    Facts:  
     OEO_00000504  OEO_00000242,
     <http://purl.obolibrary.org/obo/BFO_0000050>  OEO_00010167
    
    
Individual: OEO_00010363

    Annotations: 
        OEO_00010037 "CRF 2.E.1",
        <http://purl.obolibrary.org/obo/IAO_0000115> "The CRF sector (IPCC 2006) 'integrated circuit or semiconductor' is an industry sector defined by the 2006 IPCC Guidelines for National Greenhouse Gas Inventories:
Emissions of CF4, C2F6, C3F8, c-C4F8, C4F6, C4F8O, C5F8, CHF3, CH2F2, NF3 and SF6 from uses of these gases in Integrated Circuit (IC) manufacturing in rapidly evolving ways and in varying amounts, which depend on product
(e.g., memory or logic devices) and equipment manufacturer.",
        <http://purl.obolibrary.org/obo/IAO_0000119> "2006 IPCC Guidelines for National Greenhouse Gas Inventories, Volume 1, Chapter 8.5, https://www.ipcc-nggip.iges.or.jp/public/2006gl/",
        <http://purl.obolibrary.org/obo/IAO_0000233> "issue: https://github.com/OpenEnergyPlatform/ontology/issues/1401
pull request: https://github.com/OpenEnergyPlatform/ontology/pull/1440

move to oeo-sector 
issue: https://github.com/OpenEnergyPlatform/ontology/issues/1399
pull request: https://github.com/OpenEnergyPlatform/ontology/pull/1724",
        rdfs:label "CRF sector (IPCC 2006): integrated circuit or semiconductor"@en
    
    Types: 
        OEO_00000227
    
    Facts:  
     OEO_00000504  OEO_00000242,
     <http://purl.obolibrary.org/obo/BFO_0000050>  OEO_00010170
    
    
Individual: OEO_00010364

    Annotations: 
        OEO_00010037 "CRF 2.E.2",
        <http://purl.obolibrary.org/obo/IAO_0000115> "The CRF sector (IPCC 2006) 'TFT flat panel display' is an industry sector defined by the 2006 IPCC Guidelines for National Greenhouse Gas Inventories:
Uses and emissions of predominantly CF4, CHF3, NF3 and SF6 during the fabrication of thin-film transistors (TFTs) on glass substrates for flat panel display manufacture. In addition to these gases, C2F6, C3F8 and c-C4F8 may also be used and emitted during the manufacture of thin and smart displays.",
        <http://purl.obolibrary.org/obo/IAO_0000119> "2006 IPCC Guidelines for National Greenhouse Gas Inventories, Volume 1, Chapter 8.5, https://www.ipcc-nggip.iges.or.jp/public/2006gl/",
        <http://purl.obolibrary.org/obo/IAO_0000233> "issue: https://github.com/OpenEnergyPlatform/ontology/issues/1401
pull request: https://github.com/OpenEnergyPlatform/ontology/pull/1440

move to oeo-sector 
issue: https://github.com/OpenEnergyPlatform/ontology/issues/1399
pull request: https://github.com/OpenEnergyPlatform/ontology/pull/1724",
        rdfs:label "CRF sector (IPCC 2006): TFT flat panel display"@en
    
    Types: 
        OEO_00000227
    
    Facts:  
     OEO_00000504  OEO_00000242,
     <http://purl.obolibrary.org/obo/BFO_0000050>  OEO_00010170
    
    
Individual: OEO_00010365

    Annotations: 
        OEO_00010037 "CRF 2.E.3",
        <http://purl.obolibrary.org/obo/IAO_0000115> "The CRF sector (IPCC 2006) 'photovoltaics' is an industry sector defined by the 2006 IPCC Guidelines for National Greenhouse Gas Inventories:
Photovoltaic cell manufacture may use and emit CF4 and C2F6 among others.",
        <http://purl.obolibrary.org/obo/IAO_0000119> "2006 IPCC Guidelines for National Greenhouse Gas Inventories, Volume 1, Chapter 8.5, https://www.ipcc-nggip.iges.or.jp/public/2006gl/",
        <http://purl.obolibrary.org/obo/IAO_0000233> "move to oeo-sector 
issue: https://github.com/OpenEnergyPlatform/ontology/issues/1399
pull request: https://github.com/OpenEnergyPlatform/ontology/pull/1724",
        rdfs:label "CRF sector (IPCC 2006): photovoltaics"@en
    
    Types: 
        OEO_00000227
    
    Facts:  
     OEO_00000504  OEO_00000242,
     <http://purl.obolibrary.org/obo/BFO_0000050>  OEO_00010170
    
    
Individual: OEO_00010366

    Annotations: 
        OEO_00010037 "CRF 2.E.4",
        <http://purl.obolibrary.org/obo/IAO_0000115> "The CRF sector (IPCC 2006) 'heat transfer fluid' is an industry sector defined by the 2006 IPCC Guidelines for National Greenhouse Gas Inventories:
Heat transfer fluids, which include several fully fluorinated carbon compounds (either in pure form or in mixtures) with six or more carbon atoms, used and emitted during IC manufacture, testing and assembly. They are used in chillers, temperature shock testers and vapour phase reflow soldering.",
        <http://purl.obolibrary.org/obo/IAO_0000119> "2006 IPCC Guidelines for National Greenhouse Gas Inventories, Volume 1, Chapter 8.5, https://www.ipcc-nggip.iges.or.jp/public/2006gl/",
        <http://purl.obolibrary.org/obo/IAO_0000233> "issue: https://github.com/OpenEnergyPlatform/ontology/issues/1401
pull request: https://github.com/OpenEnergyPlatform/ontology/pull/1440

move to oeo-sector 
issue: https://github.com/OpenEnergyPlatform/ontology/issues/1399
pull request: https://github.com/OpenEnergyPlatform/ontology/pull/1724",
        rdfs:label "CRF sector (IPCC 2006): heat transfer fluid"@en
    
    Types: 
        OEO_00000227
    
    Facts:  
     OEO_00000504  OEO_00000242,
     <http://purl.obolibrary.org/obo/BFO_0000050>  OEO_00010170
    
    
Individual: OEO_00010367

    Annotations: 
        OEO_00010037 "CRF 2.E.5",
        <http://purl.obolibrary.org/obo/IAO_0000115> "The CRF sector (IPCC 2006) 'electronics industry - other' is an industry sector defined by the 2006 IPCC Guidelines for National Greenhouse Gas Inventories",
        <http://purl.obolibrary.org/obo/IAO_0000119> "2006 IPCC Guidelines for National Greenhouse Gas Inventories, Volume 1, Chapter 8.5, https://www.ipcc-nggip.iges.or.jp/public/2006gl/",
        <http://purl.obolibrary.org/obo/IAO_0000233> "issue: https://github.com/OpenEnergyPlatform/ontology/issues/1401
pull request: https://github.com/OpenEnergyPlatform/ontology/pull/1440

move to oeo-sector 
issue: https://github.com/OpenEnergyPlatform/ontology/issues/1399
pull request: https://github.com/OpenEnergyPlatform/ontology/pull/1724",
        rdfs:label "CRF sector (IPCC 2006): electronics industry - other"@en
    
    Types: 
        OEO_00000227
    
    Facts:  
     OEO_00000504  OEO_00000242,
     <http://purl.obolibrary.org/obo/BFO_0000050>  OEO_00010170
    
    
Individual: OEO_00010368

    Annotations: 
        OEO_00010037 "CRF 2.F.1",
        <http://purl.obolibrary.org/obo/IAO_0000115> "The CRF sector (IPCC 2006) 'refrigeration and air conditioning' is an industry sector defined by the 2006 IPCC Guidelines for National Greenhouse Gas Inventories:
Refrigeration and air-conditioning systems are usually classified in six application domains or categories. These categories utilise different technologies such as heat exchangers, expansion devices, pipings and compressors. The six application domains are domestic refrigeration, commercial refrigeration, industrial processes, transport refrigeration, stationary air conditioning, mobile airconditioning systems. For all these applications, various HFCs are selectively replacing CFCs and HCFCs. For example, in developed countries, HFC-134a has replaced CFC-12 in domestic refrigeration and mobile air conditioning systems, and blends of HFCs such as R-407C (HFC-32/HFC-125/HFC-134a) and R-410A (HFC-32/HFC-125) are replacing HCFC-22 mainly in stationary air conditioning. Other, non HFC substances are used to replace CFCs and HCFCs such as iso-butane in domestic refrigeration or ammonia in industrial refrigeration. HFC- 152a is also being considered for mobile air conditioning in several regions.",
        <http://purl.obolibrary.org/obo/IAO_0000119> "2006 IPCC Guidelines for National Greenhouse Gas Inventories, Volume 1, Chapter 8.5, https://www.ipcc-nggip.iges.or.jp/public/2006gl/",
        <http://purl.obolibrary.org/obo/IAO_0000233> "issue: https://github.com/OpenEnergyPlatform/ontology/issues/1401
pull request: https://github.com/OpenEnergyPlatform/ontology/pull/1440

move to oeo-sector 
issue: https://github.com/OpenEnergyPlatform/ontology/issues/1399
pull request: https://github.com/OpenEnergyPlatform/ontology/pull/1724",
        rdfs:label "CRF sector (IPCC 2006): refrigeration and air conditioning"@en
    
    Types: 
        OEO_00000227
    
    Facts:  
     OEO_00000504  OEO_00000242,
     <http://purl.obolibrary.org/obo/BFO_0000050>  OEO_00010171
    
    
Individual: OEO_00010369

    Annotations: 
        OEO_00010037 "CRF 2.F.2",
        <http://purl.obolibrary.org/obo/IAO_0000115> "The CRF sector (IPCC 2006) 'foam blowing agents' is an industry sector defined by the 2006 IPCC Guidelines for National Greenhouse Gas Inventories:
HFCs are being used as replacements for CFCs and HCFCs in foams, particularly in closed-cell insulation applications. Compounds that are being used include HFC-245fa, HFC-365mfc, HFC-227ea, HFC-134a, and HFC-152a. The processes and applications for which these various HFCs are being used include insulation boards and panels, pipe sections, sprayed systems and onecomponent gap filling foams. For open-cell foams, such as integral skin products for automotive steering wheels and facias, emissions of HFCs used as blowing agents are likely to occur during the manufacturing process. In closedcell foam, emissions not only occur during the manufacturing phase, but usually extend into the in-use phase and often the majority of emission occurs at the endof-life (de-commissioning losses). Accordingly, emissions can occur over a period of up to 50 years or even longer.",
        <http://purl.obolibrary.org/obo/IAO_0000119> "2006 IPCC Guidelines for National Greenhouse Gas Inventories, Volume 1, Chapter 8.5, https://www.ipcc-nggip.iges.or.jp/public/2006gl/",
        <http://purl.obolibrary.org/obo/IAO_0000233> "issue: https://github.com/OpenEnergyPlatform/ontology/issues/1401
pull request: https://github.com/OpenEnergyPlatform/ontology/pull/1440

move to oeo-sector 
issue: https://github.com/OpenEnergyPlatform/ontology/issues/1399
pull request: https://github.com/OpenEnergyPlatform/ontology/pull/1724",
        rdfs:label "CRF sector (IPCC 2006): foam blowing agents"@en
    
    Types: 
        OEO_00000227
    
    Facts:  
     OEO_00000504  OEO_00000242,
     <http://purl.obolibrary.org/obo/BFO_0000050>  OEO_00010171
    
    
Individual: OEO_00010370

    Annotations: 
        OEO_00010037 "CRF 2.F.3",
        <http://purl.obolibrary.org/obo/IAO_0000115> "The CRF sector (IPCC 2006) 'fire protection' is an industry sector defined by the 2006 IPCC Guidelines for National Greenhouse Gas Inventories:
There are two general types of fire protection (fire suppression) equipment that use greenhouse gases as partial replacements for halons: portable (streaming) equipment, and fixed (flooding) equipment. The non-ozone depleting, industrial gases HFCs, PFCs and more recently a fluoroketone are mainly used as substitutes for halons, typically halon 1301, in flooding equipment. PFCs played an early role in halon 1301 replacement but current use is limited to replenishment of previously installed systems. HFCs in portable equipment, typically replacing halon 1211, are available but have achieved very limited market acceptance due primarily to their high cost. PFC use in new portable extinguishers is currently limited to a small amount (few percent) in an HCFC blend.",
        <http://purl.obolibrary.org/obo/IAO_0000119> "2006 IPCC Guidelines for National Greenhouse Gas Inventories, Volume 1, Chapter 8.5, https://www.ipcc-nggip.iges.or.jp/public/2006gl/",
        <http://purl.obolibrary.org/obo/IAO_0000233> "issue: https://github.com/OpenEnergyPlatform/ontology/issues/1401
pull request: https://github.com/OpenEnergyPlatform/ontology/pull/1440

move to oeo-sector 
issue: https://github.com/OpenEnergyPlatform/ontology/issues/1399
pull request: https://github.com/OpenEnergyPlatform/ontology/pull/1724",
        rdfs:label "CRF sector (IPCC 2006): fire protection"@en
    
    Types: 
        OEO_00000227
    
    Facts:  
     OEO_00000504  OEO_00000242,
     <http://purl.obolibrary.org/obo/BFO_0000050>  OEO_00010171
    
    
Individual: OEO_00010371

    Annotations: 
        OEO_00010037 "CRF 2.F.4",
        <http://purl.obolibrary.org/obo/IAO_0000115> "The CRF sector (IPCC 2006) 'aerosols' is an industry sector defined by the 2006 IPCC Guidelines for National Greenhouse Gas Inventories:
Most aerosol packages now contain hydrocarbon (HC) as propellants but, in a small fraction of the total, HFCs and PFCs may be used as propellants or solvents. Emissions from aerosols usually occur shortly after production, on average six months after sale. During the use of aerosols, 100% of the chemical is emitted. The 5 main sources are metered dose inhalers (MDIs), personal care products (e.g. hair care, deodorant, shaving cream), household products (e.g. air-fresheners, oven and fabric cleaners), industrial products (e.g. special cleaning sprays such as those for operating electrical contact, lubricants, pipe-freezers) and other general products (e.g. silly string, tire inflators, claxons), although in some regions the use of such general products is restricted. The HFCs currently used as propellants are HFC 134a, HFC 227ea, and HFC 152a. The substance HFC 43 10mee and a PFC, perfluorohexane, are used as solvents in industrial aerosol products.",
        <http://purl.obolibrary.org/obo/IAO_0000119> "2006 IPCC Guidelines for National Greenhouse Gas Inventories, Volume 1, Chapter 8.5, https://www.ipcc-nggip.iges.or.jp/public/2006gl/",
        <http://purl.obolibrary.org/obo/IAO_0000233> "issue: https://github.com/OpenEnergyPlatform/ontology/issues/1401
pull request: https://github.com/OpenEnergyPlatform/ontology/pull/1440

move to oeo-sector 
issue: https://github.com/OpenEnergyPlatform/ontology/issues/1399
pull request: https://github.com/OpenEnergyPlatform/ontology/pull/1724",
        rdfs:label "CRF sector (IPCC 2006): aerosols"@en
    
    Types: 
        OEO_00000227
    
    Facts:  
     OEO_00000504  OEO_00000242,
     <http://purl.obolibrary.org/obo/BFO_0000050>  OEO_00010171
    
    
Individual: OEO_00010372

    Annotations: 
        OEO_00010037 "CRF 2.F.5",
        <http://purl.obolibrary.org/obo/IAO_0000115> "The CRF sector (IPCC 2006) 'solvents' is an industry sector defined by the 2006 IPCC Guidelines for National Greenhouse Gas Inventories:
HFCs and, to a much lesser extent PFCs, are being used as substitutes for ozone depleting substances (most notably CFC-113). Typical HFCs used are HFC-365mfc and HFC-43-10mee. Use of these fluorinated replacements is much less widespread than the ozone depleting substances they replace. Re-capture and re-use is also much more widely practiced The primary areas of use are precision cleaning, electronics cleaning, metal cleaning and deposition applications. Emissions from aerosols containing solvents should be reported undercategory 2F4 \"Aerosols\" rather than under this category.",
        <http://purl.obolibrary.org/obo/IAO_0000119> "2006 IPCC Guidelines for National Greenhouse Gas Inventories, Volume 1, Chapter 8.5, https://www.ipcc-nggip.iges.or.jp/public/2006gl/",
        <http://purl.obolibrary.org/obo/IAO_0000233> "issue: https://github.com/OpenEnergyPlatform/ontology/issues/1401
pull request: https://github.com/OpenEnergyPlatform/ontology/pull/1440

move to oeo-sector 
issue: https://github.com/OpenEnergyPlatform/ontology/issues/1399
pull request: https://github.com/OpenEnergyPlatform/ontology/pull/1724",
        rdfs:label "CRF sector (IPCC 2006): solvents"@en
    
    Types: 
        OEO_00000227
    
    Facts:  
     OEO_00000504  OEO_00000242,
     <http://purl.obolibrary.org/obo/BFO_0000050>  OEO_00010171
    
    
Individual: OEO_00010373

    Annotations: 
        OEO_00010037 "CRF 2.F.6",
        <http://purl.obolibrary.org/obo/IAO_0000115> "The CRF sector (IPCC 2006) 'other applications' is an industry sector defined by the 2006 IPCC Guidelines for National Greenhouse Gas Inventories:
The properties of ozone depleting substances have made them attractive for a variety of niche applications not covered in other sub-source categories. These include electronics testing, heat transfer, dielectric fluid and medical applications. The properties of HFCs and PFCs are equally attractive in some of these sectors and they have been adopted as substitutes. There are also some historical uses of PFCs, as well as emerging use of HFCs, in these applications. These applications have leakage rates ranging from 100% emissive in year of application to around 1% per annum.",
        <http://purl.obolibrary.org/obo/IAO_0000119> "2006 IPCC Guidelines for National Greenhouse Gas Inventories, Volume 1, Chapter 8.5, https://www.ipcc-nggip.iges.or.jp/public/2006gl/",
        <http://purl.obolibrary.org/obo/IAO_0000233> "issue: https://github.com/OpenEnergyPlatform/ontology/issues/1401
pull request: https://github.com/OpenEnergyPlatform/ontology/pull/1440

move to oeo-sector 
issue: https://github.com/OpenEnergyPlatform/ontology/issues/1399
pull request: https://github.com/OpenEnergyPlatform/ontology/pull/1724",
        rdfs:label "CRF sector (IPCC 2006): other applications"@en
    
    Types: 
        OEO_00000227
    
    Facts:  
     OEO_00000504  OEO_00000242,
     <http://purl.obolibrary.org/obo/BFO_0000050>  OEO_00010171
    
    
Individual: OEO_00010374

    Annotations: 
        OEO_00010037 "CRF 2.G.1",
        <http://purl.obolibrary.org/obo/IAO_0000115> "The CRF sector (IPCC 2006) 'electrical equipment' is an industry sector defined by the 2006 IPCC Guidelines for National Greenhouse Gas Inventories:
Electrical equipment is used in the transmission and distribution of electricity above 1 kV. SF6 is used in gasinsulated switchgear (GIS), gas circuit breakers (GCB), gas-insulated transformers (GIT), gas-insulated lines (GIL), outdoor gas-insulated instrument transformers, reclosers, switches, ring main units and other equipment.",
        <http://purl.obolibrary.org/obo/IAO_0000119> "2006 IPCC Guidelines for National Greenhouse Gas Inventories, Volume 1, Chapter 8.5, https://www.ipcc-nggip.iges.or.jp/public/2006gl/",
        <http://purl.obolibrary.org/obo/IAO_0000233> "issue: https://github.com/OpenEnergyPlatform/ontology/issues/1401
pull request: https://github.com/OpenEnergyPlatform/ontology/pull/1440

move to oeo-sector 
issue: https://github.com/OpenEnergyPlatform/ontology/issues/1399
pull request: https://github.com/OpenEnergyPlatform/ontology/pull/1724",
        rdfs:label "CRF sector (IPCC 2006): electrical equipment"@en
    
    Types: 
        OEO_00000227
    
    Facts:  
     OEO_00000504  OEO_00000242,
     <http://purl.obolibrary.org/obo/BFO_0000050>  OEO_00010172
    
    
Individual: OEO_00010375

    Annotations: 
        OEO_00010037 "CRF 2.G.2",
        <http://purl.obolibrary.org/obo/IAO_0000115> "The CRF sector (IPCC 2006) 'SF6 and PFCs from other product use' is an industry sector defined by the 2006 IPCC Guidelines for National Greenhouse Gas Inventories:
Identified remaining applications in this source category include:
- SF6 and PFCs used in military applications, particularly SF6 used in airborne radar systems, e.g., AWACS (Airborne Warning and Control System), and PFCs used as heat transfer fluids in high-powered electronic applications;
- SF6 used in equipment in university and research particle accelerators;
- SF6 used in equipment in industrial and medical particle accelerators;
- ‘Adiabatic’ applications utilising the low permeability through rubber of SF6 and some PFCs, e.g., car tires and sport shoe soles;
- SF6 used in sound-proof windows;
- PFCs used as heat transfer fluids in commercial and consumer applications;
- PFCs used in cosmetics and in medical applications;
- Other uses e.g. gas-air tracer in research and leak detectors.",
        <http://purl.obolibrary.org/obo/IAO_0000119> "2006 IPCC Guidelines for National Greenhouse Gas Inventories, Volume 3, Chapter 8.3, https://www.ipcc-nggip.iges.or.jp/public/2006gl/",
        <http://purl.obolibrary.org/obo/IAO_0000233> "issue: https://github.com/OpenEnergyPlatform/ontology/issues/1401
pull request: https://github.com/OpenEnergyPlatform/ontology/pull/1440

move to oeo-sector 
issue: https://github.com/OpenEnergyPlatform/ontology/issues/1399
pull request: https://github.com/OpenEnergyPlatform/ontology/pull/1724",
        rdfs:label "CRF sector (IPCC 2006): SF6 and PFCs from other product use"@en
    
    Types: 
        OEO_00000227
    
    Facts:  
     OEO_00000504  OEO_00000242,
     <http://purl.obolibrary.org/obo/BFO_0000050>  OEO_00010172
    
    
Individual: OEO_00010376

    Annotations: 
        OEO_00010037 "CRF 2.G.3",
        <http://purl.obolibrary.org/obo/IAO_0000115> "The CRF sector (IPCC 2006) 'N2O from product use' is an industry sector defined by the 2006 IPCC Guidelines for National Greenhouse Gas Inventories:
Evaporative emissions of nitrous oxide (N2O) can arise from various types of product use, including:
- Medical applications (anaesthetic use, analgesic use and veterinary use);
- Use as a propellant in aerosol products, primarily in food industry (pressure-packaged whipped cream, etc);
- Oxidising agent and etchant used in semiconductor manufacturing;
- Oxidising agent used, with acetylene, in atomic absorption spectrometry;
- Production of sodium azide, which is used to inflate airbags;
- Fuel oxidant in auto racing; and
- Oxidising agent in blowtorches used by jewelers and others.",
        <http://purl.obolibrary.org/obo/IAO_0000119> "2006 IPCC Guidelines for National Greenhouse Gas Inventories, Volume 3, Chapter 8.4.1, https://www.ipcc-nggip.iges.or.jp/public/2006gl/",
        <http://purl.obolibrary.org/obo/IAO_0000233> "issue: https://github.com/OpenEnergyPlatform/ontology/issues/1401
pull request: https://github.com/OpenEnergyPlatform/ontology/pull/1440

move to oeo-sector 
issue: https://github.com/OpenEnergyPlatform/ontology/issues/1399
pull request: https://github.com/OpenEnergyPlatform/ontology/pull/1724",
        rdfs:label "CRF sector (IPCC 2006): N2O from product use"@en
    
    Types: 
        OEO_00000227
    
    Facts:  
     OEO_00000504  OEO_00000242,
     <http://purl.obolibrary.org/obo/BFO_0000050>  OEO_00010172
    
    
Individual: OEO_00010377

    Annotations: 
        OEO_00010037 "CRF 2.G.4",
        <http://purl.obolibrary.org/obo/IAO_0000115> "The CRF sector (IPCC 2006) 'other product manufacture and use - other' is an industry sector defined by the 2006 IPCC Guidelines for National Greenhouse Gas Inventories",
        <http://purl.obolibrary.org/obo/IAO_0000119> "2006 IPCC Guidelines for National Greenhouse Gas Inventories, Volume 1, Chapter 8.5, https://www.ipcc-nggip.iges.or.jp/public/2006gl/",
        <http://purl.obolibrary.org/obo/IAO_0000233> "issue: https://github.com/OpenEnergyPlatform/ontology/issues/1401
pull request: https://github.com/OpenEnergyPlatform/ontology/pull/1440

move to oeo-sector 
issue: https://github.com/OpenEnergyPlatform/ontology/issues/1399
pull request: https://github.com/OpenEnergyPlatform/ontology/pull/1724",
        rdfs:label "CRF sector (IPCC 2006): other product manufacture and use - other"@en
    
    Types: 
        OEO_00000227
    
    Facts:  
     OEO_00000504  OEO_00000242,
     <http://purl.obolibrary.org/obo/BFO_0000050>  OEO_00010172
    
    
Individual: OEO_00010389

    Annotations: 
        <http://purl.obolibrary.org/obo/IAO_0000115> "The RED sector electricity is an electricity sector defined by the Renewable Energy Directive sector division.",
        <http://purl.obolibrary.org/obo/IAO_0000233> "issue: https://github.com/OpenEnergyPlatform/ontology/issues/1443
pull request: https://github.com/OpenEnergyPlatform/ontology/pull/1446

move to oeo-sector 
issue: https://github.com/OpenEnergyPlatform/ontology/issues/1399
pull request: https://github.com/OpenEnergyPlatform/ontology/pull/1724",
        rdfs:label "RED sector: electricity"@en
    
    Types: 
        OEO_00000145
    
    Facts:  
     OEO_00000504  OEO_00000355
    
    
Individual: OEO_00010390

    Annotations: 
        <http://purl.obolibrary.org/obo/IAO_0000115> "The RED sector heating and cooling is a heating and cooling sector defined by the Renewable Energy Directive sector division.",
        <http://purl.obolibrary.org/obo/IAO_0000233> "issue: https://github.com/OpenEnergyPlatform/ontology/issues/1443
pull request: https://github.com/OpenEnergyPlatform/ontology/pull/1446

move to oeo-sector 
issue: https://github.com/OpenEnergyPlatform/ontology/issues/1399
pull request: https://github.com/OpenEnergyPlatform/ontology/pull/1724",
        rdfs:label "RED sector: heating and cooling"@en
    
    Types: 
        OEO_00000213
    
    Facts:  
     OEO_00000504  OEO_00000355
    
    
Individual: OEO_00010391

    Annotations: 
        <http://purl.obolibrary.org/obo/IAO_0000115> "The RED sector heating and cooling is a heating and cooling sector defined by the Renewable Energy Directive sector division.",
        <http://purl.obolibrary.org/obo/IAO_0000233> "issue: https://github.com/OpenEnergyPlatform/ontology/issues/1443
pull request: https://github.com/OpenEnergyPlatform/ontology/pull/1446

move to oeo-sector 
issue: https://github.com/OpenEnergyPlatform/ontology/issues/1399
pull request: https://github.com/OpenEnergyPlatform/ontology/pull/1724",
        rdfs:label "RED sector: transport"@en
    
    Types: 
        OEO_00000422
    
    Facts:  
     OEO_00000504  OEO_00000355
    
    
DisjointClasses: 
    OEO_00000145,OEO_00000213,OEO_00000422

DifferentIndividuals: 
    OEO_00010131,OEO_00010134,OEO_00010135

DifferentIndividuals: 
    OEO_00010305,OEO_00010306,OEO_00010307,OEO_00010308,OEO_00010309,OEO_00010310,OEO_00010311

