<?xml version="1.0"?>
<rdf:RDF xmlns="http://openenergy-platform.org/ontology/oeo/imports/ro-module.owl#"
     xml:base="http://openenergy-platform.org/ontology/oeo/imports/ro-module.owl"
     xmlns:dc="http://purl.org/dc/elements/1.1/"
     xmlns:obo="http://purl.obolibrary.org/obo/"
     xmlns:owl="http://www.w3.org/2002/07/owl#"
     xmlns:rdf="http://www.w3.org/1999/02/22-rdf-syntax-ns#"
     xmlns:xml="http://www.w3.org/XML/1998/namespace"
     xmlns:xsd="http://www.w3.org/2001/XMLSchema#"
     xmlns:foaf="http://xmlns.com/foaf/0.1/"
     xmlns:rdfs="http://www.w3.org/2000/01/rdf-schema#"
     xmlns:terms="http://purl.org/dc/terms/"
     xmlns:oboInOwl="http://www.geneontology.org/formats/oboInOwl#">
    <owl:Ontology rdf:about="http://openenergy-platform.org/ontology/oeo/imports/ro-module.owl">
        <owl:versionIRI rdf:resource="http://openenergy-platform.org/ontology/oeo/dev/imports/ro-module.owl"/>
        <rdfs:comment rdf:datatype="http://www.w3.org/2001/XMLSchema#string">This file contains externally imported content from the Relations Ontology (RO) for import into the Open Energy Ontology (OEO). It is automatically extracted using ROBOT from the term list ro-terms.txt.</rdfs:comment>
    </owl:Ontology>
    


    <!-- 
    ///////////////////////////////////////////////////////////////////////////////////////
    //
    // Annotation properties
    //
    ///////////////////////////////////////////////////////////////////////////////////////
     -->

    


    <!-- http://purl.obolibrary.org/obo/IAO_0000111 -->

    <owl:AnnotationProperty rdf:about="http://purl.obolibrary.org/obo/IAO_0000111">
        <rdfs:label xml:lang="en">editor preferred term</rdfs:label>
    </owl:AnnotationProperty>
    


    <!-- http://purl.obolibrary.org/obo/IAO_0000112 -->

    <owl:AnnotationProperty rdf:about="http://purl.obolibrary.org/obo/IAO_0000112">
        <obo:IAO_0000114 rdf:resource="http://purl.obolibrary.org/obo/IAO_0000122"/>
        <rdfs:label xml:lang="en">example of usage</rdfs:label>
    </owl:AnnotationProperty>
    


    <!-- http://purl.obolibrary.org/obo/IAO_0000114 -->

    <owl:AnnotationProperty rdf:about="http://purl.obolibrary.org/obo/IAO_0000114">
        <rdfs:label xml:lang="en">has curation status</rdfs:label>
    </owl:AnnotationProperty>
    


    <!-- http://purl.obolibrary.org/obo/IAO_0000115 -->

    <owl:AnnotationProperty rdf:about="http://purl.obolibrary.org/obo/IAO_0000115">
        <obo:IAO_0000114 rdf:resource="http://purl.obolibrary.org/obo/IAO_0000122"/>
        <rdfs:label xml:lang="en">definition</rdfs:label>
        <rdfs:label rdf:datatype="http://www.w3.org/2001/XMLSchema#string">definition</rdfs:label>
    </owl:AnnotationProperty>
    


    <!-- http://purl.obolibrary.org/obo/IAO_0000116 -->

    <owl:AnnotationProperty rdf:about="http://purl.obolibrary.org/obo/IAO_0000116">
        <obo:IAO_0000114 rdf:resource="http://purl.obolibrary.org/obo/IAO_0000122"/>
        <rdfs:label xml:lang="en">editor note</rdfs:label>
    </owl:AnnotationProperty>
    


    <!-- http://purl.obolibrary.org/obo/IAO_0000117 -->

    <owl:AnnotationProperty rdf:about="http://purl.obolibrary.org/obo/IAO_0000117">
        <obo:IAO_0000114 rdf:resource="http://purl.obolibrary.org/obo/IAO_0000122"/>
        <rdfs:label xml:lang="en">term editor</rdfs:label>
    </owl:AnnotationProperty>
    


    <!-- http://purl.obolibrary.org/obo/IAO_0000118 -->

    <owl:AnnotationProperty rdf:about="http://purl.obolibrary.org/obo/IAO_0000118">
        <obo:IAO_0000114 rdf:resource="http://purl.obolibrary.org/obo/IAO_0000125"/>
        <rdfs:label xml:lang="en">alternative term</rdfs:label>
    </owl:AnnotationProperty>
    


    <!-- http://purl.obolibrary.org/obo/IAO_0000119 -->

    <owl:AnnotationProperty rdf:about="http://purl.obolibrary.org/obo/IAO_0000119">
        <obo:IAO_0000114 rdf:resource="http://purl.obolibrary.org/obo/IAO_0000122"/>
        <rdfs:label xml:lang="en">definition source</rdfs:label>
    </owl:AnnotationProperty>
    


    <!-- http://purl.obolibrary.org/obo/IAO_0000232 -->

    <owl:AnnotationProperty rdf:about="http://purl.obolibrary.org/obo/IAO_0000232">
        <obo:IAO_0000114 rdf:resource="http://purl.obolibrary.org/obo/IAO_0000122"/>
        <rdfs:label xml:lang="en">curator note</rdfs:label>
    </owl:AnnotationProperty>
    


    <!-- http://purl.obolibrary.org/obo/RO_0001900 -->

    <owl:AnnotationProperty rdf:about="http://purl.obolibrary.org/obo/RO_0001900">
        <obo:IAO_0000115>An assertion that holds between an OWL Object Property and a temporal interpretation that elucidates how OWL Class Axioms that use this property are to be interpreted in a temporal context.</obo:IAO_0000115>
        <rdfs:label xml:lang="en">temporal interpretation</rdfs:label>
        <foaf:page rdf:datatype="http://www.w3.org/2001/XMLSchema#anyURI">https://github.com/oborel/obo-relations/wiki/ROAndTime</foaf:page>
    </owl:AnnotationProperty>
    


    <!-- http://purl.obolibrary.org/obo/RO_0040042 -->

    <owl:AnnotationProperty rdf:about="http://purl.obolibrary.org/obo/RO_0040042">
        <obo:IAO_0000112>part-of is homeomorphic for independent continuants.</obo:IAO_0000112>
        <obo:IAO_0000115>R is homemorphic for C iff (1) there exists some x,y such that x R y, and x and y instantiate C and (2) for all x, if x is an instance of C, and there exists some y some such that x R y, then it follows that y is an instance of C.</obo:IAO_0000115>
        <oboInOwl:created_by rdf:datatype="http://www.w3.org/2001/XMLSchema#string">cjm</oboInOwl:created_by>
        <oboInOwl:creation_date rdf:datatype="http://www.w3.org/2001/XMLSchema#dateTime">2018-10-21T19:46:34Z</oboInOwl:creation_date>
        <rdfs:comment>R homeomorphic-for C expands to: C SubClassOf R only C. Additionally, for any class D that is disjoint with C, we can also expand to C DisjointWith R some D, D DisjointWith R some C.</rdfs:comment>
        <rdfs:label>is homeomorphic for</rdfs:label>
        <rdfs:seeAlso rdf:resource="https://github.com/oborel/obo-relations/issues/164"/>
    </owl:AnnotationProperty>
    


    <!-- http://purl.org/dc/elements/1.1/source -->

    <owl:AnnotationProperty rdf:about="http://purl.org/dc/elements/1.1/source"/>
    


    <!-- http://purl.org/dc/terms/source -->

    <owl:AnnotationProperty rdf:about="http://purl.org/dc/terms/source"/>
    


    <!-- http://www.geneontology.org/formats/oboInOwl#created_by -->

    <owl:AnnotationProperty rdf:about="http://www.geneontology.org/formats/oboInOwl#created_by"/>
    


    <!-- http://www.geneontology.org/formats/oboInOwl#creation_date -->

    <owl:AnnotationProperty rdf:about="http://www.geneontology.org/formats/oboInOwl#creation_date"/>
    


    <!-- http://www.geneontology.org/formats/oboInOwl#hasDbXref -->

    <owl:AnnotationProperty rdf:about="http://www.geneontology.org/formats/oboInOwl#hasDbXref"/>
    


    <!-- http://www.geneontology.org/formats/oboInOwl#hasRelatedSynonym -->

    <owl:AnnotationProperty rdf:about="http://www.geneontology.org/formats/oboInOwl#hasRelatedSynonym">
        <rdfs:label rdf:datatype="http://www.w3.org/2001/XMLSchema#string">has_related_synonym</rdfs:label>
    </owl:AnnotationProperty>
    


    <!-- http://www.geneontology.org/formats/oboInOwl#inSubset -->

    <owl:AnnotationProperty rdf:about="http://www.geneontology.org/formats/oboInOwl#inSubset">
        <rdfs:label rdf:datatype="http://www.w3.org/2001/XMLSchema#string">in_subset</rdfs:label>
    </owl:AnnotationProperty>
    


    <!-- http://www.w3.org/2000/01/rdf-schema#comment -->

    <owl:AnnotationProperty rdf:about="http://www.w3.org/2000/01/rdf-schema#comment"/>
    


    <!-- http://www.w3.org/2000/01/rdf-schema#label -->

    <owl:AnnotationProperty rdf:about="http://www.w3.org/2000/01/rdf-schema#label"/>
    


    <!-- http://www.w3.org/2000/01/rdf-schema#seeAlso -->

    <owl:AnnotationProperty rdf:about="http://www.w3.org/2000/01/rdf-schema#seeAlso"/>
    


    <!-- http://xmlns.com/foaf/0.1/page -->

    <owl:AnnotationProperty rdf:about="http://xmlns.com/foaf/0.1/page"/>
    


    <!-- 
    ///////////////////////////////////////////////////////////////////////////////////////
    //
    // Object Properties
    //
    ///////////////////////////////////////////////////////////////////////////////////////
     -->

    


    <!-- http://purl.obolibrary.org/obo/BFO_0000050 -->

    <owl:ObjectProperty rdf:about="http://purl.obolibrary.org/obo/BFO_0000050">
        <rdfs:subPropertyOf rdf:resource="http://www.w3.org/2002/07/owl#topObjectProperty"/>
        <owl:inverseOf rdf:resource="http://purl.obolibrary.org/obo/BFO_0000051"/>
        <obo:IAO_0000111 xml:lang="en">is part of</obo:IAO_0000111>
        <obo:IAO_0000112 xml:lang="en">my brain is part of my body (continuant parthood, two material entities)</obo:IAO_0000112>
        <obo:IAO_0000112 xml:lang="en">my stomach cavity is part of my stomach (continuant parthood, immaterial entity is part of material entity)</obo:IAO_0000112>
        <obo:IAO_0000112 xml:lang="en">this day is part of this year (occurrent parthood)</obo:IAO_0000112>
        <obo:IAO_0000115 xml:lang="en">a core relation that holds between a part and its whole</obo:IAO_0000115>
        <obo:IAO_0000116 xml:lang="en">Everything is part of itself. Any part of any part of a thing is itself part of that thing. Two distinct things cannot be part of each other.</obo:IAO_0000116>
        <obo:IAO_0000116 xml:lang="en">Occurrents are not subject to change and so parthood between occurrents holds for all the times that the part exists. Many continuants are subject to change, so parthood between continuants will only hold at certain times, but this is difficult to specify in OWL. See https://code.google.com/p/obo-relations/wiki/ROAndTime</obo:IAO_0000116>
        <obo:IAO_0000116 xml:lang="en">Parthood requires the part and the whole to have compatible classes: only an occurrent can be part of an occurrent; only a process can be part of a process; only a continuant can be part of a continuant; only an independent continuant can be part of an independent continuant; only an immaterial entity can be part of an immaterial entity; only a specifically dependent continuant can be part of a specifically dependent continuant; only a generically dependent continuant can be part of a generically dependent continuant. (This list is not exhaustive.)

A continuant cannot be part of an occurrent: use &apos;participates in&apos;. An occurrent cannot be part of a continuant: use &apos;has participant&apos;. A material entity cannot be part of an immaterial entity: use &apos;has location&apos;. A specifically dependent continuant cannot be part of an independent continuant: use &apos;inheres in&apos;. An independent continuant cannot be part of a specifically dependent continuant: use &apos;bearer of&apos;.</obo:IAO_0000116>
        <obo:IAO_0000118 xml:lang="en">part_of</obo:IAO_0000118>
        <obo:RO_0001900 rdf:resource="http://purl.obolibrary.org/obo/RO_0001901"/>
        <obo:RO_0040042 rdf:resource="http://purl.obolibrary.org/obo/BFO_0000002"/>
        <obo:RO_0040042 rdf:resource="http://purl.obolibrary.org/obo/BFO_0000003"/>
        <obo:RO_0040042 rdf:resource="http://purl.obolibrary.org/obo/BFO_0000004"/>
        <obo:RO_0040042 rdf:resource="http://purl.obolibrary.org/obo/BFO_0000017"/>
        <obo:RO_0040042 rdf:resource="http://purl.obolibrary.org/obo/BFO_0000019"/>
        <obo:RO_0040042 rdf:resource="http://purl.obolibrary.org/obo/BFO_0000020"/>
        <obo:RO_0040042 rdf:resource="http://purl.obolibrary.org/obo/BFO_0000031"/>
        <rdfs:label xml:lang="en">part of</rdfs:label>
        <rdfs:seeAlso rdf:resource="http://ontologydesignpatterns.org/wiki/Community:Parts_and_Collections"/>
        <rdfs:seeAlso rdf:resource="http://ontologydesignpatterns.org/wiki/Submissions:PartOf"/>
        <rdfs:seeAlso>http://www.obofoundry.org/ro/#OBO_REL:part_of</rdfs:seeAlso>
    </owl:ObjectProperty>
    


    <!-- http://purl.obolibrary.org/obo/BFO_0000051 -->

    <owl:ObjectProperty rdf:about="http://purl.obolibrary.org/obo/BFO_0000051">
        <rdfs:subPropertyOf rdf:resource="http://www.w3.org/2002/07/owl#topObjectProperty"/>
        <obo:IAO_0000111 xml:lang="en">has part</obo:IAO_0000111>
        <obo:IAO_0000112 xml:lang="en">my body has part my brain (continuant parthood, two material entities)</obo:IAO_0000112>
        <obo:IAO_0000112 xml:lang="en">my stomach has part my stomach cavity (continuant parthood, material entity has part immaterial entity)</obo:IAO_0000112>
        <obo:IAO_0000112 xml:lang="en">this year has part this day (occurrent parthood)</obo:IAO_0000112>
        <obo:IAO_0000115 xml:lang="en">a core relation that holds between a whole and its part</obo:IAO_0000115>
        <obo:IAO_0000116 xml:lang="en">Everything has itself as a part. Any part of any part of a thing is itself part of that thing. Two distinct things cannot have each other as a part.</obo:IAO_0000116>
        <obo:IAO_0000116 xml:lang="en">Occurrents are not subject to change and so parthood between occurrents holds for all the times that the part exists. Many continuants are subject to change, so parthood between continuants will only hold at certain times, but this is difficult to specify in OWL. See https://code.google.com/p/obo-relations/wiki/ROAndTime</obo:IAO_0000116>
        <obo:IAO_0000116 xml:lang="en">Parthood requires the part and the whole to have compatible classes: only an occurrent have an occurrent as part; only a process can have a process as part; only a continuant can have a continuant as part; only an independent continuant can have an independent continuant as part; only a specifically dependent continuant can have a specifically dependent continuant as part; only a generically dependent continuant can have a generically dependent continuant as part. (This list is not exhaustive.)

A continuant cannot have an occurrent as part: use &apos;participates in&apos;. An occurrent cannot have a continuant as part: use &apos;has participant&apos;. An immaterial entity cannot have a material entity as part: use &apos;location of&apos;. An independent continuant cannot have a specifically dependent continuant as part: use &apos;bearer of&apos;. A specifically dependent continuant cannot have an independent continuant as part: use &apos;inheres in&apos;.</obo:IAO_0000116>
        <obo:IAO_0000118 xml:lang="en">has_part</obo:IAO_0000118>
        <obo:RO_0001900 rdf:resource="http://purl.obolibrary.org/obo/RO_0001901"/>
        <rdfs:label xml:lang="en">has part</rdfs:label>
    </owl:ObjectProperty>
    


    <!-- http://purl.obolibrary.org/obo/BFO_0000062 -->

    <owl:ObjectProperty rdf:about="http://purl.obolibrary.org/obo/BFO_0000062">
        <rdfs:subPropertyOf rdf:resource="http://purl.obolibrary.org/obo/RO_0002086"/>
        <obo:IAO_0000111 xml:lang="en">preceded by</obo:IAO_0000111>
        <obo:IAO_0000115 xml:lang="en">x is preceded by y if and only if the time point at which y ends is before or equivalent to the time point at which x starts. Formally: x preceded by y iff ω(y) &lt;= α(x), where α is a function that maps a process to a start point, and ω is a function that maps a process to an end point.</obo:IAO_0000115>
        <obo:IAO_0000116 xml:lang="en">An example is: translation preceded_by transcription; aging preceded_by development (not however death preceded_by aging). Where derives_from links classes of continuants, preceded_by links classes of processes. Clearly, however, these two relations are not independent of each other. Thus if cells of type C1 derive_from cells of type C, then any cell division involving an instance of C1 in a given lineage is preceded_by cellular processes involving an instance of C.    The assertion P preceded_by P1 tells us something about Ps in general: that is, it tells us something about what happened earlier, given what we know about what happened later. Thus it does not provide information pointing in the opposite direction, concerning instances of P1 in general; that is, that each is such as to be succeeded by some instance of P. Note that an assertion to the effect that P preceded_by P1 is rather weak; it tells us little about the relations between the underlying instances in virtue of which the preceded_by relation obtains. Typically we will be interested in stronger relations, for example in the relation immediately_preceded_by, or in relations which combine preceded_by with a condition to the effect that the corresponding instances of P and P1 share participants, or that their participants are connected by relations of derivation, or (as a first step along the road to a treatment of causality) that the one process in some way affects (for example, initiates or regulates) the other.</obo:IAO_0000116>
        <obo:IAO_0000118 xml:lang="en">is preceded by</obo:IAO_0000118>
        <obo:IAO_0000118 xml:lang="en">preceded_by</obo:IAO_0000118>
        <dc:source>http://www.obofoundry.org/ro/#OBO_REL:preceded_by</dc:source>
        <oboInOwl:inSubset rdf:resource="http://purl.obolibrary.org/obo/ro/subsets#ro-eco"/>
        <rdfs:label xml:lang="en">preceded by</rdfs:label>
    </owl:ObjectProperty>
    


    <!-- http://purl.obolibrary.org/obo/BFO_0000063 -->

    <owl:ObjectProperty rdf:about="http://purl.obolibrary.org/obo/BFO_0000063">
        <rdfs:subPropertyOf rdf:resource="http://purl.obolibrary.org/obo/RO_0002222"/>
        <obo:IAO_0000111 xml:lang="en">precedes</obo:IAO_0000111>
        <obo:IAO_0000115 xml:lang="en">x precedes y if and only if the time point at which x ends is before or equivalent to the time point at which y starts. Formally: x precedes y iff ω(x) &lt;= α(y), where α is a function that maps a process to a start point, and ω is a function that maps a process to an end point.</obo:IAO_0000115>
        <oboInOwl:inSubset rdf:resource="http://purl.obolibrary.org/obo/ro/subsets#ro-eco"/>
        <rdfs:label xml:lang="en">precedes</rdfs:label>
    </owl:ObjectProperty>
    


    <!-- http://purl.obolibrary.org/obo/RO_0000053 -->

    <owl:ObjectProperty rdf:about="http://purl.obolibrary.org/obo/RO_0000053">
        <obo:IAO_0000111 xml:lang="en">bearer of</obo:IAO_0000111>
        <obo:IAO_0000112 xml:lang="en">this apple is bearer of this red color</obo:IAO_0000112>
        <obo:IAO_0000112 xml:lang="en">this vase is bearer of this fragility</obo:IAO_0000112>
        <obo:IAO_0000115 xml:lang="en">a relation between an independent continuant (the bearer) and a specifically dependent continuant (the dependent), in which the dependent specifically depends on the bearer for its existence</obo:IAO_0000115>
        <obo:IAO_0000116 xml:lang="en">A bearer can have many dependents, and its dependents can exist for different periods of time, but none of its dependents can exist when the bearer does not exist.</obo:IAO_0000116>
        <obo:IAO_0000118 xml:lang="en">bearer_of</obo:IAO_0000118>
        <obo:IAO_0000118 xml:lang="en">is bearer of</obo:IAO_0000118>
        <obo:RO_0001900 rdf:resource="http://purl.obolibrary.org/obo/RO_0001901"/>
        <rdfs:label xml:lang="en">bearer of</rdfs:label>
    </owl:ObjectProperty>
    


    <!-- http://purl.obolibrary.org/obo/RO_0000056 -->

    <owl:ObjectProperty rdf:about="http://purl.obolibrary.org/obo/RO_0000056">
        <rdfs:subPropertyOf rdf:resource="http://www.w3.org/2002/07/owl#topObjectProperty"/>
        <obo:IAO_0000111 xml:lang="en">participates in</obo:IAO_0000111>
        <obo:IAO_0000112 xml:lang="en">this blood clot participates in this blood coagulation</obo:IAO_0000112>
        <obo:IAO_0000112 xml:lang="en">this input material (or this output material) participates in this process</obo:IAO_0000112>
        <obo:IAO_0000112 xml:lang="en">this investigator participates in this investigation</obo:IAO_0000112>
        <obo:IAO_0000115 xml:lang="en">a relation between a continuant and a process, in which the continuant is somehow involved in the process</obo:IAO_0000115>
        <obo:IAO_0000118 xml:lang="en">participates_in</obo:IAO_0000118>
        <rdfs:label xml:lang="en">participates in</rdfs:label>
    </owl:ObjectProperty>
    


    <!-- http://purl.obolibrary.org/obo/RO_0000057 -->

    <owl:ObjectProperty rdf:about="http://purl.obolibrary.org/obo/RO_0000057">
        <rdfs:subPropertyOf rdf:resource="http://www.w3.org/2002/07/owl#topObjectProperty"/>
        <obo:IAO_0000111 xml:lang="en">has participant</obo:IAO_0000111>
        <obo:IAO_0000112 xml:lang="en">this blood coagulation has participant this blood clot</obo:IAO_0000112>
        <obo:IAO_0000112 xml:lang="en">this investigation has participant this investigator</obo:IAO_0000112>
        <obo:IAO_0000112 xml:lang="en">this process has participant this input material (or this output material)</obo:IAO_0000112>
        <obo:IAO_0000115 xml:lang="en">a relation between a process and a continuant, in which the continuant is somehow involved in the process</obo:IAO_0000115>
        <obo:IAO_0000116 xml:lang="en">Has_participant is a primitive instance-level relation between a process, a continuant, and a time at which the continuant participates in some way in the process. The relation obtains, for example, when this particular process of oxygen exchange across this particular alveolar membrane has_participant this particular sample of hemoglobin at this particular time.</obo:IAO_0000116>
        <obo:IAO_0000118 xml:lang="en">has_participant</obo:IAO_0000118>
        <dc:source>http://www.obofoundry.org/ro/#OBO_REL:has_participant</dc:source>
        <rdfs:label xml:lang="en">has participant</rdfs:label>
    </owl:ObjectProperty>
    


    <!-- http://purl.obolibrary.org/obo/RO_0000085 -->

    <owl:ObjectProperty rdf:about="http://purl.obolibrary.org/obo/RO_0000085">
        <rdfs:subPropertyOf rdf:resource="http://purl.obolibrary.org/obo/RO_0000053"/>
        <obo:IAO_0000112 xml:lang="en">this enzyme has function this catalysis function (more colloquially: this enzyme has this catalysis function)</obo:IAO_0000112>
        <obo:IAO_0000115 xml:lang="en">a relation between an independent continuant (the bearer) and a function, in which the function specifically depends on the bearer for its existence</obo:IAO_0000115>
        <obo:IAO_0000116 xml:lang="en">A bearer can have many functions, and its functions can exist for different periods of time, but none of its functions can exist when the bearer does not exist. A function need not be realized at all the times that the function exists.</obo:IAO_0000116>
        <obo:IAO_0000118 xml:lang="en">has_function</obo:IAO_0000118>
        <rdfs:label xml:lang="en">has function</rdfs:label>
    </owl:ObjectProperty>
    


    <!-- http://purl.obolibrary.org/obo/RO_0000086 -->

    <owl:ObjectProperty rdf:about="http://purl.obolibrary.org/obo/RO_0000086">
        <rdfs:subPropertyOf rdf:resource="http://purl.obolibrary.org/obo/RO_0000053"/>
        <rdfs:range rdf:resource="http://purl.obolibrary.org/obo/BFO_0000019"/>
        <obo:IAO_0000112 xml:lang="en">this apple has quality this red color</obo:IAO_0000112>
        <obo:IAO_0000115 xml:lang="en">a relation between an independent continuant (the bearer) and a quality, in which the quality specifically depends on the bearer for its existence</obo:IAO_0000115>
        <obo:IAO_0000116 xml:lang="en">A bearer can have many qualities, and its qualities can exist for different periods of time, but none of its qualities can exist when the bearer does not exist.</obo:IAO_0000116>
        <obo:IAO_0000118 xml:lang="en">has_quality</obo:IAO_0000118>
        <rdfs:label xml:lang="en">has quality</rdfs:label>
    </owl:ObjectProperty>
    


    <!-- http://purl.obolibrary.org/obo/RO_0000087 -->

    <owl:ObjectProperty rdf:about="http://purl.obolibrary.org/obo/RO_0000087">
        <rdfs:subPropertyOf rdf:resource="http://purl.obolibrary.org/obo/RO_0000053"/>
        <obo:IAO_0000112 xml:lang="en">this person has role this investigator role (more colloquially: this person has this role of investigator)</obo:IAO_0000112>
        <obo:IAO_0000115 xml:lang="en">a relation between an independent continuant or energy (the bearer) and a role, in which the role specifically depends on the bearer for its existence</obo:IAO_0000115>
        <obo:IAO_0000116 xml:lang="en">A bearer can have many roles, and its roles can exist for different periods of time, but none of its roles can exist when the bearer does not exist. A role need not be realized at all the times that the role exists.</obo:IAO_0000116>
        <obo:IAO_0000118 xml:lang="en">has_role</obo:IAO_0000118>
        <rdfs:label xml:lang="en">has role</rdfs:label>
    </owl:ObjectProperty>
    


    <!-- http://purl.obolibrary.org/obo/RO_0000091 -->

    <owl:ObjectProperty rdf:about="http://purl.obolibrary.org/obo/RO_0000091">
        <rdfs:subPropertyOf rdf:resource="http://purl.obolibrary.org/obo/RO_0000053"/>
        <obo:IAO_0000115 xml:lang="en">a relation between an independent continuant (the bearer) and a disposition, in which the disposition specifically depends on the bearer for its existence</obo:IAO_0000115>
        <rdfs:label xml:lang="en">has disposition</rdfs:label>
    </owl:ObjectProperty>
    


    <!-- http://purl.obolibrary.org/obo/RO_0001015 -->

    <owl:ObjectProperty rdf:about="http://purl.obolibrary.org/obo/RO_0001015">
        <rdfs:subPropertyOf rdf:resource="http://www.w3.org/2002/07/owl#topObjectProperty"/>
        <owl:inverseOf rdf:resource="http://purl.obolibrary.org/obo/RO_0001025"/>
        <obo:IAO_0000111 xml:lang="en">is location of</obo:IAO_0000111>
        <obo:IAO_0000112 xml:lang="en">my head is the location of my brain</obo:IAO_0000112>
        <obo:IAO_0000112 xml:lang="en">this cage is the location of this rat</obo:IAO_0000112>
        <obo:IAO_0000115 xml:lang="en">a relation between two independent continuants, the location and the target, in which the target is entirely within the location</obo:IAO_0000115>
        <obo:IAO_0000116 xml:lang="en">Most location relations will only hold at certain times, but this is difficult to specify in OWL. See https://code.google.com/p/obo-relations/wiki/ROAndTime</obo:IAO_0000116>
        <obo:IAO_0000118 xml:lang="en">location_of</obo:IAO_0000118>
        <obo:RO_0001900 rdf:resource="http://purl.obolibrary.org/obo/RO_0001901"/>
        <rdfs:label xml:lang="en">location of</rdfs:label>
    </owl:ObjectProperty>
    


    <!-- http://purl.obolibrary.org/obo/RO_0001025 -->

    <owl:ObjectProperty rdf:about="http://purl.obolibrary.org/obo/RO_0001025">
        <rdfs:subPropertyOf rdf:resource="http://www.w3.org/2002/07/owl#topObjectProperty"/>
        <obo:IAO_0000111 xml:lang="en">located in</obo:IAO_0000111>
        <obo:IAO_0000112 xml:lang="en">my brain is located in my head</obo:IAO_0000112>
        <obo:IAO_0000112 xml:lang="en">this rat is located in this cage</obo:IAO_0000112>
        <obo:IAO_0000115 xml:lang="en">a relation between two independent continuants, the target and the location, in which the target is entirely within the location</obo:IAO_0000115>
        <obo:IAO_0000116 xml:lang="en">Location as a relation between instances: The primitive instance-level relation c located_in r at t reflects the fact that each continuant is at any given time associated with exactly one spatial region, namely its exact location. Following we can use this relation to define a further instance-level location relation - not between a continuant and the region which it exactly occupies, but rather between one continuant and another. c is located in c1, in this sense, whenever the spatial region occupied by c is part_of the spatial region occupied by c1.    Note that this relation comprehends both the relation of exact location between one continuant and another which obtains when r and r1 are identical (for example, when a portion of fluid exactly fills a cavity), as well as those sorts of inexact location relations which obtain, for example, between brain and head or between ovum and uterus</obo:IAO_0000116>
        <obo:IAO_0000116 xml:lang="en">Most location relations will only hold at certain times, but this is difficult to specify in OWL. See https://code.google.com/p/obo-relations/wiki/ROAndTime</obo:IAO_0000116>
        <obo:IAO_0000118 xml:lang="en">located_in</obo:IAO_0000118>
        <obo:RO_0001900 rdf:resource="http://purl.obolibrary.org/obo/RO_0001901"/>
        <dc:source>http://www.obofoundry.org/ro/#OBO_REL:located_in</dc:source>
        <rdfs:label xml:lang="en">located in</rdfs:label>
    </owl:ObjectProperty>
    


    <!-- http://purl.obolibrary.org/obo/RO_0002081 -->

    <owl:ObjectProperty rdf:about="http://purl.obolibrary.org/obo/RO_0002081">
        <rdfs:subPropertyOf rdf:resource="http://purl.obolibrary.org/obo/RO_0002222"/>
        <obo:IAO_0000117>David Osumi-Sutherland</obo:IAO_0000117>
        <obo:IAO_0000118 xml:lang="en">&lt;=</obo:IAO_0000118>
        <oboInOwl:inSubset rdf:resource="http://purl.obolibrary.org/obo/ro/subsets#ro-eco"/>
        <rdfs:comment>Primitive instance level timing relation between events</rdfs:comment>
        <rdfs:label xml:lang="en">before or simultaneous with</rdfs:label>
    </owl:ObjectProperty>
    


    <!-- http://purl.obolibrary.org/obo/RO_0002082 -->

    <owl:ObjectProperty rdf:about="http://purl.obolibrary.org/obo/RO_0002082">
        <rdfs:subPropertyOf rdf:resource="http://purl.obolibrary.org/obo/RO_0002081"/>
        <obo:IAO_0000117>David Osumi-Sutherland</obo:IAO_0000117>
        <oboInOwl:inSubset rdf:resource="http://purl.obolibrary.org/obo/ro/subsets#ro-eco"/>
        <rdfs:comment xml:lang="en">t1 simultaneous_with t2 iff:=  t1 before_or_simultaneous_with t2  and not (t1 before t2)</rdfs:comment>
        <rdfs:label xml:lang="en">simultaneous with</rdfs:label>
    </owl:ObjectProperty>
    


    <!-- http://purl.obolibrary.org/obo/RO_0002083 -->

    <owl:ObjectProperty rdf:about="http://purl.obolibrary.org/obo/RO_0002083">
        <rdfs:subPropertyOf rdf:resource="http://purl.obolibrary.org/obo/RO_0002081"/>
        <obo:IAO_0000117>David Osumi-Sutherland</obo:IAO_0000117>
        <oboInOwl:inSubset rdf:resource="http://purl.obolibrary.org/obo/ro/subsets#ro-eco"/>
        <rdfs:comment xml:lang="en">t1 before t2 iff:=  t1 before_or_simulataneous_with t2  and not (t1 simultaeous_with t2)</rdfs:comment>
        <rdfs:label xml:lang="en">before</rdfs:label>
    </owl:ObjectProperty>
    


    <!-- http://purl.obolibrary.org/obo/RO_0002086 -->

    <owl:ObjectProperty rdf:about="http://purl.obolibrary.org/obo/RO_0002086">
        <rdfs:subPropertyOf rdf:resource="http://purl.obolibrary.org/obo/RO_0002222"/>
        <obo:IAO_0000117>David Osumi-Sutherland</obo:IAO_0000117>
        <oboInOwl:inSubset rdf:resource="http://purl.obolibrary.org/obo/ro/subsets#ro-eco"/>
        <rdfs:comment xml:lang="en">X ends_after Y iff: end(Y) before_or_simultaneous_with end(X)</rdfs:comment>
        <rdfs:label xml:lang="en">ends after</rdfs:label>
    </owl:ObjectProperty>
    


    <!-- http://purl.obolibrary.org/obo/RO_0002089 -->

    <owl:ObjectProperty rdf:about="http://purl.obolibrary.org/obo/RO_0002089">
        <rdfs:subPropertyOf rdf:resource="http://purl.obolibrary.org/obo/RO_0002222"/>
        <obo:IAO_0000117>David Osumi-Sutherland</obo:IAO_0000117>
        <oboInOwl:inSubset rdf:resource="http://purl.obolibrary.org/obo/ro/subsets#ro-eco"/>
        <rdfs:label xml:lang="en">starts before</rdfs:label>
    </owl:ObjectProperty>
    


    <!-- http://purl.obolibrary.org/obo/RO_0002091 -->

    <owl:ObjectProperty rdf:about="http://purl.obolibrary.org/obo/RO_0002091">
        <rdfs:subPropertyOf rdf:resource="http://purl.obolibrary.org/obo/RO_0002222"/>
        <obo:IAO_0000117>David Osumi-Sutherland</obo:IAO_0000117>
        <obo:IAO_0000118>io</obo:IAO_0000118>
        <oboInOwl:inSubset rdf:resource="http://purl.obolibrary.org/obo/ro/subsets#ro-eco"/>
        <rdfs:comment xml:lang="en">X starts_during Y iff: (start(Y) before_or_simultaneous_with start(X)) AND (start(X) before_or_simultaneous_with end(Y))</rdfs:comment>
        <rdfs:label xml:lang="en">starts during</rdfs:label>
    </owl:ObjectProperty>
    


    <!-- http://purl.obolibrary.org/obo/RO_0002092 -->

    <owl:ObjectProperty rdf:about="http://purl.obolibrary.org/obo/RO_0002092">
        <rdfs:subPropertyOf rdf:resource="http://purl.obolibrary.org/obo/RO_0002091"/>
        <rdfs:subPropertyOf rdf:resource="http://purl.obolibrary.org/obo/RO_0002093"/>
        <obo:IAO_0000117>David Osumi-Sutherland</obo:IAO_0000117>
        <obo:IAO_0000118>d</obo:IAO_0000118>
        <obo:IAO_0000118>during</obo:IAO_0000118>
        <oboInOwl:inSubset rdf:resource="http://purl.obolibrary.org/obo/ro/subsets#ro-eco"/>
        <rdfs:comment xml:lang="en">X happens_during Y iff: (start(Y) before_or_simultaneous_with start(X)) AND (end(X) before_or_simultaneous_with end(Y))</rdfs:comment>
        <rdfs:label xml:lang="en">happens during</rdfs:label>
    </owl:ObjectProperty>
    


    <!-- http://purl.obolibrary.org/obo/RO_0002093 -->

    <owl:ObjectProperty rdf:about="http://purl.obolibrary.org/obo/RO_0002093">
        <rdfs:subPropertyOf rdf:resource="http://purl.obolibrary.org/obo/RO_0002222"/>
        <obo:IAO_0000117>David Osumi-Sutherland</obo:IAO_0000117>
        <obo:IAO_0000118>o</obo:IAO_0000118>
        <obo:IAO_0000118>overlaps</obo:IAO_0000118>
        <oboInOwl:inSubset rdf:resource="http://purl.obolibrary.org/obo/ro/subsets#ro-eco"/>
        <rdfs:comment xml:lang="en">X ends_during Y iff: ((start(Y) before_or_simultaneous_with end(X)) AND end(X) before_or_simultaneous_with end(Y). </rdfs:comment>
        <rdfs:label xml:lang="en">ends during</rdfs:label>
    </owl:ObjectProperty>
    


    <!-- http://purl.obolibrary.org/obo/RO_0002222 -->

    <owl:ObjectProperty rdf:about="http://purl.obolibrary.org/obo/RO_0002222">
        <rdfs:subPropertyOf rdf:resource="http://www.w3.org/2002/07/owl#topObjectProperty"/>
        <obo:IAO_0000114 rdf:resource="http://purl.obolibrary.org/obo/IAO_0000125"/>
        <obo:IAO_0000117>Chris Mungall</obo:IAO_0000117>
        <obo:IAO_0000119 rdf:resource="https://en.wikipedia.org/wiki/Allen%27s_interval_algebra"/>
        <obo:IAO_0000232>Do not use this relation directly. It is ended as a grouping for relations between occurrents involving the relative timing of their starts and ends.</obo:IAO_0000232>
        <terms:source rdf:datatype="http://www.w3.org/2001/XMLSchema#anyURI">https://docs.google.com/document/d/1kBv1ep_9g3sTR-SD3jqzFqhuwo9TPNF-l-9fUDbO6rM/edit?pli=1</terms:source>
        <oboInOwl:inSubset rdf:resource="http://purl.obolibrary.org/obo/ro/subsets#ro-eco"/>
        <rdfs:comment>A relation that holds between two occurrents. This is a grouping relation that collects together all the Allen relations.</rdfs:comment>
        <rdfs:label xml:lang="en">temporally related to</rdfs:label>
    </owl:ObjectProperty>
    


    <!-- http://purl.obolibrary.org/obo/RO_0002223 -->

    <owl:ObjectProperty rdf:about="http://purl.obolibrary.org/obo/RO_0002223">
        <rdfs:subPropertyOf rdf:resource="http://www.w3.org/2002/07/owl#topObjectProperty"/>
        <owl:inverseOf rdf:resource="http://purl.obolibrary.org/obo/RO_0002224"/>
        <obo:IAO_0000114 rdf:resource="http://purl.obolibrary.org/obo/IAO_0000125"/>
        <obo:IAO_0000115>inverse of starts with</obo:IAO_0000115>
        <obo:IAO_0000117>Chris Mungall</obo:IAO_0000117>
        <obo:IAO_0000119>Allen</obo:IAO_0000119>
        <oboInOwl:inSubset rdf:resource="http://purl.obolibrary.org/obo/ro/subsets#ro-eco"/>
        <rdfs:label xml:lang="en">starts</rdfs:label>
    </owl:ObjectProperty>
    


    <!-- http://purl.obolibrary.org/obo/RO_0002224 -->

    <owl:ObjectProperty rdf:about="http://purl.obolibrary.org/obo/RO_0002224">
        <rdfs:subPropertyOf rdf:resource="http://www.w3.org/2002/07/owl#topObjectProperty"/>
        <obo:IAO_0000112>Every insulin receptor signaling pathway starts with the binding of a ligand to the insulin receptor</obo:IAO_0000112>
        <obo:IAO_0000114 rdf:resource="http://purl.obolibrary.org/obo/IAO_0000125"/>
        <obo:IAO_0000115>x starts with y if and only if x has part y and the time point at which x starts is equivalent to the time point at which y starts. Formally: α(y) = α(x) ∧ ω(y) &lt; ω(x), where α is a function that maps a process to a start point, and ω is a function that maps a process to an end point.</obo:IAO_0000115>
        <obo:IAO_0000117>Chris Mungall</obo:IAO_0000117>
        <obo:IAO_0000118>started by</obo:IAO_0000118>
        <oboInOwl:inSubset rdf:resource="http://purl.obolibrary.org/obo/ro/subsets#ro-eco"/>
        <rdfs:label xml:lang="en">starts with</rdfs:label>
    </owl:ObjectProperty>
    


    <!-- http://purl.obolibrary.org/obo/RO_0002229 -->

    <owl:ObjectProperty rdf:about="http://purl.obolibrary.org/obo/RO_0002229">
        <rdfs:subPropertyOf rdf:resource="http://www.w3.org/2002/07/owl#topObjectProperty"/>
        <owl:inverseOf rdf:resource="http://purl.obolibrary.org/obo/RO_0002230"/>
        <obo:IAO_0000114 rdf:resource="http://purl.obolibrary.org/obo/IAO_0000125"/>
        <obo:IAO_0000115>inverse of ends with</obo:IAO_0000115>
        <obo:IAO_0000117>Chris Mungall</obo:IAO_0000117>
        <oboInOwl:inSubset rdf:resource="http://purl.obolibrary.org/obo/ro/subsets#ro-eco"/>
        <rdfs:label xml:lang="en">ends</rdfs:label>
    </owl:ObjectProperty>
    


    <!-- http://purl.obolibrary.org/obo/RO_0002230 -->

    <owl:ObjectProperty rdf:about="http://purl.obolibrary.org/obo/RO_0002230">
        <rdfs:subPropertyOf rdf:resource="http://www.w3.org/2002/07/owl#topObjectProperty"/>
        <obo:IAO_0000114 rdf:resource="http://purl.obolibrary.org/obo/IAO_0000125"/>
        <obo:IAO_0000115>x ends with y if and only if x has part y and the time point at which x ends is equivalent to the time point at which y ends. Formally: α(y) &gt; α(x) ∧ ω(y) = ω(x), where α is a function that maps a process to a start point, and ω is a function that maps a process to an end point.</obo:IAO_0000115>
        <obo:IAO_0000117>Chris Mungall</obo:IAO_0000117>
        <obo:IAO_0000118>finished by</obo:IAO_0000118>
        <oboInOwl:inSubset rdf:resource="http://purl.obolibrary.org/obo/ro/subsets#ro-eco"/>
        <rdfs:label xml:lang="en">ends with</rdfs:label>
    </owl:ObjectProperty>
    


    <!-- http://purl.obolibrary.org/obo/RO_0002233 -->

    <owl:ObjectProperty rdf:about="http://purl.obolibrary.org/obo/RO_0002233">
        <rdfs:subPropertyOf rdf:resource="http://purl.obolibrary.org/obo/RO_0000057"/>
        <obo:IAO_0000114 rdf:resource="http://purl.obolibrary.org/obo/IAO_0000125"/>
        <obo:IAO_0000115>p has input c iff: p is a process, c is a continuant, c is a participant in p, c is present at the start of p, and the state of c is modified during p.</obo:IAO_0000115>
        <obo:IAO_0000117>Chris Mungall</obo:IAO_0000117>
        <obo:IAO_0000118>consumes</obo:IAO_0000118>
        <oboInOwl:inSubset rdf:resource="http://purl.obolibrary.org/obo/ro/subsets#ro-eco"/>
        <rdfs:label xml:lang="en">has input</rdfs:label>
    </owl:ObjectProperty>
    


    <!-- http://purl.obolibrary.org/obo/RO_0002234 -->

    <owl:ObjectProperty rdf:about="http://purl.obolibrary.org/obo/RO_0002234">
        <rdfs:subPropertyOf rdf:resource="http://purl.obolibrary.org/obo/RO_0000057"/>
        <obo:IAO_0000114 rdf:resource="http://purl.obolibrary.org/obo/IAO_0000125"/>
        <obo:IAO_0000115>p has output c iff c is a participant in p, c is present at the end of p, and c is not present at the beginning of p.</obo:IAO_0000115>
        <obo:IAO_0000117>Chris Mungall</obo:IAO_0000117>
        <obo:IAO_0000118>produces</obo:IAO_0000118>
        <oboInOwl:inSubset rdf:resource="http://purl.obolibrary.org/obo/ro/subsets#ro-eco"/>
        <rdfs:label xml:lang="en">has output</rdfs:label>
    </owl:ObjectProperty>
    


    <!-- http://purl.obolibrary.org/obo/RO_0002328 -->

    <owl:ObjectProperty rdf:about="http://purl.obolibrary.org/obo/RO_0002328">
        <rdfs:subPropertyOf rdf:resource="http://www.w3.org/2002/07/owl#topObjectProperty"/>
        <obo:IAO_0000115>A grouping relationship for any relationship directly involving a function, or that holds because of a function of one of the related entities.</obo:IAO_0000115>
        <obo:IAO_0000117>Chris Mungall</obo:IAO_0000117>
        <obo:IAO_0000232>This is a grouping relation that collects relations used for the purpose of connecting structure and function</obo:IAO_0000232>
        <rdfs:label xml:lang="en">functionally related to</rdfs:label>
    </owl:ObjectProperty>
    


    <!-- http://purl.obolibrary.org/obo/RO_0002352 -->

    <owl:ObjectProperty rdf:about="http://purl.obolibrary.org/obo/RO_0002352">
        <rdfs:subPropertyOf rdf:resource="http://purl.obolibrary.org/obo/RO_0000056"/>
        <rdfs:subPropertyOf rdf:resource="http://purl.obolibrary.org/obo/RO_0002328"/>
        <obo:IAO_0000115>inverse of has input</obo:IAO_0000115>
        <obo:IAO_0000117>Chris Mungall</obo:IAO_0000117>
        <oboInOwl:inSubset rdf:resource="http://purl.obolibrary.org/obo/RO_0002259"/>
        <oboInOwl:inSubset rdf:resource="http://purl.obolibrary.org/obo/ro/subsets#ro-eco"/>
        <rdfs:label xml:lang="en">input of</rdfs:label>
    </owl:ObjectProperty>
    


    <!-- http://purl.obolibrary.org/obo/RO_0002353 -->

    <owl:ObjectProperty rdf:about="http://purl.obolibrary.org/obo/RO_0002353">
        <rdfs:subPropertyOf rdf:resource="http://purl.obolibrary.org/obo/RO_0000056"/>
        <rdfs:subPropertyOf rdf:resource="http://purl.obolibrary.org/obo/RO_0002328"/>
        <obo:IAO_0000115>inverse of has output</obo:IAO_0000115>
        <obo:IAO_0000117>Chris Mungall</obo:IAO_0000117>
        <oboInOwl:inSubset rdf:resource="http://purl.obolibrary.org/obo/RO_0002259"/>
        <oboInOwl:inSubset rdf:resource="http://purl.obolibrary.org/obo/ro/subsets#ro-eco"/>
        <rdfs:label xml:lang="en">output of</rdfs:label>
    </owl:ObjectProperty>
    


    <!-- http://purl.obolibrary.org/obo/RO_0002410 -->

    <owl:ObjectProperty rdf:about="http://purl.obolibrary.org/obo/RO_0002410">
        <rdfs:subPropertyOf rdf:resource="http://www.w3.org/2002/07/owl#topObjectProperty"/>
        <obo:IAO_0000114 rdf:resource="http://purl.obolibrary.org/obo/IAO_0000428"/>
        <obo:IAO_0000115>This relation groups causal relations between material entities and causal relations between processes</obo:IAO_0000115>
        <obo:IAO_0000116>This branch of the ontology deals with causal relations between entities. It is divided into two branches: causal relations between occurrents/processes, and causal relations between material entities. We take an &apos;activity flow-centric approach&apos;, with the former as primary, and define causal relations between material entities in terms of causal relations between occurrents.

To define causal relations in an activity-flow type network, we make use of 3 primitives:

 * Temporal: how do the intervals of the two occurrents relate? 
 * Is the causal relation regulatory?
 * Is the influence positive or negative

The first of these can be formalized in terms of the Allen Interval Algebra. Informally, the 3 bins we care about are &apos;direct&apos;, &apos;indirect&apos; or overlapping. Note that all causal relations should be classified under a RO temporal relation (see the branch under &apos;temporally related to&apos;). Note that all causal relations are temporal, but not all temporal relations are causal. Two occurrents can be related in time without being causally connected. We take causal influence to be primitive, elucidated as being such that has the upstream changed, some qualities of the donwstream would necessarily be modified.

For the second, we consider a relationship to be regulatory if the system in which the activities occur is capable of altering the relationship to achieve some objective. This could include changing the rate of production of a molecule.

For the third, we consider the effect of the upstream process on the output(s) of the downstream process. If the level of output is increased, or the rate of production of the output is increased, then the direction is increased. Direction can be positive, negative or neutral or capable of either direction. Two positives in succession yield a positive, two negatives in succession yield a positive, otherwise the default assumption is that the net effect is canceled and the influence is neutral.

Each of these 3 primitives can be composed to yield a cross-product of different relation types.</obo:IAO_0000116>
        <obo:IAO_0000117>Chris Mungall</obo:IAO_0000117>
        <obo:IAO_0000232>Do not use this relation directly. It is intended as a grouping for a diverse set of relations, all involving cause and effect.</obo:IAO_0000232>
        <rdfs:label xml:lang="en">causally related to</rdfs:label>
    </owl:ObjectProperty>
    


    <!-- http://purl.obolibrary.org/obo/RO_0002418 -->

    <owl:ObjectProperty rdf:about="http://purl.obolibrary.org/obo/RO_0002418">
        <rdfs:subPropertyOf rdf:resource="http://purl.obolibrary.org/obo/RO_0002501"/>
        <obo:IAO_0000115>p &apos;causally upstream or within&apos; q iff (1) the end of p is before the end of q and (2) the execution of p exerts some causal influence over the outputs of q; i.e. if p was abolished or the outputs of p were to be modified, this would necessarily affect q.</obo:IAO_0000115>
        <obo:IAO_0000116>We would like to make this disjoint with &apos;preceded by&apos;, but this is prohibited in OWL2</obo:IAO_0000116>
        <obo:IAO_0000117>Chris Mungall</obo:IAO_0000117>
        <obo:IAO_0000118>influences (processual)</obo:IAO_0000118>
        <oboInOwl:hasRelatedSynonym>affects</oboInOwl:hasRelatedSynonym>
        <rdfs:label>causally upstream of or within</rdfs:label>
    </owl:ObjectProperty>
    


    <!-- http://purl.obolibrary.org/obo/RO_0002427 -->

    <owl:ObjectProperty rdf:about="http://purl.obolibrary.org/obo/RO_0002427">
        <rdfs:subPropertyOf rdf:resource="http://purl.obolibrary.org/obo/RO_0002501"/>
        <obo:IAO_0000115>inverse of causally upstream of or within</obo:IAO_0000115>
        <obo:IAO_0000117>Chris Mungall</obo:IAO_0000117>
        <obo:IAO_0000119 rdf:resource="http://purl.obolibrary.org/obo/ro/docs/causal-relations"/>
        <oboInOwl:inSubset rdf:resource="http://purl.obolibrary.org/obo/RO_0002259"/>
        <rdfs:label>causally downstream of or within</rdfs:label>
    </owl:ObjectProperty>
    


    <!-- http://purl.obolibrary.org/obo/RO_0002501 -->

    <owl:ObjectProperty rdf:about="http://purl.obolibrary.org/obo/RO_0002501">
        <rdfs:subPropertyOf rdf:resource="http://purl.obolibrary.org/obo/RO_0002410"/>
        <obo:IAO_0000115>p is causally related to q if and only if p or any part of p and q or any part of q are linked by a chain of events where each event pair is one of direct activation or direct inhibition. p may be upstream, downstream, part of or a container of q.</obo:IAO_0000115>
        <obo:IAO_0000117>Chris Mungall</obo:IAO_0000117>
        <obo:IAO_0000119 rdf:resource="http://purl.obolibrary.org/obo/ro/docs/causal-relations"/>
        <obo:IAO_0000232>Do not use this relation directly. It is intended as a grouping for a diverse set of relations, all involving cause and effect.</obo:IAO_0000232>
        <rdfs:label>causal relation between processes</rdfs:label>
    </owl:ObjectProperty>
    


    <!-- http://purl.obolibrary.org/obo/RO_0002505 -->

    <owl:ObjectProperty rdf:about="http://purl.obolibrary.org/obo/RO_0002505">
        <rdfs:subPropertyOf rdf:resource="http://purl.obolibrary.org/obo/RO_0000057"/>
        <obo:IAO_0000112>&apos;lysine biosynthetic process via diaminopimelate&apos; SubClassOf has_intermediate some diaminopimelate</obo:IAO_0000112>
        <obo:IAO_0000115>p has intermediate c if and only if p has parts p1, p2 and p1 has output c, and p2 has input c</obo:IAO_0000115>
        <obo:IAO_0000117>Chris Mungall</obo:IAO_0000117>
        <obo:IAO_0000118>has intermediate product</obo:IAO_0000118>
        <oboInOwl:inSubset rdf:resource="http://purl.obolibrary.org/obo/ro/subsets#ro-eco"/>
        <rdfs:label>has intermediate</rdfs:label>
    </owl:ObjectProperty>
    


    <!-- http://purl.obolibrary.org/obo/RO_0002615 -->

    <owl:ObjectProperty rdf:about="http://purl.obolibrary.org/obo/RO_0002615">
        <rdfs:subPropertyOf rdf:resource="http://www.w3.org/2002/07/owl#topObjectProperty"/>
        <owl:inverseOf rdf:resource="http://purl.obolibrary.org/obo/RO_0003301"/>
        <rdfs:label>has model</rdfs:label>
    </owl:ObjectProperty>
    


    <!-- http://purl.obolibrary.org/obo/RO_0003000 -->

    <owl:ObjectProperty rdf:about="http://purl.obolibrary.org/obo/RO_0003000">
        <rdfs:subPropertyOf rdf:resource="http://www.w3.org/2002/07/owl#topObjectProperty"/>
        <obo:IAO_0000114 rdf:resource="http://purl.obolibrary.org/obo/IAO_0000125"/>
        <obo:IAO_0000115 rdf:datatype="http://www.w3.org/2001/XMLSchema#string">a produces b if some process that occurs_in a has_output b, where a and b are material entities. Examples: hybridoma cell line produces monoclonal antibody reagent; chondroblast produces avascular GAG-rich matrix.</obo:IAO_0000115>
        <obo:IAO_0000117>Melissa Haendel</obo:IAO_0000117>
        <oboInOwl:inSubset rdf:resource="http://purl.obolibrary.org/obo/ro/subsets#ro-eco"/>
        <rdfs:comment rdf:datatype="http://www.w3.org/2001/XMLSchema#string">Note that this definition doesn&apos;t quite distinguish the output of a transformation process from a production process, which is related to the identity/granularity issue.</rdfs:comment>
        <rdfs:label xml:lang="en">produces</rdfs:label>
    </owl:ObjectProperty>
    


    <!-- http://purl.obolibrary.org/obo/RO_0003001 -->

    <owl:ObjectProperty rdf:about="http://purl.obolibrary.org/obo/RO_0003001">
        <rdfs:subPropertyOf rdf:resource="http://www.w3.org/2002/07/owl#topObjectProperty"/>
        <obo:IAO_0000114 rdf:resource="http://purl.obolibrary.org/obo/IAO_0000125"/>
        <obo:IAO_0000115>a produced_by b iff some process that occurs_in b has_output a.</obo:IAO_0000115>
        <obo:IAO_0000117>Melissa Haendel</obo:IAO_0000117>
        <oboInOwl:inSubset rdf:resource="http://purl.obolibrary.org/obo/ro/subsets#ro-eco"/>
        <rdfs:label xml:lang="en">produced by</rdfs:label>
    </owl:ObjectProperty>
    


    <!-- http://purl.obolibrary.org/obo/RO_0003301 -->

    <owl:ObjectProperty rdf:about="http://purl.obolibrary.org/obo/RO_0003301">
        <rdfs:subPropertyOf rdf:resource="http://www.w3.org/2002/07/owl#topObjectProperty"/>
        <obo:IAO_0000115>A relation between a biological, experimental, or computational artifact and an entity it is used to study, in virtue of its replicating or approximating features of the studied entity.</obo:IAO_0000115>
        <obo:IAO_0000117>Matthew Brush</obo:IAO_0000117>
        <obo:IAO_0000118 xml:lang="en">is used to study</obo:IAO_0000118>
        <rdfs:comment>The primary use case for this relation was to link a biological model system such as a cell line or model organism to a disease it is used to investigate, in virtue of the model system exhibiting features similar to that of the disease of interest. But the relation is defined more broadly to support other use cases, such as linking genes in which alterations are made to create model systems to the condition the system is used to interrogate, or computational models to real-world phenomena they are defined to simulate.</rdfs:comment>
        <rdfs:label xml:lang="en">has role in modeling</rdfs:label>
    </owl:ObjectProperty>
    


    <!-- http://purl.obolibrary.org/obo/RO_0004007 -->

    <owl:ObjectProperty rdf:about="http://purl.obolibrary.org/obo/RO_0004007">
        <rdfs:subPropertyOf rdf:resource="http://purl.obolibrary.org/obo/RO_0000057"/>
        <obo:IAO_0000115>p &apos;has primary input ot output&apos; c iff either (a) p &apos;has primary input&apos; c or (b) p &apos;has primary output&apos; c.</obo:IAO_0000115>
        <oboInOwl:created_by rdf:datatype="http://www.w3.org/2001/XMLSchema#string">cjm</oboInOwl:created_by>
        <oboInOwl:creation_date rdf:datatype="http://www.w3.org/2001/XMLSchema#dateTime">2018-12-13T11:26:17Z</oboInOwl:creation_date>
        <rdfs:label>has primary input or output</rdfs:label>
    </owl:ObjectProperty>
    


    <!-- http://purl.obolibrary.org/obo/RO_0004008 -->

    <owl:ObjectProperty rdf:about="http://purl.obolibrary.org/obo/RO_0004008">
        <rdfs:subPropertyOf rdf:resource="http://purl.obolibrary.org/obo/RO_0002234"/>
        <rdfs:subPropertyOf rdf:resource="http://purl.obolibrary.org/obo/RO_0004007"/>
        <obo:IAO_0000115>p has primary output c if (a) p has output c and (b) the goal of process is to modify, produce, or transform c.</obo:IAO_0000115>
        <oboInOwl:created_by rdf:datatype="http://www.w3.org/2001/XMLSchema#string">cjm</oboInOwl:created_by>
        <oboInOwl:creation_date rdf:datatype="http://www.w3.org/2001/XMLSchema#dateTime">2018-12-13T11:26:32Z</oboInOwl:creation_date>
        <rdfs:label>has primary output</rdfs:label>
    </owl:ObjectProperty>
    <owl:Axiom>
        <owl:annotatedSource rdf:resource="http://purl.obolibrary.org/obo/RO_0004008"/>
        <owl:annotatedProperty rdf:resource="http://purl.obolibrary.org/obo/IAO_0000115"/>
        <owl:annotatedTarget>p has primary output c if (a) p has output c and (b) the goal of process is to modify, produce, or transform c.</owl:annotatedTarget>
        <oboInOwl:hasDbXref>GOC:cjm</oboInOwl:hasDbXref>
        <oboInOwl:hasDbXref>GOC:dph</oboInOwl:hasDbXref>
        <oboInOwl:hasDbXref>GOC:kva</oboInOwl:hasDbXref>
        <oboInOwl:hasDbXref>GOC:pt</oboInOwl:hasDbXref>
        <rdfs:comment>PMID:27812932</rdfs:comment>
    </owl:Axiom>
    


    <!-- http://purl.obolibrary.org/obo/RO_0004009 -->

    <owl:ObjectProperty rdf:about="http://purl.obolibrary.org/obo/RO_0004009">
        <rdfs:subPropertyOf rdf:resource="http://purl.obolibrary.org/obo/RO_0002233"/>
        <rdfs:subPropertyOf rdf:resource="http://purl.obolibrary.org/obo/RO_0004007"/>
        <obo:IAO_0000115>p has primary input c if (a) p has input c and (b) the goal of process is to modify, consume, or transform c.</obo:IAO_0000115>
        <oboInOwl:created_by rdf:datatype="http://www.w3.org/2001/XMLSchema#string">cjm</oboInOwl:created_by>
        <oboInOwl:creation_date rdf:datatype="http://www.w3.org/2001/XMLSchema#dateTime">2018-12-13T11:26:56Z</oboInOwl:creation_date>
        <rdfs:label>has primary input</rdfs:label>
    </owl:ObjectProperty>
    <owl:Axiom>
        <owl:annotatedSource rdf:resource="http://purl.obolibrary.org/obo/RO_0004009"/>
        <owl:annotatedProperty rdf:resource="http://purl.obolibrary.org/obo/IAO_0000115"/>
        <owl:annotatedTarget>p has primary input c if (a) p has input c and (b) the goal of process is to modify, consume, or transform c.</owl:annotatedTarget>
        <oboInOwl:hasDbXref>GOC:cjm</oboInOwl:hasDbXref>
        <oboInOwl:hasDbXref>GOC:dph</oboInOwl:hasDbXref>
        <oboInOwl:hasDbXref>GOC:kva</oboInOwl:hasDbXref>
        <oboInOwl:hasDbXref>GOC:pt</oboInOwl:hasDbXref>
        <rdfs:comment>PMID:27812932</rdfs:comment>
    </owl:Axiom>
    


    <!-- http://www.w3.org/2002/07/owl#topObjectProperty -->

    <owl:ObjectProperty rdf:about="http://www.w3.org/2002/07/owl#topObjectProperty"/>
    


    <!-- 
    ///////////////////////////////////////////////////////////////////////////////////////
    //
    // Classes
    //
    ///////////////////////////////////////////////////////////////////////////////////////
     -->

    


    <!-- http://purl.obolibrary.org/obo/BFO_0000019 -->

    <owl:Class rdf:about="http://purl.obolibrary.org/obo/BFO_0000019"/>
    


    <!-- http://purl.obolibrary.org/obo/BFO_0000040 -->

    <owl:Class rdf:about="http://purl.obolibrary.org/obo/BFO_0000040"/>
    


    <!-- http://purl.obolibrary.org/obo/RO_0002577 -->

    <owl:Class rdf:about="http://purl.obolibrary.org/obo/RO_0002577">
        <rdfs:subClassOf rdf:resource="http://purl.obolibrary.org/obo/BFO_0000040"/>
        <obo:IAO_0000115>A material entity consisting of multiple components that are causally integrated.</obo:IAO_0000115>
        <obo:IAO_0000116>May be replaced by a BFO class, as discussed in http://www.jbiomedsem.com/content/4/1/43</obo:IAO_0000116>
        <obo:IAO_0000117>Chris Mungall</obo:IAO_0000117>
        <obo:IAO_0000119>http://www.jbiomedsem.com/content/4/1/43</obo:IAO_0000119>
        <rdfs:label>system</rdfs:label>
    </owl:Class>
    


    <!-- 
    ///////////////////////////////////////////////////////////////////////////////////////
    //
    // Annotations
    //
    ///////////////////////////////////////////////////////////////////////////////////////
     -->

    <rdf:Description rdf:about="http://purl.obolibrary.org/obo/RO_0002323">
        <obo:IAO_0000232>Do not use this relation directly. It is ended as a grouping for a diverse set of relations, all involving parthood or connectivity relationships</obo:IAO_0000232>
        <obo:IAO_0000115>A mereological relationship or a topological relationship</obo:IAO_0000115>
        <obo:RO_0001900 rdf:resource="http://purl.obolibrary.org/obo/RO_0001901"/>
        <rdfs:label xml:lang="en">mereotopologically related to</rdfs:label>
        <obo:IAO_0000117>Chris Mungall</obo:IAO_0000117>
    </rdf:Description>
</rdf:RDF>



<!-- Generated by the OWL API (version 4.5.6) https://github.com/owlcs/owlapi -->

